<?xml version='1.0' encoding='UTF-8'?>
<!DOCTYPE rdf:RDF [
    <!ENTITY cnt 'http://www.w3.org/2011/content#'>
    <!ENTITY dao 'http://www.semanticdesktop.org/ontologies/2011/10/05/dao#'>
    <!ENTITY dc 'http://purl.org/dc/elements/1.1/'>
    <!ENTITY dcam 'http://purl.org/dc/dcam/'>
    <!ENTITY dcon 'http://www.semanticdesktop.org/ontologies/2011/10/05/dcon#'>
    <!ENTITY dcterms 'http://purl.org/dc/terms/'>
    <!ENTITY dctypes 'http://purl.org/dc/dcmitype/'>
    <!ENTITY ddo 'http://www.semanticdesktop.org/ontologies/2011/10/05/ddo#'>
    <!ENTITY dplo 'http://www.semanticdesktop.org/ontologies/2011/10/05/dlpo#'>
    <!ENTITY dpo 'http://www.semanticdesktop.org/ontologies/2011/10/05/dpo#'>
    <!ENTITY drmo 'http://www.semanticdesktop.org/ontologies/2012/03/06/drmo#'>
    <!ENTITY duho 'http://www.semanticdesktop.org/ontologies/2011/10/05/duho#'>
    <!ENTITY foaf 'http://xmlns.com/foaf/0.1/'>
    <!ENTITY nao 'http://www.semanticdesktop.org/ontologies/2007/08/15/nao#'>
    <!ENTITY ncal 'http://www.semanticdesktop.org/ontologies/2007/04/02/ncal#'>
    <!ENTITY nco 'http://www.semanticdesktop.org/ontologies/2007/03/22/nco#'>
    <!ENTITY ndo 'http://www.semanticdesktop.org/ontologies/2010/04/30/ndo#'>
    <!ENTITY nexif 'http://www.semanticdesktop.org/ontologies/2007/05/10/nexif#'>
    <!ENTITY nfo 'http://www.semanticdesktop.org/ontologies/2007/03/22/nfo#'>
    <!ENTITY nid3 'http://www.semanticdesktop.org/ontologies/2007/05/10/nid3#'>
    <!ENTITY nie 'http://www.semanticdesktop.org/ontologies/2007/01/19/nie#'>
    <!ENTITY nmm 'http://www.semanticdesktop.org/ontologies/2009/02/19/nmm#'>
    <!ENTITY nmo 'http://www.semanticdesktop.org/ontologies/2007/03/22/nmo#'>
    <!ENTITY nrl 'http://www.semanticdesktop.org/ontologies/2007/08/15/nrl#'>
    <!ENTITY ns 'http://www.w3.org/2003/06/sw-vocab-status/ns#'>
    <!ENTITY nso 'http://www.semanticdesktop.org/ontologies/2009/11/08/nso#'>
    <!ENTITY nuao 'http://www.semanticdesktop.org/ontologies/2010/01/25/nuao#'>
    <!ENTITY oa 'http://www.w3.org/ns/oa#'>
    <!ENTITY owl 'http://www.w3.org/2002/07/owl#'>
    <!ENTITY pimo 'http://www.semanticdesktop.org/ontologies/2007/11/01/pimo#'>
    <!ENTITY protege 'http://protege.stanford.edu/system#'>
    <!ENTITY prov 'http://www.w3.org/ns/prov#'>
    <!ENTITY rdf 'http://www.w3.org/1999/02/22-rdf-syntax-ns#'>
    <!ENTITY rdfs 'http://www.w3.org/2000/01/rdf-schema#'>
    <!ENTITY scos 'http://www.w3.org/2004/02/skos/core#'>
    <!ENTITY tmo 'http://www.semanticdesktop.org/ontologies/2008/05/20/tmo#'>
    <!ENTITY xsd 'http://www.w3.org/2001/XMLSchema#'>
]>

<rdf:RDF
    xmlns:cnt="&cnt;"
    xmlns:dao="&dao;"
    xmlns:dc="&dc;"
    xmlns:dcam="&dcam;"
    xmlns:dcon="&dcon;"
    xmlns:dcterms="&dcterms;"
    xmlns:dctypes="&dctypes;"
    xmlns:ddo="&ddo;"
    xmlns:dplo="&dplo;"
    xmlns:dpo="&dpo;"
    xmlns:drmo="&drmo;"
    xmlns:duho="&duho;"
    xmlns:foaf="&foaf;"
    xmlns:nao="&nao;"
    xmlns:ncal="&ncal;"
    xmlns:nco="&nco;"
    xmlns:ndo="&ndo;"
    xmlns:nexif="&nexif;"
    xmlns:nfo="&nfo;"
    xmlns:nid3="&nid3;"
    xmlns:nie="&nie;"
    xmlns:nmm="&nmm;"
    xmlns:nmo="&nmo;"
    xmlns:nrl="&nrl;"
    xmlns:ns="&ns;"
    xmlns:nso="&nso;"
    xmlns:nuao="&nuao;"
    xmlns:oa="&oa;"
    xmlns:owl="&owl;"
    xmlns:pimo="&pimo;"
    xmlns:protege="&protege;"
    xmlns:prov="&prov;"
    xmlns:rdf="&rdf;"
    xmlns:rdfs="&rdfs;"
    xmlns:scos="&scos;"
    xmlns:tmo="&tmo;"
    xmlns:xsd="&xsd;"
>
<rdf:Property rdf:about="&ncal;sequence"
    rdfs:label="sequence">
  <nrl:maxCardinality rdf:datatype="&xsd;integer">1</nrl:maxCardinality>
  <rdfs:comment>This property defines the revision sequence number of the calendar component within a sequence of revisions. Inspired by RFC 2445 sec. 4.8.7.4</rdfs:comment>
  <rdfs:domain rdf:resource="&ncal;UnionOfEventJournalTodo"/>
  <rdfs:range rdf:resource="&xsd;integer"/>
</rdf:Property>

<rdf:Property rdf:about="&cnt;doctypeName">
  <rdf:type rdf:resource="&owl;ObjectProperty"/>
  <rdfs:comment xml:lang="en">The document type name.</rdfs:comment>
  <rdfs:domain rdf:resource="&cnt;DoctypeDecl"/>
  <rdfs:label xml:lang="en">Document type name</rdfs:label>
  <rdfs:range rdf:resource="&rdfs;Literal"/>
</rdf:Property>

<rdf:Property rdf:about="&ncal;bymonthday"
    rdfs:label="bymonthday">
  <rdfs:comment>Day of the month when the event should recur. Defined in RFC 2445 sec. 4.3.10</rdfs:comment>
  <rdfs:domain rdf:resource="&ncal;RecurrenceRule"/>
  <rdfs:range rdf:resource="&xsd;integer"/>
</rdf:Property>

<rdf:Property rdf:about="&nid3;uniqueFileIdentifier"
    rdfs:label="uniqueFileIdentifier">
  <rdfs:comment>This frame's purpose is to be able to identify the audio file in a database that may contain more information relevant to the content. Since standardisation of such a database is beyond this document, all frames begin with a null-terminated string with a URL containing an email address, or a link to a location where an email address can be found, that belongs to the organisation responsible for this specific database implementation. Questions regarding the database should be sent to the indicated email address. The URL should not be used for the actual database queries. The string "http://www.id3.org/dummy/ufid.html" should be used for tests. Software that isn't told otherwise may safely remove such frames. The 'Owner identifier' must be non-empty (more than just a termination). The 'Owner identifier' is then followed by the actual identifier, which may be up to 64 bytes. There may be more than one "UFID" frame in a tag, but only one with the same 'Owner identifier'.</rdfs:comment>
  <rdfs:domain rdf:resource="&nid3;ID3Audio"/>
  <rdfs:range rdf:resource="&xsd;string"/>
  <rdfs:subPropertyOf rdf:resource="&nie;identifier"/>
</rdf:Property>

<rdf:Property rdf:about="&nco;voiceMail"
    nrl:maxCardinality="1"
    rdfs:label="voiceMail">
  <rdfs:comment>Indicates if the given number accepts voice mail. (e.g. there is an answering machine). Inspired by TYPE=msg parameter of the TEL property defined in RFC 2426 sec. 3.3.1</rdfs:comment>
  <rdfs:domain rdf:resource="&nco;VoicePhoneNumber"/>
  <rdfs:range rdf:resource="&xsd;boolean"/>
</rdf:Property>

<rdf:Property rdf:about="&tmo;dateTime"
    nrl:maxCardinality="1"
    rdfs:label="dateTime">
  <rdfs:comment>dateTime subsumes various properties with Range XMLSchema:dateTime. If possible they are further grouped by "abstract" properties.</rdfs:comment>
  <rdfs:range rdf:resource="&xsd;dateTime"/>
</rdf:Property>

<rdf:Property rdf:about="&nfo;fileOwner"
    rdfs:label="fileOwner">
  <nrl:maxCardinality rdf:datatype="&xsd;integer">1</nrl:maxCardinality>
  <rdfs:comment>The owner of the file as defined by the file system access rights feature.</rdfs:comment>
  <rdfs:domain rdf:resource="&nfo;FileDataObject"/>
  <rdfs:range rdf:resource="&nco;Contact"/>
</rdf:Property>

<rdf:Property rdf:about="&nid3;publishersWebpage"
    rdfs:label="publishersWebpage">
  <rdfs:comment>WPUB
The 'Publishers official webpage' frame is a URL pointing at the official wepage for the publisher.</rdfs:comment>
  <rdfs:domain rdf:resource="&nid3;ID3Audio"/>
  <rdfs:range rdf:resource="&rdfs;Resource"/>
</rdf:Property>

<rdf:Property rdf:about="&tmo;transmissionStateChangesFrom"
    nrl:maxCardinality="1"
    rdfs:label="transmissionStateChangesFrom">
  <rdfs:domain rdf:resource="&tmo;TransmissionState"/>
  <rdfs:range rdf:resource="&tmo;TransmissionState"/>
  <rdfs:subPropertyOf rdf:resource="&tmo;stateTypeRole"/>
</rdf:Property>

<rdf:Property rdf:about="&ncal;sentBy"
    rdfs:label="sentBy">
  <rdfs:comment>To specify the calendar user that is acting on behalf of the calendar user specified by the property. Inspired by RFC 2445 sec. 4.2.18. The original data type of this property was a mailto: URI. This has been changed to nco:Contact to promote integration between NCO and NCAL.</rdfs:comment>
  <rdfs:domain rdf:resource="&ncal;AttendeeOrOrganizer"/>
  <rdfs:range rdf:resource="&nco;Contact"/>
</rdf:Property>

<rdfs:Class rdf:about="&dplo;MultimediaPost"
    rdfs:label="Multimedia Post">
  <rdfs:comment>A livepost consisting of a multimedia item, including links to online items. Further subclasses represent video, audio or image posts, as defined by various instances of the NFO (File Ontology).</rdfs:comment>
  <rdfs:subClassOf rdf:resource="&dplo;LivePost"/>
</rdfs:Class>

<rdfs:Class rdf:about="&tmo;Interdependence"
    rdfs:label="Interdependence">
  <rdfs:subClassOf rdf:resource="&tmo;UndirectedDependency"/>
</rdfs:Class>

<owl:NamedIndividual rdf:about="&oa;linking">
  <rdf:type rdf:resource="&oa;Motivation"/>
  <rdfs:comment xml:lang="en">The motivation that represents an untyped link to a resource related to the target.</rdfs:comment>
  <scos:inScheme rdf:resource="&oa;motivationScheme"/>
  <scos:prefLabel xml:lang="en">linking</scos:prefLabel>
</owl:NamedIndividual>

<rdf:Property rdf:about="&nexif;interoperabilityIndex"
    rdfs:label="interoperabilityIndex">
  <rdfs:subPropertyOf rdf:resource="http://www.kanzaki.com/ns/exif#interoperabilityIndex"/>
  <rdfs:subPropertyOf rdf:resource="&nexif;interopInfo"/>
  <rdfs:comment>Indicates the identification of the Interoperability rule. 'R98' = conforming to R98 file specification of Recommended Exif Interoperability Rules (ExifR98) or to DCF basic file stipulated by Design Rule for Camera File System. 'THM' = conforming to DCF thumbnail file stipulated by Design rule for Camera File System.
tagNumber: 1</rdfs:comment>
  <rdfs:domain rdf:resource="&nexif;Photo"/>
  <rdfs:range rdf:resource="&xsd;string"/>
</rdf:Property>

<rdf:Property rdf:about="&nexif;gpsTrackRef"
    rdfs:label="gpsTrackRef">
  <rdfs:subPropertyOf rdf:resource="http://www.kanzaki.com/ns/exif#gpsTrackRef"/>
  <rdfs:subPropertyOf rdf:resource="&nexif;gpsInfo"/>
  <rdfs:comment>tagNumber: 14
The reference for giving the direction of GPS receiver movement. 'T' denotes true direction and 'M' is magnetic direction.</rdfs:comment>
  <rdfs:domain rdf:resource="&nexif;Photo"/>
  <rdfs:range rdf:resource="&xsd;string"/>
</rdf:Property>

<ncal:JournalStatus rdf:about="&ncal;cancelledJournalStatus"
    rdfs:label="cancelledJournalStatus"/>

<rdfs:Class rdf:about="&ncal;AttachmentEncoding"
    rdfs:label="AttachmentEncoding">
  <rdfs:comment>Attachment encoding. This class has been introduced to express the limited vocabulary of values for the ncal:encoding property. See the documentation of ncal:encoding for details.</rdfs:comment>
  <rdfs:subClassOf rdf:resource="&rdfs;Resource"/>
</rdfs:Class>

<rdf:Property rdf:about="&tmo;containsTask"
    rdfs:label="containsTask">
  <rdfs:domain rdf:resource="&tmo;TaskContainer"/>
  <rdfs:range rdf:resource="&tmo;Task"/>
  <rdfs:subPropertyOf rdf:resource="&pimo;hasPart"/>
</rdf:Property>

<rdf:Property rdf:about="&nid3;userDefinedFrameDescription"
    rdfs:comment="Description of a user-defined frame."
    rdfs:label="userDefinedFrameDescription">
  <rdfs:domain rdf:resource="&nid3;UserDefinedFrame"/>
  <rdfs:range rdf:resource="&xsd;string"/>
</rdf:Property>

<rdf:Property rdf:about="&dpo;minVisibility"
    rdfs:label="Minimum Visibility">
  <rdfs:comment>A subproperty of dpo:minValue that defines a lowerbound on the observed visibility (in kilometres) such that it can classify as a dpo:WeatherCondition instance. It can be used in conjunction with dpo:maxVisibility to state that specific instances of dpo:WeatherCondition have a pre-defined range of observable real-world visibility levels. In addition, they can also be used with various other weather conditions values and ranges to define complex weather condition types.</rdfs:comment>
  <rdfs:domain rdf:resource="&dpo;WeatherConditions"/>
  <rdfs:range rdf:resource="&xsd;nonNegativeInteger"/>
  <rdfs:subPropertyOf rdf:resource="&dpo;minValue"/>
</rdf:Property>

<rdf:Property rdf:about="&pimo;isWriteable"
    rdfs:label="is writeable">
  <rdfs:comment>Defines if this information model can be modified by the user of the system. This is usually false for imported ontologies and true for the user's own PersonalInformationModel.</rdfs:comment>
  <rdfs:range rdf:resource="&rdfs;Literal"/>
</rdf:Property>

<rdf:Property rdf:about="&nuao;lastEvent"
    rdfs:comment="The start time of the last event"
    rdfs:label="last event">
  <nrl:maxCardinality rdf:datatype="&xsd;nonNegativeInteger">1</nrl:maxCardinality>
  <rdfs:domain rdf:resource="&rdfs;Resource"/>
  <rdfs:range rdf:resource="&xsd;dateTime"/>
</rdf:Property>

<rdfs:Class rdf:about="&ncal;UnionOfTimezoneObservanceEventFreebusyJournalTimezoneTodo"
    rdfs:label="UnionOfTimezoneObservanceEventFreebusyJournalTimezoneTodo">
  <rdfs:subClassOf rdf:resource="&ncal;UnionParentClass"/>
</rdfs:Class>

<rdf:Property rdf:about="&nco;role"
    rdfs:label="role">
  <rdfs:comment>Role an object represented by this contact represents in the organization. This might include 'Programmer', 'Manager', 'Sales Representative'. Be careful to avoid confusion with the title property. An equivalent of the 'ROLE' property as defined in RFC 2426. Sec. 3.5.2. Note the difference between nco:Role class and nco:role property.</rdfs:comment>
  <rdfs:domain rdf:resource="&nco;Affiliation"/>
  <rdfs:range rdf:resource="&xsd;string"/>
</rdf:Property>

<owl:ObjectProperty rdf:about="&oa;item">
  <rdfs:comment xml:lang="en">The relationship between a multiplicity construct node and its constituent resources.

There MUST be 1 or more item relationships for each multiplicity construct oa:Choice, oa:Composite and oa:List.</rdfs:comment>
  <rdfs:isDefinedBy rdf:resource="&oa;"/>
  <rdfs:label xml:lang="en">item</rdfs:label>
  <rdfs:subPropertyOf rdf:resource="&rdfs;member"/>
</owl:ObjectProperty>

<rdf:Property rdf:about="&nid3;originalFilename"
    rdfs:label="originalFilename">
  <rdfs:comment>TOFN
The 'Original filename' frame contains the preferred filename for the file, since some media doesn't allow the desired length of the filename. The filename is case sensitive and includes its suffix.</rdfs:comment>
  <rdfs:domain rdf:resource="&nid3;ID3Audio"/>
  <rdfs:range rdf:resource="&xsd;string"/>
</rdf:Property>

<rdf:Property rdf:about="&ncal;comment"
    rdfs:label="comment">
  <rdfs:comment>Non-processing information intended to provide a comment to the calendar user. Inspired by RFC 2445 sec. 4.8.1.4 with the following reservations:  the LANGUAGE parameter has been discarded. Please use xml:lang literals to express language. For the ALTREP parameter use the commentAltRep property.</rdfs:comment>
  <rdfs:domain rdf:resource="&ncal;UnionOfTimezoneObservanceEventFreebusyJournalTimezoneTodo"/>
  <rdfs:range rdf:resource="&xsd;string"/>
  <rdfs:subPropertyOf rdf:resource="&nie;comment"/>
</rdf:Property>

<rdfs:Class rdf:about="&foaf;OnlineEcommerceAccount"
    rdfs:comment="An online e-commerce account."
    rdfs:label="Online E-commerce Account"
    ns:term_status="unstable">
  <rdf:type rdf:resource="&owl;Class"/>
  <rdfs:isDefinedBy rdf:resource="&foaf;"/>
  <rdfs:subClassOf rdf:resource="&foaf;OnlineAccount"/>
</rdfs:Class>

<rdfs:Class rdf:about="&dcon;Environment"
    rdfs:label="Environment">
  <rdfs:comment>The environment aspect covers context elements relating to current or forecasted environmental conditions, as experienced directly by the user, or by sensors in their surroundings.</rdfs:comment>
  <rdfs:subClassOf rdf:resource="&dcon;Aspect"/>
</rdfs:Class>

<rdfs:Class rdf:about="&nco;VoicePhoneNumber"
    rdfs:label="VoicePhoneNumber">
  <rdfs:comment>A telephone number with voice communication capabilities. Class inspired by the TYPE=voice parameter of the TEL property defined in RFC 2426 sec. 3.3.1</rdfs:comment>
  <rdfs:subClassOf rdf:resource="&nco;PhoneNumber"/>
</rdfs:Class>

<rdf:Property rdf:about="&dcterms;bibliographicCitation">
  <rdfs:subPropertyOf rdf:resource="&dc;identifier"/>
  <rdfs:subPropertyOf rdf:resource="&dcterms;identifier"/>
  <dcterms:description xml:lang="en">Recommended practice is to include sufficient bibliographic detail to identify the resource as unambiguously as possible.</dcterms:description>
  <dcterms:hasVersion rdf:resource="http://dublincore.org/usage/terms/history/#bibliographicCitation-002"/>
  <dcterms:issued rdf:datatype="&xsd;date">2003-02-15</dcterms:issued>
  <dcterms:modified rdf:datatype="&xsd;date">2008-01-14</dcterms:modified>
  <rdfs:comment xml:lang="en">A bibliographic reference for the resource.</rdfs:comment>
  <rdfs:domain rdf:resource="&dcterms;BibliographicResource"/>
  <rdfs:isDefinedBy rdf:resource="&dcterms;"/>
  <rdfs:label xml:lang="en">Bibliographic Citation</rdfs:label>
  <rdfs:range rdf:resource="&rdfs;Literal"/>
</rdf:Property>

<rdf:Property rdf:about="&nfo;pageNumber"
    rdfs:comment="Page linked by the bookmark."
    rdfs:label="pageNumber">
  <nrl:maxCardinality rdf:datatype="&xsd;integer">1</nrl:maxCardinality>
  <rdfs:domain rdf:resource="&nfo;Bookmark"/>
  <rdfs:range rdf:resource="&xsd;integer"/>
</rdf:Property>

<tmo:Importance rdf:about="&tmo;TMO_Instance_Importance_04"
    rdfs:label="TMO_Instance_Importance_04"/>

<rdfs:Class rdf:about="&pimo;ClassRole"
    rdfs:label="ClassRole">
  <rdfs:comment>Roles of classes in PIMO: concrete instances are Abstract and Concrete.</rdfs:comment>
  <rdfs:subClassOf rdf:resource="&rdfs;Resource"/>
</rdfs:Class>

<rdf:Property rdf:about="&nfo;permissions"
    rdfs:label="permissions">
  <nrl:maxCardinality rdf:datatype="&xsd;integer">1</nrl:maxCardinality>
  <rdfs:comment>A string containing the permissions of a file. A feature common in many UNIX-like operating systems.</rdfs:comment>
  <rdfs:domain rdf:resource="&nfo;FileDataObject"/>
  <rdfs:range rdf:resource="&xsd;string"/>
</rdf:Property>

<rdf:Property rdf:about="&nexif;printImageMatchingIFDPointer"
    rdfs:comment="tagNumber: 50341
A pointer to the print image matching IFD"
    rdfs:label="printImageMatchingIFDPointer">
  <rdfs:subPropertyOf rdf:resource="http://www.kanzaki.com/ns/exif#printImageMatching_IFD_Pointer"/>
  <rdfs:subPropertyOf rdf:resource="&nexif;ifdPointer"/>
  <rdfs:domain rdf:resource="&nexif;Photo"/>
  <rdfs:range rdf:resource="&nexif;Photo"/>
</rdf:Property>

<rdf:Property rdf:about="&dpo;minHour"
    rdfs:label="Minimum Hour">
  <rdfs:comment>A subproperty of dpo:minValue that defines a lowerbound on the observed time (in hours, i.e., between 0 signifying midnight and 23 signifying 11pm) such that it can classify as a dpo:TimePeriod instance. It can be used in conjunction with dpo:maxHour, i.e. specific instances of dpo:TimePeriod have a pre-defined observable 24-hour-based period.</rdfs:comment>
  <rdfs:domain rdf:resource="&dpo;TimePeriod"/>
  <rdfs:range rdf:resource="&xsd;integer"/>
  <rdfs:subPropertyOf rdf:resource="&dpo;maxValue"/>
</rdf:Property>

<nrl:RuleViewSpecification rdf:about="&pimo;RuleViewSpecificationInferOccurrences"
    rdfs:label="RuleViewSpecificationInferOccurrences"/>

<rdfs:Class rdf:about="&ncal;AccessClassification"
    rdfs:label="AccessClassification">
  <rdfs:comment>Access classification of a calendar component. Introduced to express 
the set of values for the ncal:class property. The user may use instances
provided with this ontology or create his/her own with desired semantics.
See the documentation of ncal:class for details.</rdfs:comment>
  <rdfs:subClassOf rdf:resource="&rdfs;Resource"/>
</rdfs:Class>

<rdf:Property rdf:about="&foaf;myersBriggs"
    rdfs:comment="A Myers Briggs (MBTI) personality classification."
    rdfs:label="myersBriggs"
    ns:term_status="testing">
  <rdf:type rdf:resource="&owl;DatatypeProperty"/>
  <rdfs:domain rdf:resource="&foaf;Person"/>
  <rdfs:isDefinedBy rdf:resource="&foaf;"/>
  <rdfs:range rdf:resource="&rdfs;Literal"/>
</rdf:Property>

<rdf:Property rdf:about="&dcon;humidity"
    rdfs:label="Humidity Value">
  <rdfs:comment>Registers an actual humidity level value element attribute to an active weather condition in the current context.</rdfs:comment>
  <rdfs:domain rdf:resource="&dpo;WeatherConditions"/>
  <rdfs:range rdf:resource="&xsd;nonNegativeInteger"/>
  <rdfs:subPropertyOf rdf:resource="&dcon;hasContextAttribute"/>
</rdf:Property>

<rdf:Property rdf:about="&ncal;url"
    rdfs:label="url">
  <nrl:maxCardinality rdf:datatype="&xsd;integer">1</nrl:maxCardinality>
  <rdfs:comment>This property defines a Uniform Resource Locator (URL) associated with the iCalendar object. Inspired by the RFC 2445 sec. 4.8.4.6. Original range had been specified as URI.</rdfs:comment>
  <rdfs:domain rdf:resource="&ncal;UnionOfEventFreebusyJournalTodo"/>
  <rdfs:range rdf:resource="&rdfs;Resource"/>
</rdf:Property>

<rdfs:Class rdf:about="&pimo;Agent"
    protege:role="abstract"
    rdfs:label="Agent">
  <pimo:classRole rdf:resource="&pimo;AbstractClass"/>
  <rdfs:comment>An agent (eg. person, group, software or physical artifact). The Agent class is the class of agents; things that do stuff. A well known sub-class is Person, representing people. Other kinds of agents include Organization and Group.
(inspired by FOAF).
Agent is not a subclass of NAO:Party.</rdfs:comment>
  <rdfs:subClassOf rdf:resource="&pimo;Thing"/>
</rdfs:Class>

<dcam:VocabularyEncodingScheme rdf:about="&dcterms;IMT">
  <dcterms:hasVersion rdf:resource="http://dublincore.org/usage/terms/history/#IMT-004"/>
  <dcterms:issued rdf:datatype="&xsd;date">2000-07-11</dcterms:issued>
  <dcterms:modified rdf:datatype="&xsd;date">2008-01-14</dcterms:modified>
  <rdfs:comment xml:lang="en">The set of media types specified by the Internet Assigned Numbers Authority.</rdfs:comment>
  <rdfs:isDefinedBy rdf:resource="&dcterms;"/>
  <rdfs:label xml:lang="en">IMT</rdfs:label>
  <rdfs:seeAlso rdf:resource="http://www.iana.org/assignments/media-types/"/>
</dcam:VocabularyEncodingScheme>

<rdf:Property rdf:about="&nfo;height"
    rdfs:comment="Visual content height in pixels."
    rdfs:label="height">
  <nrl:maxCardinality rdf:datatype="&xsd;integer">1</nrl:maxCardinality>
  <rdfs:domain rdf:resource="&nfo;Visual"/>
  <rdfs:range rdf:resource="&xsd;integer"/>
</rdf:Property>

<tmo:Delegability rdf:about="&tmo;TMO_Instance_Delegability_Low"
    rdfs:label="TMO_Instance_Delegability_Low"/>

<rdf:Property rdf:about="&nexif;jpegInterchangeFormat"
    rdfs:label="jpegInterchangeFormat">
  <rdfs:subPropertyOf rdf:resource="http://www.kanzaki.com/ns/exif#jpegInterchangeFormat"/>
  <rdfs:subPropertyOf rdf:resource="&nexif;recOffset"/>
  <rdfs:comment>tagNumber: 513
The offset to the start byte (SOI) of JPEG compressed thumbnail data. This is not used for primary image JPEG data.</rdfs:comment>
  <rdfs:domain rdf:resource="&nexif;Photo"/>
  <rdfs:range rdf:resource="&xsd;integer"/>
</rdf:Property>

<rdfs:Class rdf:about="&nco;MessagingNumber"
    rdfs:comment="A number that can accept textual messages."
    rdfs:label="MessagingNumber">
  <rdfs:subClassOf rdf:resource="&nco;PhoneNumber"/>
</rdfs:Class>

<rdf:Description rdf:about="&dpo;minUVIndex"
    rdfs:label="Minimum UV Index">
  <rdfs:comment></rdfs:comment>
  <rdfs:comment>A subproperty of dpo:minValue that defines a lowerbound on the observed uv index levels (linear scale of between 0 and 12 signifying 11+) such that it can classify as a dpo:WeatherCondition instance. It can be used in conjunction with dpo:maxUVIndex to state that specific instances of dpo:WeatherCondition have a pre-defined range of observable real-world UV index levels. In addition, they can also be used with various other weather conditions values and ranges to define complex weather condition types.</rdfs:comment>
  <rdfs:domain rdf:resource="&dpo;WeatherConditions"/>
  <rdfs:range rdf:resource="&xsd;nonNegativeInteger"/>
  <rdfs:subPropertyOf rdf:resource="&dpo;minValue"/>
</rdf:Description>

<ncal:EventStatus rdf:about="&ncal;tentativeStatus"
    rdfs:label="tentativeStatus"/>

<tmo:Importance rdf:about="&tmo;TMO_Instance_Importance_08"
    rdfs:label="TMO_Instance_Importance_08"/>

<rdf:Property rdf:about="&nie;links"
    rdfs:label="links">
  <rdfs:comment>A linking relation. A piece of content links/mentions a piece of data</rdfs:comment>
  <rdfs:domain rdf:resource="&nie;InformationElement"/>
  <rdfs:range rdf:resource="&nie;DataObject"/>
  <rdfs:subPropertyOf rdf:resource="&nie;relatedTo"/>
</rdf:Property>

<ncal:TodoStatus rdf:about="&ncal;completedStatus"
    rdfs:label="completedStatus"/>

<rdfs:Class rdf:about="&foaf;PersonalProfileDocument"
    rdfs:comment="A personal profile RDF document."
    rdfs:label="PersonalProfileDocument"
    ns:term_status="testing">
  <rdf:type rdf:resource="&owl;Class"/>
  <rdfs:subClassOf rdf:resource="&foaf;Document"/>
</rdfs:Class>

<rdf:Property rdf:about="&nmo;isRead"
    rdfs:label="isRead">
  <nrl:maxCardinality rdf:datatype="&xsd;integer">1</nrl:maxCardinality>
  <rdfs:comment>A flag that states the fact that a MailboxDataObject has been read.</rdfs:comment>
  <rdfs:domain rdf:resource="&nmo;Message"/>
  <rdfs:range rdf:resource="&xsd;boolean"/>
</rdf:Property>

<rdf:Property rdf:about="&dcterms;license">
  <rdfs:subPropertyOf rdf:resource="&dc;rights"/>
  <rdfs:subPropertyOf rdf:resource="&dcterms;rights"/>
  <dcterms:hasVersion rdf:resource="http://dublincore.org/usage/terms/history/#license-002"/>
  <dcterms:issued rdf:datatype="&xsd;date">2004-06-14</dcterms:issued>
  <dcterms:modified rdf:datatype="&xsd;date">2008-01-14</dcterms:modified>
  <rdfs:comment xml:lang="en">A legal document giving official permission to do something with the resource.</rdfs:comment>
  <rdfs:isDefinedBy rdf:resource="&dcterms;"/>
  <rdfs:label xml:lang="en">License</rdfs:label>
  <rdfs:range rdf:resource="&dcterms;LicenseDocument"/>
</rdf:Property>

<rdf:Property rdf:about="&foaf;topic"
    rdfs:comment="A topic of some page or document."
    rdfs:label="topic"
    ns:term_status="testing">
  <rdf:type rdf:resource="&owl;ObjectProperty"/>
  <rdfs:domain rdf:resource="&foaf;Document"/>
  <rdfs:isDefinedBy rdf:resource="&foaf;"/>
  <rdfs:range rdf:resource="&owl;Thing"/>
  <owl:inverseOf rdf:resource="&foaf;page"/>
</rdf:Property>

<rdf:Property rdf:about="&nco;addressLocation"
    nrl:maxCardinality="1"
    rdfs:comment="The geographical location of a postal address."
    rdfs:label="addressLocation">
  <rdfs:domain rdf:resource="&nco;PostalAddress"/>
  <rdfs:range rdf:resource="http://www.w3.org/2003/01/geo/wgs84_pos#Point"/>
</rdf:Property>

<rdfs:Class rdf:about="&dcon;LiveContext"
    rdfs:label="LiveContext">
  <rdfs:comment>This class represents the uninterpreted state of the users as sensed through their devices. Instances of this class should be limited, since they are meant to represent realtime, 'live' raw context information as sensed through a variety of a user's devices, their applications and sensors. Although one unique instance should represent the dynamically changing live context, additional instances can be used to contain live context information for the recent past.</rdfs:comment>
  <rdfs:subClassOf rdf:resource="&dcon;Context"/>
</rdfs:Class>

<rdf:Property rdf:about="&nco;logo"
    rdfs:label="logo">
  <rdfs:comment>Logo of a company. Inspired by the LOGO property defined in RFC 2426 sec. 3.5.3</rdfs:comment>
  <rdfs:domain rdf:resource="&nco;OrganizationContact"/>
  <rdfs:range rdf:resource="&nie;DataObject"/>
  <rdfs:subPropertyOf rdf:resource="&nie;hasPart"/>
</rdf:Property>

<rdf:Property rdf:about="&nexif;artist"
    rdfs:comment="tagNumber: 315
Person who created the image"
    rdfs:label="artist">
  <rdfs:subPropertyOf rdf:resource="http://www.kanzaki.com/ns/exif#artist"/>
  <rdfs:subPropertyOf rdf:resource="&nco;creator"/>
  <rdfs:subPropertyOf rdf:resource="&nexif;exifAttribute"/>
  <rdfs:domain rdf:resource="&nexif;Photo"/>
  <rdfs:range rdf:resource="&nco;Contact"/>
</rdf:Property>

<rdf:Property rdf:about="&nfo;wordCount"
    rdfs:comment="The amount of words in a text document."
    rdfs:label="wordCount">
  <nrl:maxCardinality rdf:datatype="&xsd;integer">1</nrl:maxCardinality>
  <rdfs:domain rdf:resource="&nfo;TextDocument"/>
  <rdfs:range rdf:resource="&xsd;integer"/>
</rdf:Property>

<rdfs:Class rdf:about="&nrl;ExternalViewSpecification"
    rdfs:label="ExternalViewSpecification">
  <rdfs:comment>Represents an external view specification, this usually being a program which automatically generates the required view for an input graph</rdfs:comment>
  <rdfs:subClassOf rdf:resource="&nrl;ViewSpecification"/>
</rdfs:Class>

<rdf:Property rdf:about="&dcon;weight"
    rdfs:label="Item Weight">
  <rdfs:comment>This property assigns different weights to specific context aspects and/or elements, in order to better characterise a situation. As weights can be attached to both dcon:Element and dcon:Aspect instances, the domain of this property is generalised to dcon:Observation. However, the attachment of weights to other instances is not considered correct application of the DCON vocabulary. Expected weight values range from 0 (no impact on situation), to 1 (high impact on a situation). In addition, the dcon:isRequired property defines a necessity relationship between a context element and a situation, whereas the dcon:isExcluder property defines the inverse.</rdfs:comment>
  <rdfs:domain rdf:resource="&dcon;Observation"/>
  <rdfs:range rdf:resource="&xsd;float"/>
</rdf:Property>

<rdf:Property rdf:about="&nfo;sampleCount"
    rdfs:comment="The amount of samples in an audio clip."
    rdfs:label="sampleCount">
  <nrl:maxCardinality rdf:datatype="&xsd;integer">1</nrl:maxCardinality>
  <rdfs:domain rdf:resource="&nfo;Audio"/>
  <rdfs:range rdf:resource="&xsd;integer"/>
  <rdfs:subPropertyOf rdf:resource="&nfo;count"/>
</rdf:Property>

<rdf:Property rdf:about="&dc;description">
  <dcterms:description xml:lang="en">Description may include but is not limited to: an abstract, a table of contents, a graphical representation, or a free-text account of the resource.</dcterms:description>
  <dcterms:hasVersion rdf:resource="http://dublincore.org/usage/terms/history/#description-006"/>
  <dcterms:issued rdf:datatype="&xsd;date">1999-07-02</dcterms:issued>
  <dcterms:modified rdf:datatype="&xsd;date">2008-01-14</dcterms:modified>
  <rdf:type rdf:resource="&owl;AnnotationProperty"/>
  <rdfs:comment xml:lang="en">An account of the resource.</rdfs:comment>
  <rdfs:isDefinedBy rdf:resource="&dc;"/>
  <rdfs:label xml:lang="en">Description</rdfs:label>
  <scos:note xml:lang="en">A second property with the same name as this property has been declared in the dcterms: namespace (http://purl.org/dc/terms/).  See the Introduction to the document "DCMI Metadata Terms" (http://dublincore.org/documents/dcmi-terms/) for an explanation.</scos:note>
</rdf:Property>

<rdfs:Class rdf:about="&nao;FreeDesktopIcon"
    rdfs:label="freedesktopicon">
  <rdfs:comment>Represents a desktop icon as defined in the FreeDesktop Icon Naming Standard (http://standards.freedesktop.org/icon-naming-spec/icon-naming-spec-latest.html).</rdfs:comment>
  <rdfs:subClassOf rdf:resource="&nao;Symbol"/>
</rdfs:Class>

<pimo:ClassRole rdf:about="&pimo;AbstractClass"
    rdfs:label="AbstractClass"/>

<rdf:Property rdf:about="&pimo;hasTag"
    rdfs:label="has tag">
  <rdfs:subPropertyOf rdf:resource="&nao;hasTag"/>
  <rdfs:subPropertyOf rdf:resource="&pimo;objectProperty"/>
  <nrl:inverseProperty rdf:resource="&pimo;isTagFor"/>
  <rdfs:comment>The subject's contents describes the object. Or the subject can be seen as belonging to the thing described by the object.  Similar semantics as skos:subject.</rdfs:comment>
  <rdfs:domain rdf:resource="&pimo;Thing"/>
  <rdfs:range rdf:resource="&pimo;Tag"/>
</rdf:Property>

<rdf:Property rdf:about="&nco;hasAffiliation"
    rdfs:comment="Links a PersonContact with an Affiliation."
    rdfs:label="hasAffiliation">
  <rdfs:domain rdf:resource="&nco;PersonContact"/>
  <rdfs:range rdf:resource="&nco;Affiliation"/>
</rdf:Property>

<rdf:Property rdf:about="&nrl;minCardinality"
    rdfs:label="minCardinality">
  <rdfs:comment>Specifies a minimum value cardinality for a specific property</rdfs:comment>
  <rdfs:domain rdf:resource="&rdf;Property"/>
  <rdfs:range rdf:resource="&rdfs;Literal"/>
</rdf:Property>

<rdfs:Class rdf:about="&cnt;ContentAsBase64">
  <rdf:type rdf:resource="&owl;Class"/>
  <rdfs:comment xml:lang="en">The base64 encoded content (can be used for binary content).</rdfs:comment>
  <rdfs:label xml:lang="en">Base64 content</rdfs:label>
  <rdfs:subClassOf rdf:resource="&cnt;Content"/>
</rdfs:Class>

<rdf:Property rdf:about="&pimo;wikiText"
    nrl:maxCardinality="1"
    rdfs:label="wiki text">
  <rdfs:comment>A wiki-like free-text description of a Thing or a Class. The text can be formatted using a limited set of HTML elements and can contain links to other Things. The format is described in detail in the WIF specification (http://semanticweb.org/wiki/Wiki_Interchange_Format).</rdfs:comment>
  <rdfs:domain rdf:resource="&pimo;ClassOrThing"/>
  <rdfs:range rdf:resource="&rdfs;Literal"/>
</rdf:Property>

<nco:Gender rdf:about="&nco;female"
    rdfs:comment="A Female"
    rdfs:label="female"/>

<tmo:PersonInvolvementRole rdf:about="&tmo;TMO_Instance_PersonInvolvementRole_Co-worker"
    rdfs:label="TMO_Instance_PersonInvolvementRole_Co-worker"/>

<rdfs:Class rdf:about="&dplo;LivePost"
    rdfs:label="LivePost">
  <rdfs:subClassOf rdf:resource="http://rdfs.org/sioc/ns#Post"/>
  <rdfs:subClassOf rdf:resource="&nie;InformationElement"/>
  <rdfs:comment>A generic representation of personal information intended for instant online sharing, typically over social networks. Extended through various subclasses. When an item is shared as a livepost, it can be managed as a separate new entity. For this purpose, all LivePost instances also become instances of nie:InformationElements.</rdfs:comment>
</rdfs:Class>

<rdf:Property rdf:about="&pimo;hasRootTopic"
    rdfs:label="root topic">
  <rdfs:comment>The root topics of this PersonalInformationModel's topic hierarchy. Every topic that has no pimo:superTopic is a root topic. Semantically equivalent to skos:hasTopConcept.</rdfs:comment>
  <rdfs:domain rdf:resource="&pimo;PersonalInformationModel"/>
  <rdfs:range rdf:resource="&pimo;Topic"/>
</rdf:Property>

<nrl:InverseFunctionalProperty rdf:about="&nao;personalIdentifier"
    rdfs:comment="Defines a personal string identifier for a resource"
    rdfs:label="personal identifier">
  <rdf:type rdf:resource="&rdf;Property"/>
  <rdfs:range rdf:resource="&rdfs;Literal"/>
  <rdfs:subPropertyOf rdf:resource="&nao;identifier"/>
</nrl:InverseFunctionalProperty>

<rdfs:Class rdf:about="&nco;Affiliation"
    rdfs:label="Affiliation">
  <rdfs:comment>Aggregates three properties defined in RFC2426. Originally all three were attached directly to a person. One person could have only one title and one role within one organization. This class is intended to lift this limitation.</rdfs:comment>
  <rdfs:subClassOf rdf:resource="&nco;Role"/>
</rdfs:Class>

<rdf:Property rdf:about="&nfo;foundry"
    rdfs:comment="The foundry, the organization that created the font."
    rdfs:label="foundry">
  <nrl:maxCardinality rdf:datatype="&xsd;integer">1</nrl:maxCardinality>
  <rdfs:domain rdf:resource="&nfo;Font"/>
  <rdfs:range rdf:resource="&nco;Contact"/>
  <rdfs:subPropertyOf rdf:resource="&nco;creator"/>
</rdf:Property>

<rdf:Property rdf:about="&dc;coverage">
  <dcterms:description xml:lang="en">Spatial topic and spatial applicability may be a named place or a location specified by its geographic coordinates. Temporal topic may be a named period, date, or date range. A jurisdiction may be a named administrative entity or a geographic place to which the resource applies. Recommended best practice is to use a controlled vocabulary such as the Thesaurus of Geographic Names [TGN]. Where appropriate, named places or time periods can be used in preference to numeric identifiers such as sets of coordinates or date ranges.</dcterms:description>
  <dcterms:hasVersion rdf:resource="http://dublincore.org/usage/terms/history/#coverage-006"/>
  <dcterms:issued rdf:datatype="&xsd;date">1999-07-02</dcterms:issued>
  <dcterms:modified rdf:datatype="&xsd;date">2008-01-14</dcterms:modified>
  <rdfs:comment xml:lang="en">The spatial or temporal topic of the resource, the spatial applicability of the resource, or the jurisdiction under which the resource is relevant.</rdfs:comment>
  <rdfs:isDefinedBy rdf:resource="&dc;"/>
  <rdfs:label xml:lang="en">Coverage</rdfs:label>
  <scos:note xml:lang="en">A second property with the same name as this property has been declared in the dcterms: namespace (http://purl.org/dc/terms/).  See the Introduction to the document "DCMI Metadata Terms" (http://dublincore.org/documents/dcmi-terms/) for an explanation.</scos:note>
</rdf:Property>

<rdfs:Class rdf:about="&tmo;PersonInvolvement"
    rdfs:label="PersonInvolvement">
  <rdfs:subClassOf rdf:resource="&pimo;Association"/>
  <rdfs:subClassOf rdf:resource="&rdfs;Resource"/>
  <rdfs:comment>PersonInvolvement  realizes n-ary associations to Persons which are realtedd to an task. The involvement is further characterized by an PersonTaskRole.</rdfs:comment>
</rdfs:Class>

<rdf:Property rdf:about="&nco;contactUID"
    nrl:maxCardinality="1"
    rdfs:label="contactUID">
  <rdfs:comment>A value that represents a globally unique  identifier corresponding to the individual or resource associated with the Contact. An equivalent of the 'UID' property defined in RFC 2426 Sec. 3.6.7</rdfs:comment>
  <rdfs:domain rdf:resource="&nco;Contact"/>
  <rdfs:range rdf:resource="&xsd;string"/>
  <rdfs:subPropertyOf rdf:resource="&nie;identifier"/>
</rdf:Property>

<rdf:Property rdf:about="&nexif;shutterSpeedValue"
    rdfs:label="shutterSpeedValue">
  <rdfs:subPropertyOf rdf:resource="http://www.kanzaki.com/ns/exif#shutterSpeedValue"/>
  <rdfs:subPropertyOf rdf:resource="&nexif;pictTaking"/>
  <rdfs:comment>tagNumber: 37377
Shutter speed. The unit is the APEX (Additive System of Photographic Exposure) setting</rdfs:comment>
  <rdfs:domain rdf:resource="&nexif;Photo"/>
  <rdfs:range rdf:resource="&xsd;float"/>
</rdf:Property>

<rdf:Property rdf:about="&tmo;abilityCarrierInvolvement"
    rdfs:label="abilityCarrierInvolvement">
  <nrl:inverseProperty rdf:resource="&tmo;abilityCarrierTask"/>
  <rdfs:domain rdf:resource="&tmo;Task"/>
  <rdfs:range rdf:resource="&tmo;AbilityCarrierInvolvement"/>
</rdf:Property>

<rdf:Property rdf:about="&nao;directTrust"
    rdfs:label="direct trust">
  <rdfs:comment>A direct trust value assigned to an agent, either manually by a user or semi-/automatically by a system. Allowed values range from 0 (no trust) to 1 (very high trust).</rdfs:comment>
  <rdfs:domain rdf:resource="&pimo;Agent"/>
  <rdfs:range rdf:resource="&xsd;double"/>
  <rdfs:subPropertyOf rdf:resource="&nao;trustLevel"/>
</rdf:Property>

<rdf:Property rdf:about="&nao;favouritedBy"
    rdfs:label="favourited by">
  <rdfs:comment>Signifies social endorsment by an agent, by way of marking the resource as a favourite.</rdfs:comment>
  <rdfs:domain rdf:resource="&rdfs;Resource"/>
  <rdfs:range rdf:resource="&nao;Party"/>
  <rdfs:subPropertyOf rdf:resource="&nao;endorsedBy"/>
</rdf:Property>

<rdfs:Class rdf:about="&ncal;AlarmAction"
    rdfs:label="AlarmAction">
  <rdfs:comment>Action to be performed on alarm. This class has been introduced to express the limited set of values of the ncal:action property. Please refer to the documentation of ncal:action for details.</rdfs:comment>
  <rdfs:subClassOf rdf:resource="&rdfs;Resource"/>
</rdfs:Class>

<rdf:Property rdf:about="&nexif;pimSharpness"
    rdfs:comment="Sharpness info for print image matching
tagNumber: 13"
    rdfs:label="pimSharpness">
  <rdfs:subPropertyOf rdf:resource="http://www.kanzaki.com/ns/exif#pimSharpness"/>
  <rdfs:subPropertyOf rdf:resource="&nexif;pimInfo"/>
  <rdfs:domain rdf:resource="&nexif;Photo"/>
  <rdfs:range rdf:resource="&xsd;string"/>
</rdf:Property>

<rdf:Property rdf:about="&pimo;hasFolder"
    rdfs:label="has folder">
  <rdfs:comment>Folders can be used to store information elements related to a Thing or Class. This property can be used to connect a Class or Thing to existing Folders. Implementations can suggest annotations for documents stored inside these folders or  suggest the folder for new documents related to the Thing or Class.</rdfs:comment>
  <rdfs:domain rdf:resource="&pimo;ClassOrThing"/>
  <rdfs:range rdf:resource="&nfo;Folder"/>
</rdf:Property>

<rdf:Property rdf:about="&dcon;forecastWeather"
    rdfs:label="Forecast Weather">
  <rdfs:comment>Refers to a forecast, pre-defined weather condition characterising a context instance.</rdfs:comment>
  <rdfs:domain rdf:resource="&dcon;Environment"/>
  <rdfs:range rdf:resource="&dpo;WeatherConditions"/>
  <rdfs:subPropertyOf rdf:resource="&dcon;hasContextElement"/>
</rdf:Property>

<rdf:Property rdf:about="&nie;created"
    nrl:maxCardinality="1"
    rdfs:label="created">
  <rdfs:subPropertyOf rdf:resource="&dcterms;created"/>
  <rdfs:subPropertyOf rdf:resource="&nie;modified"/>
  <rdfs:subPropertyOf rdf:resource="&nao;created"/>
  <rdfs:comment>Date of creation of the DataObject. Note that this date refers to the creation of the DataObject itself (i.e. the physical representation). Compare with nie:contentCreated.</rdfs:comment>
  <rdfs:domain rdf:resource="&nie;DataObject"/>
  <rdfs:range rdf:resource="&xsd;dateTime"/>
</rdf:Property>

<rdf:Property rdf:about="&nid3;generalEncapsulatedObject"
    rdfs:label="generalEncapsulatedObject">
  <rdfs:comment>An arbitrary file embedded in an audio file. Inspired by http://www.id3.org/id3v2.3.0 sec. 
4.16)</rdfs:comment>
  <rdfs:domain rdf:resource="&nid3;ID3Audio"/>
  <rdfs:range rdf:resource="&nie;DataObject"/>
  <rdfs:subPropertyOf rdf:resource="&nie;hasPart"/>
</rdf:Property>

<rdf:Property rdf:about="&nie;byteSize"
    nrl:maxCardinality="1"
    rdfs:label="byteSize">
  <rdfs:comment>The overall size of the data object in bytes. That means the space taken by the DataObject in its container, and not the size of the content that is of interest to the user. For cases where the content size is different (e.g. in compressed files the content is larger, in messages the content excludes headings and is smaller) use more specific properties, not necessarily subproperties of this one.</rdfs:comment>
  <rdfs:domain rdf:resource="&nie;DataObject"/>
  <rdfs:range rdf:resource="&xsd;integer"/>
</rdf:Property>

<rdf:Property rdf:about="&nexif;focalPlaneYResolution"
    rdfs:label="focalPlaneYResolution">
  <rdfs:subPropertyOf rdf:resource="http://www.kanzaki.com/ns/exif#focalPlaneYResolution"/>
  <rdfs:subPropertyOf rdf:resource="&nexif;pictTaking"/>
  <rdfs:subPropertyOf rdf:resource="&nexif;resolution"/>
  <rdfs:comment>tagNumber: 41487
The number of pixels in the image height (Y) direction per FocalPlaneResolutionUnit on the camera focal plane.</rdfs:comment>
  <rdfs:domain rdf:resource="&nexif;Photo"/>
  <rdfs:range rdf:resource="&xsd;float"/>
</rdf:Property>

<rdf:Property rdf:about="&scos;note">
  <rdf:type rdf:resource="&owl;AnnotationProperty"/>
  <rdfs:isDefinedBy rdf:resource="http://www.w3.org/2004/02/skos/core"/>
  <rdfs:label xml:lang="en">note</rdfs:label>
  <scos:definition xml:lang="en">A general note, for any purpose.</scos:definition>
  <scos:scopeNote xml:lang="en">This property may be used directly, or as a super-property for more specific note types.</scos:scopeNote>
</rdf:Property>

<rdfs:Class rdf:about="&foaf;OnlineGamingAccount"
    rdfs:comment="An online gaming account."
    rdfs:label="Online Gaming Account"
    ns:term_status="unstable">
  <rdf:type rdf:resource="&owl;Class"/>
  <rdfs:isDefinedBy rdf:resource="&foaf;"/>
  <rdfs:subClassOf rdf:resource="&foaf;OnlineAccount"/>
</rdfs:Class>

<rdf:Property rdf:about="&foaf;account"
    rdfs:comment="Indicates an account held by this agent."
    rdfs:label="account"
    ns:term_status="testing">
  <rdf:type rdf:resource="&owl;ObjectProperty"/>
  <rdfs:domain rdf:resource="&foaf;Agent"/>
  <rdfs:isDefinedBy rdf:resource="&foaf;"/>
  <rdfs:range rdf:resource="&foaf;OnlineAccount"/>
</rdf:Property>

<rdf:Property rdf:about="&nrl;externalRealizer"
    rdfs:label="externalRealizer">
  <rdfs:comment>Points to the location of the realizer for the external view specification</rdfs:comment>
  <rdfs:domain rdf:resource="&nrl;ExternalViewSpecification"/>
  <rdfs:range rdf:resource="&rdfs;Literal"/>
</rdf:Property>

<nrl:TransitiveProperty rdf:about="&pimo;superTopic"
    rdfs:label="broader topic">
  <rdfs:subPropertyOf rdf:resource="&pimo;objectProperty"/>
  <rdfs:subPropertyOf rdf:resource="&pimo;partOf"/>
  <nrl:inverseProperty rdf:resource="&pimo;subTopic"/>
  <rdf:type rdf:resource="&rdf;Property"/>
  <rdfs:comment>The object topic is more general in meaning than the subject topic. Transitive. Similar to skos:broader.</rdfs:comment>
  <rdfs:domain rdf:resource="&pimo;Topic"/>
  <rdfs:range rdf:resource="&pimo;Topic"/>
</nrl:TransitiveProperty>

<rdfs:Class rdf:about="&nrl;Schema"
    rdfs:comment="Represents a named graph containing schematic data"
    rdfs:label="Schema">
  <rdfs:subClassOf rdf:resource="&nrl;Data"/>
</rdfs:Class>

<rdf:Property rdf:about="&ncal;bysecond"
    rdfs:comment="Second of a recurrence. Defined in RFC 2445 sec. 4.3.10"
    rdfs:label="bysecond">
  <rdfs:domain rdf:resource="&ncal;RecurrenceRule"/>
  <rdfs:range rdf:resource="&xsd;integer"/>
</rdf:Property>

<rdf:Property rdf:about="&dplo;isComposedOf"
    rdfs:label="is composed of">
  <rdfs:comment>One online post can simultaneously consist of various types of livepost subclasses as defined by DLPO. These are semantically related to the parent post through this property.</rdfs:comment>
  <rdfs:domain rdf:resource="&dplo;LivePost"/>
  <rdfs:range rdf:resource="&dplo;LivePost"/>
  <rdfs:subPropertyOf rdf:resource="&nao;hasSubResource"/>
</rdf:Property>

<rdf:Property rdf:about="&nexif;gpsDest"
    rdfs:label="gpsDest">
  <rdfs:comment>Location of the destination. This property aggregates values of two other properties from the original exif specification. gpsDestLatitude (tag number 20) and gpsDestLongitude (tag number 22)</rdfs:comment>
  <rdfs:range rdf:resource="http://www.w3.org/2003/01/geo/wgs84_pos#Point"/>
  <rdfs:subPropertyOf rdf:resource="&nexif;geo"/>
</rdf:Property>

<rdf:Property rdf:about="&tmo;attachmentTask"
    nrl:maxCardinality="1"
    rdfs:label="attachmentTask">
  <nrl:inverseProperty rdf:resource="&tmo;attachment"/>
  <rdfs:comment>Inverse of attachment, connects an Attachment Association to the associated Task. Is required for every instance of Attachment.</rdfs:comment>
  <rdfs:domain rdf:resource="&tmo;Attachment"/>
  <rdfs:range rdf:resource="&tmo;Task"/>
  <rdfs:subPropertyOf rdf:resource="&pimo;associationMember"/>
</rdf:Property>

<rdf:Property rdf:about="&dcterms;spatial">
  <rdfs:subPropertyOf rdf:resource="&dc;coverage"/>
  <rdfs:subPropertyOf rdf:resource="&dcterms;coverage"/>
  <dcterms:hasVersion rdf:resource="http://dublincore.org/usage/terms/history/#spatial-003"/>
  <dcterms:issued rdf:datatype="&xsd;date">2000-07-11</dcterms:issued>
  <dcterms:modified rdf:datatype="&xsd;date">2008-01-14</dcterms:modified>
  <rdfs:comment xml:lang="en">Spatial characteristics of the resource.</rdfs:comment>
  <rdfs:isDefinedBy rdf:resource="&dcterms;"/>
  <rdfs:label xml:lang="en">Spatial Coverage</rdfs:label>
  <rdfs:range rdf:resource="&dcterms;Location"/>
</rdf:Property>

<rdf:Property rdf:about="&rdfs;range">
  <rdfs:comment xml:lang="en">A range of the subject property.</rdfs:comment>
  <rdfs:domain rdf:resource="&rdf;Property"/>
  <rdfs:isDefinedBy rdf:resource="&rdfs;"/>
  <rdfs:label xml:lang="en">range</rdfs:label>
  <rdfs:range rdf:resource="&rdfs;Class"/>
</rdf:Property>

<dcam:VocabularyEncodingScheme rdf:about="&dcterms;LCC">
  <dcterms:hasVersion rdf:resource="http://dublincore.org/usage/terms/history/#LCC-003"/>
  <dcterms:issued rdf:datatype="&xsd;date">2000-07-11</dcterms:issued>
  <dcterms:modified rdf:datatype="&xsd;date">2008-01-14</dcterms:modified>
  <rdfs:comment xml:lang="en">The set of conceptual resources specified by the Library of Congress Classification.</rdfs:comment>
  <rdfs:isDefinedBy rdf:resource="&dcterms;"/>
  <rdfs:label xml:lang="en">LCC</rdfs:label>
  <rdfs:seeAlso rdf:resource="http://lcweb.loc.gov/catdir/cpso/lcco/lcco.html"/>
</dcam:VocabularyEncodingScheme>

<rdf:Property rdf:about="&nrl;rule"
    rdfs:label="rule">
  <rdfs:comment>Specifies rules for a view specification that is driven by rules</rdfs:comment>
  <rdfs:domain rdf:resource="&nrl;RuleViewSpecification"/>
  <rdfs:range rdf:resource="&rdfs;Literal"/>
</rdf:Property>

<rdf:Property rdf:about="&dpo;maxPrecipitation"
    rdfs:label="Maximum Precipitation">
  <rdfs:comment>A subproperty of dpo:maxValue that defines an upperbound on the observed precipitation levels (in millimetres per hour) such that it can classify as a dpo:WeatherCondition instance. It can be used in conjunction with dpo:minPrecipitation to state that specific instances of dpo:WeatherCondition have a pre-defined range of observable real-world precipitation levels. In addition, they can also be used with various other weather conditions values and ranges to define complex weather condition types.</rdfs:comment>
  <rdfs:domain rdf:resource="&dpo;WeatherConditions"/>
  <rdfs:range rdf:resource="&xsd;nonNegativeInteger"/>
  <rdfs:subPropertyOf rdf:resource="&dpo;maxValue"/>
</rdf:Property>

<rdf:Property rdf:about="&nid3;contentGroupDescription"
    rdfs:label="contentGroupDescription">
  <rdfs:comment>TIT1
The 'Content group description' frame is used if the sound belongs to a larger category of sounds/music. For example, classical music is often sorted in different musical sections (e.g. "Piano Concerto", "Weather - Hurricane").</rdfs:comment>
  <rdfs:domain rdf:resource="&nid3;ID3Audio"/>
  <rdfs:range rdf:resource="&xsd;string"/>
</rdf:Property>

<rdf:Property rdf:about="&nso;includes"
    rdfs:label="includes">
  <nrl:minCardinality rdf:datatype="&xsd;nonNegativeInteger">1</nrl:minCardinality>
  <rdfs:comment>Enables a 'whitelist' membership property for agents with respect to privacy preferences as defined by the PPO Ontology. If included within the access space of a privacy preference, an agent will have access to the resources within. At least one agent must be defined for whitelist membership in an access space.</rdfs:comment>
  <rdfs:domain rdf:resource="&nso;AccessSpace"/>
  <rdfs:range rdf:resource="&pimo;Agent"/>
  <rdfs:subPropertyOf rdf:resource="http://vocab.deri.ie/ppo#hasAccessAgent"/>
</rdf:Property>

<rdf:Property rdf:about="&ncal;categories"
    rdfs:label="categories">
  <rdfs:comment>Categories for a calendar component. Inspired by RFC 2445 sec 4.8.1.2 with the following reservations: The LANGUAGE parameter has been discarded. Please use xml:lang literals to express multiple languages. This property can specify multiple comma-separated categories. The order of categories doesn't matter. Please use a separate triple for each category.</rdfs:comment>
  <rdfs:domain rdf:resource="&ncal;UnionOfEventJournalTodo"/>
  <rdfs:range rdf:resource="&xsd;string"/>
</rdf:Property>

<rdf:Property rdf:about="&nexif;fileSource"
    rdfs:label="fileSource">
  <rdfs:subPropertyOf rdf:resource="http://www.kanzaki.com/ns/exif#fileSource"/>
  <rdfs:subPropertyOf rdf:resource="&nexif;pictTaking"/>
  <rdfs:comment>The image source. If a DSC recorded the image, this tag value of this tag always be set to 3, indicating that the image was recorded on a DSC.
tagNumber: 41728</rdfs:comment>
  <rdfs:domain rdf:resource="&nexif;Photo"/>
  <rdfs:range rdf:resource="&xsd;string"/>
</rdf:Property>

<rdf:Property rdf:about="&nie;comment"
    rdfs:comment="A user comment about an InformationElement."
    rdfs:label="comment">
  <rdfs:domain rdf:resource="&nie;InformationElement"/>
  <rdfs:range rdf:resource="&xsd;string"/>
</rdf:Property>

<rdf:Property rdf:about="&nao;isDataGraphFor"
    rdfs:label="is data graph for">
  <nrl:inverseProperty rdf:resource="&nao;hasDataGraph"/>
  <rdfs:comment>Links a named graph to the resource for which it contains metadata. Its typical usage would be to link the graph containing extracted file metadata to the file resource. This allows for easy maintenance later on. Inverse property of nao:hasDataGraph.</rdfs:comment>
  <rdfs:domain rdf:resource="&nrl;InstanceBase"/>
  <rdfs:range rdf:resource="&rdfs;Resource"/>
</rdf:Property>

<rdf:Property rdf:about="&nie;hasLogicalPart"
    rdfs:label="hasLogicalPart">
  <nrl:inverseProperty rdf:resource="&nie;isLogicalPartOf"/>
  <rdfs:comment>Generic property used to express 'logical' containment relationships between InformationElements. NIE extensions are encouraged to provide more specific subproperties of this one. It is advisable for actual instances of InformationElement to use those specific subproperties. Note the difference between 'physical' containment (hasPart) and logical containment (hasLogicalPart)</rdfs:comment>
  <rdfs:domain rdf:resource="&nie;InformationElement"/>
  <rdfs:range rdf:resource="&nie;InformationElement"/>
  <rdfs:subPropertyOf rdf:resource="&dcterms;hasPart"/>
</rdf:Property>

<rdf:Property rdf:about="&nuao;firstModification"
    rdfs:comment="The start time of the first modification"
    rdfs:label="first modification event">
  <nrl:maxCardinality rdf:datatype="&xsd;nonNegativeInteger">1</nrl:maxCardinality>
  <rdfs:domain rdf:resource="&rdfs;Resource"/>
  <rdfs:range rdf:resource="&xsd;dateTime"/>
</rdf:Property>

<nrl:DefiningProperty rdf:about="&nmm;producer"
    rdfs:comment="Producer"
    rdfs:label="producer">
  <rdf:type rdf:resource="&rdf;Property"/>
  <rdfs:domain rdf:resource="&nfo;Video"/>
  <rdfs:range rdf:resource="&nco;Contact"/>
  <rdfs:subPropertyOf rdf:resource="&nco;contributor"/>
</nrl:DefiningProperty>

<rdf:Property rdf:about="&nco;sound"
    rdfs:label="sound">
  <rdfs:comment>Sound clip attached to a Contact. The DataObject referred to by this property is usually interpreted as an nfo:Audio. Inspired by the SOUND property defined in RFC 2425 sec. 3.6.6.</rdfs:comment>
  <rdfs:domain rdf:resource="&nco;Contact"/>
  <rdfs:range rdf:resource="&nie;DataObject"/>
  <rdfs:subPropertyOf rdf:resource="&nie;hasPart"/>
</rdf:Property>

<rdf:Property rdf:about="&dcon;altitude"
    rdfs:comment="States the current altitude (metres above sea level)"
    rdfs:label="Altitude Value">
  <rdfs:domain rdf:resource="&dpo;Altitude"/>
  <rdfs:range rdf:resource="&xsd;float"/>
  <rdfs:subPropertyOf rdf:resource="&dcon;hasContextAttribute"/>
</rdf:Property>

<rdf:Property rdf:about="&nso;isPrivacyPreferenceOf"
    rdfs:label="is privacy preference of">
  <nrl:inverseProperty rdf:resource="&nso;hasPrivacyPreference"/>
  <rdfs:comment>Links privacy preferences to the agent that owns them. Inverse of hasPrivacyPreference.</rdfs:comment>
  <rdfs:domain rdf:resource="http://vocab.deri.ie/ppo#PrivacyPreference"/>
  <rdfs:range rdf:resource="&pimo;Agent"/>
</rdf:Property>

<rdf:Property rdf:about="&nexif;pixelXDimension"
    rdfs:label="pixelXDimension">
  <rdfs:subPropertyOf rdf:resource="http://www.kanzaki.com/ns/exif#pixelXDimension"/>
  <rdfs:subPropertyOf rdf:resource="&nexif;imageConfig"/>
  <rdfs:subPropertyOf rdf:resource="&nexif;width"/>
  <rdfs:comment>Information specific to compressed data. When a compressed file is recorded, the valid width of the meaningful image shall be recorded in this tag, whether or not there is padding data or a restart marker. This tag should not exist in an uncompressed file.
tagNumber: 40962</rdfs:comment>
  <rdfs:domain rdf:resource="&nexif;Photo"/>
  <rdfs:range rdf:resource="&xsd;string"/>
</rdf:Property>

<rdf:Property rdf:about="&nco;emailAddress"
    rdfs:label="emailAddress">
  <nrl:maxCardinality rdf:datatype="&xsd;integer">1</nrl:maxCardinality>
  <rdfs:domain rdf:resource="&nco;EmailAddress"/>
  <rdfs:range rdf:resource="&xsd;string"/>
</rdf:Property>

<rdf:Property rdf:about="&nexif;apertureValue"
    rdfs:label="apertureValue">
  <rdfs:subPropertyOf rdf:resource="http://www.kanzaki.com/ns/exif#apertureValue"/>
  <rdfs:subPropertyOf rdf:resource="&nexif;pictTaking"/>
  <rdfs:comment>tagNumber: 37378
The lens aperture. The unit is the APEX value.</rdfs:comment>
  <rdfs:domain rdf:resource="&nexif;Photo"/>
  <rdfs:range rdf:resource="&xsd;float"/>
</rdf:Property>

<rdf:Property rdf:about="&nrl;graphMetadataFor"
    rdfs:label="graphMetadataFor">
  <nrl:minCardinality rdf:datatype="&xsd;nonNegativeInteger">1</nrl:minCardinality>
  <rdfs:comment>Links a metadata graph to the graph that is being described. A unique value is compulsory</rdfs:comment>
  <rdfs:domain rdf:resource="&nrl;GraphMetadata"/>
  <rdfs:range rdf:resource="&nrl;Graph"/>
</rdf:Property>

<rdf:Property rdf:about="&nexif;primaryChromaticities"
    rdfs:label="primaryChromaticities">
  <rdfs:subPropertyOf rdf:resource="http://www.kanzaki.com/ns/exif#primaryChromaticities"/>
  <rdfs:subPropertyOf rdf:resource="&nexif;imageDataCharacter"/>
  <rdfs:comment>The chromaticity of the three primary colors of the image. Normally this tag is not necessary, since color space is specified in the color space information tag (ColorSpace).
tagNumber: 319</rdfs:comment>
  <rdfs:domain rdf:resource="&nexif;Photo"/>
  <rdfs:range rdf:resource="&xsd;string"/>
</rdf:Property>

<rdfs:Class rdf:about="&nfo;ArchiveItem"
    rdfs:comment="A file entity inside an archive."
    rdfs:label="ArchiveItem">
  <rdfs:subClassOf rdf:resource="&nfo;EmbeddedFileDataObject"/>
</rdfs:Class>

<rdfs:Class rdf:about="&rdfs;ContainerMembershipProperty">
  <rdfs:comment xml:lang="en">The class of container membership properties, rdf:_1, rdf:_2, ...,
                    all of which are sub-properties of 'member'.</rdfs:comment>
  <rdfs:isDefinedBy rdf:resource="&rdfs;"/>
  <rdfs:label xml:lang="en">ContainerMembershipProperty</rdfs:label>
  <rdfs:subClassOf rdf:resource="&rdf;Property"/>
</rdfs:Class>

<rdfs:Class rdf:about="&tmo;TaskDependency"
    protege:role="abstract"
    rdfs:label="TaskDependency">
  <rdfs:subClassOf rdf:resource="&pimo;Association"/>
  <rdfs:subClassOf rdf:resource="&rdfs;Resource"/>
  <rdfs:comment>Between the tasks, further dependencies may exist. These dependencies allow for a graph network structure. For ease of use, dependencies should not be too frequent, otherwise the primarily character of a hierarchy would be diminished and a consequent graph representation would become considerable. However, such a graph representation has other drawbacks, the user is likely to loose oversight, tree structures are more helpful in structuring the work.

A dependency relation is characterized by the type of the relation and by an additional description. There are different possibilities for dependency relations between tasks.</rdfs:comment>
</rdfs:Class>

<rdf:Property rdf:about="&nmm;albumPeakGain"
    rdfs:comment="ReplayGain album(audiophile) peak gain"
    rdfs:label="album peak gain">
  <nrl:maxCardinality rdf:datatype="&xsd;integer">1</nrl:maxCardinality>
  <rdfs:domain rdf:resource="&nmm;MusicAlbum"/>
  <rdfs:range rdf:resource="&xsd;float"/>
</rdf:Property>

<rdf:Property rdf:about="&nexif;stripOffsets"
    rdfs:label="stripOffsets">
  <rdfs:subPropertyOf rdf:resource="http://www.kanzaki.com/ns/exif#stripOffsets"/>
  <rdfs:subPropertyOf rdf:resource="&nexif;recOffset"/>
  <rdfs:comment>For each strip, the byte offset of that strip. With JPEG compressed data this designation is not needed and is omitted.
tagNumber: 273</rdfs:comment>
  <rdfs:domain rdf:resource="&nexif;Photo"/>
  <rdfs:range rdf:resource="&xsd;string"/>
</rdf:Property>

<owl:Class rdf:about="&oa;Motivation">
  <rdfs:comment xml:lang="en">The Motivation for creating an Annotation, indicated with oa:motivatedBy, is a reason for its creation, and might include things like oa:replying to another annotation, oa:commenting on a resource, or oa:linking to a related resource.

Each Annotation SHOULD have at least one oa:motivatedBy relationship to an instance of oa:Motivation, which is a subClass of skos:Concept.</rdfs:comment>
  <rdfs:isDefinedBy rdf:resource="&oa;"/>
  <rdfs:label xml:lang="en">Motivation</rdfs:label>
  <rdfs:subClassOf rdf:resource="&scos;Concept"/>
</owl:Class>

<rdf:Property rdf:about="&nmo;messageFrom"
    rdfs:comment="The sender of the message"
    rdfs:label="from">
  <nrl:maxCardinality rdf:datatype="&xsd;integer">1</nrl:maxCardinality>
  <rdfs:domain rdf:resource="&nmo;Message"/>
  <rdfs:range rdf:resource="&nco;ContactMedium"/>
</rdf:Property>

<rdf:Property rdf:about="&nao;description"
    rdfs:comment="A non-technical textual annotation for a resource"
    rdfs:label="description">
  <rdfs:subPropertyOf rdf:resource="&nao;annotation"/>
  <rdfs:subPropertyOf rdf:resource="&rdfs;comment"/>
  <rdfs:range rdf:resource="&rdfs;Literal"/>
</rdf:Property>

<rdf:Property rdf:about="&tmo;priority"
    nrl:maxCardinality="1"
    rdfs:label="priority">
  <rdfs:domain rdf:resource="&tmo;Task"/>
  <rdfs:range rdf:resource="&tmo;Priority"/>
  <rdfs:subPropertyOf rdf:resource="&tmo;timemanagement"/>
</rdf:Property>

<rdf:Property rdf:about="&ncal;attachmentUri"
    rdfs:label="attachmentUri">
  <nrl:maxCardinality rdf:datatype="&xsd;integer">1</nrl:maxCardinality>
  <rdfs:comment>The uri of the attachment. Created to express the actual value of the ATTACH property defined in RFC 2445 sec. 4.8.1.1. This property expresses the default URI datatype of that property. see ncal:attachmentContents for the BINARY datatype.</rdfs:comment>
  <rdfs:domain rdf:resource="&ncal;Attachment"/>
  <rdfs:range rdf:resource="&rdfs;Resource"/>
</rdf:Property>

<rdf:Property rdf:about="&nid3;time"
    rdfs:label="time">
  <rdfs:comment>TIME
The 'Time' frame is a numeric string in the HHMM format containing the time for the recording. This field is always four characters long.</rdfs:comment>
  <rdfs:domain rdf:resource="&nid3;ID3Audio"/>
  <rdfs:range rdf:resource="&xsd;string"/>
</rdf:Property>

<rdfs:Class rdf:about="&nrl;GraphView"
    rdfs:label="GraphView">
  <rdfs:comment>Identifies a graph which is itself a view of another named graph</rdfs:comment>
  <rdfs:subClassOf rdf:resource="&nrl;Graph"/>
</rdfs:Class>

<rdf:Property rdf:about="&tmo;subTask"
    rdfs:label="subTask">
  <nrl:inverseProperty rdf:resource="&tmo;superTask"/>
  <rdfs:domain rdf:resource="&tmo;Task"/>
  <rdfs:range rdf:resource="&tmo;Task"/>
  <rdfs:subPropertyOf rdf:resource="&pimo;hasPart"/>
</rdf:Property>

<rdf:Property rdf:about="&pimo;taskDueTime"
    nrl:maxCardinality="1"
    rdfs:label="task due time">
  <rdfs:comment>when is this task due? Represented in ISO 8601, example: 2003-11-22T17:00:00</rdfs:comment>
  <rdfs:domain rdf:resource="&pimo;Task"/>
  <rdfs:range rdf:resource="&xsd;dateTime"/>
  <rdfs:subPropertyOf rdf:resource="&pimo;datatypeProperty"/>
</rdf:Property>

<rdfs:Class rdf:about="&dpo;EnvironmentalIndicator"
    rdfs:label="Environmental Indicator">
  <rdfs:comment>Quantifiable presence components concerning the environment surrounding the agent are grouped under this abstract class. </rdfs:comment>
  <rdfs:subClassOf rdf:resource="&dpo;QuantifiableComponent"/>
</rdfs:Class>

<rdf:Property rdf:about="&nid3;mediaType"
    rdfs:label="mediaType">
  <rdfs:comment>TMED
The 'Media type' frame describes from which media the sound originated. This may be a text string or a reference to the predefined media types found in the list below. References are made within "(" and ")" and are optionally followed by a text refinement, e.g. "(MC) with four channels". If a text refinement should begin with a "(" character it should be replaced with "((" in the same way as in the "TCO" frame. Predefined refinements is appended after the media type, e.g. "(CD/A)" or "(VID/PAL/VHS)".
See http://www.id3.org/id3v2.3.0 for details.</rdfs:comment>
  <rdfs:domain rdf:resource="&nid3;ID3Audio"/>
  <rdfs:range rdf:resource="&xsd;string"/>
</rdf:Property>

<rdf:Property rdf:about="&tmo;taskId"
    nrl:maxCardinality="1"
    nrl:minCardinality="1"
    rdfs:label="taskId">
  <rdfs:comment>The Task Identifier allows a unique identification of a task object within the range of all Nepomuk objects.
The Task Identifier is automatically generated during the creation of a task. The generation of identifiers (IDs) is a Nepomuk architecture issue (Wp2000/WP6000).</rdfs:comment>
  <rdfs:domain rdf:resource="&tmo;Task"/>
  <rdfs:range rdf:resource="&rdfs;Literal"/>
</rdf:Property>

<rdf:Property rdf:about="&nao;hasSymbol"
    rdfs:label="has symbol">
  <rdfs:comment>Annotation for a resource in the form of a visual representation. Typically the symbol is a double-typed image file or a nao:FreeDesktopIcon.</rdfs:comment>
  <rdfs:domain rdf:resource="&rdfs;Resource"/>
  <rdfs:range rdf:resource="&nao;Symbol"/>
</rdf:Property>

<rdf:Property rdf:about="&nmm;trackNumber"
    rdfs:comment="Track number of the music in its album"
    rdfs:label="track number">
  <nrl:maxCardinality rdf:datatype="&xsd;integer">1</nrl:maxCardinality>
  <rdfs:domain rdf:resource="&nmm;MusicPiece"/>
  <rdfs:range rdf:resource="&xsd;integer"/>
</rdf:Property>

<rdf:Property rdf:about="&dpo;minCloudcover"
    rdfs:label="Minimum Cloud Cover">
  <rdfs:comment>A subproperty of dpo:minValue that defines a lowerbound on the observed cloud cover (as a percentage) such that it can classify as a dpo:WeatherCondition instance. It can be used in conjunction with dpo:maxCloudCover to state that specific instances of dpo:WeatherCondition have a pre-defined range of observable real-world cloud cover levels. In addition, they can also be used with various other weather conditions values and ranges to define complex weather condition types.</rdfs:comment>
  <rdfs:domain rdf:resource="&dpo;WeatherConditions"/>
  <rdfs:range rdf:resource="&xsd;nonNegativeInteger"/>
  <rdfs:subPropertyOf rdf:resource="&dpo;minValue"/>
</rdf:Property>

<rdfs:Class rdf:about="&tmo;TaskTransmission"
    rdfs:label="TaskTransmission">
  <rdfs:comment>On the SSD, tasks are not restricted to one person and may cross from
the PTM of one person to the PTM of another. With transmission, we
refer to the process of sending a task from one person (sender) to one
or more other persons (receiver(s)) (see Section 5.2.1.3 Task
Transmission). Task delegation and task transfer are two special kinds of
task transmission which are described at the end of this section. In
addition, the collaborative task is realized by task transmission.
For the process of sending a task, some information is required. This
information is also modelled in the task ontology. This information is still
useful after the process of sending a task was completed. Task Delegation is a process where the sender of the task restricts the
access rights of the receiver. This includes the right to distribute further
this task and additionally the obligation to give feedback to the sender.
The person that receives a task by delegation usually has not the full
control about the task. The attributes described in the following section
have the purpose to enable such "access rights". The receiver will also
probably have obligations regarding what to report to whom at which
time.
In contrast, the simplest case is that all rights are granted to the receiver
and there is no feedback desired by the sender. What to do with the task
may be apparent by the organization context, or it may be left to the
receiver. This is like sending an email but with the advantage that the
information is transferred in the "task space" of the participating persons.</rdfs:comment>
  <rdfs:subClassOf rdf:resource="&rdfs;Resource"/>
</rdfs:Class>

<rdf:Property rdf:about="&pimo;creator"
    nrl:maxCardinality="1"
    nrl:minCardinality="1"
    rdfs:label="creator">
  <nrl:inverseProperty rdf:resource="&pimo;createdPimo"/>
  <rdfs:comment>The creator of the Personal Information Model. A subproperty of NAO:creator. The human being whose mental models are represented in the PIMO. Range is an Agent.</rdfs:comment>
  <rdfs:domain rdf:resource="&pimo;PersonalInformationModel"/>
  <rdfs:range rdf:resource="&pimo;Agent"/>
  <rdfs:subPropertyOf rdf:resource="&nao;creator"/>
</rdf:Property>

<rdfs:Class rdf:about="&dplo;Checkin"
    rdfs:label="Checkin Post">
  <rdfs:comment>Represents the live posting of information related to a user's detected or proclaimed physical location, as defined by an established instance of pimo:Location.</rdfs:comment>
  <rdfs:subClassOf rdf:resource="&dplo;PresencePost"/>
</rdfs:Class>

<rdf:Property rdf:about="&nmm;musicBrainzTrackID"
    rdfs:comment="MusicBrainz track ID"
    rdfs:label="musicbrainz track ID">
  <nrl:maxCardinality rdf:datatype="&xsd;integer">1</nrl:maxCardinality>
  <rdfs:domain rdf:resource="&nmm;MusicPiece"/>
  <rdfs:range rdf:resource="&xsd;integer"/>
  <rdfs:subPropertyOf rdf:resource="&nie;identifier"/>
</rdf:Property>

<rdf:Property rdf:about="&scos;scopeNote">
  <rdf:type rdf:resource="&owl;AnnotationProperty"/>
  <rdfs:isDefinedBy rdf:resource="http://www.w3.org/2004/02/skos/core"/>
  <rdfs:label xml:lang="en">scope note</rdfs:label>
  <rdfs:subPropertyOf rdf:resource="&scos;note"/>
  <scos:definition xml:lang="en">A note that helps to clarify the meaning and/or the use of a concept.</scos:definition>
</rdf:Property>

<tmo:TransmissionState rdf:about="&tmo;TMO_Instance_TransmissionState_Accepted_NotTransmitted"
    rdfs:label="TMO_Instance_TransmissionState_Accepted_NotTransmitted"/>

<tmo:PersonInvolvementRole rdf:about="&tmo;TMO_Instance_PersonInvolvementRole_Creator"
    rdfs:label="TMO_Instance_PersonInvolvementRole_Creator"/>

<rdf:Property rdf:about="&nrl;cardinality"
    rdfs:label="cardinality">
  <rdfs:comment>Specifies the precise value cardinality for a specific property</rdfs:comment>
  <rdfs:domain rdf:resource="&rdf;Property"/>
  <rdfs:range rdf:resource="&rdfs;Literal"/>
</rdf:Property>

<rdf:Property rdf:about="&dcterms;coverage">
  <dcterms:description xml:lang="en">Spatial topic and spatial applicability may be a named place or a location specified by its geographic coordinates. Temporal topic may be a named period, date, or date range. A jurisdiction may be a named administrative entity or a geographic place to which the resource applies. Recommended best practice is to use a controlled vocabulary such as the Thesaurus of Geographic Names [TGN]. Where appropriate, named places or time periods can be used in preference to numeric identifiers such as sets of coordinates or date ranges.</dcterms:description>
  <dcterms:hasVersion rdf:resource="http://dublincore.org/usage/terms/history/#coverageT-001"/>
  <dcterms:issued rdf:datatype="&xsd;date">2008-01-14</dcterms:issued>
  <dcterms:modified rdf:datatype="&xsd;date">2008-01-14</dcterms:modified>
  <rdfs:comment xml:lang="en">The spatial or temporal topic of the resource, the spatial applicability of the resource, or the jurisdiction under which the resource is relevant.</rdfs:comment>
  <rdfs:isDefinedBy rdf:resource="&dcterms;"/>
  <rdfs:label xml:lang="en">Coverage</rdfs:label>
  <rdfs:range rdf:resource="&dcterms;LocationPeriodOrJurisdiction"/>
  <rdfs:subPropertyOf rdf:resource="&dc;coverage"/>
</rdf:Property>

<rdf:Property rdf:about="&nid3;language"
    rdfs:label="language">
  <nao:deprecated rdf:datatype="&xsd;boolean">true</nao:deprecated>
  <rdfs:comment>TLAN
The 'Language(s)' frame should contain the languages of the text or lyrics spoken or sung in the audio. The language is represented with three characters according to ISO-639-2. If more than one language is used in the text their language codes should follow according to their usage. Deprecated in favor of the more generic nie:language.</rdfs:comment>
  <rdfs:domain rdf:resource="&nid3;ID3Audio"/>
  <rdfs:range rdf:resource="&xsd;string"/>
  <rdfs:subPropertyOf rdf:resource="&nie;language"/>
</rdf:Property>

<rdf:Property rdf:about="&nfo;frontChannels"
    rdfs:comment="Number of front channels."
    rdfs:label="frontChannels">
  <nrl:maxCardinality rdf:datatype="&xsd;integer">1</nrl:maxCardinality>
  <rdfs:range rdf:resource="&xsd;integer"/>
  <rdfs:subPropertyOf rdf:resource="&nfo;channels"/>
</rdf:Property>

<rdf:Property rdf:about="&nfo;belongsToContainer"
    rdfs:label="belongsToContainer">
  <rdfs:comment>Models the containment relations between Files and Folders (or CompressedFiles).</rdfs:comment>
  <rdfs:domain rdf:resource="&nie;DataObject"/>
  <rdfs:range rdf:resource="&nfo;DataContainer"/>
  <rdfs:subPropertyOf rdf:resource="&nie;isPartOf"/>
</rdf:Property>

<rdfs:Class rdf:about="&tmo;PredecessorDependency"
    rdfs:label="PredecessorDependency">
  <rdfs:comment>In a  PredecessorDependency the dependencyMemberA is the task which is to be executed before dependencyMemberB.</rdfs:comment>
  <rdfs:subClassOf rdf:resource="&tmo;PredecessorSuccessorDependency"/>
</rdfs:Class>

<rdf:Property rdf:about="&nexif;dateTimeDigitized"
    rdfs:label="dateTimeDigitized">
  <rdfs:subPropertyOf rdf:resource="http://www.kanzaki.com/ns/exif#dateTimeDigitized"/>
  <rdfs:subPropertyOf rdf:resource="&nexif;date"/>
  <rdfs:subPropertyOf rdf:resource="&nexif;dateAndOrTime"/>
  <rdfs:comment>The date and time when the image was stored as digital data. If, for example, an image was captured by DSC and at the same time the file was recorded, then the DateTimeOriginal and DateTimeDigitized will have the same contents.
tagNumber: 36868</rdfs:comment>
  <rdfs:domain rdf:resource="&nexif;Photo"/>
  <rdfs:range rdf:resource="&xsd;dateTime"/>
</rdf:Property>

<tmo:Delegability rdf:about="&tmo;TMO_Instance_Delegability_High"
    rdfs:label="TMO_Instance_Delegability_High"/>

<rdf:Property rdf:about="&nexif;yResolution"
    rdfs:label="yResolution">
  <rdfs:subPropertyOf rdf:resource="http://www.kanzaki.com/ns/exif#yResolution"/>
  <rdfs:subPropertyOf rdf:resource="&nexif;imageDataStruct"/>
  <rdfs:subPropertyOf rdf:resource="&nexif;resolution"/>
  <rdfs:comment>tagNumber: 283
The number of pixels per ResolutionUnit in the ImageLength direction. The same value as XResolution is designated.</rdfs:comment>
  <rdfs:domain rdf:resource="&nexif;Photo"/>
  <rdfs:range rdf:resource="&xsd;float"/>
</rdf:Property>

<rdfs:Class rdf:about="&nfo;FilesystemImage"
    rdfs:label="FilesystemImage">
  <nao:deprecated rdf:datatype="&xsd;boolean">true</nao:deprecated>
  <rdfs:comment>An image of a filesystem. Instances of this class may include CD images, DVD images or hard disk partition images created by various pieces of software (e.g. Norton Ghost). Deprecated in favor of nfo:Filesystem.</rdfs:comment>
  <rdfs:subClassOf rdf:resource="&nfo;Filesystem"/>
</rdfs:Class>

<rdfs:Class rdf:about="&nfo;Visual"
    rdfs:comment="File containing visual content."
    rdfs:label="Visual">
  <rdfs:subClassOf rdf:resource="&nfo;Media"/>
</rdfs:Class>

<rdfs:Class rdf:about="&nmm;Movie"
    rdfs:comment="A Movie"
    rdfs:label="movie">
  <rdfs:subClassOf rdf:resource="&nfo;Video"/>
</rdfs:Class>

<rdf:Property rdf:about="&nexif;brightnessValue"
    rdfs:label="brightnessValue">
  <rdfs:subPropertyOf rdf:resource="http://www.kanzaki.com/ns/exif#brightnessValue"/>
  <rdfs:subPropertyOf rdf:resource="&nexif;pictTaking"/>
  <rdfs:comment>tagNumber: 37379
The value of brightness. The unit is the APEX value. Ordinarily it is given in the range of -99.99 to 99.99. Note that if the numerator of the recorded value is FFFFFFFF.H, Unknown shall be indicated.</rdfs:comment>
  <rdfs:domain rdf:resource="&nexif;Photo"/>
  <rdfs:range rdf:resource="&xsd;float"/>
</rdf:Property>

<rdf:Property rdf:about="&ncal;uid"
    rdfs:label="uid">
  <nrl:maxCardinality rdf:datatype="&xsd;integer">1</nrl:maxCardinality>
  <rdfs:comment>This property defines the persistent, globally unique identifier for the calendar component. Inspired by the RFC 2445 sec 4.8.4.7</rdfs:comment>
  <rdfs:domain rdf:resource="&ncal;UnionOfEventFreebusyJournalTodo"/>
  <rdfs:range rdf:resource="&xsd;string"/>
  <rdfs:subPropertyOf rdf:resource="&nie;identifier"/>
</rdf:Property>

<rdf:Property rdf:about="&foaf;skypeID"
    rdfs:comment="A Skype ID"
    rdfs:label="Skype ID"
    ns:term_status="testing">
  <rdf:type rdf:resource="&owl;DatatypeProperty"/>
  <rdfs:domain rdf:resource="&foaf;Agent"/>
  <rdfs:isDefinedBy rdf:resource="&foaf;"/>
  <rdfs:range rdf:resource="&rdfs;Literal"/>
  <rdfs:subPropertyOf rdf:resource="&foaf;nick"/>
</rdf:Property>

<rdf:Property rdf:about="&nexif;exifIFDPointer"
    rdfs:label="exifIFDPointer">
  <rdfs:subPropertyOf rdf:resource="http://www.kanzaki.com/ns/exif#exif_IFD_Pointer"/>
  <rdfs:subPropertyOf rdf:resource="&nexif;ifdPointer"/>
  <rdfs:comment>tagNumber: 34665
A pointer to the Exif IFD, which is a set of tags for recording Exif-specific attribute information.</rdfs:comment>
  <rdfs:domain rdf:resource="&nexif;Photo"/>
  <rdfs:range rdf:resource="&nexif;Photo"/>
</rdf:Property>

<rdf:Property rdf:about="&scos;narrowerTransitive">
  <rdf:type rdf:resource="&owl;ObjectProperty"/>
  <rdf:type rdf:resource="&owl;TransitiveProperty"/>
  <rdfs:isDefinedBy rdf:resource="http://www.w3.org/2004/02/skos/core"/>
  <rdfs:label xml:lang="en">has narrower transitive</rdfs:label>
  <rdfs:subPropertyOf rdf:resource="&scos;semanticRelation"/>
  <owl:inverseOf rdf:resource="&scos;broaderTransitive"/>
  <scos:definition>skos:narrowerTransitive is a transitive superproperty of skos:narrower.</scos:definition>
  <scos:scopeNote xml:lang="en">By convention, skos:narrowerTransitive is not used to make assertions. Rather, the properties can be used to draw inferences about the transitive closure of the hierarchical relation, which is useful e.g. when implementing a simple query expansion algorithm in a search application.</scos:scopeNote>
</rdf:Property>

<rdf:Property rdf:about="&tmo;sendDateTime"
    nrl:maxCardinality="1"
    rdfs:label="sendDateTime">
  <rdfs:domain rdf:resource="&tmo;TaskTransmission"/>
  <rdfs:range rdf:resource="&xsd;dateTime"/>
  <rdfs:subPropertyOf rdf:resource="&tmo;dateTime"/>
</rdf:Property>

<nrl:DefiningProperty rdf:about="&nmm;writer"
    rdfs:comment="Writer"
    rdfs:label="writer">
  <rdf:type rdf:resource="&rdf;Property"/>
  <rdfs:domain rdf:resource="&nfo;Video"/>
  <rdfs:range rdf:resource="&nco;Contact"/>
  <rdfs:subPropertyOf rdf:resource="&nco;contributor"/>
</nrl:DefiningProperty>

<owl:ObjectProperty rdf:about="&oa;motivatedBy">
  <rdfs:comment xml:lang="en">The relationship between an Annotation and a Motivation, indicating the reasons why the Annotation was created.

Each Annotation SHOULD have at least one oa:motivatedBy relationship, and MAY be more than 1.</rdfs:comment>
  <rdfs:domain rdf:resource="&oa;Annotation"/>
  <rdfs:isDefinedBy rdf:resource="&oa;"/>
  <rdfs:label xml:lang="en">motivatedBy</rdfs:label>
  <rdfs:range rdf:resource="&oa;Motivation"/>
</owl:ObjectProperty>

<tmo:PersonInvolvementRole rdf:about="&tmo;TMO_Instance_PersonInvolvementRole_Suggested"
    rdfs:label="TMO_Instance_PersonInvolvementRole_Suggested"/>

<rdfs:Class rdf:about="&ncal;NcalTimeEntity"
    rdfs:label="NcalTimeEntity">
  <rdfs:comment>A time entity. Conceived as a common superclass for NcalDateTime and NcalPeriod. According to RFC 2445 both DateTime and Period can be interpreted in different timezones. The first case is explored in many properties. The second case is theoretically possible in ncal:rdate property. Therefore the timezone properties have been defined at this level.</rdfs:comment>
  <rdfs:subClassOf rdf:resource="&rdfs;Resource"/>
</rdfs:Class>

<rdf:Property rdf:about="&nie;title"
    nrl:maxCardinality="1"
    rdfs:comment="Name given to an InformationElement"
    rdfs:label="title">
  <rdfs:subPropertyOf rdf:resource="&dc;title"/>
  <rdfs:subPropertyOf rdf:resource="&nao;prefLabel"/>
  <rdfs:domain rdf:resource="&nie;InformationElement"/>
  <rdfs:range rdf:resource="&xsd;string"/>
</rdf:Property>

<rdf:Property rdf:about="&pimo;dtstart"
    nrl:maxCardinality="1"
    rdfs:label="start date">
  <rdfs:comment>This property specifies when the process begins. Inspired by NCAL:dtstart.</rdfs:comment>
  <rdfs:domain rdf:resource="&pimo;ProcessConcept"/>
  <rdfs:range rdf:resource="&xsd;dateTime"/>
  <rdfs:subPropertyOf rdf:resource="&pimo;datatypeProperty"/>
</rdf:Property>

<rdf:Property rdf:about="&nco;nameHonorificPrefix"
    rdfs:label="nameHonorificPrefix">
  <rdfs:comment>A prefix for the name of the object represented by this Contact. See documentation for the 'nameFamily' property for details.</rdfs:comment>
  <rdfs:domain rdf:resource="&nco;PersonName"/>
  <rdfs:range rdf:resource="&xsd;string"/>
</rdf:Property>

<rdf:Property rdf:about="&tmo;logEntry"
    rdfs:label="logEntry">
  <rdfs:domain rdf:resource="&tmo;Task"/>
  <rdfs:range rdf:resource="&rdfs;Resource"/>
</rdf:Property>

<rdf:Property rdf:about="&tmo;taskDescription"
    nrl:maxCardinality="1"
    rdfs:label="taskDescription">
  <rdfs:comment>The task description helps users to understand the goal and the proceeding of a task. It can also describe the context of a task. The task description is composed at minimum of a summary of what is done to reach the goal. The task description is the main source for identifying related information, e.g., suitable patterns.
A Task Description can be either an informal, described textual content (TextualDescription) or it can be a more formally structured representation (FormalDescription).
Technology considerations: Informal descriptions allow for text similarity processing, a formal description allows for applying case based similarity measures.</rdfs:comment>
  <rdfs:domain rdf:resource="&tmo;Task"/>
  <rdfs:subPropertyOf rdf:resource="&nao;description"/>
</rdf:Property>

<owl:NamedIndividual rdf:about="&oa;bookmarking">
  <rdf:type rdf:resource="&oa;Motivation"/>
  <rdfs:comment xml:lang="en">The motivation that represents the creation of a bookmark to the target resources or recorded point or points within one or more resources. For example, an Annotation that bookmarks the point in a text where the reader finished reading. Bookmark Annotations may or may not have a Body resource.</rdfs:comment>
  <scos:inScheme rdf:resource="&oa;motivationScheme"/>
  <scos:prefLabel xml:lang="en">bookmarking</scos:prefLabel>
</owl:NamedIndividual>

<rdf:Property rdf:about="&nao;status"
    rdfs:label="status">
  <nrl:maxCardinality rdf:datatype="&xsd;nonNegativeInteger">1</nrl:maxCardinality>
  <rdfs:comment>Specifies the status of a graph, stable, unstable or testing</rdfs:comment>
  <rdfs:domain rdf:resource="&nrl;Data"/>
  <rdfs:range rdf:resource="&rdfs;Literal"/>
  <rdfs:subPropertyOf rdf:resource="&nao;annotation"/>
</rdf:Property>

<rdf:Property rdf:about="&dplo;relatedResource"
    rdfs:label="has related resource">
  <rdfs:comment>This property (a sub-property of nao:isRelated) is used to refer to resources that are related to the livepost, as opposed to being the resource being shared (refer to dlpo:definingResource). Typical uses for this property is to represent items (e.g. people) tagged to a livepost.</rdfs:comment>
  <rdfs:domain rdf:resource="&dplo;LivePost"/>
  <rdfs:range rdf:resource="&rdfs;Resource"/>
  <rdfs:subPropertyOf rdf:resource="&nao;isRelated"/>
</rdf:Property>

<rdf:Property rdf:about="&dcon;upcomingEvent"
    rdfs:label="Upcoming Event">
  <rdfs:comment>Refers to an upcoming event characterising a context instance.</rdfs:comment>
  <rdfs:domain rdf:resource="&dcon;Schedule"/>
  <rdfs:range rdf:resource="&ncal;Event"/>
  <rdfs:subPropertyOf rdf:resource="&dcon;hasContextElement"/>
</rdf:Property>

<rdfs:Class rdf:about="&tmo;TaskState"
    rdfs:label="TaskState">
  <rdfs:comment>The task state property allows tracking a task during its lifecycle. Initially the state is just "created". 
The TaskState class was modeled so that for each state can be set which the typical prior and posterior states are. This has the advantage that e.g. a UI can retrieve the allowed states at runtime from the ontology; rather can having this potentially changing knowledge hard coded. But the prior and posterior states are only defaults; the human user is always free to change the state.</rdfs:comment>
  <rdfs:subClassOf rdf:resource="&tmo;StateTypeRole"/>
</rdfs:Class>

<rdf:Property rdf:about="&tmo;superTask"
    nrl:maxCardinality="1"
    rdfs:label="superTask">
  <rdfs:subPropertyOf rdf:resource="&pimo;partOf"/>
  <rdfs:subPropertyOf rdf:resource="&tmo;taskReference"/>
  <nrl:inverseProperty rdf:resource="&tmo;subTask"/>
  <rdfs:domain rdf:resource="&tmo;Task"/>
  <rdfs:range rdf:resource="&tmo;Task"/>
</rdf:Property>

<rdf:Property rdf:about="&nexif;makerNote"
    rdfs:comment="Manufacturer notes
tagNumber: 37500"
    rdfs:label="makerNote">
  <rdfs:subPropertyOf rdf:resource="http://www.kanzaki.com/ns/exif#makerNote"/>
  <rdfs:subPropertyOf rdf:resource="&nexif;userInfo"/>
  <rdfs:domain rdf:resource="&nexif;Photo"/>
  <rdfs:range rdf:resource="&xsd;string"/>
</rdf:Property>

<rdf:Property rdf:about="&cnt;rest">
  <rdf:type rdf:resource="&owl;ObjectProperty"/>
  <rdfs:comment xml:lang="en">The XML content following the document type declaration.</rdfs:comment>
  <rdfs:domain rdf:resource="&cnt;ContentAsXML"/>
  <rdfs:label xml:lang="en">XML rest</rdfs:label>
  <rdfs:range rdf:resource="&rdfs;XMLLiteral"/>
</rdf:Property>

<rdfs:Class rdf:about="&ncal;UnionOfTimezoneObservanceEventJournalTimezoneTodo"
    rdfs:label="UnionOfTimezoneObservanceEventJournalTimezoneTodo">
  <rdfs:subClassOf rdf:resource="&ncal;UnionParentClass"/>
</rdfs:Class>

<nfo:CompressionType rdf:about="&nfo;losslessCompressionType"
    rdfs:label="losslessCompressionType"/>

<rdf:Property rdf:about="&pimo;occurrence"
    rdfs:label="occurrence">
  <rdfs:comment>The subject Thing is represented also in the object resource. All facts added to the object resource are valid for the subject thing. The subject is the canonical represtation of the object. In particual, this implies when (?object ?p ?v) -&gt; (?subject ?p ?v) and (?s ?p ?object) -&gt; (?s ?p ?subject). The class of the object is not defined, but should be compatible with the class of the subject. Occurrence relations can be inferred through same identifiers or referencingOccurrence relations.</rdfs:comment>
  <rdfs:domain rdf:resource="&pimo;Thing"/>
  <rdfs:range rdf:resource="&rdfs;Resource"/>
</rdf:Property>

<rdfs:Class rdf:about="&dpo;Temperature"
    rdfs:label="Temperature">
  <rdfs:comment>Quantifiable presence components concerning the detected temperature in the environment surrounding the agent.</rdfs:comment>
  <rdfs:subClassOf rdf:resource="&dpo;EnvironmentalIndicator"/>
</rdfs:Class>

<rdf:Property rdf:about="&foaf;gender"
    rdfs:label="gender"
    ns:term_status="testing">
  <rdf:type rdf:resource="&owl;DatatypeProperty"/>
  <rdf:type rdf:resource="&owl;FunctionalProperty"/>
  <rdfs:comment>The gender of this Agent (typically but not necessarily 'male' or 'female').</rdfs:comment>
  <rdfs:domain rdf:resource="&foaf;Agent"/>
  <rdfs:isDefinedBy rdf:resource="&foaf;"/>
  <rdfs:range rdf:resource="&rdfs;Literal"/>
</rdf:Property>

<rdf:Property rdf:about="&ncal;attendee"
    rdfs:label="attendee">
  <rdfs:comment>The property defines an "Attendee" within a calendar component. Inspired by RFC 2445 sec. 4.8.4.1. Originally this property accepted many parameters. The Attendee class has been introduced to express them all. Note that NCAL is aligned with NCO. The actual value (of the CAL-ADDRESS type) is expressed as an instance of nco:Contact. Remember that the CN parameter has been removed from NCAL. Instead that value should be expressed using nco:fullname property of the above mentioned nco:Contact instance. The RFC stated that whenever this property is attached to a Valarm instance, the Attendee cannot have any parameters apart from involvedContact.</rdfs:comment>
  <rdfs:domain rdf:resource="&ncal;UnionOfAlarmEventFreebusyJournalTodo"/>
  <rdfs:range rdf:resource="&ncal;Attendee"/>
</rdf:Property>

<rdfs:Class rdf:about="&dcterms;Policy">
  <dcterms:hasVersion rdf:resource="http://dublincore.org/usage/terms/history/#Policy-001"/>
  <dcterms:issued rdf:datatype="&xsd;date">2008-01-14</dcterms:issued>
  <rdfs:comment xml:lang="en">A plan or course of action by an authority, intended to influence and determine decisions, actions, and other matters.</rdfs:comment>
  <rdfs:isDefinedBy rdf:resource="&dcterms;"/>
  <rdfs:label xml:lang="en">Policy</rdfs:label>
</rdfs:Class>

<rdf:Property rdf:about="&nco;phoneNumber"
    nrl:maxCardinality="1"
    rdfs:label="phoneNumber">
  <rdfs:domain rdf:resource="&nco;PhoneNumber"/>
  <rdfs:range rdf:resource="&xsd;string"/>
</rdf:Property>

<owl:AnnotationProperty rdf:about="http://xmlns.com/wot/0.1/src_assurance"/>

<tmo:PersonInvolvementRole rdf:about="&tmo;TMO_Instance_PersonInvolvementRole_InternalObserver"
    rdfs:label="TMO_Instance_PersonInvolvementRole_InternalObserver"/>

<rdfs:Class rdf:about="&ncal;UnionParentClass"
    rdfs:label="UnionParentClass">
  <rdfs:subClassOf rdf:resource="&rdfs;Resource"/>
</rdfs:Class>

<owl:Class rdf:about="&oa;SpecificResource">
  <rdfs:comment xml:lang="en">A resource identifies part of another Source resource, a particular representation of a resource, a resource with styling hints for renders, or any combination of these. 

The Specific Resource takes the role of oa:hasBody or oa:hasTarget in an oa:Annotation instead of the Source resource.

There MUST be exactly 1 oa:hasSource relationship associated with a Specific Resource.

There MUST be exactly 0 or 1 oa:hasSelector relationship associated with a Specific Resource.

There MAY be 0 or 1 oa:hasState relationship for each Specific Resource.

If the Specific Resource has an HTTP URI, then the exact segment of the Source resource that it identifies, and only the segment, MUST be returned when the URI is dereferenced. For example, if the segment of interest is a region of an image and the Specific Resource has an HTTP URI, then dereferencing it MUST return the selected region of the image as it was at the time when the annotation was created. Typically this would be a burden to support, and thus the Specific Resource SHOULD be identified by a globally unique URI, such as a UUID URN. If it is not considered important to allow other Annotations or systems to refer to the Specific Resource, then a blank node MAY be used instead.</rdfs:comment>
  <rdfs:isDefinedBy rdf:resource="&oa;"/>
  <rdfs:label xml:lang="en">SpecificResource</rdfs:label>
</owl:Class>

<rdf:Property rdf:about="&dcterms;isVersionOf">
  <rdfs:subPropertyOf rdf:resource="&dc;relation"/>
  <rdfs:subPropertyOf rdf:resource="&dcterms;relation"/>
  <dcterms:description xml:lang="en">Changes in version imply substantive changes in content rather than differences in format.</dcterms:description>
  <dcterms:hasVersion rdf:resource="http://dublincore.org/usage/terms/history/#isVersionOf-003"/>
  <dcterms:issued rdf:datatype="&xsd;date">2000-07-11</dcterms:issued>
  <dcterms:modified rdf:datatype="&xsd;date">2008-01-14</dcterms:modified>
  <rdfs:comment xml:lang="en">A related resource of which the described resource is a version, edition, or adaptation.</rdfs:comment>
  <rdfs:isDefinedBy rdf:resource="&dcterms;"/>
  <rdfs:label xml:lang="en">Is Version Of</rdfs:label>
  <scos:note xml:lang="en">This term is intended to be used with non-literal values as defined in the DCMI Abstract Model (http://dublincore.org/documents/abstract-model/).  As of December 2007, the DCMI Usage Board is seeking a way to express this intention with a formal range declaration.</scos:note>
</rdf:Property>

<tmo:TaskState rdf:about="&tmo;TMO_Instance_TaskState_Completed"
    rdfs:label="TMO_Instance_TaskState_Completed"/>

<rdfs:Class rdf:about="&nrl;Graph"
    rdfs:comment="Represents a named graph"
    rdfs:label="Graph">
  <rdfs:subClassOf rdf:resource="http://www.w3.org/2004/03/trix/rdfg-1#Graph"/>
</rdfs:Class>

<rdfs:Class rdf:about="&dcterms;RightsStatement">
  <dcterms:hasVersion rdf:resource="http://dublincore.org/usage/terms/history/#RightsStatement-001"/>
  <dcterms:issued rdf:datatype="&xsd;date">2008-01-14</dcterms:issued>
  <rdfs:comment xml:lang="en">A statement about the intellectual property rights (IPR) held in or over a Resource, a legal document giving official permission to do something with a resource, or a statement about access rights.</rdfs:comment>
  <rdfs:isDefinedBy rdf:resource="&dcterms;"/>
  <rdfs:label xml:lang="en">Rights Statement</rdfs:label>
</rdfs:Class>

<rdf:Property rdf:about="&dcterms;modified">
  <rdfs:subPropertyOf rdf:resource="&dc;date"/>
  <rdfs:subPropertyOf rdf:resource="&dcterms;date"/>
  <dcterms:hasVersion rdf:resource="http://dublincore.org/usage/terms/history/#modified-003"/>
  <dcterms:issued rdf:datatype="&xsd;date">2000-07-11</dcterms:issued>
  <dcterms:modified rdf:datatype="&xsd;date">2008-01-14</dcterms:modified>
  <rdfs:comment xml:lang="en">Date on which the resource was changed.</rdfs:comment>
  <rdfs:isDefinedBy rdf:resource="&dcterms;"/>
  <rdfs:label xml:lang="en">Date Modified</rdfs:label>
  <rdfs:range rdf:resource="&rdfs;Literal"/>
</rdf:Property>

<ncal:CalendarUserType rdf:about="&ncal;resourceUserType"
    rdfs:label="resourceUserType"/>

<rdfs:Class rdf:about="&nco;CellPhoneNumber"
    rdfs:label="CellPhoneNumber">
  <rdfs:subClassOf rdf:resource="&nco;MessagingNumber"/>
  <rdfs:subClassOf rdf:resource="&nco;VoicePhoneNumber"/>
  <rdfs:comment>A cellular phone number. Inspired by the (TYPE=cell) parameter of the TEL property as defined in RFC 2426 sec  3.3.1. Usually a cellular phone can accept voice calls as well as textual messages (SMS), therefore this class has two superclasses.</rdfs:comment>
</rdfs:Class>

<rdf:Property rdf:about="&ncal;byminute"
    rdfs:comment="Minute of recurrence. Defined in RFC 2445 sec. 4.3.10"
    rdfs:label="byminute">
  <rdfs:domain rdf:resource="&ncal;RecurrenceRule"/>
  <rdfs:range rdf:resource="&xsd;integer"/>
</rdf:Property>

<rdf:Property rdf:about="&nrl;superGraphOf"
    rdfs:label="superGraphOf">
  <nrl:inverseProperty rdf:resource="&nrl;subGraphOf"/>
  <rdfs:comment>Specifies a subsumption relationship between two graphs, meaning that the object graph is included in the subject graph</rdfs:comment>
  <rdfs:domain rdf:resource="&nrl;Graph"/>
  <rdfs:range rdf:resource="&nrl;Graph"/>
</rdf:Property>

<rdf:Property rdf:about="&ddo;deviceName"
    rdfs:comment="Represents a person-defined name for a device."
    rdfs:label="deviceName">
  <rdfs:domain rdf:resource="&ddo;Device"/>
  <rdfs:range rdf:resource="&xsd;string"/>
  <rdfs:subPropertyOf rdf:resource="&nao;personalIdentifier"/>
</rdf:Property>

<owl:Ontology rdf:about="&foaf;"
    dc:title="Friend of a Friend (FOAF) vocabulary">
  <dc:description>The Friend of a Friend (FOAF) RDF vocabulary, described using W3C RDF Schema and the Web Ontology Language.</dc:description>
</owl:Ontology>

<nrl:TransitiveProperty rdf:about="&pimo;subTopic"
    rdfs:label="sub topic">
  <rdfs:subPropertyOf rdf:resource="&pimo;hasPart"/>
  <rdfs:subPropertyOf rdf:resource="&pimo;objectProperty"/>
  <nrl:inverseProperty rdf:resource="&pimo;superTopic"/>
  <rdf:type rdf:resource="&rdf;Property"/>
  <rdfs:comment>The object topic is more specific in meaning than the subject topic. Transitive. Similar in meaning to skos:narrower</rdfs:comment>
  <rdfs:domain rdf:resource="&pimo;Topic"/>
  <rdfs:range rdf:resource="&pimo;Topic"/>
</nrl:TransitiveProperty>

<rdf:Property rdf:about="&dpo;maxWeek"
    rdfs:label="Maximum Week">
  <rdfs:comment>A subproperty of dpo:maxValue that defines an upperbound on the observed week of the year (i.e., between 1 and 52) such that it can classify as a dpo:TimePeriod instance. It can be used in conjunction with dpo:minWeek, i.e. specific instances of dpo:TimePeriod have a pre-defined observable week number-based period.</rdfs:comment>
  <rdfs:domain rdf:resource="&dpo;TimePeriod"/>
  <rdfs:range rdf:resource="&xsd;integer"/>
  <rdfs:subPropertyOf rdf:resource="&dpo;maxValue"/>
</rdf:Property>

<tmo:TaskState rdf:about="&tmo;TMO_Instance_TaskState_Terminated"
    rdfs:label="TMO_Instance_TaskState_Terminated"/>

<rdf:Property rdf:about="&ncal;requestStatus"
    rdfs:label="requestStatus">
  <nrl:maxCardinality rdf:datatype="&xsd;integer">1</nrl:maxCardinality>
  <rdfs:comment>This property defines the status code returned for a scheduling request. Inspired by RFC 2445 sec. 4.8.8.2. Original value of this property was a four-element structure. The RequestStatus class has been introduced to express it. In RFC 2445 this property could have the LANGUAGE parameter. This has been discarded in this ontology. Use xml:lang literals to express it if necessary.</rdfs:comment>
  <rdfs:domain rdf:resource="&ncal;UnionOfEventFreebusyJournalTodo"/>
  <rdfs:range rdf:resource="&ncal;RequestStatus"/>
</rdf:Property>

<owl:ObjectProperty rdf:about="&oa;hasSource">
  <rdfs:comment xml:lang="en">The relationship between a oa:SpecificResource and the resource that it is a more specific representation of. 

There MUST be exactly 1 oa:hasSource relationship associated with a Specific Resource.</rdfs:comment>
  <rdfs:domain rdf:resource="&oa;SpecificResource"/>
  <rdfs:isDefinedBy rdf:resource="&oa;"/>
  <rdfs:label xml:lang="en">hasSource</rdfs:label>
</owl:ObjectProperty>

<rdf:Property rdf:about="&nfo;fileLastAccessed"
    rdfs:comment="Time when the file was last accessed."
    rdfs:label="fileLastAccessed">
  <nrl:maxCardinality rdf:datatype="&xsd;integer">1</nrl:maxCardinality>
  <rdfs:domain rdf:resource="&nfo;FileDataObject"/>
  <rdfs:range rdf:resource="&xsd;dateTime"/>
  <rdfs:subPropertyOf rdf:resource="&dc;date"/>
</rdf:Property>

<tmo:Urgency rdf:about="&tmo;TMO_Instance_Urgency_10"
    rdfs:label="TMO_Instance_Urgency_10"/>

<rdf:Property rdf:about="&nfo;hasMediaStream"
    rdfs:label="hasMediaStream">
  <rdfs:comment>Connects a media container with a single media stream contained within.</rdfs:comment>
  <rdfs:domain rdf:resource="&nfo;Media"/>
  <rdfs:range rdf:resource="&nie;DataObject"/>
  <rdfs:subPropertyOf rdf:resource="&nie;hasPart"/>
</rdf:Property>

<rdfs:Class rdf:about="&dctypes;Dataset">
  <dcam:memberOf rdf:resource="&dcterms;DCMIType"/>
  <dcterms:description xml:lang="en">Examples include lists, tables, and databases.  A dataset may be useful for direct machine processing.</dcterms:description>
  <dcterms:hasVersion rdf:resource="http://dublincore.org/usage/terms/history/#Dataset-003"/>
  <dcterms:issued rdf:datatype="&xsd;date">2000-07-11</dcterms:issued>
  <dcterms:modified rdf:datatype="&xsd;date">2008-01-14</dcterms:modified>
  <rdfs:comment xml:lang="en">Data encoded in a defined structure.</rdfs:comment>
  <rdfs:isDefinedBy rdf:resource="&dctypes;"/>
  <rdfs:label xml:lang="en">Dataset</rdfs:label>
</rdfs:Class>

<rdf:Property rdf:about="&dcon;averageSpeed"
    rdfs:label="Average Speed">
  <rdfs:comment>Refers to a pre-defined speed range characterising a context instance.</rdfs:comment>
  <rdfs:domain rdf:resource="&dcon;SpaTem"/>
  <rdfs:range rdf:resource="&dpo;Movement"/>
  <rdfs:subPropertyOf rdf:resource="&dcon;hasContextElement"/>
</rdf:Property>

<rdf:Property rdf:about="&rdf;rest">
  <rdfs:comment xml:lang="en">The rest of the subject RDF list after the first item.</rdfs:comment>
  <rdfs:domain rdf:resource="&rdf;List"/>
  <rdfs:isDefinedBy rdf:resource="&rdf;"/>
  <rdfs:label xml:lang="en">rest</rdfs:label>
  <rdfs:range rdf:resource="&rdf;List"/>
</rdf:Property>

<rdfs:Class rdf:about="&tmo;AbilityCarrierRole"
    rdfs:label="AbilityCarrierRole">
  <rdfs:comment>Examples instances  of AbilityCarrirRoles are e.g. "requested", "required" and "used" which further specify the type a person was involved in.</rdfs:comment>
  <rdfs:subClassOf rdf:resource="&tmo;StateTypeRole"/>
</rdfs:Class>

<rdf:Property rdf:about="&nmm;synopsis"
    rdfs:label="synopsis">
  <nrl:maxCardinality rdf:datatype="&xsd;integer">1</nrl:maxCardinality>
  <rdfs:comment>Long form description of video content (plot, premise, etc.)</rdfs:comment>
  <rdfs:domain rdf:resource="&nfo;Video"/>
  <rdfs:range rdf:resource="&xsd;string"/>
  <rdfs:subPropertyOf rdf:resource="&nie;description"/>
</rdf:Property>

<rdf:Property rdf:about="&nexif;flash"
    rdfs:label="flash">
  <rdfs:subPropertyOf rdf:resource="http://www.kanzaki.com/ns/exif#flash"/>
  <rdfs:subPropertyOf rdf:resource="&nexif;pictTaking"/>
  <rdfs:comment>tagNumber: 37385
The status of flash when the image was shot.</rdfs:comment>
  <rdfs:domain rdf:resource="&nexif;Photo"/>
  <rdfs:range rdf:resource="&xsd;string"/>
</rdf:Property>

<rdfs:Class rdf:about="&nfo;Archive"
    rdfs:label="Archive">
  <rdfs:comment>A compressed file. May contain other files or folder inside. </rdfs:comment>
  <rdfs:subClassOf rdf:resource="&nfo;DataContainer"/>
</rdfs:Class>

<rdf:Property rdf:about="&nmo;from"
    rdfs:comment="deprecated in favor of nmo:messageFrom"
    rdfs:label="from">
  <nao:deprecated rdf:datatype="&xsd;boolean">true</nao:deprecated>
  <rdfs:domain rdf:resource="&nmo;Message"/>
  <rdfs:range rdf:resource="&nco;Contact"/>
</rdf:Property>

<rdf:Property rdf:about="&nid3;unsynchronizedTextContentDescriptor"
    rdfs:label="unsynchronizedTextContentDescriptor">
  <rdfs:comment>The content descriptor of the unsynchronized text. Inspired by the Content Descriptor field of the USLT frame, defined in ID3 2.3.0 Spec sec. 4.9</rdfs:comment>
  <rdfs:domain rdf:resource="&nid3;ID3Audio"/>
  <rdfs:range rdf:resource="&xsd;string"/>
</rdf:Property>

<ncal:AccessClassification rdf:about="&ncal;confidentialClassification"
    rdfs:label="confidentialClassification"/>

<rdf:Property rdf:about="&nao;version"
    rdfs:comment="Specifies the version of a graph, in numeric format"
    rdfs:label="version">
  <nrl:maxCardinality rdf:datatype="&xsd;nonNegativeInteger">1</nrl:maxCardinality>
  <rdfs:domain rdf:resource="&nrl;Data"/>
  <rdfs:range rdf:resource="&xsd;float"/>
  <rdfs:subPropertyOf rdf:resource="&nao;annotation"/>
</rdf:Property>

<rdf:Property rdf:about="&dcterms;instructionalMethod">
  <dcterms:description xml:lang="en">Instructional Method will typically include ways of presenting instructional materials or conducting instructional activities, patterns of learner-to-learner and learner-to-instructor interactions, and mechanisms by which group and individual levels of learning are measured.  Instructional methods include all aspects of the instruction and learning processes from planning and implementation through evaluation and feedback.</dcterms:description>
  <dcterms:hasVersion rdf:resource="http://dublincore.org/usage/terms/history/#instructionalMethod-002"/>
  <dcterms:issued rdf:datatype="&xsd;date">2005-06-13</dcterms:issued>
  <dcterms:modified rdf:datatype="&xsd;date">2008-01-14</dcterms:modified>
  <rdfs:comment xml:lang="en">A process, used to engender knowledge, attitudes and skills, that the described resource is designed to support.</rdfs:comment>
  <rdfs:isDefinedBy rdf:resource="&dcterms;"/>
  <rdfs:label xml:lang="en">Instructional Method</rdfs:label>
  <rdfs:range rdf:resource="&dcterms;MethodOfInstruction"/>
</rdf:Property>

<rdfs:Class rdf:about="&ddo;WiFi"
    rdfs:label="WiFi">
  <rdfs:comment>A wireless local area network that allows computerised devices to exchange data wirelessly. Devices can connect to a wireless network via a wireless network access point. </rdfs:comment>
  <rdfs:subClassOf rdf:resource="&ddo;LocalAreaNetwork"/>
</rdfs:Class>

<ncal:TodoStatus rdf:about="&ncal;inProcessStatus"
    rdfs:label="inProcessStatus"/>

<rdfs:Class rdf:about="&nmm;MusicPiece"
    rdfs:label="music">
  <rdfs:comment>Used to assign music-specific properties such a BPM to video and audio</rdfs:comment>
  <rdfs:subClassOf rdf:resource="&nfo;Audio"/>
</rdfs:Class>

<rdf:Property rdf:about="&nexif;resolutionUnit"
    rdfs:label="resolutionUnit">
  <rdfs:subPropertyOf rdf:resource="http://www.kanzaki.com/ns/exif#resolutionUnit"/>
  <rdfs:subPropertyOf rdf:resource="&nexif;imageDataStruct"/>
  <rdfs:comment>tagNumber: 296
The unit for measuring XResolution and YResolution. The same unit is used for both XResolution and YResolution. If the image resolution in unknown, 2 (inches) is designated.</rdfs:comment>
  <rdfs:domain rdf:resource="&nexif;Photo"/>
  <rdfs:range rdf:resource="&xsd;string"/>
</rdf:Property>

<rdf:Property rdf:about="&ncal;relatedToSibling"
    rdfs:label="relatedToSibling">
  <rdfs:comment>The property is used to represent a relationship or reference between one calendar component and another. Inspired by RFC 2445 sec. 4.8.4.5. Originally this property had a RELTYPE parameter. It has been decided that it is more natural to introduce three different properties to express the values of that parameter. This property expresses the RELATED-TO property with RELTYPE=SIBLING parameter.</rdfs:comment>
  <rdfs:domain rdf:resource="&ncal;UnionOfEventJournalTodo"/>
  <rdfs:range rdf:resource="&xsd;string"/>
  <rdfs:subPropertyOf rdf:resource="&ncal;ncalRelation"/>
</rdf:Property>

<rdf:Property rdf:about="&scos;editorialNote">
  <rdf:type rdf:resource="&owl;AnnotationProperty"/>
  <rdfs:isDefinedBy rdf:resource="http://www.w3.org/2004/02/skos/core"/>
  <rdfs:label xml:lang="en">editorial note</rdfs:label>
  <rdfs:subPropertyOf rdf:resource="&scos;note"/>
  <scos:definition xml:lang="en">A note for an editor, translator or maintainer of the vocabulary.</scos:definition>
</rdf:Property>

<tmo:PersonInvolvementRole rdf:about="&tmo;TMO_Instance_PersonInvolvementRole_Owner"
    rdfs:label="TMO_Instance_PersonInvolvementRole_Owner"/>

<rdf:Property rdf:about="&foaf;yahooChatID"
    rdfs:comment="A Yahoo chat ID"
    rdfs:label="Yahoo chat ID"
    ns:term_status="testing">
  <rdf:type rdf:resource="&owl;DatatypeProperty"/>
  <rdf:type rdf:resource="&owl;InverseFunctionalProperty"/>
  <rdfs:domain rdf:resource="&foaf;Agent"/>
  <rdfs:isDefinedBy rdf:resource="&foaf;"/>
  <rdfs:range rdf:resource="&rdfs;Literal"/>
  <rdfs:subPropertyOf rdf:resource="&foaf;nick"/>
</rdf:Property>

<rdfs:Class rdf:about="&tmo;AssociationDependency"
    rdfs:label="AssociationDependency">
  <rdfs:subClassOf rdf:resource="&tmo;UndirectedDependency"/>
</rdfs:Class>

<rdfs:Class rdf:about="&pimo;SocialEvent"
    rdfs:label="Social Event">
  <rdfs:subClassOf rdf:resource="&pimo;Event"/>
  <rdfs:subClassOf rdf:resource="&pimo;Locatable"/>
  <rdfs:comment>A social occasion or activity. (Definition from Merriam-Webster)</rdfs:comment>
</rdfs:Class>

<rdf:Property rdf:about="&scos;narrower">
  <rdf:type rdf:resource="&owl;ObjectProperty"/>
  <rdfs:comment xml:lang="en">Narrower concepts are typically rendered as children in a concept hierarchy (tree).</rdfs:comment>
  <rdfs:isDefinedBy rdf:resource="http://www.w3.org/2004/02/skos/core"/>
  <rdfs:label xml:lang="en">has narrower</rdfs:label>
  <rdfs:subPropertyOf rdf:resource="&scos;narrowerTransitive"/>
  <owl:inverseOf rdf:resource="&scos;broader"/>
  <scos:definition xml:lang="en">Relates a concept to a concept that is more specific in meaning.</scos:definition>
  <scos:scopeNote xml:lang="en">By convention, skos:broader is only used to assert an immediate (i.e. direct) hierarchical link between two conceptual resources.</scos:scopeNote>
</rdf:Property>

<rdf:Property rdf:about="&nfo;fileSize"
    rdfs:label="fileSize">
  <nrl:maxCardinality rdf:datatype="&xsd;integer">1</nrl:maxCardinality>
  <rdfs:comment>The size of the file in bytes. For compressed files it means the size of the packed file, not of the contents. For folders it means the aggregated size of all contained files and folders </rdfs:comment>
  <rdfs:domain rdf:resource="&nfo;FileDataObject"/>
  <rdfs:range rdf:resource="&xsd;integer"/>
  <rdfs:subPropertyOf rdf:resource="&nie;byteSize"/>
</rdf:Property>

<rdfs:Class rdf:about="&nmo;MailboxDataObject"
    rdfs:label="MailboxDataObject">
  <rdfs:comment>An entity encountered in a mailbox. Most common interpretations for such an entity include Message or Folder</rdfs:comment>
  <rdfs:subClassOf rdf:resource="&nie;DataObject"/>
</rdfs:Class>

<rdfs:Class rdf:about="&cnt;Content">
  <rdf:type rdf:resource="&owl;Class"/>
  <rdfs:comment xml:lang="en">The content.</rdfs:comment>
  <rdfs:label xml:lang="en">Content</rdfs:label>
</rdfs:Class>

<rdf:Property rdf:about="&nmo;messageId"
    rdfs:label="messageId">
  <rdfs:comment>An identifier of a message. This property has been inspired by the message-id property defined in RFC 2822, Sec. 3.6.4. It should be used for all kinds of identifiers used by various messaging applications to connect multiple messages into conversations. For email messageids, values are according to RFC2822/sec 3.6.4 and the literal value in RDF must include the brackets.</rdfs:comment>
  <rdfs:domain rdf:resource="&nmo;Message"/>
  <rdfs:range rdf:resource="&xsd;string"/>
  <rdfs:subPropertyOf rdf:resource="&nie;identifier"/>
</rdf:Property>

<owl:Class rdf:about="&oa;HttpRequestState">
  <rdfs:comment xml:lang="en">A resource which describes how to retrieve an appropriate representation of the Source resource for the Annotation, based on the HTTP Request headers to send to the server.

There MUST be exactly 1 rdf:value property per HttpRequestState, containing HTTP request headers as a single, complete string, exactly as they would appear in an HTTP request. </rdfs:comment>
  <rdfs:isDefinedBy rdf:resource="&oa;"/>
  <rdfs:label xml:lang="en">HttpRequestState</rdfs:label>
  <rdfs:subClassOf rdf:resource="&oa;State"/>
</owl:Class>

<rdf:Property rdf:about="&ncal;byyearday"
    rdfs:label="byyearday">
  <rdfs:comment>Day of the year the event should occur. Defined in RFC 2445 sec. 4.3.10</rdfs:comment>
  <rdfs:domain rdf:resource="&ncal;RecurrenceRule"/>
  <rdfs:range rdf:resource="&xsd;integer"/>
</rdf:Property>

<rdfs:Class rdf:about="&dcterms;LinguisticSystem">
  <dcterms:description xml:lang="en">Examples include written, spoken, sign, and computer languages.</dcterms:description>
  <dcterms:hasVersion rdf:resource="http://dublincore.org/usage/terms/history/#LinguisticSystem-001"/>
  <dcterms:issued rdf:datatype="&xsd;date">2008-01-14</dcterms:issued>
  <rdfs:comment xml:lang="en">A system of signs, symbols, sounds, gestures, or rules used in communication.</rdfs:comment>
  <rdfs:isDefinedBy rdf:resource="&dcterms;"/>
  <rdfs:label xml:lang="en">Linguistic System</rdfs:label>
</rdfs:Class>

<rdf:Property rdf:about="&nid3;encodedBy"
    rdfs:label="encodedBy">
  <rdfs:comment>TENC
The 'Encoded by' frame contains the name of the person or organisation that encoded the audio file. This field may contain a copyright message, if the audio file also is copyrighted by the encoder.
Note that the RDF representation doesn't allow the copyright message in this field. Please move it to the copyrightMessage field.</rdfs:comment>
  <rdfs:domain rdf:resource="&nid3;ID3Audio"/>
  <rdfs:range rdf:resource="&nco;Contact"/>
  <rdfs:subPropertyOf rdf:resource="&nco;contributor"/>
</rdf:Property>

<rdfs:Datatype rdf:about="&dcterms;ISO3166">
  <dcterms:hasVersion rdf:resource="http://dublincore.org/usage/terms/history/#ISO3166-004"/>
  <dcterms:issued rdf:datatype="&xsd;date">2000-07-11</dcterms:issued>
  <dcterms:modified rdf:datatype="&xsd;date">2008-01-14</dcterms:modified>
  <rdfs:comment xml:lang="en">The set of codes listed in ISO 3166-1 for the representation of names of countries.</rdfs:comment>
  <rdfs:isDefinedBy rdf:resource="&dcterms;"/>
  <rdfs:label xml:lang="en">ISO 3166</rdfs:label>
  <rdfs:seeAlso rdf:resource="http://www.iso.org/iso/en/prods-services/iso3166ma/02iso-3166-code-lists/list-en1.html"/>
</rdfs:Datatype>

<rdf:Property rdf:about="&tmo;nextReviewIntervall"
    nrl:maxCardinality="1"
    rdfs:label="nextReviewIntervall">
  <rdfs:domain rdf:resource="&tmo;Task"/>
  <rdfs:range rdf:resource="&xsd;integer"/>
</rdf:Property>

<ncal:JournalStatus rdf:about="&ncal;finalStatus"
    rdfs:label="finalStatus"/>

<rdfs:Class rdf:about="&nrl;NonDefiningProperty"
    rdfs:label="non-defining property">
  <rdfs:comment>A non-defining property's value is not part of what defines a resource, it rather
                          is part of the resource's state or expresses an opinion about the resource. Whenever
                          comparing resources or sharing them the value of this property should not be taken into
                          account. By default all properties with a resource range are to be treated as
                          non-defining properties unless they are marked as nrl:DefiningProperty.</rdfs:comment>
  <rdfs:subClassOf rdf:resource="&rdf;Property"/>
</rdfs:Class>

<rdf:Property rdf:about="&ncal;contact"
    rdfs:label="contact">
  <rdfs:comment>The property is used to represent contact information or alternately a reference to contact information associated with the calendar component. Inspired by RFC 2445 sec. 4.8.4.2 with the following reservations: the LANGUAGE parameter has been discarded. Please use xml:lang literals to express language. For the ALTREP parameter use the contactAltRep property.RFC doesn't define any format for the string.</rdfs:comment>
  <rdfs:domain rdf:resource="&ncal;UnionOfEventFreebusyJournalTodo"/>
  <rdfs:range rdf:resource="&xsd;string"/>
</rdf:Property>

<rdf:Property rdf:about="&tmo;taskStateChangesFrom"
    nrl:maxCardinality="1"
    rdfs:label="taskStateChangesFrom">
  <rdfs:domain rdf:resource="&tmo;TaskState"/>
  <rdfs:range rdf:resource="&tmo;TaskState"/>
  <rdfs:subPropertyOf rdf:resource="&tmo;stateTypeRole"/>
</rdf:Property>

<owl:Class rdf:about="&oa;DataPositionSelector">
  <rdfs:comment xml:lang="en">A Selector which describes a range of data based on its start and end positions within the byte stream of the representation.

Each DataPositionSelector MUST have exactly 1 oa:start property.

Each TextPositionSelector MUST have exactly 1 oa:end property.

See oa:TextPositionSelector for selection at normalized character level rather than bytestream level.</rdfs:comment>
  <rdfs:isDefinedBy rdf:resource="&oa;"/>
  <rdfs:label xml:lang="en">DataPositionSelector</rdfs:label>
  <rdfs:subClassOf rdf:resource="&oa;Selector"/>
</owl:Class>

<rdfs:Class rdf:about="&ncal;Attendee"
    rdfs:label="Attendee">
  <rdfs:comment>An attendee of an event. This class has been introduced to serve as the range for ncal:attendee property. See documentation of ncal:attendee for details.</rdfs:comment>
  <rdfs:subClassOf rdf:resource="&ncal;AttendeeOrOrganizer"/>
</rdfs:Class>

<rdfs:Class rdf:about="&drmo;ResourceDeleted"
    rdfs:label="Resource Deleted">
  <rdfs:comment>Describes a condition which is triggered by a deletion of a PIM resource.</rdfs:comment>
  <rdfs:subClassOf rdf:resource="&drmo;Condition"/>
</rdfs:Class>

<rdfs:Class rdf:about="&pimo;Meeting"
    rdfs:label="Meeting">
  <rdfs:comment>The social act of assembling for some common purpose; "his meeting with the salesman was the high point of his day". (Definition from SUMO)</rdfs:comment>
  <rdfs:subClassOf rdf:resource="&pimo;SocialEvent"/>
</rdfs:Class>

<rdf:Property rdf:about="&tmo;attachmentRole"
    nrl:maxCardinality="1"
    rdfs:label="attachmentRole">
  <rdfs:domain rdf:resource="&tmo;Attachment"/>
  <rdfs:range rdf:resource="&tmo;AttachmentRole"/>
  <rdfs:subPropertyOf rdf:resource="&tmo;stateTypeRole"/>
</rdf:Property>

<rdf:Property rdf:about="&nrl;inverseProperty"
    rdfs:comment="Links two properties and specifies their inverse behaviour"
    rdfs:label="inverseProperty">
  <rdfs:domain rdf:resource="&rdf;Property"/>
  <rdfs:range rdf:resource="&rdf;Property"/>
</rdf:Property>

<rdfs:Class rdf:about="&nrl;DocumentGraph"
    rdfs:label="DocumentGraph">
  <rdfs:comment>A marker class to identify named graphs that exist within a physical document</rdfs:comment>
  <rdfs:subClassOf rdf:resource="&nrl;Graph"/>
</rdfs:Class>

<rdf:Property rdf:about="&nexif;unknown"
    rdfs:comment="An Exif tag whose meaning is not known"
    rdfs:label="unknown">
  <rdfs:domain rdf:resource="&nexif;Photo"/>
  <rdfs:range rdf:resource="&xsd;string"/>
  <rdfs:subPropertyOf rdf:resource="http://www.kanzaki.com/ns/exif#_unknown"/>
</rdf:Property>

<rdfs:Class rdf:about="&nfo;Executable"
    rdfs:comment="An executable file."
    rdfs:label="Executable">
  <rdfs:subClassOf rdf:resource="&nie;InformationElement"/>
</rdfs:Class>

<ncal:ParticipationStatus rdf:about="&ncal;acceptedParticipationStatus"
    rdfs:label="acceptedParticipationStatus"/>

<rdfs:Datatype rdf:about="&dcterms;RFC1766">
  <dcterms:hasVersion rdf:resource="http://dublincore.org/usage/terms/history/#RFC1766-003"/>
  <dcterms:issued rdf:datatype="&xsd;date">2000-07-11</dcterms:issued>
  <dcterms:modified rdf:datatype="&xsd;date">2008-01-14</dcterms:modified>
  <rdfs:comment xml:lang="en">The set of tags, constructed according to RFC 1766, for the identification of languages.</rdfs:comment>
  <rdfs:isDefinedBy rdf:resource="&dcterms;"/>
  <rdfs:label xml:lang="en">RFC 1766</rdfs:label>
  <rdfs:seeAlso rdf:resource="http://www.ietf.org/rfc/rfc1766.txt"/>
</rdfs:Datatype>

<tmo:PersonInvolvementRole rdf:about="&tmo;TMO_Instance_PersonInvolvementRole_Involved"
    rdfs:label="TMO_Instance_PersonInvolvementRole_Involved"/>

<rdf:Property rdf:about="&dpo;maxYear"
    rdfs:label="Maximum Year">
  <rdfs:comment>A subproperty of dpo:maxValue that defines an upperbound on the observed calendar year such that it can classify as a dpo:TimePeriod instance. It can be used in conjunction with dpo:minYear, i.e. specific instances of dpo:TimePeriod have a pre-defined observable year-based period.</rdfs:comment>
  <rdfs:domain rdf:resource="&dpo;TimePeriod"/>
  <rdfs:range rdf:resource="&xsd;integer"/>
  <rdfs:subPropertyOf rdf:resource="&dpo;minValue"/>
</rdf:Property>

<rdf:Property rdf:about="&nao;contributor"
    rdfs:label="contributor">
  <rdfs:subPropertyOf rdf:resource="&dc;contributor"/>
  <rdfs:subPropertyOf rdf:resource="&nao;annotation"/>
  <rdfs:comment>Refers to a single or a group of individuals that contributed to a resource</rdfs:comment>
  <rdfs:domain rdf:resource="&rdfs;Resource"/>
  <rdfs:range rdf:resource="&nao;Party"/>
</rdf:Property>

<rdfs:Class rdf:about="&dcterms;Jurisdiction">
  <dcterms:hasVersion rdf:resource="http://dublincore.org/usage/terms/history/#Jurisdiction-001"/>
  <dcterms:issued rdf:datatype="&xsd;date">2008-01-14</dcterms:issued>
  <rdfs:comment xml:lang="en">The extent or range of judicial, law enforcement, or other authority.</rdfs:comment>
  <rdfs:isDefinedBy rdf:resource="&dcterms;"/>
  <rdfs:label xml:lang="en">Jurisdiction</rdfs:label>
  <rdfs:subClassOf rdf:resource="&dcterms;LocationPeriodOrJurisdiction"/>
</rdfs:Class>

<ncal:RecurrenceFrequency rdf:about="&ncal;yearly"
    rdfs:label="yearly"/>

<rdf:Property rdf:about="&dcon;distanceCovered"
    rdfs:label="Distance Covered">
  <rdfs:comment>Specifies the distance travelled while performing the activity.</rdfs:comment>
  <rdfs:domain rdf:resource="&dpo;Activity"/>
  <rdfs:range rdf:resource="&xsd;nonNegativeInteger"/>
  <rdfs:subPropertyOf rdf:resource="&dcon;hasContextAttribute"/>
</rdf:Property>

<rdf:Property rdf:about="&dcon;dateTime"
    rdfs:label="Date and Time Value">
  <rdfs:comment>States the exact date and time value for a pre-defined time period in the current context.</rdfs:comment>
  <rdfs:domain rdf:resource="&dpo;TimePeriod"/>
  <rdfs:range rdf:resource="&xsd;dateTime"/>
  <rdfs:subPropertyOf rdf:resource="&dcon;hasContextAttribute"/>
</rdf:Property>

<owl:DatatypeProperty rdf:about="&oa;prefix">
  <rdfs:comment xml:lang="en">A snippet of text that occurs immediately before the text which is being selected.

See oa:TextQuoteSelector.</rdfs:comment>
  <rdfs:domain rdf:resource="&oa;Selector"/>
  <rdfs:isDefinedBy rdf:resource="&oa;"/>
  <rdfs:label xml:lang="en">prefix</rdfs:label>
</owl:DatatypeProperty>

<rdf:Property rdf:about="&nexif;sceneType"
    rdfs:label="sceneType">
  <rdfs:subPropertyOf rdf:resource="http://www.kanzaki.com/ns/exif#sceneType"/>
  <rdfs:subPropertyOf rdf:resource="&nexif;pictTaking"/>
  <rdfs:comment>tagNumber: 41729
The type of scene. If a DSC recorded the image, this tag value shall always be set to 1, indicating that the image was directly photographed.</rdfs:comment>
  <rdfs:domain rdf:resource="&nexif;Photo"/>
  <rdfs:range rdf:resource="&xsd;string"/>
</rdf:Property>

<rdf:Property rdf:about="&nid3;composer"
    rdfs:label="composer">
  <rdfs:comment>TCOM
The 'Composer(s)' frame is intended for the name of the composer(s). They are seperated with the "/" character.
Note that in the RDF representation each composer is represented with a separate triple.</rdfs:comment>
  <rdfs:domain rdf:resource="&nid3;ID3Audio"/>
  <rdfs:range rdf:resource="&nco;Contact"/>
  <rdfs:subPropertyOf rdf:resource="&nco;creator"/>
</rdf:Property>

<rdf:Property rdf:about="&dpo;minWeek"
    rdfs:label="Minimum Week">
  <rdfs:comment>A subproperty of dpo:minValue that defines a lowerbound on the observed week of the year (i.e., between 1 and 52) such that it can classify as a dpo:TimePeriod instance. It can be used in conjunction with dpo:maxWeek, i.e. specific instances of dpo:TimePeriod have a pre-defined observable week number-based period.</rdfs:comment>
  <rdfs:domain rdf:resource="&dpo;TimePeriod"/>
  <rdfs:range rdf:resource="&xsd;integer"/>
  <rdfs:subPropertyOf rdf:resource="&dpo;minValue"/>
</rdf:Property>

<rdf:Property rdf:about="&nexif;photometricInterpretation"
    rdfs:label="photometricInterpretation">
  <rdfs:subPropertyOf rdf:resource="http://www.kanzaki.com/ns/exif#photometricInterpretation"/>
  <rdfs:subPropertyOf rdf:resource="&nexif;imageDataStruct"/>
  <rdfs:comment>Pixel composition. In JPEG compressed data a JPEG marker is used instead of this tag.
tagNumber: 262</rdfs:comment>
  <rdfs:domain rdf:resource="&nexif;Photo"/>
  <rdfs:range rdf:resource="&xsd;string"/>
</rdf:Property>

<ncal:Weekday rdf:about="&ncal;sunday"
    rdfs:label="sunday"/>

<rdf:Property rdf:about="&foaf;msnChatID"
    rdfs:comment="An MSN chat ID"
    rdfs:label="MSN chat ID"
    ns:term_status="testing">
  <rdf:type rdf:resource="&owl;DatatypeProperty"/>
  <rdf:type rdf:resource="&owl;InverseFunctionalProperty"/>
  <rdfs:domain rdf:resource="&foaf;Agent"/>
  <rdfs:isDefinedBy rdf:resource="&foaf;"/>
  <rdfs:range rdf:resource="&rdfs;Literal"/>
  <rdfs:subPropertyOf rdf:resource="&foaf;nick"/>
</rdf:Property>

<rdfs:Class rdf:about="&rdfs;Class">
  <rdf:type rdf:resource="&owl;Class"/>
  <rdfs:comment xml:lang="en">The class of classes.</rdfs:comment>
  <rdfs:isDefinedBy rdf:resource="&rdfs;"/>
  <rdfs:label xml:lang="en">Class</rdfs:label>
  <rdfs:subClassOf rdf:resource="&rdfs;Resource"/>
</rdfs:Class>

<rdfs:Class rdf:about="&nfo;MindMap"
    rdfs:label="MindMap">
  <rdfs:comment>A MindMap, created by a mind-mapping utility. Examples might include FreeMind or mind mapper.</rdfs:comment>
  <rdfs:subClassOf rdf:resource="&nfo;Document"/>
</rdfs:Class>

<rdf:Property rdf:about="&dcon;snowfalldegree"
    rdfs:label="Snowfall Degree Value">
  <rdfs:comment>Registers an actual snowfall degree value element attribute to an active weather condition in the current context.</rdfs:comment>
  <rdfs:domain rdf:resource="&dpo;WeatherConditions"/>
  <rdfs:range rdf:resource="&xsd;nonNegativeInteger"/>
  <rdfs:subPropertyOf rdf:resource="&dcon;hasContextAttribute"/>
</rdf:Property>

<rdf:Property rdf:about="&nao;hasDataGraph"
    rdfs:label="has data graph">
  <nrl:inverseProperty rdf:resource="&nao;isDataGraphFor"/>
  <rdfs:comment>Links a resource to the graph which contains its metadata. Its typical usage would be to link the file resource to the graph containing its extracted file metadata. This allows for easy maintenance later on. Inverse property of nao:isDataGraphFor.</rdfs:comment>
  <rdfs:domain rdf:resource="&rdfs;Resource"/>
  <rdfs:range rdf:resource="&nrl;InstanceBase"/>
</rdf:Property>

<rdf:Property rdf:about="&ncal;relatedToParent"
    rdfs:label="relatedToParent">
  <rdfs:comment>The property is used to represent a relationship or reference between one calendar component and another. Inspired by RFC 2445 sec. 4.8.4.5. Originally this property had a RELTYPE parameter. It has been decided that it is more natural to introduce three different properties to express the values of that parameter. This property expresses the RELATED-TO property with no RELTYPE parameter (the default value is PARENT), or with explicit RELTYPE=PARENT parameter.</rdfs:comment>
  <rdfs:domain rdf:resource="&ncal;UnionOfEventJournalTodo"/>
  <rdfs:range rdf:resource="&xsd;string"/>
  <rdfs:subPropertyOf rdf:resource="&ncal;ncalRelation"/>
</rdf:Property>

<rdf:Property rdf:about="&ddo;networkID"
    rdfs:label="networkID">
  <rdfs:comment>Attaches a name to a network. Use ddo:accessPointID and ddo:cellID for more specific identification.</rdfs:comment>
  <rdfs:domain rdf:resource="&ddo;Network"/>
  <rdfs:range rdf:resource="&xsd;string"/>
</rdf:Property>

<rdf:Property rdf:about="&ncal;due"
    rdfs:label="due">
  <nrl:maxCardinality rdf:datatype="&xsd;integer">1</nrl:maxCardinality>
  <rdfs:comment>This property defines the date and time that a to-do is expected to be completed. Inspired by RFC 2445 sec. 4.8.2.3</rdfs:comment>
  <rdfs:domain rdf:resource="&ncal;Todo"/>
  <rdfs:range rdf:resource="&ncal;NcalDateTime"/>
</rdf:Property>

<rdfs:Class rdf:about="&rdfs;Datatype">
  <rdfs:comment xml:lang="en">The class of RDF datatypes.</rdfs:comment>
  <rdfs:isDefinedBy rdf:resource="&rdfs;"/>
  <rdfs:label xml:lang="en">Datatype</rdfs:label>
  <rdfs:subClassOf rdf:resource="&rdfs;Class"/>
</rdfs:Class>

<nfo:EncryptionStatus rdf:about="&nfo;decryptedStatus"
    rdfs:label="DecryptedStatus"/>

<tmo:AttachmentRole rdf:about="&tmo;TMO_Instance_AttachmentRole_Desired_Requested"
    rdfs:label="TMO_Instance_AttachmentRole_Desired_Requested"/>

<rdfs:Class rdf:about="&nfo;Trash"
    rdfs:label="Trash">
  <rdfs:comment>Represents a container for deleted files, a feature common in modern operating systems.</rdfs:comment>
  <rdfs:subClassOf rdf:resource="&nfo;DataContainer"/>
</rdfs:Class>

<rdf:Property rdf:about="&nco;title"
    nrl:maxCardinality="1"
    rdfs:label="title">
  <rdfs:comment>The official title  the object represented by this contact in an organization. E.g. 'CEO', 'Director, Research and Development', 'Junior Software Developer/Analyst' etc. An equivalent of the 'TITLE' property defined in RFC 2426 Sec. 3.5.1</rdfs:comment>
  <rdfs:domain rdf:resource="&nco;Affiliation"/>
  <rdfs:range rdf:resource="&xsd;string"/>
</rdf:Property>

<rdf:Property rdf:about="&nexif;height"
    rdfs:comment="Height of an object"
    rdfs:label="height">
  <rdfs:subPropertyOf rdf:resource="http://www.kanzaki.com/ns/exif#height"/>
  <rdfs:subPropertyOf rdf:resource="&nexif;length"/>
  <rdfs:domain rdf:resource="&nexif;Photo"/>
  <rdfs:range rdf:resource="&xsd;integer"/>
</rdf:Property>

<rdfs:Class rdf:about="&dctypes;Sound">
  <dcam:memberOf rdf:resource="&dcterms;DCMIType"/>
  <dcterms:description xml:lang="en">Examples include a music playback file format, an audio compact disc, and recorded speech or sounds.</dcterms:description>
  <dcterms:hasVersion rdf:resource="http://dublincore.org/usage/terms/history/#Sound-003"/>
  <dcterms:issued rdf:datatype="&xsd;date">2000-07-11</dcterms:issued>
  <dcterms:modified rdf:datatype="&xsd;date">2008-01-14</dcterms:modified>
  <rdfs:comment xml:lang="en">A resource primarily intended to be heard.</rdfs:comment>
  <rdfs:isDefinedBy rdf:resource="&dctypes;"/>
  <rdfs:label xml:lang="en">Sound</rdfs:label>
</rdfs:Class>

<owl:Class rdf:about="&oa;CssStyle">
  <rdfs:comment xml:lang="en">A resource which describes styles for resources participating in the Annotation using CSS.

Specific Resources MAY be assigned a CSS style class using oa:styleClass.

The CSS resource MAY have its own dereferencable URI that provides the information. For example, "Style1" in the diagram below might actually have the URI "http://www.example.com/styles/annotations.css". It MAY be embedded within the Annotation using the inline constructions described in Embedding Resources.</rdfs:comment>
  <rdfs:isDefinedBy rdf:resource="&oa;"/>
  <rdfs:label xml:lang="en">CssStyle</rdfs:label>
  <rdfs:subClassOf rdf:resource="&oa;Style"/>
</owl:Class>

<rdf:Property rdf:about="&ncal;periodDuration"
    rdfs:label="periodDuration">
  <nrl:maxCardinality rdf:datatype="&xsd;integer">1</nrl:maxCardinality>
  <rdfs:comment>Duration of a period of time. Inspired by the second part of a structured value of the PERIOD datatype specified in RFC 2445 sec. 4.3.9. Note that a single NcalPeriod instance shouldn't have the periodEnd and periodDuration properties specified simultaneously.</rdfs:comment>
  <rdfs:domain rdf:resource="&ncal;NcalPeriod"/>
  <rdfs:range rdf:resource="&xsd;duration"/>
</rdf:Property>

<rdf:Property rdf:about="&nexif;deviceSettingDescription"
    rdfs:label="deviceSettingDescription">
  <rdfs:subPropertyOf rdf:resource="http://www.kanzaki.com/ns/exif#deviceSettingDescription"/>
  <rdfs:subPropertyOf rdf:resource="&nexif;pictTaking"/>
  <rdfs:comment>tagNumber: 41995
Information on the picture-taking conditions of a particular camera model. The tag is used only to indicate the picture-taking conditions in the reader.</rdfs:comment>
  <rdfs:domain rdf:resource="&nexif;Photo"/>
  <rdfs:range rdf:resource="&xsd;string"/>
</rdf:Property>

<rdf:Property rdf:about="&nexif;oecf"
    rdfs:label="oecf">
  <rdfs:subPropertyOf rdf:resource="http://www.kanzaki.com/ns/exif#oecf"/>
  <rdfs:subPropertyOf rdf:resource="&nexif;pictTaking"/>
  <rdfs:comment>tagNumber: 34856
Indicates the Opto-Electric Conversion Function (OECF) specified in ISO 14524. OECF is the relationship between the camera optical input and the image values.</rdfs:comment>
  <rdfs:domain rdf:resource="&nexif;Photo"/>
  <rdfs:range rdf:resource="&xsd;string"/>
</rdf:Property>

<nco:IMStatusType rdf:about="&nco;IMStatusTypeUnknown"
    rdfs:label="unknown"/>

<rdf:Property rdf:about="&drmo;hasSubject"
    rdfs:comment="Specifies the received of the action."
    rdfs:label="has Subject">
  <rdfs:domain rdf:resource="&drmo;Action"/>
  <rdfs:range rdf:resource="&rdfs;Resource"/>
</rdf:Property>

<rdfs:Class rdf:about="&dplo;PresencePost"
    rdfs:label="Presence Post">
  <rdfs:comment>A livepost consisting of information related to a user's presence, as defined by a set of DPO (Presence Ontology) instances.</rdfs:comment>
  <rdfs:subClassOf rdf:resource="&dplo;LivePost"/>
</rdfs:Class>

<rdf:Property rdf:about="&scos;narrowMatch">
  <rdfs:subPropertyOf rdf:resource="&scos;mappingRelation"/>
  <rdfs:subPropertyOf rdf:resource="&scos;narrower"/>
  <rdf:type rdf:resource="&owl;ObjectProperty"/>
  <rdfs:isDefinedBy rdf:resource="http://www.w3.org/2004/02/skos/core"/>
  <rdfs:label xml:lang="en">has narrower match</rdfs:label>
  <owl:inverseOf rdf:resource="&scos;broadMatch"/>
  <scos:definition xml:lang="en">skos:narrowMatch is used to state a hierarchical mapping link between two conceptual resources in different concept schemes.</scos:definition>
</rdf:Property>

<rdf:Property rdf:about="&ncal;completed"
    rdfs:label="completed">
  <nrl:maxCardinality rdf:datatype="&xsd;integer">1</nrl:maxCardinality>
  <rdfs:comment>This property defines the date and time that a to-do was actually completed. Inspired by RFC 2445 sec. 4.8.2.1. Note that the RFC allows ONLY UTC time values for this property.</rdfs:comment>
  <rdfs:domain rdf:resource="&ncal;Todo"/>
  <rdfs:range rdf:resource="&xsd;dateTime"/>
</rdf:Property>

<rdf:Property rdf:about="&nexif;gpsVersionID"
    rdfs:label="gpsVersionID">
  <rdfs:subPropertyOf rdf:resource="http://www.kanzaki.com/ns/exif#gpsVersionID"/>
  <rdfs:subPropertyOf rdf:resource="&nexif;gpsInfo"/>
  <rdfs:subPropertyOf rdf:resource="&nexif;versionInfo"/>
  <rdfs:comment>The version of GPSInfoIFD. The version is given as 2.2.0.0. This tag is mandatory when GPSInfo tag is present.
tagNumber: 0</rdfs:comment>
  <rdfs:domain rdf:resource="&nexif;Photo"/>
  <rdfs:range rdf:resource="&xsd;string"/>
</rdf:Property>

<owl:Ontology rdf:about="http://www.w3.org/2011/content">
  <rdfs:comment xml:lang="en">Representing Content in RDF as defined by http://www.w3.org/TR/Content-in-RDF/</rdfs:comment>
  <rdfs:isDefinedBy rdf:resource="http://www.w3.org/TR/Content-in-RDF/"/>
  <rdfs:label xml:lang="en">Representing Content in RDF</rdfs:label>
  <rdfs:seeAlso rdf:resource="http://www.w3.org/WAI/intro/earl"/>
  <owl:imports rdf:resource="&dcterms;"/>
  <owl:versionInfo xml:lang="en">Working Draft 29 April 2011</owl:versionInfo>
</owl:Ontology>

<owl:DatatypeProperty rdf:about="&oa;annotatedAt">
  <rdfs:comment xml:lang="en">The time at which the Annotation was created. 

There SHOULD be exactly 1 oa:annotatedAt property per Annotation, and MUST NOT be more than 1. The datetime MUST be expressed in the xsd:dateTime format, and SHOULD have a timezone specified.</rdfs:comment>
  <rdfs:domain rdf:resource="&oa;Annotation"/>
  <rdfs:isDefinedBy rdf:resource="&oa;"/>
  <rdfs:label xml:lang="en">annotatedAt</rdfs:label>
  <rdfs:range rdf:resource="&xsd;dateTimeStamp"/>
</owl:DatatypeProperty>

<rdf:Property rdf:about="&foaf;mbox"
    rdfs:label="personal mailbox"
    ns:term_status="stable">
  <rdf:type rdf:resource="&owl;InverseFunctionalProperty"/>
  <rdf:type rdf:resource="&owl;ObjectProperty"/>
  <rdfs:comment>A  personal mailbox, ie. an Internet mailbox associated with exactly one owner, the first owner of this mailbox. This is a 'static inverse functional property', in that  there is (across time and change) at most one individual that ever has any particular value for foaf:mbox.</rdfs:comment>
  <rdfs:domain rdf:resource="&foaf;Agent"/>
  <rdfs:isDefinedBy rdf:resource="&foaf;"/>
  <rdfs:range rdf:resource="&owl;Thing"/>
</rdf:Property>

<rdf:Property rdf:about="&nexif;exifdata"
    rdfs:comment="An Exif IFD data entry"
    rdfs:label="exifdata">
  <rdfs:domain rdf:resource="&nexif;Photo"/>
  <rdfs:range rdf:resource="&xsd;string"/>
  <rdfs:subPropertyOf rdf:resource="http://www.kanzaki.com/ns/exif#exifdata"/>
</rdf:Property>

<rdfs:Class rdf:about="&nco;ContactList"
    rdfs:label="ContactList">
  <rdfs:comment>A contact list, this class represents an addressbook or a contact list of an IM application. Contacts inside a contact list can belong to contact groups.</rdfs:comment>
  <rdfs:subClassOf rdf:resource="&nie;InformationElement"/>
</rdfs:Class>

<rdfs:Datatype rdf:about="&dcterms;W3CDTF">
  <dcterms:hasVersion rdf:resource="http://dublincore.org/usage/terms/history/#W3CDTF-003"/>
  <dcterms:issued rdf:datatype="&xsd;date">2000-07-11</dcterms:issued>
  <dcterms:modified rdf:datatype="&xsd;date">2008-01-14</dcterms:modified>
  <rdfs:comment xml:lang="en">The set of dates and times constructed according to the W3C Date and Time Formats Specification.</rdfs:comment>
  <rdfs:isDefinedBy rdf:resource="&dcterms;"/>
  <rdfs:label xml:lang="en">W3C-DTF</rdfs:label>
  <rdfs:seeAlso rdf:resource="http://www.w3.org/TR/NOTE-datetime"/>
</rdfs:Datatype>

<tmo:TransmissionType rdf:about="&tmo;TMO_Instance_TransmissionType_Join"
    rdfs:label="TMO_Instance_TransmissionType_Join"/>

<owl:ObjectProperty rdf:about="&oa;equivalentTo">
  <rdfs:comment xml:lang="en">The subject and object resources of the oa:equivalentTo relationship represent the same resource, but potentially have different metadata such as oa:serializedBy, oa:serializedAt and serialization format.  oa:equivalentTo is a symmetrical and transitive relationship; if A oa:equivalentTo B, then it is also true that B oa:equivalent A; and that if B oa:equivalentTo C, then it is also true that A oa:equivalentTo C. 

The Annotation MAY include 0 or more instances of the oa:equivalentTo relationship between copies of the Annotation or other resources, and SHOULD include as many as are available.

If a system publishes an embedded resource (a cnt:Content) at a new HTTP URI, then it SHOULD express the oa:equivalentTo relationship between the resource's URN and the new URI from which it is available.</rdfs:comment>
  <rdfs:isDefinedBy rdf:resource="&oa;"/>
  <rdfs:label xml:lang="en">equivalentTo</rdfs:label>
  <rdfs:subPropertyOf rdf:resource="&prov;alternateOf"/>
</owl:ObjectProperty>

<rdf:Property rdf:about="&ncal;transp"
    rdfs:label="transp">
  <nrl:maxCardinality rdf:datatype="&xsd;integer">1</nrl:maxCardinality>
  <rdfs:comment>Defines whether an event is transparent or not  to busy time searches. Inspired by RFC 2445 sec.4.8.2.7. Values for this property can be chosen from a limited vocabulary. To express this a TimeTransparency class has been introduced.</rdfs:comment>
  <rdfs:domain rdf:resource="&ncal;Event"/>
  <rdfs:range rdf:resource="&ncal;TimeTransparency"/>
</rdf:Property>

<rdf:Property rdf:about="&nao;maintainedBy"
    rdfs:label="maintained by">
  <rdfs:comment>The agent that maintains this resource, ie. created it and knows what to do with it.</rdfs:comment>
  <rdfs:domain rdf:resource="&rdfs;Resource"/>
  <rdfs:range rdf:resource="&nao;Agent"/>
  <rdfs:subPropertyOf rdf:resource="&nao;annotation"/>
</rdf:Property>

<rdf:Property rdf:about="&tmo;dueDate"
    nrl:maxCardinality="1"
    rdfs:label="dueDate">
  <rdfs:subPropertyOf rdf:resource="&pimo;taskDueTime"/>
  <rdfs:subPropertyOf rdf:resource="&tmo;dateTime"/>
  <rdfs:domain rdf:resource="&tmo;Task"/>
  <rdfs:range rdf:resource="&xsd;dateTime"/>
</rdf:Property>

<rdf:Property rdf:about="&ncal;prodid"
    rdfs:label="prodid">
  <rdfs:comment>This property specifies the identifier for the product that created the iCalendar object. Defined in RFC 2445 sec. 4.7.2</rdfs:comment>
  <rdfs:domain rdf:resource="&ncal;Calendar"/>
  <rdfs:range rdf:resource="&xsd;string"/>
  <rdfs:subPropertyOf rdf:resource="&nie;generator"/>
</rdf:Property>

<rdf:Property rdf:about="&pimo;hasGlobalNamespace"
    rdfs:label="global namespace">
  <rdfs:comment>The global namespace of this user using the semdesk uri scheme, based on the Global Identifier of the user. Example semdesk://bob@example.com/things/. See http://dev.nepomuk.semanticdesktop.org/repos/trunk/doc/2008_09_semdeskurischeme/index.html</rdfs:comment>
  <rdfs:domain rdf:resource="&pimo;PersonalInformationModel"/>
  <rdfs:range rdf:resource="&rdfs;Literal"/>
</rdf:Property>

<rdf:Property rdf:about="&nco;hobby"
    rdfs:label="hobby">
  <rdfs:comment>A hobby associated with a PersonContact. This property can be used to express hobbies and interests.</rdfs:comment>
  <rdfs:domain rdf:resource="&nco;PersonContact"/>
  <rdfs:range rdf:resource="&nco;Hobby"/>
</rdf:Property>

<rdf:Property rdf:about="&ncal;tzoffsetto"
    rdfs:label="tzoffsetto">
  <nrl:maxCardinality rdf:datatype="&xsd;integer">1</nrl:maxCardinality>
  <rdfs:comment>This property specifies the offset which is in use in this time zone observance. nspired by RFC 2445 sec. 4.8.3.4. The original domain was underspecified. It said that this property must appear within a Timezone component. In this ontology a TimezoneObservance class has been introduced to clarify this specification. The original range was UTC-OFFSET. There is no equivalent among the XSD datatypes so plain string was chosen.</rdfs:comment>
  <rdfs:domain rdf:resource="&ncal;TimezoneObservance"/>
  <rdfs:range rdf:resource="&xsd;string"/>
</rdf:Property>

<owl:ObjectProperty rdf:about="&oa;annotatedBy">
  <rdfs:comment xml:lang="en">The object of the relationship is a resource that identifies the agent responsible for creating the Annotation. This may be either a human or software agent. 

There SHOULD be exactly 1 oa:annotatedBy relationship per Annotation, but MAY be 0 or more than 1, as the Annotation may be anonymous, or multiple agents may have worked together on it.

It is RECOMMENDED to use these and other FOAF terms to describe agents: foaf:Person, prov:SoftwareAgent, foaf:Organization, foaf:name, foaf:mbox, foaf:openid, foaf:homepage</rdfs:comment>
  <rdfs:domain rdf:resource="&oa;Annotation"/>
  <rdfs:isDefinedBy rdf:resource="&oa;"/>
  <rdfs:label xml:lang="en">annotatedBy</rdfs:label>
  <rdfs:subPropertyOf rdf:resource="&prov;wasAttributedTo"/>
</owl:ObjectProperty>

<rdf:Property rdf:about="&dcon;currentAbsoluteAltitude"
    rdfs:label="Current Absolute Altitude">
  <rdfs:comment>States the current absolute altitude (metres above ground level)</rdfs:comment>
  <rdfs:domain rdf:resource="&dcon;SpaTem"/>
  <rdfs:range rdf:resource="&dpo;Altitude"/>
  <rdfs:subPropertyOf rdf:resource="&dcon;hasContextElement"/>
</rdf:Property>

<owl:NamedIndividual rdf:about="&oa;highlighting">
  <rdf:type rdf:resource="&oa;Motivation"/>
  <rdfs:comment xml:lang="en">The motivation that represents a highlighted section of the target resource or segment. For example to draw attention to the selected text that the annotator disagrees with. A Highlight may or may not have a Body resource</rdfs:comment>
  <scos:inScheme rdf:resource="&oa;motivationScheme"/>
  <scos:prefLabel xml:lang="en">highlighting</scos:prefLabel>
</owl:NamedIndividual>

<ncal:AlarmAction rdf:about="&ncal;displayAction"
    rdfs:label="displayAction"/>

<rdf:Property rdf:about="&nexif;gpsSpeed"
    rdfs:comment="The speed of GPS receiver movement.
tagNumber: 13"
    rdfs:label="gpsSpeed">
  <rdfs:subPropertyOf rdf:resource="http://www.kanzaki.com/ns/exif#gpsSpeed"/>
  <rdfs:subPropertyOf rdf:resource="&nexif;gpsInfo"/>
  <rdfs:domain rdf:resource="&nexif;Photo"/>
  <rdfs:range rdf:resource="&xsd;string"/>
</rdf:Property>

<dcam:VocabularyEncodingScheme rdf:about="&dcterms;DDC">
  <dcterms:hasVersion rdf:resource="http://dublincore.org/usage/terms/history/#DDC-003"/>
  <dcterms:issued rdf:datatype="&xsd;date">2000-07-11</dcterms:issued>
  <dcterms:modified rdf:datatype="&xsd;date">2008-01-14</dcterms:modified>
  <rdfs:comment xml:lang="en">The set of conceptual resources specified by the Dewey Decimal Classification.</rdfs:comment>
  <rdfs:isDefinedBy rdf:resource="&dcterms;"/>
  <rdfs:label xml:lang="en">DDC</rdfs:label>
  <rdfs:seeAlso rdf:resource="http://www.oclc.org/dewey/"/>
</dcam:VocabularyEncodingScheme>

<rdf:Property rdf:about="&ncal;percentComplete"
    rdfs:label="percentComplete">
  <rdfs:comment>This property is used by an assignee or delegatee of a to-do to convey the percent completion of a to-do to the Organizer. Inspired by RFC 2445 sec. 4.8.1.8</rdfs:comment>
  <rdfs:domain rdf:resource="&ncal;Todo"/>
  <rdfs:range rdf:resource="&xsd;integer"/>
</rdf:Property>

<tmo:Delegability rdf:about="&tmo;TMO_Instance_Delegability_Medium"
    rdfs:label="TMO_Instance_Delegability_Medium"/>

<rdfs:Class rdf:about="&nfo;DataContainer"
    rdfs:label="DataContainer">
  <rdfs:comment>A superclass for all entities, whose primary purpose is to serve as containers for other data object. They usually don't have any "meaning" by themselves. Examples include folders, archives and optical disc images.</rdfs:comment>
  <rdfs:subClassOf rdf:resource="&nie;InformationElement"/>
</rdfs:Class>

<rdfs:Class rdf:about="&nmm;MusicAlbum"
    rdfs:label="music album">
  <rdfs:comment>The music album as provided by the publisher. Not to be confused with media lists or collections.</rdfs:comment>
  <rdfs:subClassOf rdf:resource="&nfo;MediaList"/>
</rdfs:Class>

<rdf:Property rdf:about="&nexif;compressedBitsPerPixel"
    rdfs:label="compressedBitsPerPixel">
  <rdfs:subPropertyOf rdf:resource="http://www.kanzaki.com/ns/exif#compressedBitsPerPixel"/>
  <rdfs:subPropertyOf rdf:resource="&nexif;imageConfig"/>
  <rdfs:comment>tagNumber: 37122
Information specific to compressed data. The compression mode used for a compressed image is indicated in unit bits per pixel.</rdfs:comment>
  <rdfs:domain rdf:resource="&nexif;Photo"/>
  <rdfs:range rdf:resource="&xsd;string"/>
</rdf:Property>

<rdfs:Class rdf:about="&rdf;Alt">
  <rdfs:comment xml:lang="en">The class of containers of alternatives.</rdfs:comment>
  <rdfs:isDefinedBy rdf:resource="&rdf;"/>
  <rdfs:label xml:lang="en">Alt</rdfs:label>
  <rdfs:subClassOf rdf:resource="&rdfs;Container"/>
</rdfs:Class>

<rdfs:Class rdf:about="&foaf;Agent"
    rdfs:label="Agent"
    ns:term_status="stable">
  <rdf:type rdf:resource="&owl;Class"/>
  <rdfs:comment>An agent (eg. person, group, software or physical artifact).</rdfs:comment>
  <owl:equivalentClass rdf:resource="&dcterms;Agent"/>
</rdfs:Class>

<rdf:Property rdf:about="&nexif;geo"
    rdfs:label="geo">
  <rdfs:comment>Geometric data such as latitude, longitude and altitude. Usually saved as rational number.</rdfs:comment>
  <rdfs:domain rdf:resource="&nexif;Photo"/>
  <rdfs:subPropertyOf rdf:resource="http://www.kanzaki.com/ns/exif#geo"/>
</rdf:Property>

<rdfs:Class rdf:about="&dpo;NonQuantifiableComponent"
    rdfs:label="Non Quantifiable Component">
  <rdfs:comment>Non-qauntifiable presence components refer to interpreted context properties that can be resolved to a more abstract representations that have the ability to recur. For example, a location in which an agent finds itself in can be resolved to a known place that is known, or saved. Although the location is a temporal property bound to the agent's context (i.e., it is always changing), the place is independent of time (i.e., the agent can return to that place repeatedly).</rdfs:comment>
  <rdfs:subClassOf rdf:resource="&dpo;PresenceComponent"/>
</rdfs:Class>

<rdf:Property rdf:about="&nmm;albumTrackCount"
    rdfs:comment="The number of tracks in a music album."
    rdfs:label="album track count">
  <nrl:maxCardinality rdf:datatype="&xsd;integer">1</nrl:maxCardinality>
  <rdfs:domain rdf:resource="&nmm;MusicAlbum"/>
  <rdfs:range rdf:resource="&xsd;integer"/>
</rdf:Property>

<rdf:Property rdf:about="&nmm;hasSeasonEpisode"
    rdfs:comment="Relates a TV Show season to its episodes"
    rdfs:label="has episode">
  <nrl:inverseProperty rdf:resource="&nmm;isPartOfSeason"/>
  <rdfs:domain rdf:resource="&nmm;TVSeason"/>
  <rdfs:range rdf:resource="&nmm;TVShow"/>
  <rdfs:subPropertyOf rdf:resource="&nie;hasLogicalPart"/>
</rdf:Property>

<rdf:Property rdf:about="&nid3;partOfSet"
    rdfs:label="partOfSet">
  <rdfs:comment>TPOS
The 'Part of a set' frame is a numeric string that describes which part of a set the audio came from. This frame is used if the source described in the "TALB" frame is divided into several mediums, e.g. a double CD. The value may be extended with a "/" character and a numeric string containing the total number of parts in the set. E.g. "1/2".</rdfs:comment>
  <rdfs:domain rdf:resource="&nid3;ID3Audio"/>
  <rdfs:range rdf:resource="&xsd;string"/>
</rdf:Property>

<ncal:AlarmAction rdf:about="&ncal;procedureAction"
    rdfs:label="procedureAction"/>

<rdf:Description rdf:about="&dcterms;">
  <dcterms:modified rdf:datatype="&xsd;date">2012-06-14</dcterms:modified>
  <dcterms:publisher rdf:resource="http://purl.org/dc/aboutdcmi#DCMI"/>
  <dcterms:title xml:lang="en">DCMI Metadata Terms - other</dcterms:title>
</rdf:Description>

<rdf:Property rdf:about="&nco;extendedAddress"
    nrl:maxCardinality="1"
    rdfs:label="extendedAddress">
  <rdfs:comment>An extended part of an address. This field might be used to express parts of an address that aren't include in the name of the Contact but also aren't part of the actual location. Usually the streed address and following fields are enough for a postal letter to arrive. Examples may include ('University of California Campus building 45', 'Sears Tower 34th floor' etc.) Inspired by the second part of the value of the 'ADR' property as defined in RFC 2426, sec. 3.2.1</rdfs:comment>
  <rdfs:domain rdf:resource="&nco;PostalAddress"/>
  <rdfs:range rdf:resource="&xsd;string"/>
</rdf:Property>

<rdf:Property rdf:about="&nco;websiteUrl"
    rdfs:comment="A url of a website."
    rdfs:label="websiteUrl">
  <rdfs:domain rdf:resource="&nco;Role"/>
  <rdfs:range rdf:resource="&rdfs;Resource"/>
  <rdfs:subPropertyOf rdf:resource="&nco;url"/>
</rdf:Property>

<rdf:Property rdf:about="&scos;topConceptOf">
  <rdf:type rdf:resource="&owl;ObjectProperty"/>
  <rdfs:domain rdf:resource="&scos;Concept"/>
  <rdfs:isDefinedBy rdf:resource="http://www.w3.org/2004/02/skos/core"/>
  <rdfs:label xml:lang="en">is top concept in scheme</rdfs:label>
  <rdfs:range rdf:resource="&scos;ConceptScheme"/>
  <rdfs:subPropertyOf rdf:resource="&scos;inScheme"/>
  <owl:inverseOf rdf:resource="&scos;hasTopConcept"/>
  <scos:definition xml:lang="en">Relates a concept to the concept scheme that it is a top level concept of.</scos:definition>
</rdf:Property>

<rdf:Property rdf:about="&nid3;internetRadioStationName"
    rdfs:label="internetRadioStationName">
  <rdfs:comment>TRSN
The 'Internet radio station name' frame contains the name of the internet radio station from which the audio is streamed.</rdfs:comment>
  <rdfs:domain rdf:resource="&nid3;ID3Audio"/>
  <rdfs:range rdf:resource="&xsd;string"/>
</rdf:Property>

<rdf:Property rdf:about="&nie;coreGraph"
    rdfs:label="coreGraph">
  <nao:deprecated rdf:datatype="&xsd;boolean">true</nao:deprecated>
  <rdfs:comment>Connects the data object with the graph that contains information about it. Deprecated in favor of a more generic nao:isDataGraphFor.</rdfs:comment>
  <rdfs:domain rdf:resource="&nie;DataObject"/>
  <rdfs:range rdf:resource="&nrl;InstanceBase"/>
</rdf:Property>

<rdf:Property rdf:about="&dpo;relatedActivity"
    rdfs:label="Related Activity">
  <rdfs:comment>Links a place to specific activities, both of which are stored in the PIM, e.g., a dpo:Place representing 'SportsCentre' to a dpo:Activity representing 'Sports'.</rdfs:comment>
  <rdfs:domain rdf:resource="&dpo;Place"/>
  <rdfs:range rdf:resource="&dpo;Activity"/>
  <rdfs:subPropertyOf rdf:resource="&nao;isRelated"/>
</rdf:Property>

<rdf:Property rdf:about="&dcon;brightnessLevel"
    rdfs:label="Brightness Level Value">
  <rdfs:comment>Registers an actual environmental brightness value element attribute to an active brightness level range in the current context.</rdfs:comment>
  <rdfs:domain rdf:resource="&dpo;Brightness"/>
  <rdfs:range rdf:resource="&xsd;float"/>
  <rdfs:subPropertyOf rdf:resource="&dcon;hasContextAttribute"/>
</rdf:Property>

<rdf:Property rdf:about="&tmo;urgency"
    nrl:maxCardinality="1"
    rdfs:label="urgency">
  <rdfs:domain rdf:resource="&tmo;Task"/>
  <rdfs:range rdf:resource="&tmo;Urgency"/>
  <rdfs:subPropertyOf rdf:resource="&tmo;timemanagement"/>
</rdf:Property>

<rdf:Property rdf:about="&dcterms;format">
  <dcterms:description xml:lang="en">Examples of dimensions include size and duration. Recommended best practice is to use a controlled vocabulary such as the list of Internet Media Types [MIME].</dcterms:description>
  <dcterms:hasVersion rdf:resource="http://dublincore.org/usage/terms/history/#formatT-001"/>
  <dcterms:issued rdf:datatype="&xsd;date">2008-01-14</dcterms:issued>
  <dcterms:modified rdf:datatype="&xsd;date">2008-01-14</dcterms:modified>
  <rdfs:comment xml:lang="en">The file format, physical medium, or dimensions of the resource.</rdfs:comment>
  <rdfs:isDefinedBy rdf:resource="&dcterms;"/>
  <rdfs:label xml:lang="en">Format</rdfs:label>
  <rdfs:range rdf:resource="&dcterms;MediaTypeOrExtent"/>
  <rdfs:subPropertyOf rdf:resource="&dc;format"/>
</rdf:Property>

<rdf:Property rdf:about="&dpo;minAltitude"
    rdfs:label="Minimum Altitude">
  <rdfs:comment>A subproperty of dpo:minValue that defines a lowerbound on the observed altitude height value (in metres) such that it can classify as a dpo:Altitude instance. It can be used in conjunction with dpo:maxAltitude, i.e. specific instances of dpo:Altitude have a pre-defined range of observable real-world agent altitude.</rdfs:comment>
  <rdfs:domain rdf:resource="&dpo;Altitude"/>
  <rdfs:range rdf:resource="&xsd;float"/>
  <rdfs:subPropertyOf rdf:resource="&dpo;minValue"/>
</rdf:Property>

<rdfs:Class rdf:about="&ncal;Organizer"
    rdfs:label="Organizer">
  <rdfs:comment>An organizer of an event. This class has been introduced to serve as a range of ncal:organizer property. See documentation of ncal:organizer for details.</rdfs:comment>
  <rdfs:subClassOf rdf:resource="&ncal;AttendeeOrOrganizer"/>
</rdfs:Class>

<rdf:Property rdf:about="&scos;relatedMatch">
  <rdf:type rdf:resource="&owl;ObjectProperty"/>
  <rdf:type rdf:resource="&owl;SymmetricProperty"/>
  <rdfs:subPropertyOf rdf:resource="&scos;mappingRelation"/>
  <rdfs:subPropertyOf rdf:resource="&scos;related"/>
  <rdfs:isDefinedBy rdf:resource="http://www.w3.org/2004/02/skos/core"/>
  <rdfs:label xml:lang="en">has related match</rdfs:label>
  <scos:definition xml:lang="en">skos:relatedMatch is used to state an associative mapping link between two conceptual resources in different concept schemes.</scos:definition>
</rdf:Property>

<nco:IMCapability rdf:about="&nco;imCapabilityAudio"/>

<owl:Class rdf:about="&oa;SvgSelector">
  <rdfs:comment xml:lang="en">A Selector which selects an area specified as an SVG shape.

The SVG document should either be retrievable by resolving the URI of this resource, or be included as an Embedded Resource using cnt:Content.

It is RECOMMENDED that the document contain only a single shape element and that element SHOULD be one of: path, rect, circle, ellipse, polyline, polygon or g. The g element SHOULD ONLY be used to construct a multi-element group, for example to define a donut shape requiring an outer circle and a clipped inner circle.

The dimensions of both the shape and the SVG canvas MUST be relative to the dimensions of the Source resource. For example, given an image which is 600 pixels by 400 pixels, and the desired section is a circle of 100 pixel radius at the center of the image, then the SVG element would be: &lt;circle cx="300" cy="200" r="100"/&gt;

It is NOT RECOMMENDED to include style information within the SVG element, nor Javascript, animation, text or other non shape oriented information. Clients SHOULD ignore such information if present.</rdfs:comment>
  <rdfs:isDefinedBy rdf:resource="&oa;"/>
  <rdfs:label xml:lang="en">SvgSelector</rdfs:label>
  <rdfs:subClassOf rdf:resource="&oa;Selector"/>
</owl:Class>

<rdfs:Class rdf:about="&ddo;Device"
    rdfs:label="Device">
  <rdfs:comment>A computerised device or gadget containing digital information, e.g. desktops, laptops, tablets and smart phones. Subclass of nie:DataSource, as a source of personal information.</rdfs:comment>
  <rdfs:subClassOf rdf:resource="&nie;DataSource"/>
</rdfs:Class>

<rdf:Property rdf:about="&nco;streetAddress"
    nrl:maxCardinality="1"
    rdfs:label="streetAddress">
  <rdfs:comment>The streed address. Inspired by the third part of the value of the 'ADR' property as defined in RFC 2426, sec. 3.2.1</rdfs:comment>
  <rdfs:domain rdf:resource="&nco;PostalAddress"/>
  <rdfs:range rdf:resource="&xsd;string"/>
</rdf:Property>

<rdf:Property rdf:about="&nexif;customRendered"
    rdfs:label="customRendered">
  <rdfs:subPropertyOf rdf:resource="http://www.kanzaki.com/ns/exif#customRendered"/>
  <rdfs:subPropertyOf rdf:resource="&nexif;pictTaking"/>
  <rdfs:comment>The use of special processing on image data, such as rendering geared to output. When special processing is performed, the reader is expected to disable or minimize any further processing.
tagNumber: 41985</rdfs:comment>
  <rdfs:domain rdf:resource="&nexif;Photo"/>
  <rdfs:range rdf:resource="&xsd;string"/>
</rdf:Property>

<rdf:Property rdf:about="&nexif;gpsDestDistanceRef"
    rdfs:label="gpsDestDistanceRef">
  <rdfs:subPropertyOf rdf:resource="http://www.kanzaki.com/ns/exif#gpsDestDistanceRef"/>
  <rdfs:subPropertyOf rdf:resource="&nexif;gpsInfo"/>
  <rdfs:comment>Indicates the unit used to express the distance to the destination point. 'K', 'M' and 'N' represent kilometers, miles and knots.
tagNumber: 25</rdfs:comment>
  <rdfs:domain rdf:resource="&nexif;Photo"/>
  <rdfs:range rdf:resource="&xsd;string"/>
</rdf:Property>

<rdf:Property rdf:about="&nexif;gainControl"
    rdfs:label="gainControl">
  <rdfs:subPropertyOf rdf:resource="http://www.kanzaki.com/ns/exif#gainControl"/>
  <rdfs:subPropertyOf rdf:resource="&nexif;pictTaking"/>
  <rdfs:comment>tagNumber: 41991
The degree of overall image gain adjustment.</rdfs:comment>
  <rdfs:domain rdf:resource="&nexif;Photo"/>
  <rdfs:range rdf:resource="&xsd;string"/>
</rdf:Property>

<rdf:Property rdf:about="&nexif;relatedImageFileFormat"
    rdfs:comment="Related image file format
tagNumber: 4096"
    rdfs:label="relatedImageFileFormat">
  <rdfs:subPropertyOf rdf:resource="http://www.kanzaki.com/ns/exif#relatedImageFileFormat"/>
  <rdfs:subPropertyOf rdf:resource="&nexif;interopInfo"/>
  <rdfs:domain rdf:resource="&nexif;Photo"/>
  <rdfs:range rdf:resource="&xsd;string"/>
</rdf:Property>

<rdfs:Class rdf:about="&ddo;GSM"
    rdfs:label="GSM">
  <rdfs:comment>Global System for Mobile Communications (GSM) is a second generation (2G) of standards for digital cellular networks.</rdfs:comment>
  <rdfs:subClassOf rdf:resource="&ddo;CellularNetwork"/>
</rdfs:Class>

<rdf:Property rdf:about="&ncal;bymonth"
    rdfs:label="bymonth">
  <rdfs:comment>Number of the month of the recurrence. Valid values are integers from 1 (January) to 12 (December). Defined in RFC 2445 sec. 4.3.10</rdfs:comment>
  <rdfs:domain rdf:resource="&ncal;RecurrenceRule"/>
  <rdfs:range rdf:resource="&xsd;integer"/>
</rdf:Property>

<rdfs:Class rdf:about="&drmo;Rule"
    rdfs:label="Rule">
  <rdfs:comment>Defines a declarative rule. A rule instance joins (drmo:isComposedOf) a number of antecedents (condition instances) with a number of consequent (actions)</rdfs:comment>
</rdfs:Class>

<rdfs:Class rdf:about="&ncal;TimeTransparency"
    rdfs:label="TimeTransparency">
  <rdfs:comment>Time transparency. Introduced to provide a way to express
the limited vocabulary for the values of ncal:transp property.
See documentation of ncal:transp for details.</rdfs:comment>
  <rdfs:subClassOf rdf:resource="&rdfs;Resource"/>
</rdfs:Class>

<rdf:Property rdf:about="&ncal;exdate"
    rdfs:label="exdate">
  <rdfs:comment>This property defines the list of date/time exceptions for a recurring calendar component. Inspired by RFC 2445 sec. 4.8.5.1</rdfs:comment>
  <rdfs:domain rdf:resource="&ncal;UnionOfEventJournalTimezoneTodo"/>
  <rdfs:range rdf:resource="&ncal;NcalDateTime"/>
</rdf:Property>

<rdf:Property rdf:about="&nexif;transferFunction"
    rdfs:label="transferFunction">
  <rdfs:subPropertyOf rdf:resource="http://www.kanzaki.com/ns/exif#transferFunction"/>
  <rdfs:subPropertyOf rdf:resource="&nexif;imageDataCharacter"/>
  <rdfs:comment>tagNumber: 301
A transfer function for the image, described in tabular style. Normally this tag is not necessary, since color space is specified in the color space information tag (ColorSpace).</rdfs:comment>
  <rdfs:domain rdf:resource="&nexif;Photo"/>
  <rdfs:range rdf:resource="&xsd;string"/>
</rdf:Property>

<rdf:Property rdf:about="&nco;representative"
    rdfs:label="representative">
  <rdfs:comment>An object that represent an object represented by this Contact. Usually this property is used to link a Contact to an organization, to a contact to the representative of this organization the user directly interacts with. An equivalent for the 'AGENT' property defined in RFC 2426 Sec. 3.5.4</rdfs:comment>
  <rdfs:domain rdf:resource="&nco;Contact"/>
  <rdfs:range rdf:resource="&nco;Contact"/>
</rdf:Property>

<rdf:Property rdf:about="&dcterms;identifier">
  <dcterms:description xml:lang="en">Recommended best practice is to identify the resource by means of a string conforming to a formal identification system. </dcterms:description>
  <dcterms:hasVersion rdf:resource="http://dublincore.org/usage/terms/history/#identifierT-001"/>
  <dcterms:issued rdf:datatype="&xsd;date">2008-01-14</dcterms:issued>
  <dcterms:modified rdf:datatype="&xsd;date">2008-01-14</dcterms:modified>
  <rdfs:comment xml:lang="en">An unambiguous reference to the resource within a given context.</rdfs:comment>
  <rdfs:isDefinedBy rdf:resource="&dcterms;"/>
  <rdfs:label xml:lang="en">Identifier</rdfs:label>
  <rdfs:range rdf:resource="&rdfs;Literal"/>
  <rdfs:subPropertyOf rdf:resource="&dc;identifier"/>
</rdf:Property>

<rdf:Property rdf:about="&nid3;albumTitle"
    rdfs:label="albumTitle">
  <rdfs:comment>TALB
The 'Album/Movie/Show title' frame is intended for the title of the recording(/source of sound) which the audio in the file is taken from.</rdfs:comment>
  <rdfs:domain rdf:resource="&nid3;ID3Audio"/>
  <rdfs:range rdf:resource="&xsd;string"/>
</rdf:Property>

<rdfs:Class rdf:about="&nfo;DeletedResource"
    rdfs:label="DeletedResource">
  <rdfs:comment>A file entity that has been deleted from the original source. Usually such entities are stored within various kinds of 'Trash' or 'Recycle Bin' folders.</rdfs:comment>
  <rdfs:subClassOf rdf:resource="&nfo;FileDataObject"/>
</rdfs:Class>

<rdf:Property rdf:about="&nexif;resolution"
    rdfs:label="resolution">
  <rdfs:comment>a rational number representing a resolution. Could be a subProperty of other general schema.</rdfs:comment>
  <rdfs:domain rdf:resource="&nexif;Photo"/>
  <rdfs:range rdf:resource="&xsd;float"/>
  <rdfs:subPropertyOf rdf:resource="http://www.kanzaki.com/ns/exif#resolution"/>
</rdf:Property>

<rdf:Property rdf:about="&rdf;value">
  <rdfs:comment xml:lang="en">Idiomatic property used for structured values.</rdfs:comment>
  <rdfs:domain rdf:resource="&rdfs;Resource"/>
  <rdfs:isDefinedBy rdf:resource="&rdf;"/>
  <rdfs:label xml:lang="en">value</rdfs:label>
  <rdfs:range rdf:resource="&rdfs;Resource"/>
</rdf:Property>

<rdf:Property rdf:about="&nfo;depicts"
    rdfs:comment="Relates an image to the information elements it depicts."
    rdfs:label="depicts">
  <nrl:inverseProperty rdf:resource="&nfo;depiction"/>
  <rdfs:domain rdf:resource="&nfo;Image"/>
  <rdfs:range rdf:resource="&rdfs;Resource"/>
</rdf:Property>

<rdf:Property rdf:about="&nao;hasSuperResource"
    rdfs:label="has Superresource">
  <nrl:inverseProperty rdf:resource="&nao;hasSubResource"/>
  <rdfs:comment>Defines a relationship between a resource and one or more super resources</rdfs:comment>
  <rdfs:range rdf:resource="&rdfs;Resource"/>
  <rdfs:subPropertyOf rdf:resource="&nao;isRelated"/>
</rdf:Property>

<nrl:DefiningProperty rdf:about="&nmm;series"
    rdfs:comment="series"
    rdfs:label="series">
  <nrl:inverseProperty rdf:resource="&nmm;hasEpisode"/>
  <nrl:maxCardinality rdf:datatype="&xsd;integer">1</nrl:maxCardinality>
  <rdf:type rdf:resource="&rdf;Property"/>
  <rdfs:domain rdf:resource="&nmm;TVShow"/>
  <rdfs:range rdf:resource="&nmm;TVSeries"/>
</nrl:DefiningProperty>

<rdfs:Class rdf:about="&nrl;Ontology"
    rdfs:comment="Represents a named graph having the role of an Ontology"
    rdfs:label="Ontology">
  <rdfs:subClassOf rdf:resource="&nrl;Schema"/>
</rdfs:Class>

<rdf:Property rdf:about="&dcon;caloriesExpended"
    rdfs:label="Calories Expended">
  <rdfs:comment>Specifies the amount of calories burnt while performing the activity.</rdfs:comment>
  <rdfs:domain rdf:resource="&dpo;Activity"/>
  <rdfs:range rdf:resource="&xsd;nonNegativeInteger"/>
  <rdfs:subPropertyOf rdf:resource="&dcon;hasContextAttribute"/>
</rdf:Property>

<rdf:Property rdf:about="&foaf;knows"
    rdfs:label="knows"
    ns:term_status="stable">
  <rdf:type rdf:resource="&owl;ObjectProperty"/>
  <rdfs:comment>A person known by this person (indicating some level of reciprocated interaction between the parties).</rdfs:comment>
  <rdfs:domain rdf:resource="&foaf;Person"/>
  <rdfs:isDefinedBy rdf:resource="&foaf;"/>
  <rdfs:range rdf:resource="&foaf;Person"/>
</rdf:Property>

<rdf:Property rdf:about="&dcterms;hasVersion">
  <rdfs:subPropertyOf rdf:resource="&dc;relation"/>
  <rdfs:subPropertyOf rdf:resource="&dcterms;relation"/>
  <dcterms:hasVersion rdf:resource="http://dublincore.org/usage/terms/history/#hasVersion-003"/>
  <dcterms:issued rdf:datatype="&xsd;date">2000-07-11</dcterms:issued>
  <dcterms:modified rdf:datatype="&xsd;date">2008-01-14</dcterms:modified>
  <rdfs:comment xml:lang="en">A related resource that is a version, edition, or adaptation of the described resource.</rdfs:comment>
  <rdfs:isDefinedBy rdf:resource="&dcterms;"/>
  <rdfs:label xml:lang="en">Has Version</rdfs:label>
  <scos:note xml:lang="en">This term is intended to be used with non-literal values as defined in the DCMI Abstract Model (http://dublincore.org/documents/abstract-model/).  As of December 2007, the DCMI Usage Board is seeking a way to express this intention with a formal range declaration.</scos:note>
</rdf:Property>

<rdf:Property rdf:about="&dcterms;hasPart">
  <rdfs:subPropertyOf rdf:resource="&dc;relation"/>
  <rdfs:subPropertyOf rdf:resource="&dcterms;relation"/>
  <dcterms:hasVersion rdf:resource="http://dublincore.org/usage/terms/history/#hasPart-003"/>
  <dcterms:issued rdf:datatype="&xsd;date">2000-07-11</dcterms:issued>
  <dcterms:modified rdf:datatype="&xsd;date">2008-01-14</dcterms:modified>
  <rdfs:comment xml:lang="en">A related resource that is included either physically or logically in the described resource.</rdfs:comment>
  <rdfs:isDefinedBy rdf:resource="&dcterms;"/>
  <rdfs:label xml:lang="en">Has Part</rdfs:label>
  <scos:note xml:lang="en">This term is intended to be used with non-literal values as defined in the DCMI Abstract Model (http://dublincore.org/documents/abstract-model/).  As of December 2007, the DCMI Usage Board is seeking a way to express this intention with a formal range declaration.</scos:note>
</rdf:Property>

<rdf:Property rdf:about="&nco;country"
    rdfs:label="country">
  <nrl:maxCardinality rdf:datatype="&xsd;integer">1</nrl:maxCardinality>
  <rdfs:comment>A part of an address specyfing the country. Inspired by the seventh part of the value of the 'ADR' property as defined in RFC 2426, sec. 3.2.1</rdfs:comment>
  <rdfs:domain rdf:resource="&nco;PostalAddress"/>
  <rdfs:range rdf:resource="&xsd;string"/>
</rdf:Property>

<rdf:Property rdf:about="&ncal;class"
    rdfs:label="class">
  <nrl:maxCardinality rdf:datatype="&xsd;integer">1</nrl:maxCardinality>
  <rdfs:comment>Defines the access classification for a calendar component. Inspired by RFC 2445 sec. 4.8.1.3 with the following reservations:  this property has limited vocabulary. Possible values are:  PUBLIC, PRIVATE and CONFIDENTIAL. The default is PUBLIC. Those values are expressed as instances of the AccessClassification class. The user may create his/her own if necessary.</rdfs:comment>
  <rdfs:domain rdf:resource="&ncal;UnionOfEventJournalTodo"/>
  <rdfs:range rdf:resource="&ncal;AccessClassification"/>
</rdf:Property>

<rdf:Property rdf:about="&nmo;plainTextMessageContent"
    rdfs:label="plainTextMessageContent">
  <rdfs:comment>Plain text representation of the body of the message. For multipart messages, all parts are concatenated into the value of this property. Attachments, whose mimeTypes are different from text/plain or message/rfc822 are considered separate DataObjects and are therefore not included in the value of this property.</rdfs:comment>
  <rdfs:domain rdf:resource="&nmo;Message"/>
  <rdfs:range rdf:resource="&xsd;string"/>
  <rdfs:subPropertyOf rdf:resource="&nie;plainTextContent"/>
</rdf:Property>

<rdf:Property rdf:about="&drmo;hasResourceType"
    rdfs:label="has Resource Type">
  <rdfs:comment>This property allows the user to define the resource type of the condition blocks. This is the RDF type that the triples look for when attempting to match conditions. For example, a rule triggered when a person is nearby, will have a condition of type pimo:Person.</rdfs:comment>
  <rdfs:domain rdf:resource="&drmo;Action"/>
  <rdfs:range rdf:resource="&rdfs;Resource"/>
</rdf:Property>

<rdf:Property rdf:about="&nexif;flashEnergy"
    rdfs:label="flashEnergy">
  <rdfs:subPropertyOf rdf:resource="http://www.kanzaki.com/ns/exif#flashEnergy"/>
  <rdfs:subPropertyOf rdf:resource="&nexif;pictTaking"/>
  <rdfs:comment>tagNumber: 41483
The strobe energy at the time the image is captured, as measured in Beam Candle Power Seconds (BCPS).</rdfs:comment>
  <rdfs:domain rdf:resource="&nexif;Photo"/>
  <rdfs:range rdf:resource="&xsd;float"/>
</rdf:Property>

<owl:Class rdf:about="&scos;ConceptScheme">
  <rdfs:isDefinedBy rdf:resource="http://www.w3.org/2004/02/skos/core"/>
  <rdfs:label xml:lang="en">Concept Scheme</rdfs:label>
  <owl:disjointWith rdf:resource="&scos;Concept"/>
  <scos:definition xml:lang="en">A set of concepts, optionally including statements about semantic relationships between those concepts.</scos:definition>
  <scos:example xml:lang="en">Thesauri, classification schemes, subject heading lists, taxonomies, 'folksonomies', and other types of controlled vocabulary are all examples of concept schemes. Concept schemes are also embedded in glossaries and terminologies.</scos:example>
  <scos:scopeNote xml:lang="en">A concept scheme may be defined to include concepts from different sources.</scos:scopeNote>
</owl:Class>

<rdfs:Class rdf:about="&dcon;Schedule"
    rdfs:label="Schedule">
  <rdfs:comment>The schedule aspect covers context elements relating to personal scheduling. Typically this includes elements managed by calendaring or task management tools.</rdfs:comment>
  <rdfs:subClassOf rdf:resource="&dcon;Aspect"/>
</rdfs:Class>

<rdf:Property rdf:about="&pimo;tagLabel"
    nrl:maxCardinality="1"
    nrl:minCardinality="1"
    rdfs:label="tag label">
  <rdfs:subPropertyOf rdf:resource="&nao;personalIdentifier"/>
  <rdfs:subPropertyOf rdf:resource="&nao;prefLabel"/>
  <rdfs:comment>The unique label of the tag. The label must be unique within the scope of one PersonalInformationModel. It is required and a subproperty of nao:prefLabel. It clarifies the use of nao:personalIdentifier by restricting the scope to tags. Semantically equivalent to skos:prefLabel, where uniqueness of labels is also recommended.</rdfs:comment>
  <rdfs:domain rdf:resource="&pimo;Tag"/>
  <rdfs:range rdf:resource="&rdfs;Literal"/>
</rdf:Property>

<nrl:RuleViewSpecification rdf:about="&pimo;RuleViewSpecificationGroundingClosure"
    rdfs:label="RuleViewSpecificationGroundingClosure"/>

<rdfs:Class rdf:about="&ncal;Todo"
    rdfs:label="Todo">
  <rdfs:subClassOf rdf:resource="&nie;InformationElement"/>
  <rdfs:subClassOf rdf:resource="&ncal;UnionOfAlarmEventFreebusyJournalTodo"/>
  <rdfs:subClassOf rdf:resource="&ncal;UnionOfAlarmEventFreebusyTodo"/>
  <rdfs:subClassOf rdf:resource="&ncal;UnionOfAlarmEventJournalTodo"/>
  <rdfs:subClassOf rdf:resource="&ncal;UnionOfAlarmEventTodo"/>
  <rdfs:subClassOf rdf:resource="&ncal;UnionOfEventFreebusyJournalTodo"/>
  <rdfs:subClassOf rdf:resource="&ncal;UnionOfEventJournalTimezoneTodo"/>
  <rdfs:subClassOf rdf:resource="&ncal;UnionOfEventJournalTodo"/>
  <rdfs:subClassOf rdf:resource="&ncal;UnionOfEventTodo"/>
  <rdfs:subClassOf rdf:resource="&ncal;UnionOfTimezoneObservanceEventFreebusyJournalTimezoneTodo"/>
  <rdfs:subClassOf rdf:resource="&ncal;UnionOfTimezoneObservanceEventFreebusyTimezoneTodo"/>
  <rdfs:subClassOf rdf:resource="&ncal;UnionOfTimezoneObservanceEventJournalTimezoneTodo"/>
  <rdfs:comment>Provide a grouping of calendar properties that describe a to-do.</rdfs:comment>
</rdfs:Class>

<rdf:Property rdf:about="&pimo;hasPart"
    rdfs:label="has part">
  <nrl:inverseProperty rdf:resource="&pimo;partOf"/>
  <rdfs:comment>The object is part of the subject. Like a page is part of a book or an engine is part of a car. You can make sub-properties of this to reflect more detailed relations. The semantics of this relations is the same as skos:narrowerPartitive</rdfs:comment>
  <rdfs:domain rdf:resource="&pimo;Thing"/>
  <rdfs:range rdf:resource="&pimo;Thing"/>
  <rdfs:subPropertyOf rdf:resource="&pimo;objectProperty"/>
</rdf:Property>

<owl:Class rdf:about="&oa;FragmentSelector">
  <rdfs:comment xml:lang="en">A Selector which describes the segment of interest in a representation, through the use of the fragment identifier component of a URI.

It is RECOMMENDED to use oa:FragmentSelector as the selector on a Specific Resource rather than annotating the fragment URI directly, in order to improve discoverability of annotation on the Source.

The oa:FragmentSelector MUST have exactly 1 rdf:value property, containing the fragment identifier component of a URI that describes the segment of interest in the resource, excluding the initial "#".

The Fragment Selector SHOULD have a dcterms:conformsTo relationship with the object being the specification that defines the syntax of the fragment, for instance &lt;http://tools.ietf.org/rfc/rfc3236&gt; for HTML fragments. </rdfs:comment>
  <rdfs:isDefinedBy rdf:resource="&oa;"/>
  <rdfs:label xml:lang="en">FragmentSelector</rdfs:label>
  <rdfs:subClassOf rdf:resource="&oa;Selector"/>
</owl:Class>

<rdfs:Class rdf:about="&ncal;UnionOfEventFreebusy"
    rdfs:label="UnionOfEventFreebusy">
  <rdfs:subClassOf rdf:resource="&ncal;UnionParentClass"/>
</rdfs:Class>

<rdf:Property rdf:about="&tmo;targetStartTime"
    nrl:maxCardinality="1"
    rdfs:label="targetStartTime">
  <rdfs:subPropertyOf rdf:resource="&tmo;startTime"/>
  <rdfs:subPropertyOf rdf:resource="&tmo;targetTime"/>
  <rdfs:domain rdf:resource="&tmo;Task"/>
  <rdfs:range rdf:resource="&xsd;dateTime"/>
</rdf:Property>

<rdf:Property rdf:about="&dcon;currentBrightness"
    rdfs:label="Current Brightness">
  <rdfs:comment>Refers to a pre-defined environmental brightness level characterising a context instance.</rdfs:comment>
  <rdfs:domain rdf:resource="&dcon;Environment"/>
  <rdfs:range rdf:resource="&dpo;Brightness"/>
  <rdfs:subPropertyOf rdf:resource="&dcon;hasContextElement"/>
</rdf:Property>

<rdfs:Class rdf:about="&ncal;TriggerRelation"
    rdfs:label="TriggerRelation">
  <rdfs:comment>The relation between the trigger and its parent calendar component. This class has been introduced to express the limited vocabulary for the ncal:related property. See the documentation for ncal:related for more details.</rdfs:comment>
  <rdfs:subClassOf rdf:resource="&rdfs;Resource"/>
</rdfs:Class>

<rdf:Property rdf:about="&nco;contributor"
    rdfs:label="contributor">
  <rdfs:subPropertyOf rdf:resource="&dc;contributor"/>
  <rdfs:subPropertyOf rdf:resource="&nao;contributor"/>
  <rdfs:comment>An entity responsible for making contributions to the content of the InformationElement.</rdfs:comment>
  <rdfs:domain rdf:resource="&nie;InformationElement"/>
  <rdfs:range rdf:resource="&nco;Contact"/>
</rdf:Property>

<rdf:Property rdf:about="&dpo;dayOfMonth"
    rdfs:label="Day of the Month">
  <rdfs:comment>A subproperty of dpo:value that defines an exact date/time value (a day in a month, i.e., between 1 and 31) such that it can classify as a dpo:TimePeriod instance.</rdfs:comment>
  <rdfs:domain rdf:resource="&dpo;TimePeriod"/>
  <rdfs:range rdf:resource="&xsd;integer"/>
  <rdfs:subPropertyOf rdf:resource="&dpo;value"/>
</rdf:Property>

<rdf:Property rdf:about="&nexif;lightSource"
    rdfs:label="lightSource">
  <rdfs:subPropertyOf rdf:resource="http://www.kanzaki.com/ns/exif#lightSource"/>
  <rdfs:subPropertyOf rdf:resource="&nexif;pictTaking"/>
  <rdfs:comment>tagNumber: 37384
Light source such as Daylight, Tungsten, Flash etc.</rdfs:comment>
  <rdfs:domain rdf:resource="&nexif;Photo"/>
  <rdfs:range rdf:resource="&xsd;string"/>
</rdf:Property>

<rdf:Property rdf:about="&nmo;headerName"
    nrl:maxCardinality="1"
    rdfs:comment="Name of the message header."
    rdfs:label="headerName">
  <rdfs:domain rdf:resource="&nmo;MessageHeader"/>
  <rdfs:range rdf:resource="&xsd;string"/>
</rdf:Property>

<rdf:Property rdf:about="&nexif;saturation"
    rdfs:label="saturation">
  <rdfs:subPropertyOf rdf:resource="http://www.kanzaki.com/ns/exif#saturation"/>
  <rdfs:subPropertyOf rdf:resource="&nexif;pictTaking"/>
  <rdfs:comment>The direction of saturation processing applied by the camera when the image was shot.
tagNumber: 41993</rdfs:comment>
  <rdfs:domain rdf:resource="&nexif;Photo"/>
  <rdfs:range rdf:resource="&xsd;string"/>
</rdf:Property>

<rdf:Property rdf:about="&cnt;standalone">
  <rdf:type rdf:resource="&owl;ObjectProperty"/>
  <rdfs:comment xml:lang="en">The standalone declaration in the XML declaration.</rdfs:comment>
  <rdfs:domain rdf:resource="&cnt;ContentAsXML"/>
  <rdfs:label xml:lang="en">XML standalone document declaration</rdfs:label>
  <rdfs:range rdf:resource="&rdfs;Literal"/>
</rdf:Property>

<rdf:Property rdf:about="&nfo;averageBitrate"
    rdfs:label="averageBitrate">
  <nrl:maxCardinality rdf:datatype="&xsd;integer">1</nrl:maxCardinality>
  <rdfs:comment>The average overall bitrate of a media container. (i.e. the size of the piece of media in bits, divided by it's duration expressed in seconds).</rdfs:comment>
  <rdfs:domain rdf:resource="&nfo;Media"/>
  <rdfs:range rdf:resource="&xsd;float"/>
  <rdfs:subPropertyOf rdf:resource="&nfo;rate"/>
</rdf:Property>

<rdf:Property rdf:about="&pimo;isInterestOf"
    rdfs:label="is interest Of">
  <rdfs:domain rdf:resource="&pimo;Tag"/>
  <rdfs:domain rdf:resource="&pimo;Topic"/>
  <nrl:inverseProperty rdf:resource="&pimo;hasInterest"/>
  <rdfs:comment>Links interests, as instances of pimo:Tag or a pimo:Topic (its subclass), to a person or a group.</rdfs:comment>
  <rdfs:range rdf:resource="&pimo;Agent"/>
  <rdfs:subPropertyOf rdf:resource="&pimo;isTagFor"/>
</rdf:Property>

<rdf:Property rdf:about="&nmo;primaryRecipient"
    rdfs:comment="deprecated in favor of primaryMessageRecipient"
    rdfs:label="primaryRecipient">
  <nao:deprecated rdf:datatype="&xsd;boolean">true</nao:deprecated>
  <rdfs:domain rdf:resource="&nmo;Message"/>
  <rdfs:range rdf:resource="&nco;Contact"/>
  <rdfs:subPropertyOf rdf:resource="&nmo;recipient"/>
</rdf:Property>

<rdfs:Class rdf:about="&nfo;OperatingSystem"
    rdfs:comment="An OperatingSystem"
    rdfs:label="OperatingSystem">
  <rdfs:subClassOf rdf:resource="&nfo;Software"/>
</rdfs:Class>

<rdf:Property rdf:about="&nfo;conflicts"
    rdfs:label="conflicts">
  <rdfs:comment>States that a piece of software is in conflict with another piece of software.</rdfs:comment>
  <rdfs:domain rdf:resource="&nfo;Software"/>
  <rdfs:range rdf:resource="&nfo;Software"/>
</rdf:Property>

<rdf:Property rdf:about="&pimo;containsLocation"
    rdfs:label="contains location">
  <nrl:inverseProperty rdf:resource="&pimo;locatedWithin"/>
  <rdfs:comment>The subject location contains the object location. For example, a building contains a room or a country contains a city.</rdfs:comment>
  <rdfs:domain rdf:resource="&pimo;Location"/>
  <rdfs:range rdf:resource="&pimo;Location"/>
  <rdfs:subPropertyOf rdf:resource="&pimo;hasPart"/>
</rdf:Property>

<rdfs:Class rdf:about="&nfo;MediaList"
    rdfs:comment="A file containing a list of media files.e.g. a playlist"
    rdfs:label="MediaList">
  <rdfs:subClassOf rdf:resource="&nie;InformationElement"/>
</rdfs:Class>

<rdf:Property rdf:about="&nfo;compressionType"
    rdfs:label="compressionType">
  <nrl:maxCardinality rdf:datatype="&xsd;integer">1</nrl:maxCardinality>
  <rdfs:comment>The type of the compression. Values include, 'lossy' and 'lossless'.</rdfs:comment>
  <rdfs:domain rdf:resource="&nfo;Media"/>
  <rdfs:range rdf:resource="&nfo;CompressionType"/>
</rdf:Property>

<rdf:Property rdf:about="http://www.w3.org/2003/01/geo/wgs84_pos#alt"
    nrl:maxCardinality="1">
  <rdfs:range rdf:resource="&xsd;float"/>
  <rdfs:subPropertyOf rdf:resource="&pimo;datatypeProperty"/>
</rdf:Property>

<rdf:Property rdf:about="&nid3;involvedPersonContact"
    rdfs:comment="An actual contact to the involved person."
    rdfs:label="involvedPersonContact">
  <rdfs:domain rdf:resource="&nid3;InvolvedPerson"/>
  <rdfs:range rdf:resource="&nco;Contact"/>
</rdf:Property>

<owl:Class rdf:about="&scos;Concept">
  <rdfs:label>Concept</rdfs:label>
  <rdfs:label xml:lang="en">Concept</rdfs:label>
  <rdfs:isDefinedBy rdf:resource="http://www.w3.org/2004/02/skos/core"/>
  <scos:definition xml:lang="en">An idea or notion; a unit of thought.</scos:definition>
</owl:Class>

<rdf:Property rdf:about="&dcterms;isFormatOf">
  <rdfs:subPropertyOf rdf:resource="&dc;relation"/>
  <rdfs:subPropertyOf rdf:resource="&dcterms;relation"/>
  <dcterms:hasVersion rdf:resource="http://dublincore.org/usage/terms/history/#isFormatOf-003"/>
  <dcterms:issued rdf:datatype="&xsd;date">2000-07-11</dcterms:issued>
  <dcterms:modified rdf:datatype="&xsd;date">2008-01-14</dcterms:modified>
  <rdfs:comment xml:lang="en">A related resource that is substantially the same as the described resource, but in another format.</rdfs:comment>
  <rdfs:isDefinedBy rdf:resource="&dcterms;"/>
  <rdfs:label xml:lang="en">Is Format Of</rdfs:label>
  <scos:note xml:lang="en">This term is intended to be used with non-literal values as defined in the DCMI Abstract Model (http://dublincore.org/documents/abstract-model/).  As of December 2007, the DCMI Usage Board is seeking a way to express this intention with a formal range declaration.</scos:note>
</rdf:Property>

<rdf:Property rdf:about="&pimo;hasMember"
    rdfs:comment="Defines which agents form part of a given person group."
    rdfs:label="has group member">
  <nrl:inverseProperty rdf:resource="&pimo;memberOf"/>
  <rdfs:domain rdf:resource="&pimo;PersonGroup"/>
  <rdfs:range rdf:resource="&pimo;Agent"/>
  <rdfs:subPropertyOf rdf:resource="&pimo;hasPart"/>
</rdf:Property>

<rdf:Property rdf:about="&nfo;hashAlgorithm"
    rdfs:label="hashAlgorithm">
  <nrl:maxCardinality rdf:datatype="&xsd;integer">1</nrl:maxCardinality>
  <rdfs:comment>Name of the algorithm used to compute the hash value. Examples might include CRC32, MD5, SHA, TTH etc.</rdfs:comment>
  <rdfs:domain rdf:resource="&nfo;FileHash"/>
  <rdfs:range rdf:resource="&xsd;string"/>
</rdf:Property>

<rdf:Property rdf:about="&dcterms;description">
  <dcterms:description xml:lang="en">Description may include but is not limited to: an abstract, a table of contents, a graphical representation, or a free-text account of the resource.</dcterms:description>
  <dcterms:hasVersion rdf:resource="http://dublincore.org/usage/terms/history/#descriptionT-001"/>
  <dcterms:issued rdf:datatype="&xsd;date">2008-01-14</dcterms:issued>
  <dcterms:modified rdf:datatype="&xsd;date">2008-01-14</dcterms:modified>
  <rdfs:comment xml:lang="en">An account of the resource.</rdfs:comment>
  <rdfs:isDefinedBy rdf:resource="&dcterms;"/>
  <rdfs:label xml:lang="en">Description</rdfs:label>
  <rdfs:subPropertyOf rdf:resource="&dc;description"/>
</rdf:Property>

<rdf:Property rdf:about="&nfo;programmingLanguage"
    rdfs:label="programmingLanguage">
  <rdfs:comment>Indicates the name of the programming language this source code file is written in. Examples might include 'C', 'C++', 'Java' etc.</rdfs:comment>
  <rdfs:domain rdf:resource="&nfo;SourceCode"/>
  <rdfs:range rdf:resource="&xsd;string"/>
</rdf:Property>

<rdfs:Class rdf:about="&ncal;UnionOfAlarmEventFreebusyJournalTodo"
    rdfs:label="UnionOfAlarmEventFreebusyJournalTodo">
  <rdfs:subClassOf rdf:resource="&ncal;UnionParentClass"/>
</rdfs:Class>

<rdf:Property rdf:about="&dpo;maxHumidity"
    rdfs:label="Maximum Humidity">
  <rdfs:comment>A subproperty of dpo:maxValue that defines an upperbound on the observed humidity value (as a percentage) such that it can classify as a dpo:WeatherCondition instance. It can be used in conjunction with dpo:minHumidity to state that specific instances of dpo:WeatherCondition have a pre-defined range of observable real-world humidity levels. In addition, they can also be used with various other weather conditions values and ranges to define complex weather condition types.</rdfs:comment>
  <rdfs:domain rdf:resource="&dpo;WeatherConditions"/>
  <rdfs:range rdf:resource="&xsd;nonNegativeInteger"/>
  <rdfs:subPropertyOf rdf:resource="&dpo;maxValue"/>
</rdf:Property>

<rdf:Property rdf:about="&pimo;isLocationOf"
    rdfs:comment="The subject location is the current location of the object."
    rdfs:label="is location of">
  <nrl:inverseProperty rdf:resource="&pimo;hasLocation"/>
  <rdfs:domain rdf:resource="&pimo;Location"/>
  <rdfs:range rdf:resource="&pimo;Thing"/>
  <rdfs:subPropertyOf rdf:resource="&pimo;isRelated"/>
</rdf:Property>

<rdf:Property rdf:about="&nco;requestedPresenceSubscriptionTo"
    rdfs:label="requestedPresenceSubscriptionTo">
  <rdfs:comment>Indicates that this IMAccount has requested a subscription to the presence information of the other IMAccount.</rdfs:comment>
  <rdfs:domain rdf:resource="&nco;IMAccount"/>
  <rdfs:range rdf:resource="&nco;IMAccount"/>
</rdf:Property>

<rdfs:Datatype rdf:about="&dcterms;RFC5646">
  <dcterms:description xml:lang="en">RFC 5646 obsoletes RFC 4646.</dcterms:description>
  <dcterms:hasVersion rdf:resource="http://dublincore.org/usage/terms/history/#RFC5646-001"/>
  <dcterms:issued rdf:datatype="&xsd;date">2010-10-11</dcterms:issued>
  <rdfs:comment xml:lang="en">The set of tags constructed according to RFC 5646 for the identification of languages.</rdfs:comment>
  <rdfs:isDefinedBy rdf:resource="&dcterms;"/>
  <rdfs:label xml:lang="en">RFC 5646</rdfs:label>
  <rdfs:seeAlso rdf:resource="http://www.ietf.org/rfc/rfc5646.txt"/>
</rdfs:Datatype>

<rdf:Property rdf:about="&nao;networkTrust"
    rdfs:label="network trust">
  <rdfs:comment>A network-derived trust value assigned to an agent, based on the shared direct trust values for the same agent, as set by participating agents in a network. Allowed values range from 0 (no trust) to 1 (very high trust).</rdfs:comment>
  <rdfs:domain rdf:resource="&pimo;Agent"/>
  <rdfs:range rdf:resource="&xsd;double"/>
  <rdfs:subPropertyOf rdf:resource="&nao;trustLevel"/>
</rdf:Property>

<rdf:Property rdf:about="&foaf;pastProject"
    rdfs:comment="A project this person has previously worked on."
    rdfs:label="past project"
    ns:term_status="testing">
  <rdf:type rdf:resource="&owl;ObjectProperty"/>
  <rdfs:domain rdf:resource="&foaf;Person"/>
  <rdfs:isDefinedBy rdf:resource="&foaf;"/>
  <rdfs:range rdf:resource="&owl;Thing"/>
</rdf:Property>

<rdf:Property rdf:about="&nso;excludes"
    rdfs:label="excludes">
  <rdfs:comment>Enables a 'blacklist' membership property for agents with respect to privacy preferences as defined by the PPO Ontology. This is useful for the logical computation of privacy preference exclusion, e.g. sharing an access space with a predefined agent group, except for agent x.</rdfs:comment>
  <rdfs:domain rdf:resource="&nso;AccessSpace"/>
  <rdfs:range rdf:resource="&pimo;Agent"/>
  <rdfs:subPropertyOf rdf:resource="http://vocab.deri.ie/ppo#hasAccessAgent"/>
</rdf:Property>

<rdfs:Class rdf:about="&tmo;TaskContainer"
    rdfs:label="TaskContainer">
  <rdfs:subClassOf rdf:resource="&pimo;Collection"/>
</rdfs:Class>

<rdfs:Class rdf:about="&nuao;Event"
    rdfs:label="event">
  <nao:userVisible rdf:datatype="&xsd;boolean">false</nao:userVisible>
  <rdfs:comment>An event: activity that have a specific start datetime and possibly a duration</rdfs:comment>
  <rdfs:subClassOf rdf:resource="&rdfs;Resource"/>
</rdfs:Class>

<rdf:Property rdf:about="&nexif;subSecTimeOriginal"
    rdfs:comment="tagNumber: 37521
DateTimeOriginal subseconds"
    rdfs:label="subSecTimeOriginal">
  <rdfs:subPropertyOf rdf:resource="http://www.kanzaki.com/ns/exif#subSecTimeOriginal"/>
  <rdfs:subPropertyOf rdf:resource="&nexif;dateAndOrTime"/>
  <rdfs:subPropertyOf rdf:resource="&nexif;subsecond"/>
  <rdfs:domain rdf:resource="&nexif;Photo"/>
  <rdfs:range rdf:resource="&xsd;string"/>
</rdf:Property>

<rdf:Property rdf:about="&dcon;currentTask"
    rdfs:label="Current Task">
  <rdfs:comment>Refers to an ongoing task characterising a context instance.</rdfs:comment>
  <rdfs:domain rdf:resource="&dcon;Schedule"/>
  <rdfs:range rdf:resource="&ncal;Todo"/>
  <rdfs:subPropertyOf rdf:resource="&dcon;hasContextElement"/>
</rdf:Property>

<rdfs:Class rdf:about="&nid3;SynchronizedTextElement"
    rdfs:label="SynchronizedTextElement">
  <rdfs:comment>An element of the synchronized text. It aggregates the actual text content, with the timestamp.</rdfs:comment>
  <rdfs:subClassOf rdf:resource="&rdfs;Resource"/>
</rdfs:Class>

<rdfs:Class rdf:about="&ncal;ParticipationStatus"
    rdfs:label="ParticipationStatus">
  <rdfs:comment>Participation Status. This class has been introduced to express the limited vocabulary of values for the ncal:partstat property. See the documentation of ncal:partstat for details.</rdfs:comment>
  <rdfs:subClassOf rdf:resource="&rdfs;Resource"/>
</rdfs:Class>

<rdf:Property rdf:about="&nid3;beatsPerMinute"
    rdfs:label="beatsPerMinute">
  <rdfs:comment>TBPM
The 'BPM' frame contains the number of beats per minute in the mainpart of the audio. The BPM is an integer and represented as a numerical string.</rdfs:comment>
  <rdfs:domain rdf:resource="&nid3;ID3Audio"/>
  <rdfs:range rdf:resource="&xsd;integer"/>
</rdf:Property>

<rdfs:Class rdf:about="&dctypes;Image">
  <dcam:memberOf rdf:resource="&dcterms;DCMIType"/>
  <dcterms:description xml:lang="en">Examples include images and photographs of physical objects, paintings, prints, drawings, other images and graphics, animations and moving pictures, film, diagrams, maps, musical notation.  Note that Image may include both electronic and physical representations.</dcterms:description>
  <dcterms:hasVersion rdf:resource="http://dublincore.org/usage/terms/history/#Image-004"/>
  <dcterms:issued rdf:datatype="&xsd;date">2000-07-11</dcterms:issued>
  <dcterms:modified rdf:datatype="&xsd;date">2008-01-14</dcterms:modified>
  <rdfs:comment xml:lang="en">A visual representation other than text.</rdfs:comment>
  <rdfs:isDefinedBy rdf:resource="&dctypes;"/>
  <rdfs:label xml:lang="en">Image</rdfs:label>
</rdfs:Class>

<rdf:Property rdf:about="&nid3;officialAudioSourceWebpage"
    rdfs:label="officialAudioSourceWebpage">
  <rdfs:comment>WOAS
The 'Official audio source webpage' frame is a URL pointing at the official webpage for the source of the audio file, e.g. a movie.</rdfs:comment>
  <rdfs:domain rdf:resource="&nid3;ID3Audio"/>
  <rdfs:range rdf:resource="&rdfs;Resource"/>
</rdf:Property>

<rdf:Property rdf:about="&nexif;exposureMode"
    rdfs:label="exposureMode">
  <rdfs:subPropertyOf rdf:resource="http://www.kanzaki.com/ns/exif#exposureMode"/>
  <rdfs:subPropertyOf rdf:resource="&nexif;pictTaking"/>
  <rdfs:comment>tagNumber: 41986
the exposure mode set when the image was shot. In auto-bracketing mode, the camera shoots a series of frames of the same scene at different exposure settings.</rdfs:comment>
  <rdfs:domain rdf:resource="&nexif;Photo"/>
  <rdfs:range rdf:resource="&xsd;string"/>
</rdf:Property>

<rdf:Property rdf:about="&nexif;gpsProcessingMethod"
    rdfs:label="gpsProcessingMethod">
  <rdfs:subPropertyOf rdf:resource="http://www.kanzaki.com/ns/exif#gpsProcessingMethod"/>
  <rdfs:subPropertyOf rdf:resource="&nexif;gpsInfo"/>
  <rdfs:comment>tagNumber: 27
A character string recording the name of the method used for location finding. The first byte indicates the character code used, and this is followed by the name of the method.</rdfs:comment>
  <rdfs:domain rdf:resource="&nexif;Photo"/>
  <rdfs:range rdf:resource="&xsd;string"/>
</rdf:Property>

<rdfs:Class rdf:about="&drmo;ResourceModified"
    rdfs:label="Resource Modified">
  <rdfs:comment>Describes a condition which is triggered by a modification to a PIM resource.</rdfs:comment>
  <rdfs:subClassOf rdf:resource="&drmo;Condition"/>
</rdfs:Class>

<rdf:Property rdf:about="&nid3;copyrightInformationURL"
    rdfs:label="copyrightInformationURL">
  <rdfs:comment>WCOP
The 'Copyright/Legal information' frame is a URL pointing at a webpage where the terms of use and ownership of the file is described.</rdfs:comment>
  <rdfs:domain rdf:resource="&nid3;ID3Audio"/>
  <rdfs:range rdf:resource="&rdfs;Resource"/>
</rdf:Property>

<rdf:Property rdf:about="&nao;prefLabel"
    rdfs:comment="A preferred label for a resource"
    rdfs:label="preferred label">
  <nrl:maxCardinality rdf:datatype="&xsd;nonNegativeInteger">1</nrl:maxCardinality>
  <rdfs:range rdf:resource="&rdfs;Literal"/>
  <rdfs:subPropertyOf rdf:resource="&rdfs;label"/>
</rdf:Property>

<rdf:Property rdf:about="&nco;imNickname"
    rdfs:comment="A nickname attached to a particular IM Account."
    rdfs:label="imNickname">
  <rdfs:domain rdf:resource="&nco;IMAccount"/>
  <rdfs:range rdf:resource="&xsd;string"/>
</rdf:Property>

<rdfs:Class rdf:about="&foaf;Organization"
    rdfs:comment="An organization."
    rdfs:label="Organization"
    ns:term_status="stable">
  <owl:disjointWith rdf:resource="&foaf;Document"/>
  <owl:disjointWith rdf:resource="&foaf;Person"/>
  <rdf:type rdf:resource="&owl;Class"/>
  <rdfs:isDefinedBy rdf:resource="&foaf;"/>
  <rdfs:subClassOf rdf:resource="&foaf;Agent"/>
</rdfs:Class>

<rdfs:Class rdf:about="&nmo;Message"
    rdfs:label="Message">
  <rdfs:comment>A message. Could be an email, instant messanging message, SMS message etc.</rdfs:comment>
  <rdfs:subClassOf rdf:resource="&nie;InformationElement"/>
</rdfs:Class>

<ncal:RecurrenceFrequency rdf:about="&ncal;monthly"
    rdfs:label="monthly"/>

<rdf:Property rdf:about="&ncal;locationAltRep"
    rdfs:label="locationAltRep">
  <rdfs:comment>Alternate representation of the event or todo location. 
Introduced to cover the ALTREP parameter of the LOCATION 
property. See documentation of ncal:location for details.</rdfs:comment>
  <rdfs:domain rdf:resource="&ncal;UnionOfEventTodo"/>
  <rdfs:range rdf:resource="&rdfs;Resource"/>
</rdf:Property>

<rdf:Property rdf:about="&nfo;totalSpace"
    rdfs:label="totalSpace">
  <nrl:maxCardinality rdf:datatype="&xsd;integer">1</nrl:maxCardinality>
  <rdfs:comment>Total storage space of the filesystem, which can be different from nie:contentSize because the latter includes filesystem format overhead.</rdfs:comment>
  <rdfs:domain rdf:resource="&nfo;Filesystem"/>
  <rdfs:range rdf:resource="&xsd;integer"/>
</rdf:Property>

<rdf:Property rdf:about="&nuao;totalFocusDuration"
    rdfs:label="total focus duration">
  <nrl:maxCardinality rdf:datatype="&xsd;nonNegativeInteger">1</nrl:maxCardinality>
  <rdfs:comment>The total amount of time a resource was in focus during a UsageEvent. This property should be used to 'compress' several FocusEvent instances into the essential information.</rdfs:comment>
  <rdfs:domain rdf:resource="&rdfs;UsageEvent"/>
  <rdfs:range rdf:resource="&xsd;duration"/>
</rdf:Property>

<rdf:Property rdf:about="&dpo;month"
    rdfs:label="Month">
  <rdfs:comment>A subproperty of dpo:value that defines an exact date/time value (a month, i.e., between 1 signifying January and 12 signifying December) such that it can classify as a dpo:TimePeriod instance.</rdfs:comment>
  <rdfs:domain rdf:resource="&dpo;TimePeriod"/>
  <rdfs:range rdf:resource="&xsd;integer"/>
  <rdfs:subPropertyOf rdf:resource="&dpo;value"/>
</rdf:Property>

<rdf:Property rdf:about="&dcterms;requires">
  <rdfs:subPropertyOf rdf:resource="&dc;relation"/>
  <rdfs:subPropertyOf rdf:resource="&dcterms;relation"/>
  <dcterms:hasVersion rdf:resource="http://dublincore.org/usage/terms/history/#requires-003"/>
  <dcterms:issued rdf:datatype="&xsd;date">2000-07-11</dcterms:issued>
  <dcterms:modified rdf:datatype="&xsd;date">2008-01-14</dcterms:modified>
  <rdfs:comment xml:lang="en">A related resource that is required by the described resource to support its function, delivery, or coherence.</rdfs:comment>
  <rdfs:isDefinedBy rdf:resource="&dcterms;"/>
  <rdfs:label xml:lang="en">Requires</rdfs:label>
  <scos:note xml:lang="en">This term is intended to be used with non-literal values as defined in the DCMI Abstract Model (http://dublincore.org/documents/abstract-model/).  As of December 2007, the DCMI Usage Board is seeking a way to express this intention with a formal range declaration.</scos:note>
</rdf:Property>

<rdf:Property rdf:about="&nao;endorsedBy"
    rdfs:label="endorsed by">
  <rdfs:comment>Signifies social endorsment of a resource by a specific agent. Endorsement includes social actions like favouriting, liking, voting for, starring a resource.</rdfs:comment>
  <rdfs:domain rdf:resource="&rdfs;Resource"/>
  <rdfs:range rdf:resource="&nao;Party"/>
</rdf:Property>

<rdfs:Class rdf:about="&nmo;MessageHeader"
    rdfs:comment="An arbitrary message header."
    rdfs:label="MessageHeader">
  <rdfs:subClassOf rdf:resource="&rdfs;Resource"/>
</rdfs:Class>

<rdfs:Class rdf:about="&dctypes;PhysicalObject">
  <dcam:memberOf rdf:resource="&dcterms;DCMIType"/>
  <dcterms:description xml:lang="en">Note that digital representations of, or surrogates for, these objects should use Image, Text or one of the other types.</dcterms:description>
  <dcterms:hasVersion rdf:resource="http://dublincore.org/usage/terms/history/#PhysicalObject-003"/>
  <dcterms:issued rdf:datatype="&xsd;date">2002-07-13</dcterms:issued>
  <dcterms:modified rdf:datatype="&xsd;date">2008-01-14</dcterms:modified>
  <rdfs:comment xml:lang="en">An inanimate, three-dimensional object or substance.</rdfs:comment>
  <rdfs:isDefinedBy rdf:resource="&dctypes;"/>
  <rdfs:label xml:lang="en">Physical Object</rdfs:label>
</rdfs:Class>

<rdf:Property rdf:about="&nco;nickname"
    rdfs:label="nickname">
  <rdfs:comment>A nickname of the Object represented by this Contact. This is an equivalent of the 'NICKNAME' property as defined in RFC 2426 Sec. 3.1.3.</rdfs:comment>
  <rdfs:domain rdf:resource="&nco;Name"/>
  <rdfs:range rdf:resource="&xsd;string"/>
</rdf:Property>

<rdf:Property rdf:about="&dcon;cloudcover"
    rdfs:label="Cloud Cover Value">
  <rdfs:comment>Registers an actual cloud cover percentage value element attribute to an active weather condition in the current context.</rdfs:comment>
  <rdfs:domain rdf:resource="&dpo;WeatherConditions"/>
  <rdfs:range rdf:resource="&xsd;nonNegativeInteger"/>
  <rdfs:subPropertyOf rdf:resource="&dcon;hasContextAttribute"/>
</rdf:Property>

<rdf:Property rdf:about="&dcon;voicesDetected"
    rdfs:label="Voices Detected">
  <rdfs:comment>Registers how many voices have been detected in the active environmental noise range in the current context.</rdfs:comment>
  <rdfs:domain rdf:resource="&dpo;Noise"/>
  <rdfs:range rdf:resource="&xsd;nonNegativeInteger"/>
  <rdfs:subPropertyOf rdf:resource="&dcon;hasContextAttribute"/>
</rdf:Property>

<rdf:Property rdf:about="&pimo;hasOrganizationMember"
    rdfs:label="organization has member">
  <nrl:inverseProperty rdf:resource="&pimo;isOrganizationMemberOf"/>
  <rdfs:comment>The subject organization has the object person or organization (Agent) as a member.</rdfs:comment>
  <rdfs:domain rdf:resource="&pimo;Organization"/>
  <rdfs:range rdf:resource="&pimo;Agent"/>
  <rdfs:subPropertyOf rdf:resource="&pimo;hasPart"/>
</rdf:Property>

<rdf:Property rdf:about="&nco;imStatus"
    rdfs:label="imStatus">
  <nrl:maxCardinality rdf:datatype="&xsd;integer">1</nrl:maxCardinality>
  <rdfs:comment>Current status of the given IM account. When this property is set, the nco:imStatusType should also always be set. Applications should attempt to parse this property to determine the presence, only falling back to the nco:imStatusType property in the case that this property's value is unrecognised. Values for this property may include 'available', 'offline', 'busy' etc. The exact choice of them is unspecified, although it is recommended to follow the guidance of the Telepathy project when choosing a string identifier http://telepathy.freedesktop.org/spec/Connection_Interface_Simple_Presence.html#description</rdfs:comment>
  <rdfs:domain rdf:resource="&nco;IMAccount"/>
  <rdfs:range rdf:resource="&xsd;string"/>
</rdf:Property>

<rdfs:Class rdf:about="&tmo;AbilityCarrier"
    protege:role="abstract"
    rdfs:label="AbilityCarrier">
  <rdfs:comment>AbilityCarrier is an abstract class which circumferences all entities which can take action or which are somehow involved in tasks.
This is in other task conceptualizations rather named "actor". But here it is named AbilityCarrier because it is not neccessarily "active".

The execution of a task relies on certain abilities. The abstract concept of
Abilitiy_Carriers circumference all those more concrete concepts
of which one can think of while working on tasks. Using this abstract
class enables to substitute such Ability Carrier's in the process of
generating patterns from task instances and vice versa in the process of
instantiating task instances from patterns without violating the schema.
With this attribute, a series of ability carrying entities (Person, Role,
Skill, OrganizationalUnit, InformalDescribedAbility)
and the role of involvement (required, request, used) is enabled. The role
hereby allows specifying how the ability carrying entity is or was
involved.</rdfs:comment>
  <rdfs:subClassOf rdf:resource="&rdfs;Resource"/>
</rdfs:Class>

<rdfs:Class rdf:about="&nfo;Audio"
    rdfs:comment="A file containing audio content"
    rdfs:label="Audio">
  <rdfs:subClassOf rdf:resource="&nfo;Media"/>
</rdfs:Class>

<nrl:GraphView rdf:about="&pimo;GroundingClosure"
    rdfs:label="GroundingClosure"/>

<rdf:Property rdf:about="&nfo;sideChannels"
    rdfs:comment="Number of side channels"
    rdfs:label="sideChannels">
  <nrl:maxCardinality rdf:datatype="&xsd;integer">1</nrl:maxCardinality>
  <rdfs:range rdf:resource="&xsd;integer"/>
  <rdfs:subPropertyOf rdf:resource="&nfo;channels"/>
</rdf:Property>

<rdfs:Class rdf:about="&nrl;TransitiveProperty"
    rdfs:comment="A marker class to identify transitive properties"
    rdfs:label="TransitiveProperty">
  <rdfs:subClassOf rdf:resource="&rdfs;Resource"/>
</rdfs:Class>

<rdf:Property rdf:about="&nmo;secondaryMessageRecipient"
    rdfs:label="secondaryRecipient">
  <rdfs:comment>A superproperty for all "additional" recipients of a message.</rdfs:comment>
  <rdfs:domain rdf:resource="&nmo;Message"/>
  <rdfs:range rdf:resource="&nco;ContactMedium"/>
  <rdfs:subPropertyOf rdf:resource="&nmo;messageRecipient"/>
</rdf:Property>

<rdf:Property rdf:about="&nexif;contrast"
    rdfs:label="contrast">
  <rdfs:subPropertyOf rdf:resource="http://www.kanzaki.com/ns/exif#contrast"/>
  <rdfs:subPropertyOf rdf:resource="&nexif;pictTaking"/>
  <rdfs:comment>tagNumber: 41992
The direction of contrast processing applied by the camera when the image was shot.</rdfs:comment>
  <rdfs:domain rdf:resource="&nexif;Photo"/>
  <rdfs:range rdf:resource="&xsd;string"/>
</rdf:Property>

<rdfs:Class rdf:about="&dplo;Message"
    rdfs:label="Message">
  <rdfs:comment>A livepost consisting of a textual message posted by either a user, or a contact, as defined by further subclasses.</rdfs:comment>
  <rdfs:subClassOf rdf:resource="&dplo;LivePost"/>
</rdfs:Class>

<rdf:Property rdf:about="&drmo;hasNegation"
    rdfs:comment="A condition block can be negated with this property."
    rdfs:label="has negation">
  <nrl:maxCardinality rdf:datatype="&xsd;nonNegativeInteger">1</nrl:maxCardinality>
  <rdfs:domain rdf:resource="&drmo;Condition"/>
  <rdfs:range rdf:resource="&xsd;boolean"/>
</rdf:Property>

<rdfs:Class rdf:about="&nmm;TVShow"
    rdfs:comment="A TV Show"
    rdfs:label="tv show">
  <rdfs:subClassOf rdf:resource="&nfo;Video"/>
</rdfs:Class>

<ncal:AttendeeRole rdf:about="&ncal;nonParticipantRole"
    rdfs:label="nonParticipantRole"/>

<rdfs:Class rdf:about="&ncal;CalendarUserType"
    rdfs:label="CalendarUserType">
  <rdfs:comment>A calendar user type. This class has been introduced to express the limited vocabulary for the ncal:cutype property. See documentation of ncal:cutype for details.</rdfs:comment>
  <rdfs:subClassOf rdf:resource="&rdfs;Resource"/>
</rdfs:Class>

<rdf:Property rdf:about="&nexif;pimContrast"
    rdfs:comment="tagNumber: 9
Contrast info for print image matching"
    rdfs:label="pimContrast">
  <rdfs:subPropertyOf rdf:resource="http://www.kanzaki.com/ns/exif#pimContrast"/>
  <rdfs:subPropertyOf rdf:resource="&nexif;pimInfo"/>
  <rdfs:domain rdf:resource="&nexif;Photo"/>
  <rdfs:range rdf:resource="&xsd;string"/>
</rdf:Property>

<rdf:Property rdf:about="&nexif;yCbCrPositioning"
    rdfs:label="yCbCrPositioning">
  <rdfs:subPropertyOf rdf:resource="http://www.kanzaki.com/ns/exif#yCbCrPositioning"/>
  <rdfs:subPropertyOf rdf:resource="&nexif;imageDataStruct"/>
  <rdfs:comment>The position of chrominance components in relation to the luminance component. This field is designated only for JPEG compressed data or uncompressed YCbCr data.
tagNumber: 531</rdfs:comment>
  <rdfs:domain rdf:resource="&nexif;Photo"/>
  <rdfs:range rdf:resource="&xsd;string"/>
</rdf:Property>

<rdf:Property rdf:about="&nao;hasSubResource"
    rdfs:label="has Subresource">
  <nrl:inverseProperty rdf:resource="&nao;hasSuperResource"/>
  <rdfs:comment>Defines a relationship between a resource and one or more sub resources. Descriptions of sub-resources are only interpretable when the super-resource exists. Deleting a super-resource should then also delete all sub-resources, and transferring a super-resource (for example, sending it to another user) must also include the sub-resource.</rdfs:comment>
  <rdfs:range rdf:resource="&rdfs;Resource"/>
  <rdfs:subPropertyOf rdf:resource="&nao;isRelated"/>
</rdf:Property>

<rdf:Property rdf:about="&dpo;value"
    rdfs:label="Value">
  <rdfs:comment>A generic property that assign a quantifiable value to a presence component. Minimum and maximum values are provided as its subproperties. Various subproperties of different types of values are also provided and apply to specific types of presence components.</rdfs:comment>
  <rdfs:domain rdf:resource="&dpo;QuantifiableComponent"/>
</rdf:Property>

<rdf:Property rdf:about="&foaf;member"
    rdfs:comment="Indicates a member of a Group"
    rdfs:label="member"
    ns:term_status="stable">
  <rdf:type rdf:resource="&owl;ObjectProperty"/>
  <rdfs:domain rdf:resource="&foaf;Group"/>
  <rdfs:isDefinedBy rdf:resource="&foaf;"/>
  <rdfs:range rdf:resource="&foaf;Agent"/>
</rdf:Property>

<rdfs:Class rdf:about="&dcterms;MethodOfInstruction">
  <dcterms:hasVersion rdf:resource="http://dublincore.org/usage/terms/history/#MethodOfInstruction-001"/>
  <dcterms:issued rdf:datatype="&xsd;date">2008-01-14</dcterms:issued>
  <rdfs:comment xml:lang="en">A process that is used to engender knowledge, attitudes, and skills.</rdfs:comment>
  <rdfs:isDefinedBy rdf:resource="&dcterms;"/>
  <rdfs:label xml:lang="en">Method of Instruction</rdfs:label>
</rdfs:Class>

<rdfs:Class rdf:about="&ncal;NcalDateTime"
    rdfs:label="NcalDateTime">
  <rdfs:subClassOf rdf:resource="&ncal;NcalTimeEntity"/>
</rdfs:Class>

<rdf:Property rdf:about="&scos;broader">
  <rdf:type rdf:resource="&owl;ObjectProperty"/>
  <rdfs:comment xml:lang="en">Broader concepts are typically rendered as parents in a concept hierarchy (tree).</rdfs:comment>
  <rdfs:isDefinedBy rdf:resource="http://www.w3.org/2004/02/skos/core"/>
  <rdfs:label xml:lang="en">has broader</rdfs:label>
  <rdfs:subPropertyOf rdf:resource="&scos;broaderTransitive"/>
  <owl:inverseOf rdf:resource="&scos;narrower"/>
  <scos:definition xml:lang="en">Relates a concept to a concept that is more general in meaning.</scos:definition>
  <scos:scopeNote xml:lang="en">By convention, skos:broader is only used to assert an immediate (i.e. direct) hierarchical link between two conceptual resources.</scos:scopeNote>
</rdf:Property>

<rdf:Property rdf:about="&nid3;textContentType"
    rdfs:label="textContentType">
  <rdfs:comment>Content type: 
$00     is other 
$01     is lyrics
$02     is text transcription
$03     is movement/part name (e.g. "Adagio")
$04     is events (e.g. "Don Quijote enters the stage")
$05     is chord (e.g. "Bb F Fsus")
$06     is trivia/'pop up' information</rdfs:comment>
  <rdfs:domain rdf:resource="&nid3;SynchronizedText"/>
  <rdfs:range rdf:resource="&xsd;string"/>
</rdf:Property>

<rdf:Property rdf:about="&nid3;conductor"
    rdfs:label="conductor">
  <rdfs:comment>TPE3
The 'Conductor' frame is used for the name of the conductor.</rdfs:comment>
  <rdfs:domain rdf:resource="&nid3;ID3Audio"/>
  <rdfs:range rdf:resource="&nco;Contact"/>
  <rdfs:subPropertyOf rdf:resource="&nco;contributor"/>
</rdf:Property>

<rdf:Property rdf:about="&tmo;attachment"
    rdfs:label="attachment">
  <nrl:inverseProperty rdf:resource="&tmo;attachmentTask"/>
  <rdfs:comment>connects a Task with an Attachment object. Attachments are associations of Things.</rdfs:comment>
  <rdfs:domain rdf:resource="&tmo;Task"/>
  <rdfs:range rdf:resource="&tmo;Attachment"/>
</rdf:Property>

<rdfs:Class rdf:about="&ncal;Weekday"
    rdfs:label="Weekday">
  <rdfs:comment>Day of the week. This class has been created to provide the limited vocabulary for ncal:byday property. See the documentation for ncal:byday for details.</rdfs:comment>
  <rdfs:subClassOf rdf:resource="&rdfs;Resource"/>
</rdfs:Class>

<rdf:Property rdf:about="&dcon;hasLiveContext"
    rdfs:label="has Live Context">
  <rdfs:comment>Links the special live context representation instance to the user. Past live contexts are logged through the use of the DUHO ontology.</rdfs:comment>
  <rdfs:domain rdf:resource="&pimo;Agent"/>
  <rdfs:range rdf:resource="&dcon;LiveContext"/>
</rdf:Property>

<tmo:Importance rdf:about="&tmo;TMO_Instance_Importance_03"
    rdfs:label="TMO_Instance_Importance_03"/>

<rdf:Property rdf:about="&nfo;colorCount"
    rdfs:comment="The number of colors used/available in a raster image."
    rdfs:label="color count">
  <nrl:maxCardinality rdf:datatype="&xsd;integer">1</nrl:maxCardinality>
  <rdfs:domain rdf:resource="&nfo;RasterImage"/>
  <rdfs:range rdf:resource="&xsd;integer"/>
</rdf:Property>

<rdf:Property rdf:about="&pimo;hasLocalNamespace"
    rdfs:label="local namespace">
  <rdfs:comment>The local namespace of this user using the semdesk uri scheme, based on the Local Identifier of the user. Example semdesk://bob@/things/. See http://dev.nepomuk.semanticdesktop.org/repos/trunk/doc/2008_09_semdeskurischeme/index.html</rdfs:comment>
  <rdfs:domain rdf:resource="&pimo;PersonalInformationModel"/>
  <rdfs:range rdf:resource="&rdfs;Literal"/>
</rdf:Property>

<ncal:FreebusyType rdf:about="&ncal;freeFreebusyType"
    rdfs:label="freeFreebusyType"/>

<rdf:Property rdf:about="&dcterms;isRequiredBy">
  <rdfs:subPropertyOf rdf:resource="&dc;relation"/>
  <rdfs:subPropertyOf rdf:resource="&dcterms;relation"/>
  <dcterms:hasVersion rdf:resource="http://dublincore.org/usage/terms/history/#isRequiredBy-003"/>
  <dcterms:issued rdf:datatype="&xsd;date">2000-07-11</dcterms:issued>
  <dcterms:modified rdf:datatype="&xsd;date">2008-01-14</dcterms:modified>
  <rdfs:comment xml:lang="en">A related resource that requires the described resource to support its function, delivery, or coherence.</rdfs:comment>
  <rdfs:isDefinedBy rdf:resource="&dcterms;"/>
  <rdfs:label xml:lang="en">Is Required By</rdfs:label>
  <scos:note xml:lang="en">This term is intended to be used with non-literal values as defined in the DCMI Abstract Model (http://dublincore.org/documents/abstract-model/).  As of December 2007, the DCMI Usage Board is seeking a way to express this intention with a formal range declaration.</scos:note>
</rdf:Property>

<rdf:Property rdf:about="&nao;trustLevel"
    rdfs:label="trust level">
  <rdfs:comment>A generalised trust level assigned to an agent, based on a combination of direct and network trust values it possesses. Allowed values range from 0 (no trust) to 1 (very high trust).</rdfs:comment>
  <rdfs:domain rdf:resource="&pimo;Agent"/>
  <rdfs:range rdf:resource="&xsd;double"/>
  <rdfs:subPropertyOf rdf:resource="&nao;annotation"/>
</rdf:Property>

<rdf:Property rdf:about="&ncal;range"
    rdfs:label="range">
  <nrl:maxCardinality rdf:datatype="&xsd;integer">1</nrl:maxCardinality>
  <rdfs:comment>To specify the effective range of recurrence instances from the instance specified by the recurrence identifier specified by the property. It is intended to express the RANGE parameter specified in RFC 2445 sec. 4.2.13. The set of possible values for this property is limited. See also the documentation for ncal:recurrenceId for more details.</rdfs:comment>
  <rdfs:domain rdf:resource="&ncal;RecurrenceIdentifier"/>
  <rdfs:range rdf:resource="&ncal;RecurrenceIdentifierRange"/>
</rdf:Property>

<rdf:Property rdf:about="&tmo;targetTime"
    nrl:maxCardinality="1"
    rdfs:label="targetTime">
  <rdfs:range rdf:resource="&xsd;dateTime"/>
  <rdfs:subPropertyOf rdf:resource="&tmo;dateTime"/>
</rdf:Property>

<rdf:Property rdf:about="&nao;pluralPrefLabel"
    rdfs:comment="The plural form of the preferred label for a resource"
    rdfs:label="preferred label plural form">
  <nrl:maxCardinality rdf:datatype="&xsd;nonNegativeInteger">1</nrl:maxCardinality>
  <rdfs:range rdf:resource="&rdfs;Literal"/>
  <rdfs:subPropertyOf rdf:resource="&rdfs;label"/>
</rdf:Property>

<rdf:Property rdf:about="&foaf;phone"
    rdfs:label="phone"
    ns:term_status="testing">
  <rdf:type rdf:resource="&owl;ObjectProperty"/>
  <rdfs:comment>A phone,  specified using fully qualified tel: URI scheme (refs: http://www.w3.org/Addressing/schemes.html#tel).</rdfs:comment>
  <rdfs:isDefinedBy rdf:resource="&foaf;"/>
</rdf:Property>

<rdf:Property rdf:about="&nco;hasPostalAddress"
    rdfs:label="hasPostalAddress">
  <rdfs:comment>The default Address for a Contact. An equivalent of the 'ADR' property as defined in RFC 2426 Sec. 3.2.1.</rdfs:comment>
  <rdfs:domain rdf:resource="&nco;Role"/>
  <rdfs:range rdf:resource="&nco;PostalAddress"/>
  <rdfs:subPropertyOf rdf:resource="&nco;hasContactMedium"/>
</rdf:Property>

<rdf:Property rdf:about="&nfo;channels"
    rdfs:label="channels">
  <nrl:maxCardinality rdf:datatype="&xsd;integer">1</nrl:maxCardinality>
  <rdfs:comment>Number of channels. This property is to be used directly if no detailed information is necessary. Otherwise use more detailed subproperties.</rdfs:comment>
  <rdfs:domain rdf:resource="&nfo;Audio"/>
  <rdfs:range rdf:resource="&xsd;integer"/>
</rdf:Property>

<rdf:Property rdf:about="&dcon;lastActive"
    rdfs:label="Last Active">
  <rdfs:comment>The last date and time for which user activity was detected on a device. This could consist of the last movement detected from the cursor/keyboard/touch screen and other device input mechanisms, as well as the last call recorded for voice communication-enabled devices.</rdfs:comment>
  <rdfs:domain rdf:resource="&nie;DataSource"/>
  <rdfs:range rdf:resource="&xsd;dateTime"/>
</rdf:Property>

<rdf:Property rdf:about="&tmo;indexPosition"
    nrl:maxCardinality="1"
    rdfs:label="indexPosition">
  <rdfs:domain rdf:resource="&tmo;Task"/>
  <rdfs:range rdf:resource="&rdfs;Literal"/>
</rdf:Property>

<rdf:Property rdf:about="&nexif;subjectDistanceRange"
    rdfs:label="subjectDistanceRange">
  <rdfs:subPropertyOf rdf:resource="http://www.kanzaki.com/ns/exif#subjectDistanceRange"/>
  <rdfs:subPropertyOf rdf:resource="&nexif;pictTaking"/>
  <rdfs:comment>The distance to the subject, such as Macro, Close View or Distant View.
tagNumber: 41996</rdfs:comment>
  <rdfs:domain rdf:resource="&nexif;Photo"/>
  <rdfs:range rdf:resource="&xsd;string"/>
</rdf:Property>

<rdf:Property rdf:about="&scos;example">
  <rdf:type rdf:resource="&owl;AnnotationProperty"/>
  <rdfs:isDefinedBy rdf:resource="http://www.w3.org/2004/02/skos/core"/>
  <rdfs:label xml:lang="en">example</rdfs:label>
  <rdfs:subPropertyOf rdf:resource="&scos;note"/>
  <scos:definition xml:lang="en">An example of the use of a concept.</scos:definition>
</rdf:Property>

<rdf:Property rdf:about="&foaf;dnaChecksum"
    rdfs:comment="A checksum for the DNA of some thing. Joke."
    rdfs:label="DNA checksum"
    ns:term_status="archaic">
  <rdf:type rdf:resource="&owl;DatatypeProperty"/>
  <rdfs:isDefinedBy rdf:resource="&foaf;"/>
  <rdfs:range rdf:resource="&rdfs;Literal"/>
</rdf:Property>

<rdf:Property rdf:about="&ncal;dtstart"
    rdfs:label="dtstart">
  <nrl:maxCardinality rdf:datatype="&xsd;integer">1</nrl:maxCardinality>
  <rdfs:comment>This property specifies when the calendar component begins. Inspired by RFC 2445 sec. 4.8.2.4</rdfs:comment>
  <rdfs:domain rdf:resource="&ncal;UnionOfTimezoneObservanceEventFreebusyTimezoneTodo"/>
  <rdfs:range rdf:resource="&ncal;NcalDateTime"/>
</rdf:Property>

<rdf:Property rdf:about="&nexif;imageDataStruct"
    rdfs:comment="An attribute relating to image data structure"
    rdfs:label="imageDataStruct">
  <rdfs:subPropertyOf rdf:resource="http://www.kanzaki.com/ns/exif#imageDataStruct"/>
  <rdfs:subPropertyOf rdf:resource="&nexif;exifAttribute"/>
  <rdfs:domain rdf:resource="&nexif;Photo"/>
  <rdfs:range rdf:resource="&xsd;string"/>
</rdf:Property>

<rdf:Property rdf:about="&nie;disclaimer"
    rdfs:comment="A disclaimer"
    rdfs:label="disclaimer">
  <rdfs:range rdf:resource="&xsd;string"/>
  <rdfs:subPropertyOf rdf:resource="&nie;legal"/>
</rdf:Property>

<rdf:Property rdf:about="&nexif;gpsTrack"
    rdfs:label="gpsTrack">
  <rdfs:subPropertyOf rdf:resource="http://www.kanzaki.com/ns/exif#gpsTrack"/>
  <rdfs:subPropertyOf rdf:resource="&nexif;gpsInfo"/>
  <rdfs:comment>The direction of GPS receiver movement. The range of values is from 0.00 to 359.99.
tagNumber: 15</rdfs:comment>
  <rdfs:domain rdf:resource="&nexif;Photo"/>
  <rdfs:range rdf:resource="&xsd;string"/>
</rdf:Property>

<nco:IMStatusType rdf:about="&nco;IMStatusTypeHidden"
    rdfs:label="hidden"/>

<rdf:Property rdf:about="&dcterms;alternative">
  <rdfs:subPropertyOf rdf:resource="&dc;title"/>
  <rdfs:subPropertyOf rdf:resource="&dcterms;title"/>
  <dcterms:description xml:lang="en">The distinction between titles and alternative titles is application-specific.</dcterms:description>
  <dcterms:hasVersion rdf:resource="http://dublincore.org/usage/terms/history/#alternative-003"/>
  <dcterms:issued rdf:datatype="&xsd;date">2000-07-11</dcterms:issued>
  <dcterms:modified rdf:datatype="&xsd;date">2010-10-11</dcterms:modified>
  <rdfs:comment xml:lang="en">An alternative name for the resource.</rdfs:comment>
  <rdfs:isDefinedBy rdf:resource="&dcterms;"/>
  <rdfs:label xml:lang="en">Alternative Title</rdfs:label>
  <rdfs:range rdf:resource="&rdfs;Literal"/>
</rdf:Property>

<rdfs:Class rdf:about="&nrl;SymmetricProperty"
    rdfs:comment="A marker class to identify symmetric properties"
    rdfs:label="SymmetricProperty">
  <rdfs:subClassOf rdf:resource="&rdfs;Resource"/>
</rdfs:Class>

<ncal:EventStatus rdf:about="&ncal;confirmedStatus"
    rdfs:label="confirmedStatus"/>

<rdfs:Class rdf:about="&dcterms;LicenseDocument">
  <dcterms:hasVersion rdf:resource="http://dublincore.org/usage/terms/history/#LicenseDocument-001"/>
  <dcterms:issued rdf:datatype="&xsd;date">2008-01-14</dcterms:issued>
  <rdfs:comment xml:lang="en">A legal document giving official permission to do something with a Resource.</rdfs:comment>
  <rdfs:isDefinedBy rdf:resource="&dcterms;"/>
  <rdfs:label xml:lang="en">License Document</rdfs:label>
  <rdfs:subClassOf rdf:resource="&dcterms;RightsStatement"/>
</rdfs:Class>

<rdf:Property rdf:about="&pimo;isDefinedBy"
    nrl:maxCardinality="1"
    nrl:minCardinality="1"
    rdfs:label="is defined by">
  <rdfs:comment>Each element in a PIMO must be connected to the PIMO, to be able to track multiple PIMOs in a distributed scenario. Also, this is the way to find the user that this Thing belongs to.</rdfs:comment>
  <rdfs:domain rdf:resource="&pimo;ClassOrThingOrPropertyOrAssociation"/>
  <rdfs:range rdf:resource="&pimo;PersonalInformationModel"/>
  <rdfs:subPropertyOf rdf:resource="&nao;hasDataGraph"/>
</rdf:Property>

<nrl:TransitiveProperty rdf:about="&pimo;hasOtherConceptualization"
    rdfs:label="has other conceptualization">
  <rdfs:subPropertyOf rdf:resource="&pimo;occurrence"/>
  <rdfs:subPropertyOf rdf:resource="&rdfs;subClassOf"/>
  <rdf:type rdf:resource="&rdf;Property"/>
  <rdfs:comment>Short: hasOtherRepresentation points from a Class in your PIMO to a class in a domain ontology that represents the same class. Longer: hasOtherConceptualization means that a class of real world objects O represented by a concept C1 in the ontology has additional conceptualizations (as classes C2-Cn in different domain ontologies).
This means: IF (O_i is conceptialized by C_j in Ontology_k) AND (O_l is conceptialized by C_m in Ontology_n) THEN (O_i and O_l is the same set of objects).
hasOtherConceptualization is an transitive relation, but not equivalent (not symmetric nor reflexive).</rdfs:comment>
  <rdfs:domain rdf:resource="&rdfs;Class"/>
  <rdfs:range rdf:resource="&rdfs;Class"/>
</nrl:TransitiveProperty>

<rdfs:Class rdf:about="&nfo;Presentation"
    rdfs:label="Presentation">
  <rdfs:comment>A Presentation made by some presentation software (Corel Presentations, OpenOffice Impress, MS Powerpoint etc.)</rdfs:comment>
  <rdfs:subClassOf rdf:resource="&nfo;Document"/>
</rdfs:Class>

<rdf:Property rdf:about="&nexif;gpsDestBearingRef"
    rdfs:label="gpsDestBearingRef">
  <rdfs:subPropertyOf rdf:resource="http://www.kanzaki.com/ns/exif#gpsDestBearingRef"/>
  <rdfs:subPropertyOf rdf:resource="&nexif;gpsInfo"/>
  <rdfs:comment>Indicates the reference used for giving the bearing to the destination point. 'T' denotes true direction and 'M' is magnetic direction.
tagNumber: 23</rdfs:comment>
  <rdfs:domain rdf:resource="&nexif;Photo"/>
  <rdfs:range rdf:resource="&xsd;string"/>
</rdf:Property>

<rdf:Property rdf:about="&nid3;hasSynchronizedTextElement"
    rdfs:comment="Links the synchronized text object with the text elements."
    rdfs:label="hasSynchronizedTextElement">
  <rdfs:domain rdf:resource="&nid3;SynchronizedText"/>
  <rdfs:range rdf:resource="&nid3;SynchronizedTextElement"/>
</rdf:Property>

<rdf:Property rdf:about="&ncal;delegatedFrom"
    rdfs:label="delegatedFrom">
  <rdfs:comment>To specify the calendar users that have delegated their participation to the calendar user specified by the property. Inspired by RFC 2445 sec. 4.2.4. Originally the value type for this property was CAL-ADDRESS. This has been expressed as nco:Contact to promote integration between NCAL and NCO.</rdfs:comment>
  <rdfs:domain rdf:resource="&ncal;Attendee"/>
  <rdfs:range rdf:resource="&nco;Contact"/>
</rdf:Property>

<rdf:Property rdf:about="&cnt;bytes">
  <rdf:type rdf:resource="&owl;ObjectProperty"/>
  <rdfs:comment xml:lang="en">The Base64 encoded byte sequence of the content.</rdfs:comment>
  <rdfs:domain rdf:resource="&cnt;ContentAsBase64"/>
  <rdfs:label xml:lang="en">Base64 encoded byte sequence</rdfs:label>
  <rdfs:range rdf:resource="&xsd;base64Binary"/>
</rdf:Property>

<rdf:Property rdf:about="&nuao;end"
    rdfs:comment="The time the event finished"
    rdfs:label="end time">
  <nrl:maxCardinality rdf:datatype="&xsd;nonNegativeInteger">1</nrl:maxCardinality>
  <rdfs:domain rdf:resource="&nuao;Event"/>
  <rdfs:range rdf:resource="&xsd;dateTime"/>
</rdf:Property>

<rdf:Property rdf:about="&dcterms;hasFormat">
  <rdfs:subPropertyOf rdf:resource="&dc;relation"/>
  <rdfs:subPropertyOf rdf:resource="&dcterms;relation"/>
  <dcterms:hasVersion rdf:resource="http://dublincore.org/usage/terms/history/#hasFormat-003"/>
  <dcterms:issued rdf:datatype="&xsd;date">2000-07-11</dcterms:issued>
  <dcterms:modified rdf:datatype="&xsd;date">2008-01-14</dcterms:modified>
  <rdfs:comment xml:lang="en">A related resource that is substantially the same as the pre-existing described resource, but in another format.</rdfs:comment>
  <rdfs:isDefinedBy rdf:resource="&dcterms;"/>
  <rdfs:label xml:lang="en">Has Format</rdfs:label>
  <scos:note xml:lang="en">This term is intended to be used with non-literal values as defined in the DCMI Abstract Model (http://dublincore.org/documents/abstract-model/).  As of December 2007, the DCMI Usage Board is seeking a way to express this intention with a formal range declaration.</scos:note>
</rdf:Property>

<tmo:TransmissionType rdf:about="&tmo;TMO_Instance_TransmissionType_Transfer"
    rdfs:label="TMO_Instance_TransmissionType_Transfer"/>

<rdfs:Class rdf:about="&nfo;SoftwareItem"
    rdfs:label="SoftwareItem">
  <rdfs:comment>A DataObject representing a piece of software. Examples of interpretations of a SoftwareItem include an Application and an OperatingSystem.</rdfs:comment>
  <rdfs:subClassOf rdf:resource="&nie;DataObject"/>
</rdfs:Class>

<rdfs:Class rdf:about="&dplo;AudioPost"
    rdfs:label="Audio Post">
  <rdfs:comment>Represents the live posting of audio file, or a link to online media such as podcasts, music, etc., as defined by instances of nfo:Audio.</rdfs:comment>
  <rdfs:subClassOf rdf:resource="&dplo;MultimediaPost"/>
</rdfs:Class>

<rdf:Property rdf:about="&nrl;subGraphOf"
    rdfs:label="subGraphOf">
  <nrl:inverseProperty rdf:resource="&nrl;superGraphOf"/>
  <rdfs:comment>Specifies a containment relationship between two graphs, meaning that the subject graph is included in the object graph</rdfs:comment>
  <rdfs:domain rdf:resource="&nrl;Graph"/>
  <rdfs:range rdf:resource="&nrl;Graph"/>
  <rdfs:subPropertyOf rdf:resource="http://www.w3.org/2004/03/trix/rdfg-1#subGraphOf"/>
</rdf:Property>

<tmo:Importance rdf:about="&tmo;TMO_Instance_Importance_05"
    rdfs:label="TMO_Instance_Importance_05"/>

<rdf:Property rdf:about="&nexif;gpsLatitudeRef"
    rdfs:label="gpsLatitudeRef">
  <rdfs:subPropertyOf rdf:resource="http://www.kanzaki.com/ns/exif#gpsLatitudeRef"/>
  <rdfs:subPropertyOf rdf:resource="&nexif;gpsInfo"/>
  <rdfs:comment>tagNumber: 1
Indicates whether the latitude is north or south latitude. The ASCII value 'N' indicates north latitude, and 'S' is south latitude.</rdfs:comment>
  <rdfs:domain rdf:resource="&nexif;Photo"/>
  <rdfs:range rdf:resource="&xsd;string"/>
</rdf:Property>

<owl:ObjectProperty rdf:about="&oa;styledBy">
  <rdfs:comment xml:lang="en">The relationship between a oa:Annotation and a oa:Style.

There MAY be 0 or 1 styledBy relationships for each Annotation.

If there are multiple Style resources that must be associated with the Annotation, then the use of the Multiplicity Constructs oa:Choice, oa:Composite or oa:List is RECOMMENDED.</rdfs:comment>
  <rdfs:domain rdf:resource="&oa;Annotation"/>
  <rdfs:isDefinedBy rdf:resource="&oa;"/>
  <rdfs:label xml:lang="en">styledBy</rdfs:label>
  <rdfs:range rdf:resource="&oa;Style"/>
</owl:ObjectProperty>

<rdf:Property rdf:about="&nco;creator"
    rdfs:label="creator">
  <rdfs:subPropertyOf rdf:resource="&dc;creator"/>
  <rdfs:subPropertyOf rdf:resource="&nco;contributor"/>
  <rdfs:subPropertyOf rdf:resource="&nao;creator"/>
  <rdfs:comment>Creator of an information element, an entity primarily responsible for the creation of the content of the data object.</rdfs:comment>
  <rdfs:domain rdf:resource="&nie;InformationElement"/>
  <rdfs:range rdf:resource="&nco;Contact"/>
</rdf:Property>

<rdfs:Class rdf:about="&duho;PrivacyPreferenceLog"
    rdfs:label="Privacy Preference Log">
  <rdfs:comment>A log that is used to document a specific type of resources: a user's changing privacy preferences. Thus, it is meant to contain past instances of ppo:PrivacyPreference from the Privacy Prefernece Ontology (PPO).</rdfs:comment>
  <rdfs:subClassOf rdf:resource="&duho;Log"/>
</rdfs:Class>

<rdf:Property rdf:about="&rdf;predicate">
  <rdfs:comment xml:lang="en">The predicate of the subject RDF statement.</rdfs:comment>
  <rdfs:domain rdf:resource="&rdf;Statement"/>
  <rdfs:isDefinedBy rdf:resource="&rdf;"/>
  <rdfs:label xml:lang="en">predicate</rdfs:label>
  <rdfs:range rdf:resource="&rdfs;Resource"/>
</rdf:Property>

<rdf:Property rdf:about="&nexif;focalPlaneResolutionUnit"
    rdfs:label="focalPlaneResolutionUnit">
  <rdfs:subPropertyOf rdf:resource="http://www.kanzaki.com/ns/exif#focalPlaneResolutionUnit"/>
  <rdfs:subPropertyOf rdf:resource="&nexif;pictTaking"/>
  <rdfs:comment>The unit for measuring FocalPlaneXResolution and FocalPlaneYResolution. This value is the same as the ResolutionUnit.
tagNumber: 41488</rdfs:comment>
  <rdfs:domain rdf:resource="&nexif;Photo"/>
  <rdfs:range rdf:resource="&xsd;string"/>
</rdf:Property>

<rdf:Property rdf:about="&ddo;knownNetwork"
    rdfs:label="knownNetwork">
  <rdfs:comment>Establishes a relationship between networks that have at some point in time (past or present) been either connected or in range of a device.</rdfs:comment>
  <rdfs:domain rdf:resource="&ddo;Device"/>
  <rdfs:range rdf:resource="&ddo;Network"/>
</rdf:Property>

<rdf:Property rdf:about="&foaf;schoolHomepage"
    rdfs:comment="A homepage of a school attended by the person."
    rdfs:label="schoolHomepage"
    ns:term_status="testing">
  <rdf:type rdf:resource="&owl;ObjectProperty"/>
  <rdfs:domain rdf:resource="&foaf;Person"/>
  <rdfs:isDefinedBy rdf:resource="&foaf;"/>
  <rdfs:range rdf:resource="&foaf;Document"/>
</rdf:Property>

<rdf:Property rdf:about="&foaf;focus"
    rdfs:label="focus"
    ns:term_status="testing">
  <rdf:type rdf:resource="&owl;ObjectProperty"/>
  <rdfs:comment>The underlying or 'focal' entity associated with some SKOS-described concept.</rdfs:comment>
  <rdfs:domain rdf:resource="&scos;Concept"/>
  <rdfs:isDefinedBy rdf:resource="&foaf;"/>
  <rdfs:range rdf:resource="&owl;Thing"/>
</rdf:Property>

<rdfs:Class rdf:about="&dpo;Altitude"
    rdfs:label="Altitude">
  <rdfs:comment>Quantifiable presence information concerning the agent's sensed absolute and relative altitude.</rdfs:comment>
  <rdfs:subClassOf rdf:resource="&dpo;QuantifiableComponent"/>
</rdfs:Class>

<ncal:ParticipationStatus rdf:about="&ncal;needsActionParticipationStatus"
    rdfs:label="needsActionParticipationStatus"/>

<rdfs:Class rdf:about="&nco;BirthDate"
    rdfs:label="BirthDate">
  <rdfs:comment>A class representing a person contact's birth date information. Possesses various attributes.</rdfs:comment>
  <rdfs:subClassOf rdf:resource="&rdfs;Resource"/>
</rdfs:Class>

<owl:NamedIndividual rdf:about="&oa;questioning">
  <rdf:type rdf:resource="&oa;Motivation"/>
  <rdfs:comment xml:lang="en">The motivation that represents asking a question about the target resource(s). For example to ask for assistance with a particular section of text, or question its veracity.</rdfs:comment>
  <scos:inScheme rdf:resource="&oa;motivationScheme"/>
  <scos:prefLabel xml:lang="en">questioning</scos:prefLabel>
</owl:NamedIndividual>

<tmo:PersonInvolvementRole rdf:about="&tmo;TMO_Instance_PersonInvolvementRole_Initiator"
    rdfs:label="TMO_Instance_PersonInvolvementRole_Initiator"/>

<rdf:Property rdf:about="&nao;engineeringTool"
    rdfs:comment="Specifies the engineering tool used to generate the graph"
    rdfs:label="engineering tool">
  <rdfs:domain rdf:resource="&nrl;Data"/>
  <rdfs:range rdf:resource="&rdfs;Literal"/>
  <rdfs:subPropertyOf rdf:resource="&nao;annotation"/>
</rdf:Property>

<rdf:Property rdf:about="&nexif;gpsInfo"
    rdfs:comment="An attribute relating to GPS information"
    rdfs:label="gpsInfo">
  <rdfs:subPropertyOf rdf:resource="http://www.kanzaki.com/ns/exif#gpsInfo"/>
  <rdfs:subPropertyOf rdf:resource="&nexif;exifAttribute"/>
  <rdfs:domain rdf:resource="&nexif;Photo"/>
  <rdfs:range rdf:resource="&xsd;string"/>
</rdf:Property>

<rdf:Property rdf:about="&foaf;holdsAccount"
    rdfs:comment="Indicates an account held by this agent."
    rdfs:label="account"
    ns:term_status="archaic">
  <rdf:type rdf:resource="&owl;ObjectProperty"/>
  <rdfs:domain rdf:resource="&foaf;Agent"/>
  <rdfs:isDefinedBy rdf:resource="&foaf;"/>
  <rdfs:range rdf:resource="&foaf;OnlineAccount"/>
</rdf:Property>

<tmo:TaskContainer rdf:about="&tmo;TMO_Instance_TaskContainer_archive"
    rdfs:label="TMO_Instance_TaskContainer_archive"/>

<rdf:Property rdf:about="&foaf;age"
    rdfs:comment="The age in years of some agent."
    rdfs:label="age"
    ns:term_status="unstable">
  <rdf:type rdf:resource="&owl;DatatypeProperty"/>
  <rdf:type rdf:resource="&owl;FunctionalProperty"/>
  <rdfs:domain rdf:resource="&foaf;Agent"/>
  <rdfs:isDefinedBy rdf:resource="&foaf;"/>
  <rdfs:range rdf:resource="&rdfs;Literal"/>
</rdf:Property>

<rdfs:Class rdf:about="&pimo;Association"
    rdfs:label="Association">
  <rdfs:subClassOf rdf:resource="&pimo;ClassOrThingOrPropertyOrAssociation"/>
  <rdfs:subClassOf rdf:resource="&rdfs;Resource"/>
  <rdfs:comment>An association between two or more pimo-things. This is used to model n-ary relations and metadata about relations. For example, the asociation of a person being organizational member is only effectual within a period of time (after the person joined the organization and before the person left the organization). There can be multiple periods of time when associations are valid.</rdfs:comment>
</rdfs:Class>

<rdf:Property rdf:about="&foaf;theme"
    rdfs:comment="A theme."
    rdfs:label="theme"
    ns:term_status="archaic">
  <rdf:type rdf:resource="&owl;ObjectProperty"/>
  <rdfs:domain rdf:resource="&owl;Thing"/>
  <rdfs:isDefinedBy rdf:resource="&foaf;"/>
  <rdfs:range rdf:resource="&owl;Thing"/>
</rdf:Property>

<owl:NamedIndividual rdf:about="&oa;motivationScheme">
  <rdf:type rdf:resource="&scos;ConceptScheme"/>
  <rdfs:comment xml:lang="en">The concept scheme for Open Annotation Motivations</rdfs:comment>
  <rdfs:label xml:lang="en">motivationScheme</rdfs:label>
</owl:NamedIndividual>

<rdf:Property rdf:about="&foaf;workplaceHomepage"
    rdfs:label="workplace homepage"
    ns:term_status="testing">
  <rdf:type rdf:resource="&owl;ObjectProperty"/>
  <rdfs:comment>A workplace homepage of some person; the homepage of an organization they work for.</rdfs:comment>
  <rdfs:domain rdf:resource="&foaf;Person"/>
  <rdfs:isDefinedBy rdf:resource="&foaf;"/>
  <rdfs:range rdf:resource="&foaf;Document"/>
</rdf:Property>

<rdf:Property rdf:about="&dcon;musicDetected"
    rdfs:label="Music Detected">
  <rdfs:comment>Registers whether music has been detected in the active environmental noise range in the current context.</rdfs:comment>
  <rdfs:domain rdf:resource="&dpo;Noise"/>
  <rdfs:range rdf:resource="&xsd;boolean"/>
  <rdfs:subPropertyOf rdf:resource="&dcon;hasContextAttribute"/>
</rdf:Property>

<rdf:Property rdf:about="&dcon;signal"
    rdfs:label="Signal value">
  <rdfs:comment>States the actual signal strength value for a network connection in the current context.</rdfs:comment>
  <rdfs:domain rdf:resource="&ddo;Network"/>
  <rdfs:range rdf:resource="&xsd;float"/>
  <rdfs:subPropertyOf rdf:resource="&dcon;hasContextAttribute"/>
</rdf:Property>

<rdf:Property rdf:about="&ncal;organizer"
    rdfs:label="organizer">
  <rdfs:comment>The property defines the organizer for a calendar component. Inspired by RFC 2445 sec. 4.8.4.3. Originally this property accepted many parameters. The Organizer class has been introduced to express them all. Note that NCAL is aligned with NCO. The actual value (of the CAL-ADDRESS type) is expressed as an instance of nco:Contact. Remember that the CN parameter has been removed from NCAL. Instead that value should be expressed using nco:fullname property of the above mentioned nco:Contact instance.</rdfs:comment>
  <rdfs:domain rdf:resource="&ncal;UnionOfEventFreebusyJournalTodo"/>
  <rdfs:range rdf:resource="&ncal;Organizer"/>
</rdf:Property>

<tmo:Importance rdf:about="&tmo;TMO_Instance_Importance_06"
    rdfs:label="TMO_Instance_Importance_06"/>

<rdfs:Datatype rdf:about="&dcterms;Point">
  <dcterms:hasVersion rdf:resource="http://dublincore.org/usage/terms/history/#Point-003"/>
  <dcterms:issued rdf:datatype="&xsd;date">2000-07-11</dcterms:issued>
  <dcterms:modified rdf:datatype="&xsd;date">2008-01-14</dcterms:modified>
  <rdfs:comment xml:lang="en">The set of points in space defined by their geographic coordinates according to the DCMI Point Encoding Scheme.</rdfs:comment>
  <rdfs:isDefinedBy rdf:resource="&dcterms;"/>
  <rdfs:label xml:lang="en">DCMI Point</rdfs:label>
  <rdfs:seeAlso rdf:resource="http://dublincore.org/documents/dcmi-point/"/>
</rdfs:Datatype>

<owl:ObjectProperty rdf:about="&oa;hasState">
  <rdfs:comment xml:lang="en">The relationship between a oa:SpecificResource and a oa:State resource.

There MAY be 0 or 1 oa:hasState relationship for each SpecificResource.

If there are multiple State resources that must be associated with the specific resource, then the use of the Multiplicity Constructs oa:Choice, oa:Composite or oa:List is RECOMMENDED.</rdfs:comment>
  <rdfs:domain rdf:resource="&oa;SpecificResource"/>
  <rdfs:isDefinedBy rdf:resource="&oa;"/>
  <rdfs:label xml:lang="en">hasState</rdfs:label>
  <rdfs:range rdf:resource="&oa;State"/>
</owl:ObjectProperty>

<tmo:Urgency rdf:about="&tmo;TMO_Instance_Urgency_09"
    rdfs:label="TMO_Instance_Urgency_09"/>

<rdf:Property rdf:about="&dc;relation">
  <dcterms:description xml:lang="en">Recommended best practice is to identify the related resource by means of a string conforming to a formal identification system. </dcterms:description>
  <dcterms:hasVersion rdf:resource="http://dublincore.org/usage/terms/history/#relation-006"/>
  <dcterms:issued rdf:datatype="&xsd;date">1999-07-02</dcterms:issued>
  <dcterms:modified rdf:datatype="&xsd;date">2008-01-14</dcterms:modified>
  <rdfs:comment xml:lang="en">A related resource.</rdfs:comment>
  <rdfs:isDefinedBy rdf:resource="&dc;"/>
  <rdfs:label xml:lang="en">Relation</rdfs:label>
  <scos:note xml:lang="en">A second property with the same name as this property has been declared in the dcterms: namespace (http://purl.org/dc/terms/).  See the Introduction to the document "DCMI Metadata Terms" (http://dublincore.org/documents/dcmi-terms/) for an explanation.</scos:note>
</rdf:Property>

<rdf:Property rdf:about="&nid3;comments"
    rdfs:label="comments">
  <nao:deprecated rdf:datatype="&xsd;boolean">true</nao:deprecated>
  <rdfs:comment>COMM - This frame is indended for any kind of full text information that does not fit in any other frame. It consists of a frame header followed by encoding, language and content descriptors and is ended with the actual comment as a text string. Newline characters are allowed in the comment text string. There may be more than one comment frame in each tag, but only one with the same language and content descriptor. Deprecated in favor of the more generic nie:comment.</rdfs:comment>
  <rdfs:domain rdf:resource="&nid3;ID3Audio"/>
  <rdfs:range rdf:resource="&xsd;string"/>
  <rdfs:subPropertyOf rdf:resource="&nie;comment"/>
</rdf:Property>

<nrl:GraphView rdf:about="&pimo;InferOccurrences"
    rdfs:label="InferOccurrences"/>

<rdf:Property rdf:about="&tmo;actualCompletion"
    nrl:maxCardinality="1"
    rdfs:label="actualCompletion">
  <rdfs:domain rdf:resource="&tmo;Task"/>
  <rdfs:range rdf:resource="&rdfs;Literal"/>
  <rdfs:subPropertyOf rdf:resource="&tmo;progress"/>
</rdf:Property>

<rdfs:Class rdf:about="&nie;DataSource"
    rdfs:label="DataSource">
  <rdfs:comment>A superclass for all entities from which DataObjects can be extracted. Each entity represents a native application or some other system that manages information that may be of interest to the user of the Semantic Desktop. Subclasses may include FileSystems, Mailboxes, Calendars, websites etc. The exact choice of subclasses and their properties is considered application-specific. Each data extraction application is supposed to provide it's own DataSource ontology. Such an ontology should contain supported data source types coupled with properties necessary for the application to gain access to the data sources.  (paths, urls, passwords  etc...)</rdfs:comment>
  <rdfs:subClassOf rdf:resource="&rdfs;Resource"/>
</rdfs:Class>

<owl:ObjectProperty rdf:about="&oa;default">
  <rdfs:comment xml:lang="en">The constituent resource of a oa:Choice to use as a default option, if there is no other means to determine which would be most appropriate.

There SHOULD be exactly 1 default relationship for each Choice.</rdfs:comment>
  <rdfs:domain rdf:resource="&oa;Choice"/>
  <rdfs:isDefinedBy rdf:resource="&oa;"/>
  <rdfs:label xml:lang="en">default</rdfs:label>
  <rdfs:subPropertyOf rdf:resource="&oa;item"/>
</owl:ObjectProperty>

<rdf:Property rdf:about="&nmo;messageReplyTo"
    rdfs:comment="An address where the reply should be sent."
    rdfs:label="replyTo">
  <nrl:maxCardinality rdf:datatype="&xsd;integer">1</nrl:maxCardinality>
  <rdfs:domain rdf:resource="&nmo;Message"/>
  <rdfs:range rdf:resource="&nco;ContactMedium"/>
</rdf:Property>

<rdfs:Class rdf:about="&nco;BbsNumber"
    rdfs:label="BbsNumber">
  <rdfs:comment>A Bulletin Board System (BBS) phone number. Inspired by the (TYPE=bbsl) parameter of the TEL property as defined in RFC 2426 sec  3.3.1.</rdfs:comment>
  <rdfs:subClassOf rdf:resource="&nco;ModemNumber"/>
</rdfs:Class>

<rdf:Property rdf:about="&dcterms;isReplacedBy">
  <rdfs:subPropertyOf rdf:resource="&dc;relation"/>
  <rdfs:subPropertyOf rdf:resource="&dcterms;relation"/>
  <dcterms:hasVersion rdf:resource="http://dublincore.org/usage/terms/history/#isReplacedBy-003"/>
  <dcterms:issued rdf:datatype="&xsd;date">2000-07-11</dcterms:issued>
  <dcterms:modified rdf:datatype="&xsd;date">2008-01-14</dcterms:modified>
  <rdfs:comment xml:lang="en">A related resource that supplants, displaces, or supersedes the described resource.</rdfs:comment>
  <rdfs:isDefinedBy rdf:resource="&dcterms;"/>
  <rdfs:label xml:lang="en">Is Replaced By</rdfs:label>
  <scos:note xml:lang="en">This term is intended to be used with non-literal values as defined in the DCMI Abstract Model (http://dublincore.org/documents/abstract-model/).  As of December 2007, the DCMI Usage Board is seeking a way to express this intention with a formal range declaration.</scos:note>
</rdf:Property>

<rdf:Property rdf:about="&tmo;targetEndTime"
    nrl:maxCardinality="1"
    rdfs:label="targetEndTime">
  <rdfs:subPropertyOf rdf:resource="&tmo;endTime"/>
  <rdfs:subPropertyOf rdf:resource="&tmo;targetTime"/>
  <rdfs:domain rdf:resource="&tmo;Task"/>
  <rdfs:range rdf:resource="&xsd;dateTime"/>
</rdf:Property>

<rdf:Property rdf:about="&dpo;dayOfWeek"
    rdfs:label="Day of the Week">
  <rdfs:comment>A subproperty of dpo:value that defines an exact date/time value (a day in a week, i.e., between 1 signifying Monday and 7 signifying Sunday) such that it can classify as a dpo:TimePeriod instance.</rdfs:comment>
  <rdfs:domain rdf:resource="&dpo;TimePeriod"/>
  <rdfs:range rdf:resource="&xsd;integer"/>
  <rdfs:subPropertyOf rdf:resource="&dpo;value"/>
</rdf:Property>

<rdfs:Class rdf:about="&dpo;Availability"
    rdfs:label="Availability">
  <rdfs:comment>Non-quantifiable presence information concerning the current broadcast virtual availability of the agent.</rdfs:comment>
  <rdfs:subClassOf rdf:resource="&dpo;NonQuantifiableComponent"/>
</rdfs:Class>

<rdf:Property rdf:about="&nco;locality"
    rdfs:label="locality">
  <nrl:maxCardinality rdf:datatype="&xsd;integer">1</nrl:maxCardinality>
  <rdfs:comment>Locality or City. Inspired by the fourth part of the value of the 'ADR' property as defined in RFC 2426, sec. 3.2.1</rdfs:comment>
  <rdfs:domain rdf:resource="&nco;PostalAddress"/>
  <rdfs:range rdf:resource="&xsd;string"/>
</rdf:Property>

<rdf:Property rdf:about="&dpo;maxHour"
    rdfs:label="Maximum Hour">
  <rdfs:comment>A subproperty of dpo:maxValue that defines an upperbound on the observed time (in hours, i.e., between 0 signifying midnight and 23 signifying 11pm) such that it can classify as a dpo:TimePeriod instance. It can be used in conjunction with dpo:minHour, i.e. specific instances of dpo:TimePeriod have a pre-defined observable 24-hour-based period.</rdfs:comment>
  <rdfs:domain rdf:resource="&dpo;TimePeriod"/>
  <rdfs:range rdf:resource="&xsd;integer"/>
  <rdfs:subPropertyOf rdf:resource="&dpo;maxValue"/>
</rdf:Property>

<rdf:Property rdf:about="&nao;userVisible"
    rdfs:label="user visible">
  <nao:userVisible rdf:datatype="&xsd;boolean">false</nao:userVisible>
  <nrl:maxCardinality rdf:datatype="&xsd;integer">1</nrl:maxCardinality>
  <rdfs:comment>Mark a property, class, or even resource as user visible or not. Non-user-visible entities should never be presented to the user. By default everything is user-visible.</rdfs:comment>
  <rdfs:domain rdf:resource="&rdfs;Resource"/>
  <rdfs:range rdf:resource="&xsd;boolean"/>
</rdf:Property>

<rdf:Property rdf:about="&nexif;flashpixVersion"
    rdfs:label="flashpixVersion">
  <rdfs:subPropertyOf rdf:resource="http://www.kanzaki.com/ns/exif#flashpixVersion"/>
  <rdfs:subPropertyOf rdf:resource="&nexif;versionInfo"/>
  <rdfs:comment>tagNumber: 40960
The Flashpix format version supported by a FPXR file. If the FPXR function supports Flashpix format Ver. 1.0, this is indicated similarly to ExifVersion by recording "0100" as 4-byte ASCII.</rdfs:comment>
  <rdfs:domain rdf:resource="&nexif;Photo"/>
  <rdfs:range rdf:resource="&xsd;string"/>
</rdf:Property>

<rdf:Property rdf:about="&nco;department"
    rdfs:label="department">
  <rdfs:comment>Department. The organizational unit within the organization.</rdfs:comment>
  <rdfs:domain rdf:resource="&nco;Affiliation"/>
  <rdfs:range rdf:resource="&xsd;string"/>
</rdf:Property>

<rdf:Property rdf:about="&dpo;minWaveHeight"
    rdfs:label="Maximum Wave Height">
  <rdfs:comment>A subproperty of dpo:minValue that defines a lowerbound on the observed wave height (in metres) such that it can classify as a dpo:WeatherCondition instance. It can be used in conjunction with dpo:maxWaveHeight to state that specific instances of dpo:WeatherCondition have a pre-defined range of observable real-world wave heights in a body of water. In addition, they can also be used with various other weather conditions values and ranges to define complex weather condition types.</rdfs:comment>
  <rdfs:domain rdf:resource="&dpo;WeatherConditions"/>
  <rdfs:range rdf:resource="&xsd;float"/>
  <rdfs:subPropertyOf rdf:resource="&dpo;minValue"/>
</rdf:Property>

<rdfs:Class rdf:about="&nfo;Font"
    rdfs:comment="A font."
    rdfs:label="Font">
  <rdfs:subClassOf rdf:resource="&nie;InformationElement"/>
</rdfs:Class>

<rdf:Property rdf:about="&ncal;descriptionAltRep"
    rdfs:label="descriptionAltRep">
  <rdfs:comment>Alternate representation of the calendar entity description. Introduced to cover 
the ALTREP parameter of the DESCRIPTION property. See 
documentation of ncal:description for details.</rdfs:comment>
  <rdfs:domain rdf:resource="&ncal;UnionOfAlarmEventJournalTodo"/>
  <rdfs:range rdf:resource="&rdfs;Resource"/>
</rdf:Property>

<rdf:Property rdf:about="&scos;related">
  <rdf:type rdf:resource="&owl;ObjectProperty"/>
  <rdf:type rdf:resource="&owl;SymmetricProperty"/>
  <rdfs:comment xml:lang="en">skos:related is disjoint with skos:broaderTransitive</rdfs:comment>
  <rdfs:isDefinedBy rdf:resource="http://www.w3.org/2004/02/skos/core"/>
  <rdfs:label xml:lang="en">has related</rdfs:label>
  <rdfs:subPropertyOf rdf:resource="&scos;semanticRelation"/>
  <scos:definition xml:lang="en">Relates a concept to a concept with which there is an associative semantic relationship.</scos:definition>
</rdf:Property>

<rdfs:Class rdf:about="&pimo;Tag"
    protege:role="abstract"
    rdfs:label="Tag">
  <rdfs:subClassOf rdf:resource="&nao;Tag"/>
  <rdfs:subClassOf rdf:resource="&pimo;Thing"/>
  <pimo:classRole rdf:resource="&pimo;AbstractClass"/>
  <rdfs:comment>Tags in the context of PIMO. A marker class for Things that are used to categorize documents (or other things). Tags must be a kind of Thing and must have a unique label. Documents should not be Tags by default.</rdfs:comment>
</rdfs:Class>

<rdf:Property rdf:about="&nmm;seasonNumber"
    rdfs:comment="The number of a season"
    rdfs:label="season number">
  <nrl:cardinality rdf:datatype="&xsd;integer">1</nrl:cardinality>
  <rdfs:domain rdf:resource="&nmm;TVSeason"/>
  <rdfs:range rdf:resource="&xsd;integer"/>
</rdf:Property>

<ncal:EventStatus rdf:about="&ncal;cancelledEventStatus"
    rdfs:label="cancelledEventStatus"/>

<rdfs:Class rdf:about="&ndo;Torrent"
    rdfs:label="torrent">
  <rdfs:comment>A .torrent file which contains references(ndo:TorrentedFile) to files available via BitTorrent. The references are pointed to via nie:hasLogicalPart</rdfs:comment>
  <rdfs:subClassOf rdf:resource="&nie;InformationElement"/>
</rdfs:Class>

<rdf:Property rdf:about="&ncal;journalStatus"
    rdfs:label="status">
  <nrl:maxCardinality rdf:datatype="&xsd;integer">1</nrl:maxCardinality>
  <rdfs:comment>Defines the overall status or confirmation for a journal entry. Based on the STATUS property defined in RFC 2445 sec. 4.8.1.11.</rdfs:comment>
  <rdfs:domain rdf:resource="&ncal;Journal"/>
  <rdfs:range rdf:resource="&ncal;JournalStatus"/>
</rdf:Property>

<rdf:Property rdf:about="&cnt;version">
  <rdf:type rdf:resource="&owl;ObjectProperty"/>
  <rdfs:comment xml:lang="en">The XML version declared in the XML declaration.</rdfs:comment>
  <rdfs:domain rdf:resource="&cnt;ContentAsXML"/>
  <rdfs:label xml:lang="en">XML version</rdfs:label>
  <rdfs:range rdf:resource="&rdfs;Literal"/>
</rdf:Property>

<ncal:RecurrenceFrequency rdf:about="&ncal;minutely"
    rdfs:label="minutely"/>

<rdfs:Class rdf:about="&ncal;NcalPeriod"
    rdfs:label="NcalPeriod">
  <rdfs:comment>A period of time. Inspired by the PERIOD datatype specified in RFC 2445 sec. 4.3.9</rdfs:comment>
  <rdfs:subClassOf rdf:resource="&ncal;NcalTimeEntity"/>
</rdfs:Class>

<owl:NamedIndividual rdf:about="&oa;replying">
  <rdf:type rdf:resource="&oa;Motivation"/>
  <rdfs:comment xml:lang="en">The motivation that represents a reply to a previous statement, either an Annotation or another resource. For example providing the assistance requested in the above.</rdfs:comment>
  <scos:inScheme rdf:resource="&oa;motivationScheme"/>
  <scos:prefLabel xml:lang="en">replying</scos:prefLabel>
</owl:NamedIndividual>

<rdf:Property rdf:about="&dcterms;dateCopyrighted">
  <rdfs:subPropertyOf rdf:resource="&dc;date"/>
  <rdfs:subPropertyOf rdf:resource="&dcterms;date"/>
  <dcterms:hasVersion rdf:resource="http://dublincore.org/usage/terms/history/#dateCopyrighted-002"/>
  <dcterms:issued rdf:datatype="&xsd;date">2002-07-13</dcterms:issued>
  <dcterms:modified rdf:datatype="&xsd;date">2008-01-14</dcterms:modified>
  <rdfs:comment xml:lang="en">Date of copyright.</rdfs:comment>
  <rdfs:isDefinedBy rdf:resource="&dcterms;"/>
  <rdfs:label xml:lang="en">Date Copyrighted</rdfs:label>
  <rdfs:range rdf:resource="&rdfs;Literal"/>
</rdf:Property>

<rdfs:Class rdf:about="&pimo;Person"
    rdfs:label="Person">
  <rdfs:subClassOf rdf:resource="&nao;Party"/>
  <rdfs:subClassOf rdf:resource="&pimo;Agent"/>
  <rdfs:subClassOf rdf:resource="&pimo;Locatable"/>
  <rdfs:comment>Represents a person. Either living, dead, real or imaginary. (Definition from foaf:Person)</rdfs:comment>
</rdfs:Class>

<rdfs:Class rdf:about="&nco;ContactGroup"
    rdfs:label="ContactGroup">
  <rdfs:comment>A group of Contacts. Could be used to express a group in an addressbook or on a contact list of an IM application. One contact can belong to many groups.</rdfs:comment>
  <rdfs:subClassOf rdf:resource="&nie;InformationElement"/>
</rdfs:Class>

<rdf:Property rdf:about="&dpo;lastActive"
    rdfs:label="Last Active">
  <rdfs:comment>Stores the last date and time at which a particular presence component was last observed, by any of an agent's sensors.</rdfs:comment>
  <rdfs:domain rdf:resource="&dpo;PresenceComponent"/>
  <rdfs:range rdf:resource="&xsd;dateTime"/>
</rdf:Property>

<rdf:Property rdf:about="&nuao;modificationCount"
    rdfs:comment="The total number of modifications"
    rdfs:label="modification count">
  <nrl:maxCardinality rdf:datatype="&xsd;nonNegativeInteger">1</nrl:maxCardinality>
  <rdfs:domain rdf:resource="&rdfs;Resource"/>
  <rdfs:range rdf:resource="&xsd;nonNegativeInteger"/>
</rdf:Property>

<rdf:Property rdf:about="&nco;fullname"
    nrl:maxCardinality="1"
    rdfs:label="fullname">
  <rdfs:comment>To specify the formatted text corresponding to the name of the object the Contact represents. An equivalent of the FN property as defined in RFC 2426 Sec. 3.1.1.</rdfs:comment>
  <rdfs:domain rdf:resource="&nco;Name"/>
  <rdfs:range rdf:resource="&xsd;string"/>
  <rdfs:subPropertyOf rdf:resource="&nie;title"/>
</rdf:Property>

<rdf:Property rdf:about="&nmm;musicBrainzAlbumID"
    rdfs:comment="MusicBrainz album ID"
    rdfs:label="musicbrainz album ID">
  <nrl:maxCardinality rdf:datatype="&xsd;integer">1</nrl:maxCardinality>
  <rdfs:domain rdf:resource="&nmm;MusicAlbum"/>
  <rdfs:range rdf:resource="&xsd;string"/>
  <rdfs:subPropertyOf rdf:resource="&nie;identifier"/>
</rdf:Property>

<rdf:Property rdf:about="&nexif;ifdPointer"
    rdfs:comment="A tag that refers a child IFD"
    rdfs:label="ifdPointer">
  <rdfs:subPropertyOf rdf:resource="http://www.kanzaki.com/ns/exif#ifdPointer"/>
  <rdfs:subPropertyOf rdf:resource="&nexif;exifAttribute"/>
  <rdfs:domain rdf:resource="&nexif;Photo"/>
  <rdfs:range rdf:resource="&nexif;Photo"/>
</rdf:Property>

<rdf:Property rdf:about="&ncal;recurrenceIdDateTime"
    rdfs:label="recurrenceIdDateTime">
  <nrl:maxCardinality rdf:datatype="&xsd;integer">1</nrl:maxCardinality>
  <rdfs:comment>The date and time of a recurrence identifier. Provided to express the actual value of the ncal:recurrenceId property. See documentation for ncal:recurrenceId for details.</rdfs:comment>
  <rdfs:domain rdf:resource="&ncal;RecurrenceIdentifier"/>
  <rdfs:range rdf:resource="&ncal;NcalDateTime"/>
</rdf:Property>

<rdf:Property rdf:about="&nid3;unsynchronizedTextContent"
    rdfs:label="unsynchronizedTextContent">
  <rdfs:comment>Unsynchronized text content. Inspired by the content part of the USLT frame defined in the ID3 2.3.0 Spec sec. 4.9</rdfs:comment>
  <rdfs:domain rdf:resource="&nid3;ID3Audio"/>
  <rdfs:range rdf:resource="&xsd;string"/>
  <rdfs:subPropertyOf rdf:resource="&nie;plainTextContent"/>
</rdf:Property>

<rdf:Property rdf:about="&nrl;semanticsDefinedBy"
    rdfs:label="semanticsDefinedBy">
  <rdfs:comment>Points to the human readable specifications for a representation of some declarative semantics</rdfs:comment>
  <rdfs:domain rdf:resource="&nrl;Semantics"/>
  <rdfs:range rdf:resource="&rdfs;Resource"/>
</rdf:Property>

<rdf:Property rdf:about="&nmo;emailTo"
    rdfs:comment="The primary intended recipient of an email."
    rdfs:label="to">
  <rdfs:domain rdf:resource="&nmo;Email"/>
  <rdfs:range rdf:resource="&nco;ContactMedium"/>
  <rdfs:subPropertyOf rdf:resource="&nmo;primaryMessageRecipient"/>
</rdf:Property>

<rdf:Property rdf:about="&nfo;hashValue"
    rdfs:comment="The actual value of the hash."
    rdfs:label="hashValue">
  <nrl:cardinality rdf:datatype="&xsd;integer">1</nrl:cardinality>
  <rdfs:domain rdf:resource="&nfo;FileHash"/>
  <rdfs:range rdf:resource="&xsd;string"/>
</rdf:Property>

<rdf:Property rdf:about="&ncal;contactAltRep"
    rdfs:label="contactAltRep">
  <rdfs:comment>Alternate representation of the contact property. Introduced to cover 
the ALTREP parameter of the CONTACT property. See 
documentation of ncal:contact for details.</rdfs:comment>
  <rdfs:domain rdf:resource="&ncal;UnionOfEventFreebusyJournalTodo"/>
  <rdfs:range rdf:resource="&rdfs;Resource"/>
</rdf:Property>

<rdf:Property rdf:about="&drmo;isComposedOf"
    rdfs:label="is composed of">
  <rdfs:comment>The isComposedOf property defines the condition blocks of a Rule</rdfs:comment>
  <rdfs:domain rdf:resource="&drmo;Rule"/>
  <rdfs:range rdf:resource="&drmo;Condition"/>
</rdf:Property>

<rdfs:Class rdf:about="&nfo;Software"
    rdfs:label="Software">
  <rdfs:subClassOf rdf:resource="&nie;InformationElement"/>
  <rdfs:subClassOf rdf:resource="&nao;Agent"/>
  <rdfs:comment>A piece of software. Examples may include applications and the operating system. This interpretation most commonly applies to SoftwareItems.</rdfs:comment>
</rdfs:Class>

<rdf:Property rdf:about="&ncal;ncalTimezone"
    rdfs:label="ncalTimezone">
  <nrl:maxCardinality rdf:datatype="&xsd;integer">1</nrl:maxCardinality>
  <rdfs:comment>The timezone instance that should be used to interpret an NcalDateTime. The purpose of this property is similar to the TZID parameter specified in RFC 2445 sec. 4.2.19</rdfs:comment>
  <rdfs:domain rdf:resource="&ncal;NcalDateTime"/>
  <rdfs:range rdf:resource="&ncal;Timezone"/>
</rdf:Property>

<rdf:Property rdf:about="&nie;identifier"
    rdfs:label="identifier">
  <rdfs:subPropertyOf rdf:resource="&dc;identifier"/>
  <rdfs:subPropertyOf rdf:resource="&nao;identifier"/>
  <rdfs:comment>An unambiguous reference to the InformationElement within a given context. Recommended best practice is to identify the resource by means of a string conforming to a formal identification system.</rdfs:comment>
  <rdfs:domain rdf:resource="&nie;InformationElement"/>
  <rdfs:range rdf:resource="&xsd;string"/>
</rdf:Property>

<tmo:Urgency rdf:about="&tmo;TMO_Instance_Urgency_02"
    rdfs:label="TMO_Instance_Urgency_02"/>

<rdf:Property rdf:about="&ncal;lastModified"
    rdfs:label="lastModified">
  <nrl:maxCardinality rdf:datatype="&xsd;integer">1</nrl:maxCardinality>
  <rdfs:comment>The property specifies the date and time that the information associated with the calendar component was last revised in the calendar store. Note: This is analogous to the modification date and time for a file in the file system. Inspired by RFC 2445 sec. 4.8.7.3. Note that the RFC allows ONLY UTC time values for this property.</rdfs:comment>
  <rdfs:domain rdf:resource="&ncal;UnionOfEventJournalTimezoneTodo"/>
  <rdfs:range rdf:resource="&xsd;dateTime"/>
</rdf:Property>

<rdf:Property rdf:about="&dc;language">
  <dcterms:description xml:lang="en">Recommended best practice is to use a controlled vocabulary such as RFC 4646 [RFC4646].</dcterms:description>
  <dcterms:hasVersion rdf:resource="http://dublincore.org/usage/terms/history/#language-007"/>
  <dcterms:issued rdf:datatype="&xsd;date">1999-07-02</dcterms:issued>
  <dcterms:modified rdf:datatype="&xsd;date">2008-01-14</dcterms:modified>
  <rdfs:comment xml:lang="en">A language of the resource.</rdfs:comment>
  <rdfs:isDefinedBy rdf:resource="&dc;"/>
  <rdfs:label xml:lang="en">Language</rdfs:label>
  <rdfs:seeAlso rdf:resource="http://www.ietf.org/rfc/rfc4646.txt"/>
  <scos:note xml:lang="en">A second property with the same name as this property has been declared in the dcterms: namespace (http://purl.org/dc/terms/).  See the Introduction to the document "DCMI Metadata Terms" (http://dublincore.org/documents/dcmi-terms/) for an explanation.</scos:note>
</rdf:Property>

<rdf:Property rdf:about="&dcon;currentMode"
    rdfs:label="Current Mode">
  <rdfs:comment>Refers to the mode of the data source from which a context element has been retrieved, at retrieval time. A data source can consist of a service, an account, an application, or a device.  </rdfs:comment>
  <rdfs:domain rdf:resource="&nie;DataSource"/>
  <rdfs:range rdf:resource="&nie;Mode"/>
</rdf:Property>

<rdfs:Class rdf:about="&nie;Mode"
    rdfs:label="Mode">
  <rdfs:comment>Representation for a standard set of device/application/service modes, corresponding to various sets of modes that are either inbuilt in a device (e.g. inbuilt phone modes such as silent, loud, general, vibrate, etc.) or available for applications and online services (e.g. IM system modes such as busy, available, invisible, etc.)</rdfs:comment>
</rdfs:Class>

<nrl:DefiningProperty rdf:about="&nmm;assistantDirector"
    rdfs:label="assistant director">
  <rdf:type rdf:resource="&rdf;Property"/>
  <rdfs:domain rdf:resource="&nfo;Video"/>
  <rdfs:range rdf:resource="&nco;Contact"/>
  <rdfs:subPropertyOf rdf:resource="&nco;contributor"/>
</nrl:DefiningProperty>

<rdf:Property rdf:about="&ddo;ipAddress"
    rdfs:comment="Defines the known IP address for a computer network."
    rdfs:label="ipAddress">
  <rdfs:domain rdf:resource="&ddo;ComputerNetwork"/>
  <rdfs:range rdf:resource="&xsd;string"/>
</rdf:Property>

<nrl:SymmetricProperty rdf:about="&nrl;equivalentGraph"
    rdfs:comment="Links two equivalent named graphs. A symmetric property"
    rdfs:label="equivalentGraph">
  <rdf:type rdf:resource="&rdf;Property"/>
  <rdfs:domain rdf:resource="&nrl;Graph"/>
  <rdfs:range rdf:resource="&nrl;Graph"/>
  <rdfs:subPropertyOf rdf:resource="http://www.w3.org/2004/03/trix/rdfg-1#equivalentGraph"/>
</nrl:SymmetricProperty>

<rdf:Property rdf:about="&scos;closeMatch">
  <rdf:type rdf:resource="&owl;ObjectProperty"/>
  <rdf:type rdf:resource="&owl;SymmetricProperty"/>
  <rdfs:isDefinedBy rdf:resource="http://www.w3.org/2004/02/skos/core"/>
  <rdfs:label xml:lang="en">has close match</rdfs:label>
  <rdfs:subPropertyOf rdf:resource="&scos;mappingRelation"/>
  <scos:definition xml:lang="en">skos:closeMatch is used to link two concepts that are sufficiently similar that they can be used interchangeably in some information retrieval applications. In order to avoid the possibility of "compound errors" when combining mappings across more than two concept schemes, skos:closeMatch is not declared to be a transitive property.</scos:definition>
</rdf:Property>

<rdf:Property rdf:about="&nmm;internationalStandardRecordingCode"
    rdfs:comment="ISRC ID. Format: 'CC-XXX-YY-NNNNN'"
    rdfs:label="international standard recording code">
  <nrl:maxCardinality rdf:datatype="&xsd;integer">1</nrl:maxCardinality>
  <rdfs:domain rdf:resource="&nmm;MusicAlbum"/>
  <rdfs:range rdf:resource="&xsd;string"/>
  <rdfs:subPropertyOf rdf:resource="&nie;identifier"/>
</rdf:Property>

<rdfs:Class rdf:about="&nfo;RemoteDataObject"
    rdfs:label="RemoteDataObject">
  <rdfs:comment>A file data object stored at a remote location. Don't confuse this class with a RemotePortAddress. This one applies to a particular resource, RemotePortAddress applies to an address, that can have various interpretations.</rdfs:comment>
  <rdfs:subClassOf rdf:resource="&nfo;FileDataObject"/>
</rdfs:Class>

<rdf:Property rdf:about="&nmm;genre"
    rdfs:comment="Genre"
    rdfs:label="genre">
  <rdfs:domain rdf:resource="&nfo;Media"/>
  <rdfs:range rdf:resource="&xsd;string"/>
</rdf:Property>

<rdfs:Class rdf:about="&pimo;OrganizationMember"
    rdfs:label="Member">
  <rdfs:comment>The role of one or multiple persons being a member in one or multiple organizations. Use pimo:organization and pimo:roleHolder to link to the organizations and persons.</rdfs:comment>
  <rdfs:subClassOf rdf:resource="&pimo;PersonRole"/>
</rdfs:Class>

<rdf:Property rdf:about="&ncal;returnStatus"
    rdfs:label="returnStatus">
  <nrl:maxCardinality rdf:datatype="&xsd;integer">1</nrl:maxCardinality>
  <rdfs:comment>Short return status. Inspired by the first element of the structured value of the REQUEST-STATUS property described in RFC 2445 sec. 4.8.8.2.

The short return status is a PERIOD character (US-ASCII decimal 46) separated 3-tuple of integers. For example, "3.1.1". The successive  levels of integers provide for a successive level of status code granularity.

The following are initial classes for the return status code. Individual iCalendar object methods will define specific return status codes for these classes. In addition, other classes for the return status code may be defined using the registration process defined later in this memo.

 1.xx - Preliminary success. This class of status of status code indicates that the request has request has been initially processed but that completion is pending.

2.xx -Successful. This class of status code indicates that the request was completed successfuly. However, the exact status code can indicate that a fallback has been taken.

3.xx - Client Error. This class of status code indicates that the request was not successful. The error is the result of either a syntax or a semantic error in the client formatted request. Request should not be retried until the condition in the request is corrected.

4.xx - Scheduling Error. This class of status code indicates that the request was not successful. Some sort of error occurred within the  calendaring and scheduling service, not directly related to the request itself.</rdfs:comment>
  <rdfs:domain rdf:resource="&ncal;RequestStatus"/>
  <rdfs:range rdf:resource="&xsd;string"/>
</rdf:Property>

<rdfs:Class rdf:about="&nuao;UsageEvent"
    rdfs:label="desktop event">
  <rdfs:comment>An event of primary or intended use of the resource by the user. Primary or intended use is defined as the use by the consumer of the resource, such as watching a movie or listening to a song. Not to be confused with a low-level read on a file.</rdfs:comment>
  <rdfs:subClassOf rdf:resource="&nuao;DesktopEvent"/>
</rdfs:Class>

<rdf:Property rdf:about="&nexif;referenceBlackWhite"
    rdfs:label="referenceBlackWhite">
  <rdfs:subPropertyOf rdf:resource="http://www.kanzaki.com/ns/exif#referenceBlackWhite"/>
  <rdfs:subPropertyOf rdf:resource="&nexif;imageDataCharacter"/>
  <rdfs:comment>tagNumber: 532
The reference black point value and reference white point value. The color space is declared in a color space information tag, with the default being the value that gives the optimal image characteristics Interoperability these conditions.</rdfs:comment>
  <rdfs:domain rdf:resource="&nexif;Photo"/>
  <rdfs:range rdf:resource="&xsd;string"/>
</rdf:Property>

<rdf:Property rdf:about="&dcterms;provenance">
  <dcterms:description xml:lang="en">The statement may include a description of any changes successive custodians made to the resource.</dcterms:description>
  <dcterms:hasVersion rdf:resource="http://dublincore.org/usage/terms/history/#provenance-002"/>
  <dcterms:issued rdf:datatype="&xsd;date">2004-09-20</dcterms:issued>
  <dcterms:modified rdf:datatype="&xsd;date">2008-01-14</dcterms:modified>
  <rdfs:comment xml:lang="en">A statement of any changes in ownership and custody of the resource since its creation that are significant for its authenticity, integrity, and interpretation.</rdfs:comment>
  <rdfs:isDefinedBy rdf:resource="&dcterms;"/>
  <rdfs:label xml:lang="en">Provenance</rdfs:label>
  <rdfs:range rdf:resource="&dcterms;ProvenanceStatement"/>
</rdf:Property>

<rdf:Property rdf:about="&foaf;openid"
    rdfs:comment="An OpenID for an Agent."
    rdfs:label="openid"
    ns:term_status="testing">
  <rdf:type rdf:resource="&owl;InverseFunctionalProperty"/>
  <rdf:type rdf:resource="&owl;ObjectProperty"/>
  <rdfs:domain rdf:resource="&foaf;Agent"/>
  <rdfs:isDefinedBy rdf:resource="&foaf;"/>
  <rdfs:range rdf:resource="&foaf;Document"/>
  <rdfs:subPropertyOf rdf:resource="&foaf;isPrimaryTopicOf"/>
</rdf:Property>

<rdf:Property rdf:about="&nao;iconName"
    rdfs:label="iconname">
  <nrl:minCardinality rdf:datatype="&xsd;nonNegativeInteger">1</nrl:minCardinality>
  <rdfs:comment>Defines a name for a FreeDesktop Icon as defined in the FreeDesktop Icon Naming Standard</rdfs:comment>
  <rdfs:domain rdf:resource="&nao;FreeDesktopIcon"/>
  <rdfs:range rdf:resource="&rdfs;Literal"/>
  <rdfs:subPropertyOf rdf:resource="&nao;identifier"/>
</rdf:Property>

<rdfs:Class rdf:about="&ncal;FreebusyPeriod"
    rdfs:label="FreebusyPeriod">
  <rdfs:comment>An aggregate of a period and a freebusy type. This class has been introduced to serve as a range of the ncal:freebusy property. See documentation for ncal:freebusy for details. Note that the specification of freebusy property states that the period is to be expressed using UTC time, so the timezone properties should NOT be used for instances of this class.</rdfs:comment>
  <rdfs:subClassOf rdf:resource="&ncal;NcalPeriod"/>
</rdfs:Class>

<rdf:Property rdf:about="&foaf;depicts"
    rdfs:comment="A thing depicted in this representation."
    rdfs:label="depicts"
    ns:term_status="testing">
  <rdf:type rdf:resource="&owl;ObjectProperty"/>
  <rdfs:domain rdf:resource="&foaf;Image"/>
  <rdfs:isDefinedBy rdf:resource="&foaf;"/>
  <rdfs:range rdf:resource="&owl;Thing"/>
  <owl:inverseOf rdf:resource="&foaf;depiction"/>
</rdf:Property>

<rdf:Property rdf:about="&dplo;definingResource"
    rdfs:label="has defining resource">
  <rdfs:comment>As many resources that are shared as liveposts exist beforehand, this property (a sub-property of nao:hasSuperResource) is provided to make this link explicit. Therefore a livepost (videopost, eventpost, availabilitypost, etc.) can be linked to the representation of the original resource being shared online (video, event, availability, etc.)</rdfs:comment>
  <rdfs:domain rdf:resource="&dplo;LivePost"/>
  <rdfs:range rdf:resource="&rdfs;Resource"/>
  <rdfs:subPropertyOf rdf:resource="&nao;hasSuperResource"/>
</rdf:Property>

<rdf:Property rdf:about="&dcterms;title">
  <dcterms:hasVersion rdf:resource="http://dublincore.org/usage/terms/history/#titleT-002"/>
  <dcterms:issued rdf:datatype="&xsd;date">2008-01-14</dcterms:issued>
  <dcterms:modified rdf:datatype="&xsd;date">2010-10-11</dcterms:modified>
  <rdfs:comment xml:lang="en">A name given to the resource.</rdfs:comment>
  <rdfs:isDefinedBy rdf:resource="&dcterms;"/>
  <rdfs:label xml:lang="en">Title</rdfs:label>
  <rdfs:range rdf:resource="&rdfs;Literal"/>
  <rdfs:subPropertyOf rdf:resource="&dc;title"/>
</rdf:Property>

<rdfs:Class rdf:about="&tmo;StateTypeRole"
    rdfs:label="StateTypeRole">
  <rdfs:comment>StateTypeRole is an abstract class which subsumes various other classes which represent "states" or roles e.g. in role based modelling conpetualisations.</rdfs:comment>
  <rdfs:subClassOf rdf:resource="&rdfs;Resource"/>
</rdfs:Class>

<rdfs:Class rdf:about="&nfo;Placemark"
    rdfs:label="Placemark">
  <rdfs:comment>One placemark within a placemark container/file. Use nie:title for the name/label, nao:creator for defining the creator.</rdfs:comment>
  <rdfs:subClassOf rdf:resource="&nie;InformationElement"/>
</rdfs:Class>

<rdf:Property rdf:about="&nid3;paymentURL"
    rdfs:label="paymentURL">
  <rdfs:comment>WPAY
The 'Payment' frame is a URL pointing at a webpage that will handle the process of paying for this file.</rdfs:comment>
  <rdfs:domain rdf:resource="&nid3;ID3Audio"/>
  <rdfs:range rdf:resource="&rdfs;Resource"/>
</rdf:Property>

<rdf:Property rdf:about="&dcon;currentNoise"
    rdfs:label="Current Noise">
  <rdfs:comment>Refers to a pre-defined environmental noise level characterising a context instance.</rdfs:comment>
  <rdfs:domain rdf:resource="&dcon;Environment"/>
  <rdfs:range rdf:resource="&dpo;Noise"/>
  <rdfs:subPropertyOf rdf:resource="&dcon;hasContextElement"/>
</rdf:Property>

<rdf:Property rdf:about="&nexif;gpsImgDirectionRef"
    rdfs:label="gpsImgDirectionRef">
  <rdfs:subPropertyOf rdf:resource="http://www.kanzaki.com/ns/exif#gpsImgDirectionRef"/>
  <rdfs:subPropertyOf rdf:resource="&nexif;gpsInfo"/>
  <rdfs:comment>tagNumber: 16
The reference for giving the direction of the image when it is captured. 'T' denotes true direction and 'M' is magnetic direction.</rdfs:comment>
  <rdfs:domain rdf:resource="&nexif;Photo"/>
  <rdfs:range rdf:resource="&xsd;string"/>
</rdf:Property>

<rdf:Property rdf:about="&nfo;lfeChannels"
    rdfs:comment="Number of Low Frequency Expansion (subwoofer) channels."
    rdfs:label="lfeChannels">
  <nrl:maxCardinality rdf:datatype="&xsd;integer">1</nrl:maxCardinality>
  <rdfs:range rdf:resource="&xsd;integer"/>
  <rdfs:subPropertyOf rdf:resource="&nfo;channels"/>
</rdf:Property>

<rdfs:Class rdf:about="&pimo;ClassOrThingOrPropertyOrAssociation"
    protege:role="abstract"
    rdfs:comment="Superclass of resources that can be generated by the user."
    rdfs:label="ClassOrThingOrPropertyOrAssociation">
  <pimo:classRole rdf:resource="&pimo;AbstractClass"/>
  <rdfs:subClassOf rdf:resource="&rdfs;Resource"/>
</rdfs:Class>

<rdf:Property rdf:about="&nao;isTagFor"
    rdfs:comment="States which resources a tag is associated with"
    rdfs:label="is tag for">
  <nrl:inverseProperty rdf:resource="&nao;hasTag"/>
  <rdfs:domain rdf:resource="&nao;Tag"/>
  <rdfs:range rdf:resource="&rdfs;Resource"/>
  <rdfs:subPropertyOf rdf:resource="&nao;annotation"/>
</rdf:Property>

<rdf:Property rdf:about="&nmm;setSize"
    rdfs:comment="The number of parts in the set."
    rdfs:label="set size">
  <nrl:maxCardinality rdf:datatype="&xsd;integer">1</nrl:maxCardinality>
  <rdfs:domain rdf:resource="&nmm;MusicAlbum"/>
  <rdfs:range rdf:resource="&xsd;integer"/>
</rdf:Property>

<rdfs:Class rdf:about="&ncal;RecurrenceIdentifier"
    rdfs:label="RecurrenceIdentifier">
  <rdfs:comment>Recurrence Identifier. Introduced to provide a structure for the value of ncal:recurrenceId property. See the documentation of ncal:recurrenceId for details.</rdfs:comment>
  <rdfs:subClassOf rdf:resource="&rdfs;Resource"/>
</rdfs:Class>

<rdf:Property rdf:about="&foaf;jabberID"
    rdfs:comment="A jabber ID for something."
    rdfs:label="jabber ID"
    ns:term_status="testing">
  <rdf:type rdf:resource="&owl;DatatypeProperty"/>
  <rdf:type rdf:resource="&owl;InverseFunctionalProperty"/>
  <rdfs:domain rdf:resource="&foaf;Agent"/>
  <rdfs:isDefinedBy rdf:resource="&foaf;"/>
  <rdfs:range rdf:resource="&rdfs;Literal"/>
</rdf:Property>

<rdf:Property rdf:about="&ncal;byweekno"
    rdfs:label="byweekno">
  <rdfs:comment>The number of the week an event should recur. Defined in RFC 2445 sec. 4.3.10</rdfs:comment>
  <rdfs:domain rdf:resource="&ncal;RecurrenceRule"/>
  <rdfs:range rdf:resource="&xsd;integer"/>
</rdf:Property>

<nrl:TransitiveProperty rdf:about="&dplo;repostOf"
    rdfs:label="repost of">
  <nrl:inverseProperty rdf:resource="&dplo;hasRepost"/>
  <nrl:maxCardinality rdf:datatype="&xsd;nonNegativeInteger">1</nrl:maxCardinality>
  <rdf:type rdf:resource="&rdf;Property"/>
  <rdfs:comment>Links to the original of a reposted livepost. This property is transitive, and is the inverse of dlpo:hasRepost.</rdfs:comment>
  <rdfs:domain rdf:resource="&dplo;LivePost"/>
  <rdfs:range rdf:resource="&dplo;LivePost"/>
</nrl:TransitiveProperty>

<rdfs:Class rdf:about="&ncal;AttendeeOrOrganizer"
    rdfs:comment="A common superclass for ncal:Attendee and ncal:Organizer."
    rdfs:label="AttendeeOrOrganizer">
  <rdfs:subClassOf rdf:resource="&rdfs;Resource"/>
</rdfs:Class>

<rdf:Property rdf:about="&dpo;maxBrightnessLevel"
    rdfs:label="Maximum Brightness Level">
  <rdfs:comment>A subproperty of dpo:maxValue that defines an upperbound on the observed brightness level value (in SI lux units) such that it can classify as a dpo:Brightness instance. It can be used in conjunction with dpo:minBrightnessLevel, i.e. specific instances of dpo:Brightness have a pre-defined range of observable real-world surrounding brightness levels.</rdfs:comment>
  <rdfs:domain rdf:resource="&dpo;Brightness"/>
  <rdfs:range rdf:resource="&xsd;float"/>
  <rdfs:subPropertyOf rdf:resource="&dpo;maxValue"/>
</rdf:Property>

<rdf:Property rdf:about="&tmo;createdBy"
    nrl:maxCardinality="1"
    rdfs:label="createdBy">
  <rdfs:domain rdf:resource="&tmo;Attachment"/>
  <rdfs:range rdf:resource="&pimo;Person"/>
</rdf:Property>

<rdf:Property rdf:about="&dcon;positiveInstance"
    rdfs:label="Positive Instance">
  <rdfs:comment>Situations are characterised through a series of past live context instances, required for its training. This property points to one or more positive instances, i.e., past actual live contexts snapshots during which it was determined that the abstract situation was active.</rdfs:comment>
  <rdfs:domain rdf:resource="&dcon;Situation"/>
  <rdfs:range rdf:resource="&duho;ContextLog"/>
</rdf:Property>

<rdfs:Class rdf:about="&ncal;RequestStatus"
    rdfs:label="RequestStatus">
  <rdfs:comment>Request Status. A class that was introduced to provide a structure for the value of ncal:requestStatus property. See documentation for ncal:requestStatus for details.</rdfs:comment>
  <rdfs:subClassOf rdf:resource="&rdfs;Resource"/>
</rdfs:Class>

<rdf:Property rdf:about="&nexif;exifVersion"
    rdfs:comment="tagNumber: 36864
Exif Version"
    rdfs:label="exifVersion">
  <rdfs:subPropertyOf rdf:resource="http://www.kanzaki.com/ns/exif#exifVersion"/>
  <rdfs:subPropertyOf rdf:resource="&nexif;versionInfo"/>
  <rdfs:domain rdf:resource="&nexif;Photo"/>
  <rdfs:range rdf:resource="&xsd;string"/>
</rdf:Property>

<rdf:Property rdf:about="&nid3;fileType"
    rdfs:label="fileType">
  <rdfs:comment>TFLT
The 'File type' frame indicates which type of audio this tag defines. The following type and refinements are defined: 
MPG MPEG Audio; 
/1 MPEG 1/2 layer I;
/2 MPEG 1/2 layer II;
/3 MPEG 1/2 layer III;
/2.5 MPEG 2.5;
/AAC Advanced audio compression;
VQF Transform-domain Weighted Interleave Vector Quantization;
PCM Pulse Code Modulated audio;</rdfs:comment>
  <rdfs:domain rdf:resource="&nid3;ID3Audio"/>
  <rdfs:range rdf:resource="&xsd;string"/>
</rdf:Property>

<rdf:Property rdf:about="&nexif;relatedFile"
    rdfs:comment="Tag Relating to Related File Information"
    rdfs:label="relatedFile">
  <rdfs:subPropertyOf rdf:resource="http://www.kanzaki.com/ns/exif#relatedFile"/>
  <rdfs:subPropertyOf rdf:resource="&nexif;exifAttribute"/>
  <rdfs:domain rdf:resource="&nexif;Photo"/>
  <rdfs:range rdf:resource="&xsd;string"/>
</rdf:Property>

<rdf:Property rdf:about="&nco;containsContact"
    rdfs:label="containsContact">
  <rdfs:comment>A property used to group contacts into contact groups. This 
    property was NOT defined in the VCARD standard. See documentation for the 
    'ContactList' class for details</rdfs:comment>
  <rdfs:domain rdf:resource="&nco;ContactList"/>
  <rdfs:range rdf:resource="&nco;ContactListDataObject"/>
  <rdfs:subPropertyOf rdf:resource="&nie;hasPart"/>
</rdf:Property>

<rdf:Property rdf:about="&ddo;carrierID"
    rdfs:comment="Attaches a human-readable name to a cellular network."
    rdfs:label="cellID">
  <rdfs:domain rdf:resource="&ddo;CellularNetwork"/>
  <rdfs:range rdf:resource="&xsd;string"/>
</rdf:Property>

<rdf:Property rdf:about="&nfo;horizontalResolution"
    rdfs:label="horizontalResolution">
  <nrl:maxCardinality rdf:datatype="&xsd;integer">1</nrl:maxCardinality>
  <rdfs:comment>Horizontal resolution of an image (if printed). Expressed in DPI.</rdfs:comment>
  <rdfs:domain rdf:resource="&nfo;Image"/>
  <rdfs:range rdf:resource="&xsd;integer"/>
</rdf:Property>

<rdf:Property rdf:about="&rdfs;label">
  <rdfs:comment xml:lang="en">A human-readable name for the subject.</rdfs:comment>
  <rdfs:domain rdf:resource="&rdfs;Resource"/>
  <rdfs:isDefinedBy rdf:resource="&rdfs;"/>
  <rdfs:label xml:lang="en">label</rdfs:label>
  <rdfs:range rdf:resource="&rdfs;Literal"/>
</rdf:Property>

<rdf:Property rdf:about="&nexif;pixelYDimension"
    rdfs:label="pixelYDimension">
  <rdfs:subPropertyOf rdf:resource="http://www.kanzaki.com/ns/exif#pixelYDimension"/>
  <rdfs:subPropertyOf rdf:resource="&nexif;height"/>
  <rdfs:subPropertyOf rdf:resource="&nexif;imageConfig"/>
  <rdfs:comment>Information specific to compressed data. When a compressed file is recorded, the valid height of the meaningful image shall be recorded in this tag, whether or not there is padding data or a restart marker. This tag should not exist in an uncompressed file. Since data padding is unnecessary in the vertical direction, the number of lines recorded in this valid image height tag will in fact be the same as that recorded in the SOF.
tagNumber: 40963</rdfs:comment>
  <rdfs:domain rdf:resource="&nexif;Photo"/>
  <rdfs:range rdf:resource="&xsd;integer"/>
</rdf:Property>

<rdf:Property rdf:about="&nao;identifier"
    rdfs:comment="Defines a generic identifier for a resource"
    rdfs:label="identifier">
  <rdfs:domain rdf:resource="&rdfs;Resource"/>
</rdf:Property>

<rdf:Property rdf:about="&dcterms;accrualMethod">
  <dcterms:hasVersion rdf:resource="http://dublincore.org/usage/terms/history/#accrualMethod-003"/>
  <dcterms:issued rdf:datatype="&xsd;date">2005-06-13</dcterms:issued>
  <dcterms:modified rdf:datatype="&xsd;date">2010-10-11</dcterms:modified>
  <rdfs:comment xml:lang="en">The method by which items are added to a collection.</rdfs:comment>
  <rdfs:domain rdf:resource="&dctypes;Collection"/>
  <rdfs:isDefinedBy rdf:resource="&dcterms;"/>
  <rdfs:label xml:lang="en">Accrual Method</rdfs:label>
  <rdfs:range rdf:resource="&dcterms;MethodOfAccrual"/>
</rdf:Property>

<rdfs:Class rdf:about="&dplo;BlogPost"
    rdfs:label="Blogpost">
  <rdfs:subClassOf rdf:resource="http://rdfs.org/sioc/types#BlogPost"/>
  <rdfs:subClassOf rdf:resource="&dplo;WebDocumentPost"/>
  <rdfs:comment>Represents a livepost referring to an online note, as defined by instances of nfo:RemoteDataObject, or known instances of pimo:Blogpost.</rdfs:comment>
</rdfs:Class>

<rdf:Property rdf:about="&nid3;publisher"
    rdfs:label="publisher">
  <rdfs:comment>TPUB
The 'Publisher' frame simply contains the name of the label or publisher.</rdfs:comment>
  <rdfs:domain rdf:resource="&nid3;ID3Audio"/>
  <rdfs:range rdf:resource="&nco;Contact"/>
  <rdfs:subPropertyOf rdf:resource="&nco;publisher"/>
</rdf:Property>

<rdf:Property rdf:about="&nco;gender"
    rdfs:comment="Gender of the given contact."
    rdfs:label="gender">
  <nrl:maxCardinality rdf:datatype="&xsd;integer">1</nrl:maxCardinality>
  <rdfs:domain rdf:resource="&nco;PersonContact"/>
  <rdfs:range rdf:resource="&nco;Gender"/>
</rdf:Property>

<rdf:Property rdf:about="&tmo;progress"
    nrl:maxCardinality="1"
    rdfs:label="progress">
  <rdfs:range rdf:resource="&rdfs;Literal"/>
</rdf:Property>

<rdf:Property rdf:about="&scos;broadMatch">
  <rdfs:subPropertyOf rdf:resource="&scos;broader"/>
  <rdfs:subPropertyOf rdf:resource="&scos;mappingRelation"/>
  <rdf:type rdf:resource="&owl;ObjectProperty"/>
  <rdfs:isDefinedBy rdf:resource="http://www.w3.org/2004/02/skos/core"/>
  <rdfs:label xml:lang="en">has broader match</rdfs:label>
  <owl:inverseOf rdf:resource="&scos;narrowMatch"/>
  <scos:definition xml:lang="en">skos:broadMatch is used to state a hierarchical mapping link between two conceptual resources in different concept schemes.</scos:definition>
</rdf:Property>

<rdf:Property rdf:about="&ncal;partstat"
    rdfs:label="partstat">
  <rdfs:comment>To specify the participation status for the calendar user specified by the property. Inspired by RFC 2445 sec. 4.2.12. Originally this parameter had three sets of allowed values. Which set applied to a particular case - depended on the type of calendar entity this parameter occured in. (event, todo, journal entry). This would be awkward to model in RDF so a single ParticipationStatus class has been introduced. Terms of the values vocabulary are expressed as instances of this class. Users are advised to pay attention which instances they use.</rdfs:comment>
  <rdfs:domain rdf:resource="&ncal;Attendee"/>
  <rdfs:range rdf:resource="&ncal;ParticipationStatus"/>
</rdf:Property>

<rdfs:Class rdf:about="&drmo;Action"
    rdfs:label="Action">
  <rdfs:comment>Defines the action(s) to be executed if a rule's conditions are satisfied. The Action class specifies an action instance (e.g. 'Notify'), whose semantics are understood by the system and result in specific actions being extracted. This corresponds to the consequent part of a production rule.</rdfs:comment>
</rdfs:Class>

<rdfs:Class rdf:about="&nexif;Photo"
    rdfs:label="Photo">
  <rdfs:subClassOf rdf:resource="http://www.kanzaki.com/ns/exif#IFD"/>
  <rdfs:subClassOf rdf:resource="&nfo;RasterImage"/>
  <rdfs:comment>A photo, an image captured using a camera, an EXIF Image File Directory. Implementation notes: use nie:copyright to store copyright notices.</rdfs:comment>
</rdfs:Class>

<rdf:Property rdf:about="&scos;hasTopConcept">
  <rdf:type rdf:resource="&owl;ObjectProperty"/>
  <rdfs:domain rdf:resource="&scos;ConceptScheme"/>
  <rdfs:isDefinedBy rdf:resource="http://www.w3.org/2004/02/skos/core"/>
  <rdfs:label xml:lang="en">has top concept</rdfs:label>
  <rdfs:range rdf:resource="&scos;Concept"/>
  <owl:inverseOf rdf:resource="&scos;topConceptOf"/>
  <scos:definition xml:lang="en">Relates, by convention, a concept scheme to a concept which is topmost in the broader/narrower concept hierarchies for that scheme, providing an entry point to these hierarchies.</scos:definition>
</rdf:Property>

<rdfs:Class rdf:about="&dpo;Direction"
    rdfs:label="Direction">
  <rdfs:comment>Quantifiable presence information concerning the agent's sensed absolute and relative altitude.</rdfs:comment>
  <rdfs:subClassOf rdf:resource="&dpo;QuantifiableComponent"/>
</rdfs:Class>

<ncal:AttendeeRole rdf:about="&ncal;optParticipantRole"
    rdfs:label="optParticipantRole"/>

<rdf:Property rdf:about="&pimo;roleContext"
    rdfs:label="role context">
  <rdfs:comment>The context where the role-holder impersonates this role. For example, the company where a person is employed.</rdfs:comment>
  <rdfs:domain rdf:resource="&pimo;PersonRole"/>
  <rdfs:range rdf:resource="&pimo;Thing"/>
  <rdfs:subPropertyOf rdf:resource="&pimo;associationMember"/>
</rdf:Property>

<rdf:Property rdf:about="&nie;copyright"
    rdfs:comment="Content copyright"
    rdfs:label="copyright">
  <rdfs:subPropertyOf rdf:resource="&dcterms;accessRights"/>
  <rdfs:subPropertyOf rdf:resource="&nie;legal"/>
  <rdfs:range rdf:resource="&xsd;string"/>
</rdf:Property>

<rdf:Property rdf:about="&nid3;musicCDIdentifier"
    rdfs:label="musicCDIdentifier">
  <rdfs:comment>This frame is intended for music that comes from a CD, so that the CD can be identified in databases such as the CDDB. The frame consists of a binary dump of the Table Of Contents, TOC, from the CD, which is a header of 4 bytes and then 8 bytes/track on the CD plus 8 bytes for the 'lead out' making a maximum of 804 bytes. The offset to the beginning of every track on the CD should be described with a four bytes absolute CD-frame address per track, and not with absolute time. This frame requires a present and valid "TRCK" frame, even if the CD's only got one track. There may only be one "MCDI" frame in each tag.</rdfs:comment>
  <rdfs:domain rdf:resource="&nid3;ID3Audio"/>
  <rdfs:range rdf:resource="&xsd;string"/>
</rdf:Property>

<rdfs:Class rdf:about="&cnt;ContentAsXML">
  <rdf:type rdf:resource="&owl;Class"/>
  <rdfs:comment xml:lang="en">The XML content (can only be used for XML-wellformed content).</rdfs:comment>
  <rdfs:label xml:lang="en">XML content</rdfs:label>
  <rdfs:subClassOf rdf:resource="&cnt;Content"/>
</rdfs:Class>

<nrl:DefiningProperty rdf:about="&nie;isPartOf"
    rdfs:label="isPartOf">
  <rdf:type rdf:resource="&nrl;FunctionalProperty"/>
  <rdf:type rdf:resource="&rdf;Property"/>
  <nao:userVisible rdf:datatype="&xsd;boolean">false</nao:userVisible>
  <nrl:inverseProperty rdf:resource="&nie;hasPart"/>
  <rdfs:comment>Generic property used to express containment relationships between DataObjects. NIE extensions are encouraged to provide more specific subproperties of this one. It is advisable for actual instances of DataObjects to use those specific subproperties. Note to the developers: Please be aware of the distinction between containment relation and provenance. The isPartOf relation models physical containment, a nie:DataObject (e.g. an nfo:Attachment) is a 'physical' part of an nie:InformationElement (a nmo:Message). Also, please note the difference between physical containment (isPartOf) and logical containment (isLogicalPartOf) the former has more strict meaning. They may occur independently of each other.</rdfs:comment>
  <rdfs:domain rdf:resource="&nie;DataObject"/>
  <rdfs:range rdf:resource="&nie;InformationElement"/>
  <rdfs:subPropertyOf rdf:resource="&dcterms;isPartOf"/>
</nrl:DefiningProperty>

<rdf:Property rdf:about="&drmo;hasPropertyOperator"
    rdfs:comment="Defines the relational operator for the condition value"
    rdfs:label="has property operator">
  <nrl:maxCardinality rdf:datatype="&xsd;nonNegativeInteger">1</nrl:maxCardinality>
  <rdfs:domain rdf:resource="&drmo;Condition"/>
  <rdfs:range rdf:resource="&xsd;string"/>
</rdf:Property>

<rdfs:Class rdf:about="&nid3;UserDefinedFrame"
    rdfs:label="UserDefinedFrame">
  <rdfs:comment>This frame is intended for one-string text information concerning the audiofile in a similar way to the other "T"-frames. The frame body consists of a description of the string, represented as a terminated string, followed by the actual string. There may be more than one "TXXX" frame in each tag, but only one with the same description.</rdfs:comment>
  <rdfs:subClassOf rdf:resource="&rdfs;Resource"/>
</rdfs:Class>

<owl:DatatypeProperty rdf:about="&oa;serializedAt">
  <rdfs:comment xml:lang="en">The time at which the agent referenced by oa:serializedBy generated the first serialization of the Annotation, and any subsequent substantially different one. The annotation graph MUST have changed for this property to be updated, and as such represents the last modified datestamp for the Annotation. This might be used to determine if it should be re-imported into a triplestore when discovered. 

There MAY be exactly 1 oa:serializedAt property per Annotation, and MUST NOT be more than 1. The datetime MUST be expressed in the xsd:dateTime format, and SHOULD have a timezone specified.</rdfs:comment>
  <rdfs:domain rdf:resource="&oa;Annotation"/>
  <rdfs:isDefinedBy rdf:resource="&oa;"/>
  <rdfs:label xml:lang="en">serializedAt</rdfs:label>
  <rdfs:range rdf:resource="&xsd;dateTimeStamp"/>
</owl:DatatypeProperty>

<rdf:Property rdf:about="&nexif;imageDescription"
    rdfs:label="imageDescription">
  <rdfs:subPropertyOf rdf:resource="http://www.kanzaki.com/ns/exif#imageDescription"/>
  <rdfs:subPropertyOf rdf:resource="&nie;title"/>
  <rdfs:subPropertyOf rdf:resource="&nexif;exifAttribute"/>
  <rdfs:comment>tagNumber: 270
A character string giving the title of the image. It may be a comment such as "1988 company picnic" or the like. Two-byte character codes cannot be used. When a 2-byte code is necessary, the Exif Private tag UserComment is to be used.</rdfs:comment>
  <rdfs:domain rdf:resource="&nexif;Photo"/>
  <rdfs:range rdf:resource="&xsd;string"/>
</rdf:Property>

<ncal:CalendarUserType rdf:about="&ncal;roomUserType"
    rdfs:label="roomUserType"/>

<rdfs:Class rdf:about="&ncal;TimezoneObservance"
    rdfs:label="TimezoneObservance">
  <rdfs:subClassOf rdf:resource="&ncal;UnionOfTimezoneObservanceEventFreebusyJournalTimezoneTodo"/>
  <rdfs:subClassOf rdf:resource="&ncal;UnionOfTimezoneObservanceEventFreebusyTimezoneTodo"/>
  <rdfs:subClassOf rdf:resource="&ncal;UnionOfTimezoneObservanceEventJournalTimezoneTodo"/>
</rdfs:Class>

<rdfs:Class rdf:about="&dcon;Context"
    rdfs:label="Context">
  <rdfs:comment>This RDF Graph contains information that can be used to characterise the state of an entity, where an entity can be a user's device or the user themselves. Although this abstract class is not intended for direct use, there are two main distinguishible subclasses. dcon:LiveContext represents uninterpreted states for a user's (multiple) devices, whereas dcon:Situation represents interpreted user states. There are three levels of representation for context: Aspects at the highest level, a set of Elements for each aspect, and a number of Attributes for each element.</rdfs:comment>
  <rdfs:subClassOf rdf:resource="&nrl;InstanceBase"/>
</rdfs:Class>

<owl:NamedIndividual rdf:about="&oa;editing">
  <rdf:type rdf:resource="&oa;Motivation"/>
  <rdfs:comment xml:lang="en">The motivation that represents a request for a modification or edit to the target resource. For example, an Annotation that requests a typo to be corrected.</rdfs:comment>
  <scos:inScheme rdf:resource="&oa;motivationScheme"/>
  <scos:prefLabel xml:lang="en">editing</scos:prefLabel>
</owl:NamedIndividual>

<owl:NamedIndividual rdf:about="&oa;moderating">
  <rdf:type rdf:resource="&oa;Motivation"/>
  <rdfs:comment xml:lang="en">The motivation that represents an assignment of value or quality to the target resource(s). For example annotating an Annotation to moderate it up in a trust network or threaded discussion.</rdfs:comment>
  <scos:inScheme rdf:resource="&oa;motivationScheme"/>
  <scos:prefLabel xml:lang="en">moderating</scos:prefLabel>
</owl:NamedIndividual>

<rdf:Property rdf:about="&pimo;associationEffectual"
    rdfs:label="association effectual during">
  <rdfs:comment>During which time is this association effective? If omitted, the association is always effective. Start time and end-time may be left open, an open start time indicates that the fact is unknown, an open end-time indicates that the end-date is either unknown or the association has not ended.
There can be multiple effectual periods.</rdfs:comment>
  <rdfs:domain rdf:resource="&pimo;Association"/>
  <rdfs:range rdf:resource="&rdfs;Resource"/>
</rdf:Property>

<rdf:Property rdf:about="&dpo;minMonth"
    rdfs:label="Minimum Month">
  <rdfs:comment>A subproperty of dpo:minValue that defines a lowerbound on the observed month (i.e., between 1 signifying January and 12 signifying December) such that it can classify as a dpo:TimePeriod instance. It can be used in conjunction with dpo:maxMonth, i.e. specific instances of dpo:TimePeriod have a pre-defined observable month number-based period.</rdfs:comment>
  <rdfs:domain rdf:resource="&dpo;TimePeriod"/>
  <rdfs:range rdf:resource="&xsd;integer"/>
  <rdfs:subPropertyOf rdf:resource="&dpo;maxValue"/>
</rdf:Property>

<rdf:Property rdf:about="&nexif;imageWidth"
    rdfs:label="imageWidth">
  <rdfs:subPropertyOf rdf:resource="http://www.kanzaki.com/ns/exif#imageWidth"/>
  <rdfs:subPropertyOf rdf:resource="&nexif;imageDataStruct"/>
  <rdfs:subPropertyOf rdf:resource="&nexif;width"/>
  <rdfs:comment>tagNumber: 256
Image width. The number of columns of image data, equal to the number of pixels per row. In JPEG compressed data a JPEG marker is used instead of this tag.</rdfs:comment>
  <rdfs:domain rdf:resource="&nexif;Photo"/>
  <rdfs:range rdf:resource="&xsd;integer"/>
</rdf:Property>

<rdfs:Class rdf:about="&nrl;DefiningProperty"
    rdfs:label="defining property">
  <rdfs:comment>A defining property's value is part of what defines a resource, changing it means
                          means chaning the identity of the resource. The set of values of all defining
                          properties of a resource make up its identify.
                          Whenever comparing resources or sharing them the value of this property should
                          be taken into account. By default all properties with a literal range are to be
                          treated as defining properties unless they are marked as nrl:NonDefiningProperty.</rdfs:comment>
  <rdfs:subClassOf rdf:resource="&rdf;Property"/>
</rdfs:Class>

<rdfs:Class rdf:about="&dplo;VideoPost"
    rdfs:label="Video Post">
  <rdfs:comment>Represents the live posting of a video file, or a link to an online media such as podcasts, videos, etc., as defined by instances of nfo:Video.</rdfs:comment>
  <rdfs:subClassOf rdf:resource="&dplo;MultimediaPost"/>
</rdfs:Class>

<rdf:Property rdf:about="&nfo;fontFamily"
    rdfs:comment="The name of the font family."
    rdfs:label="fontFamily">
  <nrl:maxCardinality rdf:datatype="&xsd;integer">1</nrl:maxCardinality>
  <rdfs:domain rdf:resource="&nfo;Font"/>
  <rdfs:range rdf:resource="&xsd;string"/>
</rdf:Property>

<rdf:Property rdf:about="&nid3;hasSynchronizedText"
    rdfs:comment="Links the ID3Audio with an instance of SynchronizedText"
    rdfs:label="hasSynchronizedText">
  <rdfs:domain rdf:resource="&nid3;ID3Audio"/>
  <rdfs:range rdf:resource="&nid3;SynchronizedText"/>
</rdf:Property>

<rdf:Property rdf:about="&scos;altLabel">
  <rdfs:comment xml:lang="en">The range of skos:altLabel is the class of RDF plain literals.</rdfs:comment>
  <rdfs:comment xml:lang="en">skos:prefLabel, skos:altLabel and skos:hiddenLabel are pairwise disjoint properties.</rdfs:comment>
  <rdf:type rdf:resource="&owl;AnnotationProperty"/>
  <rdfs:isDefinedBy rdf:resource="http://www.w3.org/2004/02/skos/core"/>
  <rdfs:label xml:lang="en">alternative label</rdfs:label>
  <rdfs:subPropertyOf rdf:resource="&rdfs;label"/>
  <scos:definition xml:lang="en">An alternative lexical label for a resource.</scos:definition>
  <scos:example xml:lang="en">Acronyms, abbreviations, spelling variants, and irregular plural/singular forms may be included among the alternative labels for a concept. Mis-spelled terms are normally included as hidden labels (see skos:hiddenLabel).</scos:example>
</rdf:Property>

<tmo:TransmissionState rdf:about="&tmo;TMO_Instance_TransmissionState_Accepted_Transmitted"
    rdfs:label="TMO_Instance_TransmissionState_Accepted_Transmitted"/>

<rdfs:Class rdf:about="&dctypes;Collection">
  <dcam:memberOf rdf:resource="&dcterms;DCMIType"/>
  <dcterms:description xml:lang="en">A collection is described as a group; its parts may also be separately described.</dcterms:description>
  <dcterms:hasVersion rdf:resource="http://dublincore.org/usage/terms/history/#Collection-003"/>
  <dcterms:issued rdf:datatype="&xsd;date">2000-07-11</dcterms:issued>
  <dcterms:modified rdf:datatype="&xsd;date">2008-01-14</dcterms:modified>
  <rdfs:comment xml:lang="en">An aggregation of resources.</rdfs:comment>
  <rdfs:isDefinedBy rdf:resource="&dctypes;"/>
  <rdfs:label xml:lang="en">Collection</rdfs:label>
</rdfs:Class>

<rdf:Property rdf:about="&nie;rootElementOf"
    rdfs:label="rootElementOf">
  <rdfs:comment>DataObjects extracted from a single data source are organized into a containment tree. This property links the root of that tree with the datasource it has been extracted from</rdfs:comment>
  <rdfs:domain rdf:resource="&nie;InformationElement"/>
  <rdfs:range rdf:resource="&nie;DataSource"/>
</rdf:Property>

<rdf:Property rdf:about="&ncal;ncalRelation"
    rdfs:label="ncalRelation">
  <rdfs:comment>A common superproperty for all types of ncal relations. It is not to be used directly.</rdfs:comment>
  <rdfs:domain rdf:resource="&ncal;UnionOfEventJournalTodo"/>
  <rdfs:range rdf:resource="&xsd;string"/>
  <rdfs:subPropertyOf rdf:resource="&dc;relation"/>
</rdf:Property>

<rdfs:Class rdf:about="&dplo;Status"
    rdfs:comment="Represents a status message, tweet, etc. shared by a user."
    rdfs:label="Status Message">
  <rdfs:subClassOf rdf:resource="&dplo;Message"/>
</rdfs:Class>

<rdf:Property rdf:about="&foaf;accountName"
    rdfs:label="account name"
    ns:term_status="testing">
  <rdf:type rdf:resource="&owl;DatatypeProperty"/>
  <rdfs:comment>Indicates the name (identifier) associated with this online account.</rdfs:comment>
  <rdfs:domain rdf:resource="&foaf;OnlineAccount"/>
  <rdfs:isDefinedBy rdf:resource="&foaf;"/>
  <rdfs:range rdf:resource="&rdfs;Literal"/>
</rdf:Property>

<rdf:Property rdf:about="&nid3;synchronizedTextContentDescriptor"
    rdfs:label="synchronizedTextContentDescriptor">
  <rdfs:comment>Synchronized text content descriptor. Inspired by the content descriptor part of the SYLT frame defined in ID3 2.3.0 spec sec. 4.10</rdfs:comment>
  <rdfs:domain rdf:resource="&nid3;SynchronizedText"/>
  <rdfs:range rdf:resource="&xsd;string"/>
</rdf:Property>

<rdfs:Class rdf:about="&dcterms;Standard">
  <dcterms:hasVersion rdf:resource="http://dublincore.org/usage/terms/history/#Standard-001"/>
  <dcterms:issued rdf:datatype="&xsd;date">2008-01-14</dcterms:issued>
  <rdfs:comment xml:lang="en">A basis for comparison; a reference point against which other things can be evaluated.</rdfs:comment>
  <rdfs:isDefinedBy rdf:resource="&dcterms;"/>
  <rdfs:label xml:lang="en">Standard</rdfs:label>
</rdfs:Class>

<rdfs:Class rdf:about="&pimo;Country"
    rdfs:label="Country">
  <rdfs:comment>The territory occupied by a nation; "he returned to the land of his birth"; "he visited several European countries". (Definition from SUMO)</rdfs:comment>
  <rdfs:subClassOf rdf:resource="&pimo;Location"/>
</rdfs:Class>

<rdfs:Datatype rdf:about="&dcterms;Box">
  <dcterms:hasVersion rdf:resource="http://dublincore.org/usage/terms/history/#Box-003"/>
  <dcterms:issued rdf:datatype="&xsd;date">2000-07-11</dcterms:issued>
  <dcterms:modified rdf:datatype="&xsd;date">2008-01-14</dcterms:modified>
  <rdfs:comment xml:lang="en">The set of regions in space defined by their geographic coordinates according to the DCMI Box Encoding Scheme.</rdfs:comment>
  <rdfs:isDefinedBy rdf:resource="&dcterms;"/>
  <rdfs:label xml:lang="en">DCMI Box</rdfs:label>
  <rdfs:seeAlso rdf:resource="http://dublincore.org/documents/dcmi-box/"/>
</rdfs:Datatype>

<rdf:Property rdf:about="&dcon;currentEvent"
    rdfs:label="Current Event">
  <rdfs:comment>Refers to an ongoing event characterising a context instance.</rdfs:comment>
  <rdfs:domain rdf:resource="&dcon;Schedule"/>
  <rdfs:range rdf:resource="&ncal;Event"/>
  <rdfs:subPropertyOf rdf:resource="&dcon;hasContextElement"/>
</rdf:Property>

<rdf:Property rdf:about="&tmo;endTime"
    nrl:maxCardinality="1"
    rdfs:label="endTime">
  <rdfs:range rdf:resource="&xsd;dateTime"/>
  <rdfs:subPropertyOf rdf:resource="&tmo;dateTime"/>
</rdf:Property>

<rdf:Property rdf:about="&drmo;hasConstraintOnProperty"
    rdfs:label="has constraint on property">
  <rdfs:comment>Places a constraint on a condition (i.e., the domain defined for this property), such that the referred property (i.e., the range defined for this property) must have a specific value. The restricted value is defined by the use of either drmo:hasConstraintOnSubject or drmo:hasConstraintOnObject, which therefore must always be used in conjunction with this property. The constrained property in combination with the constrained subject/object are then used to query triples matching this pattern.</rdfs:comment>
  <rdfs:domain rdf:resource="&drmo;Condition"/>
  <rdfs:range rdf:resource="&rdf;Property"/>
</rdf:Property>

<rdf:Property rdf:about="&nexif;gpsInfoIFDPointer"
    rdfs:label="gpsInfoIFDPointer">
  <rdfs:subPropertyOf rdf:resource="http://www.kanzaki.com/ns/exif#gpsInfo_IFD_Pointer"/>
  <rdfs:subPropertyOf rdf:resource="&nexif;ifdPointer"/>
  <rdfs:comment>A pointer to the GPS IFD, which is a set of tags for recording GPS information.
tagNumber: 34853</rdfs:comment>
  <rdfs:domain rdf:resource="&nexif;Photo"/>
  <rdfs:range rdf:resource="&nexif;Photo"/>
</rdf:Property>

<rdf:Property rdf:about="&nexif;make"
    rdfs:comment="Manufacturer of image input equipment
tagNumber: 271"
    rdfs:label="make">
  <rdfs:subPropertyOf rdf:resource="http://www.kanzaki.com/ns/exif#make"/>
  <rdfs:subPropertyOf rdf:resource="&nexif;exifAttribute"/>
  <rdfs:domain rdf:resource="&nexif;Photo"/>
  <rdfs:range rdf:resource="&xsd;string"/>
</rdf:Property>

<dcam:VocabularyEncodingScheme rdf:about="&dcterms;DCMIType">
  <dcterms:hasVersion rdf:resource="http://dublincore.org/usage/terms/history/#DCMIType-005"/>
  <dcterms:issued rdf:datatype="&xsd;date">2000-07-11</dcterms:issued>
  <dcterms:modified rdf:datatype="&xsd;date">2012-06-14</dcterms:modified>
  <rdfs:comment xml:lang="en">The set of classes specified by the DCMI Type Vocabulary, used to categorize the nature or genre of the resource.</rdfs:comment>
  <rdfs:isDefinedBy rdf:resource="&dcterms;"/>
  <rdfs:label xml:lang="en">DCMI Type Vocabulary</rdfs:label>
  <rdfs:seeAlso rdf:resource="&dctypes;"/>
</dcam:VocabularyEncodingScheme>

<rdfs:Class rdf:about="&duho;Log"
    rdfs:label="Log">
  <rdfs:comment>A log documenting a direct or indirect aspect of user history. This includes logging changing resources such as user activities, contexts, preferences, or events in the user's system. Logging can be initiated by the user, by the system, or be set to execute automatically every period of time. Logs are instances of named graphs, and thus will contain a set of descriptive triples. The contained descriptions are bound to the logging time, and may thus no longer be valid at a later time.</rdfs:comment>
  <rdfs:subClassOf rdf:resource="&nrl;InstanceBase"/>
</rdfs:Class>

<nrl:SymmetricProperty rdf:about="&nao;isRelated"
    rdfs:label="is related to">
  <rdf:type rdf:resource="&rdf;Property"/>
  <rdfs:comment>Defines an annotation for a resource in the form of a relationship between the subject resource and another resource</rdfs:comment>
  <rdfs:range rdf:resource="&rdfs;Resource"/>
  <rdfs:subPropertyOf rdf:resource="&nao;annotation"/>
</nrl:SymmetricProperty>

<rdf:Property rdf:about="&tmo;stateTypeRole"
    nrl:maxCardinality="1"
    rdfs:label="stateTypeRole">
  <rdfs:range rdf:resource="&rdfs;Resource"/>
</rdf:Property>

<rdf:Property rdf:about="&dpo;minDayOfWeek"
    rdfs:label="Minimum Day of the Week">
  <rdfs:comment>A subproperty of dpo:minValue that defines a lowerbound on the observed day of the week (i.e., between 1 signifying Monday and 7 signifying Sunday) such that it can classify as a dpo:TimePeriod instance. It can be used in conjunction with dpo:maxDayOfWeek, i.e. specific instances of dpo:TimePeriod have a pre-defined observable 7-day week-based period.</rdfs:comment>
  <rdfs:domain rdf:resource="&dpo;TimePeriod"/>
  <rdfs:range rdf:resource="&xsd;integer"/>
  <rdfs:subPropertyOf rdf:resource="&dpo;maxValue"/>
</rdf:Property>

<rdf:Property rdf:about="&tmo;involvedPersonTask"
    nrl:maxCardinality="1"
    rdfs:label="involvedPersonTask">
  <nrl:inverseProperty rdf:resource="&tmo;involvedPersons"/>
  <rdfs:domain rdf:resource="&tmo;PersonInvolvement"/>
  <rdfs:range rdf:resource="&tmo;Task"/>
  <rdfs:subPropertyOf rdf:resource="&pimo;associationMember"/>
</rdf:Property>

<rdf:Property rdf:about="&ncal;bysetpos"
    rdfs:label="bysetpos">
  <rdfs:comment>The BYSETPOS rule part specify values which correspond to the nth occurrence within the set of events specified by the rule. Valid values are 1 to 366 or -366 to -1. It MUST only be used in conjunction with another BYxxx rule part. For example "the last work day of the month" could be represented as: RRULE: FREQ=MONTHLY; BYDAY=MO, TU, WE, TH, FR; BYSETPOS=-1. Each BYSETPOS value can include a positive (+n) or negative (-n)  integer. If present, this indicates the nth occurrence of the  specific occurrence within the set of events specified by the rule. Defined in RFC 2445 sec. 4.3.10</rdfs:comment>
  <rdfs:domain rdf:resource="&ncal;RecurrenceRule"/>
  <rdfs:range rdf:resource="&xsd;integer"/>
</rdf:Property>

<dcam:VocabularyEncodingScheme rdf:about="&dcterms;UDC">
  <dcterms:hasVersion rdf:resource="http://dublincore.org/usage/terms/history/#UDC-003"/>
  <dcterms:issued rdf:datatype="&xsd;date">2000-07-11</dcterms:issued>
  <dcterms:modified rdf:datatype="&xsd;date">2008-01-14</dcterms:modified>
  <rdfs:comment xml:lang="en">The set of conceptual resources specified by the Universal Decimal Classification.</rdfs:comment>
  <rdfs:isDefinedBy rdf:resource="&dcterms;"/>
  <rdfs:label xml:lang="en">UDC</rdfs:label>
  <rdfs:seeAlso rdf:resource="http://www.udcc.org/"/>
</dcam:VocabularyEncodingScheme>

<rdf:Property rdf:about="&pimo;objectProperty"
    rdfs:label="object property">
  <rdfs:comment>The object of statements is another Thing. Users should be able to edit statements defined with this property. Abstract super-property.</rdfs:comment>
  <rdfs:domain rdf:resource="&pimo;Thing"/>
  <rdfs:range rdf:resource="&pimo;Thing"/>
</rdf:Property>

<rdf:Property rdf:about="&nexif;orientation"
    rdfs:label="orientation">
  <rdfs:subPropertyOf rdf:resource="http://www.kanzaki.com/ns/exif#orientation"/>
  <rdfs:subPropertyOf rdf:resource="&nexif;imageDataStruct"/>
  <rdfs:comment>The image orientation viewed in terms of rows and columns. As defined in the EXIF specification this is a number between 1 and 8.</rdfs:comment>
  <rdfs:domain rdf:resource="&nexif;Photo"/>
  <rdfs:range rdf:resource="&xsd;integer"/>
</rdf:Property>

<rdf:Property rdf:about="&nuao;totalModificationDuration"
    rdfs:comment="The total duration of all modifications"
    rdfs:label="modification count">
  <nrl:maxCardinality rdf:datatype="&xsd;nonNegativeInteger">1</nrl:maxCardinality>
  <rdfs:domain rdf:resource="&rdfs;Resource"/>
  <rdfs:range rdf:resource="&xsd;duration"/>
</rdf:Property>

<owl:NamedIndividual rdf:about="&oa;commenting">
  <rdf:type rdf:resource="&oa;Motivation"/>
  <rdfs:comment xml:lang="en">The motivation that represents a commentary about or review of the target resource(s). For example to provide a commentary about a particular PDF.</rdfs:comment>
  <scos:inScheme rdf:resource="&oa;motivationScheme"/>
  <scos:prefLabel xml:lang="en">commenting</scos:prefLabel>
</owl:NamedIndividual>

<ncal:Weekday rdf:about="&ncal;saturday"
    rdfs:label="saturday"/>

<ncal:Weekday rdf:about="&ncal;monday"
    rdfs:label="monday"/>

<rdf:Property rdf:about="&nexif;yCbCrSubSampling"
    rdfs:label="yCbCrSubSampling">
  <rdfs:subPropertyOf rdf:resource="http://www.kanzaki.com/ns/exif#yCbCrSubSampling"/>
  <rdfs:subPropertyOf rdf:resource="&nexif;imageDataStruct"/>
  <rdfs:comment>The sampling ratio of chrominance components in relation to the luminance component. In JPEG compressed data a JPEG marker is used instead of this tag.
tagNumber: 530</rdfs:comment>
  <rdfs:domain rdf:resource="&nexif;Photo"/>
  <rdfs:range rdf:resource="&xsd;string"/>
</rdf:Property>

<rdf:Property rdf:about="&nfo;bitDepth"
    rdfs:label="bitDepth">
  <nrl:maxCardinality rdf:datatype="&xsd;integer">1</nrl:maxCardinality>
  <rdfs:comment>A common superproperty for all properties signifying the amount of bits for an atomic unit of data. Examples of subproperties may include bitsPerSample and bitsPerPixel</rdfs:comment>
  <rdfs:domain rdf:resource="&nfo;Media"/>
  <rdfs:range rdf:resource="&rdfs;Literal"/>
</rdf:Property>

<rdfs:Class rdf:about="&pimo;BlogPost"
    rdfs:label="Blog Post">
  <rdfs:comment>A blog note. You just want to write something down right now and need a place to do that. Add a blog-note! This is an example class for a document type, there are more detailled ontologies to model Blog-Posts (like SIOC).</rdfs:comment>
  <rdfs:subClassOf rdf:resource="&pimo;Document"/>
</rdfs:Class>

<rdf:Property rdf:about="&nid3;originalTextWriter"
    rdfs:label="originalTextWriter">
  <rdfs:comment>TOLY
The 'Original lyricist(s)/text writer(s)' frame is intended for the text writer(s) of the original recording, if for example the music in the file should be a cover of a previously released song. The text writers are seperated with the "/" character.
Note that in the RDF representation each original lyricist is represented with a separate triple.</rdfs:comment>
  <rdfs:domain rdf:resource="&nid3;ID3Audio"/>
  <rdfs:range rdf:resource="&nco;Contact"/>
  <rdfs:subPropertyOf rdf:resource="&nco;contributor"/>
</rdf:Property>

<rdf:Property rdf:about="&nid3;internationalStandardRecordingCode"
    rdfs:label="internationalStandardRecordingCode">
  <rdfs:comment>TSRC
The 'ISRC' frame should contain the International Standard Recording Code (ISRC) (12 characters).</rdfs:comment>
  <rdfs:domain rdf:resource="&nid3;ID3Audio"/>
  <rdfs:range rdf:resource="&xsd;string"/>
</rdf:Property>

<rdfs:Class rdf:about="&nuao;FocusEvent"
    rdfs:label="focus event">
  <rdfs:comment>An event which refers to the timespan in which a resource was in the focus of the user.</rdfs:comment>
  <rdfs:subClassOf rdf:resource="&nuao;DesktopEvent"/>
</rdfs:Class>

<rdf:Property rdf:about="&nexif;tagid"
    rdfs:label="tagid">
  <rdfs:subPropertyOf rdf:resource="http://www.kanzaki.com/ns/exif#tagid"/>
  <rdfs:subPropertyOf rdf:resource="&nexif;tagNumber"/>
  <rdfs:comment>The Exif tag number with context prefix, such as IFD type or maker name (for this schema definition)</rdfs:comment>
  <rdfs:domain rdf:resource="&nexif;Photo"/>
  <rdfs:range rdf:resource="&xsd;string"/>
</rdf:Property>

<rdf:Property rdf:about="&ncal;geo"
    rdfs:label="geo">
  <nrl:maxCardinality rdf:datatype="&xsd;integer">1</nrl:maxCardinality>
  <rdfs:comment>This property specifies information related to the global position for the activity specified by a calendar component. Inspired by RFC 2445 sec. 4.8.1.6</rdfs:comment>
  <rdfs:domain rdf:resource="&ncal;UnionOfEventTodo"/>
  <rdfs:range rdf:resource="http://www.w3.org/2003/01/geo/wgs84_pos#Point"/>
</rdf:Property>

<rdfs:Class rdf:about="&nrl;KnowledgeBase"
    rdfs:label="KnowledgeBase">
  <rdfs:subClassOf rdf:resource="&nrl;InstanceBase"/>
  <rdfs:subClassOf rdf:resource="&nrl;Ontology"/>
  <rdfs:comment>Represents a named graph containing both schematic and instance data</rdfs:comment>
</rdfs:Class>

<rdf:Property rdf:about="&nexif;subseconds"
    rdfs:label="subseconds">
  <rdfs:comment>A tag used to record fractions of seconds for a date property</rdfs:comment>
  <rdfs:domain rdf:resource="&nexif;Photo"/>
  <rdfs:range rdf:resource="&xsd;string"/>
  <rdfs:subPropertyOf rdf:resource="http://www.kanzaki.com/ns/exif#subseconds"/>
</rdf:Property>

<owl:ObjectProperty rdf:about="&oa;hasTarget">
  <rdfs:comment xml:lang="en">The relationship between oa:Annotation and target. The target resource is what the oa:hasBody is somewhat "about".

The target may be of any media type, and contain any type of content. The target SHOULD be identified by HTTP URIs unless they are embedded within the Annotation.

Embedded targets SHOULD be instances of cnt:ContentAsText and embed their content with cnt:chars. They SHOULD declare their media type with dc:format, and MAY indicate their language using dc:language and a RFC-3066 language tag. 

There is no OA class provided for "Target" as a target might be a body in a different annotation. However, there SHOULD be 1 or more content-based classes associated with the target resources of an Annotation, and the dctypes: vocabulary is recommended for this purpose, for instance dctypes:Text to declare textual content.</rdfs:comment>
  <rdfs:domain rdf:resource="&oa;Annotation"/>
  <rdfs:isDefinedBy rdf:resource="&oa;"/>
  <rdfs:label xml:lang="en">hasTarget</rdfs:label>
</owl:ObjectProperty>

<tmo:Urgency rdf:about="&tmo;TMO_Instance_Urgency_05"
    rdfs:label="TMO_Instance_Urgency_05"/>

<rdf:Property rdf:about="&dpo;minAbsoluteAltitude"
    rdfs:label="Minimum Absolute Altitude">
  <rdfs:comment>A variant subproperty of dpo:minAltitude that defines a lowerbound on the computed absolute altitude (i.e. altitude relative to the level of the terrain in the area), rather the observed true altitude. Can be in conjunction with dpo:maxAbsoulateAltitude.</rdfs:comment>
  <rdfs:domain rdf:resource="&dpo;Altitude"/>
  <rdfs:range rdf:resource="&xsd;float"/>
  <rdfs:subPropertyOf rdf:resource="&dpo;minValue"/>
</rdf:Property>

<rdf:Property rdf:about="&tmo;dependencyType"
    nrl:maxCardinality="1"
    nrl:minCardinality="1"
    rdfs:label="dependencyType">
  <rdfs:range rdf:resource="&rdfs;Resource"/>
</rdf:Property>

<rdf:Property rdf:about="&nfo;bitsPerSample"
    rdfs:comment="Amount of bits in each audio sample."
    rdfs:label="bitsPerSample">
  <nrl:maxCardinality rdf:datatype="&xsd;integer">1</nrl:maxCardinality>
  <rdfs:domain rdf:resource="&nfo;Audio"/>
  <rdfs:range rdf:resource="&xsd;integer"/>
  <rdfs:subPropertyOf rdf:resource="&nfo;bitDepth"/>
</rdf:Property>

<rdf:Property rdf:about="&ncal;dir"
    rdfs:label="dir">
  <rdfs:comment>Specifies a reference to a directory entry associated with the calendar user specified by the property. Inspired by RFC 2445 sec. 4.2.6. Originally the data type of the value of this parameter was URI (Usually an LDAP URI). This has been expressed as rdfs:resource.</rdfs:comment>
  <rdfs:domain rdf:resource="&ncal;AttendeeOrOrganizer"/>
  <rdfs:range rdf:resource="&rdfs;Resource"/>
</rdf:Property>

<rdf:Property rdf:about="&nmm;audienceRating"
    rdfs:label="audience rating">
  <rdfs:comment>Rating used to identify appropriate audience for video (MPAA rating, BBFC, FSK, TV content rating, etc.)</rdfs:comment>
  <rdfs:domain rdf:resource="&nfo;Video"/>
  <rdfs:range rdf:resource="&xsd;string"/>
  <rdfs:subPropertyOf rdf:resource="&nao;rating"/>
</rdf:Property>

<rdf:Property rdf:about="&nco;photo"
    rdfs:label="photo">
  <rdfs:comment>Photograph attached to a Contact. The DataObject referred to by this property is usually interpreted as an nfo:Image. Inspired by the PHOTO property defined in RFC 2426 sec. 3.1.4</rdfs:comment>
  <rdfs:domain rdf:resource="&nco;Contact"/>
  <rdfs:range rdf:resource="&nie;DataObject"/>
  <rdfs:subPropertyOf rdf:resource="&nie;hasPart"/>
</rdf:Property>

<rdf:Property rdf:about="&tmo;subTaskOrdering"
    nrl:maxCardinality="1"
    rdfs:label="subTaskOrdering">
  <rdfs:comment>Ordering of the subtasks listed in the tmo:subTasks property of this Task. This is only for ordering/sorting in GUIs, the semantic relation is defined in subTasks, and if this and subTasks differ, subTasks is the correct list.</rdfs:comment>
  <rdfs:domain rdf:resource="&tmo;Task"/>
  <rdfs:range rdf:resource="&rdf;List"/>
</rdf:Property>

<rdfs:Class rdf:about="&nfo;RemotePortAddress"
    rdfs:label="RemotePortAddress">
  <rdfs:comment>An address specifying a remote host and port. Such an address can be interpreted in many ways (examples of such interpretations include mailboxes, websites, remote calendars or filesystems), depending on an interpretation, various kinds of data may be extracted from such an address.</rdfs:comment>
  <rdfs:subClassOf rdf:resource="&nie;DataObject"/>
</rdfs:Class>

<rdf:Property rdf:about="&nexif;gpsAreaInformation"
    rdfs:label="gpsAreaInformation">
  <rdfs:subPropertyOf rdf:resource="http://www.kanzaki.com/ns/exif#gpsAreaInformation"/>
  <rdfs:subPropertyOf rdf:resource="&nexif;gpsInfo"/>
  <rdfs:comment>A character string recording the name of the GPS area. The first byte indicates the character code used, and this is followed by the name of the GPS area.
tagNumber: 28</rdfs:comment>
  <rdfs:domain rdf:resource="&nexif;Photo"/>
  <rdfs:range rdf:resource="&xsd;string"/>
</rdf:Property>

<rdf:Property rdf:about="&nie;generator"
    rdfs:label="generator">
  <rdfs:comment>Software used to "generate" the contents. E.g. a word processor name.</rdfs:comment>
  <rdfs:domain rdf:resource="&nie;InformationElement"/>
  <rdfs:range rdf:resource="&xsd;string"/>
</rdf:Property>

<nrl:DefiningProperty rdf:about="&nmm;actor"
    rdfs:comment="Actor"
    rdfs:label="actor">
  <rdf:type rdf:resource="&rdf;Property"/>
  <rdfs:domain rdf:resource="&nfo;Video"/>
  <rdfs:range rdf:resource="&nco;Contact"/>
  <rdfs:subPropertyOf rdf:resource="&nco;contributor"/>
</nrl:DefiningProperty>

<rdf:Property rdf:about="&nco;imStatusType"
    rdfs:label="instant messaging status type">
  <nrl:maxCardinality rdf:datatype="&xsd;integer">1</nrl:maxCardinality>
  <rdfs:comment>Current status type of the given IM account. When this property is set, the nco:imStatus property should also always be set. Applications should attempt to parse the nco:imStatus property to determine the presence, only falling back to this property in the case that the nco:imStatus property's value is unrecognised.</rdfs:comment>
  <rdfs:domain rdf:resource="&nco;IMAccount"/>
  <rdfs:range rdf:resource="&nco;IMStatusType"/>
</rdf:Property>

<rdfs:Class rdf:about="&nrl;ViewSpecification"
    rdfs:label="ViewSpecification">
  <rdfs:comment>Represents a specification of the means to achieve a transformation of an input graph into the required graph view</rdfs:comment>
  <rdfs:subClassOf rdf:resource="&rdfs;Resource"/>
</rdfs:Class>

<tmo:TaskContainer rdf:about="&tmo;TMO_Instance_TaskContainer_activetasks"
    rdfs:label="TMO_Instance_TaskContainer_activetasks"/>

<rdfs:Datatype rdf:about="&dcterms;ISO639-3">
  <dcterms:hasVersion rdf:resource="http://dublincore.org/usage/terms/history/#ISO639-3-001"/>
  <dcterms:issued rdf:datatype="&xsd;date">2008-01-14</dcterms:issued>
  <rdfs:comment xml:lang="en">The set of three-letter codes listed in ISO 639-3 for the representation of names of languages.</rdfs:comment>
  <rdfs:isDefinedBy rdf:resource="&dcterms;"/>
  <rdfs:label xml:lang="en">ISO 639-3</rdfs:label>
  <rdfs:seeAlso rdf:resource="http://www.sil.org/iso639-3/"/>
</rdfs:Datatype>

<rdf:Property rdf:about="&dcon;latitude"
    rdfs:comment="Records the exact latitude of the approximated location"
    rdfs:label="GPS Latitude">
  <rdfs:domain rdf:resource="&pimo;Location"/>
  <rdfs:range rdf:resource="&xsd;float"/>
  <rdfs:subPropertyOf rdf:resource="&dcon;hasContextAttribute"/>
</rdf:Property>

<rdfs:Class rdf:about="&dcterms;MethodOfAccrual">
  <dcterms:hasVersion rdf:resource="http://dublincore.org/usage/terms/history/#MethodOfAccrual-001"/>
  <dcterms:issued rdf:datatype="&xsd;date">2008-01-14</dcterms:issued>
  <rdfs:comment xml:lang="en">A method by which resources are added to a collection.</rdfs:comment>
  <rdfs:isDefinedBy rdf:resource="&dcterms;"/>
  <rdfs:label xml:lang="en">Method of Accrual</rdfs:label>
</rdfs:Class>

<rdfs:Class rdf:about="&ncal;RecurrenceRule"
    rdfs:label="RecurrenceRule">
  <rdfs:subClassOf rdf:resource="&rdfs;Resource"/>
</rdfs:Class>

<rdfs:Class rdf:about="&nco;PhoneNumber"
    rdfs:comment="A telephone number."
    rdfs:label="PhoneNumber">
  <rdfs:subClassOf rdf:resource="&nco;ContactMedium"/>
</rdfs:Class>

<rdfs:Class rdf:about="&nfo;Folder"
    rdfs:label="Folder">
  <rdfs:comment>A folder/directory. Examples of folders include folders on a filesystem and message folders in a mailbox.</rdfs:comment>
  <rdfs:subClassOf rdf:resource="&nfo;DataContainer"/>
</rdfs:Class>

<rdf:Property rdf:about="&nfo;uuid"
    rdfs:label="uuid">
  <rdfs:comment>Universally unique identifier of the filesystem. In the future, this property may have its parent changed to a more generic class.</rdfs:comment>
  <rdfs:domain rdf:resource="&nfo;Filesystem"/>
  <rdfs:range rdf:resource="&xsd;string"/>
  <rdfs:subPropertyOf rdf:resource="&nie;identifier"/>
</rdf:Property>

<rdf:Property rdf:about="&tmo;taskSource"
    nrl:maxCardinality="1"
    rdfs:label="taskSource">
  <rdfs:comment>here can be stated from which sources a task was derived. e.g from another task or from an task pattern</rdfs:comment>
  <rdfs:domain rdf:resource="&tmo;Task"/>
  <rdfs:range rdf:resource="&rdfs;Resource"/>
  <rdfs:subPropertyOf rdf:resource="&tmo;taskReference"/>
</rdf:Property>

<rdf:Property rdf:about="&foaf;fundedBy"
    rdfs:comment="An organization funding a project or person."
    rdfs:label="funded by"
    ns:term_status="archaic">
  <rdf:type rdf:resource="&owl;ObjectProperty"/>
  <rdfs:domain rdf:resource="&owl;Thing"/>
  <rdfs:isDefinedBy rdf:resource="&foaf;"/>
  <rdfs:range rdf:resource="&owl;Thing"/>
</rdf:Property>

<ncal:RecurrenceFrequency rdf:about="&ncal;hourly"
    rdfs:label="hourly"/>

<rdf:Property rdf:about="&rdf;first">
  <rdfs:comment xml:lang="en">The first item in the subject RDF list.</rdfs:comment>
  <rdfs:domain rdf:resource="&rdf;List"/>
  <rdfs:isDefinedBy rdf:resource="&rdf;"/>
  <rdfs:label xml:lang="en">first</rdfs:label>
  <rdfs:range rdf:resource="&rdfs;Resource"/>
</rdf:Property>

<rdf:Property rdf:about="&dcon;currentAvailability"
    rdfs:label="Current Availability">
  <rdfs:comment>Refers to a pre-defined personal availability characterising a context instance.</rdfs:comment>
  <rdfs:domain rdf:resource="&dcon;State"/>
  <rdfs:range rdf:resource="&dpo;Availability"/>
  <rdfs:subPropertyOf rdf:resource="&dcon;hasContextElement"/>
</rdf:Property>

<rdfs:Class rdf:about="&nrl;FunctionalProperty"
    rdfs:comment="A marker class to identify functional properties"
    rdfs:label="FunctionalProperty">
  <rdfs:subClassOf rdf:resource="&rdfs;Resource"/>
</rdfs:Class>

<rdf:Property rdf:about="&nexif;spectralSensitivity"
    rdfs:label="spectralSensitivity">
  <rdfs:subPropertyOf rdf:resource="http://www.kanzaki.com/ns/exif#spectralSensitivity"/>
  <rdfs:subPropertyOf rdf:resource="&nexif;pictTaking"/>
  <rdfs:comment>Indicates the spectral sensitivity of each channel of the camera used. The tag value is an ASCII string compatible with the standard developed by the ASTM Technical committee.
tagNumber: 34852</rdfs:comment>
  <rdfs:domain rdf:resource="&nexif;Photo"/>
  <rdfs:range rdf:resource="&xsd;string"/>
</rdf:Property>

<rdf:Property rdf:about="&nexif;subSecTime"
    rdfs:comment="tagNumber: 37520
DateTime subseconds"
    rdfs:label="subSecTime">
  <rdfs:subPropertyOf rdf:resource="http://www.kanzaki.com/ns/exif#subSecTime"/>
  <rdfs:subPropertyOf rdf:resource="&nexif;dateAndOrTime"/>
  <rdfs:subPropertyOf rdf:resource="&nexif;subsecond"/>
  <rdfs:domain rdf:resource="&nexif;Photo"/>
  <rdfs:range rdf:resource="&xsd;string"/>
</rdf:Property>

<rdf:Property rdf:about="&ncal;repeat"
    rdfs:label="repeat">
  <nrl:maxCardinality rdf:datatype="&xsd;integer">1</nrl:maxCardinality>
  <rdfs:comment>This property defines the number of time the alarm should be repeated, after the initial trigger. Inspired by RFC 2445 sec. 4.8.6.2</rdfs:comment>
  <rdfs:domain rdf:resource="&ncal;Alarm"/>
  <rdfs:range rdf:resource="&xsd;integer"/>
</rdf:Property>

<tmo:Urgency rdf:about="&tmo;TMO_Instance_Urgency_08"
    rdfs:label="TMO_Instance_Urgency_08"/>

<rdfs:Class rdf:about="&ncal;Alarm"
    rdfs:label="Alarm">
  <rdfs:subClassOf rdf:resource="&nie;InformationElement"/>
  <rdfs:subClassOf rdf:resource="&ncal;UnionOfAlarmEventFreebusyJournalTodo"/>
  <rdfs:subClassOf rdf:resource="&ncal;UnionOfAlarmEventFreebusyTodo"/>
  <rdfs:subClassOf rdf:resource="&ncal;UnionOfAlarmEventJournalTodo"/>
  <rdfs:subClassOf rdf:resource="&ncal;UnionOfAlarmEventTodo"/>
  <rdfs:comment>Provide a grouping of component properties that define an alarm.</rdfs:comment>
</rdfs:Class>

<rdf:Property rdf:about="&ncal;commentAltRep"
    rdfs:label="commentAltRep">
  <rdfs:comment>Alternate representation of the comment. Introduced to cover 
the ALTREP parameter of the COMMENT property. See 
documentation of ncal:comment for details.</rdfs:comment>
  <rdfs:domain rdf:resource="&ncal;UnionOfTimezoneObservanceEventFreebusyJournalTimezoneTodo"/>
  <rdfs:range rdf:resource="&rdfs;Resource"/>
</rdf:Property>

<rdf:Property rdf:about="&ncal;rdate"
    rdfs:label="rdate">
  <rdfs:comment>This property defines the list of date/times for a recurrence set. Inspired by RFC 2445 sec. 4.8.5.3. Note that RFC allows both DATE, DATE-TIME and PERIOD values for this property. That's why the range has been set to NcalTimeEntity.</rdfs:comment>
  <rdfs:domain rdf:resource="&ncal;UnionOfTimezoneObservanceEventJournalTimezoneTodo"/>
  <rdfs:range rdf:resource="&ncal;NcalTimeEntity"/>
</rdf:Property>

<tmo:Delegability rdf:about="&tmo;TMO_Instance_Delegability_Unrestricted"
    rdfs:label="TMO_Instance_Delegability_Unrestricted"/>

<owl:Class rdf:about="&oa;TextPositionSelector">
  <rdfs:comment xml:lang="en">An oa:Selector which describes a range of text based on its start and end positions.

The text MUST be normalized before counting characters. For a Selector that works from the bitstream rather than the rendered characters, see oa:DataPositionSelector.

Each oa:TextPositionSelector MUST have exactly 1 oa:start property.

Each oa:TextPositionSelector MUST have exactly 1 oa:end property.</rdfs:comment>
  <rdfs:isDefinedBy rdf:resource="&oa;"/>
  <rdfs:label xml:lang="en">TextPositionSelector</rdfs:label>
  <rdfs:subClassOf rdf:resource="&oa;Selector"/>
</owl:Class>

<rdf:Property rdf:about="&nfo;isPasswordProtected"
    rdfs:comment="States if a given resource is password-protected."
    rdfs:label="isPasswordProtected">
  <nrl:maxCardinality rdf:datatype="&xsd;integer">1</nrl:maxCardinality>
  <rdfs:domain rdf:resource="&nfo;ArchiveItem"/>
  <rdfs:range rdf:resource="&xsd;boolean"/>
</rdf:Property>

<rdf:Property rdf:about="&ncal;fbtype"
    rdfs:label="fbtype">
  <nrl:maxCardinality rdf:datatype="&xsd;integer">1</nrl:maxCardinality>
  <rdfs:comment>To specify the free or busy time type. Inspired by RFC 2445 sec. 4.2.9. The RFC specified a limited vocabulary for the values of this property. The terms of this vocabulary have been expressed as instances of the FreebusyType class. The user can use instances provided with this ontology or create his own.</rdfs:comment>
  <rdfs:domain rdf:resource="&ncal;FreebusyPeriod"/>
  <rdfs:range rdf:resource="&ncal;FreebusyType"/>
</rdf:Property>

<rdf:Property rdf:about="&nexif;gpsImgDirection"
    rdfs:label="gpsImgDirection">
  <rdfs:subPropertyOf rdf:resource="http://www.kanzaki.com/ns/exif#gpsImgDirection"/>
  <rdfs:subPropertyOf rdf:resource="&nexif;gpsInfo"/>
  <rdfs:comment>tagNumber: 17
The direction of the image when it was captured. The range of values is from 0.00 to 359.99.</rdfs:comment>
  <rdfs:domain rdf:resource="&nexif;Photo"/>
  <rdfs:range rdf:resource="&xsd;string"/>
</rdf:Property>

<rdf:Property rdf:about="&ddo;macAddress"
    rdfs:comment="Defines the known mac address for a computer network."
    rdfs:label="macAddress">
  <rdfs:domain rdf:resource="&ddo;ComputerNetwork"/>
  <rdfs:range rdf:resource="&xsd;string"/>
</rdf:Property>

<rdf:Property rdf:about="&nexif;gpsSpeedRef"
    rdfs:label="gpsSpeedRef">
  <rdfs:subPropertyOf rdf:resource="http://www.kanzaki.com/ns/exif#gpsSpeedRef"/>
  <rdfs:subPropertyOf rdf:resource="&nexif;gpsInfo"/>
  <rdfs:comment>tagNumber: 12
The unit used to express the GPS receiver speed of movement. 'K' 'M' and 'N' represents kilometers per hour, miles per hour, and knots.</rdfs:comment>
  <rdfs:domain rdf:resource="&nexif;Photo"/>
  <rdfs:range rdf:resource="&xsd;string"/>
</rdf:Property>

<rdfs:Class rdf:about="&rdf;Bag">
  <rdfs:comment xml:lang="en">The class of unordered containers.</rdfs:comment>
  <rdfs:isDefinedBy rdf:resource="&rdf;"/>
  <rdfs:label xml:lang="en">Bag</rdfs:label>
  <rdfs:subClassOf rdf:resource="&rdfs;Container"/>
</rdfs:Class>

<rdfs:Class rdf:about="&tmo;SuperSubTaskDependency"
    rdfs:label="SuperSubTaskDependency">
  <rdfs:comment>By means of the SuperSubTaskDependency one can further describe the subtask-supertask relation .e.g by an descriptin. This enables an n-ary relation between subtask and supertask.</rdfs:comment>
  <rdfs:subClassOf rdf:resource="&tmo;TaskDependency"/>
</rdfs:Class>

<rdf:Property rdf:about="&cnt;declaredEncoding">
  <rdf:type rdf:resource="&owl;ObjectProperty"/>
  <rdfs:comment xml:lang="en">The character encoding declared in the XML declaration.</rdfs:comment>
  <rdfs:domain rdf:resource="&cnt;ContentAsXML"/>
  <rdfs:label xml:lang="en">XML character encoding</rdfs:label>
  <rdfs:range rdf:resource="&rdfs;Literal"/>
</rdf:Property>

<rdfs:Class rdf:about="&pimo;ProcessConcept"
    protege:role="abstract"
    rdfs:label="Process Concept">
  <pimo:classRole rdf:resource="&pimo;AbstractClass"/>
  <rdfs:comment>Concepts that relate to a series of actions or operations conducing to an end. Abstract class. Defines optional start and endtime properties, names taken from NCAL.</rdfs:comment>
  <rdfs:subClassOf rdf:resource="&pimo;Thing"/>
</rdfs:Class>

<tmo:Importance rdf:about="&tmo;TMO_Instance_Importance_10"
    rdfs:label="TMO_Instance_Importance_10"/>

<nrl:DefiningProperty rdf:about="&nmm;seasonOf"
    rdfs:comment="Relates a TV Season to its series"
    rdfs:label="has season">
  <nrl:cardinality rdf:datatype="&xsd;integer">1</nrl:cardinality>
  <nrl:inverseProperty rdf:resource="&nmm;hasSeason"/>
  <rdf:type rdf:resource="&rdf;Property"/>
  <rdfs:domain rdf:resource="&nmm;TVSeason"/>
  <rdfs:range rdf:resource="&nmm;TVSeries"/>
  <rdfs:subPropertyOf rdf:resource="&nie;isLogicalPartOf"/>
</nrl:DefiningProperty>

<rdf:Property rdf:about="&foaf;maker"
    rdfs:comment="An agent that  made this thing."
    rdfs:label="maker"
    ns:term_status="stable">
  <rdf:type rdf:resource="&owl;ObjectProperty"/>
  <rdfs:domain rdf:resource="&owl;Thing"/>
  <rdfs:isDefinedBy rdf:resource="&foaf;"/>
  <rdfs:range rdf:resource="&foaf;Agent"/>
  <owl:equivalentProperty rdf:resource="&dcterms;creator"/>
  <owl:inverseOf rdf:resource="&foaf;made"/>
</rdf:Property>

<rdf:Property rdf:about="&nuao;firstEvent"
    rdfs:comment="The start time of the first event"
    rdfs:label="first event">
  <nrl:maxCardinality rdf:datatype="&xsd;nonNegativeInteger">1</nrl:maxCardinality>
  <rdfs:domain rdf:resource="&rdfs;Resource"/>
  <rdfs:range rdf:resource="&xsd;dateTime"/>
</rdf:Property>

<rdf:Property rdf:about="&nfo;colorDepth"
    rdfs:comment="Amount of bits used to express the color of each pixel."
    rdfs:label="colorDepth">
  <nrl:maxCardinality rdf:datatype="&xsd;integer">1</nrl:maxCardinality>
  <rdfs:domain rdf:resource="&nfo;Visual"/>
  <rdfs:range rdf:resource="&xsd;integer"/>
  <rdfs:subPropertyOf rdf:resource="&nfo;bitDepth"/>
</rdf:Property>

<rdf:Property rdf:about="&dcterms;available">
  <rdfs:subPropertyOf rdf:resource="&dc;date"/>
  <rdfs:subPropertyOf rdf:resource="&dcterms;date"/>
  <dcterms:hasVersion rdf:resource="http://dublincore.org/usage/terms/history/#available-003"/>
  <dcterms:issued rdf:datatype="&xsd;date">2000-07-11</dcterms:issued>
  <dcterms:modified rdf:datatype="&xsd;date">2008-01-14</dcterms:modified>
  <rdfs:comment xml:lang="en">Date (often a range) that the resource became or will become available.</rdfs:comment>
  <rdfs:isDefinedBy rdf:resource="&dcterms;"/>
  <rdfs:label xml:lang="en">Date Available</rdfs:label>
  <rdfs:range rdf:resource="&rdfs;Literal"/>
</rdf:Property>

<rdfs:Class rdf:about="&nfo;Filesystem"
    rdfs:label="Filesystem">
  <rdfs:comment>A filesystem. Examples of filesystems include hard disk partitions, removable media, but also images thereof stored in files such as ISO.</rdfs:comment>
  <rdfs:subClassOf rdf:resource="&nfo;DataContainer"/>
</rdfs:Class>

<rdf:Property rdf:about="&nie;licenseType"
    rdfs:label="licenseType">
  <rdfs:comment>The type of the license. Possible values for this field may include "GPL", "BSD", "Creative Commons" etc.</rdfs:comment>
  <rdfs:range rdf:resource="&xsd;string"/>
  <rdfs:subPropertyOf rdf:resource="&nie;legal"/>
</rdf:Property>

<ncal:Weekday rdf:about="&ncal;tuesday"
    rdfs:label="tuesday"/>

<rdf:Property rdf:about="&scos;semanticRelation">
  <rdf:type rdf:resource="&owl;ObjectProperty"/>
  <rdfs:domain rdf:resource="&scos;Concept"/>
  <rdfs:isDefinedBy rdf:resource="http://www.w3.org/2004/02/skos/core"/>
  <rdfs:label xml:lang="en">is in semantic relation with</rdfs:label>
  <rdfs:range rdf:resource="&scos;Concept"/>
  <scos:definition xml:lang="en">Links a concept to a concept related by meaning.</scos:definition>
  <scos:scopeNote xml:lang="en">This property should not be used directly, but as a super-property for all properties denoting a relationship of meaning between concepts.</scos:scopeNote>
</rdf:Property>

<rdf:Property rdf:about="&dpo;minSpeed"
    rdfs:label="Minimum Speed">
  <rdfs:comment>A subproperty of dpo:minValue that defines an lowerbound on the observed speed value (in metres per second) such that it can classify as a dpo:Movement instance. It can be used in conjunction with dpo:maxSpeed, i.e. specific instances of dpo:Movement have a pre-defined range of observable real-world agent speed levels.</rdfs:comment>
  <rdfs:domain rdf:resource="&dpo;Movement"/>
  <rdfs:range rdf:resource="&xsd;float"/>
  <rdfs:subPropertyOf rdf:resource="&dpo;minValue"/>
</rdf:Property>

<rdf:Property rdf:about="&nexif;dateAndOrTime"
    rdfs:comment="An attribute relating to Date and/or Time"
    rdfs:label="dateAndOrTime">
  <rdfs:subPropertyOf rdf:resource="http://www.kanzaki.com/ns/exif#dateAndOrTime"/>
  <rdfs:subPropertyOf rdf:resource="&nexif;exifAttribute"/>
  <rdfs:domain rdf:resource="&nexif;Photo"/>
  <rdfs:range rdf:resource="&xsd;string"/>
</rdf:Property>

<rdf:Property rdf:about="&tmo;contextTask"
    nrl:maxCardinality="1"
    rdfs:label="contextTask">
  <nrl:inverseProperty rdf:resource="&tmo;contextThread"/>
  <rdfs:range rdf:resource="&tmo;Task"/>
</rdf:Property>

<rdf:Property rdf:about="&dpo;altLocation"
    rdfs:label="Alternative Location">
  <rdfs:comment>Links a generic place type to specific locations (pimo:Location instances) that are known to be of the same type, e.g., a dpo:Place representing 'restaurants' to actual location instances representing specific restaurants. This property is also used to link generic activities (dpo:Activity instances) to one or more specific locations at which they habitually take place, e.g., an activity representing 'sports' to location instances representing sports grounds, gymnasia, etc. Due to the multiple assocations of locations to places and activities, the domain for this property is bound to dpo:NonQuantifiableComponent instances. However, it is not intended to associate locations to other subclasses of that domain.</rdfs:comment>
  <rdfs:domain rdf:resource="&dpo;NonQuantifiableComponent"/>
  <rdfs:range rdf:resource="&pimo;Location"/>
</rdf:Property>

<rdf:Property rdf:about="&ncal;tzurl"
    rdfs:label="tzurl">
  <rdfs:comment>The TZURL provides a means for a VTIMEZONE component to point to a network location that can be used to retrieve an up-to- date version of itself. Inspired by RFC 2445 sec. 4.8.3.5. Originally the range of this property had been specified as URI.</rdfs:comment>
  <rdfs:domain rdf:resource="&ncal;Timezone"/>
  <rdfs:range rdf:resource="&rdfs;Resource"/>
</rdf:Property>

<rdf:Property rdf:about="&nfo;streamPosition"
    rdfs:label="streamPosition">
  <nrl:maxCardinality rdf:datatype="&xsd;integer">1</nrl:maxCardinality>
  <rdfs:comment>Stream position of the bookmark, suitable for e.g. audio books. Expressed in milliseconds</rdfs:comment>
  <rdfs:domain rdf:resource="&nfo;Bookmark"/>
  <rdfs:range rdf:resource="&xsd;integer"/>
</rdf:Property>

<rdf:Property rdf:about="&dc;format">
  <dcterms:description xml:lang="en">Examples of dimensions include size and duration. Recommended best practice is to use a controlled vocabulary such as the list of Internet Media Types [MIME].</dcterms:description>
  <dcterms:hasVersion rdf:resource="http://dublincore.org/usage/terms/history/#format-007"/>
  <dcterms:issued rdf:datatype="&xsd;date">1999-07-02</dcterms:issued>
  <dcterms:modified rdf:datatype="&xsd;date">2008-01-14</dcterms:modified>
  <rdfs:comment xml:lang="en">The file format, physical medium, or dimensions of the resource.</rdfs:comment>
  <rdfs:isDefinedBy rdf:resource="&dc;"/>
  <rdfs:label xml:lang="en">Format</rdfs:label>
  <scos:note xml:lang="en">A second property with the same name as this property has been declared in the dcterms: namespace (http://purl.org/dc/terms/).  See the Introduction to the document "DCMI Metadata Terms" (http://dublincore.org/documents/dcmi-terms/) for an explanation.</scos:note>
</rdf:Property>

<rdf:Property rdf:about="&ncal;byhour"
    rdfs:comment="Hour of recurrence. Defined in RFC 2445 sec. 4.3.10"
    rdfs:label="byhour">
  <rdfs:domain rdf:resource="&ncal;RecurrenceRule"/>
  <rdfs:range rdf:resource="&xsd;integer"/>
</rdf:Property>

<rdf:Property rdf:about="&ncal;periodEnd"
    rdfs:label="periodEnd">
  <nrl:maxCardinality rdf:datatype="&xsd;integer">1</nrl:maxCardinality>
  <rdfs:comment>End of a period of time. Inspired by the second part of a structured value of a PERIOD datatype specified in RFC 2445 sec. 4.3.9. Note that a single NcalPeriod instance shouldn't have the periodEnd and periodDuration properties specified simultaneously.</rdfs:comment>
  <rdfs:domain rdf:resource="&ncal;NcalPeriod"/>
  <rdfs:range rdf:resource="&xsd;dateTime"/>
</rdf:Property>

<rdf:Property rdf:about="&nao;externalIdentifier"
    rdfs:label="external identifier">
  <rdfs:comment>An external identifier for a resource that has been retreived from an external source.</rdfs:comment>
  <rdfs:domain rdf:resource="&rdfs;Resource"/>
  <rdfs:range rdf:resource="&rdfs;Literal"/>
  <rdfs:subPropertyOf rdf:resource="&nao;identifier"/>
</rdf:Property>

<rdf:Property rdf:about="&nid3;backgroundArtist"
    rdfs:label="backgroundArtist">
  <rdfs:comment>TPE2
The 'Band/Orchestra/Accompaniment' frame is used for additional information about the performers in the recording.</rdfs:comment>
  <rdfs:domain rdf:resource="&nid3;ID3Audio"/>
  <rdfs:range rdf:resource="&nco;Contact"/>
  <rdfs:subPropertyOf rdf:resource="&nco;contributor"/>
</rdf:Property>

<rdf:Property rdf:about="&nfo;sampleRate"
    rdfs:comment="The amount of audio samples per second."
    rdfs:label="sampleRate">
  <nrl:maxCardinality rdf:datatype="&xsd;integer">1</nrl:maxCardinality>
  <rdfs:domain rdf:resource="&nfo;Audio"/>
  <rdfs:range rdf:resource="&xsd;float"/>
  <rdfs:subPropertyOf rdf:resource="&nfo;rate"/>
</rdf:Property>

<rdfs:Class rdf:about="&pimo;Collection"
    rdfs:label="Collection">
  <rdfs:comment>A collection of Things, independent of their class. The items in the collection share a common property. Which property may be modelled explicitly or mentioned in the description of the Collection. The requirement of explicit modelling the semantic meaning of the collection is not mandatory, as collections can be created ad-hoc. Implizit modelling can be applied by the system by learning the properties. For example, a Collection of "Coworkers" could be defined as that all elements must be of class "Person" and have an attribute "work for the same Organization as the user". Further standards can be used to model these attributes.</rdfs:comment>
  <rdfs:subClassOf rdf:resource="&pimo;Thing"/>
</rdfs:Class>

<rdfs:Class rdf:about="&ndo;P2PFile"
    rdfs:comment="A file available via a peer-to-peer network"
    rdfs:label="P2P file">
  <rdfs:subClassOf rdf:resource="&nfo;RemoteDataObject"/>
</rdfs:Class>

<rdf:Property rdf:about="&nie;plainTextContent"
    nrl:maxCardinality="1"
    rdfs:label="plainTextContent">
  <rdfs:comment>Plain-text representation of the content of a InformationElement with all markup removed. The main purpose of this property is full-text indexing and search. Its exact content is considered application-specific. The user can make no assumptions about what is and what is not contained within. Applications should use more specific properties wherever possible.</rdfs:comment>
  <rdfs:domain rdf:resource="&nie;InformationElement"/>
  <rdfs:range rdf:resource="&xsd;string"/>
</rdf:Property>

<rdf:Property rdf:about="&foaf;plan"
    rdfs:label="plan"
    ns:term_status="testing">
  <rdf:type rdf:resource="&owl;DatatypeProperty"/>
  <rdfs:comment>A .plan comment, in the tradition of finger and '.plan' files.</rdfs:comment>
  <rdfs:domain rdf:resource="&foaf;Person"/>
  <rdfs:isDefinedBy rdf:resource="&foaf;"/>
  <rdfs:range rdf:resource="&rdfs;Literal"/>
</rdf:Property>

<rdfs:Class rdf:about="&pimo;Note"
    rdfs:label="Note">
  <rdfs:comment>A note. The textual contents of the note should be expressed in the nao:description value of the note.</rdfs:comment>
  <rdfs:subClassOf rdf:resource="&pimo;Document"/>
</rdfs:Class>

<rdf:Property rdf:about="&nao;annotation"
    rdfs:comment="Generic annotation for a resource"
    rdfs:label="annotation">
  <rdfs:domain rdf:resource="&rdfs;Resource"/>
</rdf:Property>

<rdfs:Class rdf:about="&pimo;Organization"
    rdfs:label="Organization">
  <rdfs:subClassOf rdf:resource="&pimo;Agent"/>
  <rdfs:subClassOf rdf:resource="&pimo;Locatable"/>
  <rdfs:comment>An administrative and functional structure (as a business or a political party). (Definition from Merriam-Webster)</rdfs:comment>
</rdfs:Class>

<rdf:Property rdf:about="&nexif;dateTime"
    rdfs:label="dateTime">
  <rdfs:subPropertyOf rdf:resource="http://www.kanzaki.com/ns/exif#dateTime"/>
  <rdfs:subPropertyOf rdf:resource="&nie;lastModified"/>
  <rdfs:subPropertyOf rdf:resource="&nexif;date"/>
  <rdfs:subPropertyOf rdf:resource="&nexif;exifAttribute"/>
  <rdfs:comment>The date and time of image creation. In this standard it is the date and time the file was changed.
tagNumber: 306</rdfs:comment>
  <rdfs:domain rdf:resource="&nexif;Photo"/>
  <rdfs:range rdf:resource="&xsd;dateTime"/>
</rdf:Property>

<rdf:Property rdf:about="&nexif;gpsDestLongitudeRef"
    rdfs:comment="Reference for longitude of destination
tagNumber: 21"
    rdfs:label="gpsDestLongitudeRef">
  <rdfs:subPropertyOf rdf:resource="http://www.kanzaki.com/ns/exif#gpsDestLongitudeRef"/>
  <rdfs:subPropertyOf rdf:resource="&nexif;gpsInfo"/>
  <rdfs:domain rdf:resource="&nexif;Photo"/>
  <rdfs:range rdf:resource="&xsd;string"/>
</rdf:Property>

<rdf:Property rdf:about="&nid3;playlistDelay"
    rdfs:label="playlistDelay">
  <rdfs:comment>TDLY
The 'Playlist delay' defines the numbers of milliseconds of silence between every song in a playlist. The player should use the "ETC" frame, if present, to skip initial silence and silence at the end of the audio to match the 'Playlist delay' time. The time is represented as a numeric string.</rdfs:comment>
  <rdfs:domain rdf:resource="&nid3;ID3Audio"/>
  <rdfs:range rdf:resource="&xsd;integer"/>
</rdf:Property>

<rdfs:Class rdf:about="&nfo;VectorImage"
    rdfs:label="VectorImage">
  <rdfs:subClassOf rdf:resource="&nfo;Image"/>
</rdfs:Class>

<rdf:Property rdf:about="&nrl;viewOn"
    rdfs:comment="Points to a graph view over the subject named graph"
    rdfs:label="viewOn">
  <rdfs:domain rdf:resource="&nrl;GraphView"/>
  <rdfs:range rdf:resource="&nrl;Graph"/>
</rdf:Property>

<rdfs:Class rdf:about="&tmo;TransmissionState"
    rdfs:label="TransmissionState">
  <rdfs:comment>States a task can go through during transmission of an task.</rdfs:comment>
  <rdfs:subClassOf rdf:resource="&tmo;StateTypeRole"/>
</rdfs:Class>

<rdf:Property rdf:about="&foaf;logo"
    rdfs:comment="A logo representing some thing."
    rdfs:label="logo"
    ns:term_status="testing">
  <rdf:type rdf:resource="&owl;InverseFunctionalProperty"/>
  <rdf:type rdf:resource="&owl;ObjectProperty"/>
  <rdfs:domain rdf:resource="&owl;Thing"/>
  <rdfs:isDefinedBy rdf:resource="&foaf;"/>
  <rdfs:range rdf:resource="&owl;Thing"/>
</rdf:Property>

<rdfs:Class rdf:about="&dctypes;Text">
  <dcam:memberOf rdf:resource="&dcterms;DCMIType"/>
  <dcterms:description xml:lang="en">Examples include books, letters, dissertations, poems, newspapers, articles, archives of mailing lists. Note that facsimiles or images of texts are still of the genre Text.</dcterms:description>
  <dcterms:hasVersion rdf:resource="http://dublincore.org/usage/terms/history/#Text-003"/>
  <dcterms:issued rdf:datatype="&xsd;date">2000-07-11</dcterms:issued>
  <dcterms:modified rdf:datatype="&xsd;date">2008-01-14</dcterms:modified>
  <rdfs:comment xml:lang="en">A resource consisting primarily of words for reading.</rdfs:comment>
  <rdfs:isDefinedBy rdf:resource="&dctypes;"/>
  <rdfs:label xml:lang="en">Text</rdfs:label>
</rdfs:Class>

<rdf:Property rdf:about="&dcon;recordedBy"
    rdfs:label="Recorded By">
  <rdfs:comment>This property ties each element's observation to the data source that recorded it, specifically data sources of type account (dao:Account subclass) or device (ddo:Device subclass).</rdfs:comment>
  <rdfs:domain rdf:resource="&dcon;Observation"/>
  <rdfs:range rdf:resource="&nie;DataSource"/>
  <rdfs:subPropertyOf rdf:resource="&dcon;hasContextAttribute"/>
</rdf:Property>

<rdfs:Class rdf:about="&ndo;DownloadEvent"
    rdfs:label="download event">
  <rdfs:comment>A single event (from the point of view of the user) of downloading of a file or a set of files. Use nuao:involves to indicate the files involved. The event is assigned to downloaded copies of files. Can be assigned to multiple files.</rdfs:comment>
  <rdfs:subClassOf rdf:resource="&nuao;DesktopEvent"/>
</rdfs:Class>

<rdf:Property rdf:about="&tmo;dependencyOrderNumber"
    nrl:maxCardinality="1"
    nrl:minCardinality="1"
    rdfs:label="dependencyOrderNumber">
  <rdfs:domain rdf:resource="&tmo;TaskDependency"/>
  <rdfs:range rdf:resource="&xsd;int"/>
</rdf:Property>

<rdf:Property rdf:about="&nie;htmlContent"
    nrl:maxCardinality="1"
    rdfs:label="html content">
  <rdfs:comment>The HTML content of an information element. This property can be used to store text including formatting in a generic fashion.</rdfs:comment>
  <rdfs:domain rdf:resource="&nie;InformationElement"/>
  <rdfs:range rdf:resource="&xsd;string"/>
</rdf:Property>

<rdf:Property rdf:about="&pimo;roleHolder"
    rdfs:comment="the person taking the role"
    rdfs:label="role holder">
  <rdfs:domain rdf:resource="&pimo;PersonRole"/>
  <rdfs:range rdf:resource="&pimo;Person"/>
  <rdfs:subPropertyOf rdf:resource="&pimo;associationMember"/>
</rdf:Property>

<rdfs:Class rdf:about="&tmo;AbilityCarrierInvolvement"
    rdfs:label="AbilityCarrierInvolvement">
  <rdfs:subClassOf rdf:resource="&pimo;Association"/>
  <rdfs:subClassOf rdf:resource="&rdfs;Resource"/>
  <rdfs:comment>The class AbilityCarrier_Involvement ties together an AbilityCarrier with an AbilityCarrier_Role. This is a role based modelling approach. An n-ary relation is realized.</rdfs:comment>
</rdfs:Class>

<rdf:Property rdf:about="&dc;contributor">
  <dcterms:description xml:lang="en">Examples of a Contributor include a person, an organization, or a service. Typically, the name of a Contributor should be used to indicate the entity.</dcterms:description>
  <dcterms:hasVersion rdf:resource="http://dublincore.org/usage/terms/history/#contributor-006"/>
  <dcterms:issued rdf:datatype="&xsd;date">1999-07-02</dcterms:issued>
  <dcterms:modified rdf:datatype="&xsd;date">2008-01-14</dcterms:modified>
  <rdfs:comment xml:lang="en">An entity responsible for making contributions to the resource.</rdfs:comment>
  <rdfs:isDefinedBy rdf:resource="&dc;"/>
  <rdfs:label xml:lang="en">Contributor</rdfs:label>
  <scos:note xml:lang="en">A second property with the same name as this property has been declared in the dcterms: namespace (http://purl.org/dc/terms/).  See the Introduction to the document "DCMI Metadata Terms" (http://dublincore.org/documents/dcmi-terms/) for an explanation.</scos:note>
</rdf:Property>

<rdfs:Class rdf:about="&pimo;Contract"
    rdfs:label="Contract">
  <rdfs:comment>A binding agreement between two or more persons that is enforceable by law. (Definition from SUMO). This is an example class for a document type, there are more detailled ontologies to model Contracts.</rdfs:comment>
  <rdfs:subClassOf rdf:resource="&pimo;Document"/>
</rdfs:Class>

<rdf:Property rdf:about="&ncal;triggerDuration"
    rdfs:label="triggerDuration">
  <nrl:maxCardinality rdf:datatype="&xsd;integer">1</nrl:maxCardinality>
  <rdfs:comment>The duration of a trigger. This property has been created to express the VALUE=DURATION parameter of the TRIGGER property. See documentation for ncal:trigger for more details.</rdfs:comment>
  <rdfs:domain rdf:resource="&ncal;Trigger"/>
  <rdfs:range rdf:resource="&xsd;duration"/>
</rdf:Property>

<rdf:Property rdf:about="&dcon;uvindex"
    rdfs:label="UV Index Value">
  <rdfs:comment>Registers an actual UV index value element attribute to an active weather condition in the current context.</rdfs:comment>
  <rdfs:domain rdf:resource="&dpo;WeatherConditions"/>
  <rdfs:range rdf:resource="&xsd;nonNegativeInteger"/>
  <rdfs:subPropertyOf rdf:resource="&dcon;hasContextAttribute"/>
</rdf:Property>

<rdf:Property rdf:about="&dcterms;rights">
  <dcterms:description xml:lang="en">Typically, rights information includes a statement about various property rights associated with the resource, including intellectual property rights.</dcterms:description>
  <dcterms:hasVersion rdf:resource="http://dublincore.org/usage/terms/history/#rightsT-001"/>
  <dcterms:issued rdf:datatype="&xsd;date">2008-01-14</dcterms:issued>
  <dcterms:modified rdf:datatype="&xsd;date">2008-01-14</dcterms:modified>
  <rdfs:comment xml:lang="en">Information about rights held in and over the resource.</rdfs:comment>
  <rdfs:isDefinedBy rdf:resource="&dcterms;"/>
  <rdfs:label xml:lang="en">Rights</rdfs:label>
  <rdfs:range rdf:resource="&dcterms;RightsStatement"/>
  <rdfs:subPropertyOf rdf:resource="&dc;rights"/>
</rdf:Property>

<rdf:Property rdf:about="&nexif;gpsDOP"
    rdfs:label="gpsDOP">
  <rdfs:subPropertyOf rdf:resource="http://www.kanzaki.com/ns/exif#gpsDOP"/>
  <rdfs:subPropertyOf rdf:resource="&nexif;gpsInfo"/>
  <rdfs:comment>The GPS DOP (data degree of precision). An HDOP value is written during two-dimensional measurement, and PDOP during three-dimensional measurement.
tagNumber: 11</rdfs:comment>
  <rdfs:domain rdf:resource="&nexif;Photo"/>
  <rdfs:range rdf:resource="&xsd;string"/>
</rdf:Property>

<rdf:Property rdf:about="&nao;score"
    rdfs:comment="An authoritative score for an item valued between 0 and 1"
    rdfs:label="score">
  <nrl:maxCardinality rdf:datatype="&xsd;nonNegativeInteger">1</nrl:maxCardinality>
  <rdfs:domain rdf:resource="&rdfs;Resource"/>
  <rdfs:range rdf:resource="&xsd;float"/>
  <rdfs:subPropertyOf rdf:resource="&nao;annotation"/>
</rdf:Property>

<rdf:Property rdf:about="&tmo;dependencyDescription"
    nrl:maxCardinality="1"
    rdfs:comment="Endusers can clarify why they created a depedency."
    rdfs:label="dependencyDescription">
  <rdfs:domain rdf:resource="&tmo;TaskDependency"/>
  <rdfs:subPropertyOf rdf:resource="&nao;description"/>
</rdf:Property>

<owl:AnnotationProperty rdf:about="&ns;term_status"/>

<rdf:Property rdf:about="&dpo;maxCloudcover"
    rdfs:label="Maximum Cloud Cover">
  <rdfs:comment>A subproperty of dpo:maxValue that defines an upperbound on the observed cloud cover (as a percentage) such that it can classify as a dpo:WeatherCondition instance. It can be used in conjunction with dpo:minCloudCover to state that specific instances of dpo:WeatherCondition have a pre-defined range of observable real-world cloud cover levels. In addition, they can also be used with various other weather conditions values and ranges to define complex weather condition types.</rdfs:comment>
  <rdfs:domain rdf:resource="&dpo;WeatherConditions"/>
  <rdfs:range rdf:resource="&xsd;nonNegativeInteger"/>
  <rdfs:subPropertyOf rdf:resource="&dpo;maxValue"/>
</rdf:Property>

<rdfs:Class rdf:about="&dplo;ImagePost"
    rdfs:label="Image Post">
  <rdfs:comment>Represents the live posting of an image file, or a link to an online image, as defined by instances of nfo:Image.</rdfs:comment>
  <rdfs:subClassOf rdf:resource="&dplo;MultimediaPost"/>
</rdfs:Class>

<rdfs:Class rdf:about="&tmo;Role"
    rdfs:comment="examples: Architect, Developer, ..."
    rdfs:label="Role">
  <rdfs:subClassOf rdf:resource="&tmo;AbilityCarrier"/>
</rdfs:Class>

<owl:Class rdf:about="&oa;TextQuoteSelector">
  <rdfs:comment xml:lang="en">A Selector that describes a textual segment by means of quoting it, plus passages before or after it.

For example, if the document were "abcdefghijklmnopqrstuvwxyz", one could select "efg" by a oa:prefix of "abcd", the quotation of oa:exact "efg" and a oa:suffix of "hijk".

The text MUST be normalized before recording.

Each TextQuoteSelector MUST have exactly 1 oa:exact property.

Each TextQuoteSelector SHOULD have exactly 1 oa:prefix property, and MUST NOT have more than 1.

Each TextQuoteSelector SHOULD have exactly 1 oa:suffix property, and MUST NOT have more than 1.</rdfs:comment>
  <rdfs:isDefinedBy rdf:resource="&oa;"/>
  <rdfs:label xml:lang="en">TextQuoteSelector</rdfs:label>
  <rdfs:subClassOf rdf:resource="&oa;Selector"/>
</owl:Class>

<rdfs:Class rdf:about="&ncal;UnionOfEventJournalTimezoneTodo"
    rdfs:label="UnionOfEventJournalTimezoneTodo">
  <rdfs:subClassOf rdf:resource="&ncal;UnionParentClass"/>
</rdfs:Class>

<rdf:Property rdf:about="&ncal;involvedContact"
    rdfs:label="involvedContact">
  <rdfs:comment>A contact of the Attendee or the organizer involved in an event or other calendar entity. This property has been introduced to express the actual value of the ATTENDEE and ORGANIZER properties. The contact will also represent the CN parameter of those properties. See documentation of ncal:attendee or ncal:organizer for more details.</rdfs:comment>
  <rdfs:domain rdf:resource="&ncal;AttendeeOrOrganizer"/>
  <rdfs:range rdf:resource="&nco;Contact"/>
</rdf:Property>

<rdf:Property rdf:about="&nfo;fileLastModified"
    rdfs:comment="last modification date"
    rdfs:label="fileLastModified">
  <nao:deprecated rdf:datatype="&xsd;boolean">true</nao:deprecated>
  <rdfs:domain rdf:resource="&nfo;FileDataObject"/>
  <rdfs:range rdf:resource="&xsd;dateTime"/>
  <rdfs:subPropertyOf rdf:resource="&nie;lastModified"/>
</rdf:Property>

<rdf:Property rdf:about="&nmo;replyTo"
    rdfs:comment="deprecated in favor of nmo:messageReplyTo"
    rdfs:label="replyTo">
  <nao:deprecated rdf:datatype="&xsd;boolean">true</nao:deprecated>
  <rdfs:domain rdf:resource="&nmo;Message"/>
  <rdfs:range rdf:resource="&nco;Contact"/>
</rdf:Property>

<rdfs:Class rdf:about="&dcterms;BibliographicResource">
  <dcterms:hasVersion rdf:resource="http://dublincore.org/usage/terms/history/#BibliographicResource-001"/>
  <dcterms:issued rdf:datatype="&xsd;date">2008-01-14</dcterms:issued>
  <rdfs:comment xml:lang="en">A book, article, or other documentary resource.</rdfs:comment>
  <rdfs:isDefinedBy rdf:resource="&dcterms;"/>
  <rdfs:label xml:lang="en">Bibliographic Resource</rdfs:label>
</rdfs:Class>

<rdf:Property rdf:about="&dc;title">
  <dcterms:hasVersion rdf:resource="http://dublincore.org/usage/terms/history/#title-006"/>
  <dcterms:issued rdf:datatype="&xsd;date">1999-07-02</dcterms:issued>
  <dcterms:modified rdf:datatype="&xsd;date">2008-01-14</dcterms:modified>
  <rdf:type rdf:resource="&owl;AnnotationProperty"/>
  <rdfs:comment xml:lang="en">A name given to the resource.</rdfs:comment>
  <rdfs:isDefinedBy rdf:resource="&dc;"/>
  <rdfs:label xml:lang="en">Title</rdfs:label>
  <scos:note xml:lang="en">A second property with the same name as this property has been declared in the dcterms: namespace (http://purl.org/dc/terms/).  See the Introduction to the document "DCMI Metadata Terms" (http://dublincore.org/documents/dcmi-terms/) for an explanation.</scos:note>
</rdf:Property>

<rdfs:Class rdf:about="&pimo;PersonRole"
    rdfs:label="Role of Person">
  <rdfs:comment>A person takes a certain role in a given context. The role can be that of "a mentor or another person" or "giving a talk at a meeting", etc.</rdfs:comment>
  <rdfs:subClassOf rdf:resource="&pimo;Association"/>
</rdfs:Class>

<rdf:Property rdf:about="&dcterms;creator">
  <rdfs:subPropertyOf rdf:resource="&dc;creator"/>
  <rdfs:subPropertyOf rdf:resource="&dcterms;contributor"/>
  <dcterms:description xml:lang="en">Examples of a Creator include a person, an organization, or a service.</dcterms:description>
  <dcterms:hasVersion rdf:resource="http://dublincore.org/usage/terms/history/#creatorT-002"/>
  <dcterms:issued rdf:datatype="&xsd;date">2008-01-14</dcterms:issued>
  <dcterms:modified rdf:datatype="&xsd;date">2010-10-11</dcterms:modified>
  <rdfs:comment xml:lang="en">An entity primarily responsible for making the resource.</rdfs:comment>
  <rdfs:isDefinedBy rdf:resource="&dcterms;"/>
  <rdfs:label xml:lang="en">Creator</rdfs:label>
  <rdfs:range rdf:resource="&dcterms;Agent"/>
  <owl:equivalentProperty rdf:resource="&foaf;maker"/>
</rdf:Property>

<rdf:Property rdf:about="&nfo;rearChannels"
    rdfs:comment="Number of rear channels."
    rdfs:label="rearChannels">
  <nrl:maxCardinality rdf:datatype="&xsd;integer">1</nrl:maxCardinality>
  <rdfs:range rdf:resource="&xsd;integer"/>
  <rdfs:subPropertyOf rdf:resource="&nfo;channels"/>
</rdf:Property>

<ncal:ParticipationStatus rdf:about="&ncal;completedParticipationStatus"
    rdfs:label="completedParticipationStatus"/>

<rdf:Property rdf:about="&nmm;trackGain"
    rdfs:comment="ReplayGain track gain"
    rdfs:label="track gain">
  <nrl:maxCardinality rdf:datatype="&xsd;integer">1</nrl:maxCardinality>
  <rdfs:domain rdf:resource="&nmm;MusicPiece"/>
  <rdfs:range rdf:resource="&xsd;float"/>
</rdf:Property>

<rdf:Property rdf:about="&ncal;date"
    rdfs:label="date">
  <nrl:maxCardinality rdf:datatype="&xsd;integer">1</nrl:maxCardinality>
  <rdfs:comment>Date an instance of NcalDateTime refers to. It was conceived to express values in DATE datatype specified in RFC 2445 4.3.4</rdfs:comment>
  <rdfs:domain rdf:resource="&ncal;NcalDateTime"/>
  <rdfs:range rdf:resource="&xsd;date"/>
</rdf:Property>

<rdf:Property rdf:about="&nexif;rowsPerStrip"
    rdfs:label="rowsPerStrip">
  <rdfs:subPropertyOf rdf:resource="http://www.kanzaki.com/ns/exif#rowsPerStrip"/>
  <rdfs:subPropertyOf rdf:resource="&nexif;recOffset"/>
  <rdfs:comment>tagNumber: 278
The number of rows per strip. This is the number of rows in the image of one strip when an image is divided into strips. With JPEG compressed data this designation is not needed and is omitted.</rdfs:comment>
  <rdfs:domain rdf:resource="&nexif;Photo"/>
  <rdfs:range rdf:resource="&xsd;integer"/>
</rdf:Property>

<rdf:Property rdf:about="&nexif;datatype"
    rdfs:comment="The Exif field data type, such as ascii, byte, short etc."
    rdfs:label="datatype">
  <rdfs:subPropertyOf rdf:resource="&dc;type"/>
  <rdfs:subPropertyOf rdf:resource="http://www.kanzaki.com/ns/exif#datatype"/>
  <rdfs:domain rdf:resource="&nexif;Photo"/>
  <rdfs:range rdf:resource="&xsd;string"/>
</rdf:Property>

<rdf:Property rdf:about="&nexif;imageLength"
    rdfs:label="imageLength">
  <rdfs:subPropertyOf rdf:resource="http://www.kanzaki.com/ns/exif#imageLength"/>
  <rdfs:subPropertyOf rdf:resource="&nfo;height"/>
  <rdfs:subPropertyOf rdf:resource="&nexif;height"/>
  <rdfs:subPropertyOf rdf:resource="&nexif;imageDataStruct"/>
  <rdfs:comment>tagNumber: 257
Image height. The number of rows of image data. In JPEG compressed data a JPEG marker is used.</rdfs:comment>
  <rdfs:domain rdf:resource="&nexif;Photo"/>
  <rdfs:range rdf:resource="&xsd;integer"/>
</rdf:Property>

<rdfs:Class rdf:about="&dpo;Mood"
    rdfs:label="Mood">
  <rdfs:comment>Non-quantifiable presence information concerning the current broadcast virtual mood of the agent.</rdfs:comment>
  <rdfs:subClassOf rdf:resource="&dpo;NonQuantifiableComponent"/>
</rdfs:Class>

<rdfs:Class rdf:about="&dcon;SpaTem"
    rdfs:label="SpaTem">
  <rdfs:comment>The spatio-temporal aspect covers context elements relating to the current user's physical locations, movement and time.</rdfs:comment>
  <rdfs:subClassOf rdf:resource="&dcon;Aspect"/>
</rdfs:Class>

<rdf:Property rdf:about="&dcon;hasObservation"
    rdfs:label="has Observation">
  <rdfs:comment>As context Elements can have one or more observations, this property links each of them to the respective element.</rdfs:comment>
  <rdfs:domain rdf:resource="&dcon;Element"/>
  <rdfs:range rdf:resource="&dcon;Observation"/>
</rdf:Property>

<rdf:Property rdf:about="&nid3;officialArtistWebpage"
    rdfs:label="officialArtistWebpage">
  <rdfs:domain rdf:resource="&nid3;ID3Audio"/>
  <rdfs:range rdf:resource="&rdfs;Resource"/>
</rdf:Property>

<rdf:Property rdf:about="&dpo;maxDayOfWeek"
    rdfs:label="Maximum Day of the Week">
  <rdfs:comment>A subproperty of dpo:maxValue that defines an upperbound on the observed day of the week (i.e., between 1 signifying Monday and 7 signifying Sunday) such that it can classify as a dpo:TimePeriod instance. It can be used in conjunction with dpo:minDayOfWeek, i.e. specific instances of dpo:TimePeriod have a pre-defined observable 7-day week-based period.</rdfs:comment>
  <rdfs:domain rdf:resource="&dpo;TimePeriod"/>
  <rdfs:range rdf:resource="&xsd;integer"/>
  <rdfs:subPropertyOf rdf:resource="&dpo;maxValue"/>
</rdf:Property>

<rdfs:Class rdf:about="&ddo;3G"
    rdfs:label="3G">
  <rdfs:comment>3rd generation mobile telecommunications (3G) is a third generation of standards for digital cellular networks.</rdfs:comment>
  <rdfs:subClassOf rdf:resource="&ddo;CellularNetwork"/>
</rdfs:Class>

<rdf:Property rdf:about="&drmo;hasConstraintOnSubject"
    rdfs:label="Constraint on Subject">
  <rdfs:comment> Places a constraint on a condition (i.e., the domain defined for this property), such that a query can be constructed to look for an RDF triple having: i) the referred item (i.e., range defined for this property) as its subject, ii) the associated constrained property (defined by drmo:hasConstraintOnProperty) as its property, iii) and the condition (i.e., domain defined for this property) as its object. This property cannot coincide with the property hasConstraintOnObject.</rdfs:comment>
  <rdfs:domain rdf:resource="&drmo;Condition"/>
  <rdfs:range rdf:resource="&rdfs;Resource"/>
</rdf:Property>

<rdfs:Class rdf:about="&nid3;ID3Audio"
    rdfs:label="ID3Audio">
  <rdfs:comment>A File annotated with ID3 tags. Implementation notes: use nie:title for the actual name of the piece (TIT2, the 'Title/Songname/Content description' frame); use nie:language for the languages of the text or lyrics spoken or sung in the audio (TLAN, the 'Language(s)' frame); use nie:comment for any kind of full text information that does not fit in any other frame (COMM frame).</rdfs:comment>
  <rdfs:subClassOf rdf:resource="&nfo;Audio"/>
</rdfs:Class>

<rdfs:Class rdf:about="&nfo;Website"
    rdfs:label="Website">
  <rdfs:comment>A website, usually a container for remote resources, that may be interpreted as HTMLDocuments, images or other types of content.</rdfs:comment>
  <rdfs:subClassOf rdf:resource="&nie;InformationElement"/>
</rdfs:Class>

<owl:DatatypeProperty rdf:about="&oa;start">
  <rdfs:comment xml:lang="en">The starting position of the segment of text or bytes. The first character/byte in the full text/stream is position 0. The character/byte indicated at position oa:start is included within the selected segment. 

See oa:DataPositionSelector and oa:TextPositionSelector.</rdfs:comment>
  <rdfs:domain rdf:resource="&oa;Selector"/>
  <rdfs:isDefinedBy rdf:resource="&oa;"/>
  <rdfs:label xml:lang="en">start</rdfs:label>
  <rdfs:range rdf:resource="&xsd;nonNegativeInteger"/>
</owl:DatatypeProperty>

<nco:IMCapability rdf:about="&nco;imCapabilityVideo"/>

<rdfs:Class rdf:about="&nco;PagerNumber"
    rdfs:label="PagerNumber">
  <rdfs:comment>A pager phone number. Inspired by the (TYPE=pager) parameter of the TEL property as defined in RFC 2426 sec  3.3.1.</rdfs:comment>
  <rdfs:subClassOf rdf:resource="&nco;MessagingNumber"/>
</rdfs:Class>

<rdf:Property rdf:about="&foaf;mbox_sha1sum"
    rdfs:label="sha1sum of a personal mailbox URI name"
    ns:term_status="testing">
  <rdf:type rdf:resource="&owl;DatatypeProperty"/>
  <rdf:type rdf:resource="&owl;InverseFunctionalProperty"/>
  <rdfs:comment>The sha1sum of the URI of an Internet mailbox associated with exactly one owner, the  first owner of the mailbox.</rdfs:comment>
  <rdfs:domain rdf:resource="&foaf;Agent"/>
  <rdfs:isDefinedBy rdf:resource="&foaf;"/>
  <rdfs:range rdf:resource="&rdfs;Literal"/>
</rdf:Property>

<rdf:Property rdf:about="&tmo;transmissionTask"
    nrl:maxCardinality="1"
    nrl:minCardinality="1"
    rdfs:label="transmissionTask">
  <nrl:inverseProperty rdf:resource="&tmo;taskTransmission"/>
  <rdfs:domain rdf:resource="&tmo;TaskTransmission"/>
  <rdfs:range rdf:resource="&tmo;Task"/>
  <rdfs:subPropertyOf rdf:resource="&tmo;taskReference"/>
</rdf:Property>

<owl:Class rdf:about="&oa;Tag">
  <rdfs:comment xml:lang="en">A class assigned to the Body when it is a tag, such as a embedded text string with cnt:chars.

Tags are typically keywords or labels, and used for organization, description or discovery of the resource being tagged. In the Semantic Web, URIs are used instead of strings to avoid the issue of polysemy where one word has multiple meanings, such usage MUST be indicated using the subclass oa:SemanticTag.

Annotations that tag resources, either with text or semantic tags, SHOULD also have the oa:tagging motivation to make the reason for the Annotation more clear to applications, and MAY have other motivations as well.</rdfs:comment>
  <rdfs:isDefinedBy rdf:resource="&oa;"/>
  <rdfs:label xml:lang="en">Tag</rdfs:label>
</owl:Class>

<rdf:Property rdf:about="&nco;note"
    rdfs:label="note">
  <rdfs:comment>A note about the object represented by this Contact. An equivalent for the 'NOTE' property defined in RFC 2426 Sec. 3.6.2</rdfs:comment>
  <rdfs:domain rdf:resource="&nco;Contact"/>
  <rdfs:range rdf:resource="&xsd;string"/>
  <rdfs:subPropertyOf rdf:resource="&nie;description"/>
</rdf:Property>

<rdf:Property rdf:about="&nco;belongsToGroup"
    rdfs:comment="Links a Contact with a ContactGroup it belongs to."
    rdfs:label="addressLocation">
  <rdfs:domain rdf:resource="&nco;Contact"/>
  <rdfs:range rdf:resource="&nco;ContactGroup"/>
</rdf:Property>

<rdf:Property rdf:about="&tmo;taskName"
    nrl:maxCardinality="1"
    rdfs:label="taskName">
  <rdfs:comment>The Task Name helps the user to identify a task in a list. It should be expressive enough to give a meaningful recognition. Details should be written in the description attribute instead. A name attribute is not allowed to contain line breaks.</rdfs:comment>
  <rdfs:domain rdf:resource="&tmo;Task"/>
  <rdfs:range rdf:resource="&rdfs;Literal"/>
  <rdfs:subPropertyOf rdf:resource="&nao;prefLabel"/>
</rdf:Property>

<rdf:Property rdf:about="&dc;identifier">
  <dcterms:description xml:lang="en">Recommended best practice is to identify the resource by means of a string conforming to a formal identification system. </dcterms:description>
  <dcterms:hasVersion rdf:resource="http://dublincore.org/usage/terms/history/#identifier-006"/>
  <dcterms:issued rdf:datatype="&xsd;date">1999-07-02</dcterms:issued>
  <dcterms:modified rdf:datatype="&xsd;date">2008-01-14</dcterms:modified>
  <rdfs:comment xml:lang="en">An unambiguous reference to the resource within a given context.</rdfs:comment>
  <rdfs:isDefinedBy rdf:resource="&dc;"/>
  <rdfs:label xml:lang="en">Identifier</rdfs:label>
  <scos:note xml:lang="en">A second property with the same name as this property has been declared in the dcterms: namespace (http://purl.org/dc/terms/).  See the Introduction to the document "DCMI Metadata Terms" (http://dublincore.org/documents/dcmi-terms/) for an explanation.</scos:note>
</rdf:Property>

<rdfs:Class rdf:about="&dcon;Aspect"
    rdfs:label="Aspect">
  <rdfs:comment>At the highlest level, context information is classified under a number of context Aspects. These are provided as subclasses of this abstract class, which is not intended for direct use.</rdfs:comment>
</rdfs:Class>

<rdf:Property rdf:about="&nco;contactMediumComment"
    rdfs:label="contactMediumComment">
  <nao:deprecated rdf:datatype="&xsd;boolean">true</nao:deprecated>
  <rdfs:comment>A comment about the contact medium. (Deprecated in favor of nie:comment or nao:description - based on the context)</rdfs:comment>
  <rdfs:domain rdf:resource="&nco;ContactMedium"/>
  <rdfs:range rdf:resource="&xsd;string"/>
</rdf:Property>

<ncal:JournalStatus rdf:about="&ncal;draftStatus"
    rdfs:label="draftStatus"/>

<rdfs:Class rdf:about="&tmo;SuccessorDependency"
    rdfs:label="SuccessorDependency">
  <rdfs:comment>In a SuccessorrDependency the dependencyMemberA is the task which is to be executed after dependencyMemberB.</rdfs:comment>
  <rdfs:subClassOf rdf:resource="&tmo;PredecessorSuccessorDependency"/>
</rdfs:Class>

<rdf:Property rdf:about="&dcon;networkSpeed"
    rdfs:label="Network Speed Value">
  <rdfs:comment>States the actual speed value for a network connection in the current context.</rdfs:comment>
  <rdfs:domain rdf:resource="&ddo;Network"/>
  <rdfs:range rdf:resource="&xsd;float"/>
  <rdfs:subPropertyOf rdf:resource="&dcon;hasContextAttribute"/>
</rdf:Property>

<rdf:Property rdf:about="&foaf;workInfoHomepage"
    rdfs:label="work info homepage"
    ns:term_status="testing">
  <rdf:type rdf:resource="&owl;ObjectProperty"/>
  <rdfs:comment>A work info homepage of some person; a page about their work for some organization.</rdfs:comment>
  <rdfs:domain rdf:resource="&foaf;Person"/>
  <rdfs:isDefinedBy rdf:resource="&foaf;"/>
  <rdfs:range rdf:resource="&foaf;Document"/>
</rdf:Property>

<rdfs:Class rdf:about="&ncal;Attachment"
    rdfs:label="Attachment">
  <rdfs:subClassOf rdf:resource="&nfo;Attachment"/>
  <rdfs:subClassOf rdf:resource="&rdfs;Resource"/>
  <rdfs:comment>An object attached to a calendar entity. This class has been introduced to serve as a structured value of the ncal:attach property. See the documentation of ncal:attach for details.</rdfs:comment>
</rdfs:Class>

<rdf:Property rdf:about="&ddo;sourceDevice"
    rdfs:label="Source Device">
  <rdfs:comment>Identifies the device that is, or has, enabled a specific Bluetooth network.</rdfs:comment>
  <rdfs:domain rdf:resource="&ddo;Bluetooth"/>
  <rdfs:range rdf:resource="&ddo;Device"/>
</rdf:Property>

<rdfs:Class rdf:about="&ncal;Journal"
    rdfs:label="Journal">
  <rdfs:subClassOf rdf:resource="&nie;InformationElement"/>
  <rdfs:subClassOf rdf:resource="&ncal;UnionOfAlarmEventFreebusyJournalTodo"/>
  <rdfs:subClassOf rdf:resource="&ncal;UnionOfAlarmEventJournalTodo"/>
  <rdfs:subClassOf rdf:resource="&ncal;UnionOfEventFreebusyJournalTodo"/>
  <rdfs:subClassOf rdf:resource="&ncal;UnionOfEventJournalTimezoneTodo"/>
  <rdfs:subClassOf rdf:resource="&ncal;UnionOfEventJournalTodo"/>
  <rdfs:subClassOf rdf:resource="&ncal;UnionOfTimezoneObservanceEventFreebusyJournalTimezoneTodo"/>
  <rdfs:subClassOf rdf:resource="&ncal;UnionOfTimezoneObservanceEventJournalTimezoneTodo"/>
  <rdfs:comment>Provide a grouping of component properties that describe a journal entry.</rdfs:comment>
</rdfs:Class>

<rdfs:Class rdf:about="&nfo;FileHash"
    rdfs:label="FileHash">
  <rdfs:comment>A fingerprint of the file, generated by some hashing function.</rdfs:comment>
  <rdfs:subClassOf rdf:resource="&rdfs;Resource"/>
</rdfs:Class>

<rdf:Property rdf:about="&nexif;whitePoint"
    rdfs:label="whitePoint">
  <rdfs:subPropertyOf rdf:resource="http://www.kanzaki.com/ns/exif#whitePoint"/>
  <rdfs:subPropertyOf rdf:resource="&nexif;imageDataCharacter"/>
  <rdfs:comment>The chromaticity of the white point of the image. Normally this tag is not necessary, since color space is specified in the color space information tag (ColorSpace).
tagNumber: 318</rdfs:comment>
  <rdfs:domain rdf:resource="&nexif;Photo"/>
  <rdfs:range rdf:resource="&xsd;string"/>
</rdf:Property>

<rdfs:Class rdf:about="&tmo;PersonInvolvementRole"
    rdfs:label="PersonInvolvementRole">
  <rdfs:comment>They further specify the type a person was related to an task.
Examples instances  of AttachmentRoles are e.g.</rdfs:comment>
  <rdfs:subClassOf rdf:resource="&tmo;StateTypeRole"/>
</rdfs:Class>

<rdf:Property rdf:about="&nco;publishesPresenceTo"
    rdfs:label="publishesPresenceTo">
  <rdfs:comment>Indicates that this IMAccount publishes its presence information to the other IMAccount.</rdfs:comment>
  <rdfs:domain rdf:resource="&nco;IMAccount"/>
  <rdfs:range rdf:resource="&nco;IMAccount"/>
</rdf:Property>

<rdf:Property rdf:about="&nmo;bcc"
    rdfs:comment="deprecated in favor of nmo:emailBcc"
    rdfs:label="bcc">
  <nao:deprecated rdf:datatype="&xsd;boolean">true</nao:deprecated>
  <rdfs:domain rdf:resource="&nmo;Email"/>
  <rdfs:range rdf:resource="&nco;Contact"/>
  <rdfs:subPropertyOf rdf:resource="&nmo;secondaryRecipient"/>
</rdf:Property>

<rdf:Property rdf:about="&rdfs;domain">
  <rdfs:comment xml:lang="en">A domain of the subject property.</rdfs:comment>
  <rdfs:domain rdf:resource="&rdf;Property"/>
  <rdfs:isDefinedBy rdf:resource="&rdfs;"/>
  <rdfs:label xml:lang="en">domain</rdfs:label>
  <rdfs:range rdf:resource="&rdfs;Class"/>
</rdf:Property>

<rdf:Property rdf:about="&ncal;daylight"
    rdfs:label="daylight">
  <nrl:maxCardinality rdf:datatype="&xsd;integer">1</nrl:maxCardinality>
  <rdfs:comment>Links a timezone with it's daylight observance. This property has no direct equivalent in the RFC 2445. It has been inspired by the structure of the Vtimezone component defined in sec.4.6.5</rdfs:comment>
  <rdfs:domain rdf:resource="&ncal;Timezone"/>
  <rdfs:range rdf:resource="&ncal;TimezoneObservance"/>
</rdf:Property>

<rdf:Property rdf:about="&tmo;abilityCarrier"
    nrl:maxCardinality="1"
    nrl:minCardinality="1"
    rdfs:label="abilityCarrier">
  <rdfs:domain rdf:resource="&tmo;AbilityCarrierInvolvement"/>
  <rdfs:range rdf:resource="&tmo;AbilityCarrier"/>
  <rdfs:subPropertyOf rdf:resource="&pimo;associationMember"/>
</rdf:Property>

<tmo:TransmissionState rdf:about="&tmo;TMO_Instance_TransmissionState_Rejected_Transmitted"
    rdfs:label="TMO_Instance_TransmissionState_Rejected_Transmitted"/>

<rdf:Property rdf:about="&nco;hasPhoneNumber"
    rdfs:label="hasPhoneNumber">
  <rdfs:comment>A number for telephony communication with the object represented by this Contact. An equivalent of the 'TEL' property defined in RFC 2426 Sec. 3.3.1</rdfs:comment>
  <rdfs:domain rdf:resource="&nco;Role"/>
  <rdfs:range rdf:resource="&nco;PhoneNumber"/>
  <rdfs:subPropertyOf rdf:resource="&nco;hasContactMedium"/>
</rdf:Property>

<rdf:Property rdf:about="&nmm;hasSeason"
    rdfs:comment="Relates a TV Series to its seasons"
    rdfs:label="has season">
  <nrl:inverseProperty rdf:resource="&nmm;seasonOf"/>
  <rdfs:domain rdf:resource="&nmm;TVSeries"/>
  <rdfs:range rdf:resource="&nmm;TVSeason"/>
  <rdfs:subPropertyOf rdf:resource="&nie;hasLogicalPart"/>
</rdf:Property>

<rdf:Property rdf:about="&foaf;givenname"
    rdfs:comment="The given name of some person."
    rdfs:label="Given name"
    ns:term_status="archaic">
  <rdf:type rdf:resource="&owl;DatatypeProperty"/>
  <rdfs:isDefinedBy rdf:resource="&foaf;"/>
</rdf:Property>

<rdf:Property rdf:about="&tmo;receiveDateTime"
    nrl:maxCardinality="1"
    rdfs:label="receiveDateTime">
  <rdfs:domain rdf:resource="&tmo;TaskTransmission"/>
  <rdfs:range rdf:resource="&xsd;dateTime"/>
  <rdfs:subPropertyOf rdf:resource="&tmo;dateTime"/>
</rdf:Property>

<rdf:Property rdf:about="&ncal;duration"
    rdfs:label="duration">
  <nrl:maxCardinality rdf:datatype="&xsd;integer">1</nrl:maxCardinality>
  <rdfs:comment>The property specifies a positive duration of time. Inspired by RFC 2445 sec. 4.8.2.5</rdfs:comment>
  <rdfs:domain rdf:resource="&ncal;UnionOfAlarmEventFreebusyTodo"/>
  <rdfs:range rdf:resource="&xsd;duration"/>
</rdf:Property>

<rdfs:Class rdf:about="&dpo;TimePeriod"
    rdfs:label="Time Period">
  <rdfs:comment>Quantifiable presence information concerning pre-established time periods in an agent's days, weeks, months, and years.</rdfs:comment>
  <rdfs:subClassOf rdf:resource="&dpo;QuantifiableComponent"/>
</rdfs:Class>

<rdfs:Class rdf:about="&nco;IMStatusType"
    rdfs:label="instant messaging status type">
  <rdfs:comment>The status type of an IMAccount. Based on the Connection_Presence_Type enumeration of the Telepathy project: http://telepathy.freedesktop.org/spec/Connection_Interface_Simple_Presence.html#Enum:Connection_Presence_Type</rdfs:comment>
  <rdfs:subClassOf rdf:resource="&rdfs;Resource"/>
</rdfs:Class>

<rdfs:Class rdf:about="&cnt;ContentAsText">
  <rdf:type rdf:resource="&owl;Class"/>
  <rdfs:comment xml:lang="en">The text content (can be used for text content).</rdfs:comment>
  <rdfs:label xml:lang="en">Text content</rdfs:label>
  <rdfs:subClassOf rdf:resource="&cnt;Content"/>
</rdfs:Class>

<rdfs:Class rdf:about="&nco;ContactListDataObject"
    rdfs:label="ContactListDataObject">
  <rdfs:comment>An entity occuring on a contact list (usually interpreted as an nco:Contact)</rdfs:comment>
  <rdfs:subClassOf rdf:resource="&nie;DataObject"/>
</rdfs:Class>

<rdf:Property rdf:about="&dcon;validity"
    rdfs:label="Validity Period">
  <rdfs:comment>Live context element observations have different validity periods, which mean they remain active only for a specified time interval after they have been sensed or otherwise detected. The value for this property denotes the time when the element observation's relevance expires.</rdfs:comment>
  <rdfs:domain rdf:resource="&dcon;Observation"/>
  <rdfs:range rdf:resource="&xsd;dateTime"/>
  <rdfs:subPropertyOf rdf:resource="&dcon;hasContextAttribute"/>
</rdf:Property>

<rdf:Property rdf:about="&dplo;replyOf"
    rdfs:label="reply of">
  <nrl:inverseProperty rdf:resource="&dplo;hasReply"/>
  <nrl:maxCardinality rdf:datatype="&xsd;nonNegativeInteger">1</nrl:maxCardinality>
  <rdfs:comment>Links an in-reply-to livepost to the original livepost. This property is transitive, and is the inverse of dlpo:hasReply.</rdfs:comment>
  <rdfs:domain rdf:resource="&dplo;LivePost"/>
  <rdfs:range rdf:resource="&dplo;LivePost"/>
  <rdfs:subPropertyOf rdf:resource="http://rdfs.org/sioc/ns#reply_of"/>
</rdf:Property>

<rdf:Property rdf:about="&scos;definition">
  <rdf:type rdf:resource="&owl;AnnotationProperty"/>
  <rdfs:isDefinedBy rdf:resource="http://www.w3.org/2004/02/skos/core"/>
  <rdfs:label xml:lang="en">definition</rdfs:label>
  <rdfs:subPropertyOf rdf:resource="&scos;note"/>
  <scos:definition xml:lang="en">A statement or formal explanation of the meaning of a concept.</scos:definition>
</rdf:Property>

<nrl:InverseFunctionalProperty rdf:about="&nrl;coreGraphMetadataFor"
    rdfs:label="coreGraphMetadataFor">
  <rdf:type rdf:resource="&rdf;Property"/>
  <rdfs:comment>Links a metadata graph to the graph for which it specifies the core graph properties including the semantics and the graph namespace. A graph can have only one unique core metadata graph</rdfs:comment>
  <rdfs:domain rdf:resource="&nrl;GraphMetadata"/>
  <rdfs:range rdf:resource="&nrl;Graph"/>
  <rdfs:subPropertyOf rdf:resource="&nrl;graphMetadataFor"/>
</nrl:InverseFunctionalProperty>

<rdf:Property rdf:about="&nexif;fNumber"
    rdfs:comment="tagNumber: 33437
F number"
    rdfs:label="fNumber">
  <rdfs:subPropertyOf rdf:resource="http://www.kanzaki.com/ns/exif#fNumber"/>
  <rdfs:subPropertyOf rdf:resource="&nexif;pictTaking"/>
  <rdfs:domain rdf:resource="&nexif;Photo"/>
  <rdfs:range rdf:resource="&xsd;float"/>
</rdf:Property>

<rdf:Property rdf:about="&dcon;connection"
    rdfs:label="connection">
  <rdfs:comment>Refers to a pre-defined traveling direction characterising a context instance.</rdfs:comment>
  <rdfs:domain rdf:resource="&dcon;Connectivity"/>
  <rdfs:range rdf:resource="&ddo;Network"/>
  <rdfs:subPropertyOf rdf:resource="&dcon;hasContextElement"/>
</rdf:Property>

<rdf:Property rdf:about="&nfo;deletionDate"
    rdfs:comment="The date and time of the deletion."
    rdfs:label="deletionDate">
  <nrl:maxCardinality rdf:datatype="&xsd;integer">1</nrl:maxCardinality>
  <rdfs:domain rdf:resource="&nfo;DeletedResource"/>
  <rdfs:range rdf:resource="&xsd;dateTime"/>
</rdf:Property>

<rdf:Property rdf:about="&nexif;subsecond"
    rdfs:label="subsecond"/>

<rdf:Property rdf:about="&tmo;dependency"
    rdfs:label="dependency">
  <rdfs:domain rdf:resource="&tmo;Task"/>
  <rdfs:range rdf:resource="&tmo;TaskDependency"/>
</rdf:Property>

<ncal:RecurrenceIdentifierRange rdf:about="&ncal;thisAndPriorRange"
    rdfs:label="thisAndPriorRange"/>

<tmo:PersonInvolvementRole rdf:about="&tmo;TMO_Instance_PersonInvolvementRole_Controller"
    rdfs:label="TMO_Instance_PersonInvolvementRole_Controller"/>

<rdf:Description rdf:about="&dctypes;">
  <dcterms:modified rdf:datatype="&xsd;date">2012-06-14</dcterms:modified>
  <dcterms:publisher rdf:resource="http://purl.org/dc/aboutdcmi#DCMI"/>
  <dcterms:title xml:lang="en">DCMI Type Vocabulary</dcterms:title>
</rdf:Description>

<rdfs:Class rdf:about="&ddo;LocalAreaNetwork"
    rdfs:label="LocalAreaNetwork">
  <rdfs:comment>A Local Area Network (LAN) is a private computer network that enables communication among computerised devices in a limited area.</rdfs:comment>
  <rdfs:subClassOf rdf:resource="&ddo;ComputerNetwork"/>
</rdfs:Class>

<rdf:Property rdf:about="&dpo;maxAltitude"
    rdfs:label="Maximum Altitude">
  <rdfs:comment>A subproperty of dpo:maxValue that defines an upperbound on the observed altitude height value (in metres) such that it can classify as a dpo:Altitude instance. It can be used in conjunction with dpo:minAltitude, i.e. specific instances of dpo:Altitude have a pre-defined range of observable real-world agent altitude.</rdfs:comment>
  <rdfs:domain rdf:resource="&dpo;Altitude"/>
  <rdfs:range rdf:resource="&xsd;float"/>
  <rdfs:subPropertyOf rdf:resource="&dpo;maxValue"/>
</rdf:Property>

<rdf:Property rdf:about="&dcon;duration"
    rdfs:comment="Specifies the duration since the start of the activity."
    rdfs:label="Duration">
  <rdfs:domain rdf:resource="&dpo;Activity"/>
  <rdfs:range rdf:resource="&xsd;nonNegativeInteger"/>
  <rdfs:subPropertyOf rdf:resource="&dcon;hasContextAttribute"/>
</rdf:Property>

<tmo:Urgency rdf:about="&tmo;TMO_Instance_Urgency_07"
    rdfs:label="TMO_Instance_Urgency_07"/>

<rdfs:Class rdf:about="&rdf;Seq">
  <rdfs:comment xml:lang="en">The class of ordered containers.</rdfs:comment>
  <rdfs:isDefinedBy rdf:resource="&rdf;"/>
  <rdfs:label xml:lang="en">Seq</rdfs:label>
  <rdfs:subClassOf rdf:resource="&rdfs;Container"/>
</rdfs:Class>

<rdf:Property rdf:about="&ncal;member"
    rdfs:label="member">
  <rdfs:comment>To specify the group or list membership of the calendar user specified by the property. Inspired by RFC 2445 sec. 4.2.11. Originally this parameter had a value type of CAL-ADDRESS. This has been expressed as nco:Contact to promote integration between NCAL and NCO</rdfs:comment>
  <rdfs:domain rdf:resource="&ncal;Attendee"/>
  <rdfs:range rdf:resource="&nco;Contact"/>
</rdf:Property>

<dcterms:AgentClass rdf:about="&dcterms;Agent">
  <dcterms:description xml:lang="en">Examples of Agent include person, organization, and software agent.</dcterms:description>
  <dcterms:hasVersion rdf:resource="http://dublincore.org/usage/terms/history/#Agent-001"/>
  <dcterms:issued rdf:datatype="&xsd;date">2008-01-14</dcterms:issued>
  <rdf:type rdf:resource="&rdfs;Class"/>
  <rdfs:comment xml:lang="en">A resource that acts or has the power to act.</rdfs:comment>
  <rdfs:isDefinedBy rdf:resource="&dcterms;"/>
  <rdfs:label xml:lang="en">Agent</rdfs:label>
</dcterms:AgentClass>

<rdf:Property rdf:about="&ncal;todoStatus"
    rdfs:label="status">
  <nrl:maxCardinality rdf:datatype="&xsd;integer">1</nrl:maxCardinality>
  <rdfs:comment>Defines the overall status or confirmation for a todo. Based on the STATUS property defined in RFC 2445 sec. 4.8.1.11.</rdfs:comment>
  <rdfs:domain rdf:resource="&ncal;Todo"/>
  <rdfs:range rdf:resource="&ncal;TodoStatus"/>
</rdf:Property>

<rdfs:Class rdf:about="&ncal;UnionOfAlarmEventFreebusyTodo"
    rdfs:label="UnionOfAlarmEventFreebusyTodo">
  <rdfs:subClassOf rdf:resource="&ncal;UnionParentClass"/>
</rdfs:Class>

<rdfs:Class rdf:about="&dpo;PresenceComponent"
    rdfs:label="Presence Component">
  <rdfs:comment>Represents a wide variety of components relating to a user's presence, which is an ensemble of physical and virtual context properties relating to an agent's circumstances and activities. User context properties obtained from different kinds of sensors can be interpreted, resolved or mapped to loosely-defined or fuzzy presence component counterparts. A characteristic of these components is that they are independent of time, i.e., each component can characterise an agent's presence in multiple and different times. Presence components are subclasses of pimo:Thing, and have two main subclasses: quantifiable and non-quantifiable presence components.</rdfs:comment>
  <rdfs:subClassOf rdf:resource="&pimo;Thing"/>
</rdfs:Class>

<nrl:TransitiveProperty rdf:about="&drmo;precededBy"
    rdfs:label="preceeded by">
  <nrl:inverseProperty rdf:resource="&drmo;succeededBy"/>
  <rdf:type rdf:resource="&rdf;Property"/>
  <rdfs:comment>TWO conditions (A and B) may be composed together using the precededBy Property. If Condition B is preceded by Condition A, the actions are only triggered if Condition A happens at any time before Condition B. This is the inverse property of drmo:succeededBy.</rdfs:comment>
  <rdfs:domain rdf:resource="&drmo;Condition"/>
  <rdfs:range rdf:resource="&drmo;Condition"/>
</nrl:TransitiveProperty>

<rdf:Property rdf:about="&nfo;freeSpace"
    rdfs:comment="Unoccupied storage space of the filesystem."
    rdfs:label="freeSpace">
  <nrl:maxCardinality rdf:datatype="&xsd;integer">1</nrl:maxCardinality>
  <rdfs:domain rdf:resource="&nfo;Filesystem"/>
  <rdfs:range rdf:resource="&xsd;integer"/>
</rdf:Property>

<ncal:RecurrenceIdentifierRange rdf:about="&ncal;thisAndFutureRange"
    rdfs:label="thisAndFutureRange"/>

<rdf:Property rdf:about="&nexif;gpsStatus"
    rdfs:label="gpsStatus">
  <rdfs:subPropertyOf rdf:resource="http://www.kanzaki.com/ns/exif#gpsStatus"/>
  <rdfs:subPropertyOf rdf:resource="&nexif;gpsInfo"/>
  <rdfs:comment>tagNumber: 9
The status of the GPS receiver when the image is recorded. 'A' means measurement is in progress, and 'V' means the measurement is Interoperability.</rdfs:comment>
  <rdfs:domain rdf:resource="&nexif;Photo"/>
  <rdfs:range rdf:resource="&xsd;string"/>
</rdf:Property>

<rdf:Property rdf:about="&rdfs;seeAlso">
  <rdfs:comment xml:lang="en">Further information about the subject resource.</rdfs:comment>
  <rdfs:domain rdf:resource="&rdfs;Resource"/>
  <rdfs:isDefinedBy rdf:resource="&rdfs;"/>
  <rdfs:label xml:lang="en">seeAlso</rdfs:label>
  <rdfs:range rdf:resource="&rdfs;Resource"/>
</rdf:Property>

<rdf:Property rdf:about="&dc;creator">
  <dcterms:description xml:lang="en">Examples of a Creator include a person, an organization, or a service. Typically, the name of a Creator should be used to indicate the entity.</dcterms:description>
  <dcterms:hasVersion rdf:resource="http://dublincore.org/usage/terms/history/#creator-006"/>
  <dcterms:issued rdf:datatype="&xsd;date">1999-07-02</dcterms:issued>
  <dcterms:modified rdf:datatype="&xsd;date">2008-01-14</dcterms:modified>
  <rdfs:comment xml:lang="en">An entity primarily responsible for making the resource.</rdfs:comment>
  <rdfs:isDefinedBy rdf:resource="&dc;"/>
  <rdfs:label xml:lang="en">Creator</rdfs:label>
  <scos:note xml:lang="en">A second property with the same name as this property has been declared in the dcterms: namespace (http://purl.org/dc/terms/).  See the Introduction to the document "DCMI Metadata Terms" (http://dublincore.org/documents/dcmi-terms/) for an explanation.</scos:note>
</rdf:Property>

<rdf:Property rdf:about="&duho;isPastDataGraphFor"
    rdfs:label="has past data graph">
  <nrl:inverseProperty rdf:resource="&nao;hasPastDataGraph"/>
  <rdfs:comment>Links a graph to the resource for which contains earlier metadata, before it changed. Its typical usage would be to persist a copy of a file's metadata before it is changed. Inverse property of duho:isPastDataGraphFor.</rdfs:comment>
  <rdfs:domain rdf:resource="&duho;Log"/>
  <rdfs:range rdf:resource="&rdfs;Resource"/>
  <rdfs:subPropertyOf rdf:resource="&nao;isDataGraphFor"/>
</rdf:Property>

<rdfs:Datatype rdf:about="&rdf;XMLLiteral">
  <rdfs:comment xml:lang="en">The class of XML literal values.</rdfs:comment>
  <rdfs:isDefinedBy rdf:resource="&rdf;"/>
  <rdfs:label xml:lang="en">XMLLiteral</rdfs:label>
  <rdfs:subClassOf rdf:resource="&rdfs;Literal"/>
</rdfs:Datatype>

<rdf:Property rdf:about="&dcterms;medium">
  <rdfs:subPropertyOf rdf:resource="&dc;format"/>
  <rdfs:subPropertyOf rdf:resource="&dcterms;format"/>
  <dcterms:hasVersion rdf:resource="http://dublincore.org/usage/terms/history/#medium-003"/>
  <dcterms:issued rdf:datatype="&xsd;date">2000-07-11</dcterms:issued>
  <dcterms:modified rdf:datatype="&xsd;date">2008-01-14</dcterms:modified>
  <rdfs:comment xml:lang="en">The material or physical carrier of the resource.</rdfs:comment>
  <rdfs:domain rdf:resource="&dcterms;PhysicalResource"/>
  <rdfs:isDefinedBy rdf:resource="&dcterms;"/>
  <rdfs:label xml:lang="en">Medium</rdfs:label>
  <rdfs:range rdf:resource="&dcterms;PhysicalMedium"/>
</rdf:Property>

<rdf:Property rdf:about="&nmo;htmlMessageContent"
    rdfs:label="htmlMessageContent">
  <rdfs:comment>HTML representation of the body of the message. For multipart messages, all parts are concatenated into the value of this property. Attachments, whose mimeTypes are different from text/plain or message/rfc822 are considered separate DataObjects and are therefore not included in the value of this property.</rdfs:comment>
  <rdfs:domain rdf:resource="&nmo;Message"/>
  <rdfs:range rdf:resource="&xsd;string"/>
  <rdfs:subPropertyOf rdf:resource="&nie;htmlContent"/>
</rdf:Property>

<rdf:Property rdf:about="&nid3;commercialInformationURL"
    rdfs:label="commercialInformationURL">
  <rdfs:comment>WCOM
The 'Commercial information' frame is a URL pointing at a webpage with information such as where the album can be bought. There may be more than one "WCOM" frame in a tag, but not with the same content.</rdfs:comment>
  <rdfs:domain rdf:resource="&nid3;ID3Audio"/>
  <rdfs:range rdf:resource="&rdfs;Resource"/>
</rdf:Property>

<rdf:Property rdf:about="&drmo;or"
    rdfs:label="or">
  <rdfs:comment>Combine TWO condition blocks together with the OR operator. For the rule to trigger its actions, only one of the conditions have to be true at any given time.</rdfs:comment>
  <rdfs:domain rdf:resource="&drmo;Condition"/>
  <rdfs:range rdf:resource="&drmo;Condition"/>
</rdf:Property>

<rdf:Property rdf:about="&pimo;hasInterest"
    rdfs:label="has interest">
  <rdfs:range rdf:resource="&pimo;Tag"/>
  <rdfs:range rdf:resource="&pimo;Topic"/>
  <nrl:inverseProperty rdf:resource="&pimo;isInterestOf"/>
  <rdfs:comment>Marks a pimo:Tag or a pimo:Topic (its subclass) as an interest of a person or a group.</rdfs:comment>
  <rdfs:domain rdf:resource="&pimo;Agent"/>
  <rdfs:subPropertyOf rdf:resource="&pimo;hasTag"/>
</rdf:Property>

<rdf:Property rdf:about="&nmo;emailBcc"
    rdfs:label="bcc">
  <rdfs:comment>A Contact that is to receive a bcc of the email. A Bcc (blind carbon copy) is a copy of an email message sent to a recipient whose email address does not appear in the message.</rdfs:comment>
  <rdfs:domain rdf:resource="&nmo;Email"/>
  <rdfs:range rdf:resource="&nco;ContactMedium"/>
  <rdfs:subPropertyOf rdf:resource="&nmo;secondaryMessageRecipient"/>
</rdf:Property>

<rdf:Property rdf:about="&foaf;lastName"
    rdfs:comment="The last name of a person."
    rdfs:label="lastName"
    ns:term_status="testing">
  <rdf:type rdf:resource="&owl;DatatypeProperty"/>
  <rdfs:domain rdf:resource="&foaf;Person"/>
  <rdfs:isDefinedBy rdf:resource="&foaf;"/>
  <rdfs:range rdf:resource="&rdfs;Literal"/>
</rdf:Property>

<rdf:Property rdf:about="&dpo;maxSpeed"
    rdfs:label="Maximum Speed">
  <rdfs:comment>A subproperty of dpo:maxValue that defines an upperbound on the observed speed value (in metres per second) such that it can classify as a dpo:Movement instance. It can be used in conjunction with dpo:minSpeed, i.e. specific instances of dpo:Movement have a pre-defined range of observable real-world agent speed levels.</rdfs:comment>
  <rdfs:domain rdf:resource="&dpo;Movement"/>
  <rdfs:range rdf:resource="&xsd;float"/>
  <rdfs:subPropertyOf rdf:resource="&dpo;maxValue"/>
</rdf:Property>

<ncal:AttachmentEncoding rdf:about="&ncal;_8bitEncoding"
    rdfs:label="_8bitEncoding"/>

<ncal:AttendeeRole rdf:about="&ncal;reqParticipantRole"
    rdfs:label="reqParticipantRole"/>

<rdf:Property rdf:about="&dcterms;extent">
  <rdfs:subPropertyOf rdf:resource="&dc;format"/>
  <rdfs:subPropertyOf rdf:resource="&dcterms;format"/>
  <dcterms:hasVersion rdf:resource="http://dublincore.org/usage/terms/history/#extent-003"/>
  <dcterms:issued rdf:datatype="&xsd;date">2000-07-11</dcterms:issued>
  <dcterms:modified rdf:datatype="&xsd;date">2008-01-14</dcterms:modified>
  <rdfs:comment xml:lang="en">The size or duration of the resource.</rdfs:comment>
  <rdfs:isDefinedBy rdf:resource="&dcterms;"/>
  <rdfs:label xml:lang="en">Extent</rdfs:label>
  <rdfs:range rdf:resource="&dcterms;SizeOrDuration"/>
</rdf:Property>

<rdf:Property rdf:about="&nexif;gpsDifferential"
    rdfs:label="gpsDifferential">
  <rdfs:subPropertyOf rdf:resource="http://www.kanzaki.com/ns/exif#gpsDifferential"/>
  <rdfs:subPropertyOf rdf:resource="&nexif;gpsInfo"/>
  <rdfs:comment>tagNumber: 30
Indicates whether differential correction is applied to the GPS receiver.</rdfs:comment>
  <rdfs:domain rdf:resource="&nexif;Photo"/>
  <rdfs:range rdf:resource="&xsd;string"/>
</rdf:Property>

<rdfs:Class rdf:about="&ncal;UnionOfEventFreebusyJournalTodo"
    rdfs:label="UnionOfEventFreebusyJournalTodo">
  <rdfs:subClassOf rdf:resource="&ncal;UnionParentClass"/>
</rdfs:Class>

<rdf:Property rdf:about="&ncal;version"
    rdfs:label="version">
  <rdfs:comment>This property specifies the identifier corresponding to the highest version number or the minimum and maximum range of the iCalendar specification that is required in order to interpret the iCalendar object. Defined in RFC 2445 sec. 4.7.4</rdfs:comment>
  <rdfs:domain rdf:resource="&ncal;Calendar"/>
  <rdfs:range rdf:resource="&xsd;string"/>
  <rdfs:subPropertyOf rdf:resource="&nie;generatorOption"/>
</rdf:Property>

<rdf:Property rdf:about="&tmo;taskTransmission"
    rdfs:label="taskTransmission">
  <nrl:inverseProperty rdf:resource="&tmo;transmissionTask"/>
  <rdfs:domain rdf:resource="&tmo;Task"/>
  <rdfs:range rdf:resource="&tmo;TaskTransmission"/>
</rdf:Property>

<rdfs:Class rdf:about="&dpo;WeatherConditions"
    rdfs:label="Weather Conditions">
  <rdfs:comment>Quantifiable presence information concerning the weather (current, forecast) in the agent's surroundings.</rdfs:comment>
  <rdfs:subClassOf rdf:resource="&dpo;QuantifiableComponent"/>
</rdfs:Class>

<rdf:Property rdf:about="&dcon;isExcluder"
    rdfs:label="is Required">
  <rdfs:comment>This property marks those context elements whose presence excludes a situation from occurring. If such an element is active, then the correspoding situation is excluded from candidate active situations.</rdfs:comment>
  <rdfs:domain rdf:resource="&dcon;Element"/>
  <rdfs:range rdf:resource="&xsd;boolean"/>
</rdf:Property>

<rdf:Property rdf:about="&nfo;occupiedSpace"
    rdfs:comment="Occupied storage space of the filesystem."
    rdfs:label="occupiedSpace">
  <nrl:maxCardinality rdf:datatype="&xsd;integer">1</nrl:maxCardinality>
  <rdfs:domain rdf:resource="&nfo;Filesystem"/>
  <rdfs:range rdf:resource="&xsd;integer"/>
</rdf:Property>

<owl:ObjectProperty rdf:about="&oa;hasScope">
  <rdfs:comment xml:lang="en">The relationship between a Specific Resource and the resource that provides the scope or context for it in this Annotation.

There MAY be 0 or more hasScope relationships for each Specific Resource.</rdfs:comment>
  <rdfs:domain rdf:resource="&oa;SpecificResource"/>
  <rdfs:isDefinedBy rdf:resource="&oa;"/>
  <rdfs:label xml:lang="en">hasScope</rdfs:label>
</owl:ObjectProperty>

<rdfs:Class rdf:about="&rdfs;Literal">
  <rdfs:comment xml:lang="en">The class of literal values, eg. textual strings and integers.</rdfs:comment>
  <rdfs:isDefinedBy rdf:resource="&rdfs;"/>
  <rdfs:label xml:lang="en">Literal</rdfs:label>
  <rdfs:subClassOf rdf:resource="&rdfs;Resource"/>
</rdfs:Class>

<rdf:Property rdf:about="&ncal;method"
    rdfs:label="method">
  <nrl:maxCardinality rdf:datatype="&xsd;integer">1</nrl:maxCardinality>
  <rdfs:comment>This property defines the iCalendar object method associated with the calendar object. Defined in RFC 2445 sec. 4.7.2</rdfs:comment>
  <rdfs:domain rdf:resource="&ncal;Calendar"/>
  <rdfs:range rdf:resource="&xsd;string"/>
</rdf:Property>

<nrl:GraphView rdf:about="&pimo;FullPimoView"
    rdfs:label="FullPimoView"/>

<rdfs:Class rdf:about="&nfo;PlacemarkContainer"
    rdfs:label="Placemark Container">
  <rdfs:comment>A data object containing placemark(s). Use nie:contentCreated to represent the date when the user created the dataobject, nao:creator for defining the creator, nie:contentLastModified for modifications. nfo:containsPlacemark to refer to individual placemarks within.</rdfs:comment>
  <rdfs:subClassOf rdf:resource="&nie;InformationElement"/>
</rdfs:Class>

<rdf:Property rdf:about="&foaf;topic_interest"
    rdfs:comment="A thing of interest to this person."
    rdfs:label="topic_interest"
    ns:term_status="testing">
  <rdf:type rdf:resource="&owl;ObjectProperty"/>
  <rdfs:domain rdf:resource="&foaf;Agent"/>
  <rdfs:isDefinedBy rdf:resource="&foaf;"/>
  <rdfs:range rdf:resource="&owl;Thing"/>
</rdf:Property>

<rdf:Property rdf:about="&nid3;userDefinedFrameValue"
    rdfs:comment="Value of a user-defined frame."
    rdfs:label="userDefinedFrameValue">
  <rdfs:domain rdf:resource="&nid3;UserDefinedFrame"/>
  <rdfs:range rdf:resource="&xsd;string"/>
</rdf:Property>

<rdf:Property rdf:about="&dcon;distance"
    rdfs:label="Distance Value">
  <rdfs:comment>Records the approximate distance between a device (as a proxy for the user) and an item. Not to be confused with dcon:distanceCovered. As this context attribute can be attached to instances of ncal:Event, pimo:Location, dpo:Place and pimo:Person, the domain of this property is generalised to dcon:Observation. However, the attachment of this attribute to other instances is not considered correct application of the DCON vocabulary.</rdfs:comment>
  <rdfs:domain rdf:resource="&dcon;Observation"/>
  <rdfs:range rdf:resource="&xsd;nonNegativeInteger"/>
  <rdfs:subPropertyOf rdf:resource="&dcon;hasContextAttribute"/>
</rdf:Property>

<rdf:Property rdf:about="&tmo;attachmentReference"
    nrl:maxCardinality="1"
    nrl:minCardinality="1"
    rdfs:label="attachmentReference">
  <rdfs:domain rdf:resource="&tmo;Attachment"/>
  <rdfs:range rdf:resource="&rdfs;Resource"/>
  <rdfs:subPropertyOf rdf:resource="&pimo;associationMember"/>
</rdf:Property>

<rdf:Property rdf:about="&dcterms;issued">
  <rdfs:subPropertyOf rdf:resource="&dc;date"/>
  <rdfs:subPropertyOf rdf:resource="&dcterms;date"/>
  <dcterms:hasVersion rdf:resource="http://dublincore.org/usage/terms/history/#issued-003"/>
  <dcterms:issued rdf:datatype="&xsd;date">2000-07-11</dcterms:issued>
  <dcterms:modified rdf:datatype="&xsd;date">2008-01-14</dcterms:modified>
  <rdfs:comment xml:lang="en">Date of formal issuance (e.g., publication) of the resource.</rdfs:comment>
  <rdfs:isDefinedBy rdf:resource="&dcterms;"/>
  <rdfs:label xml:lang="en">Date Issued</rdfs:label>
  <rdfs:range rdf:resource="&rdfs;Literal"/>
</rdf:Property>

<rdf:Property rdf:about="&nmm;beatsPerMinute"
    rdfs:comment="beats per minute"
    rdfs:label="Beats per minute">
  <rdfs:domain rdf:resource="&nmm;MusicPiece"/>
  <rdfs:range rdf:resource="&xsd;integer"/>
</rdf:Property>

<rdfs:Class rdf:about="&nrl;Configuration"
    rdfs:comment="Represents a named graph containing configuration data"
    rdfs:label="Configuration">
  <rdfs:subClassOf rdf:resource="&nrl;Data"/>
</rdfs:Class>

<rdf:Property rdf:about="&dcon;lastMovementRegistered"
    rdfs:label="Last Movement Registered">
  <rdfs:comment>The last date and time for which a portable device was detected to be moving. This information relies on embedded accelerometers and other motion sensors.</rdfs:comment>
  <rdfs:domain rdf:resource="&nie;DataSource"/>
  <rdfs:range rdf:resource="&xsd;dateTime"/>
</rdf:Property>

<rdf:Property rdf:about="&pimo;isRelated"
    rdfs:label="is related">
  <rdfs:subPropertyOf rdf:resource="&nao;isRelated"/>
  <rdfs:subPropertyOf rdf:resource="&pimo;objectProperty"/>
  <nrl:inverseProperty rdf:resource="&pimo;isRelated"/>
  <rdfs:comment>The thing is related to the other thing. Similar in meaning to skos:related. Symmetric but not transitive.</rdfs:comment>
  <rdfs:domain rdf:resource="&pimo;Thing"/>
  <rdfs:range rdf:resource="&pimo;Thing"/>
</rdf:Property>

<rdf:Property rdf:about="&dpo;maxTemperature"
    rdfs:label="Maximum Temperature">
  <rdfs:comment>A subproperty of dpo:maxValue that defines an upperbound on the observed temperature value (in degrees celcius) such that it can classify as a dpo:Temperature or dpo:WeatherCondition instance. It can be used in conjunction with dpo:minTemperature, i.e. specific instances of the former two classes have a pre-defined range of observable real-world temperatures. Since this property has the described dual-domain, the domain is generic. However, it is not meant to be attached to other types of quantifiable component instances.</rdfs:comment>
  <rdfs:domain rdf:resource="&dpo;QuantifiableComponent"/>
  <rdfs:range rdf:resource="&xsd;float"/>
  <rdfs:subPropertyOf rdf:resource="&dpo;maxValue"/>
</rdf:Property>

<rdfs:Class rdf:about="&dcterms;PhysicalResource">
  <dcterms:hasVersion rdf:resource="http://dublincore.org/usage/terms/history/#PhysicalResource-001"/>
  <dcterms:issued rdf:datatype="&xsd;date">2008-01-14</dcterms:issued>
  <rdfs:comment xml:lang="en">A material thing.</rdfs:comment>
  <rdfs:isDefinedBy rdf:resource="&dcterms;"/>
  <rdfs:label xml:lang="en">Physical Resource</rdfs:label>
</rdfs:Class>

<rdfs:Class rdf:about="&nco;IMCapability"
    rdfs:comment="Capabilities of a cetain IMAccount."
    rdfs:label="imCapability">
  <rdfs:subClassOf rdf:resource="&rdfs;Resource"/>
</rdfs:Class>

<rdfs:Class rdf:about="&dcterms;FileFormat">
  <dcterms:description xml:lang="en">Examples include the formats defined by the list of Internet Media Types.</dcterms:description>
  <dcterms:hasVersion rdf:resource="http://dublincore.org/usage/terms/history/#FileFormat-001"/>
  <dcterms:issued rdf:datatype="&xsd;date">2008-01-14</dcterms:issued>
  <rdfs:comment xml:lang="en">A digital resource format.</rdfs:comment>
  <rdfs:isDefinedBy rdf:resource="&dcterms;"/>
  <rdfs:label xml:lang="en">File Format</rdfs:label>
  <rdfs:subClassOf rdf:resource="&dcterms;MediaType"/>
</rdfs:Class>

<rdf:Property rdf:about="&dpo;minTime"
    rdfs:label="Minimum Time">
  <rdfs:comment>A subproperty of dpo:minValue that defines a lowerbound on the observed time value (in xsd:time format) such that it can classify as a dpo:TimePeriod instance.  It can be used in conjunction with dpo:maxTime, i.e. specific instances of dpo:TimePeriod have a pre-defined range of observable real-world time periods.</rdfs:comment>
  <rdfs:domain rdf:resource="&dpo;TimePeriod"/>
  <rdfs:range rdf:resource="&xsd;time"/>
  <rdfs:subPropertyOf rdf:resource="&dpo;minValue"/>
</rdf:Property>

<rdfs:Class rdf:about="&nfo;Video"
    rdfs:comment="A video file."
    rdfs:label="Video">
  <rdfs:subClassOf rdf:resource="&nfo;Visual"/>
</rdfs:Class>

<rdf:Property rdf:about="&scos;prefLabel">
  <rdfs:comment xml:lang="en">A resource has no more than one value of skos:prefLabel per language tag, and no more than one value of skos:prefLabel without language tag.</rdfs:comment>
  <rdfs:comment xml:lang="en">The range of skos:prefLabel is the class of RDF plain literals.</rdfs:comment>
  <rdfs:comment xml:lang="en">skos:prefLabel, skos:altLabel and skos:hiddenLabel are pairwise
      disjoint properties.</rdfs:comment>
  <rdf:type rdf:resource="&owl;AnnotationProperty"/>
  <rdfs:isDefinedBy rdf:resource="http://www.w3.org/2004/02/skos/core"/>
  <rdfs:label xml:lang="en">preferred label</rdfs:label>
  <rdfs:subPropertyOf rdf:resource="&rdfs;label"/>
  <scos:definition xml:lang="en">The preferred lexical label for a resource, in a given language.</scos:definition>
</rdf:Property>

<rdfs:Class rdf:about="&dcterms;MediaType">
  <dcterms:hasVersion rdf:resource="http://dublincore.org/usage/terms/history/#MediaType-001"/>
  <dcterms:issued rdf:datatype="&xsd;date">2008-01-14</dcterms:issued>
  <rdfs:comment xml:lang="en">A file format or physical medium.</rdfs:comment>
  <rdfs:isDefinedBy rdf:resource="&dcterms;"/>
  <rdfs:label xml:lang="en">Media Type</rdfs:label>
  <rdfs:subClassOf rdf:resource="&dcterms;MediaTypeOrExtent"/>
</rdfs:Class>

<tmo:AttachmentRole rdf:about="&tmo;TMO_Instance_AttachmentRole_Required"
    rdfs:label="TMO_Instance_AttachmentRole_Required"/>

<rdf:Property rdf:about="&ncal;resourcesAltRep"
    rdfs:label="resourcesAltRep">
  <rdfs:comment>Alternate representation of the resources needed for an event or todo. Introduced to cover the ALTREP parameter of the resources property. See documentation for ncal:resources for details.</rdfs:comment>
  <rdfs:domain rdf:resource="&ncal;UnionOfEventTodo"/>
  <rdfs:range rdf:resource="&rdfs;Resource"/>
</rdf:Property>

<rdf:Property rdf:about="&dcon;currentTemperature"
    rdfs:label="Current Temperature">
  <rdfs:comment>Refers to a pre-defined environmental temperature range characterising a context instance.</rdfs:comment>
  <rdfs:domain rdf:resource="&dcon;Environment"/>
  <rdfs:range rdf:resource="&dpo;Temperature"/>
  <rdfs:subPropertyOf rdf:resource="&dcon;hasContextElement"/>
</rdf:Property>

<rdfs:Class rdf:about="&dcon;Connectivity"
    rdfs:label="Connectivity">
  <rdfs:comment>The connectivity aspect covers context elements relating to the digital networks that are in range of the users' devices.</rdfs:comment>
  <rdfs:subClassOf rdf:resource="&dcon;Aspect"/>
</rdfs:Class>

<rdf:Property rdf:about="&nid3;initialKey"
    rdfs:label="initialKey">
  <rdfs:comment>TKEY
The 'Initial key' frame contains the musical key in which the sound starts. It is represented as a string with a maximum length of three characters. The ground keys are represented with "A","B","C","D","E", "F" and "G" and halfkeys represented with "b" and "#". Minor is represented as "m". Example "Cbm". Off key is represented with an "o" only.</rdfs:comment>
  <rdfs:domain rdf:resource="&nid3;ID3Audio"/>
  <rdfs:range rdf:resource="&xsd;string"/>
</rdf:Property>

<tmo:Urgency rdf:about="&tmo;TMO_Instance_Urgency_04"
    rdfs:label="TMO_Instance_Urgency_04"/>

<rdfs:Class rdf:about="&nfo;SourceCode"
    rdfs:comment="Code in a compilable or interpreted programming language."
    rdfs:label="SourceCode">
  <rdfs:subClassOf rdf:resource="&nfo;PlainTextDocument"/>
</rdfs:Class>

<rdf:Property rdf:about="&rdf;subject">
  <rdfs:comment xml:lang="en">The subject of the subject RDF statement.</rdfs:comment>
  <rdfs:domain rdf:resource="&rdf;Statement"/>
  <rdfs:isDefinedBy rdf:resource="&rdf;"/>
  <rdfs:label xml:lang="en">subject</rdfs:label>
  <rdfs:range rdf:resource="&rdfs;Resource"/>
</rdf:Property>

<rdf:Property rdf:about="&nfo;codec"
    rdfs:comment="The name of the codec necessary to decode a piece of media."
    rdfs:label="codec">
  <rdfs:domain rdf:resource="&nfo;Media"/>
  <rdfs:range rdf:resource="&rdfs;Literal"/>
</rdf:Property>

<owl:Class rdf:about="&oa;List">
  <rdfs:comment xml:lang="en">A multiplicity construct that conveys to a consuming application that all of the constituent resources are required for the Annotation to be correctly interpreted, and in a particular order. 

oa:List can be used as the object of the object of the oa:hasBody, oa:hasTarget, oa:hasSelector, oa:hasState, oa:styledBy and oa:hasScope relationships, 

There MUST be 2 or more oa:item relationships for each oa:List, with their order defined using the rdf:List construct of rdf:first/rdf:rest/rdf:nil.

All the elements of the list should also be declared using oa:item, and each of the oa:items should appear at least once in the list.</rdfs:comment>
  <rdfs:isDefinedBy rdf:resource="&oa;"/>
  <rdfs:label xml:lang="en">List</rdfs:label>
  <rdfs:subClassOf rdf:resource="&oa;Composite"/>
</owl:Class>

<rdf:Property rdf:about="&tmo;actualStartTime"
    nrl:maxCardinality="1"
    rdfs:label="actualStartTime">
  <rdfs:subPropertyOf rdf:resource="&tmo;actualTime"/>
  <rdfs:subPropertyOf rdf:resource="&tmo;startTime"/>
  <rdfs:domain rdf:resource="&tmo;Task"/>
  <rdfs:range rdf:resource="&xsd;dateTime"/>
</rdf:Property>

<rdf:Property rdf:about="&nfo;frameRate"
    rdfs:comment="Amount of video frames per second."
    rdfs:label="frameRate">
  <nrl:maxCardinality rdf:datatype="&xsd;integer">1</nrl:maxCardinality>
  <rdfs:domain rdf:resource="&nfo;Video"/>
  <rdfs:range rdf:resource="&xsd;float"/>
  <rdfs:subPropertyOf rdf:resource="&nfo;rate"/>
</rdf:Property>

<rdf:Property rdf:about="&rdf;object">
  <rdfs:comment xml:lang="en">The object of the subject RDF statement.</rdfs:comment>
  <rdfs:domain rdf:resource="&rdf;Statement"/>
  <rdfs:isDefinedBy rdf:resource="&rdf;"/>
  <rdfs:label xml:lang="en">object</rdfs:label>
  <rdfs:range rdf:resource="&rdfs;Resource"/>
</rdf:Property>

<rdfs:Class rdf:about="&nfo;SoftwareService"
    rdfs:label="SoftwareService">
  <rdfs:comment>A service published by a piece of software, either by an operating system or an application. Examples of such services may include calendar, addressbook and mailbox managed by a PIM application. This category is introduced to distinguish between data available directly from the applications (Via some Interprocess Communication Mechanisms) and data available from files on a disk. In either case both DataObjects would receive a similar interpretation (e.g. a Mailbox) and wouldn't differ on the content level.</rdfs:comment>
  <rdfs:subClassOf rdf:resource="&nie;DataObject"/>
</rdfs:Class>

<rdf:Property rdf:about="&nexif;focalPlaneXResolution"
    rdfs:label="focalPlaneXResolution">
  <rdfs:subPropertyOf rdf:resource="http://www.kanzaki.com/ns/exif#focalPlaneXResolution"/>
  <rdfs:subPropertyOf rdf:resource="&nexif;pictTaking"/>
  <rdfs:subPropertyOf rdf:resource="&nexif;resolution"/>
  <rdfs:comment>The number of pixels in the image width (X) direction per FocalPlaneResolutionUnit on the camera focal plane.
tagNumber: 41486</rdfs:comment>
  <rdfs:domain rdf:resource="&nexif;Photo"/>
  <rdfs:range rdf:resource="&xsd;float"/>
</rdf:Property>

<rdf:Property rdf:about="&nfo;encoding"
    rdfs:label="encoding">
  <nrl:maxCardinality rdf:datatype="&xsd;integer">1</nrl:maxCardinality>
  <rdfs:comment>The encoding used for the Embedded File. Examples might include BASE64 or UUEncode</rdfs:comment>
  <rdfs:domain rdf:resource="&nfo;EmbeddedFileDataObject"/>
  <rdfs:range rdf:resource="&xsd;string"/>
</rdf:Property>

<ncal:RecurrenceFrequency rdf:about="&ncal;daily"
    rdfs:label="daily"/>

<rdf:Property rdf:about="&dcterms;accrualPolicy">
  <dcterms:hasVersion rdf:resource="http://dublincore.org/usage/terms/history/#accrualPolicy-003"/>
  <dcterms:issued rdf:datatype="&xsd;date">2005-06-13</dcterms:issued>
  <dcterms:modified rdf:datatype="&xsd;date">2010-10-11</dcterms:modified>
  <rdfs:comment xml:lang="en">The policy governing the addition of items to a collection.</rdfs:comment>
  <rdfs:domain rdf:resource="&dctypes;Collection"/>
  <rdfs:isDefinedBy rdf:resource="&dcterms;"/>
  <rdfs:label xml:lang="en">Accrual Policy</rdfs:label>
  <rdfs:range rdf:resource="&dcterms;Policy"/>
</rdf:Property>

<rdf:Property rdf:about="&pimo;duration"
    nrl:maxCardinality="1"
    rdfs:label="duration">
  <rdfs:comment>The duration of the process (meeting, event, etc). Difference between start and end time.</rdfs:comment>
  <rdfs:domain rdf:resource="&pimo;ProcessConcept"/>
  <rdfs:range rdf:resource="&xsd;duration"/>
  <rdfs:subPropertyOf rdf:resource="&pimo;datatypeProperty"/>
</rdf:Property>

<ncal:AccessClassification rdf:about="&ncal;publicClassification"
    rdfs:label="publicClassification"/>

<rdf:Property rdf:about="&dpo;minTemperature"
    rdfs:label="Minimum Temperature">
  <rdfs:comment>A subproperty of dpo:minValue that defines a lowerbound on the observed temperature value (in degrees celcius) such that it can classify as a dpo:Temperature or dpo:WeatherCondition instance. It can be used in conjunction with dpo:maxTemperature, i.e. specific instances of the former two classes have a pre-defined range of observable real-world temperatures. Since this property has the described dual-domain, the domain is generic. However, it is not meant to be attached to other types of quantifiable component instances.</rdfs:comment>
  <rdfs:domain rdf:resource="&dpo;QuantifiableComponent"/>
  <rdfs:range rdf:resource="&xsd;float"/>
  <rdfs:subPropertyOf rdf:resource="&dpo;minValue"/>
</rdf:Property>

<rdf:Property rdf:about="&foaf;aimChatID"
    rdfs:comment="An AIM chat ID"
    rdfs:label="AIM chat ID"
    ns:term_status="testing">
  <rdf:type rdf:resource="&owl;DatatypeProperty"/>
  <rdf:type rdf:resource="&owl;InverseFunctionalProperty"/>
  <rdfs:domain rdf:resource="&foaf;Agent"/>
  <rdfs:isDefinedBy rdf:resource="&foaf;"/>
  <rdfs:range rdf:resource="&rdfs;Literal"/>
  <rdfs:subPropertyOf rdf:resource="&foaf;nick"/>
</rdf:Property>

<rdf:Property rdf:about="&nexif;gpsMapDatum"
    rdfs:label="gpsMapDatum">
  <rdfs:subPropertyOf rdf:resource="http://www.kanzaki.com/ns/exif#gpsMapDatum"/>
  <rdfs:subPropertyOf rdf:resource="&nexif;gpsInfo"/>
  <rdfs:comment>The geodetic survey data used by the GPS receiver. If the survey data is restricted to Japan, the value of this tag is 'TOKYO' or 'WGS-84'. If a GPS Info tag is recorded, it is strongly recommended that this tag be recorded.
tagNumber: 18</rdfs:comment>
  <rdfs:domain rdf:resource="&nexif;Photo"/>
  <rdfs:range rdf:resource="&xsd;string"/>
</rdf:Property>

<rdf:Property rdf:about="&duho;hasPastDataGraph"
    rdfs:label="has past data graph">
  <nrl:inverseProperty rdf:resource="&nao;isPastDataGraphFor"/>
  <rdfs:comment>Links a resource to the graph which contains its earlier metadata, before a change. Its typical usage would be to refer to a persisted copy of a file's metadata before it is changed. Inverse property of duho:isPastDataGraphFor.</rdfs:comment>
  <rdfs:domain rdf:resource="&rdfs;Resource"/>
  <rdfs:range rdf:resource="&duho;Log"/>
  <rdfs:subPropertyOf rdf:resource="&nao;hasDataGraph"/>
</rdf:Property>

<rdf:Property rdf:about="&ncal;cutype"
    rdfs:label="cutype">
  <rdfs:comment>To specify the type of calendar user specified by the property. Inspired by RFC 2445 sec. 4.2.3. This parameter has a limited vocabulary. The terms that may serve as values for this property have been expressed as instances of CalendarUserType class. The user may use instances provided with this ontology or create his own.</rdfs:comment>
  <rdfs:domain rdf:resource="&ncal;Attendee"/>
  <rdfs:range rdf:resource="&ncal;CalendarUserType"/>
</rdf:Property>

<rdf:Property rdf:about="&nco;hasContactMedium"
    rdfs:label="hasContactMedium">
  <rdfs:comment>A superProperty for all properties linking a Contact to an instance of a contact medium.</rdfs:comment>
  <rdfs:domain rdf:resource="&nco;Role"/>
  <rdfs:range rdf:resource="&nco;ContactMedium"/>
</rdf:Property>

<rdf:Property rdf:about="&tmo;taskReference"
    nrl:maxCardinality="1"
    rdfs:label="taskReference">
  <rdfs:domain rdf:resource="&tmo;Task"/>
  <rdfs:range rdf:resource="&tmo;Task"/>
</rdf:Property>

<rdf:Property rdf:about="&nmo;hasAttachment"
    rdfs:comment="Links a message with files that were sent as attachments."
    rdfs:label="hasAttachment">
  <rdfs:domain rdf:resource="&nmo;Message"/>
  <rdfs:range rdf:resource="&nfo;Attachment"/>
  <rdfs:subPropertyOf rdf:resource="&nie;hasPart"/>
</rdf:Property>

<rdf:Property rdf:about="&dcterms;mediator">
  <dcterms:description xml:lang="en">In an educational context, a mediator might be a parent, teacher, teaching assistant, or care-giver.</dcterms:description>
  <dcterms:hasVersion rdf:resource="http://dublincore.org/usage/terms/history/#mediator-003"/>
  <dcterms:issued rdf:datatype="&xsd;date">2001-05-21</dcterms:issued>
  <dcterms:modified rdf:datatype="&xsd;date">2008-01-14</dcterms:modified>
  <rdfs:comment xml:lang="en">An entity that mediates access to the resource and for whom the resource is intended or useful.</rdfs:comment>
  <rdfs:isDefinedBy rdf:resource="&dcterms;"/>
  <rdfs:label xml:lang="en">Mediator</rdfs:label>
  <rdfs:range rdf:resource="&dcterms;AgentClass"/>
  <rdfs:subPropertyOf rdf:resource="&dcterms;audience"/>
</rdf:Property>

<rdf:Property rdf:about="&nexif;stripByteCounts"
    rdfs:label="stripByteCounts">
  <rdfs:subPropertyOf rdf:resource="http://www.kanzaki.com/ns/exif#stripByteCounts"/>
  <rdfs:subPropertyOf rdf:resource="&nexif;recOffset"/>
  <rdfs:comment>tagNumber: 279
The total number of bytes in each strip. With JPEG compressed data this designation is not needed and is omitted.</rdfs:comment>
  <rdfs:domain rdf:resource="&nexif;Photo"/>
  <rdfs:range rdf:resource="&xsd;string"/>
</rdf:Property>

<rdf:Property rdf:about="&dpo;hasPresenceComponent"
    rdfs:label="has Presence Component">
  <rdfs:comment>Defines the owner (pimo:Agent) of the presence component, who is typically also the owner of the PIM instance. In contrast to other presence ontologies, this property is not intended to be used to describe an agent's current presence. The DCON ontology is provided to fulfil this purpose.</rdfs:comment>
  <rdfs:domain rdf:resource="&pimo;Agent"/>
  <rdfs:range rdf:resource="&dpo;PresenceComponent"/>
</rdf:Property>

<rdf:Property rdf:about="&nco;hasIMAccount"
    rdfs:label="hasIMAccount">
  <rdfs:comment>Indicates that an Instant Messaging account owned by an entity represented by this contact.</rdfs:comment>
  <rdfs:domain rdf:resource="&nco;Role"/>
  <rdfs:range rdf:resource="&nco;IMAccount"/>
  <rdfs:subPropertyOf rdf:resource="&nco;hasContactMedium"/>
</rdf:Property>

<rdf:Property rdf:about="&nfo;fileName"
    nrl:maxCardinality="1"
    rdfs:comment="Name of the file, together with the extension"
    rdfs:label="fileName">
  <rdfs:domain rdf:resource="&nfo;FileDataObject"/>
  <rdfs:range rdf:resource="&xsd;string"/>
  <rdfs:subPropertyOf rdf:resource="&nao;prefLabel"/>
</rdf:Property>

<rdf:Property rdf:about="&nco;isAccessedBy"
    rdfs:label="isKnownBy">
  <rdfs:comment>Indicates the local IMAccount by which this IMAccount is accessed. This does not imply membership of a contact list.</rdfs:comment>
  <rdfs:domain rdf:resource="&nco;IMAccount"/>
  <rdfs:range rdf:resource="&nco;IMAccount"/>
</rdf:Property>

<rdf:Property rdf:about="&nfo;definesFunction"
    rdfs:label="definesFunction">
  <rdfs:comment>A name of a function/method defined in the given source code file.</rdfs:comment>
  <rdfs:domain rdf:resource="&nfo;SourceCode"/>
  <rdfs:range rdf:resource="&xsd;string"/>
</rdf:Property>

<nrl:InverseFunctionalProperty rdf:about="&pimo;groundingOccurrence"
    rdfs:label="grounding occurrence">
  <rdf:type rdf:resource="&rdf;Property"/>
  <rdfs:comment>The subject Thing represents the entity that is described in the object InformationElement. The subject Thing is the canonical, unique representation in the personal information model for the entity described in the object. Multiple InformationElements can be the grounding occurrence of the same Thing,  one InformationElement can be the groundingOccurrence of only one Thing.</rdfs:comment>
  <rdfs:domain rdf:resource="&pimo;Thing"/>
  <rdfs:range rdf:resource="&nie;InformationElement"/>
  <rdfs:subPropertyOf rdf:resource="&pimo;occurrence"/>
</nrl:InverseFunctionalProperty>

<rdf:Property rdf:about="&dpo;maxDayOfMonth"
    rdfs:label="Maximum Day of the Month">
  <rdfs:comment>A subproperty of dpo:maxValue that defines an upperbound on the observed day of the month (i.e., between 1 and 31) such that it can classify as a dpo:TimePeriod instance. It can be used in conjunction with dpo:minDayOfMonth, i.e. specific instances of dpo:TimePeriod have a pre-defined observable monthly period.</rdfs:comment>
  <rdfs:domain rdf:resource="&dpo;TimePeriod"/>
  <rdfs:range rdf:resource="&xsd;integer"/>
  <rdfs:subPropertyOf rdf:resource="&dpo;maxValue"/>
</rdf:Property>

<rdf:Property rdf:about="&nco;imAccountType"
    nrl:maxCardinality="1"
    rdfs:label="imAccountType">
  <rdfs:comment>Type of the IM account. This may be the name of the service that provides the IM functionality. Examples might include Jabber, ICQ, MSN etc</rdfs:comment>
  <rdfs:domain rdf:resource="&nco;IMAccount"/>
  <rdfs:range rdf:resource="&xsd;string"/>
</rdf:Property>

<rdf:Property rdf:about="&nexif;width"
    rdfs:comment="Width of an object"
    rdfs:label="width">
  <rdfs:subPropertyOf rdf:resource="http://www.kanzaki.com/ns/exif#width"/>
  <rdfs:subPropertyOf rdf:resource="&nexif;length"/>
  <rdfs:domain rdf:resource="&nexif;Photo"/>
  <rdfs:range rdf:resource="&xsd;integer"/>
</rdf:Property>

<rdf:Property rdf:about="&nco;nameFamily"
    nrl:maxCardinality="1"
    rdfs:label="nameFamily">
  <rdfs:comment>The family name of an Object represented by this Contact. These applies to people that have more than one given name. The 'first' one is considered 'the' given name (see nameGiven) property. All additional ones are considered 'additional' names. The name inherited from parents is the 'family name'. e.g. For Dr. John Phil Paul Stevenson Jr. M.D. A.C.P. we have contact with: honorificPrefix: 'Dr.', nameGiven: 'John', nameAdditional: 'Phil', nameAdditional: 'Paul', nameFamily: 'Stevenson', honorificSuffix: 'Jr.', honorificSuffix: 'M.D.', honorificSuffix: 'A.C.P.'. These properties form an equivalent of the compound 'N' property as defined in RFC 2426 Sec. 3.1.2</rdfs:comment>
  <rdfs:domain rdf:resource="&nco;PersonName"/>
  <rdfs:range rdf:resource="&xsd;string"/>
</rdf:Property>

<rdf:Property rdf:about="&ncal;tzoffsetfrom"
    rdfs:label="tzoffsetfrom">
  <nrl:maxCardinality rdf:datatype="&xsd;integer">1</nrl:maxCardinality>
  <rdfs:comment>This property specifies the offset which is in use prior to this time zone observance. Inspired by RFC 2445 sec. 4.8.3.3. The original domain was underspecified. It said that this property must appear within a Timezone component. In this ontology a TimezoneObservance class has been introduced to clarify this specification. The original range was UTC-OFFSET. There is no equivalent among the XSD datatypes so plain string was chosen.</rdfs:comment>
  <rdfs:domain rdf:resource="&ncal;TimezoneObservance"/>
  <rdfs:range rdf:resource="&xsd;string"/>
</rdf:Property>

<tmo:PersonInvolvementRole rdf:about="&tmo;TMO_Instance_PersonInvolvementRole_Reviewer"
    rdfs:label="TMO_Instance_PersonInvolvementRole_Reviewer"/>

<rdf:Property rdf:about="&foaf;status"
    rdfs:label="status"
    ns:term_status="unstable">
  <rdf:type rdf:resource="&owl;DatatypeProperty"/>
  <rdfs:comment>A string expressing what the user is happy for the general public (normally) to know about their current activity.</rdfs:comment>
  <rdfs:domain rdf:resource="&foaf;Agent"/>
  <rdfs:isDefinedBy rdf:resource="&foaf;"/>
  <rdfs:range rdf:resource="&rdfs;Literal"/>
</rdf:Property>

<rdfs:Class rdf:about="&nmm;TVSeason"
    rdfs:comment="A season of a TV Show"
    rdfs:label="tv season">
  <rdfs:subClassOf rdf:resource="&nie;InformationElement"/>
</rdfs:Class>

<rdf:Property rdf:about="&tmo;taskStateChangesTo"
    nrl:maxCardinality="1"
    rdfs:label="taskStateChangesTo">
  <rdfs:domain rdf:resource="&tmo;TaskState"/>
  <rdfs:range rdf:resource="&tmo;TaskState"/>
  <rdfs:subPropertyOf rdf:resource="&tmo;stateTypeRole"/>
</rdf:Property>

<rdf:Property rdf:about="&dcterms;contributor">
  <dcterms:description xml:lang="en">Examples of a Contributor include a person, an organization, or a service.</dcterms:description>
  <dcterms:hasVersion rdf:resource="http://dublincore.org/usage/terms/history/#contributorT-001"/>
  <dcterms:issued rdf:datatype="&xsd;date">2008-01-14</dcterms:issued>
  <dcterms:modified rdf:datatype="&xsd;date">2010-10-11</dcterms:modified>
  <rdfs:comment xml:lang="en">An entity responsible for making contributions to the resource.</rdfs:comment>
  <rdfs:isDefinedBy rdf:resource="&dcterms;"/>
  <rdfs:label xml:lang="en">Contributor</rdfs:label>
  <rdfs:range rdf:resource="&dcterms;Agent"/>
  <rdfs:subPropertyOf rdf:resource="&dc;contributor"/>
</rdf:Property>

<rdf:Property rdf:about="&drmo;and"
    rdfs:label="and">
  <rdfs:comment>Combine TWO condition blocks together with the AND operator. Both conditions have to occur independent of time and order for the actions to trigger.</rdfs:comment>
  <rdfs:domain rdf:resource="&drmo;Condition"/>
  <rdfs:range rdf:resource="&drmo;Condition"/>
</rdf:Property>

<rdf:Property rdf:about="&nao;created"
    rdfs:label="created at">
  <nrl:maxCardinality rdf:datatype="&xsd;nonNegativeInteger">1</nrl:maxCardinality>
  <rdfs:comment>States the creation, or first modification time for a resource</rdfs:comment>
  <rdfs:domain rdf:resource="&rdfs;Resource"/>
  <rdfs:range rdf:resource="&xsd;dateTime"/>
  <rdfs:subPropertyOf rdf:resource="&nao;modified"/>
</rdf:Property>

<rdf:Property rdf:about="&pimo;datatypeProperty"
    rdfs:label="datatype property">
  <rdfs:comment>The object of statements is a literal, resource, or datatype value describing the subject thing. Users should be able to edit statements defined with this property. Abstract super-property.</rdfs:comment>
  <rdfs:domain rdf:resource="&pimo;Thing"/>
</rdf:Property>

<rdf:Property rdf:about="&ncal;delegatedTo"
    rdfs:label="delegatedTo">
  <rdfs:comment>To specify the calendar users to whom the calendar user specified by the property has delegated participation. Inspired by RFC 2445 sec. 4.2.5. Originally the value type for this parameter was CAL-ADDRESS. This has been expressed as nco:Contact to promote integration between NCAL and NCO.</rdfs:comment>
  <rdfs:domain rdf:resource="&ncal;Attendee"/>
  <rdfs:range rdf:resource="&nco;Contact"/>
</rdf:Property>

<rdfs:Class rdf:about="&ncal;FreebusyType"
    rdfs:label="FreebusyType">
  <rdfs:comment>Type of a Freebusy indication. This class has been introduced to serve as a limited set of values for the ncal:fbtype property. See the documentation of ncal:fbtype for details.</rdfs:comment>
  <rdfs:subClassOf rdf:resource="&rdfs;Resource"/>
</rdfs:Class>

<rdfs:Class rdf:about="&pimo;Project"
    rdfs:label="Project">
  <rdfs:comment>Any piece of work that is undertaken or attempted (Wordnet). An enterprise carefully planned to achieve a particular aim (Oxford Dictionary).</rdfs:comment>
  <rdfs:subClassOf rdf:resource="&pimo;ProcessConcept"/>
</rdfs:Class>

<rdf:Property rdf:about="&foaf;accountServiceHomepage"
    rdfs:label="account service homepage"
    ns:term_status="testing">
  <rdf:type rdf:resource="&owl;ObjectProperty"/>
  <rdfs:comment>Indicates a homepage of the service provide for this online account.</rdfs:comment>
  <rdfs:domain rdf:resource="&foaf;OnlineAccount"/>
  <rdfs:isDefinedBy rdf:resource="&foaf;"/>
  <rdfs:range rdf:resource="&foaf;Document"/>
</rdf:Property>

<rdfs:Class rdf:about="&ddo;Network"
    rdfs:label="Network">
  <rdfs:comment>A telecommunications network, connecting a collection of terminals, links and nodes which connect together to enable telecommunication between terminal users. Includes wired and wireless computer networks and cellular networks.</rdfs:comment>
</rdfs:Class>

<ncal:TriggerRelation rdf:about="&ncal;startTriggerRelation"
    rdfs:label="startTriggerRelation"/>

<rdf:Property rdf:about="&scos;historyNote">
  <rdf:type rdf:resource="&owl;AnnotationProperty"/>
  <rdfs:isDefinedBy rdf:resource="http://www.w3.org/2004/02/skos/core"/>
  <rdfs:label xml:lang="en">history note</rdfs:label>
  <rdfs:subPropertyOf rdf:resource="&scos;note"/>
  <scos:definition xml:lang="en">A note about the past state/use/meaning of a concept.</scos:definition>
</rdf:Property>

<owl:ObjectProperty rdf:about="&oa;hasSelector">
  <rdfs:comment xml:lang="en">The relationship between a oa:SpecificResource and a oa:Selector.

There MUST be exactly 0 or 1 oa:hasSelector relationship associated with a 
Specific Resource. 

If multiple Selectors are required, either to express a choice between different optional, equivalent selectors, or a chain of selectors that should all be processed, it is necessary to use oa:Choice, oa:Composite or oa:List as a selector.</rdfs:comment>
  <rdfs:domain rdf:resource="&oa;SpecificResource"/>
  <rdfs:isDefinedBy rdf:resource="&oa;"/>
  <rdfs:label xml:lang="en">hasSelector</rdfs:label>
  <rdfs:range rdf:resource="&oa;Selector"/>
</owl:ObjectProperty>

<rdf:Property rdf:about="&nrl;updatable"
    rdfs:label="updatable">
  <nrl:maxCardinality rdf:datatype="&xsd;nonNegativeInteger">1</nrl:maxCardinality>
  <rdfs:comment>A core graph metadata property, this defines whether a graph can be freely updated '1' or otherwise '0'</rdfs:comment>
  <rdfs:domain rdf:resource="&nrl;Graph"/>
  <rdfs:range rdf:resource="&xsd;boolean"/>
</rdf:Property>

<rdfs:Class rdf:about="&dctypes;InteractiveResource">
  <dcam:memberOf rdf:resource="&dcterms;DCMIType"/>
  <dcterms:description xml:lang="en">Examples include forms on Web pages, applets, multimedia learning objects, chat services, or virtual reality environments.</dcterms:description>
  <dcterms:hasVersion rdf:resource="http://dublincore.org/usage/terms/history/#InteractiveResource-003"/>
  <dcterms:issued rdf:datatype="&xsd;date">2000-07-11</dcterms:issued>
  <dcterms:modified rdf:datatype="&xsd;date">2008-01-14</dcterms:modified>
  <rdfs:comment xml:lang="en">A resource requiring interaction from the user to be understood, executed, or experienced.</rdfs:comment>
  <rdfs:isDefinedBy rdf:resource="&dctypes;"/>
  <rdfs:label xml:lang="en">Interactive Resource</rdfs:label>
</rdfs:Class>

<rdfs:Class rdf:about="&nco;DomesticDeliveryAddress"
    rdfs:label="DomesticDeliveryAddress">
  <rdfs:comment>Domestic Delivery Addresse. Class inspired by TYPE=dom parameter of the ADR property defined in RFC 2426 sec. 3.2.1</rdfs:comment>
  <rdfs:subClassOf rdf:resource="&nco;PostalAddress"/>
</rdfs:Class>

<rdf:Property rdf:about="&nfo;fileUrl"
    rdfs:label="fileUrl">
  <nao:deprecated rdf:datatype="&xsd;boolean">true</nao:deprecated>
  <rdfs:comment>URL of the file. It points at the location of the file. In cases where creating a simple file:// or http:// URL for a file is difficult (e.g. for files inside compressed archives) the applications are encouraged to use conventions defined by Apache Commons VFS Project at http://jakarta.apache.org/  commons/ vfs/ filesystems.html.</rdfs:comment>
  <rdfs:domain rdf:resource="&nfo;FileDataObject"/>
  <rdfs:range rdf:resource="&rdfs;Resource"/>
  <rdfs:subPropertyOf rdf:resource="&nie;url"/>
</rdf:Property>

<rdf:Property rdf:about="&nexif;gpsSatellites"
    rdfs:label="gpsSatellites">
  <rdfs:subPropertyOf rdf:resource="http://www.kanzaki.com/ns/exif#gpsSatellites"/>
  <rdfs:subPropertyOf rdf:resource="&nexif;gpsInfo"/>
  <rdfs:comment>tagNumber: 8
The GPS satellites used for measurements. This tag can be used to describe the number of satellites, their ID number, angle of elevation, azimuth, SNR and other information in ASCII notation. The format is not specified. If the GPS receiver is incapable of taking measurements, value of the tag shall be set to NULL.</rdfs:comment>
  <rdfs:domain rdf:resource="&nexif;Photo"/>
  <rdfs:range rdf:resource="&xsd;string"/>
</rdf:Property>

<rdfs:Class rdf:about="&pimo;City"
    rdfs:label="City">
  <rdfs:comment>A large and densely populated urban area; may include several independent administrative districts; "Ancient Troy was a great city". (Definition from SUMO)</rdfs:comment>
  <rdfs:subClassOf rdf:resource="&pimo;Location"/>
</rdfs:Class>

<rdfs:Class rdf:about="&nco;PostalAddress"
    rdfs:label="PostalAddress">
  <rdfs:comment>A postal address. A class aggregating the various parts of a value for the 'ADR' property as defined in RFC 2426 Sec. 3.2.1.</rdfs:comment>
  <rdfs:subClassOf rdf:resource="&nco;ContactMedium"/>
</rdfs:Class>

<rdf:Property rdf:about="&tmo;dependencyMemberA"
    nrl:maxCardinality="1"
    nrl:minCardinality="1"
    rdfs:label="dependencyMemberA">
  <rdfs:subPropertyOf rdf:resource="&pimo;associationMember"/>
  <rdfs:subPropertyOf rdf:resource="&tmo;taskReference"/>
  <rdfs:comment>The semantic of this relation is defined in the sublclass of undirected Dependency on which this property is stated. (The subject of the statment where this property is expressed)</rdfs:comment>
  <rdfs:domain rdf:resource="&tmo;TaskDependency"/>
  <rdfs:range rdf:resource="&tmo;Task"/>
</rdf:Property>

<rdf:Property rdf:about="&nrl;hasSpecification"
    rdfs:label="hasSpecification">
  <rdfs:comment>Points to the representation of the view specification required to generate the graph view in question</rdfs:comment>
  <rdfs:domain rdf:resource="&nrl;GraphView"/>
  <rdfs:range rdf:resource="&nrl;ViewSpecification"/>
</rdf:Property>

<rdf:Property rdf:about="&cnt;characterEncoding">
  <rdf:type rdf:resource="&owl;ObjectProperty"/>
  <rdfs:comment xml:lang="en">The character encoding used to create a character sequence from a byte sequence or vice versa.</rdfs:comment>
  <rdfs:domain rdf:resource="&cnt;Content"/>
  <rdfs:label xml:lang="en">Character encoding</rdfs:label>
  <rdfs:range rdf:resource="&rdfs;Literal"/>
</rdf:Property>

<pimo:ClassRole rdf:about="&pimo;ConcreteClass"
    rdfs:label="ConcreteClass"/>

<rdfs:Class rdf:about="&nfo;Cursor"
    rdfs:comment="A Cursor."
    rdfs:label="Cursor">
  <rdfs:subClassOf rdf:resource="&nfo;RasterImage"/>
</rdfs:Class>

<rdf:Property rdf:about="&nfo;rate"
    rdfs:label="rate">
  <rdfs:comment>A common superproperty for all properties specifying the media rate. Examples of subproperties may include frameRate for video and sampleRate for audio. This property is expressed in units per second.</rdfs:comment>
  <rdfs:domain rdf:resource="&nfo;Media"/>
  <rdfs:range rdf:resource="&xsd;float"/>
</rdf:Property>

<rdfs:Class rdf:about="&nfo;Bookmark"
    rdfs:label="Bookmark">
  <rdfs:comment>A bookmark of a webbrowser. Use nie:title for the name/label, nie:contentCreated to represent the date when the user added the bookmark, and nie:contentLastModified for modifications. nfo:bookmarks to store the link.</rdfs:comment>
  <rdfs:subClassOf rdf:resource="&nie;InformationElement"/>
</rdfs:Class>

<rdfs:Class rdf:about="&dcterms;MediaTypeOrExtent">
  <dcterms:hasVersion rdf:resource="http://dublincore.org/usage/terms/history/#MediaTypeOrExtent-001"/>
  <dcterms:issued rdf:datatype="&xsd;date">2008-01-14</dcterms:issued>
  <rdfs:comment xml:lang="en">A media type or extent.</rdfs:comment>
  <rdfs:isDefinedBy rdf:resource="&dcterms;"/>
  <rdfs:label xml:lang="en">Media Type or Extent</rdfs:label>
</rdfs:Class>

<rdfs:Class rdf:about="&nfo;Spreadsheet"
    rdfs:label="Spreadsheet">
  <rdfs:comment>A spreadsheet, created by a spreadsheet application. Examples might include Gnumeric, OpenOffice Calc or MS Excel.</rdfs:comment>
  <rdfs:subClassOf rdf:resource="&nfo;Document"/>
</rdfs:Class>

<tmo:TaskContainer rdf:about="&tmo;TMO_Instance_TaskContainer_outbox"
    rdfs:label="TMO_Instance_TaskContainer_outbox"/>

<nrl:RuleViewSpecification rdf:about="&pimo;RuleViewSpecificationOccurrenceClosure"
    rdfs:label="RuleViewSpecificationOccurrenceClosure"/>

<rdf:Property rdf:about="&nao;privacyLevel"
    rdfs:label="privacy level">
  <rdfs:comment>A privacy level as defined for a resource. Allowed values range from 0 (private) to 1 (public).</rdfs:comment>
  <rdfs:domain rdf:resource="&rdfs;Resource"/>
  <rdfs:range rdf:resource="&xsd;double"/>
  <rdfs:subPropertyOf rdf:resource="&nao;annotation"/>
</rdf:Property>

<rdfs:Class rdf:about="&nrl;InverseFunctionalProperty"
    rdfs:comment="A marker class to identify inverse functional properties"
    rdfs:label="InverseFunctionalProperty">
  <rdfs:subClassOf rdf:resource="&rdfs;Resource"/>
</rdfs:Class>

<rdfs:Class rdf:about="&dpo;Brightness"
    rdfs:label="Brightness">
  <rdfs:comment>Quantifiable presence components concerning the brightness levels in the environment surrounding the agent.</rdfs:comment>
  <rdfs:subClassOf rdf:resource="&dpo;EnvironmentalIndicator"/>
</rdfs:Class>

<rdf:Property rdf:about="&nfo;characterCount"
    rdfs:comment="The amount of characters in the document."
    rdfs:label="characterCount">
  <nrl:maxCardinality rdf:datatype="&xsd;integer">1</nrl:maxCardinality>
  <rdfs:domain rdf:resource="&nfo;TextDocument"/>
  <rdfs:range rdf:resource="&xsd;integer"/>
</rdf:Property>

<nrl:TransitiveProperty rdf:about="&pimo;hasOtherSlot"
    rdfs:label="represented by other slot">
  <rdfs:range rdf:resource="&rdf;Property"/>
  <rdfs:range rdf:resource="&rdfs;Resource"/>
  <rdf:type rdf:resource="&rdf;Property"/>
  <rdfs:comment>hasOtherSlot points from a clot  in your PIMO to a slot in a domain ontology that represents the same connection idea.</rdfs:comment>
  <rdfs:domain rdf:resource="&rdf;Property"/>
  <rdfs:subPropertyOf rdf:resource="&rdfs;subPropertyOf"/>
</nrl:TransitiveProperty>

<owl:ObjectProperty rdf:about="&oa;serializedBy">
  <rdfs:comment xml:lang="en">The object of the relationship is the agent, likely software, responsible for generating the serialization of the Annotation's serialization. 

It is RECOMMENDED to use these and other FOAF terms to describe agents: foaf:Person, prov:SoftwareAgent, foaf:Organization, foaf:name, foaf:mbox, foaf:openid, foaf:homepage

There MAY be 0 or more oa:serializedBy relationships per Annotation.</rdfs:comment>
  <rdfs:domain rdf:resource="&oa;Annotation"/>
  <rdfs:isDefinedBy rdf:resource="&oa;"/>
  <rdfs:label xml:lang="en">serializedBy</rdfs:label>
  <rdfs:subPropertyOf rdf:resource="&prov;wasAttributedTo"/>
</owl:ObjectProperty>

<rdf:Property rdf:about="&nexif;mm"
    rdfs:comment="A length with unit of mm"
    rdfs:label="mm">
  <rdfs:subPropertyOf rdf:resource="http://www.kanzaki.com/ns/exif#mm"/>
  <rdfs:subPropertyOf rdf:resource="&nexif;length"/>
  <rdfs:domain rdf:resource="&nexif;Photo"/>
  <rdfs:range rdf:resource="&xsd;string"/>
</rdf:Property>

<rdfs:Class rdf:about="&drmo;Condition"
    rdfs:label="Condition">
  <rdfs:comment>Defines condition blocks for rules on which queries and logic tests are performed. Each condition can have constraints (also instances of drmo:Condition) recursively. Multiple conditions in a rule are combined together using a number of logical and event operators. This class can be extended to allow the representation of condition templates, specific to the system's needs.</rdfs:comment>
</rdfs:Class>

<rdfs:Class rdf:about="&ncal;CalendarScale"
    rdfs:label="CalendarScale">
  <rdfs:comment>A calendar scale. This class has been introduced to provide the limited vocabulary for the ncal:calscale property.</rdfs:comment>
  <rdfs:subClassOf rdf:resource="&rdfs;Resource"/>
</rdfs:Class>

<rdfs:Class rdf:about="&pimo;Topic"
    rdfs:label="Topic">
  <rdfs:subClassOf rdf:resource="&pimo;Tag"/>
  <rdfs:subClassOf rdf:resource="&pimo;Thing"/>
  <rdfs:comment>A topic is the subject of a discussion or document. Topics are distinguished from Things in their taxonomic nature, examples are scientific areas such as "Information Science", "Biology", or categories used in content syndication such as "Sports", "Politics". They are specific to the user's domain.</rdfs:comment>
</rdfs:Class>

<rdf:Property rdf:about="&foaf;isPrimaryTopicOf"
    rdfs:comment="A document that this thing is the primary topic of."
    rdfs:label="is primary topic of"
    ns:term_status="stable">
  <rdf:type rdf:resource="&owl;InverseFunctionalProperty"/>
  <rdfs:domain rdf:resource="&owl;Thing"/>
  <rdfs:isDefinedBy rdf:resource="&foaf;"/>
  <rdfs:range rdf:resource="&foaf;Document"/>
  <rdfs:subPropertyOf rdf:resource="&foaf;page"/>
  <owl:inverseOf rdf:resource="&foaf;primaryTopic"/>
</rdf:Property>

<rdfs:Class rdf:about="&ncal;RecurrenceIdentifierRange"
    rdfs:label="RecurrenceIdentifierRange">
  <rdfs:comment>Recurrence Identifier Range. This class has been created to provide means to express the limited set of values for the ncal:range property. See documentation for ncal:range for details.</rdfs:comment>
  <rdfs:subClassOf rdf:resource="&rdfs;Resource"/>
</rdfs:Class>

<rdf:Property rdf:about="&ncal;eventStatus"
    rdfs:label="status">
  <nrl:maxCardinality rdf:datatype="&xsd;integer">1</nrl:maxCardinality>
  <rdfs:comment>Defines the overall status or confirmation for an Event. Based on the STATUS property defined in RFC 2445 sec. 4.8.1.11.</rdfs:comment>
  <rdfs:domain rdf:resource="&ncal;Event"/>
  <rdfs:range rdf:resource="&ncal;EventStatus"/>
</rdf:Property>

<rdfs:Class rdf:about="&pimo;ClassOrThing"
    protege:role="abstract"
    rdfs:label="ClassOrThing">
  <pimo:classRole rdf:resource="&pimo;AbstractClass"/>
  <rdfs:comment>Superclass of class and thing. To add properties to both class and thing.</rdfs:comment>
  <rdfs:subClassOf rdf:resource="&pimo;ClassOrThingOrPropertyOrAssociation"/>
</rdfs:Class>

<rdf:Property rdf:about="&dcon;fogfactor"
    rdfs:label="Fog Factor Value">
  <rdfs:comment>Registers an actual fog factor value element attribute to an active weather condition in the current context.</rdfs:comment>
  <rdfs:domain rdf:resource="&dpo;WeatherConditions"/>
  <rdfs:range rdf:resource="&xsd;nonNegativeInteger"/>
  <rdfs:subPropertyOf rdf:resource="&dcon;hasContextAttribute"/>
</rdf:Property>

<rdf:Property rdf:about="&tmo;transmissionFrom"
    nrl:maxCardinality="1"
    nrl:minCardinality="1"
    rdfs:label="transmissionFrom">
  <rdfs:domain rdf:resource="&tmo;TaskTransmission"/>
  <rdfs:range rdf:resource="&pimo;Person"/>
</rdf:Property>

<rdfs:Class rdf:about="&nrl;AsymmetricProperty"
    rdfs:comment="A marker class to identify asymmetric properties"
    rdfs:label="AsymmetricProperty">
  <rdfs:subClassOf rdf:resource="&rdfs;Resource"/>
</rdfs:Class>

<rdfs:Class rdf:about="&ncal;UnionOfAlarmEventJournalTodo"
    rdfs:label="UnionOfAlarmEventJournalTodo">
  <rdfs:subClassOf rdf:resource="&ncal;UnionParentClass"/>
</rdfs:Class>

<rdf:Property rdf:about="&nfo;verticalResolution"
    rdfs:label="verticalResolution">
  <nrl:maxCardinality rdf:datatype="&xsd;integer">1</nrl:maxCardinality>
  <rdfs:comment>Vertical resolution of an Image (if printed). Expressed in DPI</rdfs:comment>
  <rdfs:domain rdf:resource="&nfo;Image"/>
  <rdfs:range rdf:resource="&xsd;integer"/>
</rdf:Property>

<rdf:Property rdf:about="&dplo;textualContent"
    rdfs:label="Textual Content">
  <nrl:maxCardinality rdf:datatype="&xsd;nonNegativeInteger">1</nrl:maxCardinality>
  <rdfs:comment>The textual content of a Livepost, as it appears an online stream.</rdfs:comment>
  <rdfs:domain rdf:resource="&dplo;LivePost"/>
  <rdfs:range rdf:resource="&xsd;string"/>
</rdf:Property>

<rdf:Property rdf:about="&nmo;messageSender"
    rdfs:label="sender">
  <nrl:maxCardinality rdf:datatype="&xsd;integer">1</nrl:maxCardinality>
  <rdfs:comment>The person or agent submitting the message to the network, if other from the one given with the nmo:from property. Defined in RFC 822 sec. 4.4.2</rdfs:comment>
  <rdfs:domain rdf:resource="&nmo;Message"/>
  <rdfs:range rdf:resource="&nco;ContactMedium"/>
  <rdfs:subPropertyOf rdf:resource="&nmo;messageRecipient"/>
</rdf:Property>

<tmo:AttachmentRole rdf:about="&tmo;TMO_Instance_AttachmentRole_Related"
    rdfs:label="TMO_Instance_AttachmentRole_Related"/>

<rdf:Property rdf:about="&nmm;trackPeakGain"
    rdfs:comment="ReplayGain track peak gain"
    rdfs:label="track peak gain">
  <nrl:maxCardinality rdf:datatype="&xsd;integer">1</nrl:maxCardinality>
  <rdfs:domain rdf:resource="&nmm;MusicPiece"/>
  <rdfs:range rdf:resource="&xsd;float"/>
</rdf:Property>

<rdfs:Class rdf:about="&tmo;AttachmentRole"
    rdfs:label="AttachmentRole">
  <rdfs:comment>AttachmentRoles further specify the type of how an attachment relates to a task. Example instances  of AttachmentRoles are e.g. "desired_request", "required" and "used".</rdfs:comment>
  <rdfs:subClassOf rdf:resource="&tmo;StateTypeRole"/>
</rdfs:Class>

<rdfs:Class rdf:about="&ncal;Calendar"
    rdfs:label="Calendar">
  <rdfs:comment>A calendar. Inspirations for this class can be traced to the VCALENDAR component defined in RFC 2445 sec. 4.4, but it may just as well be used to represent any kind of Calendar.</rdfs:comment>
  <rdfs:subClassOf rdf:resource="&nie;InformationElement"/>
</rdfs:Class>

<rdfs:Class rdf:about="&nuao;DesktopEvent"
    rdfs:label="desktop event">
  <rdfs:comment>A desktop event: activity performed by an user. A "hook" class that should be extended by other ontologies such as desktop service ontology to specify which application or service was involved in the desktop event.</rdfs:comment>
  <rdfs:subClassOf rdf:resource="&nuao;Event"/>
</rdfs:Class>

<rdf:Property rdf:about="&dcterms;publisher">
  <dcterms:description xml:lang="en">Examples of a Publisher include a person, an organization, or a service.</dcterms:description>
  <dcterms:hasVersion rdf:resource="http://dublincore.org/usage/terms/history/#publisherT-001"/>
  <dcterms:issued rdf:datatype="&xsd;date">2008-01-14</dcterms:issued>
  <dcterms:modified rdf:datatype="&xsd;date">2010-10-11</dcterms:modified>
  <rdfs:comment xml:lang="en">An entity responsible for making the resource available.</rdfs:comment>
  <rdfs:isDefinedBy rdf:resource="&dcterms;"/>
  <rdfs:label xml:lang="en">Publisher</rdfs:label>
  <rdfs:range rdf:resource="&dcterms;Agent"/>
  <rdfs:subPropertyOf rdf:resource="&dc;publisher"/>
</rdf:Property>

<rdf:Property rdf:about="&dcterms;accessRights">
  <rdfs:subPropertyOf rdf:resource="&dc;rights"/>
  <rdfs:subPropertyOf rdf:resource="&dcterms;rights"/>
  <dcterms:description xml:lang="en">Access Rights may include information regarding access or restrictions based on privacy, security, or other policies.</dcterms:description>
  <dcterms:hasVersion rdf:resource="http://dublincore.org/usage/terms/history/#accessRights-002"/>
  <dcterms:issued rdf:datatype="&xsd;date">2003-02-15</dcterms:issued>
  <dcterms:modified rdf:datatype="&xsd;date">2008-01-14</dcterms:modified>
  <rdfs:comment xml:lang="en">Information about who can access the resource or an indication of its security status.</rdfs:comment>
  <rdfs:isDefinedBy rdf:resource="&dcterms;"/>
  <rdfs:label xml:lang="en">Access Rights</rdfs:label>
  <rdfs:range rdf:resource="&dcterms;RightsStatement"/>
</rdf:Property>

<rdf:Property rdf:about="&dpo;maxNoiseLevel"
    rdfs:label="Maximum Noise Level">
  <rdfs:comment>A subproperty of dpo:maxValue that defines an upperbound on the observed loudness level value (in decibels) such that it can classify as a dpo:Noise instance. It can be used in conjunction with dpo:minNoiseLevel, i.e. specific instances of dpo:Noise have a pre-defined range of observable real-world surrounding noise levels.</rdfs:comment>
  <rdfs:domain rdf:resource="&dpo;Noise"/>
  <rdfs:range rdf:resource="&xsd;float"/>
  <rdfs:subPropertyOf rdf:resource="&dpo;maxValue"/>
</rdf:Property>

<tmo:Importance rdf:about="&tmo;TMO_Instance_Importance_09"
    rdfs:label="TMO_Instance_Importance_09"/>

<rdfs:Class rdf:about="&dpo;QuantifiableComponent"
    rdfs:label="Quantifiable Component">
  <rdfs:comment>A presence component that can be quantified. In this case, discrete user context properties obtained from sensors can be mapped to their loosely-defined fuzzy counterparts. Thus for example, the actual and dynamic temperature of an agent's environment can be mapped to an existing category that is saved as an instance of a presence component. Each of these categories has a number of attributes that define its valid actual data range, e.g., a presence component representing 'hot' weather conditions around an agent will be enabled (i.e., it becomes part of the agent's presence) only if the actual sensed temperature lies within the ranges defined by the value limits. As most quantifiable presence components posses this restrictions, tree generic properties are applicable: dpo:value, dpo:minValue, dpo:maxValue.</rdfs:comment>
  <rdfs:subClassOf rdf:resource="&dpo;PresenceComponent"/>
</rdfs:Class>

<owl:Class rdf:about="&oa;Style">
  <rdfs:comment xml:lang="en">A resource which describes the style in which the selection or resource should be rendered, indicated with oa:styledBy from an oa:Annotation.

This class is not used directly in Annotations, only its subclasses are.

The content of the resource provides the rendering hints about the Annotation's constituent resources. 

The Specifier's description MAY be conveyed as an external or embedded resource (cnt:Content), or as RDF properties within the graph. The description SHOULD use existing standards whenever possible. If the Specifier has an HTTP URI, then its description, and only its description, MUST be returned when the URI is dereferenced.</rdfs:comment>
  <rdfs:isDefinedBy rdf:resource="&oa;"/>
  <rdfs:label xml:lang="en">Style</rdfs:label>
</owl:Class>

<rdf:Property rdf:about="&dcon;absoluteAltitude"
    rdfs:label="Absolute Altitude Value">
  <rdfs:comment>States the current absolute altitude (metres above ground level)</rdfs:comment>
  <rdfs:domain rdf:resource="&dpo;Altitude"/>
  <rdfs:range rdf:resource="&xsd;float"/>
  <rdfs:subPropertyOf rdf:resource="&dcon;hasContextAttribute"/>
</rdf:Property>

<rdf:Property rdf:about="&dcon;minutes"
    rdfs:label="Hours and Minutes elapsed">
  <rdfs:comment>Derived from the dateTime, this property stores the exact amount of minutes elapsed since the start of the current day. Implicitly also stores the number of elapsed hours. Thus, a value of 0 means that the current day has just started whereas a value of 1439 indicates the end of a day.</rdfs:comment>
  <rdfs:domain rdf:resource="&dpo;TimePeriod"/>
  <rdfs:range rdf:resource="&xsd;nonNegativeInteger"/>
  <rdfs:subPropertyOf rdf:resource="&dcon;hasContextAttribute"/>
</rdf:Property>

<rdf:Property rdf:about="&nie;isStoredAs"
    rdfs:label="isStoredAs">
  <nrl:inverseProperty rdf:resource="&nie;interpretedAs"/>
  <rdfs:comment>Links the information element with the DataObject it is stored in.</rdfs:comment>
  <rdfs:domain rdf:resource="&nie;InformationElement"/>
  <rdfs:range rdf:resource="&nie;DataObject"/>
</rdf:Property>

<rdfs:Datatype rdf:about="&dcterms;Period">
  <dcterms:hasVersion rdf:resource="http://dublincore.org/usage/terms/history/#Period-003"/>
  <dcterms:issued rdf:datatype="&xsd;date">2000-07-11</dcterms:issued>
  <dcterms:modified rdf:datatype="&xsd;date">2008-01-14</dcterms:modified>
  <rdfs:comment xml:lang="en">The set of time intervals defined by their limits according to the DCMI Period Encoding Scheme.</rdfs:comment>
  <rdfs:isDefinedBy rdf:resource="&dcterms;"/>
  <rdfs:label xml:lang="en">DCMI Period</rdfs:label>
  <rdfs:seeAlso rdf:resource="http://dublincore.org/documents/dcmi-period/"/>
</rdfs:Datatype>

<rdfs:Class rdf:about="&foaf;LabelProperty"
    rdfs:label="Label Property"
    ns:term_status="unstable">
  <rdf:type rdf:resource="&owl;Class"/>
  <rdfs:comment>A foaf:LabelProperty is any RDF property with texual values that serve as labels.</rdfs:comment>
  <rdfs:isDefinedBy rdf:resource="&foaf;"/>
</rdfs:Class>

<rdf:Property rdf:about="&tmo;startTime"
    nrl:maxCardinality="1"
    rdfs:label="startTime">
  <rdfs:range rdf:resource="&xsd;dateTime"/>
  <rdfs:subPropertyOf rdf:resource="&tmo;dateTime"/>
</rdf:Property>

<rdfs:Class rdf:about="&dcterms;Location">
  <dcterms:hasVersion rdf:resource="http://dublincore.org/usage/terms/history/#Location-001"/>
  <dcterms:issued rdf:datatype="&xsd;date">2008-01-14</dcterms:issued>
  <rdfs:comment xml:lang="en">A spatial region or named place.</rdfs:comment>
  <rdfs:isDefinedBy rdf:resource="&dcterms;"/>
  <rdfs:label xml:lang="en">Location</rdfs:label>
  <rdfs:subClassOf rdf:resource="&dcterms;LocationPeriodOrJurisdiction"/>
</rdfs:Class>

<rdf:Property rdf:about="&dcon;windscale"
    rdfs:label="Wind Scale Value">
  <rdfs:comment>Registers an actual wind scale value element attribute to an active weather condition in the current context.</rdfs:comment>
  <rdfs:domain rdf:resource="&dpo;WeatherConditions"/>
  <rdfs:range rdf:resource="&xsd;nonNegativeInteger"/>
  <rdfs:subPropertyOf rdf:resource="&dcon;hasContextAttribute"/>
</rdf:Property>

<rdf:Property rdf:about="&pimo;partOf"
    rdfs:label="part of">
  <nrl:inverseProperty rdf:resource="&pimo;hasPart"/>
  <rdfs:comment>This is part of the object. Like a page is part of a book or an engine is part of a car. You can make sub-properties of this to reflect more detailed relations.</rdfs:comment>
  <rdfs:domain rdf:resource="&pimo;Thing"/>
  <rdfs:range rdf:resource="&pimo;Thing"/>
  <rdfs:subPropertyOf rdf:resource="&pimo;objectProperty"/>
</rdf:Property>

<rdfs:Class rdf:about="&pimo;Task"
    rdfs:label="Task">
  <rdfs:comment>A (usually assigned) piece of work (often to be finished within a certain time). (Definition from Merriam-Webster)</rdfs:comment>
  <rdfs:subClassOf rdf:resource="&pimo;ProcessConcept"/>
</rdfs:Class>

<rdf:Property rdf:about="&nco;org"
    nrl:maxCardinality="1"
    rdfs:label="org">
  <rdfs:comment>Name of an organization or a unit within an organization the object represented by a Contact is associated with. An equivalent of the 'ORG' property defined in RFC 2426 Sec. 3.5.5</rdfs:comment>
  <rdfs:domain rdf:resource="&nco;Affiliation"/>
  <rdfs:range rdf:resource="&nco;OrganizationContact"/>
</rdf:Property>

<nco:IMStatusType rdf:about="&nco;IMStatusTypeExtendedAway"
    rdfs:label="extended away"/>

<rdf:Property rdf:about="&nie;subject"
    rdfs:comment="An overall topic of the content of a InformationElement"
    rdfs:label="subject">
  <rdfs:domain rdf:resource="&nie;InformationElement"/>
  <rdfs:range rdf:resource="&xsd;string"/>
  <rdfs:subPropertyOf rdf:resource="&dc;subject"/>
</rdf:Property>

<owl:Class rdf:about="&oa;TimeState">
  <rdfs:comment xml:lang="en">A resource which describes how to retrieve a representation of the Source resource that is temporally appropriate for the Annotation.

There MUST be at least one of oa:cachedSource or oa:when specified. If there is more than 1, each gives an alternative copy of the representation.</rdfs:comment>
  <rdfs:isDefinedBy rdf:resource="&oa;"/>
  <rdfs:label xml:lang="en">TimeState</rdfs:label>
  <rdfs:subClassOf rdf:resource="&oa;State"/>
</owl:Class>

<rdf:Property rdf:about="&nmo;secondaryRecipient"
    rdfs:comment="deprecated in favor of nmo:secondaryMessageRecipient"
    rdfs:label="secondaryRecipient">
  <nao:deprecated rdf:datatype="&xsd;boolean">true</nao:deprecated>
  <rdfs:domain rdf:resource="&nmo;Message"/>
  <rdfs:range rdf:resource="&nco;Contact"/>
  <rdfs:subPropertyOf rdf:resource="&nmo;recipient"/>
</rdf:Property>

<nco:IMStatusType rdf:about="&nco;IMStatusTypeBusy"
    rdfs:label="busy"/>

<rdfs:Class rdf:about="&nfo;RasterImage"
    rdfs:comment="A raster image."
    rdfs:label="RasterImage">
  <rdfs:subClassOf rdf:resource="&nfo;Image"/>
</rdfs:Class>

<rdf:Property rdf:about="&nso;sharedOn"
    rdfs:label="shared on">
  <rdfs:comment>Records the time and date of when a resource was shared. Effectively, this could also coincide with the creation time of a local copy of the shared resource. This does not conflict with the original resource and content creation times, as defined by nao:created, nao:modified, nao:lastMofied and the subproperties nie:created, nie:modified, nie:lastModified, nie:contentCreated,nie:contentModified and nie:contentLastModified.</rdfs:comment>
  <rdfs:domain rdf:resource="&rdfs;Resource"/>
  <rdfs:range rdf:resource="&xsd;dateTime"/>
</rdf:Property>

<rdfs:Class rdf:about="&nmo;Email"
    rdfs:comment="An email."
    rdfs:label="Email">
  <rdfs:subClassOf rdf:resource="&nmo;Message"/>
</rdfs:Class>

<rdf:Property rdf:about="&foaf;sha1"
    rdfs:comment="A sha1sum hash, in hex."
    rdfs:label="sha1sum (hex)"
    ns:term_status="unstable">
  <rdf:type rdf:resource="&owl;DatatypeProperty"/>
  <rdfs:domain rdf:resource="&foaf;Document"/>
  <rdfs:isDefinedBy rdf:resource="&foaf;"/>
</rdf:Property>

<rdf:Property rdf:about="&nie;interpretedAs"
    rdfs:label="interpretedAs">
  <nrl:inverseProperty rdf:resource="&nie;isStoredAs"/>
  <rdfs:comment>Links the DataObject with the InformationElement it is interpreted as.</rdfs:comment>
  <rdfs:domain rdf:resource="&nie;DataObject"/>
  <rdfs:range rdf:resource="&nie;InformationElement"/>
</rdf:Property>

<rdf:Property rdf:about="&dpo;maxSnowfallDegree"
    rdfs:label="Maximum Snowfall Degree">
  <rdfs:comment>A subproperty of dpo:maxValue that defines an upperbound on the observed snowfall (in millimetres per hour) such that it can classify as a dpo:WeatherCondition instance. It can be used in conjunction with dpo:minSnowfallDegree to state that specific instances of dpo:WeatherCondition have a pre-defined range of observable real-world snowfall levels. In addition, they can also be used with various other weather conditions values and ranges to define complex weather condition types.</rdfs:comment>
  <rdfs:domain rdf:resource="&dpo;WeatherConditions"/>
  <rdfs:range rdf:resource="&xsd;nonNegativeInteger"/>
  <rdfs:subPropertyOf rdf:resource="&dpo;maxValue"/>
</rdf:Property>

<rdf:Property rdf:about="&nfo;commentCharacterCount"
    rdfs:label="commentCharacterCount">
  <nrl:maxCardinality rdf:datatype="&xsd;integer">1</nrl:maxCardinality>
  <rdfs:comment>The amount of character in comments i.e. characters ignored by the compiler/interpreter.</rdfs:comment>
  <rdfs:domain rdf:resource="&nfo;SourceCode"/>
  <rdfs:range rdf:resource="&xsd;integer"/>
</rdf:Property>

<rdf:Property rdf:about="&nco;nameAdditional"
    rdfs:label="nameAdditional">
  <rdfs:comment>Additional given name of an object represented by this contact. See documentation for 'nameFamily' property for details.</rdfs:comment>
  <rdfs:domain rdf:resource="&nco;PersonName"/>
  <rdfs:range rdf:resource="&xsd;string"/>
</rdf:Property>

<rdf:Property rdf:about="&pimo;locatedWithin"
    rdfs:label="located within">
  <nrl:inverseProperty rdf:resource="&pimo;containsLocation"/>
  <rdfs:comment>The subject location is contained within the object location. For example, a room is located within a building or a city is located within a country.</rdfs:comment>
  <rdfs:domain rdf:resource="&pimo;Location"/>
  <rdfs:range rdf:resource="&pimo;Location"/>
  <rdfs:subPropertyOf rdf:resource="&pimo;partOf"/>
</rdf:Property>

<tmo:TaskContainer rdf:about="&tmo;TMO_Instance_TaskContainer_inbox"
    rdfs:label="TMO_Instance_TaskContainer_inbox"/>

<rdf:Property rdf:about="&nexif;imageUniqueID"
    rdfs:label="imageUniqueID">
  <rdfs:subPropertyOf rdf:resource="&dc;identifier"/>
  <rdfs:subPropertyOf rdf:resource="http://www.kanzaki.com/ns/exif#imageUniqueID"/>
  <rdfs:subPropertyOf rdf:resource="&nie;identifier"/>
  <rdfs:subPropertyOf rdf:resource="&nexif;exifAttribute"/>
  <rdfs:comment>An identifier assigned uniquely to each image. It is recorded as an ASCII string equivalent to hexadecimal notation and 128-bit fixed length.
tagNumber: 42016</rdfs:comment>
  <rdfs:domain rdf:resource="&nexif;Photo"/>
  <rdfs:range rdf:resource="&xsd;string"/>
</rdf:Property>

<rdf:Property rdf:about="&nexif;recOffset"
    rdfs:comment="An attribute relating to recording offset"
    rdfs:label="recOffset">
  <rdfs:subPropertyOf rdf:resource="http://www.kanzaki.com/ns/exif#recOffset"/>
  <rdfs:subPropertyOf rdf:resource="&nexif;exifAttribute"/>
  <rdfs:domain rdf:resource="&nexif;Photo"/>
  <rdfs:range rdf:resource="&xsd;integer"/>
</rdf:Property>

<rdf:Property rdf:about="&tmo;actualEndTime"
    nrl:maxCardinality="1"
    rdfs:label="actualEndTime">
  <rdfs:subPropertyOf rdf:resource="&tmo;actualTime"/>
  <rdfs:subPropertyOf rdf:resource="&tmo;endTime"/>
  <rdfs:domain rdf:resource="&tmo;Task"/>
  <rdfs:range rdf:resource="&xsd;dateTime"/>
</rdf:Property>

<rdf:Property rdf:about="&ncal;encoding"
    rdfs:label="encoding">
  <nrl:maxCardinality rdf:datatype="&xsd;integer">1</nrl:maxCardinality>
  <rdfs:comment>To specify an alternate inline encoding for the property value. Inspired by RFC 2445 sec. 4.2.7. Originally this property had a limited vocabulary. ('8BIT' and 'BASE64'). The terms of this vocabulary have been expressed as instances of the AttachmentEncoding class</rdfs:comment>
  <rdfs:domain rdf:resource="&ncal;Attachment"/>
  <rdfs:range rdf:resource="&ncal;AttachmentEncoding"/>
</rdf:Property>

<rdf:Property rdf:about="&nexif;date"
    rdfs:label="date">
  <rdfs:subPropertyOf rdf:resource="&dc;date"/>
  <rdfs:subPropertyOf rdf:resource="http://www.kanzaki.com/ns/exif#date"/>
  <rdfs:comment>a date information. Usually saved as YYYY:MM:DD (HH:MM:SS) format in Exif data, but represented here as W3C-DTF format</rdfs:comment>
  <rdfs:domain rdf:resource="&nexif;Photo"/>
  <rdfs:range rdf:resource="&xsd;dateTime"/>
</rdf:Property>

<tmo:PersonInvolvementRole rdf:about="&tmo;TMO_Instance_PersonInvolvementRole_Executor"
    rdfs:label="TMO_Instance_PersonInvolvementRole_Executor"/>

<tmo:TaskState rdf:about="&tmo;TMO_Instance_TaskState_Deleted"
    rdfs:label="TMO_Instance_TaskState_Deleted"/>

<rdf:Property rdf:about="&ncal;rsvp"
    rdfs:label="rsvp">
  <nrl:maxCardinality rdf:datatype="&xsd;integer">1</nrl:maxCardinality>
  <rdfs:comment>To specify whether there is an expectation of a favor of a reply from the calendar user specified by the property value. Inspired by RFC 2445 sec. 4.2.17</rdfs:comment>
  <rdfs:domain rdf:resource="&ncal;Attendee"/>
  <rdfs:range rdf:resource="&xsd;boolean"/>
</rdf:Property>

<rdfs:Class rdf:about="&rdfs;Resource">
  <rdfs:comment xml:lang="en">The class resource, everything.</rdfs:comment>
  <rdfs:isDefinedBy rdf:resource="&rdfs;"/>
  <rdfs:label xml:lang="en">Resource</rdfs:label>
</rdfs:Class>

<rdf:Property rdf:about="&rdfs;subPropertyOf">
  <rdfs:comment xml:lang="en">The subject is a subproperty of a property.</rdfs:comment>
  <rdfs:domain rdf:resource="&rdf;Property"/>
  <rdfs:isDefinedBy rdf:resource="&rdfs;"/>
  <rdfs:label xml:lang="en">subPropertyOf</rdfs:label>
  <rdfs:range rdf:resource="&rdf;Property"/>
</rdf:Property>

<rdf:Property rdf:about="&nexif;sceneCaptureType"
    rdfs:label="sceneCaptureType">
  <rdfs:subPropertyOf rdf:resource="http://www.kanzaki.com/ns/exif#sceneCaptureType"/>
  <rdfs:subPropertyOf rdf:resource="&nexif;pictTaking"/>
  <rdfs:comment>tagNumber: 41990
The type of scene that was shot. It can also be used to record the mode in which the image was shot, such as Landscape, Portrait etc. Note that this differs from the scene type (SceneType) tag.</rdfs:comment>
  <rdfs:domain rdf:resource="&nexif;Photo"/>
  <rdfs:range rdf:resource="&xsd;string"/>
</rdf:Property>

<rdf:Property rdf:about="&dpo;maxValue"
    rdfs:label="Maximum Value">
  <rdfs:comment>A subproperty of dpo:value defining an upperbound on the value observed for a real-world entity for it to classify as an instance of a specific quantifiable presence component. Various subproperties are provided and apply to specific types of presence components.</rdfs:comment>
  <rdfs:domain rdf:resource="&dpo;QuantifiableComponent"/>
  <rdfs:subPropertyOf rdf:resource="&dpo;value"/>
</rdf:Property>

<rdf:Property rdf:about="&nie;contentCreated"
    nrl:maxCardinality="1"
    rdfs:label="contentCreated">
  <rdfs:subPropertyOf rdf:resource="&nie;contentModified"/>
  <rdfs:subPropertyOf rdf:resource="&nie;informationElementDate"/>
  <rdfs:subPropertyOf rdf:resource="&nao;created"/>
  <rdfs:comment>The date of the content creation. This may not necessarily be equal to the date when the DataObject (i.e. the physical representation) itself was created. Compare with nie:created property.</rdfs:comment>
  <rdfs:domain rdf:resource="&nie;InformationElement"/>
  <rdfs:range rdf:resource="&xsd;dateTime"/>
</rdf:Property>

<rdfs:Class rdf:about="&dcon;Attention"
    rdfs:label="Attention">
  <rdfs:comment>The attention aspect covers context elements relating to the users' activities on their digital devices.</rdfs:comment>
  <rdfs:subClassOf rdf:resource="&dcon;Aspect"/>
</rdfs:Class>

<rdf:Property rdf:about="&nexif;exposureBiasValue"
    rdfs:label="exposureBiasValue">
  <rdfs:subPropertyOf rdf:resource="http://www.kanzaki.com/ns/exif#exposureBiasValue"/>
  <rdfs:subPropertyOf rdf:resource="&nexif;pictTaking"/>
  <rdfs:comment>tagNumber: 37380
The exposure bias. The unit is the APEX value. Ordinarily it is given in the range of -99.99 to 99.99.</rdfs:comment>
  <rdfs:domain rdf:resource="&nexif;Photo"/>
  <rdfs:range rdf:resource="&xsd;float"/>
</rdf:Property>

<rdf:Property rdf:about="&foaf;title"
    rdfs:comment="Title (Mr, Mrs, Ms, Dr. etc)"
    rdfs:label="title"
    ns:term_status="testing">
  <rdf:type rdf:resource="&owl;DatatypeProperty"/>
  <rdfs:isDefinedBy rdf:resource="&foaf;"/>
</rdf:Property>

<rdf:Property rdf:about="&ncal;requestStatusData"
    rdfs:label="requestStatusData">
  <rdfs:comment>Additional data associated with a request status. Inspired by the third part of the structured value for the REQUEST-STATUS property defined in RFC 2445 sec. 4.8.8.2 ("Textual exception data. For example, the offending property name and value or complete property line")</rdfs:comment>
  <rdfs:domain rdf:resource="&ncal;RequestStatus"/>
  <rdfs:range rdf:resource="&xsd;string"/>
</rdf:Property>

<rdfs:Class rdf:about="&nco;FaxNumber"
    rdfs:label="FaxNumber">
  <rdfs:comment>A fax number. Inspired by the (TYPE=fax) parameter of the TEL property as defined in RFC 2426 sec  3.3.1.</rdfs:comment>
  <rdfs:subClassOf rdf:resource="&nco;PhoneNumber"/>
</rdfs:Class>

<rdf:Property rdf:about="&nco;region"
    rdfs:label="region">
  <nrl:maxCardinality rdf:datatype="&xsd;integer">1</nrl:maxCardinality>
  <rdfs:comment>Region. Inspired by the fifth part of the value of the 'ADR' property as defined in RFC 2426, sec. 3.2.1</rdfs:comment>
  <rdfs:domain rdf:resource="&nco;PostalAddress"/>
  <rdfs:range rdf:resource="&xsd;string"/>
</rdf:Property>

<owl:NamedIndividual rdf:about="&oa;identifying">
  <rdf:type rdf:resource="&oa;Motivation"/>
  <rdfs:comment xml:lang="en">The motivation that represents the assignment of an identity to the target resource(s). For example, annotating the name of a city in a string of text with the URI that identifies it.</rdfs:comment>
  <scos:inScheme rdf:resource="&oa;motivationScheme"/>
  <scos:prefLabel xml:lang="en">identifying</scos:prefLabel>
</owl:NamedIndividual>

<ncal:Weekday rdf:about="&ncal;wednesday"
    rdfs:label="wednesday"/>

<rdf:Property rdf:about="&tmo;delegability"
    nrl:maxCardinality="1"
    rdfs:label="delegability">
  <rdfs:domain rdf:resource="&tmo;Task"/>
  <rdfs:range rdf:resource="&tmo;Delegability"/>
  <rdfs:subPropertyOf rdf:resource="&tmo;timemanagement"/>
</rdf:Property>

<rdf:Property rdf:about="&nid3;originalAlbumTitle"
    rdfs:label="originalAlbumTitle">
  <rdfs:comment>TOAL
The 'Original album/movie/show title' frame is intended for the title of the original recording (or source of sound), if for example the music in the file should be a cover of a previously released song.</rdfs:comment>
  <rdfs:domain rdf:resource="&nid3;ID3Audio"/>
  <rdfs:range rdf:resource="&xsd;string"/>
</rdf:Property>

<rdfs:Class rdf:about="&dao;Account"
    rdfs:label="Account">
  <rdfs:subClassOf rdf:resource="http://rdfs.org/sioc/ns#Container"/>
  <rdfs:subClassOf rdf:resource="&nie;DataSource"/>
  <rdfs:subClassOf rdf:resource="&pimo;Agent"/>
  <rdfs:comment>A person account, hosted in a local application or in a remote service, typically associated with a set of 		
credentials and containing identity-related as well as other forms of personal user information. Subclass of nie:DataSource, as a source of personal information.</rdfs:comment>
</rdfs:Class>

<rdf:Property rdf:about="&ncal;attach"
    rdfs:label="attach">
  <rdfs:comment>The property provides the capability to associate a document object with a calendar component. Defined in the RFC 2445 sec. 4.8.1.1</rdfs:comment>
  <rdfs:domain rdf:resource="&ncal;UnionOfAlarmEventJournalTodo"/>
  <rdfs:range rdf:resource="&ncal;Attachment"/>
  <rdfs:subPropertyOf rdf:resource="&nie;hasPart"/>
</rdf:Property>

<tmo:TaskState rdf:about="&tmo;TMO_Instance_TaskState_New"
    rdfs:label="TMO_Instance_TaskState_New"/>

<rdf:Property rdf:about="&nco;hasLocation"
    nrl:maxCardinality="1"
    rdfs:label="hasLocation">
  <rdfs:comment>Geographical location of the contact. Inspired by the 'GEO' property specified in RFC 2426 Sec. 3.4.2</rdfs:comment>
  <rdfs:domain rdf:resource="&nco;Contact"/>
  <rdfs:range rdf:resource="http://www.w3.org/2003/01/geo/wgs84_pos#Point"/>
</rdf:Property>

<rdfs:Class rdf:about="&foaf;Project"
    rdfs:comment="A project (a collective endeavour of some kind)."
    rdfs:label="Project"
    ns:term_status="testing">
  <owl:disjointWith rdf:resource="&foaf;Document"/>
  <owl:disjointWith rdf:resource="&foaf;Person"/>
  <rdf:type rdf:resource="&owl;Class"/>
  <rdfs:isDefinedBy rdf:resource="&foaf;"/>
</rdfs:Class>

<ncal:TriggerRelation rdf:about="&ncal;endTriggerRelation"
    rdfs:label="endTriggerRelation"/>

<rdf:Property rdf:about="&tmo;lastReviewDate"
    nrl:maxCardinality="1"
    rdfs:label="lastReviewDate">
  <rdfs:domain rdf:resource="&tmo;Task"/>
  <rdfs:range rdf:resource="&xsd;dateTime"/>
  <rdfs:subPropertyOf rdf:resource="&tmo;dateTime"/>
</rdf:Property>

<rdf:Property rdf:about="&nso;sharedBy"
    rdfs:label="shared by">
  <rdfs:comment>This property establishes a provenance relationship between a resource(pimo:Thing or nie:InformationElement) and the pimo:Agent (individual, or group) through which it was acquired.</rdfs:comment>
  <rdfs:domain rdf:resource="&rdfs;Resource"/>
  <rdfs:range rdf:resource="&pimo;Agent"/>
</rdf:Property>

<rdfs:Class rdf:about="&tmo;Delegability"
    rdfs:label="Delegability">
  <rdfs:subClassOf rdf:resource="&tmo;StateTypeRole"/>
</rdfs:Class>

<rdf:Property rdf:about="&nso;sharedWithContact"
    rdfs:label="shared with contact">
  <rdfs:comment>The subject resource is shared with the object contact. 
The resource and its subresources are transferred to the receiver.
An existing sharedWithContact relation implies that updates on the resource should be transferred to the contact. 
The contact may ask for updates actively, then the sharing party's software should send a new copy of the shared resource to the contact.
Domain should be either a nie:InformationElement or a pimo:Thing but no DataObject. This includes ncal:Event instances and other resources we find on a desktop.
DataObjects are the specific binary stream where an Information Element is stored, and can't be shared because the recipient will form a new binary stream to store the data object. 
As there is no superclass of both nie:InformationElement and pimo:Thing, the domain is rdfs:Resource. 
One resource can be shared to multiple contacts, the cardinality is 0..n. </rdfs:comment>
  <rdfs:domain rdf:resource="&rdfs;Resource"/>
  <rdfs:range rdf:resource="&nco;Contact"/>
  <rdfs:subPropertyOf rdf:resource="&nso;sharedWith"/>
</rdf:Property>

<rdf:Property rdf:about="&nid3;contentType"
    rdfs:label="contentType">
  <rdfs:comment>TCON

The 'Content type', which previously was stored as a one byte numeric value only, is now a numeric string. You may use one or several of the types as ID3v1.1 did or, since the category list would be impossible to maintain with accurate and up to date categories, define your own. 

References to the ID3v1 genres can be made by, as first byte, enter "(" followed by a number from the genres list (appendix A) and ended with a ")" character. This is optionally followed by a refinement, e.g. "(21)" or "(4)Eurodisco". Several references can be made in the same frame, e.g. "(51)(39)". If the refinement should begin with a "(" character it should be replaced with "((", e.g. "((I can figure out any genre)" or "(55)((I think...)". The following new content types is defined in ID3v2 and is implemented in the same way as the numerig content types, e.g. "(RX)". 
RX    Remix 
CR    Cover</rdfs:comment>
  <rdfs:domain rdf:resource="&nid3;ID3Audio"/>
  <rdfs:range rdf:resource="&xsd;string"/>
</rdf:Property>

<rdf:Property rdf:about="&cnt;internalSubset">
  <rdf:type rdf:resource="&owl;ObjectProperty"/>
  <rdfs:comment xml:lang="en">The internal document type definition subset within the document type declarations.</rdfs:comment>
  <rdfs:domain rdf:resource="&cnt;DoctypeDecl"/>
  <rdfs:label xml:lang="en">Internal DTD subset</rdfs:label>
  <rdfs:range rdf:resource="&rdfs;Literal"/>
</rdf:Property>

<rdf:Property rdf:about="&nco;age"
    rdfs:comment="Indicates the age of a person contact."
    rdfs:label="age">
  <nrl:MaxCardinality rdf:datatype="&xsd;integer">1</nrl:MaxCardinality>
  <rdfs:domain rdf:resource="&nco;BirthDate"/>
  <rdfs:range rdf:resource="&xsd;nonNegativeInteger"/>
</rdf:Property>

<rdfs:Class rdf:about="&ncal;Timezone"
    rdfs:label="Timezone">
  <rdfs:subClassOf rdf:resource="&nie;InformationElement"/>
  <rdfs:subClassOf rdf:resource="&ncal;UnionOfEventJournalTimezoneTodo"/>
  <rdfs:subClassOf rdf:resource="&ncal;UnionOfTimezoneObservanceEventFreebusyJournalTimezoneTodo"/>
  <rdfs:subClassOf rdf:resource="&ncal;UnionOfTimezoneObservanceEventFreebusyTimezoneTodo"/>
  <rdfs:subClassOf rdf:resource="&ncal;UnionOfTimezoneObservanceEventJournalTimezoneTodo"/>
  <rdfs:comment>Provide a grouping of component properties that defines a time zone.</rdfs:comment>
</rdfs:Class>

<rdf:Property rdf:about="&nie;lastRefreshed"
    nrl:maxCardinality="1"
    rdfs:label="lastRefreshed">
  <rdfs:comment>Date when information about this data object was retrieved (for the first time) or last refreshed from the data source. This property is important for metadata extraction applications that don't receive any notifications of changes in the data source and have to poll it regularly. This may lead to information becoming out of date. In these cases this property may be used to determine the age of data, which is an important element of it's dependability. </rdfs:comment>
  <rdfs:domain rdf:resource="&nie;DataObject"/>
  <rdfs:range rdf:resource="&xsd;dateTime"/>
  <rdfs:subPropertyOf rdf:resource="&dc;date"/>
</rdf:Property>

<tmo:Urgency rdf:about="&tmo;TMO_Instance_Urgency_06"
    rdfs:label="TMO_Instance_Urgency_06"/>

<rdf:Property rdf:about="http://www.w3.org/2003/01/geo/wgs84_pos#lat"
    nrl:maxCardinality="1">
  <rdfs:range rdf:resource="&xsd;float"/>
  <rdfs:subPropertyOf rdf:resource="&pimo;datatypeProperty"/>
</rdf:Property>

<rdf:Property rdf:about="&nexif;relatedImageLength"
    rdfs:comment="Related image length
tagNumber: 4098"
    rdfs:label="relatedImageLength">
  <rdfs:subPropertyOf rdf:resource="http://www.kanzaki.com/ns/exif#relatedImageLength"/>
  <rdfs:subPropertyOf rdf:resource="&nexif;height"/>
  <rdfs:subPropertyOf rdf:resource="&nexif;interopInfo"/>
  <rdfs:domain rdf:resource="&nexif;Photo"/>
  <rdfs:range rdf:resource="&xsd;integer"/>
</rdf:Property>

<owl:Class rdf:about="http://www.w3.org/2003/01/geo/wgs84_pos#SpatialThing"
    rdfs:label="Spatial Thing"/>

<rdf:Property rdf:about="&nexif;imageDataCharacter"
    rdfs:comment="An attribute relating to image data characteristics"
    rdfs:label="imageDataCharacter">
  <rdfs:subPropertyOf rdf:resource="http://www.kanzaki.com/ns/exif#imageDataCharacter"/>
  <rdfs:subPropertyOf rdf:resource="&nexif;exifAttribute"/>
  <rdfs:domain rdf:resource="&nexif;Photo"/>
  <rdfs:range rdf:resource="&xsd;string"/>
</rdf:Property>

<ncal:CalendarUserType rdf:about="&ncal;groupUserType"
    rdfs:label="groupUserType"/>

<rdf:Property rdf:about="&nuao;duration"
    rdfs:comment="Duration of the event. Deprecated in favor of nuao:end."
    rdfs:label="duration">
  <nao:deprecated rdf:datatype="&xsd;boolean">true</nao:deprecated>
  <nrl:maxCardinality rdf:datatype="&xsd;nonNegativeInteger">1</nrl:maxCardinality>
  <rdfs:domain rdf:resource="&nuao;Event"/>
  <rdfs:range rdf:resource="&xsd;duration"/>
</rdf:Property>

<rdf:Property rdf:about="&ndo;referrer"
    rdfs:label="referrer">
  <rdfs:comment>Points to the Information Element that contained the link to the download source which was used in the download event.</rdfs:comment>
  <rdfs:domain rdf:resource="&ndo;DownloadEvent"/>
  <rdfs:range rdf:resource="&nie;InformationElement"/>
</rdf:Property>

<tmo:Priority rdf:about="&tmo;TMO_Instance_Priority_High"
    rdfs:label="TMO_Instance_Priority_High"/>

<rdf:Property rdf:about="&ncal;action"
    rdfs:label="action">
  <rdfs:comment>This property defines the action to be invoked when an alarm is triggered. Inspired by RFC 2445 sec 4.8.6.1. Originally this property had a limited set of values. They are expressed as instances of the AlarmAction class.</rdfs:comment>
  <rdfs:domain rdf:resource="&ncal;Alarm"/>
  <rdfs:range rdf:resource="&ncal;AlarmAction"/>
</rdf:Property>

<rdfs:Class rdf:about="&nco;Gender"
    rdfs:label="Gender">
  <rdfs:comment>Gender. Instances of this class may include male and female.</rdfs:comment>
  <rdfs:subClassOf rdf:resource="&rdfs;Resource"/>
</rdfs:Class>

<rdf:Property rdf:about="&nexif;gpsLongitudeRef"
    rdfs:label="gpsLongitudeRef">
  <rdfs:subPropertyOf rdf:resource="http://www.kanzaki.com/ns/exif#gpsLongitudeRef"/>
  <rdfs:subPropertyOf rdf:resource="&nexif;gpsInfo"/>
  <rdfs:comment>tagNumber: 3
Indicates whether the longitude is east or west longitude. ASCII 'E' indicates east longitude, and 'W' is west longitude.</rdfs:comment>
  <rdfs:domain rdf:resource="&nexif;Photo"/>
  <rdfs:range rdf:resource="&xsd;string"/>
</rdf:Property>

<rdf:Property rdf:about="&nie;contentModified"
    rdfs:label="modified">
  <rdfs:comment>The date of a modification of the original content (not its corresponding DataObject or local copy). Compare with nie:modified.</rdfs:comment>
  <rdfs:domain rdf:resource="&nie;InformationElement"/>
  <rdfs:range rdf:resource="&xsd;dateTime"/>
</rdf:Property>

<rdfs:Class rdf:about="&dcon;Peers"
    rdfs:label="Peers">
  <rdfs:comment>The peers aspect covers context elements relating to individuals or groups surrounding the user.</rdfs:comment>
  <rdfs:subClassOf rdf:resource="&dcon;Aspect"/>
</rdfs:Class>

<rdf:Property rdf:about="&nco;hasName"
    rdfs:comment="Attaches name information to a contact."
    rdfs:label="hasName">
  <nrl:MaxCardinality rdf:datatype="&xsd;integer">1</nrl:MaxCardinality>
  <rdfs:domain rdf:resource="&nco;Contact"/>
  <rdfs:range rdf:resource="&nco;Name"/>
</rdf:Property>

<rdf:Property rdf:about="&ncal;exrule"
    rdfs:label="exrule">
  <rdfs:comment>This property defines a rule or repeating pattern for an exception to a recurrence set. Inspired by RFC 2445 sec. 4.8.5.2.</rdfs:comment>
  <rdfs:domain rdf:resource="&ncal;UnionOfEventJournalTodo"/>
  <rdfs:range rdf:resource="&ncal;RecurrenceRule"/>
</rdf:Property>

<rdfs:Class rdf:about="&tmo;Skill"
    rdfs:comment="examples are e.g. technologies like Java, XML,  ..."
    rdfs:label="Skill">
  <rdfs:subClassOf rdf:resource="&tmo;AbilityCarrier"/>
</rdfs:Class>

<rdfs:Class rdf:about="&nfo;HardDiskPartition"
    rdfs:comment="A partition on a hard disk"
    rdfs:label="HardDiskPartition">
  <rdfs:subClassOf rdf:resource="&nie;DataObject"/>
</rdfs:Class>

<rdf:Property rdf:about="&dcon;nearbyEvent"
    rdfs:label="Nearby Event">
  <rdfs:comment>Refers to nearby events that characterise a context instance.</rdfs:comment>
  <rdfs:domain rdf:resource="&dcon;SpaTem"/>
  <rdfs:range rdf:resource="&ncal;Event"/>
  <rdfs:subPropertyOf rdf:resource="&dcon;hasContextElement"/>
</rdf:Property>

<rdf:Property rdf:about="&nao;altLabel"
    rdfs:label="alternative label">
  <rdfs:comment>An alternative label alongside the preferred label for a resource</rdfs:comment>
  <rdfs:range rdf:resource="&rdfs;Literal"/>
  <rdfs:subPropertyOf rdf:resource="&rdfs;label"/>
</rdf:Property>

<rdf:Property rdf:about="&pimo;groundingForDeletedThing"
    rdfs:label="grounding for deleted thing">
  <rdfs:comment>This NIE Information Element was used as a grounding occurrence for the object Thing. The Thing was then deleted by the user manually, indicating that this Information Element should not cause an automatic creation of another Thing in the future. The object resource has no range to indicate that it was completely removed from the user's PIMO, including the rdf:type statement. Relevant for data alignment and enrichment algorithms.</rdfs:comment>
  <rdfs:range rdf:resource="&rdfs;Resource"/>
</rdf:Property>

<rdf:Property rdf:about="&nuao;involves"
    rdfs:label="involves">
  <rdfs:comment>Relates an event to the resources that are involved in the event.</rdfs:comment>
  <rdfs:domain rdf:resource="&nuao;Event"/>
  <rdfs:range rdf:resource="&rdfs;Resource"/>
</rdf:Property>

<tmo:AbilityCarrierRole rdf:about="&tmo;TMO_Instance_AbilityCarrierRole_Required"
    rdfs:label="TMO_Instance_AbilityCarrierRole_Required"/>

<rdfs:Class rdf:about="&nid3;SynchronizedText"
    rdfs:label="SynchronizedText">
  <rdfs:comment>SYLT This is another way of incorporating the words, said or sung lyrics, in the audio file as text, this time, however, in sync with the audio. It might also be used to describing events e.g. occurring on a stage or on the screen in sync with the audio. The header includes a content descriptor, represented with as terminated textstring. If no descriptor is entered, 'Content descriptor' is $00 (00) only.</rdfs:comment>
  <rdfs:subClassOf rdf:resource="&rdfs;Resource"/>
</rdfs:Class>

<rdf:Property rdf:about="&dcon;nearbyGroup"
    rdfs:label="Nearby Group">
  <rdfs:comment>Refers to a group of individuals characterising a context instance. Includes both user-defined groups, and ad-hoc groups recognised by the system.</rdfs:comment>
  <rdfs:domain rdf:resource="&dcon;Peers"/>
  <rdfs:range rdf:resource="&pimo;PersonGroup"/>
  <rdfs:subPropertyOf rdf:resource="&dcon;hasContextElement"/>
</rdf:Property>

<rdf:Property rdf:about="&dcon;dayMonth"
    rdfs:label="Day of the Month">
  <rdfs:comment>Derived from the dateTime, this property stores the number of days elapsed for the current month, where 1 indicates the first day of the month, up to a maximum value of 31.</rdfs:comment>
  <rdfs:domain rdf:resource="&dpo;TimePeriod"/>
  <rdfs:range rdf:resource="&xsd;nonNegativeInteger"/>
  <rdfs:subPropertyOf rdf:resource="&dcon;hasContextAttribute"/>
</rdf:Property>

<rdfs:Class rdf:about="&nco;VideoIMAccount"
    rdfs:comment="Deprecated in favour of nco:imCapabilityVideo."
    rdfs:label="VideoIMAccount">
  <nao:deprecated rdf:datatype="&xsd;boolean">true</nao:deprecated>
  <rdfs:subClassOf rdf:resource="&nco;AudioIMAccount"/>
</rdfs:Class>

<tmo:Priority rdf:about="&tmo;TMO_Instance_Priority_Low"
    rdfs:label="TMO_Instance_Priority_Low"/>

<rdf:Property rdf:about="&nmo;recipient"
    rdfs:comment="deprecated in favor of nmo:messageRecipient"
    rdfs:label="recipient">
  <nao:deprecated rdf:datatype="&xsd;boolean">true</nao:deprecated>
  <rdfs:domain rdf:resource="&nmo;Message"/>
  <rdfs:range rdf:resource="&nco;Contact"/>
</rdf:Property>

<rdfs:Class rdf:about="&nmo;MimeEntity"
    rdfs:comment="A MIME entity, as defined in RFC2045, Section 2.4."
    rdfs:label="MimeEntity">
  <rdfs:subClassOf rdf:resource="&nie;InformationElement"/>
</rdfs:Class>

<rdfs:Class rdf:about="&dcterms;ProvenanceStatement">
  <dcterms:hasVersion rdf:resource="http://dublincore.org/usage/terms/history/#ProvenanceStatement-001"/>
  <dcterms:issued rdf:datatype="&xsd;date">2008-01-14</dcterms:issued>
  <rdfs:comment xml:lang="en">A statement of any changes in ownership and custody of a resource since its creation that are significant for its authenticity, integrity, and interpretation.</rdfs:comment>
  <rdfs:isDefinedBy rdf:resource="&dcterms;"/>
  <rdfs:label xml:lang="en">Provenance Statement</rdfs:label>
</rdfs:Class>

<ncal:TimeTransparency rdf:about="&ncal;opaqueTransparency"
    rdfs:label="opaqueTransparency"/>

<owl:Class rdf:about="&scos;OrderedCollection">
  <rdfs:isDefinedBy rdf:resource="http://www.w3.org/2004/02/skos/core"/>
  <rdfs:label xml:lang="en">Ordered Collection</rdfs:label>
  <rdfs:subClassOf rdf:resource="&scos;Collection"/>
  <scos:definition xml:lang="en">An ordered collection of concepts, where both the grouping and the ordering are meaningful.</scos:definition>
  <scos:scopeNote xml:lang="en">Ordered collections can be used where you would like a set of concepts to be displayed in a specific order, and optionally under a 'node label'.</scos:scopeNote>
</owl:Class>

<rdf:Property rdf:about="&nexif;pimInfo"
    rdfs:comment="An attribute relating to print image matching"
    rdfs:label="pimInfo">
  <rdfs:subPropertyOf rdf:resource="http://www.kanzaki.com/ns/exif#pimInfo"/>
  <rdfs:subPropertyOf rdf:resource="&nexif;exifAttribute"/>
  <rdfs:domain rdf:resource="&nexif;Photo"/>
  <rdfs:range rdf:resource="&xsd;string"/>
</rdf:Property>

<rdf:Property rdf:about="&nfo;depiction"
    rdfs:label="depiction">
  <nrl:inverseProperty rdf:resource="&nfo;depicts"/>
  <rdfs:comment>Relates an information element to an image which depicts said element.</rdfs:comment>
  <rdfs:domain rdf:resource="&rdfs;Resource"/>
  <rdfs:range rdf:resource="&nfo;Image"/>
</rdf:Property>

<rdf:Property rdf:about="&nexif;relatedImageWidth"
    rdfs:comment="tagNumber: 4097
Related image width"
    rdfs:label="relatedImageWidth">
  <rdfs:subPropertyOf rdf:resource="http://www.kanzaki.com/ns/exif#relatedImageWidth"/>
  <rdfs:subPropertyOf rdf:resource="&nexif;interopInfo"/>
  <rdfs:subPropertyOf rdf:resource="&nexif;width"/>
  <rdfs:domain rdf:resource="&nexif;Photo"/>
  <rdfs:range rdf:resource="&xsd;string"/>
</rdf:Property>

<rdf:Property rdf:about="&nexif;pictTaking"
    rdfs:comment="An attribute relating to Picture-Taking Conditions"
    rdfs:label="pictTaking">
  <rdfs:subPropertyOf rdf:resource="http://www.kanzaki.com/ns/exif#pictTaking"/>
  <rdfs:subPropertyOf rdf:resource="&nexif;exifAttribute"/>
  <rdfs:domain rdf:resource="&nexif;Photo"/>
  <rdfs:range rdf:resource="&xsd;string"/>
</rdf:Property>

<rdfs:Class rdf:about="&ncal;TodoStatus"
    rdfs:label="TodoStatus">
  <rdfs:comment>A status of a calendar entity. This class has been introduced to express
the limited set of values for the ncal:status property. The user may
use the instances provided with this ontology or create his/her own.
See the documentation for ncal:todoStatus for details.</rdfs:comment>
  <rdfs:subClassOf rdf:resource="&rdfs;Resource"/>
</rdfs:Class>

<rdfs:Class rdf:about="&nco;IMAccount"
    rdfs:comment="An account in an Instant Messaging system."
    rdfs:label="IMAccount">
  <rdfs:subClassOf rdf:resource="&nco;ContactMedium"/>
</rdfs:Class>

<rdf:Property rdf:about="&foaf;surname"
    rdfs:comment="The surname of some person."
    rdfs:label="Surname"
    ns:term_status="archaic">
  <rdf:type rdf:resource="&owl;DatatypeProperty"/>
  <rdfs:domain rdf:resource="&foaf;Person"/>
  <rdfs:isDefinedBy rdf:resource="&foaf;"/>
  <rdfs:range rdf:resource="&rdfs;Literal"/>
</rdf:Property>

<rdf:Property rdf:about="&nexif;gpsDestLatitudeRef"
    rdfs:comment="tagNumber: 19
Reference for latitude of destination"
    rdfs:label="gpsDestLatitudeRef">
  <rdfs:subPropertyOf rdf:resource="http://www.kanzaki.com/ns/exif#gpsDestLatitudeRef"/>
  <rdfs:subPropertyOf rdf:resource="&nexif;gpsInfo"/>
  <rdfs:domain rdf:resource="&nexif;Photo"/>
  <rdfs:range rdf:resource="&xsd;string"/>
</rdf:Property>

<rdf:Property rdf:about="&pimo;isOrganizationMemberOf"
    rdfs:label="is member of organization">
  <nrl:inverseProperty rdf:resource="&pimo;hasOrganizationMember"/>
  <rdfs:comment>The subject person or organozation (Agent) is member of the object organization.</rdfs:comment>
  <rdfs:domain rdf:resource="&pimo;Agent"/>
  <rdfs:range rdf:resource="&pimo;Organization"/>
  <rdfs:subPropertyOf rdf:resource="&pimo;partOf"/>
</rdf:Property>

<owl:Class rdf:about="&oa;State">
  <rdfs:comment xml:lang="en">A resource which describes how to retrieve an appropriate representation of the Source resource, indicated with oa:hasState from the Specific Resource.

This class is not used directly in Annotations, only its subclasses are.

The Specifier's description MAY be conveyed as an external or embedded resource (cnt:Content), or as RDF properties within the graph. The description SHOULD use existing standards whenever possible. If the Specifier has an HTTP URI, then its description, and only its description, MUST be returned when the URI is dereferenced.</rdfs:comment>
  <rdfs:isDefinedBy rdf:resource="&oa;"/>
  <rdfs:label xml:lang="en">State</rdfs:label>
</owl:Class>

<rdf:Property rdf:about="&nie;relatedTo"
    rdfs:label="relatedTo">
  <rdfs:comment>A common superproperty for all relations between a piece of content and other pieces of data (which may be interpreted as other pieces of content).</rdfs:comment>
  <rdfs:domain rdf:resource="&nie;InformationElement"/>
  <rdfs:range rdf:resource="&nie;DataObject"/>
  <rdfs:subPropertyOf rdf:resource="&dc;relation"/>
</rdf:Property>

<rdfs:Class rdf:about="&dpo;Activity"
    rdfs:label="Activity">
  <rdfs:comment>Non-quantifiable presence information concerning the current activity of the agent.</rdfs:comment>
  <rdfs:subClassOf rdf:resource="&dpo;NonQuantifiableComponent"/>
</rdfs:Class>

<rdf:Property rdf:about="&nmo;to"
    rdfs:comment="deprecated in favor of nmo:emailTo"
    rdfs:label="to">
  <nao:deprecated rdf:datatype="&xsd;boolean">true</nao:deprecated>
  <rdfs:domain rdf:resource="&nmo;Email"/>
  <rdfs:range rdf:resource="&nco;Contact"/>
  <rdfs:subPropertyOf rdf:resource="&nmo;primaryRecipient"/>
</rdf:Property>

<rdf:Property rdf:about="&dpo;minYear"
    rdfs:label="Minimum Year">
  <rdfs:comment>A subproperty of dpo:minValue that defines a lowerbound on the observed calendar year such that it can classify as a dpo:TimePeriod instance. It can be used in conjunction with dpo:maxYear, i.e. specific instances of dpo:TimePeriod have a pre-defined observable year-based period.</rdfs:comment>
  <rdfs:domain rdf:resource="&dpo;TimePeriod"/>
  <rdfs:range rdf:resource="&xsd;integer"/>
  <rdfs:subPropertyOf rdf:resource="&dpo;minValue"/>
</rdf:Property>

<rdf:Property rdf:about="&nie;keyword"
    rdfs:label="keyword">
  <rdfs:comment>Adapted DublinCore: The topic of the content of the resource, as keyword. No sentences here. Recommended best practice is to select a value from a controlled vocabulary or formal classification scheme. </rdfs:comment>
  <rdfs:domain rdf:resource="&nie;InformationElement"/>
  <rdfs:range rdf:resource="&xsd;string"/>
</rdf:Property>

<rdfs:Class rdf:about="&dplo;WebDocumentPost"
    rdfs:label="Web Document Post">
  <rdfs:comment>A livepost consisting of links to remote web documents, as defined by further subclasses.</rdfs:comment>
  <rdfs:subClassOf rdf:resource="&dplo;LivePost"/>
</rdfs:Class>

<rdf:Property rdf:about="&cnt;chars">
  <rdf:type rdf:resource="&owl;ObjectProperty"/>
  <rdfs:comment xml:lang="en">The character sequence of the text content.</rdfs:comment>
  <rdfs:domain rdf:resource="&cnt;ContentAsText"/>
  <rdfs:label xml:lang="en">Character sequence</rdfs:label>
  <rdfs:range rdf:resource="&rdfs;Literal"/>
</rdf:Property>

<rdfs:Class rdf:about="&pimo;PersonGroup"
    rdfs:label="Group of Persons">
  <rdfs:subClassOf rdf:resource="&pimo;Agent"/>
  <rdfs:subClassOf rdf:resource="&pimo;Collection"/>
  <rdfs:comment>A group of Persons. They are connected to each other by sharing a common attribute, for example they all belong to the same organization or have a common interest. Refer to pimo:Collection for more information about defining collections.</rdfs:comment>
</rdfs:Class>

<rdfs:Class rdf:about="&ncal;Freebusy"
    rdfs:label="Freebusy">
  <rdfs:subClassOf rdf:resource="&nie;InformationElement"/>
  <rdfs:subClassOf rdf:resource="&ncal;UnionOfAlarmEventFreebusyJournalTodo"/>
  <rdfs:subClassOf rdf:resource="&ncal;UnionOfAlarmEventFreebusyTodo"/>
  <rdfs:subClassOf rdf:resource="&ncal;UnionOfEventFreebusy"/>
  <rdfs:subClassOf rdf:resource="&ncal;UnionOfEventFreebusyJournalTodo"/>
  <rdfs:subClassOf rdf:resource="&ncal;UnionOfTimezoneObservanceEventFreebusyJournalTimezoneTodo"/>
  <rdfs:subClassOf rdf:resource="&ncal;UnionOfTimezoneObservanceEventFreebusyTimezoneTodo"/>
  <rdfs:comment>Provide a grouping of component properties that describe either a request for free/busy time, describe a response to a request for free/busy time or describe a published set of busy time.</rdfs:comment>
</rdfs:Class>

<rdf:Property rdf:about="&foaf;made"
    rdfs:comment="Something that was made by this agent."
    rdfs:label="made"
    ns:term_status="stable">
  <rdf:type rdf:resource="&owl;ObjectProperty"/>
  <rdfs:domain rdf:resource="&foaf;Agent"/>
  <rdfs:isDefinedBy rdf:resource="&foaf;"/>
  <rdfs:range rdf:resource="&owl;Thing"/>
  <owl:inverseOf rdf:resource="&foaf;maker"/>
</rdf:Property>

<rdf:Property rdf:about="&dcon;dayWeek"
    rdfs:label="Day of the Week">
  <rdfs:comment>Derived from the dateTime, this property stores the number of days elapsed for the current week, where 1 indicates a Monday, and 7 a Sunday.</rdfs:comment>
  <rdfs:domain rdf:resource="&dpo;TimePeriod"/>
  <rdfs:range rdf:resource="&xsd;nonNegativeInteger"/>
  <rdfs:subPropertyOf rdf:resource="&dcon;hasContextAttribute"/>
</rdf:Property>

<rdf:Property rdf:about="&tmo;targetCompletion"
    nrl:maxCardinality="1"
    rdfs:label="targetCompletion">
  <rdfs:domain rdf:resource="&tmo;Task"/>
  <rdfs:range rdf:resource="&rdfs;Literal"/>
  <rdfs:subPropertyOf rdf:resource="&tmo;progress"/>
</rdf:Property>

<rdfs:Class rdf:about="&nfo;Document"
    rdfs:label="Document">
  <rdfs:comment>A generic document. A common superclass for all documents on the desktop.</rdfs:comment>
  <rdfs:subClassOf rdf:resource="&nie;InformationElement"/>
</rdfs:Class>

<rdf:Property rdf:about="&pimo;referencingOccurrence"
    rdfs:label="referencing occurrence">
  <rdfs:comment>The subject thing is described in the object document. Ideally, the document is public and its primary topic is the thing. Although this property is not inverse-functional (because the Occurrences are not canonical elements of a formal ontology) this property allows to use public documents, such as wikipedia pages, as indicators identity.  The more formal hasOtherRepresentation property can be used when an ontology about the subject exists.</rdfs:comment>
  <rdfs:domain rdf:resource="&pimo;Thing"/>
  <rdfs:range rdf:resource="&nie;InformationElement"/>
</rdf:Property>

<rdfs:Class rdf:about="&nco;Role"
    rdfs:label="Role">
  <rdfs:comment>A role played by a contact. Contacts that denote people, can have many roles (e.g. see the hasAffiliation property and Affiliation class). Contacts that denote Organizations or other Agents usually have one role.  Each role can introduce additional contact media.</rdfs:comment>
  <rdfs:subClassOf rdf:resource="&rdfs;Resource"/>
</rdfs:Class>

<rdf:Property rdf:about="&nmo;messageSubject"
    rdfs:comment="The subject of a message"
    rdfs:label="messageSubject">
  <nrl:maxCardinality rdf:datatype="&xsd;integer">1</nrl:maxCardinality>
  <rdfs:domain rdf:resource="&nmo;Message"/>
  <rdfs:range rdf:resource="&xsd;string"/>
  <rdfs:subPropertyOf rdf:resource="&nie;subject"/>
</rdf:Property>

<rdfs:Class rdf:about="&dctypes;MovingImage">
  <dcam:memberOf rdf:resource="&dcterms;DCMIType"/>
  <dcterms:description xml:lang="en">Examples include animations, movies, television programs, videos, zoetropes, or visual output from a simulation.  Instances of the type Moving Image must also be describable as instances of the broader type Image.</dcterms:description>
  <dcterms:hasVersion rdf:resource="http://dublincore.org/usage/terms/history/#MovingImage-003"/>
  <dcterms:issued rdf:datatype="&xsd;date">2003-11-18</dcterms:issued>
  <dcterms:modified rdf:datatype="&xsd;date">2008-01-14</dcterms:modified>
  <rdfs:comment xml:lang="en">A series of visual representations imparting an impression of motion when shown in succession.</rdfs:comment>
  <rdfs:isDefinedBy rdf:resource="&dctypes;"/>
  <rdfs:label xml:lang="en">Moving Image</rdfs:label>
  <rdfs:subClassOf rdf:resource="&dctypes;Image"/>
</rdfs:Class>

<rdf:Property rdf:about="&nuao;totalEventDuration"
    rdfs:comment="The total duration of all events"
    rdfs:label="event count">
  <nrl:maxCardinality rdf:datatype="&xsd;nonNegativeInteger">1</nrl:maxCardinality>
  <rdfs:domain rdf:resource="&rdfs;Resource"/>
  <rdfs:range rdf:resource="&xsd;duration"/>
</rdf:Property>

<rdf:Property rdf:about="&nie;language"
    nrl:maxCardinality="1"
    rdfs:label="language">
  <rdfs:comment>Language the InformationElement is expressed in. This property applies to the data object in its entirety. If the data object is divisible into parts expressed in multiple languages - more specific properties should be used. Users are encouraged to use the two-letter code specified in the RFC 3066</rdfs:comment>
  <rdfs:domain rdf:resource="&nie;InformationElement"/>
  <rdfs:range rdf:resource="&xsd;string"/>
  <rdfs:subPropertyOf rdf:resource="&dc;language"/>
</rdf:Property>

<rdf:Property rdf:about="&nexif;length"
    rdfs:label="length">
  <rdfs:comment>Length of an object. Could be a subProperty of other general schema.</rdfs:comment>
  <rdfs:domain rdf:resource="&nexif;Photo"/>
  <rdfs:range rdf:resource="&xsd;string"/>
  <rdfs:subPropertyOf rdf:resource="http://www.kanzaki.com/ns/exif#length"/>
</rdf:Property>

<rdf:Property rdf:about="&ncal;calscale"
    rdfs:label="calscale">
  <nrl:maxCardinality rdf:datatype="&xsd;integer">1</nrl:maxCardinality>
  <rdfs:comment>This property defines the calendar scale used for the calendar information specified in the iCalendar object. Defined in RFC 2445 sec. 4.7.1</rdfs:comment>
  <rdfs:domain rdf:resource="&ncal;Calendar"/>
  <rdfs:range rdf:resource="&ncal;CalendarScale"/>
</rdf:Property>

<rdf:Property rdf:about="&dpo;maxVisibility"
    rdfs:label="Maximum Visibility">
  <rdfs:comment>A subproperty of dpo:maxValue that defines an upperbound on the observed visibility (in kilometres) such that it can classify as a dpo:WeatherCondition instance. It can be used in conjunction with dpo:minVisibility to state that specific instances of dpo:WeatherCondition have a pre-defined range of observable real-world visibility levels. In addition, they can also be used with various other weather conditions values and ranges to define complex weather condition types.</rdfs:comment>
  <rdfs:domain rdf:resource="&dpo;WeatherConditions"/>
  <rdfs:range rdf:resource="&xsd;nonNegativeInteger"/>
  <rdfs:subPropertyOf rdf:resource="&dpo;maxValue"/>
</rdf:Property>

<nrl:GraphView rdf:about="&pimo;OccurrenceClosure"
    rdfs:label="OccurrenceClosure"/>

<rdf:Property rdf:about="&dcon;writeable"
    rdfs:label="is Writeable">
  <rdfs:comment>Specifies whether an active file (running on a device) is in read-and-write (true) or read-only mode (false) in the current context.</rdfs:comment>
  <rdfs:domain rdf:resource="&nie;InformationElement"/>
  <rdfs:range rdf:resource="&xsd;boolean"/>
  <rdfs:subPropertyOf rdf:resource="&dcon;hasContextAttribute"/>
</rdf:Property>

<rdf:Property rdf:about="&nfo;frameCount"
    rdfs:comment="The amount of frames in a video sequence."
    rdfs:label="frameCount">
  <nrl:maxCardinality rdf:datatype="&xsd;integer">1</nrl:maxCardinality>
  <rdfs:domain rdf:resource="&nfo;Video"/>
  <rdfs:range rdf:resource="&xsd;integer"/>
  <rdfs:subPropertyOf rdf:resource="&nfo;count"/>
</rdf:Property>

<rdf:Property rdf:about="&scos;broaderTransitive">
  <rdf:type rdf:resource="&owl;ObjectProperty"/>
  <rdf:type rdf:resource="&owl;TransitiveProperty"/>
  <rdfs:isDefinedBy rdf:resource="http://www.w3.org/2004/02/skos/core"/>
  <rdfs:label xml:lang="en">has broader transitive</rdfs:label>
  <rdfs:subPropertyOf rdf:resource="&scos;semanticRelation"/>
  <owl:inverseOf rdf:resource="&scos;narrowerTransitive"/>
  <scos:definition>skos:broaderTransitive is a transitive superproperty of skos:broader.</scos:definition>
  <scos:scopeNote xml:lang="en">By convention, skos:broaderTransitive is not used to make assertions. Rather, the properties can be used to draw inferences about the transitive closure of the hierarchical relation, which is useful e.g. when implementing a simple query expansion algorithm in a search application.</scos:scopeNote>
</rdf:Property>

<tmo:AbilityCarrierRole rdf:about="&tmo;TMO_Instance_AbilityCarrierRole_Used"
    rdfs:label="TMO_Instance_AbilityCarrierRole_Used"/>

<rdf:Property rdf:about="&ddo;deviceIdentifier"
    rdfs:comment="Represents the internal identifier for a device."
    rdfs:label="deviceIdentifier">
  <rdfs:domain rdf:resource="&ddo;Device"/>
  <rdfs:range rdf:resource="&xsd;string"/>
  <rdfs:subPropertyOf rdf:resource="&nao;identifier"/>
</rdf:Property>

<rdf:Property rdf:about="&pimo;createdPimo"
    rdfs:label="created Pimo">
  <nrl:inverseProperty rdf:resource="&pimo;creator"/>
  <rdfs:comment>The creator of the Personal Information Model. The human being whose mental models are represented in the PIMO.</rdfs:comment>
  <rdfs:domain rdf:resource="&pimo;Agent"/>
  <rdfs:range rdf:resource="&pimo;PersonalInformationModel"/>
</rdf:Property>

<rdfs:Class rdf:about="&dcterms;SizeOrDuration">
  <dcterms:description xml:lang="en">Examples include a number of pages, a specification of length, width, and breadth, or a period in hours, minutes, and seconds.</dcterms:description>
  <dcterms:hasVersion rdf:resource="http://dublincore.org/usage/terms/history/#SizeOrDuration-001"/>
  <dcterms:issued rdf:datatype="&xsd;date">2008-01-14</dcterms:issued>
  <rdfs:comment xml:lang="en">A dimension or extent, or a time taken to play or execute.</rdfs:comment>
  <rdfs:isDefinedBy rdf:resource="&dcterms;"/>
  <rdfs:label xml:lang="en">Size or Duration</rdfs:label>
  <rdfs:subClassOf rdf:resource="&dcterms;MediaTypeOrExtent"/>
</rdfs:Class>

<rdfs:Class rdf:about="&foaf;OnlineChatAccount"
    rdfs:comment="An online chat account."
    rdfs:label="Online Chat Account"
    ns:term_status="unstable">
  <rdf:type rdf:resource="&owl;Class"/>
  <rdfs:isDefinedBy rdf:resource="&foaf;"/>
  <rdfs:subClassOf rdf:resource="&foaf;OnlineAccount"/>
</rdfs:Class>

<rdf:Property rdf:about="&dpo;maxUVIndex"
    rdfs:label="Maximum UV Index">
  <rdfs:comment>A subproperty of dpo:minValue that defines an upperbound on the observed uv index levels (linear scale of between 0 and 12 signifying 11+) such that it can classify as a dpo:WeatherCondition instance. It can be used in conjunction with dpo:minUVIndex to state that specific instances of dpo:WeatherCondition have a pre-defined range of observable real-world UV index levels. In addition, they can also be used with various other weather conditions values and ranges to define complex weather condition types.</rdfs:comment>
  <rdfs:domain rdf:resource="&dpo;WeatherConditions"/>
  <rdfs:range rdf:resource="&xsd;nonNegativeInteger"/>
  <rdfs:subPropertyOf rdf:resource="&dpo;maxValue"/>
</rdf:Property>

<rdfs:Class rdf:about="&ddo;ComputerNetwork"
    rdfs:label="ComputerNetwork">
  <rdfs:comment>A communication channel that enables the interconnection and sharing of resources and information between a collection of hardware components and computers.</rdfs:comment>
  <rdfs:subClassOf rdf:resource="&ddo;Network"/>
</rdfs:Class>

<rdfs:Datatype rdf:about="&dcterms;URI">
  <dcterms:hasVersion rdf:resource="http://dublincore.org/usage/terms/history/#URI-003"/>
  <dcterms:issued rdf:datatype="&xsd;date">2000-07-11</dcterms:issued>
  <dcterms:modified rdf:datatype="&xsd;date">2008-01-14</dcterms:modified>
  <rdfs:comment xml:lang="en">The set of identifiers constructed according to the generic syntax for Uniform Resource Identifiers as specified by the Internet Engineering Task Force.</rdfs:comment>
  <rdfs:isDefinedBy rdf:resource="&dcterms;"/>
  <rdfs:label xml:lang="en">URI</rdfs:label>
  <rdfs:seeAlso rdf:resource="http://www.ietf.org/rfc/rfc3986.txt"/>
</rdfs:Datatype>

<rdf:Property rdf:about="&ncal;freebusy"
    rdfs:label="freebusy">
  <rdfs:comment>The property defines one or more free or busy time intervals. Inspired by RFC 2445 sec. 4.8.2.6. Note that the periods specified by this property can only be expressed with UTC times. Originally this property could have many comma-separated values. Please use a separate triple for each value.</rdfs:comment>
  <rdfs:domain rdf:resource="&ncal;Freebusy"/>
  <rdfs:range rdf:resource="&ncal;FreebusyPeriod"/>
</rdf:Property>

<rdf:Property rdf:about="&scos;hiddenLabel">
  <rdfs:comment xml:lang="en">The range of skos:hiddenLabel is the class of RDF plain literals.</rdfs:comment>
  <rdfs:comment xml:lang="en">skos:prefLabel, skos:altLabel and skos:hiddenLabel are pairwise disjoint properties.</rdfs:comment>
  <rdf:type rdf:resource="&owl;AnnotationProperty"/>
  <rdfs:isDefinedBy rdf:resource="http://www.w3.org/2004/02/skos/core"/>
  <rdfs:label xml:lang="en">hidden label</rdfs:label>
  <rdfs:subPropertyOf rdf:resource="&rdfs;label"/>
  <scos:definition xml:lang="en">A lexical label for a resource that should be hidden when generating visual displays of the resource, but should still be accessible to free text search operations.</scos:definition>
</rdf:Property>

<rdf:Property rdf:about="&nso;sharedWithGroup"
    rdfs:label="shared with group">
  <rdfs:comment>The subject resource is shared with all contacts belonging to the object contact group. 
The resource and its subresources are transferred to the receivers.
An existing sharedWithGroup relation implies that updates on the resource should be transferred to the members belonging to the group. 
The contact may ask for updates actively, then the sharing party's software should send a new copy of the shared resource to the contact.
Domain should be either a nie:InformationElement or a pimo:Thing but no DataObject. This includes ncal:Event instances and other resources we find on a desktop.
DataObjects are the specific binary stream where an Information Element is stored, and can't be shared because the recipient will form a new binary stream to store the data object. 
As there is no superclass of both nie:InformationElement and pimo:Thing, the domain is rdfs:Resource. 
One resource can be shared to multiple contact groups, the cardinality is 0..n. </rdfs:comment>
  <rdfs:domain rdf:resource="&rdfs;Resource"/>
  <rdfs:range rdf:resource="&nco;ContactGroup"/>
  <rdfs:subPropertyOf rdf:resource="&nso;sharedWith"/>
</rdf:Property>

<rdf:Property rdf:about="&nco;hasPersonName"
    rdfs:comment="Attaches name information to a person contact."
    rdfs:label="hasPersonName">
  <nrl:MaxCardinality rdf:datatype="&xsd;integer">1</nrl:MaxCardinality>
  <rdfs:domain rdf:resource="&nco;PersonContact"/>
  <rdfs:range rdf:resource="&nco;PersonName"/>
</rdf:Property>

<rdf:Property rdf:about="&pimo;organization"
    rdfs:label="organization">
  <rdfs:comment>relation to the organization in an OrganizationMember association.</rdfs:comment>
  <rdfs:domain rdf:resource="&pimo;OrganizationMember"/>
  <rdfs:range rdf:resource="&pimo;Organization"/>
  <rdfs:subPropertyOf rdf:resource="&pimo;associationMember"/>
</rdf:Property>

<rdf:Property rdf:about="&scos;notation">
  <rdf:type rdf:resource="&owl;DatatypeProperty"/>
  <rdfs:isDefinedBy rdf:resource="http://www.w3.org/2004/02/skos/core"/>
  <rdfs:label xml:lang="en">notation</rdfs:label>
  <scos:definition xml:lang="en">A notation, also known as classification code, is a string of characters such as "T58.5" or "303.4833" used to uniquely identify a concept within the scope of a given concept scheme.</scos:definition>
  <scos:scopeNote xml:lang="en">By convention, skos:notation is used with a typed literal in the object position of the triple.</scos:scopeNote>
</rdf:Property>

<rdf:Property rdf:about="&nco;isBlocked"
    nrl:maxCardinality="1"
    rdfs:comment="Indicates that this IMAccount has been blocked."
    rdfs:label="isBlocked">
  <rdfs:domain rdf:resource="&nco;IMAccount"/>
  <rdfs:range rdf:resource="&xsd;boolean"/>
</rdf:Property>

<rdf:Property rdf:about="&nexif;bitsPerSample"
    rdfs:label="bitsPerSample">
  <rdfs:subPropertyOf rdf:resource="http://www.kanzaki.com/ns/exif#bitsPerSample"/>
  <rdfs:subPropertyOf rdf:resource="&nexif;imageDataStruct"/>
  <rdfs:subPropertyOf rdf:resource="&nexif;resolution"/>
  <rdfs:comment>tagNumber: 258
The number of bits per image component. In this standard each component of the image is 8 bits, so the value for this tag is 8. See also SamplesPerPixel. In JPEG compressed data a JPEG marker is used instead of this tag.</rdfs:comment>
  <rdfs:domain rdf:resource="&nexif;Photo"/>
  <rdfs:range rdf:resource="&xsd;string"/>
</rdf:Property>

<rdf:Property rdf:about="&nie;description"
    rdfs:label="description">
  <rdfs:subPropertyOf rdf:resource="&dc;description"/>
  <rdfs:subPropertyOf rdf:resource="&nao;description"/>
  <rdfs:comment>A textual description of the resource. This property may be used for any metadata fields that provide some meta-information or comment about a resource in the form of a passage of text. This property is not to be confused with nie:plainTextContent. Use more specific subproperties wherever possible.</rdfs:comment>
  <rdfs:domain rdf:resource="&nie;InformationElement"/>
  <rdfs:range rdf:resource="&xsd;string"/>
</rdf:Property>

<rdf:Property rdf:about="&ncal;description"
    rdfs:label="description">
  <rdfs:comment>A more complete description of the calendar component, than  that provided by the ncal:summary property.Inspired by RFC 2445 sec. 4.8.1.5 with following reservations:  the LANGUAGE parameter has been discarded. Please use xml:lang literals to express language. For the ALTREP parameter use the descriptionAltRep property.</rdfs:comment>
  <rdfs:domain rdf:resource="&ncal;UnionOfAlarmEventJournalTodo"/>
  <rdfs:range rdf:resource="&xsd;string"/>
  <rdfs:subPropertyOf rdf:resource="&nie;description"/>
</rdf:Property>

<rdf:Property rdf:about="&drmo;hasConstraint"
    rdfs:label="has constraints">
  <rdfs:comment>Defines the constraints (which are of type drmo:Condition) which make up a rule's condition. This property is a subproperty of drmo:hasConstraintOnSubject, such that its range is restricted to a drmo:Condition. What this `restriction' really means is that a drmo:Condition is expected both as the domain and the range for this property. This has the effect of creating nested constraints whereby the referred condition (range defined for this property) is itself another condition. Therefore, the condition at the range of this property needs to be resolved first, before being able to apply this constraint on the condition defined in the domain. Thus the difference between this property and its superproperty is that whereas the latter will look for triples (subject, predicate, object) having one specific item (which is simply the range of drmo:hasConstraintOnSubject) as its subject, this property might result in multiple queries each of which match a different item to its subject. The pattern  to retrieve these item(s) is defined by the condition that is in the range of this property, i.e., it is defined by another set of drmo:hasConstraintOnSubject or drmo:hasConstraintOnObject and a corresponding drmo:hasConstraintOnProperty.</rdfs:comment>
  <rdfs:domain rdf:resource="&drmo;Condition"/>
  <rdfs:range rdf:resource="&drmo;Condition"/>
  <rdfs:subProperty rdf:resource="&drmo;hasConstraintOnSubject"/>
</rdf:Property>

<rdfs:Class rdf:about="&nco;PcsNumber"
    rdfs:label="PcsNumber">
  <rdfs:comment>Personal Communication Services Number. A class inspired by the TYPE=pcs parameter of the TEL property defined in RFC 2426 sec. 3.3.1</rdfs:comment>
  <rdfs:subClassOf rdf:resource="&nco;VoicePhoneNumber"/>
</rdfs:Class>

<rdf:Property rdf:about="&nexif;pimColorBalance"
    rdfs:comment="tagNumber: 11
ColorBalance info for print image matching"
    rdfs:label="pimColorBalance">
  <rdfs:subPropertyOf rdf:resource="http://www.kanzaki.com/ns/exif#pimColorBalance"/>
  <rdfs:subPropertyOf rdf:resource="&nexif;pimInfo"/>
  <rdfs:domain rdf:resource="&nexif;Photo"/>
  <rdfs:range rdf:resource="&xsd;string"/>
</rdf:Property>

<rdf:Property rdf:about="&ncal;freq"
    rdfs:label="freq">
  <nrl:maxCardinality rdf:datatype="&xsd;integer">1</nrl:maxCardinality>
  <rdfs:comment>Frequency of a recurrence rule. Defined in RFC 2445 sec. 4.3.10</rdfs:comment>
  <rdfs:domain rdf:resource="&ncal;RecurrenceRule"/>
  <rdfs:range rdf:resource="&ncal;RecurrenceFrequency"/>
</rdf:Property>

<rdfs:Class rdf:about="&nco;EmailAddress"
    rdfs:label="EmailAddress">
  <rdfs:comment>An email address. The recommended best practice is to use mailto: uris for instances of this class.</rdfs:comment>
  <rdfs:subClassOf rdf:resource="&nco;ContactMedium"/>
</rdfs:Class>

<rdf:Property rdf:about="&nco;hasCustomAttribute"
    rdfs:label="hasCustomAttribute">
  <rdfs:comment>A generic contact attribute introduced in order to enable customisation of contact details. Thus, systems using the NCO to model contact and person information, can introduce customised attributes by creating them as a subproperty of this one.</rdfs:comment>
  <rdfs:domain rdf:resource="&nco;Contact"/>
</rdf:Property>

<rdf:Property rdf:about="&nmo;headerValue"
    nrl:maxCardinality="1"
    rdfs:comment="Value of the message header."
    rdfs:label="headerValue">
  <rdfs:domain rdf:resource="&nmo;MessageHeader"/>
  <rdfs:range rdf:resource="&xsd;string"/>
</rdf:Property>

<rdf:Property rdf:about="&ncal;component"
    rdfs:label="component">
  <rdfs:comment>Links the Vcalendar instance with the calendar components. This property has no direct equivalent in the RFC specification. It has been introduced to express the containmnent relations.</rdfs:comment>
  <rdfs:domain rdf:resource="&ncal;Calendar"/>
  <rdfs:range rdf:resource="&ncal;CalendarDataObject"/>
  <rdfs:subPropertyOf rdf:resource="&nie;hasPart"/>
</rdf:Property>

<rdf:Property rdf:about="&nid3;textElementTimestamp"
    rdfs:label="textElementTimestamp">
  <rdfs:comment>The 'time stamp' is set to zero or the whole sync is omitted if located directly at the beginning of the sound. All time stamps should be sorted in chronological order. The sync can be considered as a validator of the subsequent string.</rdfs:comment>
  <rdfs:domain rdf:resource="&nid3;SynchronizedTextElement"/>
  <rdfs:range rdf:resource="&xsd;integer"/>
</rdf:Property>

<rdf:Property rdf:about="&dcterms;date">
  <dcterms:description xml:lang="en">Date may be used to express temporal information at any level of granularity.  Recommended best practice is to use an encoding scheme, such as the W3CDTF profile of ISO 8601 [W3CDTF].</dcterms:description>
  <dcterms:hasVersion rdf:resource="http://dublincore.org/usage/terms/history/#dateT-001"/>
  <dcterms:issued rdf:datatype="&xsd;date">2008-01-14</dcterms:issued>
  <dcterms:modified rdf:datatype="&xsd;date">2008-01-14</dcterms:modified>
  <rdfs:comment xml:lang="en">A point or period of time associated with an event in the lifecycle of the resource.</rdfs:comment>
  <rdfs:isDefinedBy rdf:resource="&dcterms;"/>
  <rdfs:label xml:lang="en">Date</rdfs:label>
  <rdfs:range rdf:resource="&rdfs;Literal"/>
  <rdfs:subPropertyOf rdf:resource="&dc;date"/>
</rdf:Property>

<rdfs:Class rdf:about="&nao;Tag"
    rdfs:comment="Represents a generic tag"
    rdfs:label="tag">
  <rdfs:subClassOf rdf:resource="&rdfs;Resource"/>
</rdfs:Class>

<rdfs:Class rdf:about="&dctypes;StillImage">
  <dcam:memberOf rdf:resource="&dcterms;DCMIType"/>
  <dcterms:description xml:lang="en">Examples include paintings, drawings, graphic designs, plans and maps. Recommended best practice is to assign the type Text to images of textual materials. Instances of the type Still Image must also be describable as instances of the broader type Image.</dcterms:description>
  <dcterms:hasVersion rdf:resource="http://dublincore.org/usage/terms/history/#StillImage-003"/>
  <dcterms:issued rdf:datatype="&xsd;date">2003-11-18</dcterms:issued>
  <dcterms:modified rdf:datatype="&xsd;date">2008-01-14</dcterms:modified>
  <rdfs:comment xml:lang="en">A static visual representation.</rdfs:comment>
  <rdfs:isDefinedBy rdf:resource="&dctypes;"/>
  <rdfs:label xml:lang="en">Still Image</rdfs:label>
  <rdfs:subClassOf rdf:resource="&dctypes;Image"/>
</rdfs:Class>

<rdf:Property rdf:about="&nmm;musicCDIdentifier"
    rdfs:label="music CD identifier">
  <rdfs:comment>Music CD identifier to for databases like FreeDB.org. This property is intended for music that comes from a CD, so that the CD can be identified in external databases.</rdfs:comment>
  <rdfs:domain rdf:resource="&nmm;MusicAlbum"/>
  <rdfs:range rdf:resource="&xsd;string"/>
  <rdfs:subPropertyOf rdf:resource="&nie;identifier"/>
</rdf:Property>

<rdf:Property rdf:about="&nco;hasBirthDate"
    rdfs:comment="Attaches birth date information to a person contact."
    rdfs:label="hasBirthDate">
  <nrl:MaxCardinality rdf:datatype="&xsd;integer">1</nrl:MaxCardinality>
  <rdfs:domain rdf:resource="&nco;PersonContact"/>
  <rdfs:range rdf:resource="&nco;BirthDate"/>
</rdf:Property>

<rdfs:Class rdf:about="&nco;CarPhoneNumber"
    rdfs:label="CarPhoneNumber">
  <rdfs:comment>A car phone number. Inspired by the (TYPE=car) parameter of the TEL property as defined in RFC 2426 sec  3.3.1.</rdfs:comment>
  <rdfs:subClassOf rdf:resource="&nco;VoicePhoneNumber"/>
</rdfs:Class>

<rdf:Property rdf:about="&nie;sourceMode"
    rdfs:comment="Represents a number of applicable modes for a data source."
    rdfs:label="Data Source Mode">
  <rdfs:domain rdf:resource="&nie;DataSource"/>
  <rdfs:range rdf:resource="&nie;Mode"/>
</rdf:Property>

<rdf:Property rdf:about="&dcon;temperature"
    rdfs:label="Temperature Value">
  <rdfs:comment>Registers an actual temperature value element attribute to an active weather condition or temperature range in the current context. As this context attribute applies to instances of both dpo:Temperature and dpo:WeatherConditions in the DPO Presence Ontology, the domain has been generalised to the first common DPO superclass. However, the attachment of this attribute to other instances is not considered correct application of the DCON vocabulary.</rdfs:comment>
  <rdfs:domain rdf:resource="&dpo;QuantifiableComponent"/>
  <rdfs:range rdf:resource="&xsd;float"/>
  <rdfs:subPropertyOf rdf:resource="&dcon;hasContextAttribute"/>
</rdf:Property>

<rdf:Property rdf:about="&nid3;involvment"
    rdfs:label="involvment">
  <rdfs:comment>How was this particular person involved in this particular track.</rdfs:comment>
  <rdfs:domain rdf:resource="&nid3;InvolvedPerson"/>
  <rdfs:range rdf:resource="&xsd;string"/>
</rdf:Property>

<rdfs:Class rdf:about="&pimo;State"
    rdfs:label="State">
  <rdfs:comment>Administrative subdivisions of a Nation that are broader than any other political subdivisions that may exist. This Class includes the states of the United States, as well as the provinces of Canada and European countries. (Definition from SUMO).</rdfs:comment>
  <rdfs:subClassOf rdf:resource="&pimo;Location"/>
</rdfs:Class>

<rdf:Property rdf:about="&dc;rights">
  <dcterms:description xml:lang="en">Typically, rights information includes a statement about various property rights associated with the resource, including intellectual property rights.</dcterms:description>
  <dcterms:hasVersion rdf:resource="http://dublincore.org/usage/terms/history/#rights-006"/>
  <dcterms:issued rdf:datatype="&xsd;date">1999-07-02</dcterms:issued>
  <dcterms:modified rdf:datatype="&xsd;date">2008-01-14</dcterms:modified>
  <rdfs:comment xml:lang="en">Information about rights held in and over the resource.</rdfs:comment>
  <rdfs:isDefinedBy rdf:resource="&dc;"/>
  <rdfs:label xml:lang="en">Rights</rdfs:label>
  <scos:note xml:lang="en">A second property with the same name as this property has been declared in the dcterms: namespace (http://purl.org/dc/terms/).  See the Introduction to the document "DCMI Metadata Terms" (http://dublincore.org/documents/dcmi-terms/) for an explanation.</scos:note>
</rdf:Property>

<rdfs:Class rdf:about="&ncal;UnionOfEventTodo"
    rdfs:label="UnionOfEventTodo">
  <rdfs:subClassOf rdf:resource="&ncal;UnionParentClass"/>
</rdfs:Class>

<rdf:Property rdf:about="&foaf;tipjar"
    rdfs:label="tipjar"
    ns:term_status="testing">
  <rdf:type rdf:resource="&owl;ObjectProperty"/>
  <rdfs:comment>A tipjar document for this agent, describing means for payment and reward.</rdfs:comment>
  <rdfs:domain rdf:resource="&foaf;Agent"/>
  <rdfs:isDefinedBy rdf:resource="&foaf;"/>
  <rdfs:range rdf:resource="&foaf;Document"/>
  <rdfs:subPropertyOf rdf:resource="&foaf;page"/>
</rdf:Property>

<rdf:Property rdf:about="&pimo;associationMember"
    rdfs:label="association member">
  <rdfs:comment>An super-property of all roles that an entity can have in an association. Member is the generic role of a thing in an association. Association subclasses should define sub-properties of this property. Associations can have Things as</rdfs:comment>
  <rdfs:domain rdf:resource="&pimo;Association"/>
  <rdfs:range rdf:resource="&pimo;Thing"/>
</rdf:Property>

<rdf:Property rdf:about="&ncal;created"
    rdfs:label="created">
  <nrl:maxCardinality rdf:datatype="&xsd;integer">1</nrl:maxCardinality>
  <rdfs:comment>This property specifies the date and time that the calendar information was created by the calendar user agent in the calendar store. Note: This is analogous to the creation date and time for a file in the file system. Inspired by RFC 2445 sec. 4.8.7.1. Note that this property is a subproperty of nie:created. The domain of nie:created is nie:DataObject. It is not a superclass of UnionOf_Vevent_Vjournal_Vtodo, but since that union is conceived as an 'abstract' class, and in real-life all resources referenced by this property will also be DataObjects, than this shouldn't cause too much of a problem. Note that RFC allows ONLY UTC time values for this property.</rdfs:comment>
  <rdfs:domain rdf:resource="&ncal;UnionOfEventJournalTodo"/>
  <rdfs:range rdf:resource="&xsd;dateTime"/>
  <rdfs:subPropertyOf rdf:resource="&nie;created"/>
</rdf:Property>

<rdf:Property rdf:about="&pimo;hasLocation"
    nrl:maxCardinality="1"
    rdfs:label="has location">
  <nrl:inverseProperty rdf:resource="&pimo;isLocationOf"/>
  <rdfs:comment>The subject thing is currently located at the object location.</rdfs:comment>
  <rdfs:domain rdf:resource="&pimo;Locatable"/>
  <rdfs:range rdf:resource="&pimo;Location"/>
  <rdfs:subPropertyOf rdf:resource="&pimo;isRelated"/>
</rdf:Property>

<rdfs:Class rdf:about="&foaf;Image"
    rdfs:comment="An image."
    rdfs:label="Image"
    ns:term_status="stable">
  <rdf:type rdf:resource="&owl;Class"/>
  <rdfs:isDefinedBy rdf:resource="&foaf;"/>
  <rdfs:subClassOf rdf:resource="&foaf;Document"/>
  <owl:equivalentClass rdf:resource="http://schema.org/ImageObject"/>
</rdfs:Class>

<rdf:Property rdf:about="&dcon;direction"
    rdfs:label="Direction Value">
  <rdfs:comment>States the actual direction value for a pre-defined direction range in the current context.</rdfs:comment>
  <rdfs:domain rdf:resource="&dpo;Direction"/>
  <rdfs:range rdf:resource="&xsd;string"/>
  <rdfs:subPropertyOf rdf:resource="&dcon;hasContextAttribute"/>
</rdf:Property>

<rdf:Property rdf:about="&nao;hasTopic"
    rdfs:label="has topic">
  <nrl:inverseProperty rdf:resource="&nao;isTopicOf"/>
  <rdfs:comment>Defines a relationship between two resources, where the object is a topic of the subject</rdfs:comment>
  <rdfs:range rdf:resource="&rdfs;Resource"/>
  <rdfs:subPropertyOf rdf:resource="&nao;isRelated"/>
</rdf:Property>

<nrl:DefiningProperty rdf:about="&nmm;lyricist"
    rdfs:comment="Lyricist"
    rdfs:label="lyricist">
  <rdf:type rdf:resource="&rdf;Property"/>
  <rdfs:domain rdf:resource="&nmm;MusicPiece"/>
  <rdfs:range rdf:resource="&nco;Contact"/>
  <rdfs:subPropertyOf rdf:resource="&nco;contributor"/>
</nrl:DefiningProperty>

<rdfs:Class rdf:about="&nrl;InstanceBase"
    rdfs:comment="Represents a named graph containing instance data"
    rdfs:label="InstanceBase">
  <rdfs:subClassOf rdf:resource="&nrl;Data"/>
</rdfs:Class>

<tmo:PersonInvolvementRole rdf:about="&tmo;TMO_Instance_PersonInvolvementRole_Collaborator"
    rdfs:label="TMO_Instance_PersonInvolvementRole_Collaborator"/>

<rdf:Property rdf:about="&nso;hasPrivacyPreference"
    rdfs:label="has privacy preference">
  <nrl:inverseProperty rdf:resource="&nso;isPrivacyPreferenceOf"/>
  <rdfs:comment>Enables the possibility of creating and maintaining privacy preferences regulating an agent's (typically only the current system user) access to third parties. For more information refer to the PPO Ontology, and the pimo:excludes, pimo:includes properties below.</rdfs:comment>
  <rdfs:domain rdf:resource="&pimo;Agent"/>
  <rdfs:range rdf:resource="http://vocab.deri.ie/ppo#PrivacyPreference"/>
</rdf:Property>

<rdf:Property rdf:about="&tmo;contextThread"
    nrl:maxCardinality="1"
    rdfs:label="contextThread">
  <nrl:inverseProperty rdf:resource="&tmo;contextTask"/>
  <rdfs:domain rdf:resource="&tmo;Task"/>
  <rdfs:range rdf:resource="http://ontologies.opendfki.de/repos/ontologies/wcon/workcontext#MediumTermContextThread"/>
</rdf:Property>

<rdf:Property rdf:about="&foaf;depiction"
    rdfs:comment="A depiction of some thing."
    rdfs:label="depiction"
    ns:term_status="testing">
  <rdf:type rdf:resource="&owl;ObjectProperty"/>
  <rdfs:domain rdf:resource="&owl;Thing"/>
  <rdfs:isDefinedBy rdf:resource="&foaf;"/>
  <rdfs:range rdf:resource="&foaf;Image"/>
  <owl:inverseOf rdf:resource="&foaf;depicts"/>
</rdf:Property>

<rdf:Property rdf:about="&rdfs;isDefinedBy">
  <rdfs:comment xml:lang="en">The defininition of the subject resource.</rdfs:comment>
  <rdfs:domain rdf:resource="&rdfs;Resource"/>
  <rdfs:isDefinedBy rdf:resource="&rdfs;"/>
  <rdfs:label xml:lang="en">isDefinedBy</rdfs:label>
  <rdfs:range rdf:resource="&rdfs;Resource"/>
  <rdfs:subPropertyOf rdf:resource="&rdfs;seeAlso"/>
</rdf:Property>

<tmo:TaskState rdf:about="&tmo;TMO_Instance_TaskState_Finalized"
    rdfs:label="TMO_Instance_TaskState_Finalized"/>

<tmo:TaskPrivacyState rdf:about="&tmo;TMO_Instance_TaskPrivacy_Professional"
    rdfs:label="TMO_Instance_TaskPrivacy_Professional"/>

<rdf:Property rdf:about="&nid3;recordingYear"
    rdfs:label="recordingYear">
  <rdfs:comment>TYER
The 'Year' frame is a numeric string with a year of the recording. This frames is always four characters long (until the year 10000).</rdfs:comment>
  <rdfs:domain rdf:resource="&nid3;ID3Audio"/>
  <rdfs:range rdf:resource="&xsd;integer"/>
</rdf:Property>

<rdfs:Class rdf:about="&ncal;UnionOfAlarmEventTodo"
    rdfs:label="UnionOfAlarmEventTodo">
  <rdfs:subClassOf rdf:resource="&ncal;UnionParentClass"/>
</rdfs:Class>

<rdf:Property rdf:about="&nexif;exposureTime"
    rdfs:comment="tagNumber: 33434
Exposure time, given in seconds (sec)."
    rdfs:label="exposureTime">
  <rdfs:subPropertyOf rdf:resource="http://www.kanzaki.com/ns/exif#exposureTime"/>
  <rdfs:subPropertyOf rdf:resource="&nexif;pictTaking"/>
  <rdfs:subPropertyOf rdf:resource="&nexif;seconds"/>
  <rdfs:domain rdf:resource="&nexif;Photo"/>
  <rdfs:range rdf:resource="&xsd;float"/>
</rdf:Property>

<tmo:Delegability rdf:about="&tmo;TMO_Instance_Delegability_Never"
    rdfs:label="TMO_Instance_Delegability_Never"/>

<rdf:Property rdf:about="&nfo;lineCount"
    rdfs:comment="The amount of lines in a text document"
    rdfs:label="lineCount">
  <nrl:maxCardinality rdf:datatype="&xsd;integer">1</nrl:maxCardinality>
  <rdfs:domain rdf:resource="&nfo;TextDocument"/>
  <rdfs:range rdf:resource="&xsd;integer"/>
</rdf:Property>

<owl:Ontology rdf:about="&oa;"
    owl:versionInfo="0.9.20130208">
  <dc:creator xml:lang="en">Robert Sanderson</dc:creator>
  <dc:creator xml:lang="it">Paolo Ciccarese</dc:creator>
  <dc:creator xml:lang="vls">Herbert Van de Sompel</dc:creator>
  <dc:contributor xml:lang="en">Stian Soiland-Reyes</dc:contributor>
  <dc:description xml:lang="en">The Open Annotation Core Data Model specifies an interoperable framework for creating associations between related resources, annotations, using a methodology that conforms to the Architecture of the World Wide Web. Open Annotations can easily be shared between platforms, with sufficient richness of expression to satisfy complex requirements while remaining simple enough to also allow for the most common use cases, such as attaching a piece of text to a single web resource.

An Annotation is considered to be a set of connected resources, typically including a body and target, where the body is somehow about the target. The full model supports additional functionality, enabling semantic annotations, embedding content, selecting segments of resources, choosing the appropriate representation of a resource and providing styling hints for consuming clients.</dc:description>
  <dc:title xml:lang="en">Open Annotation Data Model</dc:title>
  <dcterms:modified rdf:datatype="&xsd;dateTime">2013-02-22T21:40:51+01:00</dcterms:modified>
  <rdfs:comment xml:lang="en">The Open Annotation Core Data Model specifies an interoperable framework for creating associations between related resources, annotations, using a methodology that conforms to the Architecture of the World Wide Web.

This ontology is a non-normative OWL formalization of the textual OA specification at http://www.openannotation.org/spec/core/20130208/index.html

Note that OWL imports are disabled in the published version in order to reduce external implications, improve OWL 2 Profile conformity and increase interoperability. Some OWL tools might thus misleadingly show this ontology as (re)defining properties like skos:prefLabel.</rdfs:comment>
  <rdfs:seeAlso rdf:resource="http://www.openannotation.org/spec/core/20130208/index.html"/>
  <owl:versionIRI rdf:resource="http://www.openannotation.org/spec/core/20130208/oa.owl"/>
</owl:Ontology>

<rdf:Property rdf:about="&nexif;gpsTimeStamp"
    rdfs:label="gpsTimeStamp">
  <rdfs:subPropertyOf rdf:resource="http://www.kanzaki.com/ns/exif#gpsTimeStamp"/>
  <rdfs:subPropertyOf rdf:resource="&nexif;gpsInfo"/>
  <rdfs:comment>tagNumber: 7
The time as UTC (Coordinated Universal Time). TimeStamp is expressed as three RATIONAL values giving the hour, minute, and second.</rdfs:comment>
  <rdfs:domain rdf:resource="&nexif;Photo"/>
  <rdfs:range rdf:resource="&xsd;string"/>
</rdf:Property>

<rdf:Property rdf:about="&nmo;sentDate"
    nrl:maxCardinality="1"
    rdfs:comment="Date when this message was sent."
    rdfs:label="sentDate">
  <rdfs:subPropertyOf rdf:resource="&dc;date"/>
  <rdfs:subPropertyOf rdf:resource="&nie;contentCreated"/>
  <rdfs:domain rdf:resource="&nmo;Message"/>
  <rdfs:range rdf:resource="&xsd;dateTime"/>
</rdf:Property>

<rdfs:Class rdf:about="&tmo;TaskPrivacyState"
    rdfs:label="TaskPrivacyState">
  <rdfs:comment>Privacy Status serves for the separation between a professional and a private purpose of a task. This attribute provides with the values "professional/private" a high-level separation of privacy in terms of setting distribution and access
rights to other users for the task.
This separation may arise as a general Nepomuk issue and may therefore be handled in conjunction with a privacy preserving SSD architecture.</rdfs:comment>
  <rdfs:subClassOf rdf:resource="&tmo;StateTypeRole"/>
</rdfs:Class>

<rdfs:Class rdf:about="&nfo;MediaFileListEntry"
    rdfs:label="MediaFileListEntry">
  <rdfs:comment>A single node in the list of media files contained within an MediaList instance. This class is intended to provide a type all those links have. In valid NRL untyped resources cannot be linked. There are no properties defined for this class but the application may expect rdf:first and rdf:last links. The former points to the DataObject instance, interpreted as Media the latter points at another MediaFileListEntr. At the end of the list there is a link to rdf:nil.</rdfs:comment>
  <rdfs:subClassOf rdf:resource="&rdfs;Resource"/>
</rdfs:Class>

<rdf:Property rdf:about="&tmo;timemanagement"
    nrl:maxCardinality="1"
    rdfs:label="timemanagement">
  <rdfs:range rdf:resource="&rdfs;Literal"/>
</rdf:Property>

<rdf:Property rdf:about="&pimo;classRole"
    nrl:maxCardinality="1"
    rdfs:label="class role">
  <rdfs:comment>Annotating abstract and concrete classes. Implementations may offer the feature to hide abstract classes. By default, classes are concrete. Classes can be declared abstract by setting their classRole to abstract. Instances should not have an abstract class as type (if not inferred).</rdfs:comment>
  <rdfs:range rdf:resource="&pimo;ClassRole"/>
</rdf:Property>

<rdf:Property rdf:about="&nexif;planarConfiguration"
    rdfs:label="planarConfiguration">
  <rdfs:subPropertyOf rdf:resource="http://www.kanzaki.com/ns/exif#planarConfiguration"/>
  <rdfs:subPropertyOf rdf:resource="&nexif;imageDataStruct"/>
  <rdfs:comment>Indicates whether pixel components are recorded in chunky or planar format. In JPEG compressed files a JPEG marker is used instead of this tag. If this field does not exist, the TIFF default of 1 (chunky) is assumed.
tagNumber: 284</rdfs:comment>
  <rdfs:domain rdf:resource="&nexif;Photo"/>
  <rdfs:range rdf:resource="&xsd;string"/>
</rdf:Property>

<rdf:Property rdf:about="&nao;hasDefaultNamespaceAbbreviation"
    rdfs:label="has default namespace abbreviation">
  <nrl:maxCardinality rdf:datatype="&xsd;nonNegativeInteger">1</nrl:maxCardinality>
  <rdfs:comment>Defines the default static namespace abbreviation for a graph</rdfs:comment>
  <rdfs:domain rdf:resource="&nrl;Data"/>
  <rdfs:range rdf:resource="&rdfs;Literal"/>
  <rdfs:subPropertyOf rdf:resource="&nao;annotation"/>
</rdf:Property>

<rdf:Property rdf:about="&dcterms;source">
  <rdfs:subPropertyOf rdf:resource="&dc;source"/>
  <rdfs:subPropertyOf rdf:resource="&dcterms;relation"/>
  <dcterms:description xml:lang="en">The described resource may be derived from the related resource in whole or in part. Recommended best practice is to identify the related resource by means of a string conforming to a formal identification system.</dcterms:description>
  <dcterms:hasVersion rdf:resource="http://dublincore.org/usage/terms/history/#sourceT-001"/>
  <dcterms:issued rdf:datatype="&xsd;date">2008-01-14</dcterms:issued>
  <dcterms:modified rdf:datatype="&xsd;date">2008-01-14</dcterms:modified>
  <rdfs:comment xml:lang="en">A related resource from which the described resource is derived.</rdfs:comment>
  <rdfs:isDefinedBy rdf:resource="&dcterms;"/>
  <rdfs:label xml:lang="en">Source</rdfs:label>
  <scos:note xml:lang="en">This term is intended to be used with non-literal values as defined in the DCMI Abstract Model (http://dublincore.org/documents/abstract-model/).  As of December 2007, the DCMI Usage Board is seeking a way to express this intention with a formal range declaration.</scos:note>
</rdf:Property>

<rdf:Property rdf:about="&ncal;standard"
    rdfs:label="standard">
  <nrl:maxCardinality rdf:datatype="&xsd;integer">1</nrl:maxCardinality>
  <rdfs:comment>Links the timezone with the standard timezone observance. This property has no direct equivalent in the RFC 2445. It has been inspired by the structure of the Vtimezone component defined in sec.4.6.5</rdfs:comment>
  <rdfs:domain rdf:resource="&ncal;Timezone"/>
  <rdfs:range rdf:resource="&ncal;TimezoneObservance"/>
</rdf:Property>

<ncal:CalendarScale rdf:about="&ncal;gregorianCalendarScale"
    rdfs:label="gregorianCalendarScale"/>

<rdf:Property rdf:about="&nexif;exposureProgram"
    rdfs:label="exposureProgram">
  <rdfs:subPropertyOf rdf:resource="http://www.kanzaki.com/ns/exif#exposureProgram"/>
  <rdfs:subPropertyOf rdf:resource="&nexif;pictTaking"/>
  <rdfs:comment>tagNumber: 34850
The class of the program used by the camera to set exposure when the picture is taken.</rdfs:comment>
  <rdfs:domain rdf:resource="&nexif;Photo"/>
  <rdfs:range rdf:resource="&xsd;string"/>
</rdf:Property>

<rdf:Property rdf:about="&dcterms;created">
  <rdfs:subPropertyOf rdf:resource="&dc;date"/>
  <rdfs:subPropertyOf rdf:resource="&dcterms;date"/>
  <dcterms:hasVersion rdf:resource="http://dublincore.org/usage/terms/history/#created-003"/>
  <dcterms:issued rdf:datatype="&xsd;date">2000-07-11</dcterms:issued>
  <dcterms:modified rdf:datatype="&xsd;date">2008-01-14</dcterms:modified>
  <rdfs:comment xml:lang="en">Date of creation of the resource.</rdfs:comment>
  <rdfs:isDefinedBy rdf:resource="&dcterms;"/>
  <rdfs:label xml:lang="en">Date Created</rdfs:label>
  <rdfs:range rdf:resource="&rdfs;Literal"/>
</rdf:Property>

<ncal:AlarmAction rdf:about="&ncal;audioAction"
    rdfs:label="audioAction"/>

<rdf:Property rdf:about="&rdfs;member">
  <rdfs:comment xml:lang="en">A member of the subject resource.</rdfs:comment>
  <rdfs:domain rdf:resource="&rdfs;Resource"/>
  <rdfs:isDefinedBy rdf:resource="&rdfs;"/>
  <rdfs:label xml:lang="en">member</rdfs:label>
  <rdfs:range rdf:resource="&rdfs;Resource"/>
</rdf:Property>

<rdf:Property rdf:about="&nid3;timestampFormat"
    rdfs:label="timestampFormat">
  <rdfs:comment>Time stamp format is: 
$01 Absolute time, 32 bit sized, using MPEG frames as unit
$02 Absolute time, 32 bit sized, using milliseconds as unit</rdfs:comment>
  <rdfs:domain rdf:resource="&nid3;SynchronizedText"/>
  <rdfs:range rdf:resource="&xsd;string"/>
</rdf:Property>

<ncal:TimeTransparency rdf:about="&ncal;transparentTransparency"
    rdfs:label="transparentTransparency"/>

<rdf:Property rdf:about="&ncal;bydayModifier"
    rdfs:label="bydayModifier">
  <nrl:maxCardinality rdf:datatype="&xsd;integer">1</nrl:maxCardinality>
  <rdfs:comment>An integer modifier for the BYDAY rule part.    Each BYDAY value can also be preceded by a positive (+n) or negative  (-n) integer. If present, this indicates the nth occurrence of the specific day within the MONTHLY or YEARLY RRULE. For example, within a MONTHLY rule, +1MO (or simply 1MO) represents the first Monday within the month, whereas -1MO represents the last Monday of the month. If an integer modifier is not present, it means all days of this type within the specified frequency. For example, within a MONTHLY rule, MO represents all Mondays within the month. Inspired by RFC 2445 sec. 4.3.10</rdfs:comment>
  <rdfs:domain rdf:resource="&ncal;BydayRulePart"/>
  <rdfs:range rdf:resource="&xsd;integer"/>
</rdf:Property>

<tmo:Urgency rdf:about="&tmo;TMO_Instance_Urgency_03"
    rdfs:label="TMO_Instance_Urgency_03"/>

<tmo:PersonInvolvementRole rdf:about="&tmo;TMO_Instance_PersonInvolvementRole_Analyst"
    rdfs:label="TMO_Instance_PersonInvolvementRole_Analyst"/>

<rdf:Property rdf:about="&nco;end"
    rdfs:label="end">
  <nrl:maxCardinality rdf:datatype="&xsd;integer">1</nrl:maxCardinality>
  <rdfs:comment>End datetime for the role, such as: the datetime of leaving a project or organization, datetime of ending employment, datetime of divorce. If absent or set to a date in the future, the role is currently active.</rdfs:comment>
  <rdfs:domain rdf:resource="&nco;Role"/>
  <rdfs:range rdf:resource="&xsd;dateTime"/>
</rdf:Property>

<rdf:Property rdf:about="&dcon;hasContextAttribute"
    rdfs:label="has Context Attribute">
  <rdfs:comment>Amongst other static attributes, context elements (or rather, their observations) have various context-related attributes, i.e. attributes which are bound to a particular time and context. This generic property links this type of attributes to the elements' observations, and is not intended for direct use. Instead, specific subproperties are provided for each supported element type. In order for observations to inherit these subproperties, each needs to be typed according to the element's type (see note in dcon:Observation comment).</rdfs:comment>
  <rdfs:domain rdf:resource="&dcon;Observation"/>
</rdf:Property>

<rdfs:Class rdf:about="&dctypes;Software">
  <dcam:memberOf rdf:resource="&dcterms;DCMIType"/>
  <dcterms:description xml:lang="en">Examples include a C source file, MS-Windows .exe executable, or Perl script.</dcterms:description>
  <dcterms:hasVersion rdf:resource="http://dublincore.org/usage/terms/history/#Software-003"/>
  <dcterms:issued rdf:datatype="&xsd;date">2000-07-11</dcterms:issued>
  <dcterms:modified rdf:datatype="&xsd;date">2008-01-14</dcterms:modified>
  <rdfs:comment xml:lang="en">A computer program in source or compiled form.</rdfs:comment>
  <rdfs:isDefinedBy rdf:resource="&dctypes;"/>
  <rdfs:label xml:lang="en">Software</rdfs:label>
</rdfs:Class>

<ncal:TodoStatus rdf:about="&ncal;needsActionStatus"
    rdfs:label="needsActionStatus"/>

<rdf:Property rdf:about="&duho;timestamp"
    rdfs:comment="The time of creation for the Log."
    rdfs:label="Timestamp">
  <rdfs:domain rdf:resource="&duho;Log"/>
  <rdfs:range rdf:resource="&xsd;dateTime"/>
  <rdfs:subPropertyOf rdf:resource="&nao;created"/>
</rdf:Property>

<rdf:Property rdf:about="&nao;isTopicOf"
    rdfs:label="is topic of">
  <nrl:inverseProperty rdf:resource="&nao;hasTopic"/>
  <rdfs:comment>Defines a relationship between two resources, where the subject is a topic of the object</rdfs:comment>
  <rdfs:range rdf:resource="&rdfs;Resource"/>
  <rdfs:subPropertyOf rdf:resource="&nao;isRelated"/>
</rdf:Property>

<rdf:Property rdf:about="&nmm;setNumber"
    rdfs:comment="The part of a set the audio came from."
    rdfs:label="set number">
  <nrl:maxCardinality rdf:datatype="&xsd;integer">1</nrl:maxCardinality>
  <rdfs:domain rdf:resource="&nmm;MusicPiece"/>
  <rdfs:range rdf:resource="&xsd;integer"/>
</rdf:Property>

<rdf:Property rdf:about="&nexif;exposureIndex"
    rdfs:label="exposureIndex">
  <rdfs:subPropertyOf rdf:resource="http://www.kanzaki.com/ns/exif#exposureIndex"/>
  <rdfs:subPropertyOf rdf:resource="&nexif;pictTaking"/>
  <rdfs:comment>The exposure index selected on the camera or input device at the time the image is captured.
tagNumber: 41493</rdfs:comment>
  <rdfs:domain rdf:resource="&nexif;Photo"/>
  <rdfs:range rdf:resource="&xsd;float"/>
</rdf:Property>

<rdfs:Class rdf:about="&ncal;Trigger"
    rdfs:label="Trigger">
  <rdfs:comment>An alarm trigger. This class has been created to serve as the range of ncal:trigger property. See the documentation for ncal:trigger for more details.</rdfs:comment>
  <rdfs:subClassOf rdf:resource="&rdfs;Resource"/>
</rdfs:Class>

<nrl:TransitiveProperty rdf:about="&dplo;hasRepost"
    rdfs:label="has repost">
  <nrl:inverseProperty rdf:resource="&dplo;repostOf"/>
  <rdf:type rdf:resource="&rdf;Property"/>
  <rdfs:comment>Links to the repost(s) of a livepost. This property is transitive, and is the inverse of dlpo:repostOf.</rdfs:comment>
  <rdfs:domain rdf:resource="&dplo;LivePost"/>
  <rdfs:range rdf:resource="&dplo;LivePost"/>
</nrl:TransitiveProperty>

<tmo:TaskState rdf:about="&tmo;TMO_Instance_TaskState_Suspended"
    rdfs:label="TMO_Instance_TaskState_Suspended"/>

<rdf:Property rdf:about="&nuao;totalUsageDuration"
    rdfs:comment="The total duration of all usages"
    rdfs:label="usage count">
  <nrl:maxCardinality rdf:datatype="&xsd;nonNegativeInteger">1</nrl:maxCardinality>
  <rdfs:domain rdf:resource="&rdfs;Resource"/>
  <rdfs:range rdf:resource="&xsd;duration"/>
  <rdfs:subPropertyOf rdf:resource="&nuao;totalEventDuration"/>
</rdf:Property>

<rdf:Property rdf:about="&nexif;focalLengthIn35mmFilm"
    rdfs:label="focalLengthIn35mmFilm">
  <rdfs:subPropertyOf rdf:resource="http://www.kanzaki.com/ns/exif#focalLengthIn35mmFilm"/>
  <rdfs:subPropertyOf rdf:resource="&nexif;length"/>
  <rdfs:subPropertyOf rdf:resource="&nexif;pictTaking"/>
  <rdfs:comment>The equivalent focal length assuming a 35mm film camera, in mm. A value of 0 means the focal length is unknown. Note that this tag differs from the FocalLength tag.
tagNumber: 41989</rdfs:comment>
  <rdfs:domain rdf:resource="&nexif;Photo"/>
  <rdfs:range rdf:resource="&xsd;integer"/>
</rdf:Property>

<rdf:Property rdf:about="&nfo;characterPosition"
    rdfs:comment="Character position of the bookmark."
    rdfs:label="characterPosition">
  <nrl:maxCardinality rdf:datatype="&xsd;integer">1</nrl:maxCardinality>
  <rdfs:domain rdf:resource="&nfo;Bookmark"/>
  <rdfs:range rdf:resource="&xsd;integer"/>
</rdf:Property>

<owl:NamedIndividual rdf:about="&oa;tagging">
  <rdf:type rdf:resource="&oa;Motivation"/>
  <rdfs:comment xml:lang="en">The motivation that represents adding a Tag on the target resource(s). One or more of the bodies of the annotation should be typed as a oa:Tag or oa:SemanticTag.</rdfs:comment>
  <scos:inScheme rdf:resource="&oa;motivationScheme"/>
  <scos:prefLabel xml:lang="en">tagging</scos:prefLabel>
</owl:NamedIndividual>

<rdf:Property rdf:about="&dcon;activeFile"
    rdfs:label="Active File">
  <rdfs:comment>Refers to active files (running on a device) characterising a context instance.</rdfs:comment>
  <rdfs:domain rdf:resource="&dcon;Attention"/>
  <rdfs:range rdf:resource="&nie;InformationElement"/>
  <rdfs:subPropertyOf rdf:resource="&dcon;hasContextElement"/>
</rdf:Property>

<rdf:Property rdf:about="&ncal;tzid"
    rdfs:label="tzid">
  <nrl:maxCardinality rdf:datatype="&xsd;integer">1</nrl:maxCardinality>
  <rdfs:comment>This property specifies the text value that uniquely identifies the "VTIMEZONE" calendar component. Inspired by RFC 2445 sec 4.8.3.1</rdfs:comment>
  <rdfs:domain rdf:resource="&ncal;Timezone"/>
  <rdfs:range rdf:resource="&xsd;string"/>
</rdf:Property>

<rdf:Property rdf:about="&nexif;colorSpace"
    rdfs:label="colorSpace">
  <rdfs:subPropertyOf rdf:resource="http://www.kanzaki.com/ns/exif#colorSpace"/>
  <rdfs:subPropertyOf rdf:resource="&nexif;imageDataCharacter"/>
  <rdfs:comment>tagNumber: 40961
The color space information tag (ColorSpace) is always recorded as the color space specifier. Normally sRGB (=1) is used to define the color space based on the PC monitor conditions and environment.</rdfs:comment>
  <rdfs:domain rdf:resource="&nexif;Photo"/>
  <rdfs:range rdf:resource="&xsd;string"/>
</rdf:Property>

<rdf:Property rdf:about="&nexif;gpsDateStamp"
    rdfs:label="gpsDateStamp">
  <rdfs:subPropertyOf rdf:resource="http://www.kanzaki.com/ns/exif#gpsDateStamp"/>
  <rdfs:subPropertyOf rdf:resource="&nexif;date"/>
  <rdfs:subPropertyOf rdf:resource="&nexif;gpsInfo"/>
  <rdfs:comment>tagNumber: 29
date and time information relative to UTC (Coordinated Universal Time). The record format is "YYYY:MM:DD" while converted to W3C-DTF to use in RDF</rdfs:comment>
  <rdfs:domain rdf:resource="&nexif;Photo"/>
  <rdfs:range rdf:resource="&xsd;dateTime"/>
</rdf:Property>

<rdf:Property rdf:about="&nexif;xResolution"
    rdfs:label="xResolution">
  <rdfs:subPropertyOf rdf:resource="http://www.kanzaki.com/ns/exif#xResolution"/>
  <rdfs:subPropertyOf rdf:resource="&nexif;imageDataStruct"/>
  <rdfs:subPropertyOf rdf:resource="&nexif;resolution"/>
  <rdfs:comment>The number of pixels per ResolutionUnit in the ImageWidth direction. When the image resolution is unknown, 72 [dpi] is designated.
tagNumber: 282</rdfs:comment>
  <rdfs:domain rdf:resource="&nexif;Photo"/>
  <rdfs:range rdf:resource="&xsd;float"/>
</rdf:Property>

<rdf:Property rdf:about="&nid3;internetRadioStationOwner"
    rdfs:label="internetRadioStationOwner">
  <rdfs:comment>TRSO
The 'Internet radio station owner' frame contains the name of the owner of the internet radio station from which the audio is streamed.</rdfs:comment>
  <rdfs:domain rdf:resource="&nid3;ID3Audio"/>
  <rdfs:range rdf:resource="&nco;Contact"/>
</rdf:Property>

<rdf:Property rdf:about="&ddo;isSecure"
    rdfs:label="is secure">
  <rdfs:comment>States whether the network is secure (requires some form of authentication) or otherwise.</rdfs:comment>
  <rdfs:domain rdf:resource="&ddo;Network"/>
  <rdfs:range rdf:resource="&xsd;boolean"/>
</rdf:Property>

<rdf:Property rdf:about="&dcon;negativeInstance"
    rdfs:label="Negative Instance">
  <rdfs:comment>Situations are characterised through a series of past live context instances, required for its training. This property points to one or more negative instances, i.e., past actual live contexts snapshots during which it was determined that the abstract situation was not active.</rdfs:comment>
  <rdfs:domain rdf:resource="&dcon;Situation"/>
  <rdfs:range rdf:resource="&duho;ContextLog"/>
</rdf:Property>

<rdf:Property rdf:about="&dpo;minPrecipitation"
    rdfs:label="Minimum Precipitation">
  <rdfs:comment>A subproperty of dpo:minValue that defines a lowerbound on the observed precipitation levels (in millimetres per hour) such that it can classify as a dpo:WeatherCondition instance. It can be used in conjunction with dpo:maxPrecipitation to state that specific instances of dpo:WeatherCondition have a pre-defined range of observable real-world precipitation levels. In addition, they can also be used with various other weather conditions values and ranges to define complex weather condition types.</rdfs:comment>
  <rdfs:domain rdf:resource="&dpo;WeatherConditions"/>
  <rdfs:range rdf:resource="&xsd;nonNegativeInteger"/>
  <rdfs:subPropertyOf rdf:resource="&dpo;minValue"/>
</rdf:Property>

<rdf:Property rdf:about="&scos;inScheme">
  <rdf:type rdf:resource="&owl;ObjectProperty"/>
  <rdfs:isDefinedBy rdf:resource="http://www.w3.org/2004/02/skos/core"/>
  <rdfs:label xml:lang="en">is in scheme</rdfs:label>
  <rdfs:range rdf:resource="&scos;ConceptScheme"/>
  <scos:definition xml:lang="en">Relates a resource (for example a concept) to a concept scheme in which it is included.</scos:definition>
  <scos:scopeNote xml:lang="en">A concept may be a member of more than one concept scheme.</scos:scopeNote>
</rdf:Property>

<rdf:Property rdf:about="&dcterms;abstract">
  <rdfs:subPropertyOf rdf:resource="&dc;description"/>
  <rdfs:subPropertyOf rdf:resource="&dcterms;description"/>
  <dcterms:hasVersion rdf:resource="http://dublincore.org/usage/terms/history/#abstract-003"/>
  <dcterms:issued rdf:datatype="&xsd;date">2000-07-11</dcterms:issued>
  <dcterms:modified rdf:datatype="&xsd;date">2008-01-14</dcterms:modified>
  <rdfs:comment xml:lang="en">A summary of the resource.</rdfs:comment>
  <rdfs:isDefinedBy rdf:resource="&dcterms;"/>
  <rdfs:label xml:lang="en">Abstract</rdfs:label>
</rdf:Property>

<rdf:Property rdf:about="&foaf;birthday"
    rdfs:label="birthday"
    ns:term_status="unstable">
  <rdf:type rdf:resource="&owl;DatatypeProperty"/>
  <rdf:type rdf:resource="&owl;FunctionalProperty"/>
  <rdfs:comment>The birthday of this Agent, represented in mm-dd string form, eg. '12-31'.</rdfs:comment>
  <rdfs:domain rdf:resource="&foaf;Agent"/>
  <rdfs:isDefinedBy rdf:resource="&foaf;"/>
  <rdfs:range rdf:resource="&rdfs;Literal"/>
</rdf:Property>

<rdf:Property rdf:about="&rdfs;comment">
  <rdfs:comment xml:lang="en">A description of the subject resource.</rdfs:comment>
  <rdfs:domain rdf:resource="&rdfs;Resource"/>
  <rdfs:isDefinedBy rdf:resource="&rdfs;"/>
  <rdfs:label xml:lang="en">comment</rdfs:label>
  <rdfs:range rdf:resource="&rdfs;Literal"/>
</rdf:Property>

<rdf:Property rdf:about="&nexif;imageConfig"
    rdfs:comment="An attribute relating to Image Configuration"
    rdfs:label="imageConfig">
  <rdfs:subPropertyOf rdf:resource="http://www.kanzaki.com/ns/exif#imageConfig"/>
  <rdfs:subPropertyOf rdf:resource="&nexif;exifAttribute"/>
  <rdfs:domain rdf:resource="&nexif;Photo"/>
  <rdfs:range rdf:resource="&xsd;string"/>
</rdf:Property>

<rdf:Property rdf:about="&nfo;bitrateType"
    rdfs:comment="The type of the bitrate. Examples may include CBR and VBR."
    rdfs:label="bitrateType">
  <nrl:maxCardinality rdf:datatype="&xsd;integer">1</nrl:maxCardinality>
  <rdfs:domain rdf:resource="&nfo;Media"/>
  <rdfs:range rdf:resource="&xsd;string"/>
</rdf:Property>

<rdf:Property rdf:about="&dpo;minBrightnessLevel"
    rdfs:label="Minimum Brightness Level">
  <rdfs:comment>A subproperty of dpo:minValue that defines an lowerbound on the observed brightness level value (in SI lux units) such that it can classify as a dpo:Brightness instance. It can be used in conjunction with dpo:maxBrightnessLevel, i.e. specific instances of dpo:Brightness have a pre-defined range of observable real-world surrounding brightness levels.</rdfs:comment>
  <rdfs:domain rdf:resource="&dpo;Brightness"/>
  <rdfs:range rdf:resource="&xsd;float"/>
  <rdfs:subPropertyOf rdf:resource="&dpo;minValue"/>
</rdf:Property>

<rdf:Property rdf:about="&nexif;meter"
    rdfs:comment="A length with unit of meter"
    rdfs:label="meter">
  <rdfs:subPropertyOf rdf:resource="http://www.kanzaki.com/ns/exif#meter"/>
  <rdfs:subPropertyOf rdf:resource="&nexif;length"/>
  <rdfs:domain rdf:resource="&nexif;Photo"/>
  <rdfs:range rdf:resource="&xsd;string"/>
</rdf:Property>

<rdf:Property rdf:about="&dcon;speed"
    rdfs:label="Speed Value">
  <rdfs:comment>States the actual speed value for a pre-defined user movemement range in the current context.</rdfs:comment>
  <rdfs:domain rdf:resource="&dpo;Movement"/>
  <rdfs:range rdf:resource="&xsd;float"/>
  <rdfs:subPropertyOf rdf:resource="&dcon;hasContextAttribute"/>
</rdf:Property>

<rdfs:Class rdf:about="&nie;InformationElement"
    rdfs:label="InformationElement">
  <rdfs:comment>A unit of content the user works with. This is a superclass for all interpretations of a DataObject.</rdfs:comment>
  <rdfs:subClassOf rdf:resource="&rdfs;Resource"/>
</rdfs:Class>

<rdfs:Class rdf:about="&nmo;IMMessage"
    rdfs:comment="A message sent with Instant Messaging software."
    rdfs:label="IMMessage">
  <rdfs:subClassOf rdf:resource="&nmo;Message"/>
</rdfs:Class>

<rdf:Property rdf:about="&foaf;based_near"
    rdfs:label="based near"
    ns:term_status="testing">
  <rdf:type rdf:resource="&owl;ObjectProperty"/>
  <rdfs:comment>A location that something is based near, for some broadly human notion of near.</rdfs:comment>
  <rdfs:domain rdf:resource="http://www.w3.org/2003/01/geo/wgs84_pos#SpatialThing"/>
  <rdfs:isDefinedBy rdf:resource="&foaf;"/>
  <rdfs:range rdf:resource="http://www.w3.org/2003/01/geo/wgs84_pos#SpatialThing"/>
</rdf:Property>

<rdf:Property rdf:about="&scos;mappingRelation">
  <rdf:type rdf:resource="&owl;ObjectProperty"/>
  <rdfs:comment xml:lang="en">These concept mapping relations mirror semantic relations, and the data model defined below is similar (with the exception of skos:exactMatch) to the data model defined for semantic relations. A distinct vocabulary is provided for concept mapping relations, to provide a convenient way to differentiate links within a concept scheme from links between concept schemes. However, this pattern of usage is not a formal requirement of the SKOS data model, and relies on informal definitions of best practice.</rdfs:comment>
  <rdfs:isDefinedBy rdf:resource="http://www.w3.org/2004/02/skos/core"/>
  <rdfs:label xml:lang="en">is in mapping relation with</rdfs:label>
  <rdfs:subPropertyOf rdf:resource="&scos;semanticRelation"/>
  <scos:definition xml:lang="en">Relates two concepts coming, by convention, from different schemes, and that have comparable meanings</scos:definition>
</rdf:Property>

<rdf:Property rdf:about="&nuao;eventCount"
    rdfs:comment="The total number of events"
    rdfs:label="event count">
  <nrl:maxCardinality rdf:datatype="&xsd;nonNegativeInteger">1</nrl:maxCardinality>
  <rdfs:domain rdf:resource="&rdfs;Resource"/>
  <rdfs:range rdf:resource="&xsd;nonNegativeInteger"/>
</rdf:Property>

<rdf:Property rdf:about="&nso;sharedThrough"
    rdfs:label="includes">
  <nrl:cardinality rdf:datatype="&xsd;nonNegativeInteger">1</nrl:cardinality>
  <rdfs:comment>Determines the means (exactly one, required) that enable the access regulation for an access space. The supported access mean needs to be an instance of a dao:Account (e.g. a personal online account).</rdfs:comment>
  <rdfs:domain rdf:resource="&nso;AccessSpace"/>
  <rdfs:range rdf:resource="&dao;Account"/>
</rdf:Property>

<rdf:Property rdf:about="&nrl;maxCardinality"
    rdfs:label="maxCardinality">
  <rdfs:comment>Specifies a maximum value cardinality for a specific property</rdfs:comment>
  <rdfs:domain rdf:resource="&rdf;Property"/>
  <rdfs:range rdf:resource="&rdfs;Literal"/>
</rdf:Property>

<rdfs:Class rdf:about="&nfo;CompressionType"
    rdfs:label="CompressionType">
  <rdfs:comment>Type of compression. Instances of this class represent the limited set of values allowed for the nfo:compressionType property.</rdfs:comment>
  <rdfs:subClassOf rdf:resource="&rdfs;Resource"/>
</rdfs:Class>

<rdf:Property rdf:about="&nid3;originalArtist"
    rdfs:label="originalArtist">
  <rdfs:comment>TOPE
The 'Original artist(s)/performer(s)' frame is intended for the performer(s) of the original recording, if for example the music in the file should be a cover of a previously released song. The performers are seperated with the "/" character.
Note that in the RDF repressentation each orignal artist is represented with a separate triple.</rdfs:comment>
  <rdfs:domain rdf:resource="&nid3;ID3Audio"/>
  <rdfs:range rdf:resource="&nco;Contact"/>
  <rdfs:subPropertyOf rdf:resource="&nco;creator"/>
</rdf:Property>

<rdfs:Class rdf:about="&rdfs;Container">
  <rdfs:comment xml:lang="en">The class of RDF containers.</rdfs:comment>
  <rdfs:isDefinedBy rdf:resource="&rdfs;"/>
  <rdfs:label xml:lang="en">Container</rdfs:label>
  <rdfs:subClassOf rdf:resource="&rdfs;Resource"/>
</rdfs:Class>

<rdfs:Class rdf:about="&ncal;JournalStatus"
    rdfs:label="JournalStatus">
  <rdfs:comment>A status of a journal entry. This class has been introduced to express
the limited set of values for the ncal:status property. The user may
use the instances provided with this ontology or create his/her own.
See the documentation for ncal:journalStatus for details.</rdfs:comment>
  <rdfs:subClassOf rdf:resource="&rdfs;Resource"/>
</rdfs:Class>

<rdfs:Class rdf:about="&nco;Hobby"
    rdfs:label="Hobby">
  <rdfs:comment>Instances of this class represent personal hobbies and interests.</rdfs:comment>
  <rdfs:subClassOf rdf:resource="&rdfs;Resource"/>
</rdfs:Class>

<dcam:VocabularyEncodingScheme rdf:about="&dcterms;MESH">
  <dcterms:hasVersion rdf:resource="http://dublincore.org/usage/terms/history/#MESH-003"/>
  <dcterms:issued rdf:datatype="&xsd;date">2000-07-11</dcterms:issued>
  <dcterms:modified rdf:datatype="&xsd;date">2008-01-14</dcterms:modified>
  <rdfs:comment xml:lang="en">The set of labeled concepts specified by the Medical Subject Headings.</rdfs:comment>
  <rdfs:isDefinedBy rdf:resource="&dcterms;"/>
  <rdfs:label xml:lang="en">MeSH</rdfs:label>
  <rdfs:seeAlso rdf:resource="http://www.nlm.nih.gov/mesh/meshhome.html"/>
</dcam:VocabularyEncodingScheme>

<rdf:Property rdf:about="&ncal;count"
    rdfs:label="count">
  <nrl:maxCardinality rdf:datatype="&xsd;integer">1</nrl:maxCardinality>
  <rdfs:comment>How many times should an event be repeated. Defined in RFC 2445 sec. 4.3.10</rdfs:comment>
  <rdfs:domain rdf:resource="&ncal;RecurrenceRule"/>
  <rdfs:range rdf:resource="&xsd;integer"/>
</rdf:Property>

<rdf:Property rdf:about="&tmo;dependencyMemberB"
    nrl:maxCardinality="1"
    nrl:minCardinality="1"
    rdfs:label="dependencyMemberB">
  <rdfs:subPropertyOf rdf:resource="&pimo;associationMember"/>
  <rdfs:subPropertyOf rdf:resource="&tmo;taskReference"/>
  <rdfs:comment>The semantic of this relation is defined in the sublclass of undirected Dependency on which this property is stated. (The subject of the statment where this property is expressed)</rdfs:comment>
  <rdfs:domain rdf:resource="&tmo;TaskDependency"/>
  <rdfs:range rdf:resource="&tmo;Task"/>
</rdf:Property>

<rdfs:Class rdf:about="&nfo;WebDataObject"
    rdfs:label="web data object">
  <rdfs:comment>An information resources of which representations (files, streams) can be retrieved through a web server. They may be generated at retrieval time. Typical examples are pages served by PHP or AJAX or mp3 streams.</rdfs:comment>
  <rdfs:subClassOf rdf:resource="&nie;DataObject"/>
</rdfs:Class>

<rdf:Property rdf:about="&nmm;albumGain"
    rdfs:comment="ReplayGain album(audiophile) gain"
    rdfs:label="album gain">
  <nrl:maxCardinality rdf:datatype="&xsd;integer">1</nrl:maxCardinality>
  <rdfs:domain rdf:resource="&nmm;MusicAlbum"/>
  <rdfs:range rdf:resource="&xsd;float"/>
</rdf:Property>

<rdfs:Class rdf:about="&dcon;Observation"
    rdfs:label="Observation">
  <rdfs:comment>Each context Element can have one or more observations, e.g. from different source or device. These are linked to each element through the dcon:hasObservation property. In order to inherit the context attributes relevant for the element's type, observations need to be multi-typed. For example, each observation of a nie:InformationElement must also be defined as a nie:InformationElement instance, so that it can inherit all context attributes having the element's type in their domain specification. However, this does not mean that an observation is also an element, but merely that it must have the same type. Other defining properties of an observation are the data source (dcon:recordedBy) and the observation time (dcon:recordedAt). A validity property (dcon:validity) is also provided, and is intended to regulate the time frame during which an observation is considered valid.</rdfs:comment>
</rdfs:Class>

<rdfs:Class rdf:about="&tmo;UndirectedDependency"
    rdfs:comment="A symmetric relations between task."
    rdfs:label="UndirectedDependency">
  <rdfs:subClassOf rdf:resource="&tmo;TaskDependency"/>
</rdfs:Class>

<rdf:Property rdf:about="&ncal;recurrenceId"
    rdfs:label="recurrenceId">
  <nrl:maxCardinality rdf:datatype="&xsd;integer">1</nrl:maxCardinality>
  <rdfs:comment>This property is used in conjunction with the "UID" and "SEQUENCE" property to identify a specific instance of a recurring "VEVENT", "VTODO" or "VJOURNAL" calendar component. The property value is the effective value of the "DTSTART" property of the recurrence instance. Inspired by the RFC 2445 sec. 4.8.4.4</rdfs:comment>
  <rdfs:domain rdf:resource="&ncal;UnionOfEventJournalTimezoneTodo"/>
  <rdfs:range rdf:resource="&ncal;RecurrenceIdentifier"/>
</rdf:Property>

<rdf:Property rdf:about="&nrl;hasSemantics"
    rdfs:label="hasSemantics">
  <rdfs:comment>Points to a representation of the declarative semantics for a graph role</rdfs:comment>
  <rdfs:domain rdf:resource="&nrl;Data"/>
  <rdfs:range rdf:resource="&nrl;Semantics"/>
</rdf:Property>

<rdfs:Class rdf:about="&ncal;CalendarDataObject"
    rdfs:label="CalendarDataObject">
  <rdfs:comment>A DataObject found in a calendar. It is usually interpreted as one of the calendar entity types (e.g. Event, Journal, Todo etc.)</rdfs:comment>
  <rdfs:subClassOf rdf:resource="&nie;DataObject"/>
</rdfs:Class>

<rdf:Property rdf:about="&ncal;byday"
    rdfs:label="byday">
  <rdfs:comment>Weekdays the recurrence should occur. Defined in RFC 2445 sec. 4.3.10</rdfs:comment>
  <rdfs:domain rdf:resource="&ncal;RecurrenceRule"/>
  <rdfs:range rdf:resource="&ncal;BydayRulePart"/>
</rdf:Property>

<ncal:ParticipationStatus rdf:about="&ncal;delegatedParticipationStatus"
    rdfs:label="delegatedParticipationStatus"/>

<rdf:Property rdf:about="&tmo;abilityCarrierRole"
    nrl:maxCardinality="1"
    nrl:minCardinality="1"
    rdfs:label="abilityCarrierRole">
  <rdfs:domain rdf:resource="&tmo;AbilityCarrierInvolvement"/>
  <rdfs:range rdf:resource="&tmo;AbilityCarrierRole"/>
  <rdfs:subPropertyOf rdf:resource="&tmo;stateTypeRole"/>
</rdf:Property>

<rdf:Property rdf:about="&nco;foafUrl"
    rdfs:comment="The URL of the FOAF file."
    rdfs:label="foafUrl">
  <rdfs:domain rdf:resource="&nco;Role"/>
  <rdfs:range rdf:resource="&rdfs;Resource"/>
  <rdfs:subPropertyOf rdf:resource="&nco;url"/>
</rdf:Property>

<rdf:Property rdf:about="&dcon;noiseLevel"
    rdfs:label="Noise Level Value">
  <rdfs:comment>Registers an actual environmental noise level value element attribute to an active noise level range in the current context.</rdfs:comment>
  <rdfs:domain rdf:resource="&dpo;Noise"/>
  <rdfs:range rdf:resource="&xsd;float"/>
  <rdfs:subPropertyOf rdf:resource="&dcon;hasContextAttribute"/>
</rdf:Property>

<rdf:Property rdf:about="&dcon;hasContextElement"
    rdfs:label="Has Context Element">
  <rdfs:comment>Context aspects categorise elements relating to the same category of context information. Individual context elements are linked to each aspect through this generic property, which is not intended for direct use. Instead, specific subproperties for each supported element is provided.</rdfs:comment>
  <rdfs:domain rdf:resource="&dcon;Aspect"/>
  <rdfs:range rdf:resource="&dcon;Element"/>
</rdf:Property>

<rdf:Property rdf:about="&nexif;componentsConfiguration"
    rdfs:label="componentsConfiguration">
  <rdfs:subPropertyOf rdf:resource="http://www.kanzaki.com/ns/exif#componentsConfiguration"/>
  <rdfs:subPropertyOf rdf:resource="&nexif;imageConfig"/>
  <rdfs:comment>Information specific to compressed data. The channels of each component are arranged in order from the 1st component to the 4th. For uncompressed data the data arrangement is given in the PhotometricInterpretation tag. However, since PhotometricInterpretation can only express the order of Y,Cb and Cr, this tag is provided for cases when compressed data uses components other than Y, Cb, and Cr and to enable support of other sequences.
tagNumber: 37121</rdfs:comment>
  <rdfs:domain rdf:resource="&nexif;Photo"/>
  <rdfs:range rdf:resource="&xsd;string"/>
</rdf:Property>

<rdfs:Class rdf:about="&nfo;BookmarkFolder"
    rdfs:label="Bookmark Folder">
  <rdfs:comment>A folder with bookmarks of a webbrowser. Use nfo:containsBookmark to relate Bookmarks. Folders can contain subfolders, use containsBookmarkFolder to relate them.</rdfs:comment>
  <rdfs:subClassOf rdf:resource="&nie;InformationElement"/>
</rdfs:Class>

<rdf:Property rdf:about="&nie;contentSize"
    nrl:maxCardinality="1"
    rdfs:label="contentSize">
  <rdfs:comment>The size of the content. This property can be used whenever the size of the content of an InformationElement differs from the size of the DataObject. (e.g. because of compression, encoding, encryption or any other representation issues). The contentSize in expressed in bytes.</rdfs:comment>
  <rdfs:domain rdf:resource="&nie;InformationElement"/>
  <rdfs:range rdf:resource="&xsd;integer"/>
</rdf:Property>

<nrl:TransitiveProperty rdf:about="&drmo;succeededBy"
    rdfs:label="succeeded by">
  <nrl:inverseProperty rdf:resource="&drmo;precededBy"/>
  <rdf:type rdf:resource="&rdf;Property"/>
  <rdfs:comment>TWO conditions (A and B) may be composed together using the succeededBy Property. If Condition A is succeeded by Condition B, the actions are only triggered if Condition B happens at any time after Condition A. This is the inverse property of drmo:precededBy.</rdfs:comment>
  <rdfs:domain rdf:resource="&drmo;Condition"/>
  <rdfs:range rdf:resource="&drmo;Condition"/>
</nrl:TransitiveProperty>

<rdfs:Class rdf:about="&dpo;Noise"
    rdfs:label="Noise">
  <rdfs:comment>Quantifiable presence components concerning the audible noise levels in the environment surrounding the agent.</rdfs:comment>
  <rdfs:subClassOf rdf:resource="&dpo;EnvironmentalIndicator"/>
</rdfs:Class>

<rdfs:Class rdf:about="&nrl;DiscardableInstanceBase"
    rdfs:label="DiscardableInstanceBase">
  <rdfs:comment>A named graph containing instance data that can be recreated by analyzing the original resources. Intended to be used by metadata extractors.</rdfs:comment>
  <rdfs:subClassOf rdf:resource="&nrl;InstanceBase"/>
</rdfs:Class>

<rdfs:Class rdf:about="&nco;ModemNumber"
    rdfs:label="ModemNumber">
  <rdfs:comment>A modem phone number. Inspired by the (TYPE=modem) parameter of the TEL property as defined in RFC 2426 sec  3.3.1.</rdfs:comment>
  <rdfs:subClassOf rdf:resource="&nco;PhoneNumber"/>
</rdfs:Class>

<rdf:Description rdf:about="&dc;">
  <dcterms:modified rdf:datatype="&xsd;date">2012-06-14</dcterms:modified>
  <dcterms:publisher rdf:resource="http://purl.org/dc/aboutdcmi#DCMI"/>
  <dcterms:title xml:lang="en">Dublin Core Metadata Element Set, Version 1.1</dcterms:title>
</rdf:Description>

<rdf:Property rdf:about="&nexif;pimBrightness"
    rdfs:comment="Brightness info for print image matching
tagNumber: 10"
    rdfs:label="pimBrightness">
  <rdfs:subPropertyOf rdf:resource="http://www.kanzaki.com/ns/exif#pimBrightness"/>
  <rdfs:subPropertyOf rdf:resource="&nexif;pimInfo"/>
  <rdfs:domain rdf:resource="&nexif;Photo"/>
  <rdfs:range rdf:resource="&xsd;string"/>
</rdf:Property>

<rdf:Property rdf:about="&rdfs;subClassOf">
  <rdfs:comment xml:lang="en">The subject is a subclass of a class.</rdfs:comment>
  <rdfs:domain rdf:resource="&rdfs;Class"/>
  <rdfs:isDefinedBy rdf:resource="&rdfs;"/>
  <rdfs:label xml:lang="en">subClassOf</rdfs:label>
  <rdfs:range rdf:resource="&rdfs;Class"/>
</rdf:Property>

<ncal:ParticipationStatus rdf:about="&ncal;inProcessParticipationStatus"
    rdfs:label="inProcessParticipationStatus"/>

<rdfs:Class rdf:about="&nfo;LocalFileDataObject"
    rdfs:label="local file">
  <rdfs:comment>A local file data object which is stored on a local file system. Its nie:url always uses the file:/ protocol. The main use of this class is to distinguish local and non-local files.</rdfs:comment>
  <rdfs:subClassOf rdf:resource="&nfo;FileDataObject"/>
</rdfs:Class>

<owl:Class rdf:about="&oa;SemanticTag">
  <rdfs:comment xml:lang="en">A class assigned to the Body when it is a semantic tagging resource; a URI that identifies a concept, rather than an embedded string, frequently a term from a controlled vocabulary.

It is NOT RECOMMENDED to use the URI of a document as a Semantic Tag, as it might also be used as a regular Body in other Annotations which would inherit the oa:SemanticTag class assignment. Instead it is more appropriate to create a new URI and link it to the document, using the foaf:page predicate.</rdfs:comment>
  <rdfs:isDefinedBy rdf:resource="&oa;"/>
  <rdfs:label xml:lang="en">SemanticTag</rdfs:label>
  <rdfs:subClassOf rdf:resource="&oa;Tag"/>
</owl:Class>

<rdfs:Class rdf:about="&duho;ContextLog"
    rdfs:label="Context Log">
  <rdfs:comment>A log that is used to document a specific type of resource: a user's changing context. Thus, it is meant to contain past instances, or snapshots, of dcon:Context from the Context Ontology (DCON).</rdfs:comment>
  <rdfs:subClassOf rdf:resource="&duho;Log"/>
</rdfs:Class>

<rdf:Property rdf:about="&ndo;copiedFrom"
    rdfs:label="copied from">
  <rdfs:comment>Links a DataObject with its copy. This relation means that originally the Data Objects were copies but might have changed subsequentially.</rdfs:comment>
  <rdfs:domain rdf:resource="&nie;DataObject"/>
  <rdfs:range rdf:resource="&nie;DataObject"/>
</rdf:Property>

<rdf:Property rdf:about="&ddo;owns"
    rdfs:label="owns">
  <rdfs:comment>Defines an ownership relationship between a person and a computerised device.</rdfs:comment>
  <rdfs:domain rdf:resource="&pimo;Person"/>
  <rdfs:range rdf:resource="&ddo;Device"/>
</rdf:Property>

<rdf:Property rdf:about="&tmo;involvedPerson"
    nrl:maxCardinality="1"
    nrl:minCardinality="1"
    rdfs:label="involvedPerson">
  <rdfs:domain rdf:resource="&tmo;PersonInvolvement"/>
  <rdfs:range rdf:resource="&pimo;Person"/>
  <rdfs:subPropertyOf rdf:resource="&pimo;associationMember"/>
</rdf:Property>

<rdf:Property rdf:about="&nfo;containsBookmarkFolder"
    rdfs:comment="The folder contains a bookmark folder."
    rdfs:label="contains folder">
  <rdfs:domain rdf:resource="&nfo;BookmarkFolder"/>
  <rdfs:range rdf:resource="&nfo;BookmarkFolder"/>
  <rdfs:subPropertyOf rdf:resource="&nie;hasLogicalPart"/>
</rdf:Property>

<rdfs:Class rdf:about="&ddo;Ethernet"
    rdfs:label="Ethernet">
  <rdfs:comment>A wired local area network enabling computerised devices to exchange streams of data.</rdfs:comment>
  <rdfs:subClassOf rdf:resource="&ddo;LocalAreaNetwork"/>
</rdfs:Class>

<rdf:Property rdf:about="&nuao;lastModification"
    rdfs:comment="The start time of the last modification"
    rdfs:label="last modification">
  <nrl:maxCardinality rdf:datatype="&xsd;nonNegativeInteger">1</nrl:maxCardinality>
  <rdfs:domain rdf:resource="&rdfs;Resource"/>
  <rdfs:range rdf:resource="&xsd;dateTime"/>
</rdf:Property>

<rdfs:Class rdf:about="&nso;AccessSpace"
    rdfs:label="Access Space">
  <rdfs:comment>A subclass of ppo:AccessSpace, this class enables the regulation of access to a space containing resources. Resource membership is still defined through the PPO properties, e.g. ppo:appliesToResource. However, within the context of this ontology, access is given to agents using the local nso:includes and nso:excludes relationships. In addition, multiple access spaces can be defined for a privacy preference, each regulating access to different agents through different access means (e.g. personal accounts). This relationship is defined using the nso:sharedThrough property.</rdfs:comment>
  <rdfs:subClassOf rdf:resource="http://vocab.deri.ie/ppo#AccessSpace"/>
</rdfs:Class>

<ncal:Weekday rdf:about="&ncal;friday"
    rdfs:label="friday"/>

<rdf:Property rdf:about="&scos;member">
  <rdf:type rdf:resource="&owl;ObjectProperty"/>
  <rdfs:domain rdf:resource="&scos;Collection"/>
  <rdfs:isDefinedBy rdf:resource="http://www.w3.org/2004/02/skos/core"/>
  <rdfs:label xml:lang="en">has member</rdfs:label>
  <rdfs:range>
    <owl:Class>
      <owl:unionOf rdf:parseType="Collection">
        <rdf:Description rdf:about="&scos;Concept"/>
        <rdf:Description rdf:about="&scos;Collection"/>
      </owl:unionOf>
    </owl:Class>
  </rdfs:range>
  <scos:definition xml:lang="en">Relates a collection to one of its members.</scos:definition>
</rdf:Property>

<rdfs:Class rdf:about="&ncal;AttendeeRole"
    rdfs:label="AttendeeRole">
  <rdfs:comment>A role the attendee is going to play during an event. This class has been introduced to express the limited vocabulary for the values of ncal:role property. Please refer to the documentation of ncal:role for details.</rdfs:comment>
  <rdfs:subClassOf rdf:resource="&rdfs;Resource"/>
</rdfs:Class>

<rdf:Property rdf:about="&dpo;minValue"
    rdfs:label="Minimum Value">
  <rdfs:comment>A subproperty of dpo:value defining a lowerbound on the value observed for a real-world entity for it to classify as an instance of a specific quantifiable presence component. Various subproperties are provided and apply to specific types of presence components.</rdfs:comment>
  <rdfs:domain rdf:resource="&dpo;QuantifiableComponent"/>
  <rdfs:subPropertyOf rdf:resource="&dpo;value"/>
</rdf:Property>

<rdf:Property rdf:about="&foaf;thumbnail"
    rdfs:comment="A derived thumbnail image."
    rdfs:label="thumbnail"
    ns:term_status="testing">
  <rdf:type rdf:resource="&owl;ObjectProperty"/>
  <rdfs:domain rdf:resource="&foaf;Image"/>
  <rdfs:isDefinedBy rdf:resource="&foaf;"/>
  <rdfs:range rdf:resource="&foaf;Image"/>
</rdf:Property>

<owl:Class rdf:about="&oa;Choice">
  <rdfs:comment xml:lang="en">A multiplicity construct that conveys to a consuming application that it should select one of the constituent resources to display to the user, and not render/use all of them. 

oa:Choice can be used as the object of the object of the oa:hasBody, oa:hasTarget, oa:hasSelector, oa:hasState, oa:styledBy and oa:hasScope relationships, 

There MUST be 1 or more oa:item relationships for each oa:Choice.

There SHOULD be exactly 1 default relationship for each Choice.</rdfs:comment>
  <rdfs:isDefinedBy rdf:resource="&oa;"/>
  <rdfs:label xml:lang="en">Choice</rdfs:label>
  <rdfs:subClassOf rdf:resource="&rdf;Alt"/>
</owl:Class>

<rdf:Property rdf:about="&rdf;type">
  <rdfs:comment xml:lang="en">The subject is an instance of a class.</rdfs:comment>
  <rdfs:domain rdf:resource="&rdfs;Resource"/>
  <rdfs:isDefinedBy rdf:resource="&rdf;"/>
  <rdfs:label xml:lang="en">type</rdfs:label>
  <rdfs:range rdf:resource="&rdfs;Class"/>
</rdf:Property>

<rdfs:Class rdf:about="&nco;IsdnNumber"
    rdfs:label="IsdnNumber">
  <rdfs:comment>An ISDN phone number. Inspired by the (TYPE=isdn) parameter of the TEL property as defined in RFC 2426 sec  3.3.1.</rdfs:comment>
  <rdfs:subClassOf rdf:resource="&nco;VoicePhoneNumber"/>
</rdfs:Class>

<dcam:VocabularyEncodingScheme rdf:about="&dcterms;TGN">
  <dcterms:hasVersion rdf:resource="http://dublincore.org/usage/terms/history/#TGN-003"/>
  <dcterms:issued rdf:datatype="&xsd;date">2000-07-11</dcterms:issued>
  <dcterms:modified rdf:datatype="&xsd;date">2008-01-14</dcterms:modified>
  <rdfs:comment xml:lang="en">The set of places specified by the Getty Thesaurus of Geographic Names.</rdfs:comment>
  <rdfs:isDefinedBy rdf:resource="&dcterms;"/>
  <rdfs:label xml:lang="en">TGN</rdfs:label>
  <rdfs:seeAlso rdf:resource="http://www.getty.edu/research/tools/vocabulary/tgn/index.html"/>
</dcam:VocabularyEncodingScheme>

<rdf:Property rdf:about="&dpo;maxTime"
    rdfs:label="Maximum Time">
  <rdfs:comment>A subproperty of dpo:maxValue that defines an upperbound on the observed time value (in xsd:time format) such that it can classify as a dpo:TimePeriod instance. It can be used in conjunction with dpo:minTime, i.e. specific instances of dpo:TimePeriod have a pre-defined range of observable time periods.</rdfs:comment>
  <rdfs:domain rdf:resource="&dpo;TimePeriod"/>
  <rdfs:range rdf:resource="&xsd;time"/>
  <rdfs:subPropertyOf rdf:resource="&dpo;maxValue"/>
</rdf:Property>

<tmo:TransmissionState rdf:about="&tmo;TMO_Instance_TransmissionState_Rejected_NotTransmitted"
    rdfs:label="TMO_Instance_TransmissionState_Rejected_NotTransmitted"/>

<rdf:Property rdf:about="&foaf;icqChatID"
    rdfs:comment="An ICQ chat ID"
    rdfs:label="ICQ chat ID"
    ns:term_status="testing">
  <rdf:type rdf:resource="&owl;DatatypeProperty"/>
  <rdf:type rdf:resource="&owl;InverseFunctionalProperty"/>
  <rdfs:domain rdf:resource="&foaf;Agent"/>
  <rdfs:isDefinedBy rdf:resource="&foaf;"/>
  <rdfs:range rdf:resource="&rdfs;Literal"/>
  <rdfs:subPropertyOf rdf:resource="&foaf;nick"/>
</rdf:Property>

<rdf:Property rdf:about="&nfo;containsBookmark"
    rdfs:comment="The folder contains a bookmark."
    rdfs:label="contains bookmark">
  <rdfs:domain rdf:resource="&nfo;BookmarkFolder"/>
  <rdfs:range rdf:resource="&nfo;Bookmark"/>
  <rdfs:subPropertyOf rdf:resource="&nie;hasLogicalPart"/>
</rdf:Property>

<rdf:Property rdf:about="&nao;numericRating"
    rdfs:label="numeric rating">
  <rdfs:subPropertyOf rdf:resource="&nao;rating"/>
  <rdfs:subPropertyOf rdf:resource="&nao;scoreParameter"/>
  <nrl:maxCardinality rdf:datatype="&xsd;nonNegativeInteger">1</nrl:maxCardinality>
  <rdfs:comment> Annotation for a resource in the form of a numeric rating (float value), allowed values are between 1 and 10 whereas 0 is interpreted as not set</rdfs:comment>
  <rdfs:domain rdf:resource="&rdfs;Resource"/>
  <rdfs:range rdf:resource="&xsd;integer"/>
</rdf:Property>

<rdf:Property rdf:about="&cnt;leadingMisc">
  <rdf:type rdf:resource="&owl;ObjectProperty"/>
  <rdfs:comment xml:lang="en">The XML content preceding the document type declaration.</rdfs:comment>
  <rdfs:domain rdf:resource="&cnt;ContentAsXML"/>
  <rdfs:label xml:lang="en">XML leading misc</rdfs:label>
  <rdfs:range rdf:resource="&rdfs;XMLLiteral"/>
</rdf:Property>

<rdf:Property rdf:about="&nfo;interlaceMode"
    rdfs:comment="True if the image is interlaced, false if not."
    rdfs:label="interlaceMode">
  <nrl:maxCardinality rdf:datatype="&xsd;integer">1</nrl:maxCardinality>
  <rdfs:domain rdf:resource="&nfo;Visual"/>
  <rdfs:range rdf:resource="&xsd;boolean"/>
</rdf:Property>

<rdf:Property rdf:about="&tmo;abilityCarrierTask"
    nrl:maxCardinality="1"
    rdfs:label="abilityCarrierTask">
  <nrl:inverseProperty rdf:resource="&tmo;abilityCarrierInvolvement"/>
  <rdfs:domain rdf:resource="&tmo;AbilityCarrierInvolvement"/>
  <rdfs:range rdf:resource="&tmo;Task"/>
  <rdfs:subPropertyOf rdf:resource="&pimo;associationMember"/>
</rdf:Property>

<rdf:Property rdf:about="&ncal;triggerDateTime"
    rdfs:label="triggerDateTime">
  <nrl:maxCardinality rdf:datatype="&xsd;integer">1</nrl:maxCardinality>
  <rdfs:comment>The exact date and time of the trigger. This property has been created to express the VALUE=DATE, and VALUE=DATE-TIME parameters of the TRIGGER property. See the documentation for ncal:trigger for more details</rdfs:comment>
  <rdfs:domain rdf:resource="&ncal;Trigger"/>
  <rdfs:range rdf:resource="&xsd;dateTime"/>
</rdf:Property>

<rdfs:Class rdf:about="&ncal;RecurrenceFrequency"
    rdfs:label="RecurrenceFrequency">
  <rdfs:comment>Frequency of a recurrence rule. This class has been introduced to express a limited set of allowed values for the ncal:freq property. See the documentation of ncal:freq for details.</rdfs:comment>
  <rdfs:subClassOf rdf:resource="&rdfs;Resource"/>
</rdfs:Class>

<rdf:Property rdf:about="&tmo;transmissionTo"
    nrl:maxCardinality="1"
    nrl:minCardinality="1"
    rdfs:label="transmissionTo">
  <rdfs:domain rdf:resource="&tmo;TaskTransmission"/>
  <rdfs:range rdf:resource="&pimo;Person"/>
</rdf:Property>

<rdf:Property rdf:about="&foaf;page"
    rdfs:comment="A page or document about this thing."
    rdfs:label="page"
    ns:term_status="stable">
  <rdf:type rdf:resource="&owl;ObjectProperty"/>
  <rdfs:domain rdf:resource="&owl;Thing"/>
  <rdfs:isDefinedBy rdf:resource="&foaf;"/>
  <rdfs:range rdf:resource="&foaf;Document"/>
  <owl:inverseOf rdf:resource="&foaf;topic"/>
</rdf:Property>

<nrl:DefiningProperty rdf:about="&nmm;cinematographer"
    rdfs:label="cinematographer">
  <rdf:type rdf:resource="&rdf;Property"/>
  <rdfs:domain rdf:resource="&nfo;Video"/>
  <rdfs:range rdf:resource="&nco;Contact"/>
  <rdfs:subPropertyOf rdf:resource="&nco;contributor"/>
</nrl:DefiningProperty>

<rdf:Property rdf:about="&foaf;currentProject"
    rdfs:comment="A current project this person works on."
    rdfs:label="current project"
    ns:term_status="testing">
  <rdf:type rdf:resource="&owl;ObjectProperty"/>
  <rdfs:domain rdf:resource="&foaf;Person"/>
  <rdfs:isDefinedBy rdf:resource="&foaf;"/>
  <rdfs:range rdf:resource="&owl;Thing"/>
</rdf:Property>

<tmo:TaskPrivacyState rdf:about="&tmo;TMO_Instance_TaskPrivacy_Private"
    rdfs:label="TMO_Instance_TaskPrivacy_Private"/>

<rdf:Property rdf:about="&nao;rating"
    rdfs:label="rating">
  <rdfs:comment>Annotation for a resource in the form of an unrestricted rating</rdfs:comment>
  <rdfs:domain rdf:resource="&rdfs;Resource"/>
  <rdfs:subPropertyOf rdf:resource="&nao;annotation"/>
</rdf:Property>

<rdfs:Class rdf:about="&drmo;ResourceCreated"
    rdfs:label="ResourceCreated">
  <rdfs:comment>Describes a condition which is triggered by a newly created resource in the PIM.</rdfs:comment>
  <rdfs:subClassOf rdf:resource="&drmo;Condition"/>
</rdfs:Class>

<rdfs:Resource rdf:about="&nie;DataSourceGraph"
    rdfs:label="Data Source Graph">
  <rdfs:comment>Represents the sum of all information that has been obtained from a data source. Each data source has its own personal information graph. When a data source is deleted, the graph becomes redundant and should also be deleted. If two or more items in two or more data source graphs are determined to be equivalent, they are integrated at the PIMO level, and the integrated representation plus the links to the original items are stored in the pimo:PersonalInformationModel graph.</rdfs:comment>
  <rdfs:subClassOf rdf:resource="&nrl;InstanceBase"/>
</rdfs:Resource>

<rdf:Property rdf:about="&nexif;relatedSoundFile"
    rdfs:comment="Related audio file
tagNumber: 40964"
    rdfs:label="relatedSoundFile">
  <rdfs:subPropertyOf rdf:resource="http://www.kanzaki.com/ns/exif#relatedSoundFile"/>
  <rdfs:subPropertyOf rdf:resource="&nexif;relatedFile"/>
  <rdfs:domain rdf:resource="&nexif;Photo"/>
  <rdfs:range rdf:resource="&xsd;string"/>
</rdf:Property>

<rdf:Property rdf:about="&dcterms;educationLevel">
  <dcterms:hasVersion rdf:resource="http://dublincore.org/usage/terms/history/#educationLevel-002"/>
  <dcterms:issued rdf:datatype="&xsd;date">2002-07-13</dcterms:issued>
  <dcterms:modified rdf:datatype="&xsd;date">2008-01-14</dcterms:modified>
  <rdfs:comment xml:lang="en">A class of entity, defined in terms of progression through an educational or training context, for which the described resource is intended.</rdfs:comment>
  <rdfs:isDefinedBy rdf:resource="&dcterms;"/>
  <rdfs:label xml:lang="en">Audience Education Level</rdfs:label>
  <rdfs:range rdf:resource="&dcterms;AgentClass"/>
  <rdfs:subPropertyOf rdf:resource="&dcterms;audience"/>
</rdf:Property>

<tmo:PersonInvolvementRole rdf:about="&tmo;TMO_Instance_PersonInvolvementRole_ExternalObserver"
    rdfs:label="TMO_Instance_PersonInvolvementRole_ExternalObserver"/>

<rdf:Property rdf:about="&ncal;priority"
    rdfs:label="priority">
  <nrl:maxCardinality rdf:datatype="&xsd;integer">1</nrl:maxCardinality>
  <rdfs:comment>The property defines the relative priority for a calendar component. Inspired by RFC 2445 sec. 4.8.1.9</rdfs:comment>
  <rdfs:domain rdf:resource="&ncal;UnionOfEventTodo"/>
  <rdfs:range rdf:resource="&xsd;integer"/>
</rdf:Property>

<rdf:Property rdf:about="&dcon;currentAltitude"
    rdfs:comment="States the current altitude (metres above sea level)"
    rdfs:label="Current Altitude">
  <rdfs:domain rdf:resource="&dcon;SpaTem"/>
  <rdfs:range rdf:resource="&dpo;Altitude"/>
  <rdfs:subPropertyOf rdf:resource="&dcon;hasContextElement"/>
</rdf:Property>

<tmo:Urgency rdf:about="&tmo;TMO_Instance_Urgency_01"
    rdfs:label="TMO_Instance_Urgency_01"/>

<nco:IMCapability rdf:about="&nco;imCapabilityText"/>

<rdf:Property rdf:about="&nfo;definesGlobalVariable"
    rdfs:label="definesGlobalVariable">
  <rdfs:comment>Name of a global variable defined within the source code file.</rdfs:comment>
  <rdfs:domain rdf:resource="&nfo;SourceCode"/>
  <rdfs:range rdf:resource="&xsd;string"/>
</rdf:Property>

<rdfs:Class rdf:about="&nco;AudioIMAccount"
    rdfs:comment="Deprecated in favour of nco:imCapabilityAudio."
    rdfs:label="AudioIMAccount">
  <nao:deprecated rdf:datatype="&xsd;boolean">true</nao:deprecated>
  <rdfs:subClassOf rdf:resource="&nco;IMAccount"/>
</rdfs:Class>

<rdf:Property rdf:about="&nmo;receivedDate"
    rdfs:comment="Date when this message was received."
    rdfs:label="receivedDate">
  <nrl:maxCardinality rdf:datatype="&xsd;integer">1</nrl:maxCardinality>
  <rdfs:domain rdf:resource="&nmo;Message"/>
  <rdfs:range rdf:resource="&xsd;dateTime"/>
  <rdfs:subPropertyOf rdf:resource="&dc;date"/>
</rdf:Property>

<rdf:Property rdf:about="&nid3;officialInternetRadioStationHomepage"
    rdfs:label="officialInternetRadioStationHomepage">
  <rdfs:comment>WORS
The 'Official internet radio station homepage' contains a URL pointing at the homepage of the internet radio station.</rdfs:comment>
  <rdfs:domain rdf:resource="&nid3;ID3Audio"/>
  <rdfs:range rdf:resource="&rdfs;Resource"/>
</rdf:Property>

<rdf:Property rdf:about="&ncal;location"
    rdfs:label="location">
  <nrl:maxCardinality rdf:datatype="&xsd;integer">1</nrl:maxCardinality>
  <rdfs:comment>Defines the intended venue for the activity defined by a calendar component. Inspired by RFC 2445 sec 4.8.1.7 with the following reservations:  the LANGUAGE parameter has been discarded. Please use xml:lang literals to express language.  For the ALTREP parameter use the locationAltRep property.</rdfs:comment>
  <rdfs:domain rdf:resource="&ncal;UnionOfEventTodo"/>
  <rdfs:range rdf:resource="&xsd;string"/>
</rdf:Property>

<rdf:Property rdf:about="&nid3;recordingDate"
    rdfs:label="recordingDate">
  <rdfs:comment>TRDA
The 'Recording dates' frame is a intended to be used as complement to the "TYER", "TDAT" and "TIME" frames. E.g. "4th-7th June, 12th June" in combination with the "TYER" frame.</rdfs:comment>
  <rdfs:domain rdf:resource="&nid3;ID3Audio"/>
  <rdfs:range rdf:resource="&xsd;string"/>
</rdf:Property>

<rdf:Property rdf:about="&foaf;weblog"
    rdfs:label="weblog"
    ns:term_status="stable">
  <rdf:type rdf:resource="&owl;InverseFunctionalProperty"/>
  <rdf:type rdf:resource="&owl;ObjectProperty"/>
  <rdfs:comment>A weblog of some thing (whether person, group, company etc.).</rdfs:comment>
  <rdfs:domain rdf:resource="&foaf;Agent"/>
  <rdfs:isDefinedBy rdf:resource="&foaf;"/>
  <rdfs:range rdf:resource="&foaf;Document"/>
  <rdfs:subPropertyOf rdf:resource="&foaf;page"/>
</rdf:Property>

<rdf:Property rdf:about="&nid3;userDefinedFrame"
    rdfs:comment="Links the ID3 file to a user-defined frame."
    rdfs:label="userDefinedFrame">
  <rdfs:domain rdf:resource="&nid3;ID3Audio"/>
  <rdfs:range rdf:resource="&nid3;UserDefinedFrame"/>
</rdf:Property>

<rdfs:Class rdf:about="&tmo;Attachment"
    rdfs:label="Attachment">
  <rdfs:subClassOf rdf:resource="&pimo;Association"/>
  <rdfs:subClassOf rdf:resource="&rdfs;Resource"/>
  <rdfs:comment>By means of attachments, references to other resources can be established. Resources are information objects. Every Thing, which can be referenced, on the SSD is an information object. In contrast to the usual SSD references/associations, here additionally information can be specified. Further metadata about the role an attachment plays can be stated by means of instances of AttachmentRole. It can be expressed what the Role of attachment is e.g., regarding "desired/requested" or "required" or "potentially useful / somehow related" or "used/produced/achieved". The reference property models the actual link to the attached piece of information.</rdfs:comment>
</rdfs:Class>

<nrl:DefiningProperty rdf:about="&nmm;director"
    rdfs:comment="Director"
    rdfs:label="director">
  <rdf:type rdf:resource="&rdf;Property"/>
  <rdfs:domain rdf:resource="&nfo;Video"/>
  <rdfs:range rdf:resource="&nco;Contact"/>
  <rdfs:subPropertyOf rdf:resource="&nco;contributor"/>
</nrl:DefiningProperty>

<rdf:Property rdf:about="&nco;blogUrl"
    rdfs:comment="A Blog url."
    rdfs:label="blogUrl">
  <rdfs:domain rdf:resource="&nco;Role"/>
  <rdfs:range rdf:resource="&rdfs;Resource"/>
  <rdfs:subPropertyOf rdf:resource="&nco;url"/>
</rdf:Property>

<rdf:Property rdf:about="&nrl;ruleLanguage"
    rdfs:label="ruleLanguage">
  <rdfs:comment>Specifies the rule language for a view specification that is driven by rules</rdfs:comment>
  <rdfs:domain rdf:resource="&nrl;RuleViewSpecification"/>
  <rdfs:range rdf:resource="&rdfs;Literal"/>
</rdf:Property>

<rdf:Property rdf:about="&nuao;start"
    rdfs:comment="The time of the start of the event"
    rdfs:label="start time">
  <nrl:maxCardinality rdf:datatype="&xsd;nonNegativeInteger">1</nrl:maxCardinality>
  <rdfs:domain rdf:resource="&nuao;Event"/>
  <rdfs:range rdf:resource="&xsd;dateTime"/>
</rdf:Property>

<tmo:TaskState rdf:about="&tmo;TMO_Instance_TaskState_Running"
    rdfs:label="TMO_Instance_TaskState_Running"/>

<rdf:Property rdf:about="&ncal;dtstamp"
    rdfs:label="dtstamp">
  <nrl:maxCardinality rdf:datatype="&xsd;integer">1</nrl:maxCardinality>
  <rdfs:comment>The property indicates the date/time that the instance of the iCalendar object was created. Inspired by RFC 2445 sec. 4.8.7.1. Note that the RFC allows ONLY UTC values for this property.</rdfs:comment>
  <rdfs:domain rdf:resource="&ncal;UnionOfEventFreebusyJournalTodo"/>
  <rdfs:range rdf:resource="&xsd;dateTime"/>
</rdf:Property>

<rdf:Property rdf:about="&ncal;dateTime"
    rdfs:label="dateTime">
  <nrl:maxCardinality rdf:datatype="&xsd;integer">1</nrl:maxCardinality>
  <rdfs:comment>Representation of a date an instance of NcalDateTime actually refers to. It's purpose is to express values in DATE-TIME datatype, as defined in RFC 2445 sec. 4.3.5</rdfs:comment>
  <rdfs:domain rdf:resource="&ncal;NcalDateTime"/>
  <rdfs:range rdf:resource="&xsd;dateTime"/>
</rdf:Property>

<rdf:Property rdf:about="&dcterms;temporal">
  <rdfs:subPropertyOf rdf:resource="&dc;coverage"/>
  <rdfs:subPropertyOf rdf:resource="&dcterms;coverage"/>
  <dcterms:hasVersion rdf:resource="http://dublincore.org/usage/terms/history/#temporal-003"/>
  <dcterms:issued rdf:datatype="&xsd;date">2000-07-11</dcterms:issued>
  <dcterms:modified rdf:datatype="&xsd;date">2008-01-14</dcterms:modified>
  <rdfs:comment xml:lang="en">Temporal characteristics of the resource.</rdfs:comment>
  <rdfs:isDefinedBy rdf:resource="&dcterms;"/>
  <rdfs:label xml:lang="en">Temporal Coverage</rdfs:label>
  <rdfs:range rdf:resource="&dcterms;PeriodOfTime"/>
</rdf:Property>

<rdf:Property rdf:about="&ncal;related"
    rdfs:label="related">
  <rdfs:comment>To specify the relationship of the alarm trigger with respect to the start or end of the calendar component. Inspired by RFC 2445 4.2.14. The RFC has specified two possible values for this property ('START' and 'END') they have been expressed as instances of the TriggerRelation class.</rdfs:comment>
  <rdfs:domain rdf:resource="&ncal;Trigger"/>
  <rdfs:range rdf:resource="&ncal;TriggerRelation"/>
</rdf:Property>

<rdf:Property rdf:about="&nao;hasDefaultNamespace"
    rdfs:comment="Defines the default static namespace for a graph"
    rdfs:label="has default namespace">
  <nrl:maxCardinality rdf:datatype="&xsd;nonNegativeInteger">1</nrl:maxCardinality>
  <rdfs:domain rdf:resource="&nrl;Data"/>
  <rdfs:range rdf:resource="&rdfs;Literal"/>
  <rdfs:subPropertyOf rdf:resource="&nao;annotation"/>
</rdf:Property>

<ncal:ParticipationStatus rdf:about="&ncal;tentativeParticipationStatus"
    rdfs:label="tentativeParticipationStatus"/>

<rdf:Property rdf:about="&nao;lastModified"
    rdfs:comment="States the last modification time for a resource"
    rdfs:label="last modified at">
  <nrl:maxCardinality rdf:datatype="&xsd;nonNegativeInteger">1</nrl:maxCardinality>
  <rdfs:domain rdf:resource="&rdfs;Resource"/>
  <rdfs:range rdf:resource="&xsd;dateTime"/>
  <rdfs:subPropertyOf rdf:resource="&nao;modified"/>
</rdf:Property>

<tmo:TransmissionState rdf:about="&tmo;TMO_Instance_TransmissionState_NotTransmitted"
    rdfs:label="TMO_Instance_TransmissionState_NotTransmitted"/>

<owl:ObjectProperty rdf:about="&oa;cachedSource">
  <rdfs:comment xml:lang="en">A link to a copy of the Source resource's representation appropriate for the Annotation, typically a copy of the original at the time that the Annotation was created</rdfs:comment>
  <rdfs:domain rdf:resource="&oa;TimeState"/>
  <rdfs:isDefinedBy rdf:resource="&oa;"/>
  <rdfs:label xml:lang="en">cachedSource</rdfs:label>
</owl:ObjectProperty>

<nrl:Graph rdf:about="&nrl;DefaultGraph"
    rdfs:label="DefaultGraph">
  <rdfs:comment>Represents the default graph, the graph which contains any triple that does not belong to any other named graph</rdfs:comment>
</nrl:Graph>

<rdf:Property rdf:about="&pimo;attendee"
    rdfs:comment="A social event is attended by a person."
    rdfs:label="attendee">
  <nrl:inverseProperty rdf:resource="&pimo;attends"/>
  <rdfs:domain rdf:resource="&pimo;SocialEvent"/>
  <rdfs:range rdf:resource="&pimo;Person"/>
  <rdfs:subPropertyOf rdf:resource="&pimo;isRelated"/>
</rdf:Property>

<rdf:Property rdf:about="&nie;generatorOption"
    rdfs:label="generatorOption">
  <rdfs:comment>A common superproperty for all settings used by the generating software. This may include compression settings, algorithms, autosave, interlaced/non-interlaced etc. Note that this property has no range specified and therefore should not be used directly. Always use more specific properties.</rdfs:comment>
  <rdfs:domain rdf:resource="&nie;InformationElement"/>
</rdf:Property>

<nrl:DefiningProperty rdf:about="&nfo;hasHash"
    rdfs:comment="Links the file with it's hash value."
    rdfs:label="hasHash">
  <nao:userVisible rdf:datatype="&xsd;boolean">false</nao:userVisible>
  <rdf:type rdf:resource="&rdf;Property"/>
  <rdfs:domain rdf:resource="&nfo;FileDataObject"/>
  <rdfs:range rdf:resource="&nfo;FileHash"/>
</nrl:DefiningProperty>

<rdfs:Class rdf:about="&nco;InternationalDeliveryAddress"
    rdfs:label="InternationalDeliveryAddress">
  <rdfs:comment>International Delivery Addresse. Class inspired by TYPE=intl parameter of the ADR property defined in RFC 2426 sec. 3.2.1</rdfs:comment>
  <rdfs:subClassOf rdf:resource="&nco;PostalAddress"/>
</rdfs:Class>

<rdf:Property rdf:about="&pimo;memberOf"
    rdfs:label="member of group">
  <nrl:inverseProperty rdf:resource="&pimo;hasMember"/>
  <rdfs:comment>This property can be used to organise agents within groups. Supplemented with an inverse property.</rdfs:comment>
  <rdfs:domain rdf:resource="&pimo;Agent"/>
  <rdfs:range rdf:resource="&pimo;PersonGroup"/>
  <rdfs:subPropertyOf rdf:resource="&pimo;partOf"/>
</rdf:Property>

<rdf:Property rdf:about="&nexif;interoperabilityVersion"
    rdfs:comment="tagNumber: 2
Interoperability Version"
    rdfs:label="interoperabilityVersion">
  <rdfs:subPropertyOf rdf:resource="http://www.kanzaki.com/ns/exif#interoperabilityVersion"/>
  <rdfs:subPropertyOf rdf:resource="&nexif;interopInfo"/>
  <rdfs:domain rdf:resource="&nexif;Photo"/>
  <rdfs:range rdf:resource="&xsd;string"/>
</rdf:Property>

<rdf:Property rdf:about="&dcterms;conformsTo">
  <rdfs:subPropertyOf rdf:resource="&dc;relation"/>
  <rdfs:subPropertyOf rdf:resource="&dcterms;relation"/>
  <dcterms:hasVersion rdf:resource="http://dublincore.org/usage/terms/history/#conformsTo-003"/>
  <dcterms:issued rdf:datatype="&xsd;date">2001-05-21</dcterms:issued>
  <dcterms:modified rdf:datatype="&xsd;date">2008-01-14</dcterms:modified>
  <rdfs:comment xml:lang="en">An established standard to which the described resource conforms.</rdfs:comment>
  <rdfs:isDefinedBy rdf:resource="&dcterms;"/>
  <rdfs:label xml:lang="en">Conforms To</rdfs:label>
  <rdfs:range rdf:resource="&dcterms;Standard"/>
</rdf:Property>

<rdf:Property rdf:about="&nexif;digitalZoomRatio"
    rdfs:label="digitalZoomRatio">
  <rdfs:subPropertyOf rdf:resource="http://www.kanzaki.com/ns/exif#digitalZoomRatio"/>
  <rdfs:subPropertyOf rdf:resource="&nexif;pictTaking"/>
  <rdfs:comment>tagNumber: 41988
The digital zoom ratio when the image was shot. If the numerator of the recorded value is 0, this indicates that digital zoom was not used.</rdfs:comment>
  <rdfs:domain rdf:resource="&nexif;Photo"/>
  <rdfs:range rdf:resource="&xsd;float"/>
</rdf:Property>

<rdf:Property rdf:about="&tmo;taskState"
    nrl:maxCardinality="1"
    nrl:minCardinality="1"
    rdfs:label="taskState">
  <rdfs:comment>The task state describes the current state of the task as described in Section 5.2.7.</rdfs:comment>
  <rdfs:domain rdf:resource="&tmo;Task"/>
  <rdfs:range rdf:resource="&tmo;TaskState"/>
  <rdfs:subPropertyOf rdf:resource="&tmo;stateTypeRole"/>
</rdf:Property>

<nfo:EncryptionStatus rdf:about="&nfo;encryptedStatus"
    rdfs:label="EncryptedStatus"/>

<rdfs:Class rdf:about="&dcterms;AgentClass">
  <dcterms:description xml:lang="en">Examples of Agent Class include groups seen as classes, such as students, women, charities, lecturers.</dcterms:description>
  <dcterms:hasVersion rdf:resource="http://dublincore.org/usage/terms/history/#AgentClass-003"/>
  <dcterms:issued rdf:datatype="&xsd;date">2008-01-14</dcterms:issued>
  <dcterms:modified rdf:datatype="&xsd;date">2012-06-14</dcterms:modified>
  <rdfs:comment xml:lang="en">A group of agents.</rdfs:comment>
  <rdfs:isDefinedBy rdf:resource="&dcterms;"/>
  <rdfs:label xml:lang="en">Agent Class</rdfs:label>
  <rdfs:subClassOf rdf:resource="&rdfs;Class"/>
</rdfs:Class>

<owl:DatatypeProperty rdf:about="&oa;styleClass">
  <rdfs:comment xml:lang="en">The string name of the class used in the CSS description that should be applied to the Specific Resource.

There MAY be 0 or more styleClass properties on a Specific Resource.

See oa:CssStyle.</rdfs:comment>
  <rdfs:domain rdf:resource="&oa;SpecificResource"/>
  <rdfs:isDefinedBy rdf:resource="&oa;"/>
  <rdfs:label xml:lang="en">styleClass</rdfs:label>
</owl:DatatypeProperty>

<rdfs:Class rdf:about="&nfo;Icon"
    rdfs:label="Icon">
  <rdfs:comment>An Icon (regardless of whether it's a raster or a vector icon. A resource representing an icon could have two types (Icon and Raster, or Icon and Vector) if required.</rdfs:comment>
  <rdfs:subClassOf rdf:resource="&nfo;Image"/>
</rdfs:Class>

<rdfs:Class rdf:about="&ncal;BydayRulePart"
    rdfs:label="BydayRulePart">
  <rdfs:comment>Expresses the compound value of a byday part of a recurrence rule. It stores the weekday and the integer modifier. Inspired by RFC 2445 sec. 4.3.10</rdfs:comment>
  <rdfs:subClassOf rdf:resource="&rdfs;Resource"/>
</rdfs:Class>

<nrl:DefiningProperty rdf:about="&nie;isLogicalPartOf"
    rdfs:label="isLogicalPartOf">
  <nrl:inverseProperty rdf:resource="&nie;hasLogicalPart"/>
  <rdf:type rdf:resource="&rdf;Property"/>
  <rdfs:comment>Generic property used to express 'logical' containment relationships between DataObjects. NIE extensions are encouraged to provide more specific subproperties of this one. It is advisable for actual instances of InformationElement to use those specific subproperties. Note the difference between 'physical' containment (isPartOf) and logical containment (isLogicalPartOf)</rdfs:comment>
  <rdfs:domain rdf:resource="&nie;InformationElement"/>
  <rdfs:range rdf:resource="&nie;InformationElement"/>
  <rdfs:subPropertyOf rdf:resource="&dcterms;isPartOf"/>
</nrl:DefiningProperty>

<rdf:Property rdf:about="&nid3;originalReleaseYear"
    rdfs:label="originalReleaseYear">
  <rdfs:comment>TORY
The 'Original release year' frame is intended for the year when the original recording, if for example the music in the file should be a cover of a previously released song, was released. The field is formatted as in the "TYER" frame.</rdfs:comment>
  <rdfs:domain rdf:resource="&nid3;ID3Audio"/>
  <rdfs:range rdf:resource="&xsd;integer"/>
</rdf:Property>

<rdf:Property rdf:about="&nco;postalcode"
    rdfs:label="postalcode">
  <nrl:maxCardinality rdf:datatype="&xsd;integer">1</nrl:maxCardinality>
  <rdfs:comment>Postal Code. Inspired by the sixth part of the value of the 'ADR' property as defined in RFC 2426, sec. 3.2.1</rdfs:comment>
  <rdfs:domain rdf:resource="&nco;PostalAddress"/>
  <rdfs:range rdf:resource="&xsd;string"/>
</rdf:Property>

<rdf:Property rdf:about="&nfo;definesClass"
    rdfs:comment="Name of a class defined in the source code file."
    rdfs:label="definesClass">
  <rdfs:domain rdf:resource="&nfo;SourceCode"/>
  <rdfs:range rdf:resource="&xsd;string"/>
</rdf:Property>

<rdf:Property rdf:about="&nao;hasTag"
    rdfs:comment="Defines an existing tag for a resource"
    rdfs:label="has tag">
  <nrl:inverseProperty rdf:resource="&nao;isTagFor"/>
  <rdfs:domain rdf:resource="&rdfs;Resource"/>
  <rdfs:range rdf:resource="&nao;Tag"/>
  <rdfs:subPropertyOf rdf:resource="&nao;annotation"/>
</rdf:Property>

<rdfs:Class rdf:about="&dpo;Movement"
    rdfs:label="Movement">
  <rdfs:comment>Quantifiable presence information concerning the agent's sensed speed of movement.</rdfs:comment>
  <rdfs:subClassOf rdf:resource="&dpo;QuantifiableComponent"/>
</rdfs:Class>

<rdf:Property rdf:about="&nexif;pimSaturation"
    rdfs:comment="tagNumber: 12
Saturation info for print image matching"
    rdfs:label="pimSaturation">
  <rdfs:subPropertyOf rdf:resource="http://www.kanzaki.com/ns/exif#pimSaturation"/>
  <rdfs:subPropertyOf rdf:resource="&nexif;pimInfo"/>
  <rdfs:domain rdf:resource="&nexif;Photo"/>
  <rdfs:range rdf:resource="&xsd;string"/>
</rdf:Property>

<tmo:PersonInvolvementRole rdf:about="&tmo;TMO_Instance_PersonInvolvementRole_Observer"
    rdfs:label="TMO_Instance_PersonInvolvementRole_Observer"/>

<rdf:Property rdf:about="&pimo;attends"
    rdfs:comment="A person attends a social event."
    rdfs:label="attends event">
  <nrl:inverseProperty rdf:resource="&pimo;attendee"/>
  <rdfs:domain rdf:resource="&pimo;Person"/>
  <rdfs:range rdf:resource="&pimo;SocialEvent"/>
  <rdfs:subPropertyOf rdf:resource="&pimo;isRelated"/>
</rdf:Property>

<rdf:Property rdf:about="&cnt;dtDecl">
  <rdf:type rdf:resource="&owl;ObjectProperty"/>
  <rdfs:comment xml:lang="en">The document type declaration.</rdfs:comment>
  <rdfs:domain rdf:resource="&cnt;ContentAsXML"/>
  <rdfs:label xml:lang="en">Document type declaration</rdfs:label>
  <rdfs:range rdf:resource="&cnt;DoctypeDecl"/>
</rdf:Property>

<rdf:Property rdf:about="&nie;informationElementDate"
    rdfs:label="informationElementDate">
  <rdfs:comment>A point or period of time associated with an event in the lifecycle of an Information Element. A common superproperty for all date-related properties of InformationElements in the NIE Framework.</rdfs:comment>
  <rdfs:domain rdf:resource="&nie;InformationElement"/>
  <rdfs:range rdf:resource="&xsd;dateTime"/>
  <rdfs:subPropertyOf rdf:resource="&dc;date"/>
</rdf:Property>

<rdf:Property rdf:about="&dc;source">
  <dcterms:description xml:lang="en">The described resource may be derived from the related resource in whole or in part. Recommended best practice is to identify the related resource by means of a string conforming to a formal identification system.</dcterms:description>
  <dcterms:hasVersion rdf:resource="http://dublincore.org/usage/terms/history/#source-006"/>
  <dcterms:issued rdf:datatype="&xsd;date">1999-07-02</dcterms:issued>
  <dcterms:modified rdf:datatype="&xsd;date">2008-01-14</dcterms:modified>
  <rdfs:comment xml:lang="en">A related resource from which the described resource is derived.</rdfs:comment>
  <rdfs:isDefinedBy rdf:resource="&dc;"/>
  <rdfs:label xml:lang="en">Source</rdfs:label>
  <scos:note xml:lang="en">A second property with the same name as this property has been declared in the dcterms: namespace (http://purl.org/dc/terms/).  See the Introduction to the document "DCMI Metadata Terms" (http://dublincore.org/documents/dcmi-terms/) for an explanation.</scos:note>
</rdf:Property>

<rdf:Property rdf:about="&nfo;duration"
    rdfs:comment="Duration of a media piece."
    rdfs:label="duration">
  <nrl:maxCardinality rdf:datatype="&xsd;integer">1</nrl:maxCardinality>
  <rdfs:domain rdf:resource="&nfo;Media"/>
  <rdfs:range rdf:resource="&xsd;duration"/>
</rdf:Property>

<rdfs:Class rdf:about="&foaf;Group"
    rdfs:comment="A class of Agents."
    rdfs:label="Group"
    ns:term_status="stable">
  <rdf:type rdf:resource="&owl;Class"/>
  <rdfs:subClassOf rdf:resource="&foaf;Agent"/>
</rdfs:Class>

<rdf:Property rdf:about="&nmo;messageHeader"
    rdfs:comment="Links the message with an arbitrary message header."
    rdfs:label="messageHeader">
  <rdfs:domain rdf:resource="&nmo;Message"/>
  <rdfs:range rdf:resource="&nmo;MessageHeader"/>
</rdf:Property>

<rdf:Property rdf:about="&dpo;minSnowfallDegree"
    rdfs:label="Minimum Snowfall Degree">
  <rdfs:comment>A subproperty of dpo:minValue that defines a lowerbound on the observed snowfall (in millimetres per hour) such that it can classify as a dpo:WeatherCondition instance. It can be used in conjunction with dpo:maxSnowfallDegree to state that specific instances of dpo:WeatherCondition have a pre-defined range of observable real-world snowfall levels. In addition, they can also be used with various other weather conditions values and ranges to define complex weather condition types.</rdfs:comment>
  <rdfs:domain rdf:resource="&dpo;WeatherConditions"/>
  <rdfs:range rdf:resource="&xsd;nonNegativeInteger"/>
  <rdfs:subPropertyOf rdf:resource="&dpo;minValue"/>
</rdf:Property>

<rdf:Property rdf:about="&ncal;summary"
    rdfs:label="summary">
  <rdfs:comment>Defines a short summary or subject for the calendar component. Inspired by RFC 2445 sec 4.8.1.12 with the following reservations: the LANGUAGE parameter has been discarded. Please use xml:lang literals to express language. For the ALTREP parameter use the summaryAltRep property.</rdfs:comment>
  <rdfs:domain rdf:resource="&ncal;UnionOfAlarmEventJournalTodo"/>
  <rdfs:range rdf:resource="&xsd;string"/>
</rdf:Property>

<rdf:Property rdf:about="&dcterms;dateAccepted">
  <rdfs:subPropertyOf rdf:resource="&dc;date"/>
  <rdfs:subPropertyOf rdf:resource="&dcterms;date"/>
  <dcterms:description xml:lang="en">Examples of resources to which a Date Accepted may be relevant are a thesis (accepted by a university department) or an article (accepted by a journal).</dcterms:description>
  <dcterms:hasVersion rdf:resource="http://dublincore.org/usage/terms/history/#dateAccepted-002"/>
  <dcterms:issued rdf:datatype="&xsd;date">2002-07-13</dcterms:issued>
  <dcterms:modified rdf:datatype="&xsd;date">2008-01-14</dcterms:modified>
  <rdfs:comment xml:lang="en">Date of acceptance of the resource.</rdfs:comment>
  <rdfs:isDefinedBy rdf:resource="&dcterms;"/>
  <rdfs:label xml:lang="en">Date Accepted</rdfs:label>
  <rdfs:range rdf:resource="&rdfs;Literal"/>
</rdf:Property>

<rdfs:Class rdf:about="&pimo;Room"
    rdfs:label="Room">
  <rdfs:comment>A properPart of a Building which is separated from the exterior of the Building and/or other Rooms of the Building by walls. Some Rooms may have a specific purpose, e.g. sleeping, bathing, cooking, entertainment, etc. (Definition from SUMO).</rdfs:comment>
  <rdfs:subClassOf rdf:resource="&pimo;Location"/>
</rdfs:Class>

<rdf:Property rdf:about="&nmm;releaseDate"
    rdfs:comment="The date the media was released."
    rdfs:label="release date">
  <nrl:maxCardinality rdf:datatype="&xsd;integer">1</nrl:maxCardinality>
  <rdfs:domain rdf:resource="&nfo;Media"/>
  <rdfs:range rdf:resource="&xsd;dateTime"/>
  <rdfs:subPropertyOf rdf:resource="&nie;informationElementDate"/>
</rdf:Property>

<rdf:Property rdf:about="&dcterms;isReferencedBy">
  <rdfs:subPropertyOf rdf:resource="&dc;relation"/>
  <rdfs:subPropertyOf rdf:resource="&dcterms;relation"/>
  <dcterms:hasVersion rdf:resource="http://dublincore.org/usage/terms/history/#isReferencedBy-003"/>
  <dcterms:issued rdf:datatype="&xsd;date">2000-07-11</dcterms:issued>
  <dcterms:modified rdf:datatype="&xsd;date">2008-01-14</dcterms:modified>
  <rdfs:comment xml:lang="en">A related resource that references, cites, or otherwise points to the described resource.</rdfs:comment>
  <rdfs:isDefinedBy rdf:resource="&dcterms;"/>
  <rdfs:label xml:lang="en">Is Referenced By</rdfs:label>
  <scos:note xml:lang="en">This term is intended to be used with non-literal values as defined in the DCMI Abstract Model (http://dublincore.org/documents/abstract-model/).  As of December 2007, the DCMI Usage Board is seeking a way to express this intention with a formal range declaration.</scos:note>
</rdf:Property>

<rdf:Property rdf:about="&nfo;uncompressedSize"
    rdfs:comment="Uncompressed size of the content of a compressed file."
    rdfs:label="uncompressedSize">
  <nrl:maxCardinality rdf:datatype="&xsd;integer">1</nrl:maxCardinality>
  <rdfs:domain rdf:resource="&nfo;Archive"/>
  <rdfs:range rdf:resource="&xsd;integer"/>
</rdf:Property>

<rdfs:Class rdf:about="&ncal;Event"
    rdfs:label="Event">
  <rdfs:subClassOf rdf:resource="&nie;InformationElement"/>
  <rdfs:subClassOf rdf:resource="&ncal;UnionOfAlarmEventFreebusyJournalTodo"/>
  <rdfs:subClassOf rdf:resource="&ncal;UnionOfAlarmEventFreebusyTodo"/>
  <rdfs:subClassOf rdf:resource="&ncal;UnionOfAlarmEventJournalTodo"/>
  <rdfs:subClassOf rdf:resource="&ncal;UnionOfAlarmEventTodo"/>
  <rdfs:subClassOf rdf:resource="&ncal;UnionOfEventFreebusy"/>
  <rdfs:subClassOf rdf:resource="&ncal;UnionOfEventFreebusyJournalTodo"/>
  <rdfs:subClassOf rdf:resource="&ncal;UnionOfEventJournalTimezoneTodo"/>
  <rdfs:subClassOf rdf:resource="&ncal;UnionOfEventJournalTodo"/>
  <rdfs:subClassOf rdf:resource="&ncal;UnionOfEventTodo"/>
  <rdfs:subClassOf rdf:resource="&ncal;UnionOfTimezoneObservanceEventFreebusyJournalTimezoneTodo"/>
  <rdfs:subClassOf rdf:resource="&ncal;UnionOfTimezoneObservanceEventFreebusyTimezoneTodo"/>
  <rdfs:subClassOf rdf:resource="&ncal;UnionOfTimezoneObservanceEventJournalTimezoneTodo"/>
  <rdfs:comment>Provide a grouping of component properties that describe an event.</rdfs:comment>
</rdfs:Class>

<tmo:AttachmentRole rdf:about="&tmo;TMO_Instance_AttachmentRole_Used"
    rdfs:label="TMO_Instance_AttachmentRole_Used"/>

<owl:DatatypeProperty rdf:about="&oa;exact">
  <rdfs:comment xml:lang="en">A copy of the text which is being selected, after normalization.

See oa:TextQuoteSelector.</rdfs:comment>
  <rdfs:domain rdf:resource="&oa;Selector"/>
  <rdfs:isDefinedBy rdf:resource="&oa;"/>
  <rdfs:label xml:lang="en">exact</rdfs:label>
</owl:DatatypeProperty>

<rdf:Property rdf:about="&dcon;stormdegree"
    rdfs:label="Storm Degree Value">
  <rdfs:comment>Registers an actual storm degree value element attribute to an active weather condition in the current context.</rdfs:comment>
  <rdfs:domain rdf:resource="&dpo;WeatherConditions"/>
  <rdfs:range rdf:resource="&xsd;nonNegativeInteger"/>
  <rdfs:subPropertyOf rdf:resource="&dcon;hasContextAttribute"/>
</rdf:Property>

<rdf:Property rdf:about="&dcterms;references">
  <rdfs:subPropertyOf rdf:resource="&dc;relation"/>
  <rdfs:subPropertyOf rdf:resource="&dcterms;relation"/>
  <dcterms:hasVersion rdf:resource="http://dublincore.org/usage/terms/history/#references-003"/>
  <dcterms:issued rdf:datatype="&xsd;date">2000-07-11</dcterms:issued>
  <dcterms:modified rdf:datatype="&xsd;date">2008-01-14</dcterms:modified>
  <rdfs:comment xml:lang="en">A related resource that is referenced, cited, or otherwise pointed to by the described resource.</rdfs:comment>
  <rdfs:isDefinedBy rdf:resource="&dcterms;"/>
  <rdfs:label xml:lang="en">References</rdfs:label>
  <scos:note xml:lang="en">This term is intended to be used with non-literal values as defined in the DCMI Abstract Model (http://dublincore.org/documents/abstract-model/).  As of December 2007, the DCMI Usage Board is seeking a way to express this intention with a formal range declaration.</scos:note>
</rdf:Property>

<rdf:Property rdf:about="&tmo;involvedPersons"
    rdfs:label="involvedPersons">
  <nrl:inverseProperty rdf:resource="&tmo;involvedPersonTask"/>
  <rdfs:domain rdf:resource="&tmo;Task"/>
  <rdfs:range rdf:resource="&tmo;PersonInvolvement"/>
</rdf:Property>

<rdfs:Class rdf:about="&nfo;HtmlDocument"
    rdfs:comment="A HTML document, may contain links to other files."
    rdfs:label="HtmlDocument">
  <rdfs:subClassOf rdf:resource="&nfo;PlainTextDocument"/>
</rdfs:Class>

<nfo:CompressionType rdf:about="&nfo;lossyCompressionType"
    rdfs:label="lossyCompressionType"/>

<rdf:Property rdf:about="&tmo;transmissionStateChangesTo"
    nrl:maxCardinality="1"
    rdfs:label="transmissionStateChangesTo">
  <rdfs:domain rdf:resource="&tmo;TransmissionState"/>
  <rdfs:range rdf:resource="&tmo;TransmissionState"/>
  <rdfs:subPropertyOf rdf:resource="&tmo;stateTypeRole"/>
</rdf:Property>

<rdf:Property rdf:about="&foaf;name"
    rdfs:comment="A name for some thing."
    rdfs:label="name"
    ns:term_status="testing">
  <rdf:type rdf:resource="&owl;DatatypeProperty"/>
  <rdfs:domain rdf:resource="&owl;Thing"/>
  <rdfs:isDefinedBy rdf:resource="&foaf;"/>
  <rdfs:range rdf:resource="&rdfs;Literal"/>
  <rdfs:subPropertyOf rdf:resource="&rdfs;label"/>
</rdf:Property>

<rdfs:Class rdf:about="&nrl;GraphMetadata"
    rdfs:label="GraphMetadata">
  <rdfs:comment>Represents a special named graph that contains metadata for another graph</rdfs:comment>
  <rdfs:subClassOf rdf:resource="&nrl;Data"/>
</rdfs:Class>

<rdf:Property rdf:about="&nexif;subSecTimeDigitized"
    rdfs:comment="tagNumber: 37522
DateTimeDigitized subseconds"
    rdfs:label="subSecTimeDigitized">
  <rdfs:subPropertyOf rdf:resource="http://www.kanzaki.com/ns/exif#subSecTimeDigitized"/>
  <rdfs:subPropertyOf rdf:resource="&nexif;dateAndOrTime"/>
  <rdfs:subPropertyOf rdf:resource="&nexif;subsecond"/>
  <rdfs:domain rdf:resource="&nexif;Photo"/>
  <rdfs:range rdf:resource="&xsd;string"/>
</rdf:Property>

<rdf:Property rdf:about="&nco;key"
    rdfs:label="key">
  <rdfs:comment>An encryption key attached to a contact. Inspired by the KEY property defined in RFC 2426 sec. 3.7.2</rdfs:comment>
  <rdfs:domain rdf:resource="&nco;Contact"/>
  <rdfs:range rdf:resource="&nie;DataObject"/>
  <rdfs:subPropertyOf rdf:resource="&nie;hasPart"/>
</rdf:Property>

<rdf:Property rdf:about="&dcon;nearbyPlace"
    rdfs:label="Nearby Place">
  <rdfs:range rdf:resource="&pimo;Location"/>
  <rdfs:range rdf:resource="&dpo;Place"/>
  <rdfs:comment>Refers to a nearby place type or specific location that characterises a context instance.</rdfs:comment>
  <rdfs:domain rdf:resource="&dcon;SpaTem"/>
  <rdfs:subPropertyOf rdf:resource="&dcon;hasContextElement"/>
</rdf:Property>

<rdf:Property rdf:about="&nid3;fileOwner"
    rdfs:label="fileOwner">
  <rdfs:comment>TOWN
The 'File owner/licensee' frame contains the name of the owner or licensee of the file and it's contents.</rdfs:comment>
  <rdfs:range rdf:resource="&nco;Contact"/>
  <rdfs:subPropertyOf rdf:resource="&dc;rights"/>
</rdf:Property>

<rdf:Property rdf:about="&nfo;aspectRatio"
    rdfs:comment="Visual content aspect ratio. (Width divided by Height)"
    rdfs:label="aspectRatio">
  <nrl:maxCardinality rdf:datatype="&xsd;integer">1</nrl:maxCardinality>
  <rdfs:domain rdf:resource="&nfo;Visual"/>
  <rdfs:range rdf:resource="&xsd;float"/>
</rdf:Property>

<rdfs:Class rdf:about="&nao;Party"
    rdfs:comment="Represents a single or a group of individuals"
    rdfs:label="party">
  <rdfs:subClassOf rdf:resource="&rdfs;Resource"/>
</rdfs:Class>

<rdfs:Class rdf:about="&nfo;PaginatedTextDocument"
    rdfs:label="PaginatedTextDocument">
  <rdfs:comment>A file containing a text document, that is unambiguously divided into pages. Examples might include PDF, DOC, PS, DVI etc.</rdfs:comment>
  <rdfs:subClassOf rdf:resource="&nfo;TextDocument"/>
</rdfs:Class>

<rdfs:Class rdf:about="&dctypes;Service">
  <dcam:memberOf rdf:resource="&dcterms;DCMIType"/>
  <dcterms:description xml:lang="en">Examples include a photocopying service, a banking service, an authentication service, interlibrary loans, a Z39.50 or Web server.</dcterms:description>
  <dcterms:hasVersion rdf:resource="http://dublincore.org/usage/terms/history/#Service-003"/>
  <dcterms:issued rdf:datatype="&xsd;date">2000-07-11</dcterms:issued>
  <dcterms:modified rdf:datatype="&xsd;date">2008-01-14</dcterms:modified>
  <rdfs:comment xml:lang="en">A system that provides one or more functions.</rdfs:comment>
  <rdfs:isDefinedBy rdf:resource="&dctypes;"/>
  <rdfs:label xml:lang="en">Service</rdfs:label>
</rdfs:Class>

<rdfs:Class rdf:about="&nid3;InvolvedPerson"
    rdfs:label="InvolvedPerson">
  <rdfs:comment>Since there might be a lot of people contributing to an audio file in various ways, such as musicians and technicians, the 'Text information frames' are often insufficient to list everyone involved in a project. The 'Involved people list' is a frame containing the names of those involved, and how they were involved. The body simply contains a terminated string with the involvement directly followed by a terminated string with the involvee followed by a new involvement and so on. There may only be one "IPLS" frame in each tag.
Note that in this RDF representation each InvolvedPerson is represented with a separate instance of the InvolvedPerson class and with a separate involvedPerson triple.</rdfs:comment>
  <rdfs:subClassOf rdf:resource="&rdfs;Resource"/>
</rdfs:Class>

<rdfs:Class rdf:about="&nco;Name"
    rdfs:label="Name">
  <rdfs:comment>A class representing a contact's name. Possesses various attributes.</rdfs:comment>
  <rdfs:subClassOf rdf:resource="&rdfs;Resource"/>
</rdfs:Class>

<rdfs:Class rdf:about="&dcon;Situation"
    rdfs:label="Situation">
  <rdfs:comment>This class represents one or more interpreted user states. A user situation refers to a generalised context graph that is derived from the merging of a number of positive and negative previous live context instances. These instances are linked though dcon:positiveInstance and dcon:negativeInstance. Unlike live context, situations are independent of time and have the possibility to recur. As opposed to live context, situations are also independent of devices and are instead user-centric.</rdfs:comment>
  <rdfs:subClassOf rdf:resource="&dcon;Context"/>
</rdfs:Class>

<rdf:Property rdf:about="&nco;nameHonorificSuffix"
    rdfs:label="nameHonorificSuffix">
  <rdfs:comment>A suffix for the name of the Object represented by the given object. See documentation for the 'nameFamily' for details.</rdfs:comment>
  <rdfs:domain rdf:resource="&nco;PersonName"/>
  <rdfs:range rdf:resource="&xsd;string"/>
</rdf:Property>

<rdf:Property rdf:about="&pimo;isTagFor"
    rdfs:label="is tag for">
  <rdfs:subPropertyOf rdf:resource="&nao;isTagFor"/>
  <rdfs:subPropertyOf rdf:resource="&pimo;objectProperty"/>
  <nrl:inverseProperty rdf:resource="&pimo;hasTag"/>
  <rdfs:comment>This thing is described further in the object thing. Similar  semantics as skos:isSubjectOf.</rdfs:comment>
  <rdfs:domain rdf:resource="&pimo;Tag"/>
  <rdfs:range rdf:resource="&pimo;Thing"/>
</rdf:Property>

<rdfs:Class rdf:about="&ncal;EventStatus"
    rdfs:label="EventStatus">
  <rdfs:comment>A status of an event. This class has been introduced to express
the limited set of values for the ncal:status property. The user may
use the instances provided with this ontology or create his/her own.
See the documentation for ncal:eventStatus for details.</rdfs:comment>
  <rdfs:subClassOf rdf:resource="&rdfs;Resource"/>
</rdfs:Class>

<rdf:Property rdf:about="&ncal;wkst"
    rdfs:label="wkst">
  <nrl:maxCardinality rdf:datatype="&xsd;integer">1</nrl:maxCardinality>
  <rdfs:comment>The day that's counted as the start of the week. It is used to disambiguate the byweekno rule. Defined in RFC 2445 sec. 4.3.10</rdfs:comment>
  <rdfs:domain rdf:resource="&ncal;RecurrenceRule"/>
  <rdfs:range rdf:resource="&ncal;Weekday"/>
</rdf:Property>

<ncal:CalendarUserType rdf:about="&ncal;unknownUserType"
    rdfs:label="unknownUserType"/>

<tmo:AbilityCarrierRole rdf:about="&tmo;TMO_Instance_AbilityCarrierRole_Requested"
    rdfs:label="TMO_Instance_AbilityCarrierRole_Requested"/>

<rdf:Property rdf:about="&foaf;firstName"
    rdfs:comment="The first name of a person."
    rdfs:label="firstName"
    ns:term_status="testing">
  <rdf:type rdf:resource="&owl;DatatypeProperty"/>
  <rdfs:domain rdf:resource="&foaf;Person"/>
  <rdfs:isDefinedBy rdf:resource="&foaf;"/>
  <rdfs:range rdf:resource="&rdfs;Literal"/>
</rdf:Property>

<owl:Class rdf:about="&oa;Selector">
  <rdfs:comment xml:lang="en">A resource which describes the segment of interest in a representation of a Source resource, indicated with oa:hasSelector from the Specific Resource. 

This class is not used directly in Annotations, only its subclasses are.

The nature of the Selector will be dependent on the type of the representation for which the segment is conveyed. The specific type of selector should be indicated using a subclass of oa:Selector.

The Specifier's description MAY be conveyed as an external or embedded resource (cnt:Content), or as RDF properties within the graph. The description SHOULD use existing standards whenever possible. If the Specifier has an HTTP URI, then its description, and only its description, MUST be returned when the URI is dereferenced.</rdfs:comment>
  <rdfs:isDefinedBy rdf:resource="&oa;"/>
  <rdfs:label xml:lang="en">Selector</rdfs:label>
</owl:Class>

<rdfs:Datatype rdf:about="&dcterms;RFC3066">
  <dcterms:description xml:lang="en">RFC 3066 has been obsoleted by RFC 4646.</dcterms:description>
  <dcterms:hasVersion rdf:resource="http://dublincore.org/usage/terms/history/#RFC3066-002"/>
  <dcterms:issued rdf:datatype="&xsd;date">2002-07-13</dcterms:issued>
  <dcterms:modified rdf:datatype="&xsd;date">2008-01-14</dcterms:modified>
  <rdfs:comment xml:lang="en">The set of tags constructed according to RFC 3066 for the identification of languages.</rdfs:comment>
  <rdfs:isDefinedBy rdf:resource="&dcterms;"/>
  <rdfs:label xml:lang="en">RFC 3066</rdfs:label>
  <rdfs:seeAlso rdf:resource="http://www.ietf.org/rfc/rfc3066.txt"/>
</rdfs:Datatype>

<rdf:Property rdf:about="&nco;contactGroupName"
    rdfs:label="contactGroupName">
  <nrl:maxCardinality rdf:datatype="&xsd;integer">1</nrl:maxCardinality>
  <rdfs:comment>The name of the contact group. This property was NOT defined 
    in the VCARD standard. See documentation of the 'ContactGroup' class for 
    details</rdfs:comment>
  <rdfs:domain rdf:resource="&nco;ContactGroup"/>
  <rdfs:range rdf:resource="&xsd;string"/>
  <rdfs:subPropertyOf rdf:resource="&dc;title"/>
</rdf:Property>

<rdf:Property rdf:about="&foaf;interest"
    rdfs:comment="A page about a topic of interest to this person."
    rdfs:label="interest"
    ns:term_status="testing">
  <rdf:type rdf:resource="&owl;ObjectProperty"/>
  <rdfs:domain rdf:resource="&foaf;Agent"/>
  <rdfs:isDefinedBy rdf:resource="&foaf;"/>
  <rdfs:range rdf:resource="&foaf;Document"/>
</rdf:Property>

<rdf:Property rdf:about="&tmo;taskGoal"
    rdfs:label="taskGoal">
  <rdfs:domain rdf:resource="&tmo;Task"/>
  <rdfs:range rdf:resource="&rdfs;Resource"/>
</rdf:Property>

<tmo:TransmissionType rdf:about="&tmo;TMO_Instance_TransmissionType_Delegation"
    rdfs:label="TMO_Instance_TransmissionType_Delegation"/>

<rdf:Property rdf:about="&tmo;taskPrivacyState"
    nrl:maxCardinality="1"
    rdfs:label="taskPrivacyState">
  <rdfs:comment>For the separation between professional and private purpose of a task, this attribute provides with the values "professional/private" a high level separation of privacy in terms of setting distribution rights to other users for the task.
This separation may arise as a general Nepomuk issue and may therefore be handled in conjunction with a privacy preserving SSD architecture.</rdfs:comment>
  <rdfs:domain rdf:resource="&tmo;Task"/>
  <rdfs:range rdf:resource="&tmo;TaskPrivacyState"/>
  <rdfs:subPropertyOf rdf:resource="&tmo;stateTypeRole"/>
</rdf:Property>

<rdf:Property rdf:about="&nexif;gpsDestBearing"
    rdfs:label="gpsDestBearing">
  <rdfs:subPropertyOf rdf:resource="http://www.kanzaki.com/ns/exif#gpsDestBearing"/>
  <rdfs:subPropertyOf rdf:resource="&nexif;gpsInfo"/>
  <rdfs:comment>The bearing to the destination point. The range of values is from 0.00 to 359.99.
tagNumber: 24</rdfs:comment>
  <rdfs:domain rdf:resource="&nexif;Photo"/>
  <rdfs:range rdf:resource="&xsd;string"/>
</rdf:Property>

<rdfs:Class rdf:about="&pimo;PersonalInformationModel"
    rdfs:label="Personal Information Model">
  <rdfs:subClassOf rdf:resource="&nrl;KnowledgeBase"/>
  <rdfs:subClassOf rdf:resource="&rdfs;Resource"/>
  <rdfs:comment>A Personal Information Model (PIMO) of a user. Represents the sum of all information from the personal knowledge workspace (in literature also referred to as Personal Space of Information (PSI)) which a user needs for Personal Information Management (PIM).</rdfs:comment>
</rdfs:Class>

<rdf:Property rdf:about="&dcterms;language">
  <dcterms:description xml:lang="en">Recommended best practice is to use a controlled vocabulary such as RFC 4646 [RFC4646].</dcterms:description>
  <dcterms:hasVersion rdf:resource="http://dublincore.org/usage/terms/history/#languageT-001"/>
  <dcterms:issued rdf:datatype="&xsd;date">2008-01-14</dcterms:issued>
  <dcterms:modified rdf:datatype="&xsd;date">2008-01-14</dcterms:modified>
  <rdfs:comment xml:lang="en">A language of the resource.</rdfs:comment>
  <rdfs:isDefinedBy rdf:resource="&dcterms;"/>
  <rdfs:label xml:lang="en">Language</rdfs:label>
  <rdfs:range rdf:resource="&dcterms;LinguisticSystem"/>
  <rdfs:subPropertyOf rdf:resource="&dc;language"/>
</rdf:Property>

<rdf:Property rdf:about="&dcterms;rightsHolder">
  <dcterms:hasVersion rdf:resource="http://dublincore.org/usage/terms/history/#rightsHolder-002"/>
  <dcterms:issued rdf:datatype="&xsd;date">2004-06-14</dcterms:issued>
  <dcterms:modified rdf:datatype="&xsd;date">2008-01-14</dcterms:modified>
  <rdfs:comment xml:lang="en">A person or organization owning or managing rights over the resource.</rdfs:comment>
  <rdfs:isDefinedBy rdf:resource="&dcterms;"/>
  <rdfs:label xml:lang="en">Rights Holder</rdfs:label>
  <rdfs:range rdf:resource="&dcterms;Agent"/>
</rdf:Property>

<rdf:Property rdf:about="&ncal;rrule"
    rdfs:label="rrule">
  <rdfs:comment>This property defines a rule or repeating pattern for recurring events, to-dos, or time zone definitions. sec. 4.8.5.4</rdfs:comment>
  <rdfs:domain rdf:resource="&ncal;UnionOfTimezoneObservanceEventJournalTimezoneTodo"/>
  <rdfs:range rdf:resource="&ncal;RecurrenceRule"/>
</rdf:Property>

<rdf:Property rdf:about="&nie;legal"
    rdfs:label="legal">
  <rdfs:comment>A common superproperty for all properties that point at legal information about an Information Element</rdfs:comment>
  <rdfs:domain rdf:resource="&nie;InformationElement"/>
  <rdfs:range rdf:resource="&xsd;string"/>
  <rdfs:subPropertyOf rdf:resource="&dc;rights"/>
</rdf:Property>

<owl:Ontology rdf:about="&rdfs;">
  <dc:title xml:lang="en">The RDF Schema vocabulary (RDFS)</dc:title>
  <rdfs:seeAlso rdf:resource="http://www.w3.org/2000/01/rdf-schema-more"/>
</owl:Ontology>

<rdf:Property rdf:about="&nfo;originalLocation"
    rdfs:comment="The original location of the deleted resource."
    rdfs:label="originalLocation">
  <nrl:maxCardinality rdf:datatype="&xsd;integer">1</nrl:maxCardinality>
  <rdfs:domain rdf:resource="&nfo;DeletedResource"/>
  <rdfs:range rdf:resource="&xsd;string"/>
</rdf:Property>

<rdfs:Class rdf:about="&ncal;UnionOfTimezoneObservanceEventFreebusyTimezoneTodo"
    rdfs:label="UnionOfTimezoneObservanceEventFreebusyTimezoneTodo">
  <rdfs:subClassOf rdf:resource="&ncal;UnionParentClass"/>
</rdfs:Class>

<rdf:Property rdf:about="&nuao;initiatingAgent"
    rdfs:comment="Relates an event to the agent initiating the event."
    rdfs:label="initiating agent">
  <nrl:cardinality rdf:datatype="&xsd;nonNegativeInteger">1</nrl:cardinality>
  <rdfs:domain rdf:resource="&nuao;Event"/>
  <rdfs:range rdf:resource="&nao;Agent"/>
  <rdfs:subPropertyOf rdf:resource="&nuao;involves"/>
</rdf:Property>

<rdfs:Class rdf:about="&pimo;Attendee"
    rdfs:comment="The role of someone attending a social event."
    rdfs:label="Attendee">
  <rdfs:subClassOf rdf:resource="&pimo;PersonRole"/>
</rdfs:Class>

<rdfs:Class rdf:about="&nco;Contact"
    rdfs:label="Contact">
  <rdfs:subClassOf rdf:resource="&nie;InformationElement"/>
  <rdfs:subClassOf rdf:resource="&nco;Role"/>
  <rdfs:subClassOf rdf:resource="&nao;Party"/>
  <rdfs:comment>A Contact. A piece of data that can provide means to identify or communicate with an entity.</rdfs:comment>
</rdfs:Class>

<rdf:Property rdf:about="&nie;license"
    rdfs:label="license">
  <rdfs:subPropertyOf rdf:resource="&dcterms;license"/>
  <rdfs:subPropertyOf rdf:resource="&nie;legal"/>
  <rdfs:comment>Terms and intellectual property rights licensing conditions.</rdfs:comment>
  <rdfs:range rdf:resource="&xsd;string"/>
</rdf:Property>

<tmo:Importance rdf:about="&tmo;TMO_Instance_Importance_01"
    rdfs:label="TMO_Instance_Importance_01"/>

<rdf:Property rdf:about="&foaf;familyName"
    rdfs:comment="The family name of some person."
    rdfs:label="familyName"
    ns:term_status="testing">
  <rdf:type rdf:resource="&owl;DatatypeProperty"/>
  <rdfs:domain rdf:resource="&foaf;Person"/>
  <rdfs:isDefinedBy rdf:resource="&foaf;"/>
  <rdfs:range rdf:resource="&rdfs;Literal"/>
</rdf:Property>

<rdf:Property rdf:about="&nmo;sender"
    rdfs:comment="deprecated in favor of nmo:messageSender"
    rdfs:label="sender">
  <nao:deprecated rdf:datatype="&xsd;boolean">true</nao:deprecated>
  <rdfs:domain rdf:resource="&nmo;Message"/>
  <rdfs:range rdf:resource="&nco;Contact"/>
  <rdfs:subPropertyOf rdf:resource="&nmo;recipient"/>
</rdf:Property>

<rdf:Property rdf:about="&nexif;subjectLocation"
    rdfs:label="subjectLocation">
  <rdfs:subPropertyOf rdf:resource="http://www.kanzaki.com/ns/exif#subjectLocation"/>
  <rdfs:subPropertyOf rdf:resource="&nexif;pictTaking"/>
  <rdfs:comment>The location of the main subject in the scene. The value of this tag represents the pixel at the center of the main subject relative to the left edge, prior to rotation processing as per the Rotation tag. The first value indicates the X column number and second indicates the Y row number.
tagNumber: 41492</rdfs:comment>
  <rdfs:domain rdf:resource="&nexif;Photo"/>
  <rdfs:range rdf:resource="&xsd;string"/>
</rdf:Property>

<rdf:Property rdf:about="&dcon;nearbyPerson"
    rdfs:comment="Refers to individuals characterising a context instance."
    rdfs:label="Nearby Person">
  <rdfs:domain rdf:resource="&dcon;Peers"/>
  <rdfs:range rdf:resource="&pimo;Person"/>
  <rdfs:subPropertyOf rdf:resource="&dcon;hasContextElement"/>
</rdf:Property>

<rdf:Property rdf:about="&dc;subject">
  <dcterms:description xml:lang="en">Typically, the subject will be represented using keywords, key phrases, or classification codes. Recommended best practice is to use a controlled vocabulary.</dcterms:description>
  <dcterms:hasVersion rdf:resource="http://dublincore.org/usage/terms/history/#subject-007"/>
  <dcterms:issued rdf:datatype="&xsd;date">1999-07-02</dcterms:issued>
  <dcterms:modified rdf:datatype="&xsd;date">2012-06-14</dcterms:modified>
  <rdfs:comment xml:lang="en">The topic of the resource.</rdfs:comment>
  <rdfs:isDefinedBy rdf:resource="&dc;"/>
  <rdfs:label xml:lang="en">Subject</rdfs:label>
  <scos:note xml:lang="en">A second property with the same name as this property has been declared in the dcterms: namespace (http://purl.org/dc/terms/).  See the Introduction to the document "DCMI Metadata Terms" (http://dublincore.org/documents/dcmi-terms/) for an explanation.</scos:note>
</rdf:Property>

<rdf:Property rdf:about="&nfo;bookmarks"
    rdfs:comment="The address of the linked object. Usually a web URI."
    rdfs:label="link">
  <nrl:cardinality rdf:datatype="&xsd;integer">1</nrl:cardinality>
  <rdfs:domain rdf:resource="&nfo;Bookmark"/>
  <rdfs:range rdf:resource="&nie;DataObject"/>
  <rdfs:subPropertyOf rdf:resource="&nie;links"/>
</rdf:Property>

<rdf:Property rdf:about="&nie;contentLastModified"
    nrl:maxCardinality="1"
    rdfs:label="contentLastModified">
  <rdfs:subPropertyOf rdf:resource="&nie;contentModified"/>
  <rdfs:subPropertyOf rdf:resource="&nie;informationElementDate"/>
  <rdfs:subPropertyOf rdf:resource="&nao;lastModified"/>
  <rdfs:comment>The date of the last modification of the original content (not its corresponding DataObject or local copy). Compare with nie:lastModified.</rdfs:comment>
  <rdfs:domain rdf:resource="&nie;InformationElement"/>
  <rdfs:range rdf:resource="&xsd;dateTime"/>
</rdf:Property>

<rdf:Property rdf:about="&dcon;currentPlace"
    rdfs:label="Current Place">
  <rdfs:range rdf:resource="&pimo;Location"/>
  <rdfs:range rdf:resource="&dpo;Place"/>
  <rdfs:comment>Refers to a place type or specific location that characterises a context instance.</rdfs:comment>
  <rdfs:domain rdf:resource="&dcon;SpaTem"/>
  <rdfs:subPropertyOf rdf:resource="&dcon;hasContextElement"/>
</rdf:Property>

<rdf:Property rdf:about="&dcon;inEditMode"
    rdfs:label="in Edit mode">
  <rdfs:comment>Specifies whether a writeable active file (running on a device) is being edited/written to, in the current context.</rdfs:comment>
  <rdfs:domain rdf:resource="&nie;InformationElement"/>
  <rdfs:range rdf:resource="&xsd;boolean"/>
  <rdfs:subPropertyOf rdf:resource="&dcon;hasContextAttribute"/>
</rdf:Property>

<rdfs:Class rdf:about="&nco;PersonContact"
    rdfs:label="PersonContact">
  <rdfs:comment>A Contact that denotes a Person. A person can have multiple Affiliations.</rdfs:comment>
  <rdfs:subClassOf rdf:resource="&nco;Contact"/>
</rdfs:Class>

<rdf:Property rdf:about="&nmo;messageRecipient"
    rdfs:label="recipient">
  <rdfs:comment>A common superproperty for all properties that link a message with its recipients. Please don't use this property directly.</rdfs:comment>
  <rdfs:domain rdf:resource="&nmo;Message"/>
  <rdfs:range rdf:resource="&nco;ContactMedium"/>
</rdf:Property>

<nrl:DefiningProperty rdf:about="&nmm;isPartOfSeason"
    rdfs:comment="Relates a TV Show to its season"
    rdfs:label="season">
  <nrl:inverseProperty rdf:resource="&nmm;hasSeasonEpisode"/>
  <nrl:maxCardinality rdf:datatype="&xsd;integer">1</nrl:maxCardinality>
  <rdf:type rdf:resource="&rdf;Property"/>
  <rdfs:domain rdf:resource="&nmm;TVShow"/>
  <rdfs:range rdf:resource="&nmm;TVSeason"/>
  <rdfs:subPropertyOf rdf:resource="&nie;isLogicalPartOf"/>
</nrl:DefiningProperty>

<tmo:PersonInvolvementRole rdf:about="&tmo;TMO_Instance_PersonInvolvementRole_Delegate"
    rdfs:label="TMO_Instance_PersonInvolvementRole_Delegate"/>

<rdf:Property rdf:about="&dcon;precipitation"
    rdfs:label="Precipitation Value">
  <rdfs:comment>Registers an actual precipitation value element attribute to an active weather condition in the current context.</rdfs:comment>
  <rdfs:domain rdf:resource="&dpo;WeatherConditions"/>
  <rdfs:range rdf:resource="&xsd;nonNegativeInteger"/>
  <rdfs:subPropertyOf rdf:resource="&dcon;hasContextAttribute"/>
</rdf:Property>

<rdf:Property rdf:about="&nid3;textWriter"
    rdfs:label="textWriter">
  <rdfs:comment>TEXT
The 'Lyricist(s)/Text writer(s)' frame is intended for the writer(s) of the text or lyrics in the recording. They are seperated with the "/" character.
Note that in the RDF representation each text writer is represented with a separate triple.</rdfs:comment>
  <rdfs:domain rdf:resource="&nid3;ID3Audio"/>
  <rdfs:range rdf:resource="&nco;Contact"/>
  <rdfs:subPropertyOf rdf:resource="&nco;contributor"/>
</rdf:Property>

<rdf:Property rdf:about="&dcon;activeApplication"
    rdfs:label="Active Application">
  <rdfs:comment>Refers to active applications (running on a device) characterising a context instance.</rdfs:comment>
  <rdfs:domain rdf:resource="&dcon;Attention"/>
  <rdfs:range rdf:resource="&nfo;Application"/>
  <rdfs:subPropertyOf rdf:resource="&dcon;hasContextElement"/>
</rdf:Property>

<rdf:Property rdf:about="&pimo;hasDeprecatedRepresentation"
    rdfs:label="has deprecated representation">
  <rdfs:comment>The subject Thing was represented previously using the object resource. This indicates that the object resource was a duplicate representation of the subject and merged with the subject. Implementations can use this property to resolve dangling links in distributed system. When encountering resources that are deprecated representations of a Thing, they should be replaced with the Thing. The range is not declared as we assume all knowledge about the object is gone, including its rdf:type.</rdfs:comment>
  <rdfs:domain rdf:resource="&pimo;Thing"/>
  <rdfs:range rdf:resource="&rdfs;Resource"/>
</rdf:Property>

<rdfs:Class rdf:about="&dplo;Comment"
    rdfs:label="Comment">
  <rdfs:subClassOf rdf:resource="http://rdfs.org/sioc/types#Comment"/>
  <rdfs:subClassOf rdf:resource="&dplo;Message"/>
  <rdfs:comment>Represents comments shared by a user or a contact, in reply to existing liveposts.</rdfs:comment>
</rdfs:Class>

<rdf:Property rdf:about="&drmo;hasConstraintOnGraph"
    rdfs:label="Constraint on Graph">
  <rdfs:comment>This property allow a condition test to be conducted on a specified Graph.</rdfs:comment>
  <rdfs:domain rdf:resource="&drmo;Condition"/>
  <rdfs:range rdf:resource="http://www.w3.org/2004/03/trix/rdfg-1Graph"/>
</rdf:Property>

<rdfs:Class rdf:about="&nmm;TVSeries"
    rdfs:comment="A TV Series has multiple seasons and episodes"
    rdfs:label="tv series">
  <rdfs:subClassOf rdf:resource="&nie;InformationElement"/>
</rdfs:Class>

<rdfs:Class rdf:about="&dcterms;PhysicalMedium">
  <dcterms:description xml:lang="en">Examples include paper, canvas, or DVD.</dcterms:description>
  <dcterms:hasVersion rdf:resource="http://dublincore.org/usage/terms/history/#PhysicalMedium-001"/>
  <dcterms:issued rdf:datatype="&xsd;date">2008-01-14</dcterms:issued>
  <rdfs:comment xml:lang="en">A physical material or carrier.</rdfs:comment>
  <rdfs:isDefinedBy rdf:resource="&dcterms;"/>
  <rdfs:label xml:lang="en">Physical Medium</rdfs:label>
  <rdfs:subClassOf rdf:resource="&dcterms;MediaType"/>
</rdfs:Class>

<rdf:Property rdf:about="&nao;deprecated"
    rdfs:label="deprecated">
  <nrl:maxCardinality rdf:datatype="&xsd;nonNegativeInteger">1</nrl:maxCardinality>
  <rdfs:comment>If this property is assigned, the subject class, property, or resource, is deprecated and should not be used in production systems any longer. It may be removed without further notice.</rdfs:comment>
  <rdfs:domain rdf:resource="&rdfs;Resource"/>
  <rdfs:range rdf:resource="&rdfs;Resource"/>
</rdf:Property>

<rdf:Property rdf:about="&dcon;currentActivity"
    rdfs:label="Current Activity">
  <rdfs:comment>Refers to a pre-defined activity category characterising a context instance.</rdfs:comment>
  <rdfs:domain rdf:resource="&dcon;State"/>
  <rdfs:range rdf:resource="&dpo;Activity"/>
  <rdfs:subPropertyOf rdf:resource="&dcon;hasContextElement"/>
</rdf:Property>

<rdfs:Class rdf:about="&nao;Symbol"
    rdfs:label="symbol">
  <rdfs:comment>Represents a symbol, a visual representation of a resource. Typically a local or remote file would be double-typed to be used as a symbol. An alternative is nao:FreeDesktopIcon.</rdfs:comment>
  <rdfs:subClassOf rdf:resource="&rdfs;Resource"/>
</rdfs:Class>

<owl:DatatypeProperty rdf:about="&oa;when">
  <rdfs:comment xml:lang="en">The timestamp at which the Source resource should be interpreted for the Annotation, typically the time that the Annotation was created.</rdfs:comment>
  <rdfs:domain rdf:resource="&oa;TimeState"/>
  <rdfs:isDefinedBy rdf:resource="&oa;"/>
  <rdfs:label xml:lang="en">when</rdfs:label>
  <rdfs:range rdf:resource="&xsd;dateTimeStamp"/>
</owl:DatatypeProperty>

<rdf:Property rdf:about="&nco;url"
    rdfs:label="url">
  <rdfs:comment>A uniform resource locator associated with the given role of a Contact. Inspired by the 'URL' property defined in RFC 2426 Sec. 3.6.8.</rdfs:comment>
  <rdfs:domain rdf:resource="&nco;Role"/>
  <rdfs:range rdf:resource="&rdfs;Resource"/>
</rdf:Property>

<rdfs:Class rdf:about="&foaf;OnlineAccount"
    rdfs:comment="An online account."
    rdfs:label="Online Account"
    ns:term_status="testing">
  <rdf:type rdf:resource="&owl;Class"/>
  <rdfs:isDefinedBy rdf:resource="&foaf;"/>
  <rdfs:subClassOf rdf:resource="&owl;Thing"/>
</rdfs:Class>

<rdf:Property rdf:about="&nexif;subjectArea"
    rdfs:label="subjectArea">
  <rdfs:subPropertyOf rdf:resource="http://www.kanzaki.com/ns/exif#subjectArea"/>
  <rdfs:subPropertyOf rdf:resource="&nexif;pictTaking"/>
  <rdfs:comment>tagNumber: 37396
The location and area of the main subject in the overall scene.</rdfs:comment>
  <rdfs:domain rdf:resource="&nexif;Photo"/>
  <rdfs:range rdf:resource="&xsd;string"/>
</rdf:Property>

<rdfs:Class rdf:about="&drmo;SituationActivated"
    rdfs:label="Internal System Action">
  <rdfs:comment>Describes a condition which is activated by a change in the user's situation.</rdfs:comment>
  <rdfs:subClassOf rdf:resource="&drmo;ResourceModified"/>
</rdfs:Class>

<rdf:Property rdf:about="&ncal;bydayWeekday"
    rdfs:comment="Connects a BydayRulePath with a weekday."
    rdfs:label="bydayWeekday">
  <rdfs:domain rdf:resource="&ncal;BydayRulePart"/>
  <rdfs:range rdf:resource="&ncal;Weekday"/>
</rdf:Property>

<rdfs:Class rdf:about="&ddo;Bluetooth"
    rdfs:label="Bluetooth">
  <rdfs:comment>Bluetooth networks refer to personal area networks created between computerised devices in order to exchange data over short distances.</rdfs:comment>
  <rdfs:subClassOf rdf:resource="&ddo;PersonalAreaNetwork"/>
</rdfs:Class>

<rdf:Property rdf:about="&nie;version"
    rdfs:label="version">
  <rdfs:comment>The current version of the given data object. Exact semantics is unspecified at this level. Use more specific subproperties if needed.</rdfs:comment>
  <rdfs:domain rdf:resource="&nie;InformationElement"/>
  <rdfs:range rdf:resource="&xsd;string"/>
  <rdfs:subPropertyOf rdf:resource="&dcterms;hasVersion"/>
</rdf:Property>

<rdf:Property rdf:about="&ncal;summaryAltRep"
    rdfs:label="summaryAltRep">
  <rdfs:comment>Alternate representation of the comment. Introduced to cover 
the ALTREP parameter of the SUMMARY property. See 
documentation of ncal:summary for details.</rdfs:comment>
  <rdfs:domain rdf:resource="&ncal;UnionOfAlarmEventJournalTodo"/>
  <rdfs:range rdf:resource="&rdfs;Resource"/>
</rdf:Property>

<rdf:Property rdf:about="&nexif;software"
    rdfs:label="software">
  <rdfs:subPropertyOf rdf:resource="http://www.kanzaki.com/ns/exif#software"/>
  <rdfs:subPropertyOf rdf:resource="&nexif;exifAttribute"/>
  <rdfs:comment>tagNumber: 305
The name and version of the software or firmware of the camera or image input device used to generate the image.</rdfs:comment>
  <rdfs:domain rdf:resource="&nexif;Photo"/>
  <rdfs:range rdf:resource="&xsd;string"/>
</rdf:Property>

<rdf:Property rdf:about="&nid3;trackNumber"
    rdfs:label="trackNumber">
  <rdfs:comment>TRCK
The 'Track number/Position in set' frame is a numeric string containing the order number of the audio-file on its original recording. This may be extended with a "/" character and a numeric string containing the total numer of tracks/elements on the original recording. E.g. "4/9".</rdfs:comment>
  <rdfs:domain rdf:resource="&nid3;ID3Audio"/>
  <rdfs:range rdf:resource="&xsd;string"/>
</rdf:Property>

<tmo:TransmissionState rdf:about="&tmo;TMO_Instance_TransmissionState_Transmitted"
    rdfs:label="TMO_Instance_TransmissionState_Transmitted"/>

<owl:AnnotationProperty rdf:about="http://xmlns.com/wot/0.1/assurance"/>

<rdfs:Class rdf:about="&pimo;Event"
    rdfs:label="Event">
  <rdfs:comment>Something that happens
An Event is conceived as compact in time. (Definition from Merriam-Webster)</rdfs:comment>
  <rdfs:subClassOf rdf:resource="&pimo;ProcessConcept"/>
</rdfs:Class>

<rdf:Property rdf:about="&tmo;transmissionState"
    nrl:maxCardinality="1"
    nrl:minCardinality="1"
    rdfs:label="transmissionState">
  <rdfs:domain rdf:resource="&tmo;TaskTransmission"/>
  <rdfs:range rdf:resource="&tmo;TransmissionState"/>
  <rdfs:subPropertyOf rdf:resource="&tmo;stateTypeRole"/>
</rdf:Property>

<rdf:Property rdf:about="&dpo;maxAbsoluteAltitude"
    rdfs:label="Maximum Absolute Altitude">
  <rdfs:comment>A variant subproperty of dpo:maxAltitude that defines an upperbound on the computed absolute altitude (i.e. altitude relative to the level of the terrain in the area), rather the observed true altitude. Can be used in conjunction with dpo:minAbsoulateAltitude.</rdfs:comment>
  <rdfs:domain rdf:resource="&dpo;Altitude"/>
  <rdfs:range rdf:resource="&xsd;float"/>
  <rdfs:subPropertyOf rdf:resource="&dpo;maxValue"/>
</rdf:Property>

<rdf:Property rdf:about="&nexif;compression"
    rdfs:label="compression">
  <rdfs:subPropertyOf rdf:resource="http://www.kanzaki.com/ns/exif#compression"/>
  <rdfs:subPropertyOf rdf:resource="&nexif;imageDataStruct"/>
  <rdfs:comment>The compression scheme used for the image data. When a primary image is JPEG compressed, this designation is not necessary and is omitted. When thumbnails use JPEG compression, this tag value is set to 6.
tagNumber: 259</rdfs:comment>
  <rdfs:domain rdf:resource="&nexif;Photo"/>
  <rdfs:range rdf:resource="&xsd;string"/>
</rdf:Property>

<nco:IMStatusType rdf:about="&nco;IMStatusTypeAway"
    rdfs:label="away"/>

<rdf:Property rdf:about="&nfo;fileCreated"
    rdfs:comment="File creation date"
    rdfs:label="fileCreated">
  <nrl:maxCardinality rdf:datatype="&xsd;integer">1</nrl:maxCardinality>
  <rdfs:domain rdf:resource="&nfo;FileDataObject"/>
  <rdfs:range rdf:resource="&xsd;dateTime"/>
  <rdfs:subPropertyOf rdf:resource="&nie;created"/>
</rdf:Property>

<rdf:Property rdf:about="&ddo;cellID"
    rdfs:label="cellID">
  <rdfs:comment>Identifies the known cells (tower) that is, or has, enabled a specific cellular network.</rdfs:comment>
  <rdfs:domain rdf:resource="&ddo;CellularNetwork"/>
  <rdfs:subPropertyOf rdf:resource="&ddo;networkID"/>
</rdf:Property>

<rdf:Property rdf:about="&cnt;publicId">
  <rdf:type rdf:resource="&owl;ObjectProperty"/>
  <rdfs:comment xml:lang="en">The document type declarations's public identifier.</rdfs:comment>
  <rdfs:domain rdf:resource="&cnt;DoctypeDecl"/>
  <rdfs:label xml:lang="en">Public ID</rdfs:label>
  <rdfs:range rdf:resource="&rdfs;Literal"/>
</rdf:Property>

<rdf:Property rdf:about="&nco;imID"
    rdfs:label="imID">
  <rdfs:comment>Identifier of the IM account. Examples of such identifier might include ICQ UINs, Jabber IDs, Skype names etc.</rdfs:comment>
  <rdfs:domain rdf:resource="&nco;IMAccount"/>
  <rdfs:range rdf:resource="&xsd;string"/>
  <rdfs:subPropertyOf rdf:resource="&nao;identifier"/>
</rdf:Property>

<rdf:Property rdf:about="&dplo;timestamp"
    rdfs:label="Timestamp">
  <nrl:cardinality rdf:datatype="&xsd;nonNegativeInteger">1</nrl:cardinality>
  <rdfs:comment>Records the time and date at which a Livepost is published at.</rdfs:comment>
  <rdfs:domain rdf:resource="&dplo;LivePost"/>
  <rdfs:range rdf:resource="&xsd;datetime"/>
</rdf:Property>

<rdf:Property rdf:about="&nid3;subtitle"
    rdfs:label="subtitle">
  <rdfs:comment>TIT3
The 'Subtitle/Description refinement' frame is used for information directly related to the contents title (e.g. "Op. 16" or "Performed live at Wembley").</rdfs:comment>
  <rdfs:domain rdf:resource="&nid3;ID3Audio"/>
  <rdfs:range rdf:resource="&xsd;string"/>
</rdf:Property>

<rdf:Property rdf:about="&nexif;maxApertureValue"
    rdfs:label="maxApertureValue">
  <rdfs:subPropertyOf rdf:resource="http://www.kanzaki.com/ns/exif#maxApertureValue"/>
  <rdfs:subPropertyOf rdf:resource="&nexif;pictTaking"/>
  <rdfs:comment>tagNumber: 37381
The smallest F number of the lens. The unit is the APEX value. Ordinarily it is given in the range of 00.00 to 99.99, but it is not limited to this range.</rdfs:comment>
  <rdfs:domain rdf:resource="&nexif;Photo"/>
  <rdfs:range rdf:resource="&xsd;float"/>
</rdf:Property>

<owl:Ontology rdf:about="http://www.w3.org/2004/02/skos/core">
  <dcterms:contributor>Dave Beckett</dcterms:contributor>
  <dcterms:contributor>Nikki Rogers</dcterms:contributor>
  <dcterms:contributor>Participants in W3C's Semantic Web Deployment Working Group.</dcterms:contributor>
  <dcterms:creator>Alistair Miles</dcterms:creator>
  <dcterms:creator>Sean Bechhofer</dcterms:creator>
  <dcterms:description xml:lang="en">An RDF vocabulary for describing the basic structure and content of concept schemes such as thesauri, classification schemes, subject heading lists, taxonomies, 'folksonomies', other types of controlled vocabulary, and also concept schemes embedded in glossaries and terminologies.</dcterms:description>
  <dcterms:title xml:lang="en">SKOS Vocabulary</dcterms:title>
  <rdfs:seeAlso rdf:resource="http://www.w3.org/TR/skos-reference/"/>
</owl:Ontology>

<rdf:Property rdf:about="&nuao;lastUsage"
    rdfs:comment="The start time of the last usage"
    rdfs:label="last usage">
  <nrl:maxCardinality rdf:datatype="&xsd;nonNegativeInteger">1</nrl:maxCardinality>
  <rdfs:domain rdf:resource="&rdfs;Resource"/>
  <rdfs:range rdf:resource="&xsd;dateTime"/>
  <rdfs:subPropertyOf rdf:resource="&nuao;lastEvent"/>
</rdf:Property>

<rdf:Property rdf:about="&nso;sharedWith"
    rdfs:label="shared with">
  <rdfs:comment>An alternative to nso:sharedWithContact/Group which enables the establishment of a 'shared with' relationship between a resource (pimo:Thing or nie:InformationElement) with a pimo:Agent (individual, or group).</rdfs:comment>
  <rdfs:domain rdf:resource="&rdfs;Resource"/>
  <rdfs:range rdf:resource="&pimo;Agent"/>
</rdf:Property>

<rdf:Property rdf:about="&dcon;recordedAt"
    rdfs:label="Recorded At">
  <rdfs:subPropertyOf rdf:resource="&nao;lastModified"/>
  <rdfs:subPropertyOf rdf:resource="&dcon;hasContextAttribute"/>
  <rdfs:comment>This property stores the time at which each element's observation has been generated, or last updated. Whereas for situations only the time of first occurrence is recorded, live context instances always carry the actual time.</rdfs:comment>
  <rdfs:domain rdf:resource="&dcon;Observation"/>
  <rdfs:range rdf:resource="&xsd;dateTime"/>
</rdf:Property>

<rdf:Property rdf:about="&nuao;firstUsage"
    rdfs:comment="The start time of the first usage"
    rdfs:label="first usage">
  <nrl:maxCardinality rdf:datatype="&xsd;nonNegativeInteger">1</nrl:maxCardinality>
  <rdfs:domain rdf:resource="&rdfs;Resource"/>
  <rdfs:range rdf:resource="&xsd;dateTime"/>
  <rdfs:subPropertyOf rdf:resource="&nuao;firstEvent"/>
</rdf:Property>

<ncal:RecurrenceFrequency rdf:about="&ncal;weekly"
    rdfs:label="weekly"/>

<rdfs:Class rdf:about="&nid3;UserDefinedURLFrame"
    rdfs:label="UserDefinedURLFrame">
  <rdfs:comment>This frame is intended for URL links concerning the audiofile in a similar way to the other "W"-frames. The frame body consists of a description of the string, represented as a terminated string, followed by the actual URL. The URL is always encoded with ISO-8859-1. There may be more than one "WXXX" frame in each tag, but only one with the same description.</rdfs:comment>
  <rdfs:subClassOf rdf:resource="&nid3;UserDefinedFrame"/>
</rdfs:Class>

<rdfs:Class rdf:about="&nrl;Data"
    rdfs:comment="An abstract class representing all named graph roles"
    rdfs:label="Data">
  <rdfs:subClassOf rdf:resource="&nrl;Graph"/>
</rdfs:Class>

<ncal:CalendarUserType rdf:about="&ncal;individualUserType"
    rdfs:label="individualUserType"/>

<rdfs:Class rdf:about="&nfo;Application"
    rdfs:comment="An application"
    rdfs:label="Application">
  <rdfs:subClassOf rdf:resource="&nfo;Software"/>
</rdfs:Class>

<rdf:Property rdf:about="&dpo;recurringProcess"
    rdfs:label="Recurring Process">
  <rdfs:comment>Links a generic activity to specific tasks and events (pimo:ProcessConcept instances) that are also stored in the PIM and that are known to be of the same type, e.g., a dpo:Activity representing 'sports' to a recurring event representing 'swimming lessons' stored in the agent's calendar.</rdfs:comment>
  <rdfs:domain rdf:resource="&dpo;Activity"/>
  <rdfs:range rdf:resource="&pimo;ProcessConcept"/>
</rdf:Property>

<rdf:Property rdf:about="&nexif;versionInfo"
    rdfs:comment="An attribute relating to Version"
    rdfs:label="versionInfo">
  <rdfs:subPropertyOf rdf:resource="http://www.kanzaki.com/ns/exif#versionInfo"/>
  <rdfs:subPropertyOf rdf:resource="&nexif;exifAttribute"/>
  <rdfs:domain rdf:resource="&nexif;Photo"/>
  <rdfs:range rdf:resource="&xsd;string"/>
</rdf:Property>

<rdf:Property rdf:about="&dcterms;isPartOf">
  <rdfs:subPropertyOf rdf:resource="&dc;relation"/>
  <rdfs:subPropertyOf rdf:resource="&dcterms;relation"/>
  <dcterms:hasVersion rdf:resource="http://dublincore.org/usage/terms/history/#isPartOf-003"/>
  <dcterms:issued rdf:datatype="&xsd;date">2000-07-11</dcterms:issued>
  <dcterms:modified rdf:datatype="&xsd;date">2008-01-14</dcterms:modified>
  <rdfs:comment xml:lang="en">A related resource in which the described resource is physically or logically included.</rdfs:comment>
  <rdfs:isDefinedBy rdf:resource="&dcterms;"/>
  <rdfs:label xml:lang="en">Is Part Of</rdfs:label>
  <scos:note xml:lang="en">This term is intended to be used with non-literal values as defined in the DCMI Abstract Model (http://dublincore.org/documents/abstract-model/).  As of December 2007, the DCMI Usage Board is seeking a way to express this intention with a formal range declaration.</scos:note>
</rdf:Property>

<rdfs:Class rdf:about="&dplo;EventPost"
    rdfs:label="Event Post">
  <rdfs:comment>Represents the live posting of information related to a user's detected or proclaimed attendance in an ongoing event, as defined by an established instance of pimo:Event.</rdfs:comment>
  <rdfs:subClassOf rdf:resource="&dplo;PresencePost"/>
</rdfs:Class>

<rdf:Property rdf:about="&foaf;homepage"
    rdfs:comment="A homepage for some thing."
    rdfs:label="homepage"
    ns:term_status="stable">
  <rdf:type rdf:resource="&owl;InverseFunctionalProperty"/>
  <rdf:type rdf:resource="&owl;ObjectProperty"/>
  <rdfs:subPropertyOf rdf:resource="&foaf;isPrimaryTopicOf"/>
  <rdfs:subPropertyOf rdf:resource="&foaf;page"/>
  <rdfs:domain rdf:resource="&owl;Thing"/>
  <rdfs:isDefinedBy rdf:resource="&foaf;"/>
  <rdfs:range rdf:resource="&foaf;Document"/>
</rdf:Property>

<rdf:Property rdf:about="&drmo;hasObject"
    rdfs:label="has Object">
  <rdfs:comment>Specifies the parameters needed to be passed to the executed actions.</rdfs:comment>
  <rdfs:domain rdf:resource="&drmo;Action"/>
  <rdfs:range rdf:resource="&rdfs;Resource"/>
</rdf:Property>

<rdf:Property rdf:about="&dpo;maxMonth"
    rdfs:label="Maximum Month">
  <rdfs:comment>A subproperty of dpo:maxValue that defines an upperbound on the observed month (i.e., between 1 signifying January and 12 signifying December) such that it can classify as a dpo:TimePeriod instance. It can be used in conjunction with dpo:minMonth, i.e. specific instances of dpo:TimePeriod have a pre-defined observable month number-based period.</rdfs:comment>
  <rdfs:domain rdf:resource="&dpo;TimePeriod"/>
  <rdfs:range rdf:resource="&xsd;integer"/>
  <rdfs:subPropertyOf rdf:resource="&dpo;maxValue"/>
</rdf:Property>

<rdf:Property rdf:about="&nid3;licensee"
    rdfs:label="licensee">
  <rdfs:comment>TOWN
The 'File owner/licensee' frame contains the name of the owner or licensee of the file and it's contents.</rdfs:comment>
  <rdfs:domain rdf:resource="&nid3;ID3Audio"/>
  <rdfs:range rdf:resource="&nco;Contact"/>
</rdf:Property>

<rdf:List rdf:about="&rdf;nil">
  <rdfs:comment xml:lang="en">The empty list, with no items in it. If the rest of a list is nil then the list has no more items in it.</rdfs:comment>
  <rdfs:isDefinedBy rdf:resource="&rdf;"/>
  <rdfs:label xml:lang="en">nil</rdfs:label>
</rdf:List>

<tmo:PersonInvolvementRole rdf:about="&tmo;TMO_Instance_PersonInvolvementRole_Receiver"
    rdfs:label="TMO_Instance_PersonInvolvementRole_Receiver"/>

<nrl:TransitiveProperty rdf:about="&pimo;hasOtherRepresentation"
    rdfs:label="has other representation">
  <rdf:type rdf:resource="&rdf;Property"/>
  <rdfs:comment>hasOtherRepresentation points from a Thing in your PIMO to a thing in an ontology that represents the same real world thing. 
This means that the real world object O represented by an instance I1 has additional representations (as instances I2-In of different conceptualizations).
This means: IF (I_i represents O_j in Ontology_k) AND (I_m represents O_n in Ontology_o) THEN (O_n and O_j are the same object).
hasOtherRepresentation is a transitive relation, but not equivalent (not symmetric nor reflexive). For example, the URI of a  foaf:Person representation published on the web is a hasOtherRepresentation for the person. This property is inverse functional, two Things from two information models having the same hasOtherRepresentation are considered to be representations of the same entity from the real world.</rdfs:comment>
  <rdfs:domain rdf:resource="&pimo;Thing"/>
  <rdfs:range rdf:resource="&rdfs;Resource"/>
  <rdfs:subPropertyOf rdf:resource="&pimo;occurrence"/>
</nrl:TransitiveProperty>

<owl:DatatypeProperty rdf:about="&oa;end">
  <rdfs:comment xml:lang="en">The end position of the segment of text or bytes. The first character/byte in the full text/stream is position 0. The character/byte indicated at position oa:end is NOT included within the selected segment. 

See oa:DataPositionSelector and oa:oa:TextPositionSelector.</rdfs:comment>
  <rdfs:domain rdf:resource="&oa;Selector"/>
  <rdfs:isDefinedBy rdf:resource="&oa;"/>
  <rdfs:label xml:lang="en">end</rdfs:label>
  <rdfs:range rdf:resource="&xsd;nonNegativeInteger"/>
</owl:DatatypeProperty>

<rdfs:Class rdf:about="&pimo;Locatable"
    protege:role="abstract"
    rdfs:label="Locatable">
  <pimo:classRole rdf:resource="&pimo;AbstractClass"/>
  <rdfs:comment>Things that can be at a location. Abstract class, use it as a superclass of things that can be placed in physical space.</rdfs:comment>
  <rdfs:subClassOf rdf:resource="&pimo;Thing"/>
</rdfs:Class>

<rdfs:Class rdf:about="&dcterms;LocationPeriodOrJurisdiction">
  <dcterms:hasVersion rdf:resource="http://dublincore.org/usage/terms/history/#LocationPeriodOrJurisdiction-001"/>
  <dcterms:issued rdf:datatype="&xsd;date">2008-01-14</dcterms:issued>
  <rdfs:comment xml:lang="en">A location, period of time, or jurisdiction.</rdfs:comment>
  <rdfs:isDefinedBy rdf:resource="&dcterms;"/>
  <rdfs:label xml:lang="en">Location, Period, or Jurisdiction</rdfs:label>
</rdfs:Class>

<rdf:Property rdf:about="&drmo;triggers"
    rdfs:label="triggers">
  <nrl:minCardinality rdf:datatype="&xsd;nonNegativeInteger">1</nrl:minCardinality>
  <rdfs:comment>The triggers property defines the action instances which will be triggered if rule's conditions are satisfied.</rdfs:comment>
  <rdfs:domain rdf:resource="&drmo;Rule"/>
  <rdfs:range rdf:resource="&drmo;Action"/>
</rdf:Property>

<rdfs:Class rdf:about="&nrl;Semantics"
    rdfs:comment="Represents some declarative semantics"
    rdfs:label="Semantics">
  <rdfs:subClassOf rdf:resource="&rdfs;Resource"/>
</rdfs:Class>

<rdf:Property rdf:about="&nrl;realizes"
    rdfs:label="realizes">
  <rdfs:comment>Points to a representation of the declarative semantics that the view specification realizes</rdfs:comment>
  <rdfs:domain rdf:resource="&nrl;ViewSpecification"/>
  <rdfs:range rdf:resource="&nrl;Semantics"/>
</rdf:Property>

<rdfs:Class rdf:about="&nfo;TextDocument"
    rdfs:comment="A text document"
    rdfs:label="TextDocument">
  <rdfs:subClassOf rdf:resource="&nfo;Document"/>
</rdfs:Class>

<rdfs:Class rdf:about="&dcon;State"
    rdfs:label="State">
  <rdfs:comment>The state aspect covers context elements relating to the state of either the user or their devices.</rdfs:comment>
  <rdfs:subClassOf rdf:resource="&dcon;Aspect"/>
</rdfs:Class>

<ncal:FreebusyType rdf:about="&ncal;busyFreebusyType"
    rdfs:label="busyFreebusyType"/>

<rdf:Property rdf:about="&foaf;primaryTopic"
    rdfs:comment="The primary topic of some page or document."
    rdfs:label="primary topic"
    ns:term_status="stable">
  <rdf:type rdf:resource="&owl;FunctionalProperty"/>
  <rdf:type rdf:resource="&owl;ObjectProperty"/>
  <rdfs:domain rdf:resource="&foaf;Document"/>
  <rdfs:isDefinedBy rdf:resource="&foaf;"/>
  <rdfs:range rdf:resource="&owl;Thing"/>
  <owl:inverseOf rdf:resource="&foaf;isPrimaryTopicOf"/>
</rdf:Property>

<rdfs:Class rdf:about="&foaf;Document"
    rdfs:comment="A document."
    rdfs:label="Document"
    ns:term_status="stable">
  <owl:disjointWith rdf:resource="&foaf;Organization"/>
  <owl:disjointWith rdf:resource="&foaf;Project"/>
  <rdf:type rdf:resource="&owl;Class"/>
  <rdfs:isDefinedBy rdf:resource="&foaf;"/>
  <owl:equivalentClass rdf:resource="http://schema.org/CreativeWork"/>
</rdfs:Class>

<rdf:Property rdf:about="&nexif;meteringMode"
    rdfs:label="meteringMode">
  <rdfs:subPropertyOf rdf:resource="http://www.kanzaki.com/ns/exif#meteringMode"/>
  <rdfs:subPropertyOf rdf:resource="&nexif;pictTaking"/>
  <rdfs:comment>Metering mode, such as CenterWeightedAverage, Spot, MultiSpot,Pattern, Partial etc.
tagNumber: 37383</rdfs:comment>
  <rdfs:domain rdf:resource="&nexif;Photo"/>
  <rdfs:range rdf:resource="&xsd;string"/>
</rdf:Property>

<rdfs:Class rdf:about="&nfo;EncryptionStatus"
    rdfs:label="EncryptionStatus">
  <rdfs:comment>The status of the encryption of an InformationElement. nfo:encryptedStatus means that the InformationElement has been encrypted and couldn't be decrypted by the extraction software, thus no content is available. nfo:decryptedStatus means that decryption was successfull and the content is available.</rdfs:comment>
</rdfs:Class>

<rdf:Property rdf:about="&nexif;yCbCrCoefficients"
    rdfs:label="yCbCrCoefficients">
  <rdfs:subPropertyOf rdf:resource="http://www.kanzaki.com/ns/exif#yCbCrCoefficients"/>
  <rdfs:subPropertyOf rdf:resource="&nexif;imageDataCharacter"/>
  <rdfs:comment>tagNumber: 529
The matrix coefficients for transformation from RGB to YCbCr image data.</rdfs:comment>
  <rdfs:domain rdf:resource="&nexif;Photo"/>
  <rdfs:range rdf:resource="&xsd;string"/>
</rdf:Property>

<rdf:Property rdf:about="&ncal;trigger"
    rdfs:label="trigger">
  <rdfs:comment>This property specifies when an alarm will trigger. Inspired by RFC 2445 sec. 4.8.6.3 Originally the value of this property could accept two types : duration and date-time. To express this fact a Trigger class has been introduced. It also has a related property to account for the RELATED parameter.</rdfs:comment>
  <rdfs:domain rdf:resource="&ncal;UnionOfAlarmEventTodo"/>
  <rdfs:range rdf:resource="&ncal;Trigger"/>
</rdf:Property>

<rdf:Property rdf:about="&pimo;dtend"
    nrl:maxCardinality="1"
    rdfs:label="end date">
  <rdfs:comment>This property specifies the date and time when a process ends. Inspired by NCAL:dtend.</rdfs:comment>
  <rdfs:domain rdf:resource="&pimo;ProcessConcept"/>
  <rdfs:range rdf:resource="&xsd;dateTime"/>
  <rdfs:subPropertyOf rdf:resource="&pimo;datatypeProperty"/>
</rdf:Property>

<rdfs:Class rdf:about="&foaf;Person"
    rdfs:comment="A person."
    rdfs:label="Person"
    ns:term_status="stable">
  <rdfs:subClassOf rdf:resource="http://www.w3.org/2003/01/geo/wgs84_pos#SpatialThing"/>
  <rdfs:subClassOf rdf:resource="&foaf;Agent"/>
  <owl:disjointWith rdf:resource="&foaf;Organization"/>
  <owl:disjointWith rdf:resource="&foaf;Project"/>
  <owl:equivalentClass rdf:resource="http://schema.org/Person"/>
  <owl:equivalentClass rdf:resource="http://www.w3.org/2000/10/swap/pim/contact#Person"/>
  <rdf:type rdf:resource="&owl;Class"/>
  <rdfs:isDefinedBy rdf:resource="&foaf;"/>
</rdfs:Class>

<rdf:Property rdf:about="&pimo;attendingMeeting"
    rdfs:comment="the attended meeting"
    rdfs:label="attending meeting">
  <rdfs:domain rdf:resource="&pimo;Attendee"/>
  <rdfs:range rdf:resource="&pimo;SocialEvent"/>
  <rdfs:subPropertyOf rdf:resource="&pimo;roleContext"/>
</rdf:Property>

<rdf:Property rdf:about="&nid3;encodingSettings"
    rdfs:label="encodingSettings">
  <rdfs:comment>TSSE
The 'Software/Hardware and settings used for encoding' frame includes the used audio encoder and its settings when the file was encoded. Hardware refers to hardware encoders, not the computer on which a program was run.</rdfs:comment>
  <rdfs:domain rdf:resource="&nid3;ID3Audio"/>
  <rdfs:range rdf:resource="&xsd;string"/>
</rdf:Property>

<rdf:Property rdf:about="&dcterms;tableOfContents">
  <rdfs:subPropertyOf rdf:resource="&dc;description"/>
  <rdfs:subPropertyOf rdf:resource="&dcterms;description"/>
  <dcterms:hasVersion rdf:resource="http://dublincore.org/usage/terms/history/#tableOfContents-003"/>
  <dcterms:issued rdf:datatype="&xsd;date">2000-07-11</dcterms:issued>
  <dcterms:modified rdf:datatype="&xsd;date">2008-01-14</dcterms:modified>
  <rdfs:comment xml:lang="en">A list of subunits of the resource.</rdfs:comment>
  <rdfs:isDefinedBy rdf:resource="&dcterms;"/>
  <rdfs:label xml:lang="en">Table Of Contents</rdfs:label>
</rdf:Property>

<ncal:RecurrenceFrequency rdf:about="&ncal;secondly"
    rdfs:label="secondly"/>

<rdf:Property rdf:about="&nexif;userComment"
    rdfs:label="userComment">
  <rdfs:subPropertyOf rdf:resource="http://www.kanzaki.com/ns/exif#userComment"/>
  <rdfs:subPropertyOf rdf:resource="&nexif;userInfo"/>
  <rdfs:comment>tagNumber: 37510
A tag for Exif users to write keywords or comments on the image besides those in ImageDescription, and without the character code limitations of the ImageDescription tag. The character code used in the UserComment tag is identified based on an ID code in a fixed 8-byte area at the start of the tag data area.</rdfs:comment>
  <rdfs:domain rdf:resource="&nexif;Photo"/>
  <rdfs:range rdf:resource="&xsd;string"/>
</rdf:Property>

<rdfs:Class rdf:about="&ndo;TorrentedFile"
    rdfs:comment="A file available via a BitTorrent peer-to-peer network"
    rdfs:label="torrented file">
  <rdfs:subClassOf rdf:resource="&ndo;P2PFile"/>
</rdfs:Class>

<rdf:Property rdf:about="&foaf;img"
    rdfs:label="image"
    ns:term_status="testing">
  <rdf:type rdf:resource="&owl;ObjectProperty"/>
  <rdfs:comment>An image that can be used to represent some thing (ie. those depictions which are particularly representative of something, eg. one's photo on a homepage).</rdfs:comment>
  <rdfs:domain rdf:resource="&foaf;Person"/>
  <rdfs:isDefinedBy rdf:resource="&foaf;"/>
  <rdfs:range rdf:resource="&foaf;Image"/>
  <rdfs:subPropertyOf rdf:resource="&foaf;depiction"/>
</rdf:Property>

<rdfs:Class rdf:about="&tmo;Task"
    rdfs:label="Task">
  <rdfs:comment>The tmo:task is the central entitiey of the tmo. Task can range from vague things to be possibly done in e distant future to concrete things to be done in a precise forseeable manner. It is not unrealisitc to assume that knowledge worker have hundred or more tasks a day.</rdfs:comment>
  <rdfs:subClassOf rdf:resource="&pimo;Task"/>
</rdfs:Class>

<rdf:Property rdf:about="&nid3;leadArtist"
    rdfs:label="leadArtist">
  <rdfs:comment>TPE1
The 'Lead artist(s)/Lead performer(s)/Soloist(s)/Performing group' is used for the main artist(s). They are seperated with the "/" character.</rdfs:comment>
  <rdfs:domain rdf:resource="&nid3;ID3Audio"/>
  <rdfs:range rdf:resource="&nco;Contact"/>
  <rdfs:subPropertyOf rdf:resource="&dc;creator"/>
</rdf:Property>

<rdfs:Class rdf:about="&nco;ContactMedium"
    rdfs:label="ContactMedium">
  <rdfs:comment>A superclass for all contact media - ways to contact an entity represented by a Contact instance. Some of the subclasses of this class (the various kinds of telephone numbers and postal addresses) have been inspired by the values of the TYPE parameter of ADR and TEL properties defined in RFC 2426 sec. 3.2.1. and 3.3.1 respectively. Each value is represented by an appropriate subclass with two major exceptions TYPE=home and TYPE=work. They are to be expressed by the roles these contact media are attached to i.e. contact media with TYPE=home parameter are to be attached to the default role (nco:Contact or nco:PersonContact), whereas media with TYPE=work parameter should be attached to nco:Affiliation or nco:OrganizationContact.</rdfs:comment>
  <rdfs:subClassOf rdf:resource="&rdfs;Resource"/>
</rdfs:Class>

<owl:NamedIndividual rdf:about="&oa;describing">
  <rdf:type rdf:resource="&oa;Motivation"/>
  <rdfs:comment xml:lang="en">The motivation that represents a description of the target resource(s), as opposed to a comment about them. For example describing the above PDF's contents, rather than commenting on their accuracy.</rdfs:comment>
  <scos:inScheme rdf:resource="&oa;motivationScheme"/>
  <scos:prefLabel xml:lang="en">describing</scos:prefLabel>
</owl:NamedIndividual>

<rdf:Property rdf:about="&dcterms;dateSubmitted">
  <rdfs:subPropertyOf rdf:resource="&dc;date"/>
  <rdfs:subPropertyOf rdf:resource="&dcterms;date"/>
  <dcterms:description xml:lang="en">Examples of resources to which a Date Submitted may be relevant are a thesis (submitted to a university department) or an article (submitted to a journal).</dcterms:description>
  <dcterms:hasVersion rdf:resource="http://dublincore.org/usage/terms/history/#dateSubmitted-002"/>
  <dcterms:issued rdf:datatype="&xsd;date">2002-07-13</dcterms:issued>
  <dcterms:modified rdf:datatype="&xsd;date">2008-01-14</dcterms:modified>
  <rdfs:comment xml:lang="en">Date of submission of the resource.</rdfs:comment>
  <rdfs:isDefinedBy rdf:resource="&dcterms;"/>
  <rdfs:label xml:lang="en">Date Submitted</rdfs:label>
  <rdfs:range rdf:resource="&rdfs;Literal"/>
</rdf:Property>

<rdfs:Class rdf:about="&pimo;Document"
    rdfs:label="Document">
  <rdfs:comment>A generic document. This is a placeholder class for document-management domain ontologies to subclass. Create more and specified subclasses of pimo:Document for the document types in your domain. Documents are typically instances of both NFO:Document (modeling the information element used to store the document) and a LogicalMediaType subclass. Two examples are given for what to model here: a contract for a business domain, a BlogPost for an informal domain.</rdfs:comment>
  <rdfs:subClassOf rdf:resource="&pimo;LogicalMediaType"/>
</rdfs:Class>

<ncal:Weekday rdf:about="&ncal;thursday"
    rdfs:label="thursday"/>

<rdf:Property rdf:about="&dc;date">
  <dcterms:description xml:lang="en">Date may be used to express temporal information at any level of granularity.  Recommended best practice is to use an encoding scheme, such as the W3CDTF profile of ISO 8601 [W3CDTF].</dcterms:description>
  <dcterms:hasVersion rdf:resource="http://dublincore.org/usage/terms/history/#date-006"/>
  <dcterms:issued rdf:datatype="&xsd;date">1999-07-02</dcterms:issued>
  <dcterms:modified rdf:datatype="&xsd;date">2008-01-14</dcterms:modified>
  <rdf:type rdf:resource="&owl;AnnotationProperty"/>
  <rdfs:comment xml:lang="en">A point or period of time associated with an event in the lifecycle of the resource.</rdfs:comment>
  <rdfs:isDefinedBy rdf:resource="&dc;"/>
  <rdfs:label xml:lang="en">Date</rdfs:label>
  <scos:note xml:lang="en">A second property with the same name as this property has been declared in the dcterms: namespace (http://purl.org/dc/terms/).  See the Introduction to the document "DCMI Metadata Terms" (http://dublincore.org/documents/dcmi-terms/) for an explanation.</scos:note>
</rdf:Property>

<rdfs:Class rdf:about="&dplo;NotePost"
    rdfs:label="Note Post">
  <rdfs:comment>Represents a livepost referring to an online note, as defined by instances of nfo:RemoteDataObject, or known instances of pimo:Note.</rdfs:comment>
  <rdfs:subClassOf rdf:resource="&dplo;WebDocumentPost"/>
</rdfs:Class>

<rdfs:Class rdf:about="&nrl;ReflexiveProperty"
    rdfs:comment="A marker class to identify reflexive properties"
    rdfs:label="ReflexiveProperty">
  <rdfs:subClassOf rdf:resource="&rdfs;Resource"/>
</rdfs:Class>

<rdf:Property rdf:about="&dcon;connected"
    rdfs:label="Connected">
  <rdfs:comment>Specifies whether a network in range of the user's device(s) is connected (true) or otherwise (false) in the current context.</rdfs:comment>
  <rdfs:domain rdf:resource="&ddo;Network"/>
  <rdfs:range rdf:resource="&xsd;boolean"/>
  <rdfs:subPropertyOf rdf:resource="&dcon;hasContextAttribute"/>
</rdf:Property>

<rdf:Property rdf:about="&nco;hasIMCapability"
    rdfs:comment="Indicates that an IMAccount has a certain capability."
    rdfs:label="hasIMCapability">
  <rdfs:domain rdf:resource="&nco;IMAccount"/>
  <rdfs:range rdf:resource="&nco;IMCapability"/>
</rdf:Property>

<rdf:Property rdf:about="&dcon;currentWeather"
    rdfs:label="Current Weather">
  <rdfs:comment>Refers to a pre-defined weather condition characterising a context instance.</rdfs:comment>
  <rdfs:domain rdf:resource="&dcon;Environment"/>
  <rdfs:range rdf:resource="&dpo;WeatherConditions"/>
  <rdfs:subPropertyOf rdf:resource="&dcon;hasContextElement"/>
</rdf:Property>

<owl:Class rdf:about="&scos;Collection">
  <owl:disjointWith rdf:resource="&scos;Concept"/>
  <owl:disjointWith rdf:resource="&scos;ConceptScheme"/>
  <rdfs:isDefinedBy rdf:resource="http://www.w3.org/2004/02/skos/core"/>
  <rdfs:label xml:lang="en">Collection</rdfs:label>
  <scos:definition xml:lang="en">A meaningful collection of concepts.</scos:definition>
  <scos:scopeNote xml:lang="en">Labelled collections can be used where you would like a set of concepts to be displayed under a 'node label' in the hierarchy.</scos:scopeNote>
</owl:Class>

<rdf:Property rdf:about="http://www.w3.org/2003/01/geo/wgs84_pos#long"
    nrl:maxCardinality="1">
  <rdfs:range rdf:resource="&xsd;float"/>
  <rdfs:subPropertyOf rdf:resource="&pimo;datatypeProperty"/>
</rdf:Property>

<ncal:FreebusyType rdf:about="&ncal;busyUnavailableFreebusyType"
    rdfs:label="busyUnavailableFreebusyType"/>

<rdf:Property rdf:about="&dcterms;subject">
  <dcterms:description xml:lang="en">Typically, the subject will be represented using keywords, key phrases, or classification codes. Recommended best practice is to use a controlled vocabulary.</dcterms:description>
  <dcterms:hasVersion rdf:resource="http://dublincore.org/usage/terms/history/#subjectT-002"/>
  <dcterms:issued rdf:datatype="&xsd;date">2008-01-14</dcterms:issued>
  <dcterms:modified rdf:datatype="&xsd;date">2012-06-14</dcterms:modified>
  <rdfs:comment xml:lang="en">The topic of the resource.</rdfs:comment>
  <rdfs:isDefinedBy rdf:resource="&dcterms;"/>
  <rdfs:label xml:lang="en">Subject</rdfs:label>
  <rdfs:subPropertyOf rdf:resource="&dc;subject"/>
  <scos:note xml:lang="en">This term is intended to be used with non-literal values as defined in the DCMI Abstract Model (http://dublincore.org/documents/abstract-model/).  As of December 2007, the DCMI Usage Board is seeking a way to express this intention with a formal range declaration.</scos:note>
</rdf:Property>

<rdf:Property rdf:about="&nexif;dateTimeOriginal"
    rdfs:label="dateTimeOriginal">
  <rdfs:subPropertyOf rdf:resource="http://www.kanzaki.com/ns/exif#dateTimeOriginal"/>
  <rdfs:subPropertyOf rdf:resource="&nexif;date"/>
  <rdfs:subPropertyOf rdf:resource="&nexif;dateAndOrTime"/>
  <rdfs:comment>tagNumber: 36867
The date and time when the original image data was generated. For a DSC the date and time the picture was taken are recorded.</rdfs:comment>
  <rdfs:domain rdf:resource="&nexif;Photo"/>
  <rdfs:range rdf:resource="&xsd;dateTime"/>
</rdf:Property>

<rdf:Property rdf:about="&nfo;hasMediaFileListEntry"
    rdfs:label="hasMediaFileListEntry">
  <rdfs:comment>This property is intended to point to an RDF list of MediaFiles.</rdfs:comment>
  <rdfs:domain rdf:resource="&nfo;MediaList"/>
  <rdfs:range rdf:resource="&nfo;MediaFileListEntry"/>
</rdf:Property>

<rdf:Property rdf:about="&tmo;transmissionType"
    nrl:maxCardinality="1"
    nrl:minCardinality="1"
    rdfs:label="transmissionType">
  <rdfs:domain rdf:resource="&tmo;TaskTransmission"/>
  <rdfs:range rdf:resource="&tmo;TransmissionType"/>
  <rdfs:subPropertyOf rdf:resource="&tmo;stateTypeRole"/>
</rdf:Property>

<rdf:Property rdf:about="&nexif;gpsDestDistance"
    rdfs:comment="The distance to the destination point.
tagNumber: 26"
    rdfs:label="gpsDestDistance">
  <rdfs:subPropertyOf rdf:resource="http://www.kanzaki.com/ns/exif#gpsDestDistance"/>
  <rdfs:subPropertyOf rdf:resource="&nexif;gpsInfo"/>
  <rdfs:domain rdf:resource="&nexif;Photo"/>
  <rdfs:range rdf:resource="&xsd;string"/>
</rdf:Property>

<rdf:Property rdf:about="&nfo;paletteSize"
    rdfs:label="palette size">
  <nrl:maxCardinality rdf:datatype="&xsd;integer">1</nrl:maxCardinality>
  <rdfs:comment>The number of colors defined in palette of the raster image.</rdfs:comment>
  <rdfs:domain rdf:resource="&nfo;RasterImage"/>
  <rdfs:range rdf:resource="&xsd;integer"/>
</rdf:Property>

<rdf:Property rdf:about="&nao;modified"
    rdfs:comment="States the modification time for a resource"
    rdfs:label="modified at">
  <rdfs:subPropertyOf rdf:resource="&dcterms;modified"/>
  <rdfs:subPropertyOf rdf:resource="&nao;annotation"/>
  <rdfs:domain rdf:resource="&rdfs;Resource"/>
  <rdfs:range rdf:resource="&xsd;dateTime"/>
</rdf:Property>

<rdfs:Class rdf:about="&pimo;Thing"
    rdfs:label="Thing">
  <rdfs:subClassOf rdf:resource="&pimo;ClassOrThing"/>
  <rdfs:subClassOf rdf:resource="&rdfs;Resource"/>
  <rdfs:comment>Entities that are in the direct attention of the user when doing knowledge work.</rdfs:comment>
</rdfs:Class>

<rdfs:Class rdf:about="&rdf;Statement">
  <rdfs:comment xml:lang="en">The class of RDF statements.</rdfs:comment>
  <rdfs:isDefinedBy rdf:resource="&rdf;"/>
  <rdfs:label xml:lang="en">Statement</rdfs:label>
  <rdfs:subClassOf rdf:resource="&rdfs;Resource"/>
</rdfs:Class>

<rdf:Property rdf:about="&nexif;tagNumber"
    rdfs:comment="The Exif tag number (for this schema definition)"
    rdfs:label="tagNumber">
  <rdfs:subPropertyOf rdf:resource="&dc;identifier"/>
  <rdfs:subPropertyOf rdf:resource="http://www.kanzaki.com/ns/exif#tag_number"/>
  <rdfs:domain rdf:resource="&nexif;Photo"/>
  <rdfs:range rdf:resource="&xsd;string"/>
</rdf:Property>

<rdf:Property rdf:about="&ncal;resources"
    rdfs:label="resources">
  <rdfs:comment>Defines the equipment or resources anticipated for an activity specified by a calendar entity. Inspired by RFC 2445 sec. 4.8.1.10 with the following reservations:  the LANGUAGE parameter has been discarded. Please use xml:lang literals to express language. For the ALTREP parameter use the resourcesAltRep property. This property specifies multiple resources. The order is not important. it is recommended to introduce a separate triple for each resource.</rdfs:comment>
  <rdfs:domain rdf:resource="&ncal;UnionOfEventTodo"/>
  <rdfs:range rdf:resource="&xsd;string"/>
</rdf:Property>

<rdf:Property rdf:about="&dcterms;type">
  <dcterms:description xml:lang="en">Recommended best practice is to use a controlled vocabulary such as the DCMI Type Vocabulary [DCMITYPE]. To describe the file format, physical medium, or dimensions of the resource, use the Format element.</dcterms:description>
  <dcterms:hasVersion rdf:resource="http://dublincore.org/usage/terms/history/#typeT-001"/>
  <dcterms:issued rdf:datatype="&xsd;date">2008-01-14</dcterms:issued>
  <dcterms:modified rdf:datatype="&xsd;date">2008-01-14</dcterms:modified>
  <rdfs:comment xml:lang="en">The nature or genre of the resource.</rdfs:comment>
  <rdfs:isDefinedBy rdf:resource="&dcterms;"/>
  <rdfs:label xml:lang="en">Type</rdfs:label>
  <rdfs:range rdf:resource="&rdfs;Class"/>
  <rdfs:subPropertyOf rdf:resource="&dc;type"/>
</rdf:Property>

<rdfs:Class rdf:about="&tmo;TransmissionType"
    rdfs:label="TransmissionType">
  <rdfs:comment>By means of the TransmissionType one can distinguish several different types which might imply a different business logic. e.g. delegation can mean that the results of the task fulfillment care to be reported back to the sender of the task.</rdfs:comment>
  <rdfs:subClassOf rdf:resource="&tmo;StateTypeRole"/>
</rdfs:Class>

<rdf:Property rdf:about="&nmm;artwork"
    rdfs:comment="Associated Artwork"
    rdfs:label="artwork">
  <rdfs:domain rdf:resource="&nfo;Media"/>
  <rdfs:range rdf:resource="&nfo;Image"/>
  <rdfs:subPropertyOf rdf:resource="&nfo;depiction"/>
</rdf:Property>

<rdf:Property rdf:about="&nfo;filesystemType"
    rdfs:comment="Type of filesystem such as ext3 and ntfs."
    rdfs:label="filesystemType">
  <nrl:maxCardinality rdf:datatype="&xsd;integer">1</nrl:maxCardinality>
  <rdfs:domain rdf:resource="&nfo;Filesystem"/>
  <rdfs:range rdf:resource="&xsd;string"/>
</rdf:Property>

<rdf:Property rdf:about="&ncal;periodBegin"
    rdfs:label="periodBegin">
  <nrl:maxCardinality rdf:datatype="&xsd;integer">1</nrl:maxCardinality>
  <rdfs:comment>Beginng of a period. Inspired by the first part of a structured value of the PERIOD datatype specified in RFC 2445 sec. 4.3.9</rdfs:comment>
  <rdfs:domain rdf:resource="&ncal;NcalPeriod"/>
  <rdfs:range rdf:resource="&xsd;dateTime"/>
</rdf:Property>

<rdfs:Class rdf:about="&dplo;ActivityPost"
    rdfs:label="Activity Post">
  <rdfs:comment>Represents the live posting of information related to a user's detected or proclaimed activity, as defined by a set of instances of dpo:Activity.</rdfs:comment>
  <rdfs:subClassOf rdf:resource="&dplo;PresencePost"/>
</rdfs:Class>

<rdf:Property rdf:about="&nuao;targettedResource"
    rdfs:label="targetted resource">
  <nrl:minCardinality rdf:datatype="&xsd;nonNegativeInteger">1</nrl:minCardinality>
  <rdfs:comment>Relates an event to the resource that was targetted in the event.</rdfs:comment>
  <rdfs:domain rdf:resource="&nuao;Event"/>
  <rdfs:range rdf:resource="&nie;InformationElement"/>
  <rdfs:subPropertyOf rdf:resource="&nuao;involves"/>
</rdf:Property>

<owl:Class rdf:about="&oa;Annotation">
  <rdfs:comment xml:lang="en">Typically an Annotation has a single Body (oa:hasBody), which is the comment or other descriptive resource, and a single Target (oa:hasTarget) that the Body is somehow "about". The Body provides the information which is annotating the Target. 

This "aboutness" may be further clarified or extended to notions such as classifying or identifying with oa:motivatedBy.</rdfs:comment>
  <rdfs:isDefinedBy rdf:resource="&oa;"/>
  <rdfs:label xml:lang="en">Annotation</rdfs:label>
</owl:Class>

<rdf:Property rdf:about="&nmo;emailCc"
    rdfs:label="cc">
  <rdfs:comment>A Contact that is to receive a cc of the email. A cc (carbon copy) is a copy of an email message whose recipient appears on the recipient list, so that all other recipients are aware of it.</rdfs:comment>
  <rdfs:domain rdf:resource="&nmo;Email"/>
  <rdfs:range rdf:resource="&nco;ContactMedium"/>
  <rdfs:subPropertyOf rdf:resource="&nmo;secondaryMessageRecipient"/>
</rdf:Property>

<rdf:Property rdf:about="&nco;start"
    rdfs:label="start">
  <nrl:maxCardinality rdf:datatype="&xsd;integer">1</nrl:maxCardinality>
  <rdfs:comment>Start datetime for the role, such as: the datetime of joining a project or organization, datetime of starting employment, datetime of marriage</rdfs:comment>
  <rdfs:domain rdf:resource="&nco;Role"/>
  <rdfs:range rdf:resource="&xsd;dateTime"/>
</rdf:Property>

<rdfs:Class rdf:about="&rdf;Property">
  <rdfs:comment xml:lang="en">The class of RDF properties.</rdfs:comment>
  <rdfs:isDefinedBy rdf:resource="&rdf;"/>
  <rdfs:label xml:lang="en">Property</rdfs:label>
  <rdfs:subClassOf rdf:resource="&rdfs;Resource"/>
</rdfs:Class>

<rdf:Property rdf:about="&dcterms;relation">
  <dcterms:description xml:lang="en">Recommended best practice is to identify the related resource by means of a string conforming to a formal identification system. </dcterms:description>
  <dcterms:hasVersion rdf:resource="http://dublincore.org/usage/terms/history/#relationT-001"/>
  <dcterms:issued rdf:datatype="&xsd;date">2008-01-14</dcterms:issued>
  <dcterms:modified rdf:datatype="&xsd;date">2008-01-14</dcterms:modified>
  <rdfs:comment xml:lang="en">A related resource.</rdfs:comment>
  <rdfs:isDefinedBy rdf:resource="&dcterms;"/>
  <rdfs:label xml:lang="en">Relation</rdfs:label>
  <rdfs:subPropertyOf rdf:resource="&dc;relation"/>
  <scos:note xml:lang="en">This term is intended to be used with non-literal values as defined in the DCMI Abstract Model (http://dublincore.org/documents/abstract-model/).  As of December 2007, the DCMI Usage Board is seeking a way to express this intention with a formal range declaration.</scos:note>
</rdf:Property>

<rdfs:Class rdf:about="&dcterms;Frequency">
  <dcterms:hasVersion rdf:resource="http://dublincore.org/usage/terms/history/#Frequency-001"/>
  <dcterms:issued rdf:datatype="&xsd;date">2008-01-14</dcterms:issued>
  <rdfs:comment xml:lang="en">A rate at which something recurs.</rdfs:comment>
  <rdfs:isDefinedBy rdf:resource="&dcterms;"/>
  <rdfs:label xml:lang="en">Frequency</rdfs:label>
</rdfs:Class>

<owl:DatatypeProperty rdf:about="&oa;suffix">
  <rdfs:comment xml:lang="en">The snippet of text that occurs immediately after the text which is being selected. 

See oa:TextQuoteSelector.</rdfs:comment>
  <rdfs:domain rdf:resource="&oa;Selector"/>
  <rdfs:isDefinedBy rdf:resource="&oa;"/>
  <rdfs:label xml:lang="en">suffix</rdfs:label>
</owl:DatatypeProperty>

<rdf:Property rdf:about="&ncal;tzname"
    rdfs:label="tzname">
  <rdfs:comment>Specifies the customary designation for a timezone description. Inspired by RFC 2445 sec. 4.8.3.2 The LANGUAGE parameter has been discarded. Please xml:lang literals to express languages. Original specification for the domain of this property stated that it must appear within the timezone component. In this ontology the TimezoneObservance class has been itroduced to clarify this specification.</rdfs:comment>
  <rdfs:domain rdf:resource="&ncal;TimezoneObservance"/>
  <rdfs:range rdf:resource="&xsd;string"/>
</rdf:Property>

<rdf:Property rdf:about="&scos;changeNote">
  <rdf:type rdf:resource="&owl;AnnotationProperty"/>
  <rdfs:isDefinedBy rdf:resource="http://www.w3.org/2004/02/skos/core"/>
  <rdfs:label xml:lang="en">change note</rdfs:label>
  <rdfs:subPropertyOf rdf:resource="&scos;note"/>
  <scos:definition xml:lang="en">A note about a modification to a concept.</scos:definition>
</rdf:Property>

<rdf:Property rdf:about="&tmo;importance"
    nrl:maxCardinality="1"
    rdfs:label="importance">
  <rdfs:domain rdf:resource="&tmo;Task"/>
  <rdfs:range rdf:resource="&tmo;Importance"/>
  <rdfs:subPropertyOf rdf:resource="&tmo;timemanagement"/>
</rdf:Property>

<rdf:Property rdf:about="&nfo;width"
    rdfs:comment="Visual content width in pixels."
    rdfs:label="width">
  <nrl:maxCardinality rdf:datatype="&xsd;integer">1</nrl:maxCardinality>
  <rdfs:domain rdf:resource="&nfo;Visual"/>
  <rdfs:range rdf:resource="&xsd;integer"/>
</rdf:Property>

<rdf:Property rdf:about="&foaf;geekcode"
    rdfs:label="geekcode"
    ns:term_status="archaic">
  <rdf:type rdf:resource="&owl;DatatypeProperty"/>
  <rdfs:comment>A textual geekcode for this person, see http://www.geekcode.com/geek.html</rdfs:comment>
  <rdfs:domain rdf:resource="&foaf;Person"/>
  <rdfs:isDefinedBy rdf:resource="&foaf;"/>
  <rdfs:range rdf:resource="&rdfs;Literal"/>
</rdf:Property>

<rdf:Property rdf:about="&nexif;subjectDistance"
    rdfs:label="subjectDistance">
  <rdfs:subPropertyOf rdf:resource="http://www.kanzaki.com/ns/exif#subjectDistance"/>
  <rdfs:subPropertyOf rdf:resource="&nexif;meter"/>
  <rdfs:subPropertyOf rdf:resource="&nexif;pictTaking"/>
  <rdfs:comment>tagNumber: 37382
The distance to the subject, given in meters. Note that if the numerator of the recorded value is FFFFFFFF.H, Infinity shall be indicated; and if the numerator is 0, Distance unknown shall be indicated.</rdfs:comment>
  <rdfs:domain rdf:resource="&nexif;Photo"/>
  <rdfs:range rdf:resource="&xsd;float"/>
</rdf:Property>

<rdf:Property rdf:about="&nie;depends"
    rdfs:label="depends">
  <rdfs:comment>Dependency relation. A piece of content depends on another piece of data in order to be properly understood/used/interpreted.</rdfs:comment>
  <rdfs:range rdf:resource="&nie;DataObject"/>
  <rdfs:subPropertyOf rdf:resource="&nie;relatedTo"/>
</rdf:Property>

<rdf:Property rdf:about="&ncal;until"
    rdfs:label="until">
  <rdfs:comment>The UNTIL rule part defines a date-time value which bounds the recurrence rule in an inclusive manner. If the value specified by UNTIL is synchronized with the specified recurrence, this date or date-time becomes the last instance of the recurrence. If specified as a date-time value, then it MUST be specified in an UTC time format. If not present, and the COUNT rule part is also not present, the RRULE is considered to repeat forever.</rdfs:comment>
  <rdfs:domain rdf:resource="&ncal;RecurrenceRule"/>
  <rdfs:range rdf:resource="&xsd;dateTime"/>
</rdf:Property>

<rdf:Property rdf:about="&dpo;minHumidity"
    rdfs:label="Minimum Humidity">
  <rdfs:comment>A subproperty of dpo:minValue that defines a lowerbound on the observed humidity value (as a percentage) such that it can classify as a dpo:WeatherCondition instance. It can be used in conjunction with dpo:maxHumidity to state that specific instances of dpo:WeatherCondition have a pre-defined range of observable real-world humidity levels. In addition, they can also be used with various other weather conditions values and ranges to define complex weather condition types.</rdfs:comment>
  <rdfs:domain rdf:resource="&dpo;WeatherConditions"/>
  <rdfs:range rdf:resource="&xsd;nonNegativeInteger"/>
  <rdfs:subPropertyOf rdf:resource="&dpo;minValue"/>
</rdf:Property>

<rdf:Property rdf:about="&dcon;averageDirection"
    rdfs:label="Average Direction">
  <rdfs:comment>Refers to a pre-defined traveling direction characterising a context instance.</rdfs:comment>
  <rdfs:domain rdf:resource="&dcon;SpaTem"/>
  <rdfs:range rdf:resource="&dpo;Direction"/>
  <rdfs:subPropertyOf rdf:resource="&dcon;hasContextElement"/>
</rdf:Property>

<rdfs:Class rdf:about="&tmo;PredecessorSuccessorDependency"
    protege:role="abstract"
    rdfs:label="PredecessorSuccessorDependency">
  <rdfs:comment>The PredecessorSuccessorDependency enables a directed relation between task. By means of the concrete sublcasses one can further distinguish from which point of view this relation is created.</rdfs:comment>
  <rdfs:subClassOf rdf:resource="&tmo;TaskDependency"/>
</rdfs:Class>

<ncal:AlarmAction rdf:about="&ncal;emailAction"
    rdfs:label="emailAction"/>

<rdf:Property rdf:about="&pimo;jabberId"
    nrl:maxCardinality="1"
    rdfs:label="jabber ID of the user">
  <rdfs:comment>Jabber-ID of the user. Used to communicate amongst peers in the social scenario of the semantic desktop. Use the xmpp node identifier as specified by RFC3920, see http://www.xmpp.org/specs/rfc3920.html#addressing-node. The format is the same as e-mail addresses: username@hostname.</rdfs:comment>
  <rdfs:domain rdf:resource="&pimo;Person"/>
  <rdfs:range rdf:resource="&rdfs;Literal"/>
</rdf:Property>

<rdf:Property rdf:about="&ncal;interval"
    rdfs:label="interval">
  <nrl:maxCardinality rdf:datatype="&xsd;integer">1</nrl:maxCardinality>
  <rdfs:comment>The INTERVAL rule part contains a positive integer representing how often the recurrence rule repeats. The default value is "1", meaning every second for a SECONDLY rule, or every minute for a MINUTELY rule, every hour for an HOURLY rule, every day for a DAILY rule, every week for a WEEKLY rule, every month for a MONTHLY rule andevery year for a YEARLY rule. Defined in RFC 2445 sec. 4.3.10</rdfs:comment>
  <rdfs:domain rdf:resource="&ncal;RecurrenceRule"/>
  <rdfs:range rdf:resource="&xsd;integer"/>
</rdf:Property>

<rdf:Property rdf:about="&nid3;audiofileSize"
    rdfs:label="audiofileSize">
  <rdfs:comment>TSIZ
The 'Size' frame contains the size of the audiofile in bytes, excluding the ID3v2 tag, represented as a numeric string.</rdfs:comment>
  <rdfs:domain rdf:resource="&nid3;ID3Audio"/>
  <rdfs:range rdf:resource="&xsd;integer"/>
</rdf:Property>

<rdf:Property rdf:about="&nco;birthDate"
    rdfs:label="birthDate">
  <nrl:maxCardinality rdf:datatype="&xsd;integer">1</nrl:maxCardinality>
  <rdfs:comment>Birth date of the object represented by this Contact. An equivalent of the 'BDAY' property as defined in RFC 2426 Sec. 3.1.5.</rdfs:comment>
  <rdfs:domain rdf:resource="&nco;BirthDate"/>
  <rdfs:range rdf:resource="&xsd;date"/>
  <rdfs:subPropertyOf rdf:resource="&dc;date"/>
</rdf:Property>

<rdf:Description rdf:about="&owl;Thing"
    rdfs:label="Thing"/>

<rdf:Property rdf:about="&dcon;month"
    rdfs:label="Month">
  <rdfs:comment>Derived from the dateTime, this property stores the number of months elapsed for the current year, where 1 indicates January, and 12 December.</rdfs:comment>
  <rdfs:domain rdf:resource="&dpo;TimePeriod"/>
  <rdfs:range rdf:resource="&xsd;nonNegativeInteger"/>
  <rdfs:subPropertyOf rdf:resource="&dcon;hasContextAttribute"/>
</rdf:Property>

<rdfs:Class rdf:about="&nco;ParcelDeliveryAddress"
    rdfs:label="ParcelDeliveryAddress">
  <rdfs:comment>Parcel Delivery Addresse. Class inspired by TYPE=parcel parameter of the ADR property defined in RFC 2426 sec. 3.2.1</rdfs:comment>
  <rdfs:subClassOf rdf:resource="&nco;PostalAddress"/>
</rdfs:Class>

<rdf:Property rdf:about="&dcon;upcomingTask"
    rdfs:label="Upcoming Task">
  <rdfs:comment>Refers to an upcoming task characterising a context instance.</rdfs:comment>
  <rdfs:domain rdf:resource="&dcon;Schedule"/>
  <rdfs:range rdf:resource="&ncal;Todo"/>
  <rdfs:subPropertyOf rdf:resource="&dcon;hasContextElement"/>
</rdf:Property>

<rdfs:Class rdf:about="&ddo;PersonalAreaNetwork"
    rdfs:label="PersonalAreaNetwork">
  <rdfs:comment>A Personal Area Network (PAN) is a computer network that enables intrapersonal communication amongst personal computerised devices. PANs can also be used to connect to a higher level network (including the Internet).</rdfs:comment>
  <rdfs:subClassOf rdf:resource="&ddo;ComputerNetwork"/>
</rdfs:Class>

<rdf:Property rdf:about="&dao;accountType"
    rdfs:label="accountType">
  <nrl:maxCardinality rdf:datatype="&xsd;nonNegativeInteger">1</nrl:maxCardinality>
  <rdfs:comment>Type of the account. This may be the name of the service where the account is created in. Examples might include Facebook, Twitter, di.me, etc.</rdfs:comment>
  <rdfs:domain rdf:resource="&dao;Account"/>
  <rdfs:range rdf:resource="&xsd;string"/>
</rdf:Property>

<rdf:Property rdf:about="&nmo;references"
    rdfs:label="references">
  <rdfs:comment>Signifies that a message references another message. This property is a generic one. See RFC 2822 Sec. 3.6.4</rdfs:comment>
  <rdfs:domain rdf:resource="&nmo;Message"/>
  <rdfs:range rdf:resource="&nmo;Message"/>
</rdf:Property>

<rdf:Property rdf:about="&nmo;primaryMessageRecipient"
    rdfs:comment="The primary intended recipient of a message."
    rdfs:label="primaryRecipient">
  <rdfs:domain rdf:resource="&nmo;Message"/>
  <rdfs:range rdf:resource="&nco;ContactMedium"/>
  <rdfs:subPropertyOf rdf:resource="&nmo;messageRecipient"/>
</rdf:Property>

<rdf:Property rdf:about="&dpo;minNoiseLevel"
    rdfs:label="Minimum Noise Level">
  <rdfs:comment>A subproperty of dpo:minValue that defines an lowerbound on the observed loudness level value (in decibels) such that it can classify as a dpo:Noise instance. It can be used in conjunction with dpo:maxNoiseLevel, i.e. specific instances of dpo:Noise have a pre-defined range of observable real-world surrounding noise levels.</rdfs:comment>
  <rdfs:domain rdf:resource="&dpo;Noise"/>
  <rdfs:range rdf:resource="&xsd;float"/>
  <rdfs:subPropertyOf rdf:resource="&dpo;minValue"/>
</rdf:Property>

<rdf:Property rdf:about="&dcterms;accrualPeriodicity">
  <dcterms:hasVersion rdf:resource="http://dublincore.org/usage/terms/history/#accrualPeriodicity-003"/>
  <dcterms:issued rdf:datatype="&xsd;date">2005-06-13</dcterms:issued>
  <dcterms:modified rdf:datatype="&xsd;date">2010-10-11</dcterms:modified>
  <rdfs:comment xml:lang="en">The frequency with which items are added to a collection.</rdfs:comment>
  <rdfs:domain rdf:resource="&dctypes;Collection"/>
  <rdfs:isDefinedBy rdf:resource="&dcterms;"/>
  <rdfs:label xml:lang="en">Accrual Periodicity</rdfs:label>
  <rdfs:range rdf:resource="&dcterms;Frequency"/>
</rdf:Property>

<rdf:Property rdf:about="&nao;altSymbol"
    rdfs:comment="An alternative symbol representation for a resource"
    rdfs:label="alternative symbol">
  <rdfs:domain rdf:resource="&rdfs;Resource"/>
  <rdfs:range rdf:resource="&nao;Symbol"/>
  <rdfs:subPropertyOf rdf:resource="&nao;hasSymbol"/>
</rdf:Property>

<rdfs:Class rdf:about="&dctypes;Event">
  <dcam:memberOf rdf:resource="&dcterms;DCMIType"/>
  <dcterms:description xml:lang="en">Metadata for an event provides descriptive information that is the basis for discovery of the purpose, location, duration, and responsible agents associated with an event. Examples include an exhibition, webcast, conference, workshop, open day, performance, battle, trial, wedding, tea party, conflagration.</dcterms:description>
  <dcterms:hasVersion rdf:resource="http://dublincore.org/usage/terms/history/#Event-003"/>
  <dcterms:issued rdf:datatype="&xsd;date">2000-07-11</dcterms:issued>
  <dcterms:modified rdf:datatype="&xsd;date">2008-01-14</dcterms:modified>
  <rdfs:comment xml:lang="en">A non-persistent, time-based occurrence.</rdfs:comment>
  <rdfs:isDefinedBy rdf:resource="&dctypes;"/>
  <rdfs:label xml:lang="en">Event</rdfs:label>
</rdfs:Class>

<rdfs:Class rdf:about="&nfo;Image"
    rdfs:comment="A file containing an image."
    rdfs:label="Image">
  <rdfs:subClassOf rdf:resource="&nfo;Visual"/>
</rdfs:Class>

<rdf:Property rdf:about="&nexif;sensingMethod"
    rdfs:label="sensingMethod">
  <rdfs:subPropertyOf rdf:resource="http://www.kanzaki.com/ns/exif#sensingMethod"/>
  <rdfs:subPropertyOf rdf:resource="&nexif;pictTaking"/>
  <rdfs:comment>tagNumber: 41495
The image sensor type on the camera or input device, such as One-chip color area sensor etc.</rdfs:comment>
  <rdfs:domain rdf:resource="&nexif;Photo"/>
  <rdfs:range rdf:resource="&xsd;string"/>
</rdf:Property>

<rdf:Property rdf:about="&nmm;musicAlbum"
    rdfs:comment="Album the music belongs to"
    rdfs:label="album">
  <nrl:maxCardinality rdf:datatype="&xsd;integer">1</nrl:maxCardinality>
  <rdfs:domain rdf:resource="&nmm;MusicPiece"/>
  <rdfs:range rdf:resource="&nmm;MusicAlbum"/>
  <rdfs:subPropertyOf rdf:resource="&nie;isLogicalPartOf"/>
</rdf:Property>

<rdf:Property rdf:about="&dcterms;audience">
  <dcterms:hasVersion rdf:resource="http://dublincore.org/usage/terms/history/#audience-003"/>
  <dcterms:issued rdf:datatype="&xsd;date">2001-05-21</dcterms:issued>
  <dcterms:modified rdf:datatype="&xsd;date">2008-01-14</dcterms:modified>
  <rdfs:comment xml:lang="en">A class of entity for whom the resource is intended or useful.</rdfs:comment>
  <rdfs:isDefinedBy rdf:resource="&dcterms;"/>
  <rdfs:label xml:lang="en">Audience</rdfs:label>
  <rdfs:range rdf:resource="&dcterms;AgentClass"/>
</rdf:Property>

<owl:NamedIndividual rdf:about="&oa;classifying">
  <rdf:type rdf:resource="&oa;Motivation"/>
  <rdfs:comment xml:lang="en">The motivation that represents the assignment of a classification type, typically from a controlled vocabulary, to the target resource(s). For example to classify an Image resource as a Portrait.</rdfs:comment>
  <scos:inScheme rdf:resource="&oa;motivationScheme"/>
  <scos:prefLabel xml:lang="en">classifying</scos:prefLabel>
</owl:NamedIndividual>

<rdfs:Class rdf:about="&dcon;Element"
    rdfs:label="Element">
  <rdfs:comment>Each context Aspect has a number of specific elements. These are linked to each aspect through the generic dcon:hasContextElement property. As this is an abstract class, it is not intended for direct use. Instead, element instances are typically inferred through the use of dcon:hasContextElement (and its subproperties) and dcon:hasObservation. Elements can have multiple observations (e.g. from a different source or device), linked through dcon:hasObservation.</rdfs:comment>
</rdfs:Class>

<rdfs:Class rdf:about="&nuao;ModificationEvent"
    rdfs:label="desktop event">
  <rdfs:comment>An event that lead to changes of the resource that are meaningful to the user</rdfs:comment>
  <rdfs:subClassOf rdf:resource="&nuao;DesktopEvent"/>
</rdfs:Class>

<rdfs:Class rdf:about="&nrl;RuleViewSpecification"
    rdfs:label="RuleViewSpecification">
  <rdfs:comment>Represents a view specification that is composed of a set of rules which generate the required view from the input graph upon firing</rdfs:comment>
  <rdfs:subClassOf rdf:resource="&nrl;ViewSpecification"/>
</rdfs:Class>

<nrl:InverseFunctionalProperty rdf:about="&nie;hasPart"
    rdfs:label="hasPart">
  <rdfs:subPropertyOf rdf:resource="&dcterms;hasPart"/>
  <rdfs:subPropertyOf rdf:resource="&nie;relatedTo"/>
  <nao:userVisible rdf:datatype="&xsd;boolean">false</nao:userVisible>
  <nrl:inverseProperty rdf:resource="&nie;isPartOf"/>
  <rdf:type rdf:resource="&rdf;Property"/>
  <rdfs:comment>Generic property used to express 'physical' containment relationships between DataObjects. NIE extensions are encouraged to provide more specific subproperties of this one. It is advisable for actual instances of DataObjects to use those specific subproperties. Note to the developers: Please be aware of the distinction between containment relation and provenance. The hasPart relation models physical containment, an InformationElement (a nmo:Message) can have a 'physical' part (an nfo:Attachment).  Also, please note the difference between physical containment (hasPart) and logical containment (hasLogicalPart) the former has more strict meaning. They may occur independently of each other.</rdfs:comment>
  <rdfs:domain rdf:resource="&nie;InformationElement"/>
  <rdfs:range rdf:resource="&nie;DataObject"/>
</nrl:InverseFunctionalProperty>

<rdf:Property rdf:about="&nco;hasEmailAddress"
    rdfs:label="hasEmailAddress">
  <rdfs:comment>An address for electronic mail communication with the object specified by this contact. An equivalent of the 'EMAIL' property as defined in RFC 2426 Sec. 3.3.1.</rdfs:comment>
  <rdfs:domain rdf:resource="&nco;Role"/>
  <rdfs:range rdf:resource="&nco;EmailAddress"/>
  <rdfs:subPropertyOf rdf:resource="&nco;hasContactMedium"/>
</rdf:Property>

<rdf:Property rdf:about="&nmo;inReplyTo"
    rdfs:label="inReplyTo">
  <nrl:maxCardinality rdf:datatype="&xsd;integer">1</nrl:maxCardinality>
  <rdfs:comment>Signifies that a message is a reply to another message. This feature is commonly used to link messages into conversations. Note that it is more specific than nmo:references. See RFC 2822 sec. 3.6.4</rdfs:comment>
  <rdfs:domain rdf:resource="&nmo;Message"/>
  <rdfs:range rdf:resource="&nmo;Message"/>
  <rdfs:subPropertyOf rdf:resource="&nmo;references"/>
</rdf:Property>

<rdfs:Class rdf:about="&nfo;FileDataObject"
    rdfs:label="file">
  <rdfs:comment>A resource containing a finite sequence of bytes with arbitrary information, that is available to a computer program and is usually based on some kind of durable storage. A file is durable in the sense that it remains available for programs to use after the current program has finished.</rdfs:comment>
  <rdfs:subClassOf rdf:resource="&nie;DataObject"/>
</rdfs:Class>

<tmo:PersonInvolvementRole rdf:about="&tmo;TMO_Instance_PersonInvolvementRole_Related"
    rdfs:label="TMO_Instance_PersonInvolvementRole_Related"/>

<rdfs:Class rdf:about="&rdf;List">
  <rdfs:comment xml:lang="en">The class of RDF Lists.</rdfs:comment>
  <rdfs:isDefinedBy rdf:resource="&rdf;"/>
  <rdfs:label xml:lang="en">List</rdfs:label>
  <rdfs:subClassOf rdf:resource="&rdfs;Resource"/>
</rdfs:Class>

<nrl:DefiningProperty rdf:about="&nie;url"
    nrl:maxCardinality="1"
    rdfs:label="url">
  <rdf:type rdf:resource="&rdf;Property"/>
  <rdfs:comment>URL of a DataObject. It points to the location of the object. A typial usage is FileDataObject. In cases where creating a simple file:// or http:// URL for a file is difficult (e.g. for files inside compressed archives) the applications are encouraged to use conventions defined by Apache Commons VFS Project at http://jakarta.apache.org/  commons/ vfs/ filesystems.html.</rdfs:comment>
  <rdfs:domain rdf:resource="&nie;DataObject"/>
  <rdfs:range rdf:resource="&rdfs;Resource"/>
</nrl:DefiningProperty>

<rdfs:Class rdf:about="&pimo;Location"
    rdfs:label="Location">
  <rdfs:subClassOf rdf:resource="&pimo;Thing"/>
  <rdfs:subClassOf rdf:resource="http://www.w3.org/2003/01/geo/wgs84_pos#SpatialThing"/>
  <rdfs:comment>A physical location. Subclasses are modeled for the most common locations humans work in: Building, City, Country, Room, State. This selection is intended to be applicable cross-cultural and cross-domain. City is a prototype that can be further refined for villages, etc. Subclass of a WGS84:SpatialThing, can have geo-coordinates.</rdfs:comment>
</rdfs:Class>

<rdf:Property rdf:about="&nid3;date"
    rdfs:label="date">
  <rdfs:comment>TDAT
The 'Date' frame is a numeric string in the DDMM format containing the date for the recording. This field is always four characters long.</rdfs:comment>
  <rdfs:domain rdf:resource="&nid3;ID3Audio"/>
  <rdfs:range rdf:resource="&xsd;dateTime"/>
  <rdfs:subPropertyOf rdf:resource="&nie;contentCreated"/>
</rdf:Property>

<rdf:Property rdf:about="&nexif;gps"
    rdfs:label="gps">
  <rdfs:comment>The location where the picture has been made. This property aggregates values of two properties from the original EXIF specification: gpsLatitute (tag number 2) and gpsLongitude (tag number 4), and gpsAltitude (tag number 6).</rdfs:comment>
  <rdfs:domain rdf:resource="&nexif;Photo"/>
  <rdfs:range rdf:resource="http://www.w3.org/2003/01/geo/wgs84_pos#Point"/>
  <rdfs:subPropertyOf rdf:resource="&nexif;geo"/>
</rdf:Property>

<rdfs:Class rdf:about="&ddo;CellularNetwork"
    rdfs:comment="A cell-based radio network that enables mobile telephony."
    rdfs:label="CellularNetwork">
  <rdfs:subClassOf rdf:resource="&ddo;Network"/>
</rdfs:Class>

<rdfs:Class rdf:about="&ncal;UnionOfEventJournalTodo"
    rdfs:label="UnionOfEventJournalTodo">
  <rdfs:subClassOf rdf:resource="&ncal;UnionParentClass"/>
</rdfs:Class>

<nco:IMStatusType rdf:about="&nco;IMStatusTypeAvailable"
    rdfs:label="available"/>

<rdf:Property rdf:about="&nid3;length"
    rdfs:label="length">
  <rdfs:comment>TLEN
The 'Length' frame contains the length of the audiofile in milliseconds, represented as a numeric string.</rdfs:comment>
  <rdfs:domain rdf:resource="&nid3;ID3Audio"/>
  <rdfs:range rdf:resource="&rdfs;Literal"/>
</rdf:Property>

<rdf:Property rdf:about="&dplo;hasReply"
    rdfs:label="has reply">
  <nrl:inverseProperty rdf:resource="&dplo;replyOf"/>
  <rdfs:comment>Links a livepost to its reply or response, also in the form of a livepost. This property is transitive, and is the inverse of dlpo:replyOf.</rdfs:comment>
  <rdfs:domain rdf:resource="&dplo;LivePost"/>
  <rdfs:range rdf:resource="&dplo;LivePost"/>
  <rdfs:subPropertyOf rdf:resource="http://rdfs.org/sioc/ns#has_reply"/>
</rdf:Property>

<rdf:Property rdf:about="&nexif;isoSpeedRatings"
    rdfs:label="isoSpeedRatings">
  <rdfs:subPropertyOf rdf:resource="http://www.kanzaki.com/ns/exif#isoSpeedRatings"/>
  <rdfs:subPropertyOf rdf:resource="&nexif;pictTaking"/>
  <rdfs:comment>Indicates the ISO Speed and ISO Latitude of the camera or input device as specified in ISO 12232.
tagNumber: 34855</rdfs:comment>
  <rdfs:domain rdf:resource="&nexif;Photo"/>
  <rdfs:range rdf:resource="&xsd;integer"/>
</rdf:Property>

<rdf:Property rdf:about="&nexif;samplesPerPixel"
    rdfs:label="samplesPerPixel">
  <rdfs:subPropertyOf rdf:resource="http://www.kanzaki.com/ns/exif#samplesPerPixel"/>
  <rdfs:subPropertyOf rdf:resource="&nexif;imageDataStruct"/>
  <rdfs:comment>The number of components per pixel. Since this standard applies to RGB and YCbCr images, the value set for this tag is 3. In JPEG compressed data a JPEG marker is used instead of this tag.
tagNumber: 277</rdfs:comment>
  <rdfs:domain rdf:resource="&nexif;Photo"/>
  <rdfs:range rdf:resource="&xsd;integer"/>
</rdf:Property>

<rdf:Property rdf:about="&ncal;dtend"
    rdfs:label="dtend">
  <nrl:maxCardinality rdf:datatype="&xsd;integer">1</nrl:maxCardinality>
  <rdfs:comment>This property specifies the date and time that a calendar component ends. Inspired by RFC 2445 sec. 4.8.2.2</rdfs:comment>
  <rdfs:domain rdf:resource="&ncal;UnionOfEventFreebusy"/>
  <rdfs:range rdf:resource="&ncal;NcalDateTime"/>
</rdf:Property>

<rdf:Property rdf:about="&nao;serializationLanguage"
    rdfs:label="serialization language">
  <nrl:maxCardinality rdf:datatype="&xsd;nonNegativeInteger">1</nrl:maxCardinality>
  <rdfs:comment>States the serialization language for a named graph that is represented within a document</rdfs:comment>
  <rdfs:domain rdf:resource="&nrl;DocumentGraph"/>
  <rdfs:range rdf:resource="&rdfs;Literal"/>
</rdf:Property>

<rdfs:Class rdf:about="&nco;VideoTelephoneNumber"
    rdfs:label="VideoTelephoneNumber">
  <rdfs:comment>A Video telephone number. A class inspired by the TYPE=video parameter of the TEL property defined in RFC 2426 sec. 3.3.1</rdfs:comment>
  <rdfs:subClassOf rdf:resource="&nco;VoicePhoneNumber"/>
</rdfs:Class>

<rdf:Property rdf:about="&nfo;encryptionStatus"
    rdfs:comment="The status of the encryption of the InformationElement."
    rdfs:label="encryptionStatus">
  <nrl:maxCardinality rdf:datatype="&xsd;integer">1</nrl:maxCardinality>
  <rdfs:domain rdf:resource="&nie;InformationElement"/>
  <rdfs:range rdf:resource="&nfo;EncryptionStatus"/>
</rdf:Property>

<rdf:Property rdf:about="&ncal;relatedToChild"
    rdfs:label="relatedToChild">
  <rdfs:comment>The property is used to represent a relationship or reference between one calendar component and another. Inspired by RFC 2445 sec. 4.8.4.5. Originally this property had a RELTYPE parameter. It has been decided to introduce three different properties to express the values of that parameter. This property expresses the RELATED-TO property with RELTYPE=CHILD parameter.</rdfs:comment>
  <rdfs:domain rdf:resource="&ncal;UnionOfEventJournalTodo"/>
  <rdfs:range rdf:resource="&xsd;string"/>
  <rdfs:subPropertyOf rdf:resource="&ncal;ncalRelation"/>
</rdf:Property>

<rdf:Property rdf:about="&nuao;usageCount"
    rdfs:comment="The total number of usages"
    rdfs:label="usage count">
  <nrl:maxCardinality rdf:datatype="&xsd;nonNegativeInteger">1</nrl:maxCardinality>
  <rdfs:domain rdf:resource="&rdfs;Resource"/>
  <rdfs:range rdf:resource="&xsd;nonNegativeInteger"/>
  <rdfs:subPropertyOf rdf:resource="&nuao;eventCount"/>
</rdf:Property>

<rdf:Property rdf:about="&ncal;statusDescription"
    rdfs:label="statusDescription">
  <nrl:maxCardinality rdf:datatype="&xsd;integer">1</nrl:maxCardinality>
  <rdfs:comment>Longer return status description. Inspired by the second part of the structured value of the REQUEST-STATUS property defined in RFC 2445 sec. 4.8.8.2</rdfs:comment>
  <rdfs:domain rdf:resource="&ncal;RequestStatus"/>
  <rdfs:range rdf:resource="&xsd;string"/>
</rdf:Property>

<rdf:Property rdf:about="&cnt;systemId">
  <rdf:type rdf:resource="&owl;ObjectProperty"/>
  <rdfs:comment xml:lang="en">The document type declarations's system identifier (typed: xsd:anyURI)</rdfs:comment>
  <rdfs:domain rdf:resource="&cnt;DoctypeDecl"/>
  <rdfs:label xml:lang="en">System ID</rdfs:label>
  <rdfs:range rdf:resource="&xsd;anyURI"/>
</rdf:Property>

<rdf:Property rdf:about="&nco;nameGiven"
    nrl:maxCardinality="1"
    rdfs:label="nameGiven">
  <rdfs:comment>The given name for the object represented by this Contact. See documentation for 'nameFamily' property for details.</rdfs:comment>
  <rdfs:domain rdf:resource="&nco;PersonName"/>
  <rdfs:range rdf:resource="&xsd;string"/>
</rdf:Property>

<rdfs:Class rdf:about="&nfo;Attachment"
    rdfs:label="Attachment">
  <rdfs:comment>A file attached to another data object. Many data formats allow for attachments: emails, vcards, ical events, id3 and exif...</rdfs:comment>
  <rdfs:subClassOf rdf:resource="&nfo;EmbeddedFileDataObject"/>
</rdfs:Class>

<tmo:TaskContainer rdf:about="&tmo;TMO_Instance_TaskContainer_trashtasks"
    rdfs:label="TMO_Instance_TaskContainer_trashtasks"/>

<tmo:TaskState rdf:about="&tmo;TMO_Instance_TaskState_Archived"
    rdfs:label="TMO_Instance_TaskState_Archived"/>

<rdf:Property rdf:about="&nie;dataSource"
    nrl:minCardinality="1"
    rdfs:label="dataSource">
  <rdfs:comment>Marks the provenance of a DataObject, what source does a data object come from.</rdfs:comment>
  <rdfs:domain rdf:resource="&nie;DataObject"/>
  <rdfs:range rdf:resource="&nie;DataSource"/>
  <rdfs:subPropertyOf rdf:resource="&dc;source"/>
</rdf:Property>

<rdf:Property rdf:about="&dpo;minWindScale"
    rdfs:label="Minimum Wind Scale">
  <rdfs:comment>A subproperty of dpo:minValue that defines a lowerbound on the observed windscale (on the Beaufort scale) such that it can classify as a dpo:WeatherCondition instance. It can be used in conjunction with dpo:maxWindScale to state that specific instances of dpo:WeatherCondition have a pre-defined range of observable real-world wind levels. In addition, they can also be used with various other weather conditions values and ranges to define complex weather condition types.</rdfs:comment>
  <rdfs:domain rdf:resource="&dpo;WeatherConditions"/>
  <rdfs:range rdf:resource="&xsd;nonNegativeInteger"/>
  <rdfs:subPropertyOf rdf:resource="&dpo;minValue"/>
</rdf:Property>

<rdf:Property rdf:about="&dpo;maxWindScale"
    rdfs:label="Maximum Wind Scale">
  <rdfs:comment>A subproperty of dpo:maxValue that defines an upperbound on the observed windscale (on the Beaufort scale) such that it can classify as a dpo:WeatherCondition instance. It can be used in conjunction with dpo:minWindScale to state that specific instances of dpo:WeatherCondition have a pre-defined range of observable real-world wind levels. In addition, they can also be used with various other weather conditions values and ranges to define complex weather condition types.</rdfs:comment>
  <rdfs:domain rdf:resource="&dpo;WeatherConditions"/>
  <rdfs:range rdf:resource="&xsd;nonNegativeInteger"/>
  <rdfs:subPropertyOf rdf:resource="&dpo;maxValue"/>
</rdf:Property>

<rdfs:Class rdf:about="&nfo;MediaStream"
    rdfs:label="MediaStream">
  <rdfs:comment>A stream of multimedia content, usually contained within a media container such as a movie (containing both audio and video) or a DVD (possibly containing many streams of audio and video). Most common interpretations for such a DataObject include Audio and Video.</rdfs:comment>
  <rdfs:subClassOf rdf:resource="&nie;DataObject"/>
</rdfs:Class>

<rdf:Property rdf:about="&nexif;jpegInterchangeFormatLength"
    rdfs:label="jpegInterchangeFormatLength">
  <rdfs:subPropertyOf rdf:resource="http://www.kanzaki.com/ns/exif#jpegInterchangeFormatLength"/>
  <rdfs:subPropertyOf rdf:resource="&nexif;recOffset"/>
  <rdfs:comment>The number of bytes of JPEG compressed thumbnail data. This is not used for primary image JPEG data.
tagNumber: 514</rdfs:comment>
  <rdfs:domain rdf:resource="&nexif;Photo"/>
  <rdfs:range rdf:resource="&xsd;integer"/>
</rdf:Property>

<rdf:Property rdf:about="&nid3;title"
    rdfs:label="title">
  <nao:deprecated rdf:datatype="&xsd;boolean">true</nao:deprecated>
  <rdfs:comment>TIT2
The 'Title/Songname/Content description' frame is the actual name of the piece (e.g. "Adagio", "Hurricane Donna"). Deprecated in favor of the more generic nie:title.</rdfs:comment>
  <rdfs:domain rdf:resource="&nid3;ID3Audio"/>
  <rdfs:range rdf:resource="&xsd;string"/>
  <rdfs:subPropertyOf rdf:resource="&nie;title"/>
</rdf:Property>

<rdfs:Class rdf:about="&nfo;PlainTextDocument"
    rdfs:label="PlainTextDocument">
  <rdfs:comment>A file containing plain text (ASCII, Unicode or other encodings). Examples may include TXT, HTML, XML, program source code etc.</rdfs:comment>
  <rdfs:subClassOf rdf:resource="&nfo;TextDocument"/>
</rdfs:Class>

<dcam:VocabularyEncodingScheme rdf:about="&dcterms;LCSH">
  <dcterms:hasVersion rdf:resource="http://dublincore.org/usage/terms/history/#LCSH-003"/>
  <dcterms:issued rdf:datatype="&xsd;date">2000-07-11</dcterms:issued>
  <dcterms:modified rdf:datatype="&xsd;date">2008-01-14</dcterms:modified>
  <rdfs:comment xml:lang="en">The set of labeled concepts specified by the Library of Congress Subject Headings.</rdfs:comment>
  <rdfs:isDefinedBy rdf:resource="&dcterms;"/>
  <rdfs:label xml:lang="en">LCSH</rdfs:label>
</dcam:VocabularyEncodingScheme>

<rdf:Property rdf:about="&nexif;spatialFrequencyResponse"
    rdfs:label="spatialFrequencyResponse">
  <rdfs:subPropertyOf rdf:resource="http://www.kanzaki.com/ns/exif#spatialFrequencyResponse"/>
  <rdfs:subPropertyOf rdf:resource="&nexif;pictTaking"/>
  <rdfs:comment>This tag records the camera or input device spatial frequency table and SFR values in the direction of image width, image height, and diagonal direction, as specified in ISO 12233.
tagNumber: 41484</rdfs:comment>
  <rdfs:domain rdf:resource="&nexif;Photo"/>
  <rdfs:range rdf:resource="&xsd;string"/>
</rdf:Property>

<rdf:Property rdf:about="&foaf;publications"
    rdfs:comment="A link to the publications of this person."
    rdfs:label="publications"
    ns:term_status="testing">
  <rdf:type rdf:resource="&owl;ObjectProperty"/>
  <rdfs:domain rdf:resource="&foaf;Person"/>
  <rdfs:isDefinedBy rdf:resource="&foaf;"/>
  <rdfs:range rdf:resource="&foaf;Document"/>
</rdf:Property>

<rdf:Property rdf:about="&dcterms;valid">
  <rdfs:subPropertyOf rdf:resource="&dc;date"/>
  <rdfs:subPropertyOf rdf:resource="&dcterms;date"/>
  <dcterms:hasVersion rdf:resource="http://dublincore.org/usage/terms/history/#valid-003"/>
  <dcterms:issued rdf:datatype="&xsd;date">2000-07-11</dcterms:issued>
  <dcterms:modified rdf:datatype="&xsd;date">2008-01-14</dcterms:modified>
  <rdfs:comment xml:lang="en">Date (often a range) of validity of a resource.</rdfs:comment>
  <rdfs:isDefinedBy rdf:resource="&dcterms;"/>
  <rdfs:label xml:lang="en">Date Valid</rdfs:label>
  <rdfs:range rdf:resource="&rdfs;Literal"/>
</rdf:Property>

<rdf:Property rdf:about="&dc;publisher">
  <dcterms:description xml:lang="en">Examples of a Publisher include a person, an organization, or a service. Typically, the name of a Publisher should be used to indicate the entity.</dcterms:description>
  <dcterms:hasVersion rdf:resource="http://dublincore.org/usage/terms/history/#publisher-006"/>
  <dcterms:issued rdf:datatype="&xsd;date">1999-07-02</dcterms:issued>
  <dcterms:modified rdf:datatype="&xsd;date">2008-01-14</dcterms:modified>
  <rdfs:comment xml:lang="en">An entity responsible for making the resource available.</rdfs:comment>
  <rdfs:isDefinedBy rdf:resource="&dc;"/>
  <rdfs:label xml:lang="en">Publisher</rdfs:label>
  <scos:note xml:lang="en">A second property with the same name as this property has been declared in the dcterms: namespace (http://purl.org/dc/terms/).  See the Introduction to the document "DCMI Metadata Terms" (http://dublincore.org/documents/dcmi-terms/) for an explanation.</scos:note>
</rdf:Property>

<rdf:Property rdf:about="&ncal;fmttype"
    rdfs:label="fmttype">
  <nrl:maxCardinality rdf:datatype="&xsd;integer">1</nrl:maxCardinality>
  <rdfs:comment>To specify the content type of a referenced object. Inspired by RFC 2445 sec. 4.2.8. The value of this property should be an IANA-registered content type (e.g. application/binary)</rdfs:comment>
  <rdfs:domain rdf:resource="&ncal;Attachment"/>
  <rdfs:range rdf:resource="&xsd;string"/>
</rdf:Property>

<tmo:Importance rdf:about="&tmo;TMO_Instance_Importance_07"
    rdfs:label="TMO_Instance_Importance_07"/>

<nco:IMStatusType rdf:about="&nco;IMStatusTypeOffline"
    rdfs:label="offline"/>

<rdfs:Datatype rdf:about="&dcterms;ISO639-2">
  <dcterms:hasVersion rdf:resource="http://dublincore.org/usage/terms/history/#ISO639-2-003"/>
  <dcterms:issued rdf:datatype="&xsd;date">2000-07-11</dcterms:issued>
  <dcterms:modified rdf:datatype="&xsd;date">2008-01-14</dcterms:modified>
  <rdfs:comment xml:lang="en">The three-letter alphabetic codes listed in ISO639-2 for the representation of names of languages.</rdfs:comment>
  <rdfs:isDefinedBy rdf:resource="&dcterms;"/>
  <rdfs:label xml:lang="en">ISO 639-2</rdfs:label>
  <rdfs:seeAlso rdf:resource="http://lcweb.loc.gov/standards/iso639-2/langhome.html"/>
</rdfs:Datatype>

<ncal:AttachmentEncoding rdf:about="&ncal;base64Encoding"
    rdfs:label="base64Encoding"/>

<rdf:Property rdf:about="&dcon;hasSituation"
    rdfs:label="has Situation">
  <rdfs:comment>Links one or more active/current situations to the user. Situations are stored permanently, whether currently active or otherwise.</rdfs:comment>
  <rdfs:domain rdf:resource="&pimo;Agent"/>
  <rdfs:range rdf:resource="&dcon;Situation"/>
</rdf:Property>

<rdf:Property rdf:about="&nexif;copyright"
    rdfs:label="copyright">
  <rdfs:subPropertyOf rdf:resource="&dc;rights"/>
  <rdfs:subPropertyOf rdf:resource="http://www.kanzaki.com/ns/exif#copyright"/>
  <rdfs:subPropertyOf rdf:resource="&nie;copyright"/>
  <rdfs:subPropertyOf rdf:resource="&nexif;exifAttribute"/>
  <nao:deprecated rdf:datatype="&xsd;boolean">true</nao:deprecated>
  <rdfs:comment>tagNumber: 33432
Copyright information. In this standard the tag is used to indicate both the photographer and editor copyrights. It is the copyright notice of the person or organization claiming rights to the image. Deprecated in favor of the more generic nie:copyright.</rdfs:comment>
  <rdfs:domain rdf:resource="&nexif;Photo"/>
  <rdfs:range rdf:resource="&xsd;string"/>
</rdf:Property>

<rdf:Property rdf:about="&dpo;minDayOfMonth"
    rdfs:label="Minimum Day of the Month">
  <rdfs:comment>A subproperty of dpo:minValue that defines a lowerbound on the observed day of the month (i.e., between 1 and 31) such that it can classify as a dpo:TimePeriod instance. It can be used in conjunction with dpo:maxDayOfMonth, i.e. specific instances of dpo:TimePeriod have a pre-defined observable monthly period.</rdfs:comment>
  <rdfs:domain rdf:resource="&dpo;TimePeriod"/>
  <rdfs:range rdf:resource="&xsd;integer"/>
  <rdfs:subPropertyOf rdf:resource="&dpo;minValue"/>
</rdf:Property>

<rdf:Property rdf:about="&nmm;hasEpisode"
    rdfs:comment="A TVSeries has many episodes"
    rdfs:label="has episode">
  <nrl:inverseProperty rdf:resource="&nmm;series"/>
  <rdfs:domain rdf:resource="&nmm;TVSeries"/>
  <rdfs:range rdf:resource="&nmm;TVShow"/>
</rdf:Property>

<rdf:Property rdf:about="&nmm;season"
    rdfs:label="Season">
  <nao:deprecated rdf:datatype="&xsd;boolean">true</nao:deprecated>
  <nrl:maxCardinality rdf:datatype="&xsd;integer">1</nrl:maxCardinality>
  <rdfs:comment>The season number. This property is deprecated. Use nmm:Season and nmm:hasSeason instead.</rdfs:comment>
  <rdfs:domain rdf:resource="&nmm;TVShow"/>
  <rdfs:range rdf:resource="&xsd;integer"/>
</rdf:Property>

<rdfs:Class rdf:about="&tmo;SimilarityDependence"
    rdfs:label="SimilarityDependence">
  <rdfs:subClassOf rdf:resource="&tmo;UndirectedDependency"/>
</rdfs:Class>

<rdf:Property rdf:about="&nfo;supercedes"
    rdfs:label="supercedes">
  <rdfs:comment>States that a piece of software supercedes another piece of software.</rdfs:comment>
  <rdfs:domain rdf:resource="&nfo;Software"/>
  <rdfs:range rdf:resource="&nfo;Software"/>
</rdf:Property>

<rdf:Property rdf:about="&nao;scoreParameter"
    rdfs:label="scoreparameter">
  <rdfs:comment>A marker property to mark selected properties which are input to a mathematical algorithm to generate scores for resources. Properties are marked by being defined as subproperties of this property</rdfs:comment>
  <rdfs:domain rdf:resource="&rdfs;Resource"/>
  <rdfs:range rdf:resource="&xsd;float"/>
  <rdfs:subPropertyOf rdf:resource="&nao;annotation"/>
</rdf:Property>

<rdf:Property rdf:about="&ncal;hasAlarm"
    rdfs:label="hasAlarm">
  <rdfs:comment>Links an event or a todo with a DataObject that can be interpreted as an alarm. This property has no direct equivalent in the RFC 2445. It has been provided to express this relation.</rdfs:comment>
  <rdfs:domain rdf:resource="&ncal;UnionOfEventTodo"/>
  <rdfs:range rdf:resource="&ncal;CalendarDataObject"/>
  <rdfs:subPropertyOf rdf:resource="&nie;hasPart"/>
</rdf:Property>

<rdf:Property rdf:about="&nid3;interpretedBy"
    rdfs:label="interpretedBy">
  <rdfs:comment>TPE4
The 'Interpreted, remixed, or otherwise modified by' frame contains more information about the people behind a remix and similar interpretations of another existing piece.</rdfs:comment>
  <rdfs:domain rdf:resource="&nid3;ID3Audio"/>
  <rdfs:range rdf:resource="&nco;Contact"/>
  <rdfs:subPropertyOf rdf:resource="&nco;contributor"/>
</rdf:Property>

<rdf:Property rdf:about="&foaf;family_name"
    rdfs:comment="The family name of some person."
    rdfs:label="family_name"
    ns:term_status="archaic">
  <rdf:type rdf:resource="&owl;DatatypeProperty"/>
  <rdfs:domain rdf:resource="&foaf;Person"/>
  <rdfs:isDefinedBy rdf:resource="&foaf;"/>
  <rdfs:range rdf:resource="&rdfs;Literal"/>
</rdf:Property>

<rdf:Property rdf:about="&dcon;isRequired"
    rdfs:label="is Required">
  <rdfs:comment>This property marks those context elements which are necessary for a situation to occurr. If a required element is not active, then the correspoding situation is excluded from candidate active situations.</rdfs:comment>
  <rdfs:domain rdf:resource="&dcon;Element"/>
  <rdfs:range rdf:resource="&xsd;boolean"/>
</rdf:Property>

<ncal:TodoStatus rdf:about="&ncal;cancelledTodoStatus"
    rdfs:label="cancelledTodoStatus"/>

<rdfs:Class rdf:about="&nfo;EmbeddedFileDataObject"
    rdfs:label="EmbeddedFileDataObject">
  <rdfs:comment>A file embedded in another data object. There are many ways in which a file may be embedded in another one. Use this class directly only in cases if none of the subclasses gives a better description of your case.</rdfs:comment>
  <rdfs:subClassOf rdf:resource="&nfo;FileDataObject"/>
</rdfs:Class>

<rdfs:Class rdf:about="&nao;Agent"
    rdfs:label="agent">
  <rdfs:comment>An agent is the artificial counterpart to nao:Party. It can be a software component or some service.</rdfs:comment>
  <rdfs:subClassOf rdf:resource="&rdfs;Resource"/>
</rdfs:Class>

<ncal:FreebusyType rdf:about="&ncal;busyTentativeFreebusyType"
    rdfs:label="busyTentativeFreebusyType"/>

<rdfs:Class rdf:about="&tmo;Priority"
    rdfs:label="Priority">
  <rdfs:subClassOf rdf:resource="&tmo;StateTypeRole"/>
</rdfs:Class>

<nrl:DefiningProperty rdf:about="&nmm;performer"
    rdfs:comment="Performer"
    rdfs:label="performer">
  <rdf:type rdf:resource="&rdf;Property"/>
  <rdfs:domain rdf:resource="&nmm;MusicPiece"/>
  <rdfs:range rdf:resource="&nco;Contact"/>
  <rdfs:subPropertyOf rdf:resource="&nco;contributor"/>
</nrl:DefiningProperty>

<rdf:Property rdf:about="&nexif;interoperabilityIFDPointer"
    rdfs:label="interoperabilityIFDPointer">
  <rdfs:subPropertyOf rdf:resource="http://www.kanzaki.com/ns/exif#interoperability_IFD_Pointer"/>
  <rdfs:subPropertyOf rdf:resource="&nexif;ifdPointer"/>
  <rdfs:comment>A pointer to the Interoperability IFD, which is composed of tags storing the information to ensure the Interoperability
tagNumber: 40965</rdfs:comment>
  <rdfs:domain rdf:resource="&nexif;Photo"/>
  <rdfs:range rdf:resource="&nexif;Photo"/>
</rdf:Property>

<rdfs:Class rdf:about="&tmo;Importance"
    rdfs:label="Importance">
  <rdfs:subClassOf rdf:resource="&tmo;StateTypeRole"/>
</rdfs:Class>

<rdf:Property rdf:about="&nexif;seconds"
    rdfs:comment="a mesurement of time length with unit of second"
    rdfs:label="seconds">
  <rdfs:domain rdf:resource="&nexif;Photo"/>
  <rdfs:range rdf:resource="&xsd;string"/>
  <rdfs:subPropertyOf rdf:resource="http://www.kanzaki.com/ns/exif#seconds"/>
</rdf:Property>

<ncal:ParticipationStatus rdf:about="&ncal;declinedParticipationStatus"
    rdfs:label="declinedParticipationStatus"/>

<rdfs:Class rdf:about="&nmo;Mailbox"
    rdfs:comment="A mailbox - container for MailboxDataObjects."
    rdfs:label="Mailbox">
  <rdfs:subClassOf rdf:resource="&nie;InformationElement"/>
</rdfs:Class>

<owl:ObjectProperty rdf:about="&oa;hasBody">
  <rdfs:comment xml:lang="en">The relationship between oa:Annotation and body. The body is somehow "about" the oa:hasTarget of the annotation.

The Body may be of any media type, and contain any type of content. The Body SHOULD be identified by HTTP URIs unless they are embedded within the Annotation.

Embedded bodies SHOULD be instances of cnt:ContentAsText and embed their content with cnt:chars. They SHOULD declare their media type with dc:format, and MAY indicate their language using dc:language and a RFC-3066 language tag. 

There is no OA class provided for "Body" as a body might be a target of a different annotation. However, there SHOULD be 1 or more content-based classes associated with the body resources of an Annotation, and the dctypes: vocabulary is recommended for this purpose, for instance dctypes:Text to declare textual content.</rdfs:comment>
  <rdfs:domain rdf:resource="&oa;Annotation"/>
  <rdfs:isDefinedBy rdf:resource="&oa;"/>
  <rdfs:label xml:lang="en">hasBody</rdfs:label>
</owl:ObjectProperty>

<rdf:Property rdf:about="&nexif;userInfo"
    rdfs:comment="An attribute relating to User Information"
    rdfs:label="userInfo">
  <rdfs:subPropertyOf rdf:resource="http://www.kanzaki.com/ns/exif#userInfo"/>
  <rdfs:subPropertyOf rdf:resource="&nexif;exifAttribute"/>
  <rdfs:domain rdf:resource="&nexif;Photo"/>
  <rdfs:range rdf:resource="&xsd;string"/>
</rdf:Property>

<rdf:Property rdf:about="&nid3;involvedPerson"
    rdfs:label="involvedPerson">
  <rdfs:comment>Links an ID3 file to an InvolvedPerson, an equivalent of the involvedPeopleList tag. Since there might be a lot of people contributing to an audio file in various ways, such as musicians and technicians, the 'Text information frames' are often insufficient to list everyone involved in a project. The 'Involved people list' is a frame containing the names of those involved, and how they were involved. The body simply contains a terminated string with the involvement directly followed by a terminated string with the involvee followed by a new involvement and so on. There may only be one "IPLS" frame in each tag.</rdfs:comment>
  <rdfs:domain rdf:resource="&nid3;ID3Audio"/>
  <rdfs:range rdf:resource="&nid3;InvolvedPerson"/>
</rdf:Property>

<ncal:AccessClassification rdf:about="&ncal;privateClassification"
    rdfs:label="privateClassification"/>

<rdf:Property rdf:about="&nie;characterSet"
    nrl:maxCardinality="1"
    rdfs:label="characterSet">
  <rdfs:comment>Characterset in which the content of the InformationElement was created. Example: ISO-8859-1, UTF-8. One of the registered character sets at http://www.iana.org/assignments/character-sets. This characterSet is used to interpret any textual parts of the content. If more than one characterSet is used within one data object, use more specific properties.</rdfs:comment>
  <rdfs:domain rdf:resource="&nie;InformationElement"/>
  <rdfs:range rdf:resource="&xsd;string"/>
</rdf:Property>

<rdf:Property rdf:about="&nao;prefSymbol"
    rdfs:comment="A unique preferred symbol representation for a resource"
    rdfs:label="preferred symbol">
  <nrl:maxCardinality rdf:datatype="&xsd;nonNegativeInteger">1</nrl:maxCardinality>
  <rdfs:domain rdf:resource="&rdfs;Resource"/>
  <rdfs:range rdf:resource="&nao;Symbol"/>
  <rdfs:subPropertyOf rdf:resource="&nao;hasSymbol"/>
</rdf:Property>

<rdf:Property rdf:about="&dcon;currentTime"
    rdfs:label="Current Time">
  <rdfs:comment>Refers to a pre-defined time period that characterises a context instance.</rdfs:comment>
  <rdfs:domain rdf:resource="&dcon;SpaTem"/>
  <rdfs:range rdf:resource="&dpo;TimePeriod"/>
  <rdfs:subPropertyOf rdf:resource="&dcon;hasContextElement"/>
</rdf:Property>

<rdf:Property rdf:about="&scos;exactMatch">
  <rdf:type rdf:resource="&owl;ObjectProperty"/>
  <rdf:type rdf:resource="&owl;SymmetricProperty"/>
  <rdf:type rdf:resource="&owl;TransitiveProperty"/>
  <rdfs:comment xml:lang="en">skos:exactMatch is disjoint with each of the properties skos:broadMatch and skos:relatedMatch.</rdfs:comment>
  <rdfs:isDefinedBy rdf:resource="http://www.w3.org/2004/02/skos/core"/>
  <rdfs:label xml:lang="en">has exact match</rdfs:label>
  <rdfs:subPropertyOf rdf:resource="&scos;closeMatch"/>
  <scos:definition xml:lang="en">skos:exactMatch is used to link two concepts, indicating a high degree of confidence that the concepts can be used interchangeably across a wide range of information retrieval applications. skos:exactMatch is a transitive property, and is a sub-property of skos:closeMatch.</scos:definition>
</rdf:Property>

<rdf:Property rdf:about="&nco;pobox"
    nrl:maxCardinality="1"
    rdfs:label="pobox">
  <rdfs:comment>Post office box. This is the first part of the value of the 'ADR' property as defined in RFC 2426, sec. 3.2.1</rdfs:comment>
  <rdfs:domain rdf:resource="&nco;PostalAddress"/>
  <rdfs:range rdf:resource="&xsd;string"/>
</rdf:Property>

<nco:Gender rdf:about="&nco;male"
    rdfs:comment="A Male"
    rdfs:label="male"/>

<rdf:Property rdf:about="&drmo;hasConstraintOnObject"
    rdfs:label="Constraint on Object">
  <rdfs:comment>Places a constraint on a condition (i.e., the domain defined for this property), such that a query can be constructed to look for an RDF triple having: i) the condition itself (i.e., the domain defined for this property) as its subject, ii) the associated constrained property (defined by drmo:hasConstraintOnProperty) as its property, iii) and the referred item (i.e. the range defined for this property) as its object. This property cannot coincide with the property hasConstraintOnSubject.</rdfs:comment>
  <rdfs:domain rdf:resource="&drmo;Condition"/>
  <rdfs:range rdf:resource="&rdfs;Resource"/>
</rdf:Property>

<rdf:Property rdf:about="&ddo;accessPointID"
    rdfs:comment="Attaches a human-readable name to a computer network."
    rdfs:label="accessPointID">
  <rdfs:domain rdf:resource="&ddo;ComputerNetwork"/>
  <rdfs:subPropertyOf rdf:resource="&ddo;networkID"/>
</rdf:Property>

<nrl:DefiningProperty rdf:about="&nmm;composer"
    rdfs:comment="Composer"
    rdfs:label="composer">
  <rdf:type rdf:resource="&rdf;Property"/>
  <rdfs:domain rdf:resource="&nmm;MusicPiece"/>
  <rdfs:range rdf:resource="&nco;Contact"/>
  <rdfs:subPropertyOf rdf:resource="&nco;contributor"/>
</nrl:DefiningProperty>

<rdf:Property rdf:about="&nfo;containsPlacemark"
    rdfs:label="contains Placemark">
  <rdfs:comment>Containment relation between placemark containers (files) and placemarks within.</rdfs:comment>
  <rdfs:domain rdf:resource="&nfo;PlacemarkContainer"/>
  <rdfs:range rdf:resource="&nfo;Placemark"/>
  <rdfs:subPropertyOf rdf:resource="&nie;hasLogicalPart"/>
</rdf:Property>

<rdf:Property rdf:about="&nfo;count"
    rdfs:label="count">
  <rdfs:comment>A common superproperty for all properties signifying the amount of atomic media data units. Examples of subproperties may include sampleCount and frameCount.</rdfs:comment>
  <rdfs:domain rdf:resource="&nfo;Media"/>
  <rdfs:range rdf:resource="&xsd;integer"/>
</rdf:Property>

<rdf:Property rdf:about="&nexif;gpsAltitudeRef"
    rdfs:label="gpsAltitudeRef">
  <rdfs:subPropertyOf rdf:resource="http://www.kanzaki.com/ns/exif#gpsAltitudeRef"/>
  <rdfs:subPropertyOf rdf:resource="&nexif;gpsInfo"/>
  <rdfs:comment>Indicates the altitude used as the reference altitude. If the reference is sea level and the altitude is above sea level, 0 is given. If the altitude is below sea level, a value of 1 is given and the altitude is indicated as an absolute value in the GPSAltitude tag. The reference unit is meters.
tagNumber: 5</rdfs:comment>
  <rdfs:domain rdf:resource="&nexif;Photo"/>
  <rdfs:range rdf:resource="&xsd;string"/>
</rdf:Property>

<rdfs:Class rdf:about="&nco;PersonName"
    rdfs:label="PersonName">
  <rdfs:comment>A class representing a person contact's name. Possesses various attributes.</rdfs:comment>
  <rdfs:subClassOf rdf:resource="&nco;Name"/>
</rdfs:Class>

<rdf:Property rdf:about="&dcon;inForeground"
    rdfs:label="is in the Foreground">
  <rdfs:comment>Specifies whether an active file(running on a device) is in the foreground (true) or background (false) in the current context.</rdfs:comment>
  <rdfs:domain rdf:resource="&nie;InformationElement"/>
  <rdfs:range rdf:resource="&xsd;boolean"/>
  <rdfs:subPropertyOf rdf:resource="&dcon;hasContextAttribute"/>
</rdf:Property>

<rdf:Property rdf:about="&foaf;membershipClass"
    rdfs:label="membershipClass"
    ns:term_status="unstable">
  <rdf:type rdf:resource="&owl;AnnotationProperty"/>
  <rdfs:comment>Indicates the class of individuals that are a member of a Group</rdfs:comment>
  <rdfs:isDefinedBy rdf:resource="&foaf;"/>
</rdf:Property>

<rdfs:Class rdf:about="&dplo;AvailabilityPost"
    rdfs:label="Availability Post">
  <rdfs:comment>Represents the live posting of information related to a user's detected or proclaimed availability, as defined by a set of instances of dpo:Availability.</rdfs:comment>
  <rdfs:subClassOf rdf:resource="&dplo;PresencePost"/>
</rdfs:Class>

<rdfs:Class rdf:about="&dcterms;PeriodOfTime">
  <dcterms:hasVersion rdf:resource="http://dublincore.org/usage/terms/history/#PeriodOfTime-001"/>
  <dcterms:issued rdf:datatype="&xsd;date">2008-01-14</dcterms:issued>
  <rdfs:comment xml:lang="en">An interval of time that is named or defined by its start and end dates.</rdfs:comment>
  <rdfs:isDefinedBy rdf:resource="&dcterms;"/>
  <rdfs:label xml:lang="en">Period of Time</rdfs:label>
  <rdfs:subClassOf rdf:resource="&dcterms;LocationPeriodOrJurisdiction"/>
</rdfs:Class>

<rdf:Property rdf:about="&nco;imStatusMessage"
    nrl:maxCardinality="1"
    rdfs:label="imStatusMessage">
  <rdfs:comment>A feature common in most IM systems. A message left by the user for all his/her contacts to see.</rdfs:comment>
  <rdfs:domain rdf:resource="&nco;IMAccount"/>
  <rdfs:range rdf:resource="&xsd;string"/>
</rdf:Property>

<rdfs:Class rdf:about="&tmo;AgentAbilityCarrier"
    protege:role="abstract"
    rdfs:label="AgentAbilityCarrier">
  <rdfs:subClassOf rdf:resource="&tmo;AbilityCarrier"/>
</rdfs:Class>

<rdfs:Class rdf:about="&cnt;DoctypeDecl">
  <rdf:type rdf:resource="&owl;Class"/>
  <rdfs:comment xml:lang="en">The document type declaration.</rdfs:comment>
  <rdfs:label xml:lang="en">Document type declaration</rdfs:label>
</rdfs:Class>

<rdf:Property rdf:about="&tmo;involvedPersonRole"
    nrl:maxCardinality="1"
    nrl:minCardinality="1"
    rdfs:label="involvedPersonRole">
  <rdfs:domain rdf:resource="&tmo;PersonInvolvement"/>
  <rdfs:range rdf:resource="&tmo;PersonInvolvementRole"/>
  <rdfs:subPropertyOf rdf:resource="&tmo;stateTypeRole"/>
</rdf:Property>

<rdf:Property rdf:about="&nao;creator"
    rdfs:label="creator">
  <rdfs:subPropertyOf rdf:resource="&dc;creator"/>
  <rdfs:subPropertyOf rdf:resource="&nao;annotation"/>
  <nrl:maxCardinality rdf:datatype="&xsd;nonNegativeInteger">1</nrl:maxCardinality>
  <rdfs:comment>Refers to the single or group of individuals that created the resource</rdfs:comment>
  <rdfs:domain rdf:resource="&rdfs;Resource"/>
  <rdfs:range rdf:resource="&nao;Party"/>
</rdf:Property>

<rdf:Property rdf:about="&scos;memberList">
  <rdf:type rdf:resource="&owl;FunctionalProperty"/>
  <rdf:type rdf:resource="&owl;ObjectProperty"/>
  <rdfs:comment xml:lang="en">For any resource, every item in the list given as the value of the
      skos:memberList property is also a value of the skos:member property.</rdfs:comment>
  <rdfs:domain rdf:resource="&scos;OrderedCollection"/>
  <rdfs:isDefinedBy rdf:resource="http://www.w3.org/2004/02/skos/core"/>
  <rdfs:label xml:lang="en">has member list</rdfs:label>
  <rdfs:range rdf:resource="&rdf;List"/>
  <scos:definition xml:lang="en">Relates an ordered collection to the RDF list containing its members.</scos:definition>
</rdf:Property>

<rdf:Property rdf:about="&dcterms;replaces">
  <rdfs:subPropertyOf rdf:resource="&dc;relation"/>
  <rdfs:subPropertyOf rdf:resource="&dcterms;relation"/>
  <dcterms:hasVersion rdf:resource="http://dublincore.org/usage/terms/history/#replaces-003"/>
  <dcterms:issued rdf:datatype="&xsd;date">2000-07-11</dcterms:issued>
  <dcterms:modified rdf:datatype="&xsd;date">2008-01-14</dcterms:modified>
  <rdfs:comment xml:lang="en">A related resource that is supplanted, displaced, or superseded by the described resource.</rdfs:comment>
  <rdfs:isDefinedBy rdf:resource="&dcterms;"/>
  <rdfs:label xml:lang="en">Replaces</rdfs:label>
  <scos:note xml:lang="en">This term is intended to be used with non-literal values as defined in the DCMI Abstract Model (http://dublincore.org/documents/abstract-model/).  As of December 2007, the DCMI Usage Board is seeking a way to express this intention with a formal range declaration.</scos:note>
</rdf:Property>

<rdf:Property rdf:about="&nexif;gpsMeasureMode"
    rdfs:label="gpsMeasureMode">
  <rdfs:subPropertyOf rdf:resource="http://www.kanzaki.com/ns/exif#gpsMeasureMode"/>
  <rdfs:subPropertyOf rdf:resource="&nexif;gpsInfo"/>
  <rdfs:comment>The GPS measurement mode. '2' means two-dimensional measurement and '3' means three-dimensional measurement is in progress.
tagNumber: 10</rdfs:comment>
  <rdfs:domain rdf:resource="&nexif;Photo"/>
  <rdfs:range rdf:resource="&xsd;string"/>
</rdf:Property>

<ncal:AttendeeRole rdf:about="&ncal;chairRole"
    rdfs:label="chairRole"/>

<rdfs:Class rdf:about="&tmo;Urgency"
    rdfs:label="Urgency">
  <rdfs:subClassOf rdf:resource="&tmo;StateTypeRole"/>
</rdfs:Class>

<owl:Class rdf:about="&oa;Composite"
    rdfs:label="Composite">
  <rdfs:comment xml:lang="en">A multiplicity construct that conveys to a consuming application that all of the constituent resources are required for the Annotation to be correctly interpreted. 

oa:Composite can be used as the object of the object of the oa:hasBody, oa:hasTarget, oa:hasSelector, oa:hasState, oa:styledBy and oa:hasScope relationships, 

There MUST be 2 or more oa:item relationships for each oa:Composite.</rdfs:comment>
  <rdfs:isDefinedBy rdf:resource="&oa;"/>
  <rdfs:subClassOf rdf:resource="&rdf;Bag"/>
</owl:Class>

<rdf:Property rdf:about="&ncal;role"
    rdfs:label="role">
  <rdfs:comment>To specify the participation role for the calendar user specified by the property. Inspired by the RFC 2445 sec. 4.2.16. Originally this property had a limited vocabulary for values. The terms of that vocabulary have been expressed as instances of the AttendeeRole class.</rdfs:comment>
  <rdfs:domain rdf:resource="&ncal;Attendee"/>
  <rdfs:range rdf:resource="&ncal;AttendeeRole"/>
</rdf:Property>

<rdf:Property rdf:about="&nexif;exifAttribute"
    rdfs:label="exifAttribute">
  <rdfs:comment>A property that connects an IFD (or other resource) to one of its entries (Exif attribute). Super property which integrates all Exif tags. Domain definition dropped so that this vocabulary can be used to describe not only Exif IFD, but also general image.</rdfs:comment>
  <rdfs:domain rdf:resource="&nexif;Photo"/>
  <rdfs:range rdf:resource="&xsd;string"/>
  <rdfs:subPropertyOf rdf:resource="http://www.kanzaki.com/ns/exif#exifAttribute"/>
</rdf:Property>

<rdf:Property rdf:about="&foaf;nick"
    rdfs:label="nickname"
    ns:term_status="testing">
  <rdf:type rdf:resource="&owl;DatatypeProperty"/>
  <rdfs:comment>A short informal nickname characterising an agent (includes login identifiers, IRC and other chat nicknames).</rdfs:comment>
  <rdfs:isDefinedBy rdf:resource="&foaf;"/>
</rdf:Property>

<rdf:Property rdf:about="&nfo;pageCount"
    rdfs:comment="Number of pages."
    rdfs:label="pageCount">
  <nrl:maxCardinality rdf:datatype="&xsd;integer">1</nrl:maxCardinality>
  <rdfs:domain rdf:resource="&nfo;PaginatedTextDocument"/>
  <rdfs:range rdf:resource="&xsd;integer"/>
</rdf:Property>

<rdfs:Class rdf:about="&nfo;Media"
    rdfs:label="Media">
  <rdfs:comment>A piece of media content. This class may be used to express complex media containers with many streams of various media content (both aural and visual).</rdfs:comment>
  <rdfs:subClassOf rdf:resource="&nie;InformationElement"/>
</rdfs:Class>

<dcam:VocabularyEncodingScheme rdf:about="&dcterms;NLM">
  <dcterms:hasVersion rdf:resource="http://dublincore.org/usage/terms/history/#NLM-002"/>
  <dcterms:issued rdf:datatype="&xsd;date">2005-06-13</dcterms:issued>
  <dcterms:modified rdf:datatype="&xsd;date">2008-01-14</dcterms:modified>
  <rdfs:comment xml:lang="en">The set of conceptual resources specified by the National Library of Medicine Classification.</rdfs:comment>
  <rdfs:isDefinedBy rdf:resource="&dcterms;"/>
  <rdfs:label xml:lang="en">NLM</rdfs:label>
  <rdfs:seeAlso rdf:resource="http://wwwcf.nlm.nih.gov/class/"/>
</dcam:VocabularyEncodingScheme>

<rdf:Property rdf:about="&nexif;interopInfo"
    rdfs:label="interopInfo">
  <rdfs:subPropertyOf rdf:resource="http://www.kanzaki.com/ns/exif#interopInfo"/>
  <rdfs:subPropertyOf rdf:resource="&nexif;exifAttribute"/>
  <rdfs:comment>An attribute relating to Interoperability. Tags stored in
Interoperability IFD may be defined dependently to each Interoperability rule.</rdfs:comment>
  <rdfs:domain rdf:resource="&nexif;Photo"/>
  <rdfs:range rdf:resource="&xsd;string"/>
</rdf:Property>

<rdf:Property rdf:about="&nid3;copyrightMessage"
    rdfs:label="copyrightMessage">
  <rdfs:comment>TCOP
The 'Copyright message' frame, which must begin with a year and a space character (making five characters), is intended for the copyright holder of the original sound, not the audio file itself. The absence of this frame means only that the copyright information is unavailable or has been removed, and must not be interpreted to mean that the sound is public domain. Every time this field is displayed the field must be preceded with "Copyright".</rdfs:comment>
  <rdfs:domain rdf:resource="&nid3;ID3Audio"/>
  <rdfs:range rdf:resource="&xsd;string"/>
  <rdfs:subPropertyOf rdf:resource="&dc;rights"/>
</rdf:Property>

<rdf:Property rdf:about="&nie;mimeType"
    nrl:maxCardinality="1"
    rdfs:label="mimeType">
  <rdfs:comment>The mime type of the resource, if available. Example: "text/plain". See http://www.iana.org/assignments/media-types/. This property applies to data objects that can be described with one mime type. In cases where the object as a whole has one mime type, while it's parts have other mime types, or there is no mime type that can be applied to the object as a whole, but some parts of the content have mime types - use more specific properties.</rdfs:comment>
  <rdfs:domain rdf:resource="&nie;InformationElement"/>
  <rdfs:range rdf:resource="&xsd;string"/>
</rdf:Property>

<rdfs:Class rdf:about="&nie;DataObject"
    rdfs:label="DataObject">
  <rdfs:comment>A unit of data that is created, annotated and processed on the user desktop. It represents a native structure the user works with. The usage of the term 'native' is important. It means that a DataObject can be directly mapped to a data structure maintained by a native application. This may be a file, a set of files or a part of a file. The granularity depends on the user. This class is not intended to be instantiated by itself. Use more specific subclasses.</rdfs:comment>
  <rdfs:subClassOf rdf:resource="&rdfs;Resource"/>
</rdfs:Class>

<rdf:Property rdf:about="&dcon;longitude"
    rdfs:comment="Records the exact longitude of the approximated location"
    rdfs:label="GPS Longitude">
  <rdfs:domain rdf:resource="&pimo;Location"/>
  <rdfs:range rdf:resource="&xsd;float"/>
  <rdfs:subPropertyOf rdf:resource="&dcon;hasContextAttribute"/>
</rdf:Property>

<rdf:Property rdf:about="&foaf;givenName"
    rdfs:comment="The given name of some person."
    rdfs:label="Given name"
    ns:term_status="testing">
  <rdf:type rdf:resource="&owl;DatatypeProperty"/>
  <rdfs:isDefinedBy rdf:resource="&foaf;"/>
</rdf:Property>

<rdf:Property rdf:about="&ncal;attachmentContent"
    rdfs:label="attachmentContent">
  <rdfs:comment>The uri of the attachment. Created to express the actual value of the ATTACH property defined in RFC 2445 sec. 4.8.1.1. This property expresses the BINARY datatype of that property. see ncal:attachmentUri for the URI datatype.</rdfs:comment>
  <rdfs:domain rdf:resource="&ncal;Attachment"/>
  <rdfs:range rdf:resource="&xsd;string"/>
</rdf:Property>

<rdf:Property rdf:about="&nexif;model"
    rdfs:comment="tagNumber: 272
Model of image input equipment"
    rdfs:label="model">
  <rdfs:subPropertyOf rdf:resource="http://www.kanzaki.com/ns/exif#model"/>
  <rdfs:subPropertyOf rdf:resource="&nexif;exifAttribute"/>
  <rdfs:domain rdf:resource="&nexif;Photo"/>
  <rdfs:range rdf:resource="&xsd;string"/>
</rdf:Property>

<rdf:Property rdf:about="&nid3;attachedPicture"
    rdfs:label="attachedPicture">
  <rdfs:comment>A picture attached to an audio file. The DataObject refered to by this property is usually interpreted as an nfo:Image Inspired by the attached picture tag defined in http://www.id3.org/id3v2.3.0 sec. 4.15)</rdfs:comment>
  <rdfs:domain rdf:resource="&nid3;ID3Audio"/>
  <rdfs:range rdf:resource="&nie;DataObject"/>
  <rdfs:subPropertyOf rdf:resource="&nie;hasPart"/>
</rdf:Property>

<tmo:Importance rdf:about="&tmo;TMO_Instance_Importance_02"
    rdfs:label="TMO_Instance_Importance_02"/>

<rdfs:Datatype rdf:about="&dcterms;RFC4646">
  <dcterms:description xml:lang="en">RFC 4646 obsoletes RFC 3066.</dcterms:description>
  <dcterms:hasVersion rdf:resource="http://dublincore.org/usage/terms/history/#RFC4646-001"/>
  <dcterms:issued rdf:datatype="&xsd;date">2008-01-14</dcterms:issued>
  <rdfs:comment xml:lang="en">The set of tags constructed according to RFC 4646 for the identification of languages.</rdfs:comment>
  <rdfs:isDefinedBy rdf:resource="&dcterms;"/>
  <rdfs:label xml:lang="en">RFC 4646</rdfs:label>
  <rdfs:seeAlso rdf:resource="http://www.ietf.org/rfc/rfc4646.txt"/>
</rdfs:Datatype>

<rdf:Property rdf:about="&nid3;officialFileWebpage"
    rdfs:label="officialFileWebpage">
  <rdfs:comment>WOAF
The 'Official audio file webpage' frame is a URL pointing at a file specific webpage.</rdfs:comment>
  <rdfs:domain rdf:resource="&nid3;ID3Audio"/>
  <rdfs:range rdf:resource="&rdfs;Resource"/>
</rdf:Property>

<rdf:Property rdf:about="&nmo;cc"
    rdfs:comment="deprecated in favor of nmo:emailCc"
    rdfs:label="cc">
  <nao:deprecated rdf:datatype="&xsd;boolean">true</nao:deprecated>
  <rdfs:domain rdf:resource="&nmo;Email"/>
  <rdfs:range rdf:resource="&nco;Contact"/>
  <rdfs:subPropertyOf rdf:resource="&nmo;secondaryRecipient"/>
</rdf:Property>

<rdf:Property rdf:about="&nrl;imports"
    rdfs:label="imports">
  <rdfs:comment>Models a subsumption relationship between two graphs, stating that the object graph is imported and included in the subject graph</rdfs:comment>
  <rdfs:domain rdf:resource="&nrl;Data"/>
  <rdfs:range rdf:resource="&nrl;Data"/>
  <rdfs:subPropertyOf rdf:resource="&nrl;superGraphOf"/>
</rdf:Property>

<rdfs:Class rdf:about="&pimo;Building"
    rdfs:label="Building">
  <rdfs:comment>A structure that has a roof and walls and stands more or less permanently in one place; "there was a three-story building on the corner"; "it was an imposing edifice". (Definition from SUMO).</rdfs:comment>
  <rdfs:subClassOf rdf:resource="&pimo;Location"/>
</rdfs:Class>

<rdf:Property rdf:about="&nmo;contentMimeType"
    rdfs:label="contentMimeType">
  <nrl:maxCardinality rdf:datatype="&xsd;integer">1</nrl:maxCardinality>
  <rdfs:comment>Key used to store the MIME type of the content of an object when it is different from the object's main MIME type. This value can be used, for example, to model an e-mail message whose mime type is"message/rfc822", but whose content has type "text/html". If not specified, the MIME type of the
content defaults to the value specified by the 'mimeType' property.</rdfs:comment>
  <rdfs:domain rdf:resource="&nmo;Email"/>
  <rdfs:range rdf:resource="&xsd;string"/>
  <rdfs:subPropertyOf rdf:resource="&nie;mimeType"/>
</rdf:Property>

<tmo:Priority rdf:about="&tmo;TMO_Instance_Priority_Medium"
    rdfs:label="TMO_Instance_Priority_Medium"/>

<rdf:Property rdf:about="&nie;lastModified"
    nrl:maxCardinality="1"
    rdfs:label="lastModified">
  <rdfs:subPropertyOf rdf:resource="&dc;date"/>
  <rdfs:subPropertyOf rdf:resource="&nie;modified"/>
  <rdfs:subPropertyOf rdf:resource="&nao;lastModified"/>
  <rdfs:comment>Last modification date of the DataObject. Note that this date refers to the modification of the DataObject itself (i.e. the physical representation). Compare with nie:contentLastModified.</rdfs:comment>
  <rdfs:domain rdf:resource="&nie;DataObject"/>
  <rdfs:range rdf:resource="&xsd;dateTime"/>
</rdf:Property>

<rdf:Property rdf:about="&dpo;maxWaveHeight"
    rdfs:label="Minimum Wave Height">
  <rdfs:comment>A subproperty of dpo:axValue that defines an upperbound on the observed wave height (in metres) such that it can classify as a dpo:WeatherCondition instance. It can be used in conjunction with dpo:minWaveHeight to state that specific instances of dpo:WeatherCondition have a pre-defined range of observable real-world wave heights in a body of water. In addition, they can also be used with various other weather conditions values and ranges to define complex weather condition types.</rdfs:comment>
  <rdfs:domain rdf:resource="&dpo;WeatherConditions"/>
  <rdfs:range rdf:resource="&xsd;float"/>
  <rdfs:subPropertyOf rdf:resource="&dpo;maxValue"/>
</rdf:Property>

<rdfs:Class rdf:about="&nco;OrganizationContact"
    rdfs:comment="A Contact that denotes on Organization."
    rdfs:label="OrganizationContact">
  <rdfs:subClassOf rdf:resource="&nco;Contact"/>
</rdfs:Class>

<rdf:Property rdf:about="&nmm;episodeNumber"
    rdfs:label="Episode number">
  <nrl:maxCardinality rdf:datatype="&xsd;integer">1</nrl:maxCardinality>
  <rdfs:domain rdf:resource="&nmm;TVShow"/>
  <rdfs:range rdf:resource="&xsd;integer"/>
</rdf:Property>

<rdf:Property rdf:about="&nco;publisher"
    rdfs:label="publisher">
  <rdfs:comment>An entity responsible for making the InformationElement available.</rdfs:comment>
  <rdfs:domain rdf:resource="&nie;InformationElement"/>
  <rdfs:range rdf:resource="&nco;Contact"/>
  <rdfs:subPropertyOf rdf:resource="&dc;publisher"/>
</rdf:Property>

<rdf:Property rdf:about="&nexif;cfaPattern"
    rdfs:label="cfaPattern">
  <rdfs:subPropertyOf rdf:resource="http://www.kanzaki.com/ns/exif#cfaPattern"/>
  <rdfs:subPropertyOf rdf:resource="&nexif;pictTaking"/>
  <rdfs:comment>tagNumber: 41730
The color filter array (CFA) geometric pattern of the image sensor when a one-chip color area sensor is used. It does not apply to all sensing methods.</rdfs:comment>
  <rdfs:domain rdf:resource="&nexif;Photo"/>
  <rdfs:range rdf:resource="&xsd;string"/>
</rdf:Property>

<rdf:Property rdf:about="&tmo;actualTime"
    nrl:maxCardinality="1"
    rdfs:label="actualTime">
  <rdfs:range rdf:resource="&xsd;dateTime"/>
  <rdfs:subPropertyOf rdf:resource="&tmo;dateTime"/>
</rdf:Property>

<rdf:Property rdf:about="&nexif;focalLength"
    rdfs:label="focalLength">
  <rdfs:subPropertyOf rdf:resource="http://www.kanzaki.com/ns/exif#focalLength"/>
  <rdfs:subPropertyOf rdf:resource="&nexif;mm"/>
  <rdfs:subPropertyOf rdf:resource="&nexif;pictTaking"/>
  <rdfs:comment>The actual focal length of the lens, in mm. Conversion is not made to the focal length of a 35 mm film camera.
tagNumber: 37386</rdfs:comment>
  <rdfs:domain rdf:resource="&nexif;Photo"/>
  <rdfs:range rdf:resource="&xsd;float"/>
</rdf:Property>

<rdf:Property rdf:about="&nid3;textElementContent"
    rdfs:label="textElementContent">
  <rdfs:domain rdf:resource="&nid3;SynchronizedTextElement"/>
  <rdfs:range rdf:resource="&xsd;string"/>
</rdf:Property>

<rdfs:Class rdf:about="&dpo;Place"
    rdfs:label="Place">
  <rdfs:comment>Non-quantifiable presence information concerning the type of location that an agent is currently near to. Multiple distinct locations can correspond to the same place instance.</rdfs:comment>
  <rdfs:subClassOf rdf:resource="&dpo;NonQuantifiableComponent"/>
</rdfs:Class>

<rdf:Property rdf:about="&dc;type">
  <dcterms:description xml:lang="en">Recommended best practice is to use a controlled vocabulary such as the DCMI Type Vocabulary [DCMITYPE]. To describe the file format, physical medium, or dimensions of the resource, use the Format element.</dcterms:description>
  <dcterms:hasVersion rdf:resource="http://dublincore.org/usage/terms/history/#type-006"/>
  <dcterms:issued rdf:datatype="&xsd;date">1999-07-02</dcterms:issued>
  <dcterms:modified rdf:datatype="&xsd;date">2008-01-14</dcterms:modified>
  <rdfs:comment xml:lang="en">The nature or genre of the resource.</rdfs:comment>
  <rdfs:isDefinedBy rdf:resource="&dc;"/>
  <rdfs:label xml:lang="en">Type</rdfs:label>
  <scos:note xml:lang="en">A second property with the same name as this property has been declared in the dcterms: namespace (http://purl.org/dc/terms/).  See the Introduction to the document "DCMI Metadata Terms" (http://dublincore.org/documents/dcmi-terms/) for an explanation.</scos:note>
</rdf:Property>

<rdf:Property rdf:about="&nexif;whiteBalance"
    rdfs:label="whiteBalance">
  <rdfs:subPropertyOf rdf:resource="http://www.kanzaki.com/ns/exif#whiteBalance"/>
  <rdfs:subPropertyOf rdf:resource="&nexif;pictTaking"/>
  <rdfs:comment>tagNumber: 41987
The white balance mode set when the image was shot.</rdfs:comment>
  <rdfs:domain rdf:resource="&nexif;Photo"/>
  <rdfs:range rdf:resource="&xsd;string"/>
</rdf:Property>

<rdf:Property rdf:about="&nie;modified"
    rdfs:label="modified">
  <rdfs:comment>Date the DataObject was changed in any way.  Note that this date refers to the modification of the DataObject itself (i.e. the physical representation). Compare with nie:contentModified.</rdfs:comment>
  <rdfs:domain rdf:resource="&nie;DataObject"/>
  <rdfs:range rdf:resource="&xsd;dateTime"/>
</rdf:Property>

<rdf:Property rdf:about="&nexif;sharpness"
    rdfs:label="sharpness">
  <rdfs:subPropertyOf rdf:resource="http://www.kanzaki.com/ns/exif#sharpness"/>
  <rdfs:subPropertyOf rdf:resource="&nexif;pictTaking"/>
  <rdfs:comment>tagNumber: 41994
The direction of sharpness processing applied by the camera when the image was shot.</rdfs:comment>
  <rdfs:domain rdf:resource="&nexif;Photo"/>
  <rdfs:range rdf:resource="&xsd;string"/>
</rdf:Property>

<rdfs:Class rdf:about="&pimo;LogicalMediaType"
    protege:role="abstract"
    rdfs:label="Logical Media Type">
  <pimo:classRole rdf:resource="&pimo;AbstractClass"/>
  <rdfs:comment>Logical media types represent the content aspect of information elements e.g. a flyer, a contract, a promotional video, a todo list.  The user can create new logical media types dependend on their domain: a salesman will need MarketingFlyer, Offer, Invoice while a student might create Report, Thesis and Homework. This is independent from the information element and data object (NIE/NFO) in which the media type will be stored. The same contract can be stored in a PDF file, a text file, or an HTML website.
The groundingOccurrence of a LogicalMediaType is the Document that stores the content.</rdfs:comment>
  <rdfs:subClassOf rdf:resource="&pimo;Thing"/>
</rdfs:Class>

</rdf:RDF>
